<?xml version="1.0" encoding="UTF-8"?>
<rdf:RDF xml:base="https://rdf.ag/o/beer#"
  xmlns="https://rdf.ag/o/beer#"
  xmlns:cs="http://purl.org/vocab/changeset/schema#"
  xmlns:gs1="https://gs1.org/voc/"
  xmlns:schema="https://schema.org/"
  xmlns:as="http://www.w3.org/ns/activitystreams#"
  xmlns:cc="http://creativecommons.org/ns#"
  xmlns:cereals="https://rdf.ag/o/cerealsToo#"
  xmlns:dbpedia="http://dbpedia.org/resource/"
  xmlns:bibo="http://purl.org/ontology/bibo/"
  xmlns:dcterms="http://purl.org/dc/terms/"
  xmlns:doap="http://usefulinc.com/ns/doap#"
  xmlns:eurovoc="http://eurovoc.europa.eu/"
  xmlns:sosa="http://www.w3.org/ns/sosa/"
  xmlns:foaf="http://xmlns.com/foaf/0.1/"
  xmlns:beer="https://rdf.ag/o/beer#"
  xmlns:geonames="http://sws.geonames.org/"
  xmlns:loc="http://id.loc.gov/vocabulary/relators/"
  xmlns:nif="http://persistence.uni-leipzig.org/nlp2rdf/ontologies/nif-core#"
  xmlns:oa="http://www.w3.org/ns/oa#"
  xmlns:owl="http://www.w3.org/2002/07/owl#"
  xmlns:prov="http://www.w3.org/ns/prov#"
  xmlns:rdf="http://www.w3.org/1999/02/22-rdf-syntax-ns#"
  xmlns:rdfs="http://www.w3.org/2000/01/rdf-schema#"
  xmlns:skos="http://www.w3.org/2004/02/skos/core#"
  xmlns:skosxl="http://www.w3.org/2008/05/skos-xl#"
  xmlns:time="http://www.w3.org/2006/time#"
  xmlns:vann="http://purl.org/vocab/vann/"
  xmlns:void="http://rdfs.org/ns/void#"
  xmlns:vs="http://www.w3.org/2003/06/sw-vocab-status/ns#"
  xmlns:unit="http://www.qudt.org/2.1/vocab/unit"
  xmlns:qudt="http://www.qudt.org/2.1/schema/qudt"
  xmlns:xsd="http://www.w3.org/2001/XMLSchema#">
  

  <owl:Ontology rdf:about="">
    <rdf:type rdf:resource="http://purl.org/vocommons/voaf#Vocabulary"/>
    <vann:preferredNamespacePrefix>beer</vann:preferredNamespacePrefix>
    <vann:preferredNamespaceUri>https://rdf.ag/o/beer#</vann:preferredNamespaceUri>
    <dcterms:title xml:lang="en">The Beer Ontology</dcterms:title>
    <dcterms:title xml:lang="fr">L'Ontologie de la Bière</dcterms:title>
    <rdfs:label xml:lang="en">The Beer Ontology</rdfs:label>
    <rdfs:label xml:lang="fr">L'Ontologie de la Bière</rdfs:label>
    <foaf:name xml:lang="en">The Beer Ontology</foaf:name>
    <foaf:name xml:lang="fr">L'Ontologie de la Bière</foaf:name>
    <dcterms:description xml:lang="en">The Beer Ontology is an ontology created to represent data about beer.</dcterms:description>
    <dcterms:description xml:lang="fr">L'ontologie de la Bière est une ontologie créée pour représenter des données sur la bière.</dcterms:description>
    <skos:definition xml:lang="en">The Beer Ontology is an ontology created to represent data about beer.</skos:definition>
    <skos:definition xml:lang="fr">L'Ontologie de la Bière est une ontologie créée pour représenter des données sur la bière.</skos:definition>
    <rdfs:comment xml:lang="en">The Beer Ontology is an ontology created to represent data about beer.</rdfs:comment>
    <rdfs:comment xml:lang="fr">L'Ontologie de la Bière est une ontologie créée pour représenter des données sur la bière.</rdfs:comment>
    <owl:versionInfo>ONTOLOGY_VERSION</owl:versionInfo>
    <owl:priorVersion rdf:resource="https://rdf.ag/o/beer-2021-03-24"/>
    <dcterms:date rdf:datatype="http://www.w3.org/2001/XMLSchema#date">ONTOLOGY_DATE</dcterms:date>
    <dcterms:rights>Dual license. All rights reserved.</dcterms:rights>
    <dcterms:rights rdf:resource="https://creativecommons.org/licenses/by/3.0/"/>
    <dcterms:subject rdf:resource="http://id.loc.gov/authorities/subjects/sh85012832"/>
    <vs:term_status xml:lang="en">Stable</vs:term_status>
    <vs:term_status xml:lang="fr">Stable</vs:term_status>
    <void:inDataset rdf:resource="#datasetdefinition"/>
    <dcterms:creator rdf:resource="#psw"/>
    <owl:imports rdf:resource="http://www.w3.org/ns/sosa/"/>
    <owl:imports rdf:resource="http://www.w3.org/ns/ssn/"/>
    <owl:imports rdf:resource="http://www.w3.org/ns/prov#"/>
    <owl:imports rdf:resource="http://www.w3.org/2006/time#"/>
    <owl:imports rdf:resource="http://purl.org/ontology/bibo/"/>
    <owl:imports rdf:resource="https://rdf.ag/o/BeverageGraph"/>
    <owl:imports rdf:resource="http://rdfs.org/ns/void"/>
    <owl:imports rdf:resource="http://www.w3.org/2004/02/skos/core"/>
  </owl:Ontology>

  <void:Dataset rdf:about="#datasetdefinition">
    <rdf:type rdf:resource="https://schema.org/Dataset"/>
    <rdf:type rdf:resource="http://www.w3.org/ns/dcat#Dataset"/>
    <dcterms:title xml:lang="en">The Beer Ontology</dcterms:title>
    <dcterms:title xml:lang="fr">L'Ontologie de la Bière</dcterms:title>
    <rdfs:label xml:lang="en">The Beer Ontology</rdfs:label>
    <rdfs:label xml:lang="fr">L'Ontologie de la Bière</rdfs:label>
    <foaf:name xml:lang="en">The Beer Ontology</foaf:name>
    <foaf:name xml:lang="fr">L'Ontologie de la Bière</foaf:name>
    <schema:name xml:lang="en">The Beer Ontology</schema:name>
    <schema:name xml:lang="fr">L'Ontologie de la Bière</schema:name>
    <dcterms:description xml:lang="en">The Beer Ontology is an ontology created to represent data about beer.</dcterms:description>
    <dcterms:description xml:lang="fr">L'Ontologie de la Bière est une ontologie créée pour représenter des données sur la bière.</dcterms:description>
    <skos:definition xml:lang="en">The Beer Ontology is an ontology created to represent data about beer.</skos:definition>
    <skos:definition xml:lang="fr">L'Ontologie de la Bière est une ontologie créée pour représenter des données sur la bière.</skos:definition>
    <rdfs:comment xml:lang="en">The Beer Ontology is an ontology created to represent data about beer.</rdfs:comment>
    <rdfs:comment xml:lang="fr">L'Ontologie de la Bière est une ontologie créée pour représenter des données sur la bière.</rdfs:comment>
    <schema:description xml:lang="en">The Beer Ontology is an ontology created to represent data about beer.</schema:description>
    <schema:description xml:lang="fr">L'Ontologie de la Bière est une ontologie créée pour représenter des données sur la bière.</schema:description>
    <schema:url>https://rdf.ag/o/beer-ONTOLOGY_DATE</schema:url>
    <schema:identifier>https://rdf.ag/o/beer</schema:identifier>
    <schema:license>https://creativecommons.org/licenses/by/3.0/</schema:license>
    <schema:license>Dual license. All rights reserved.</schema:license>
    <schema:creator rdf:resource="#psw"/>
    <schema:keywords>Beer</schema:keywords>    
    <schema:keywords>Brewing</schema:keywords>    
    <schema:keywords>Cider</schema:keywords> 
    <schema:version>ONTOLOGY_VERSION</schema:version>
    <void:feature rdf:resource="http://www.w3.org/ns/formats/N3"/>
    <void:feature rdf:resource="http://www.w3.org/ns/formats/N-Triples"/>
    <void:feature rdf:resource="http://www.w3.org/ns/formats/RDF_XML"/>
    <void:feature rdf:resource="http://www.w3.org/ns/formats/Turtle"/>
    <schema:distribution>
     <schema:DataDownload rdf:about="#beerXML">
      <schema:encodingFormat>XML</schema:encodingFormat>
      <schema:contentUrl>https://rdf.ag/o/beer-ONTOLOGY_DATE.owl</schema:contentUrl>
     </schema:DataDownload>
    </schema:distribution>
    
    <schema:distribution>   
     <schema:DataDownload rdf:about="#beerXMLTTL">
      <schema:encodingFormat>application/x-turtle</schema:encodingFormat>
      <schema:contentUrl>https://rdf.ag/o/beer-ONTOLOGY_DATE.ttl</schema:contentUrl>
     </schema:DataDownload>
    </schema:distribution>
    
    <schema:distribution>   
     <schema:DataDownload rdf:about="#beerXMLRDF">
      <schema:encodingFormat>application/rdf+xml</schema:encodingFormat>
      <schema:contentUrl>https://rdf.ag/o/beer-ONTOLOGY_DATE.owl</schema:contentUrl>
     </schema:DataDownload>
    </schema:distribution>   
    
    <schema:distribution>
     <schema:DataDownload rdf:about="#beerJsonld">
      <schema:encodingFormat>application/ld+json</schema:encodingFormat>
      <schema:contentUrl>https://rdf.ag/o/beer-ONTOLOGY_DATE.jsonld</schema:contentUrl>
     </schema:DataDownload>
    </schema:distribution>   
    <!-- Need to resolve better rdf for licenses. -->
    <cc:license rdf:resource="https://creativecommons.org/licenses/by/3.0/"/>
    <cc:license>Dual license. All rights reserved.</cc:license>
    <cc:Jurisdiction rdf:resource="http://dbpedia.org/resource/Canada"/>
    <cc:attributionURL rdf:resource="http://rdf.ag/"/>
    <rdfs:isDefinedBy rdf:resource="https://rdf.ag/o/beer-ONTOLOGY_DATE"/>
    <void:triples>TOTAL_TRIPLES_ONTOLOGY</void:triples>
    <void:entities>TOTAL_ENTITIES_ONTOLOGY</void:entities>
    <dcterms:subject rdf:resource="http://id.loc.gov/authorities/subjects/sh85012832"/>
    <dcterms:creator rdf:resource="#psw"/>
  </void:Dataset>
  
  <foaf:Organization rdf:about="#osw">
   <rdf:type rdf:resource="https://schema.org/Organization"/>
   <rdf:type rdf:resource="https://gs1.org/voc/Organization"/>
   <gs1:organizationName>PSW Applied Research Inc.</gs1:organizationName>
   <foaf:name>PSW Applied Research Inc.</foaf:name>
   <schema:name>PSW Applied Research Inc.</schema:name>
   <rdfs:label>PSW Applied Research Inc.</rdfs:label>
   <schema:contactPoint>
    <schema:ContactPoint rdf:about="#pswContactPoint">
     <schema:contactType>customer service</schema:contactType>
     <schema:email>info@pswappliedresearch.com</schema:email>
     <rdfs:isDefinedBy rdf:resource="https://rdf.ag/o/beer-ONTOLOGY_DATE"/>
     <void:inDataset rdf:resource="#datasetdefinition"/>
    </schema:ContactPoint>
   </schema:contactPoint>
   <rdfs:isDefinedBy rdf:resource="https://rdf.ag/o/beer-ONTOLOGY_DATE"/>
   <void:inDataset rdf:resource="#datasetdefinition"/>
  </foaf:Organization>
  
  <foaf:Person rdf:about="#singer">
   <rdf:type rdf:resource="https://schema.org/Person"/>
   <foaf:name>Jessica Singer</foaf:name>
   <rdfs:isDefinedBy rdf:resource="https://rdf.ag/o/beer-ONTOLOGY_DATE"/>
   <void:inDataset rdf:resource="#datasetdefinition"/>
  </foaf:Person>
  
  <foaf:Person rdf:about="#warren">
   <rdf:type rdf:resource="https://schema.org/Person"/>
   <foaf:name>Rob Warren</foaf:name>
   <rdfs:isDefinedBy rdf:resource="https://rdf.ag/o/beer-ONTOLOGY_DATE"/>
   <void:inDataset rdf:resource="#datasetdefinition"/>
  </foaf:Person>

 <bibo:Collection rdf:about="#bibliography">
  <rdfs:label xml:lang="en">The Beer Ontology</rdfs:label>
  <rdfs:label xml:lang="fr">L'Ontologie de la Bière</rdfs:label>
  <rdfs:isDefinedBy rdf:resource="https://rdf.ag/o/beer-ONTOLOGY_DATE"/>
  <void:inDataset rdf:resource="#datasetdefinition"/>
 </bibo:Collection>
 
 <!-- Beer Properties -->
 <owl:DatatypeProperty rdf:about="#specificgravityBeer">
    <rdfs:label xml:lang="en">Specific Gravity of Beer</rdfs:label>
    <rdfs:label xml:lang="en">Relative Gravity of Beer</rdfs:label>
    <rdfs:label xml:lang="fr">Gravité Spécifique de la Bière</rdfs:label>
    <skos:definition xml:lang="en">The ratio of the density of a beer to the density of the standard gravity of water.</skos:definition>
    <skos:definition xml:lang="fr">Le rapport de la densité d'une bière à la densité de la gravité standard de l'eau.</skos:definition>
    <rdfs:isDefinedBy rdf:resource="https://rdf.ag/o/beer-ONTOLOGY_DATE"/>
    <void:inDataset rdf:resource="#datasetdefinition"/>
 </owl:DatatypeProperty>
    
 <owl:DatatypeProperty rdf:about="#pHReading">
    <rdfs:label xml:lang="en">pH Reading</rdfs:label>
    <rdfs:label xml:lang="fr">pH</rdfs:label>
    <skos:definition xml:lang="en">The amount of free H+ ions in a substance. A pH reading determines how acidic or basic is a substance.</skos:definition>
    <skos:definition xml:lang="fr">La quantité d'ions H+ libres dans une substance. Une lecture du pH détermine à quel point une substance est acide ou basique.</skos:definition>
    <rdfs:isDefinedBy rdf:resource="https://rdf.ag/o/beer-ONTOLOGY_DATE"/>
    <void:inDataset rdf:resource="#datasetdefinition"/>
 </owl:DatatypeProperty>
 
 <owl:DatatypeProperty rdf:about="#temperatureReading">
     <rdfs:label xml:lang="en">Temperature Reading</rdfs:label>
     <rdfs:label xml:lang="fr">Température</rdfs:label>
     <skos:definition xml:lang="en">Temperature is a measure of how much energy is associated a set of molecules.</skos:definition>
     <skos:definition xml:lang="fr">La température est une mesure de la quantité d'énergie associée à un ensemble de molécules.</skos:definition>
     <!-- Liquid temp? Process or temperature of the thing inside? -->
     <rdfs:isDefinedBy rdf:resource="https://rdf.ag/o/beer-ONTOLOGY_DATE"/>
     <void:inDataset rdf:resource="#datasetdefinition"/>
 </owl:DatatypeProperty>
 
 <owl:DatatypeProperty rdf:about="#ebc">
     <foaf:name>European Brewery Convention</foaf:name>
     <rdfs:label xml:lang="en">EBC</rdfs:label>
     <skos:definition xml:lang="en">A system of measurement for determining the color of a beer or malt. The equation is: EBC=25×D×A(430) where D = dilution factor and A(430) = the light absorbance at 430 nanometers in a 1-cm cuvette.</skos:definition>
     <skos:definition xml:lang="fr">Un système de mesure pour déterminer la couleur d'une bière ou d'un malt. L'équation est: EBC = 25 × D × A (430) où D = facteur de dilution et A (430) = l'absorbance lumineuse à 430 nanomètres dans une cuvette de 1 cm.</skos:definition>
     <rdfs:comment xml:lang="en">EBC is typically used in Europe, while in North and South America the Standard Reference Method (SRM) is used. One system can be converted into another using these equations: SRM=EBC×0.508EBC=SRM×1.97</rdfs:comment>
     <rdfs:comment xml:lang="fr">EBC est généralement utilisé en Europe, tandis qu'en Amérique du Nord et du Sud, la méthode de référence standard (SRM) est utilisée. Un système peut être converti en un autre en utilisant ces équations: SRM = EBC × 0.508EBC = SRM × 1.97.</rdfs:comment>
     <prov:hadPrimarySource rdf:resource="#Brynildson2020"/>
     <rdfs:isDefinedBy rdf:resource="https://rdf.ag/o/beer-ONTOLOGY_DATE"/>
     <void:inDataset rdf:resource="#datasetdefinition"/>
 </owl:DatatypeProperty>
 
 <sosa:ObservableProperty rdf:about="#ebcValue">
     <foaf:name>European Brewery Convention</foaf:name>
     <rdfs:label xml:lang="en">EBC</rdfs:label>
     <skos:definition xml:lang="en">A system of measurement for determining the color of a beer or malt. The equation is: EBC=25×D×A(430) where D = dilution factor and A(430) = the light absorbance at 430 nanometers in a 1-cm cuvette.</skos:definition>
     <skos:definition xml:lang="fr">Un système de mesure pour déterminer la couleur d'une bière ou d'un malt. L'équation est: EBC = 25 × D × A (430) où D = facteur de dilution et A (430) = l'absorbance lumineuse à 430 nanomètres dans une cuvette de 1 cm.</skos:definition>
     <rdfs:comment xml:lang="en">EBC is typically used in Europe, while in North and South America the Standard Reference Method (SRM) is used. One system can be converted into another using these equations: SRM=EBC×0.508EBC=SRM×1.97</rdfs:comment>
     <rdfs:comment xml:lang="fr">EBC est généralement utilisé en Europe, tandis qu'en Amérique du Nord et du Sud, la méthode de référence standard (SRM) est utilisée. Un système peut être converti en un autre en utilisant ces équations: SRM = EBC × 0.508EBC = SRM × 1.97.</rdfs:comment>
     <prov:hadPrimarySource rdf:resource="#Brynildson2020"/>
     <rdfs:isDefinedBy rdf:resource="https://rdf.ag/o/beer-ONTOLOGY_DATE"/>
     <void:inDataset rdf:resource="#datasetdefinition"/>
 </sosa:ObservableProperty>
 
 <owl:DatatypeProperty rdf:about="#netContent">
     <rdfs:label xml:lang="en">Net Content</rdfs:label>
     <rdfs:label xml:lang="fr">Contenu Net</rdfs:label>
     <skos:definition xml:lang="en">The total weight of something not including the packaging.</skos:definition>
     <skos:definition xml:lang="fr">Le poids total de quelque chose sans l'emballage.</skos:definition>
     <rdfs:isDefinedBy rdf:resource="https://rdf.ag/o/beer-ONTOLOGY_DATE"/>
     <void:inDataset rdf:resource="#datasetdefinition"/>
 </owl:DatatypeProperty>
 
 <owl:DatatypeProperty rdf:about="#netVolume">
     <rdfs:label xml:lang="en">Net Volume</rdfs:label>
     <rdfs:label xml:lang="fr">Volume Net</rdfs:label>
     <skos:definition xml:lang="en">The total volume of something not including the packaging.</skos:definition>
     <skos:definition xml:lang="fr">Le volume total de quelque chose sans l'emballage.</skos:definition>
     <rdfs:isDefinedBy rdf:resource="https://rdf.ag/o/beer-ONTOLOGY_DATE"/>
     <void:inDataset rdf:resource="#datasetdefinition"/>
 </owl:DatatypeProperty>
 
 <sosa:ObservableProperty rdf:about="#abv">
     <rdfs:label xml:lang="en">Alcohol By Volume</rdfs:label>
     <rdfs:label xml:lang="en">Alcohol Per Volume</rdfs:label>
     <rdfs:label xml:lang="fr">Alcool Par Volume</rdfs:label>
     <skos:definition xml:lang="en">The amount of pure ethanol in 100mL of a solution.</skos:definition>
     <skos:definition xml:lang="fr">La quantité d'éthanol pur dans 100mL d'une solution.</skos:definition>
     <rdfs:isDefinedBy rdf:resource="https://rdf.ag/o/beer-ONTOLOGY_DATE"/>
     <void:inDataset rdf:resource="#datasetdefinition"/>
 </sosa:ObservableProperty>

 <owl:DatatypeProperty rdf:about="#abvValue">
     <rdfs:label xml:lang="en">Alcohol By Volume</rdfs:label>
     <rdfs:label xml:lang="fr">Alcohol By Volume</rdfs:label>
     <skos:definition xml:lang="en">The amount of pure ethanol in 100mL of a solution.</skos:definition>
     <skos:definition xml:lang="fr">La quantité d'éthanol pur dans 100mL d'une solution.</skos:definition>
     <rdfs:comment xml:lang="en">Alcohol by volume is a standard observable property in alcoholic beverages. It is the measurement of pure ethanol in 100 ml of a solution at a temperature of 20˚C (68˚F).
         
         The (unmaintained) bevon ontology previously maintained a property (http://rdfs.co/bevon/latest/html#term-abv) for this.</rdfs:comment>
     <rdfs:isDefinedBy rdf:resource="https://rdf.ag/o/beer-ONTOLOGY_DATE"/>
     <void:inDataset rdf:resource="#datasetdefinition"/>
     <owl:sameAs rdf:resource="https://gs1.org/voc/percentageOfAlcoholByVolume"/>
     <!-- uses this unit: Go to external page http://purl.obolibrary.org/obo/UO_0000165  -->
 </owl:DatatypeProperty>
 
 <owl:DatatypeProperty rdf:about="#ibu">
     <rdfs:label xml:lang="en">International Bittering Unit</rdfs:label>
     <rdfs:label xml:lang="en">IBU</rdfs:label>
     <skos:definition xml:lang="en">A measure of the amount of bittering chemicals found in a sample of beer. These chemicals are known for being associated with a bitter taste, therefore the IBU measurement is not a subjective measurement since the amount of chemicals present are measured empirically.</skos:definition>
     <skos:definition xml:lang="fr">Une mesure de la quantité de produits chimiques amers trouvés dans un échantillon de bière. Ces produits chimiques sont connus pour être associés à un goût amer, par conséquent, la mesure IBU n'est pas une mesure subjective puisque la quantité de produits chimiques présents est mesurée de manière empirique.</skos:definition>
     <rdfs:isDefinedBy rdf:resource="https://rdf.ag/o/beer-ONTOLOGY_DATE"/>
     <void:inDataset rdf:resource="#datasetdefinition"/>
 </owl:DatatypeProperty>
 
 <owl:objectProperty rdf:about="#brewedBy">
     <rdfs:label xml:lang="en">Brewed By</rdfs:label>
     <rdfs:label xml:lang="fr">Brassé Par</rdfs:label>
     <skos:definition xml:lang="en">The brewery that is marketing or physically brewing the beer.</skos:definition>
     <skos:definition xml:lang="fr">La brasserie qui commercialise ou qui physiquement brasse la bière. </skos:definition>
     <rdfs:comment xml:lang="en">This is likely the least defined property within this ontology. While ontologically flexible to a number of different vocabulary, it is meant as a catch-all for situations where a common sense relationship is known to exist while not being immediatly obvious.</rdfs:comment>
     <rdfs:comment xml:lang="en">Cette propriété est probablement la moins définie dans cette ontologie. Bien que flexible ontologiquement avec une equivalence à plusieurs cas et vocabulaires, elle est conçu comme un fourre-tout pour les situations où une relation "bon sens" exister sans être immédiatement évidente.</rdfs:comment>
     <rdfs:isDefinedBy rdf:resource="https://rdf.ag/o/beer-ONTOLOGY_DATE"/>
     <void:inDataset rdf:resource="#datasetdefinition"/>
     <owl:oneOf rdf:parseType="Collection">
      <owl:Thing rdf:about="https://schema.org/manufacturer"/>
      <owl:Thing rdf:about="https://gs1.org/voc/brand"/>
      <owl:Thing rdf:about="https://gs1.org/voc/manufacturer"/>
      <owl:Thing rdf:about="http://xmlns.com/foaf/0.1/maker"/>
      <owl:Thing rdf:about="http://purl.org/dc/terms/creator"/>
      <owl:Thing rdf:about="https://schema.org/creator"/>
     </owl:oneOf>
 </owl:objectProperty>
 
 <owl:DatatypeProperty rdf:about="#batchnumber">
     <rdfs:label xml:lang="en">Batch Number</rdfs:label>
     <rdfs:label xml:lang="fr">Numéro de Batch</rdfs:label>
     <skos:definition xml:lang="en">The number assigned to a specific batch.</skos:definition>
     <skos:definition xml:lang="fr">Le numéro attribué à une brassée spécifique.</skos:definition>
     <rdfs:isDefinedBy rdf:resource="https://rdf.ag/o/beer-ONTOLOGY_DATE"/>
     <void:inDataset rdf:resource="#datasetdefinition"/>
 </owl:DatatypeProperty>
 
 <owl:DatatypeProperty rdf:about="#lotnumber">
     <rdfs:label xml:lang="en">Lot Number</rdfs:label>
     <rdfs:label xml:lang="fr">Numéro de Lot</rdfs:label>
     <skos:definition xml:lang="en">The number assigned to a specific lot.</skos:definition>
     <skos:definition xml:lang="fr">Le numéro attribué à un lot spécifique.</skos:definition>
     <rdfs:isDefinedBy rdf:resource="https://rdf.ag/o/beer-ONTOLOGY_DATE"/>
     <void:inDataset rdf:resource="#datasetdefinition"/>
 </owl:DatatypeProperty>
 
 <owl:DatatypeProperty rdf:about="#lotsize">
     <rdfs:label xml:lang="en">Lot Size</rdfs:label>
     <rdfs:label xml:lang="fr">Montant du Lot</rdfs:label>
     <skos:definition xml:lang="en">The amount of product associated with a specific lot.</skos:definition>
     <skos:definition xml:lang="fr">La quantité de produit associée à un lot spécifique.</skos:definition>
     <rdfs:isDefinedBy rdf:resource="https://rdf.ag/o/beer-ONTOLOGY_DATE"/>
     <void:inDataset rdf:resource="#datasetdefinition"/>
 </owl:DatatypeProperty>
  
 <!-- Beer Activities -->
 <rdf:Description rdf:about="#BeerBrewingActivity">
    <rdfs:subClassOf rdf:resource="http://www.w3.org/2006/time#TemporalEntity"/>
    <rdfs:subClassOf rdf:resource="http://www.w3.org/ns/prov#Activity"/>
    <rdfs:subClassOf rdf:resource="http://www.w3.org/2006/time#ProperInterval"/>
    <rdfs:label xml:lang="en">Beer Brewing</rdfs:label>
    <rdfs:label xml:lang="fr">Brassage de la Bière</rdfs:label>
    <skos:definition xml:lang="en">The process of brewing beer, usualling including other processes such as Milling, Mashing, Sparging, Boiling, Wort Cooling, Fermenting, Racking, Conditioning and a Packaging process of some kind.</skos:definition>
    <skos:definition xml:lang="fr">Processus de brassage de la bière, comprenant généralement d'autres processus tels que le broyage, le brassage, le barbotage, l'ébullition, le refroidissement du moût, la fermentation, le soutirage, le conditionnement et un processus d'emballage quelconque.</skos:definition>
    <rdfs:isDefinedBy rdf:resource="https://rdf.ag/o/beer-ONTOLOGY_DATE"/>
    <void:inDataset rdf:resource="#datasetdefinition"/>
 </rdf:Description>
 
 <rdf:Description rdf:about="#BeerMillingActivity">
    <rdfs:subClassOf rdf:resource="#BeerBrewingActivity"/>
    <rdfs:label xml:lang="en">Milling</rdfs:label>
    <rdfs:label xml:lang="fr">Fraisage</rdfs:label>
    <skos:definition xml:lang="en">The process by which malts are converted to grist. To increase the surface area of the malts, they are milled and then hot water is applied so that the starch can be extracted.
        
        The grist cannot be too coarse or else the some of the starches will not be released. Nor can the grist be too fine or a paste will form and water will not be able to drain properly.</skos:definition>
    <skos:definition xml:lang="fr">Le processus par lequel les malts sont convertis en grist. Pour augmenter la surface des malts, ils sont broyés puis de l'eau chaude est appliquée afin que l'amidon puisse être extrait.
        
        Le grain ne peut pas être trop grossier, sinon certains des amidons ne seront pas libérés. Le grain ne peut pas non plus être trop fin ou une pâte se formera et l'eau ne pourra pas s'égoutter correctement.</skos:definition>
    <prov:hadPrimarySource rdf:resource="#MasterBrewersAssociationoftheAmericas1999"/>
    <rdfs:isDefinedBy rdf:resource="https://rdf.ag/o/beer-ONTOLOGY_DATE"/>
    <void:inDataset rdf:resource="#datasetdefinition"/>
 </rdf:Description>
 
 <rdf:Description rdf:about="#BeerMashingActivity">
    <rdfs:subClassOf rdf:resource="#BeerBrewingActivity"/>
    <rdfs:label xml:lang="en">Mashing</rdfs:label>
    <rdfs:label xml:lang="fr">Écrasement</rdfs:label>
    <skos:definition xml:lang="en">Similar to producing tea from tea leaves, wort is produced by allowing the the grist to steep. It is at this stage the the enzymes, mainly alpha and beta amylase, in the malt are activated.
        
        It is at this stage that the enzymes convert starch into sugar, which can be then be consumed by yeast during the fermentation process.</skos:definition>
    <skos:definition xml:lang="fr">Semblable à la production de thé à partir de feuilles de thé, le moût est produit en laissant le grist infuser. C'est à ce stade que les enzymes, principalement alpha et bêta amylase, du malt sont activées.
    
        C'est à ce stade que les enzymes transforment l'amidon en sucre, qui peut ensuite être consommé par la levure pendant le processus de fermentation.</skos:definition>
    <prov:hadPrimarySource rdf:resource="#MasterBrewersAssociationoftheAmericas1999"/>
    <rdfs:isDefinedBy rdf:resource="https://rdf.ag/o/beer-ONTOLOGY_DATE"/>
    <void:inDataset rdf:resource="#datasetdefinition"/>
 </rdf:Description>
 
 <rdf:Description rdf:about="#BeerSpargingActivity">
    <rdfs:subClassOf rdf:resource="#BeerBrewingActivity"/>
    <rdfs:label xml:lang="en">Sparging</rdfs:label>
    <rdfs:label xml:lang="fr">Barbotage</rdfs:label>
    <skos:definition xml:lang="en">Sparging is the process of sprinkling hot water over mash in order to rinse excess sugars off of the grains.</skos:definition>
    <skos:definition xml:lang="fr">Le barbotage est le processus consistant à saupoudrer de l'eau chaude sur la purée afin de rincer les sucres en excès des grains.</skos:definition>
    <prov:hadPrimarySource rdf:resource="#Brynildson2020"/>
    <rdfs:isDefinedBy rdf:resource="https://rdf.ag/o/beer-ONTOLOGY_DATE"/>
    <void:inDataset rdf:resource="#datasetdefinition"/>
 </rdf:Description>
 
 <rdf:Description rdf:about="#BeerBoilingActivity">
    <rdfs:subClassOf rdf:resource="#BeerBrewingActivity"/>
    <rdfs:label xml:lang="en">Boiling</rdfs:label>
    <rdfs:label xml:lang="fr">Bouillir</rdfs:label>
    <skos:definition xml:lang="en">After the wort has been extracted from the malt, it is necessary to boil the wort before fermation. Boiling does a number of things to the malt such as: sterilization, enzyme denaturing, color development, increasing the concentration, secondary products are distilled and oxidized and finally hop aromas are extracted and isomerized.
        
        Boiling ends at flameout, or when heat is turned off.</skos:definition>
    <skos:definition xml:lang="fr">Une fois le moût extrait du malt, il est nécessaire de faire bouillir le moût avant la fermentation. L'ébullition fait un certain nombre de choses au malt telles que: la stérilisation, la dénaturation enzymatique, le développement de la couleur, l'augmentation de la concentration, les produits secondaires sont distillés et oxydés et enfin les arômes de houblon sont extraits et isomérisés.
        
        L'ébullition se termine à l'extinction ou lorsque le chauffage est éteint.</skos:definition>
    <prov:hadPrimarySource rdf:resource="#MasterBrewersAssociationoftheAmericas1999"/>
    <rdfs:isDefinedBy rdf:resource="https://rdf.ag/o/beer-ONTOLOGY_DATE"/>
    <void:inDataset rdf:resource="#datasetdefinition"/>
 </rdf:Description>
 
 <rdf:Description rdf:about="#BeerWortCoolingActivity">
    <rdfs:subClassOf rdf:resource="#BeerBrewingActivity"/>
    <rdfs:label xml:lang="en">Wort Cooling</rdfs:label>
    <rdfs:label xml:lang="fr">Refroidissement du Moût</rdfs:label>
    <skos:definition xml:lang="en">Wort cooling, or hopstand, happens after the boiling process and heat is not longer being added. At this point the brewer may add additional hops in order boost the hops flavors that would have been destroyed during the boiling process. Wort can also be cooled to allow for any sediments to accumulate at the bottom of the tank or container, clearing up the beer.
        
        Wort has three typical methods for cooling: by air, bt water and by a refrigerant.</skos:definition>
    <skos:definition xml:lang="fr">Le refroidissement du moût, ou trémie, se produit après le processus d'ébullition et la chaleur n'est plus ajoutée. À ce stade, le brasseur peut ajouter du houblon supplémentaire afin d'augmenter les saveurs de houblon qui auraient été détruites pendant le processus d'ébullition. Le moût peut également être refroidi pour permettre à tous les sédiments de s'accumuler au fond du réservoir ou du récipient, éclaircissant ainsi la bière.
        
        Le moût a trois méthodes typiques de refroidissement: par air, par eau et par un réfrigérant.</skos:definition>
    <prov:hadPrimarySource rdf:resource="#MasterBrewersAssociationoftheAmericas1999"/>
    <rdfs:isDefinedBy rdf:resource="https://rdf.ag/o/beer-ONTOLOGY_DATE"/>
    <void:inDataset rdf:resource="#datasetdefinition"/>
 </rdf:Description>
        
 <rdf:Description rdf:about="#BeerFermentingActivity">
    <rdfs:subClassOf rdf:resource="#BeerBrewingActivity"/>
    <rdfs:label xml:lang="en">Fermentation</rdfs:label>
    <rdfs:label xml:lang="fr">Fermentation</rdfs:label>
    <skos:definition xml:lang="en">After boiling, the beer undergoes fermentation. A process by which yeasts anaerobically convert the sugars from the malts into ethanol.</skos:definition>
    <skos:definition xml:lang="fr">Après ébullition, la bière subit une fermentation. Un processus par lequel les levures convertissent de manière anaérobie les sucres des malts en éthanol.</skos:definition>
    <prov:hadPrimarySource rdf:resource="#MasterBrewersAssociationoftheAmericas1999"/>
    <rdfs:isDefinedBy rdf:resource="https://rdf.ag/o/beer-ONTOLOGY_DATE"/>
    <void:inDataset rdf:resource="#datasetdefinition"/>
</rdf:Description>

 <rdf:Description rdf:about="#BeerRackingActivity">
    <rdfs:subClassOf rdf:resource="#BeerBrewingActivity"/>
    <rdfs:label xml:lang="en">Racking</rdfs:label>
    <rdfs:label xml:lang="fr">Soutirage</rdfs:label>
    <skos:definition xml:lang="en">Beer racking is the careful transferral of the beer from one vessel to another, this must be done carefully in order to minimize the disturbance of the beer.</skos:definition>
    <skos:definition xml:lang="fr">Le soutirage de la bière est le transfert soigneux de la bière d'un récipient à un autre, cela doit être fait avec soin afin de minimiser la perturbation de la bière.</skos:definition>
    <prov:hadPrimarySource rdf:resource="#MasterBrewersAssociationoftheAmericas1999"/>
    <rdfs:isDefinedBy rdf:resource="https://rdf.ag/o/beer-ONTOLOGY_DATE"/>
    <void:inDataset rdf:resource="#datasetdefinition"/>
</rdf:Description>
 
 <rdf:Description rdf:about="#BeerConditioningActivity">
    <rdfs:subClassOf rdf:resource="#BeerBrewingActivity"/>
    <rdfs:label xml:lang="en">Conditioning</rdfs:label>
    <rdfs:label xml:lang="fr">Conditionnement</rdfs:label>
    <skos:definition xml:lang="en">Beer is conditioned to the finaly beer product by being allowed to age in vessel, usually a wooden cask, for a certain amount of time for any unwanted byproducts to be absorbed and for the aroma to mature.</skos:definition>
    <skos:definition xml:lang="fr">La bière est conditionnée au produit final de la bière en étant laissée vieillir dans un récipient, généralement un tonneau en bois, pendant un certain temps pour que tous les sous-produits indésirables soient absorbés et que l'arôme mûrisse.</skos:definition>
    <prov:hadPrimarySource rdf:resource="#MasterBrewersAssociationoftheAmericas1999"/>
    <rdfs:isDefinedBy rdf:resource="https://rdf.ag/o/beer-ONTOLOGY_DATE"/>
    <void:inDataset rdf:resource="#datasetdefinition"/>
</rdf:Description>
 
 <rdf:Description rdf:about="#PackagingActivity">
    <rdfs:subClassOf rdf:resource="#BeerBrewingActivity"/>
    <rdfs:label xml:lang="en">Packaging</rdfs:label>
    <rdfs:label xml:lang="fr">Emballage</rdfs:label>
    <skos:definition xml:lang="en">The process by which the finished beer is transferred into a container with specific labelling so that it can now be sold as a product.</skos:definition>
    <skos:definition xml:lang="fr">Le processus par lequel la bière finie est transférée dans un conteneur avec un étiquetage spécifique afin qu'elle puisse maintenant être vendue en tant que produit.</skos:definition>
    <prov:hadPrimarySource rdf:resource="#MasterBrewersAssociationoftheAmericas1999"/>
    <rdfs:isDefinedBy rdf:resource="https://rdf.ag/o/beer-ONTOLOGY_DATE"/>
    <void:inDataset rdf:resource="#datasetdefinition"/>
</rdf:Description>
 
 <rdf:Description rdf:about="#BottlingActivity">
    <rdfs:subClassOf rdf:resource="PackagingActivity"/>
    <rdfs:label xml:lang="en">Bottling</rdfs:label>
    <rdfs:label xml:lang="en">Embouteillage</rdfs:label>
    <skos:definition xml:lang="en">The process by which the finished beer is transferred into a bottle with specific labelling so that it can be sold as a bottled product.</skos:definition>
    <skos:definition xml:lang="fr">Le processus par lequel la bière finie est transférée dans une bouteille avec un étiquetage spécifique afin qu'elle puisse être vendue en tant que produit en bouteille.</skos:definition>
    <rdfs:isDefinedBy rdf:resource="https://rdf.ag/o/beer-ONTOLOGY_DATE"/>
    <void:inDataset rdf:resource="#datasetdefinition"/>
</rdf:Description>
    
 <rdf:Description rdf:about="#ShippingActivity">
    <rdfs:subClassOf rdf:resource="http://www.w3.org/2006/time#TemporalEntity"/>
    <rdfs:subClassOf rdf:resource="http://www.w3.org/ns/prov#Activity"/>
    <rdfs:label xml:lang="en">Shipping</rdfs:label>
    <rdfs:label xml:lang="fr">Expédition</rdfs:label>
    <skos:definition xml:lang="en">Once the beer has been packaged, it can then be shipped to another location to be sold.</skos:definition>
    <skos:definition xml:lang="fr">Une fois la bière emballée, elle peut être expédiée vers un autre endroit pour être vendue.</skos:definition>
    <prov:hadPrimarySource rdf:resource="#MasterBrewersAssociationoftheAmericas1999"/>
    <rdfs:isDefinedBy rdf:resource="https://rdf.ag/o/beer-ONTOLOGY_DATE"/>
    <void:inDataset rdf:resource="#datasetdefinition"/>
 </rdf:Description>
 
 <!-- Beer Vessels and Equipment -->
 <owl:Class rdf:ID="Vessel">
     <rdfs:label xml:lang="en">Vessel</rdfs:label>
     <rdfs:label xml:lang="fr">Cuve</rdfs:label>
     <skos:definition xml:lang="en">A vessel is used to carry out certain processes or for storage, with many specialized types based on the type of processing.</skos:definition>
     <skos:definition xml:lang="fr">Un cuve est utilisé pour effectuer certains processus ou pour le stockage, avec de nombreux types spécialisés en fonction du type de traitement.</skos:definition>
     <prov:hadPrimarySource rdf:resource="#NAPTA2019"/>
     <rdfs:isDefinedBy rdf:resource="http://rdf.ag/o/tnt-ONTOLOGY_DATE"/>
     <void:inDataset rdf:resource="#datasetdefinition"/>
 </owl:Class>
 
 <owl:Class rdf:ID="BrewhouseVessel">
     <rdfs:subClassOf rdf:resource="#Vessel"/>
     <rdfs:label xml:lang="en">Brewhouse Vessel</rdfs:label>
     <rdfs:label xml:lang="fr">Cuve de brasserie</rdfs:label>
     <skos:definition xml:lang="en">A brewhouse vessel is used for brewing processes or for storage in the brewing facility.</skos:definition>
     <skos:definition xml:lang="fr">Une cuve de brasserie est utilisée pour les processus de brassage ou pour le stockage dans l'installation de brassage.</skos:definition>
     <rdfs:isDefinedBy rdf:resource="http://rdf.ag/o/tnt-ONTOLOGY_DATE"/>
     <void:inDataset rdf:resource="#datasetdefinition"/>
 </owl:Class>
 
 <owl:Class rdf:ID="CerealCooker">
     <rdfs:subClassOf rdf:resource="#BrewhouseVessel"/>
     <rdfs:label xml:lang="en">Cereal Cooker</rdfs:label>
     <rdfs:label xml:lang="en">Adjunct Cooker</rdfs:label>
     <rdfs:label xml:lang="fr">Cuiseur à Céréales</rdfs:label>
     <skos:definition xml:lang="en">A cereal cooker allows a brewer to create a mash from unmalted cereal to achieve a certain flavor or aroma. The grains are heated with water until the starch begins to dissolve in the water, a process called gelatinization.</skos:definition>
     <skos:definition xml:lang="fr">Un cuiseur à céréales permet à un brasseur de créer une purée à partir de céréales non maltées pour obtenir une certaine saveur ou un certain arôme. Les grains sont chauffés avec de l'eau jusqu'à ce que l'amidon commence à se dissoudre dans l'eau, un processus appelé gélatinisation.</skos:definition>
     <prov:hadPrimarySource rdf:resource="#Oliver2012"/>
     <rdfs:isDefinedBy rdf:resource="http://rdf.ag/o/tnt-ONTOLOGY_DATE"/>
     <void:inDataset rdf:resource="#datasetdefinition"/>
 </owl:Class>
 
 <owl:Class rdf:ID="MashTun">
     <rdfs:subClassOf rdf:resource="#BrewhouseVessel"/>
     <rdfs:label xml:lang="en">Mash Tun</rdfs:label>
     <rdfs:label xml:lang="fr">Cuve-Matière</rdfs:label>
     <skos:definition xml:lang="en">A mash tun is where temperature-controlled water is mixed with milled malts until the starches in the malts are converted to sugar. The sugar dissolved in water, the wort, is then removed to continue to the next part of the brewing process.</skos:definition>
     <skos:definition xml:lang="fr">Une cuve-matière est l'endroit où de l'eau à température contrôlée est mélangée avec des malts moulus jusqu'à ce que les amidons contenus dans les malts soient convertis en sucre. Le sucre dissous dans l'eau, le moût, est ensuite éliminé pour passer à la partie suivante du processus de brassage.</skos:definition>
     <prov:hadPrimarySource rdf:resource="#Oliver2012"/>
     <rdfs:isDefinedBy rdf:resource="http://rdf.ag/o/tnt-ONTOLOGY_DATE"/>
     <void:inDataset rdf:resource="#datasetdefinition"/>
 </owl:Class>
 
 <owl:Class rdf:ID="LauterTun">
     <rdfs:subClassOf rdf:resource="#BrewhouseVessel"/>
     <rdfs:label xml:lang="en">Lauter Tun</rdfs:label>
     <rdfs:label xml:lang="fr">Cuve-Filtre</rdfs:label>
     <skos:definition xml:lang="en">A lauter tun is a brewhouse vessel used for lautering, the process of separating wort from mash solids.</skos:definition>
     <skos:definition xml:lang="fr">Une cuve-filtre est une cuve de brasserie utilisée pour la filtration du moût des solides de purée.</skos:definition>
     <prov:hadPrimarySource rdf:resource="#MasterBrewersAssociationoftheAmericas1999"/>
     <rdfs:isDefinedBy rdf:resource="http://rdf.ag/o/tnt-ONTOLOGY_DATE"/>
     <void:inDataset rdf:resource="#datasetdefinition"/>
 </owl:Class>
 
 <owl:Class rdf:ID="BrewingKettle">
     <rdfs:subClassOf rdf:resource="#BrewhouseVessel"/>
     <rdfs:label xml:lang="en">Brewing Kettle</rdfs:label>
     <rdfs:label xml:lang="fr">Bouilloire de Brassage</rdfs:label>
     <skos:definition xml:lang="en">A brewing kettle is the vessel where the wort and hops are boiled in the brewing process.</skos:definition>
     <skos:definition xml:lang="fr">Une bouilloire de brassage est le récipient dans lequel le moût et le houblon sont bouillis dans le processus de brassage.</skos:definition>
     <prov:hadPrimarySource rdf:resource="#MasterBrewersAssociationoftheAmericas1999"/>
     <rdfs:isDefinedBy rdf:resource="http://rdf.ag/o/tnt-ONTOLOGY_DATE"/>
     <void:inDataset rdf:resource="#datasetdefinition"/>
 </owl:Class>
 
 <owl:Class rdf:ID="Fermenter">
     <rdfs:subClassOf rdf:resource="#BrewhouseVessel"/>
     <rdfs:label xml:lang="en">Fermenter</rdfs:label>
     <rdfs:label xml:lang="fr">Fermenteur</rdfs:label>
     <skos:definition xml:lang="en">A fermenter is a brewing vessel where the fermentation process takes place.</skos:definition>
     <skos:definition xml:lang="fr">Un fermenteur est une cuve de brassage où se déroule le processus de fermentation.</skos:definition>
     <prov:hadPrimarySource rdf:resource="#MasterBrewersAssociationoftheAmericas1999"/>
     <rdfs:isDefinedBy rdf:resource="http://rdf.ag/o/tnt-ONTOLOGY_DATE"/>
     <void:inDataset rdf:resource="#datasetdefinition"/>
 </owl:Class>
 
 <owl:Class rdf:ID="WortChiller">
     <rdfs:subClassOf rdf:resource="#BrewhouseVessel"/>
     <rdfs:label xml:lang="en">Wort Chiller</rdfs:label>
     <rdfs:label xml:lang="fr">Refroidisseur de Moût</rdfs:label>
     <skos:definition xml:lang="en">A wort chiller is used to rapidly cool down the wort from boiling temperature to or below room temperature. These can be a type of vessel or they could simply be a heat exchanger added to a kettle near the end of boiling. Coolers can be open or closed vessels.</skos:definition>
     <skos:definition xml:lang="fr">Un refroidisseur de moût est utilisé pour refroidir rapidement le moût de la température d'ébullition à ou en dessous de la température ambiante. Il peut s'agir d'un type de récipient ou simplement d'un échangeur de chaleur ajouté à une bouilloire vers la fin de l'ébullition. Les glacières peuvent être des récipients ouverts ou fermés.</skos:definition>
     <prov:hadPrimarySource rdf:resource="#MasterBrewersAssociationoftheAmericas1999"/>
     <rdfs:isDefinedBy rdf:resource="http://rdf.ag/o/tnt-ONTOLOGY_DATE"/>
     <void:inDataset rdf:resource="#datasetdefinition"/>
 </owl:Class>
 
 <owl:Class rdf:ID="Tank">
     <rdfs:subClassOf rdf:resource="#Vessel"/>
     <rdfs:label xml:lang="en">Tank</rdfs:label>
     <rdfs:label xml:lang="fr">Réservoir</rdfs:label>
     <skos:definition xml:lang="en">A tank is a type of vessel used for containing liquids and/or gasses.</skos:definition>
     <skos:definition xml:lang="fr">Un réservoir est un type de cuve utilisé pour contenir des liquides et/ou des gaz.</skos:definition>
     <prov:hadPrimarySource rdf:resource="#NAPTA2019"/>
     <rdfs:isDefinedBy rdf:resource="http://rdf.ag/o/tnt-ONTOLOGY_DATE"/>
     <void:inDataset rdf:resource="#datasetdefinition"/>
 </owl:Class>
 
 <owl:Class rdf:ID="Silo">
     <rdfs:subClassOf rdf:resource="#Vessel"/>
     <rdfs:label xml:lang="en">Silo</rdfs:label>
     <rdfs:label xml:lang="fr">Réservoir</rdfs:label>
     <skos:definition xml:lang="en">A silo is a type of vessel used for storing bulk solids.</skos:definition>
     <skos:definition xml:lang="fr">Un silo est un type de récipient utilisé pour stocker des solides en vrac.</skos:definition>
     <prov:hadPrimarySource rdf:resource="#CARSON2015647"/>
     <rdfs:isDefinedBy rdf:resource="http://rdf.ag/o/tnt-ONTOLOGY_DATE"/>
     <void:inDataset rdf:resource="#datasetdefinition"/>
 </owl:Class>
 
 <owl:Class rdf:ID="Mill">
     <rdfs:label xml:lang="en">Mill</rdfs:label>
     <rdfs:label xml:lang="fr">Moulin</rdfs:label>
     <skos:definition xml:lang="en">A mill is a machine used to break solids into finer pieces through the process of cutting, grinding or crushing.</skos:definition>
     <skos:definition xml:lang="fr">Un moulin est une machine utilisée pour briser les solides en fines pièces par le biais du processus de coupe, de broyage ou de concassage.</skos:definition>
     <rdfs:isDefinedBy rdf:resource="http://rdf.ag/o/tnt-ONTOLOGY_DATE"/>
     <void:inDataset rdf:resource="#datasetdefinition"/>
 </owl:Class>
 
 <owl:Class rdf:ID="RodMill">
     <rdfs:subClassOf rdf:resource="#Mill"/>
     <rdfs:label xml:lang="en">Rod Mill</rdfs:label>
     <rdfs:label xml:lang="fr">Moulin à tige</rdfs:label>
     <skos:definition xml:lang="en">A rod mill uses cylinders to grind material into smaller pieces.</skos:definition>
     <skos:definition xml:lang="fr">Un moulin à tige utilise des cylindres pour broyer le matériau en plus petits morceaux.</skos:definition>
     <rdfs:isDefinedBy rdf:resource="http://rdf.ag/o/tnt-ONTOLOGY_DATE"/>
     <void:inDataset rdf:resource="#datasetdefinition"/>
 </owl:Class>
 
 <owl:Class rdf:ID="MaltMill">
     <rdfs:subClassOf rdf:resource="#RodMill"/>
     <rdfs:label xml:lang="en">Malt Mill</rdfs:label>
     <rdfs:label xml:lang="fr">Moulin à Malt</rdfs:label>
     <skos:definition xml:lang="en">A malt mill is a mill specifically for milling malts.</skos:definition>
     <skos:definition xml:lang="fr">Un moulin à malt est un moulin spécifiquement destiné à la mouture des malts.</skos:definition>
     <rdfs:isDefinedBy rdf:resource="http://rdf.ag/o/tnt-ONTOLOGY_DATE"/>
     <void:inDataset rdf:resource="#datasetdefinition"/>
 </owl:Class>
 
 <owl:Class rdf:ID="MaltMill-6-Roll">
     <rdfs:subClassOf rdf:resource="#MaltMill"/>
     <rdfs:label xml:lang="en">6 Row Malt Mill</rdfs:label>
     <rdfs:label xml:lang="fr">Moulin à Malt à 6 Rangs</rdfs:label>
     <skos:definition xml:lang="en">A 6 Row Malt Mill is a type of malt mill that has 6 rollers.</skos:definition>
     <skos:definition xml:lang="fr">Un moulin à malt à 6 rangs est un type de moulin à malt qui a 6 rouleaux.</skos:definition>
     <rdfs:isDefinedBy rdf:resource="http://rdf.ag/o/tnt-ONTOLOGY_DATE"/>
     <void:inDataset rdf:resource="#datasetdefinition"/>
 </owl:Class>
 
 <owl:Class rdf:ID="WetMaltMill">
     <rdfs:subClassOf rdf:resource="#MaltMill"/>
     <rdfs:label xml:lang="en">Wet Malt Mill</rdfs:label>
     <rdfs:label xml:lang="fr">Moulin à Malt Humide</rdfs:label>
     <skos:definition xml:lang="en">A wet malt mill has specialized roller that keep the husks of steeped malts intact.</skos:definition>
     <skos:definition xml:lang="fr">Un moulin à malt humide a un rouleau spécialisé qui garde intactes les cosses des malts trempés.</skos:definition>
     <prov:hadPrimarySource rdf:resource="#Oliver2012"/>
     <rdfs:isDefinedBy rdf:resource="http://rdf.ag/o/tnt-ONTOLOGY_DATE"/>
     <void:inDataset rdf:resource="#datasetdefinition"/>
 </owl:Class>
 
 <owl:Class rdf:ID="Centrifuge">
     <rdfs:subClassOf rdf:resource="#Vessel"/>
     <rdfs:label xml:lang="en">Centrifuge</rdfs:label>
     <rdfs:label xml:lang="fr">Une Centrifugeuse</rdfs:label>
     <skos:definition xml:lang="en">A container that accelerates a liquid by spinning to allow its components to be separated by gravity.</skos:definition>
     <skos:definition xml:lang="fr">Un récipient qui accélère un liquide en tournant pour permettre à ses composants d'être séparés par gravité.</skos:definition>
     <rdfs:isDefinedBy rdf:resource="http://rdf.ag/o/tnt-ONTOLOGY_DATE"/>
     <void:inDataset rdf:resource="#datasetdefinition"/>
 </owl:Class>
     
 <!-- Beer classes -->
 <owl:Class rdf:ID="Batch">
     <rdfs:label xml:lang="en">Batch</rdfs:label>
     <skos:definition xml:lang="en">A batch is an amount of products or goods that is produced at one time.</skos:definition>
     <skos:definition xml:lang="fr">Un batch est une quantité de produits ou de marchandises qui est produite en même temps.</skos:definition>
     <rdfs:comment xml:lang="en">The direct translation of 'batch' to french is 'lot' which is also the translation for lot (in both English and French). To avoid confusion between batches and lots, the English word for batch will be used in french.</rdfs:comment>
     <rdfs:comment xml:lang="fr">La traduction directe de "batch" en français est "lot" qui est également la traduction de lot (en anglais et en français). Pour éviter toute confusion entre les lots et les lots, le mot anglais pour batch sera utilisé en français.</rdfs:comment>
     <rdfs:isDefinedBy rdf:resource="http://rdf.ag/o/tnt-ONTOLOGY_DATE"/>
     <void:inDataset rdf:resource="#datasetdefinition"/>
 </owl:Class>
 
 <owl:Class rdf:ID="Brewery">
     <rdfs:label xml:lang="en">Brewery</rdfs:label>
     <rdfs:label xml:lang="fr">Brasserie</rdfs:label>
     <skos:definition xml:lang="en">A brewery is a location or corporate entity that produces beer.</skos:definition>
     <skos:definition xml:lang="fr">Une brasserie est une entreprise ou un lieu qui produit de la bière.</skos:definition>
     <rdfs:isDefinedBy rdf:resource="https://rdf.ag/o/beer-ONTOLOGY_DATE"/>
     <void:inDataset rdf:resource="#datasetdefinition"/>
     <rdfs:subClassOf rdf:resource="http://www.w3.org/ns/org#Organization"/>
     <rdfs:subClassOf rdf:resource="http://xmlns.com/foaf/0.1/Organization"/>
     <rdfs:subClassOf rdf:resource="http://www.w3.org/ns/prov#Agent"/>
     <rdfs:subClassOf rdf:resource="http://www.w3.org/ns/prov#Location"/>
     <rdfs:subClassOf rdf:resource="http://www.opengis.net/ont/geosparql#Feature"/>
     <rdfs:subClassOf rdf:resource="https://gs1.org/voc/Organization"/>
     <rdfs:subClassOf rdf:resource="https://schema.org/Organization"/>
 </owl:Class>
 
 <owl:Class rdf:ID="Craftbrewery">
     <rdfs:subClassOf rdf:resource="#Brewery"/>
     <rdfs:label xml:lang="en">Craft Brewery</rdfs:label>
     <rdfs:label xml:lang="fr">Brasserie Artisanale</rdfs:label>
     <skos:definition xml:lang="en">As defined by the Brewers Association, a craft brewery is a small, independent brewer.</skos:definition>
     <skos:definition xml:lang="fr">Une brasserie est une entreprise ou un lieu qui produit de la bière.</skos:definition>
     <prov:hadPrimarySource rdf:resource="#BrewersAssociation2020"/>
     <rdfs:isDefinedBy rdf:resource="https://rdf.ag/o/beer-ONTOLOGY_DATE"/>
     <void:inDataset rdf:resource="#datasetdefinition"/>
 </owl:Class>
 
 <owl:Class rdf:ID="Microbrewery">
     <rdfs:subClassOf rdf:resource="#CraftBrewery"/>
     <rdfs:label xml:lang="en">Microbrewery</rdfs:label>
     <rdfs:label xml:lang="fr">Microbrasserie</rdfs:label>
     <skos:definition xml:lang="en">Microbreweries typically sell about 75% or more of its beer off-site and produce about 15,000 barrels per year. Microbreweries will sell beer either to wholesalers, retailers or directly to the consumers (carry-out or taproom).</skos:definition>
     <skos:definition xml:lang="fr">Les microbrasseries vendent généralement environ 75% ou plus de leur bière hors site et produisent environ 15 000 barils par an. Les microbrasseries vendront de la bière soit aux grossistes, aux détaillants, soit directement aux consommateurs (à emporter ou en salle).</skos:definition>
     <prov:hadPrimarySource rdf:resource="#BrewersAssociation2020"/>
     <rdfs:isDefinedBy rdf:resource="https://rdf.ag/o/beer-ONTOLOGY_DATE"/>
     <void:inDataset rdf:resource="#datasetdefinition"/>
 </owl:Class>
 
 <owl:Class rdf:ID="Brewpub">
     <rdfs:subClassOf rdf:resource="#Craftbrewery"/>
     <rdfs:label xml:lang="en">Brewpub</rdfs:label>
     <rdfs:label xml:lang="fr">Brewpub</rdfs:label> <!-- Brasserie artisanale? -->
     <skos:definition xml:lang="en">A brewpub is a type of brewery also provides food services sells about 25% or more of its beer on site. The rest can also be sold to off site distributers or through carry-outs.</skos:definition>
     <skos:definition xml:lang="fr">Un brewpub est un type de brasserie qui fournit également des services de restauration et vend environ 25% ou plus de sa bière sur place. Le reste peut également être vendu à des distributeurs hors site ou par le biais de report.</skos:definition>
     <prov:hadPrimarySource rdf:resource="#BrewersAssociation2020"/>
     <rdfs:isDefinedBy rdf:resource="https://rdf.ag/o/beer-ONTOLOGY_DATE"/>
     <void:inDataset rdf:resource="#datasetdefinition"/>
 </owl:Class>
 
 <!--A brewery can have a taproom, taproom is a utility -->
 <owl:Class rdf:ID="TaproomBrewery">
     <rdfs:subClassOf rdf:resource="#CraftBrewery"/>
     <rdfs:label xml:lang="en">Taproom Brewery</rdfs:label>
     <rdfs:label xml:lang="fr">Brasserie Taproom</rdfs:label> <!-- ? No translation -->
     <skos:definition xml:lang="en">A taproom brewery is a brewery that sells at least 25% of their beer on-site but does not offer food services. The rest of the beer can be sold as carry-outs or to off-site retailers.</skos:definition>
     <skos:definition xml:lang="fr">Une brasserie taproom est une brasserie qui vend au moins 25% de sa bière sur place mais n'offre pas de services de restauration. Le reste de la bière peut être vendu sous forme de report ou à des détaillants hors site.</skos:definition>
     <prov:hadPrimarySource rdf:resource="#BrewersAssociation2020"/>
     <rdfs:isDefinedBy rdf:resource="https://rdf.ag/o/beer-ONTOLOGY_DATE"/>
     <void:inDataset rdf:resource="#datasetdefinition"/>
 </owl:Class>
 
 <owl:Class rdf:ID="RegionalBrewery">
     <rdfs:subClassOf rdf:resource="#CraftBrewery"/>
     <rdfs:label xml:lang="en">Regional Brewery</rdfs:label>
     <rdfs:label xml:lang="fr">Brasserie régionale</rdfs:label>
     <skos:definition xml:lang="en">A regional brewery is a brewery that produces around 15,000 to 6 million barrels of beer per year.</skos:definition>
     <skos:definition xml:lang="fr">Une brasserie régionale est une brasserie qui produit environ 15 000 à 6 millions de barils de bière par an.</skos:definition>
     <prov:hadPrimarySource rdf:resource="#BrewersAssociation2020"/>
     <rdfs:isDefinedBy rdf:resource="https://rdf.ag/o/beer-ONTOLOGY_DATE"/>
     <void:inDataset rdf:resource="#datasetdefinition"/>
 </owl:Class>
 
 <owl:Class rdf:ID="ContractBrewery">
     <rdfs:subClassOf rdf:resource="#CraftBrewery"/>
     <rdfs:label xml:lang="en">Contract Brewery</rdfs:label>
     <rdfs:label xml:lang="fr">Brasserie sous Contrat</rdfs:label>
     <skos:definition xml:lang="en">A brewery that has a contract with a company that handles the marketing and sales part of the business while the producer-brewery only focuses on brewing beer.</skos:definition>
     <skos:definition xml:lang="fr">Une brasserie qui a un contrat avec une entreprise qui gère la partie marketing et ventes de l'entreprise, tandis que la brasserie-producteur se concentre uniquement sur le brassage de la bière.</skos:definition>
     <prov:hadPrimarySource rdf:resource="#BrewersAssociation2020"/>
     <rdfs:isDefinedBy rdf:resource="https://rdf.ag/o/beer-ONTOLOGY_DATE"/>
     <void:inDataset rdf:resource="#datasetdefinition"/>
 </owl:Class>

 <owl:Class rdf:ID="OffLicense">
   <rdfs:subClassOf rdf:resource="https://schema.org/LiquorStore"/>
     <rdfs:label xml:lang="en">Off License</rdfs:label>
     <rdfs:label xml:lang="fr">Magasin</rdfs:label>
     <skos:definition xml:lang="en">An off license is a shop licensed to sell liquor to take home, attached or associated with a brewery.</skos:definition>
     <skos:definition xml:lang="fr">Un hors-permis est un magasin autorisé à vendre de l'alcool, attaché ou associé à une brasserie. </skos:definition>
     <rdfs:isDefinedBy rdf:resource="https://rdf.ag/o/beer-ONTOLOGY_DATE"/>
     <void:inDataset rdf:resource="#datasetdefinition"/>
     <rdfs:subClassOf rdf:resource="http://www.w3.org/ns/org#Organization"/>
     <rdfs:subClassOf rdf:resource="http://xmlns.com/foaf/0.1/Organization"/>
     <rdfs:subClassOf rdf:resource="http://www.w3.org/ns/prov#Agent"/>
     <rdfs:subClassOf rdf:resource="http://www.w3.org/ns/prov#Location"/>
     <rdfs:subClassOf rdf:resource="http://www.opengis.net/ont/geosparql#Feature"/>
     <rdfs:subClassOf rdf:resource="https://gs1.org/voc/Organization"/>
     <rdfs:subClassOf rdf:resource="https://schema.org/Organization"/>
 </owl:Class>
 
 <owl:Class rdf:ID="Beverage">
     <rdfs:subClassOf rdf:resource="https://schema.org/ProductGroup"/>
     <rdfs:label xml:lang="en">Beverage</rdfs:label>
     <rdfs:label xml:lang="en">Drink</rdfs:label>
     <rdfs:label xml:lang="fr">Boisson</rdfs:label>
     <skos:definition xml:lang="en">A liquid that is consumed by humans.</skos:definition>
     <skos:definition xml:lang="fr">Un liquide qui est consommé par les humains.</skos:definition>
     <rdfs:isDefinedBy rdf:resource="https://rdf.ag/o/beer-ONTOLOGY_DATE"/>
     <void:inDataset rdf:resource="#datasetdefinition"/>
 </owl:Class>

 <owl:Class rdf:ID="AlcoholicDrink">
     <rdfs:subClassOf rdf:resource="#Beverage"/>
     <rdfs:label xml:lang="en">Alcoholic Drink</rdfs:label>
     <rdfs:label xml:lang="fr">Boisson Alcoolisée</rdfs:label>
     <skos:definition xml:lang="en">A drink that contains ethanol, a type of alcohol produced by fermentation of sugar.</skos:definition>
     <skos:definition xml:lang="fr">Une boisson contenant de l'éthanol produite par la fermentation de sucres.</skos:definition>
     <rdfs:isDefinedBy rdf:resource="https://rdf.ag/o/beer-ONTOLOGY_DATE"/>
     <void:inDataset rdf:resource="#datasetdefinition"/>
 </owl:Class>
 
 <owl:Class rdf:ID="AlcoholFreeDrink">
     <rdfs:subClassOf rdf:resource="#Beverage"/>
     <rdfs:subClassOf rdf:resource="https://schema.org/ProductGroup"/>
     <rdfs:subClassOf rdf:resource="#NonAlcoholicDrink"/>
     <rdfs:label xml:lang="en">Alcohol-Free Drink</rdfs:label>
     <rdfs:label xml:lang="fr">Boisson Sans Alcool</rdfs:label> <!-- Restriction on abv -->
     <skos:definition xml:lang="en">A drink that has no detectable amount of alcohol, as specified by the FDA.</skos:definition>
     <skos:definition xml:lang="fr">Une boisson qui n'a pas de quantité détectable d'alcool, comme spécifié par la FDA.</skos:definition>
     <owl:equivalentClass>
      <owl:Restriction rdf:about="#NoDetectableAlcohol">
       <owl:onProperty rdf:resource="#abvValue"/>
       <owl:someValuesFrom>
        <owl:Datatype rdf:about="#ZeroABVValue">
         <owl:onDatatype rdf:resource="http://www.w3.org/2001/XMLSchema#float"/>
         <owl:withRestrictions>
          <rdf:Description rdf:about="#ZeroABVValueMax">
           <xsd:maxInclusive rdf:datatype="http://www.w3.org/2001/XMLSchema#float">0.0</xsd:maxInclusive>
          </rdf:Description>
         </owl:withRestrictions>
        </owl:Datatype>
       </owl:someValuesFrom>
      </owl:Restriction>
     </owl:equivalentClass>    
     <prov:hadPrimarySource rdf:resource="#USDA2005"/>
     <rdfs:isDefinedBy rdf:resource="https://rdf.ag/o/beer-ONTOLOGY_DATE"/>
     <void:inDataset rdf:resource="#datasetdefinition"/>
 </owl:Class>
 
 <owl:Class rdf:ID="NonAlcoholicDrink">
     <rdfs:subClassOf rdf:resource="#Beverage"/>
     <rdfs:subClassOf rdf:resource="https://schema.org/ProductGroup"/>
     <rdfs:label xml:lang="en">Non-Alcoholic Drink</rdfs:label>
     <rdfs:label xml:lang="fr">Boisson Non-Alcoolisé</rdfs:label> <!-- Restriction on abv -->
     <skos:definition xml:lang="en">A drink that has some detectable amount of alcohol but less than 0.5 percent of alcohol by volume, as specified by the FDA. Some flavored beverages and fruit juices could contain trace amounts of alcohol from flavoring extracts, which is why they have the term "non-alcoholic".</skos:definition>
     <skos:definition xml:lang="fr">Une boisson qui a une certaine quantité d'alcool détectable mais moins de 0,5 pour cent d'alcool en volume, comme spécifié par la FDA. Certaines boissons aromatisées et jus de fruits peuvent contenir des traces d'alcool provenant d'extraits aromatisants, c'est pourquoi ils portent le terme "non-alcoolisé".</skos:definition>
     <owl:equivalentClass>
      <owl:Restriction rdf:about="#MaxDetectableAlcohol">
       <owl:onProperty rdf:resource="#abvValue"/>
       <owl:someValuesFrom>
        <owl:Datatype rdf:about="#ZeroABVValueRange">
         <owl:onDatatype rdf:resource="http://www.w3.org/2001/XMLSchema#float"/>
         <owl:withRestrictions>
          <rdf:Description rdf:about="#ZeroABVValueMax">
           <xsd:maxInclusive rdf:datatype="http://www.w3.org/2001/XMLSchema#float">0.5</xsd:maxInclusive>
          </rdf:Description>
         </owl:withRestrictions>
        </owl:Datatype>
       </owl:someValuesFrom>
      </owl:Restriction>
     </owl:equivalentClass>    
     <prov:hadPrimarySource rdf:resource="#USDA2005"/>
     <rdfs:isDefinedBy rdf:resource="https://rdf.ag/o/beer-ONTOLOGY_DATE"/>
     <void:inDataset rdf:resource="#datasetdefinition"/>
 </owl:Class>
 
 <owl:Class rdf:ID="DealcolizedDrink">
     <rdfs:subClassOf rdf:resource="#Beverage"/>
     <rdfs:label xml:lang="en">Dealcolized Drink</rdfs:label>
     <rdfs:label xml:lang="fr">Boisson Désalcoolisé</rdfs:label> <!-- abv restriction -->
     <skos:definition xml:lang="en">A drink that is derived from an alcohol process, but the alcohol has been removed.</skos:definition>
     <skos:definition xml:lang="fr">Une boisson qui est dérivée d'un processus d'alcool, mais l'alcool a été supprimé.</skos:definition>
     <rdfs:comment xml:lang="en">Please note that this term is meant as a descriptor of a process used to create the drink.</rdfs:comment>
     <rdfs:comment xml:lang="fr">Veuillez noter que ce terme est un descripteur du processus utilisé pour créer la boisson.</rdfs:comment> 
     <owl:equivalentClass>
      <owl:Restriction rdf:about="#ProcessAlcoholRemoved">
       <owl:onProperty rdf:resource="#abvValue"/>
       <owl:someValuesFrom>
        <owl:Datatype rdf:about="#ProcessZeroABVValueRange">
         <owl:onDatatype rdf:resource="http://www.w3.org/2001/XMLSchema#float"/>
         <owl:withRestrictions>
          <rdf:Description rdf:about="#ProcesssZeroABVValueMax">
           <xsd:maxInclusive rdf:datatype="http://www.w3.org/2001/XMLSchema#float">0.0</xsd:maxInclusive>
          </rdf:Description>
         </owl:withRestrictions>
        </owl:Datatype>
       </owl:someValuesFrom>
      </owl:Restriction>
     </owl:equivalentClass>
     <prov:hadPrimarySource rdf:resource="#USDA2005"/>
     <rdfs:isDefinedBy rdf:resource="https://rdf.ag/o/beer-ONTOLOGY_DATE"/>
     <void:inDataset rdf:resource="#datasetdefinition"/>
 </owl:Class>
 
 <owl:Class rdf:ID="MaltBeverage">
     <rdfs:subClassOf rdf:resource="#Beverage"/>
     <rdfs:subClassOf rdf:resource="https://schema.org/ProductGroup"/>
     <rdfs:label xml:lang="en">Malt Beverage</rdfs:label>
     <rdfs:label xml:lang="fr">Boisson au Malt</rdfs:label>
     <skos:definition xml:lang="en">According to the FDA, a malt beverage is made through the process of alcoholic fermentation of specific materials.</skos:definition>
     <skos:definition xml:lang="fr">Selon la FDA, une boisson maltée est fabriquée par le processus de fermentation alcoolique de matériaux spécifiques.</skos:definition>
     <prov:hadPrimarySource rdf:resource="#USDA2005"/>
     <rdfs:isDefinedBy rdf:resource="https://rdf.ag/o/beer-ONTOLOGY_DATE"/>
     <void:inDataset rdf:resource="#datasetdefinition"/>
 </owl:Class>
 
 <owl:Class rdf:ID="Beer">
     <owl:disjointWith rdf:resource="#Cider"/>
     <owl:disjointWith rdf:resource="#Mead"/>
     <rdfs:subClassOf rdf:resource="#MaltBeverage"/>
     <owl:equivalentClass rdf:resource="http://purl.obolibrary.org/obo/FOODON_00001260"/>
     <rdfs:subClassOf rdf:resource="https://schema.org/ProductGroup"/>
     <rdfs:label xml:lang="en">Beer</rdfs:label>
     <rdfs:label xml:lang="fr">Bière</rdfs:label>
     <skos:definition xml:lang="en">Beer a drink that is created as a result of the fermentation of yeast malt and is flavored with hops. The fermentation process results in alcohol, however there are some beers that are specifically brewed to be non-alcoholic.</skos:definition>
     <skos:definition xml:lang="fr">La bière est une boisson créée à la suite de la fermentation du malt de levure et aromatisée au houblon. Le processus de fermentation donne de l'alcool, mais certaines bières sont spécifiquement brassées pour être non alcoolisées.</skos:definition>
     <rdfs:isDefinedBy rdf:resource="https://rdf.ag/o/beer-ONTOLOGY_DATE"/>
     <void:inDataset rdf:resource="#datasetdefinition"/>
 </owl:Class>
 
 <owl:Class rdf:ID="NonAlcoholicBeer">
     <rdfs:subClassOf rdf:resource="#Beer"/>
     <rdfs:subClassOf rdf:resource="#NonAlcoholicDrink"/>
     <rdfs:subClassOf rdf:resource="https://schema.org/ProductGroup"/>
     <rdfs:label xml:lang="en">Non Alcoholic Beer</rdfs:label>
     <rdfs:label xml:lang="en">Cereal Beverage</rdfs:label>
     <rdfs:label xml:lang="fr">Bière sans alcool</rdfs:label>
     <skos:definition xml:lang="en">A malt beverage that has less than 0.5 percent alcohol by volume. According to the FDA and the Alcohol Tax and Trade Bureau, non-alcoholic beers are not treated as beers under the International Revenue Code (IRC) because they have less than 0.5% alcohol by volume. A non-alcoholic beer must use the term "dealcoholized" or "alcohol-removed" before 'beer' on its statement of identity and must be in equal font. "Non-alcoholic" can be used as an additional label but it cannot be used instead of "dealcoholized" or "alcohol-removed".</skos:definition>
     <skos:definition xml:lang="fr">Une boisson maltée qui a moins de 0,5 pour cent d'alcool par volume. Selon la FDA et l'Alcool Tax and Trade Bureau, les bières non alcoolisées ne sont pas traitées comme des bières en vertu du Code international des revenus (IRC) car elles contiennent moins de 0,5% d'alcool en volume. Une bière sans alcool doit utiliser le terme "désalcoolisé" ou "sans alcool" avant "bière" sur sa déclaration d'identité et doit être dans la même police. "Sans alcool" peut être utilisé comme étiquette supplémentaire, mais il ne peut pas être utilisé à la place de "désalcoolisé" ou "sans alcool".</skos:definition>
     <prov:hadPrimarySource rdf:resource="#USDA2005"/>
     <prov:hadPrimarySource rdf:resource="#Mather2020"/>
     <rdfs:isDefinedBy rdf:resource="https://rdf.ag/o/beer-ONTOLOGY_DATE"/>
     <void:inDataset rdf:resource="#datasetdefinition"/>
 </owl:Class>
 
<owl:Class rdf:ID="Distillery"> 
     <owl:equivalentClass rdf:resource="https://schema.org/Distillery"/>
     <rdfs:label xml:lang="en">Distillery</rdfs:label>
     <rdfs:label xml:lang="fr">Distillerie</rdfs:label>
     <skos:definition xml:lang="en">A premise where distillation, for the purposes of making consumable alcohol, takes place.</skos:definition>
     <skos:definition xml:lang="fr">Un local où la distillation, aux fins de la fabrication d'alcool consommable, a lieu.</skos:definition>
     <rdfs:isDefinedBy rdf:resource="https://rdf.ag/o/beer-ONTOLOGY_DATE"/>
     <void:inDataset rdf:resource="#datasetdefinition"/>
     <rdfs:subClassOf rdf:resource="http://www.w3.org/ns/org#Organization"/>
     <rdfs:subClassOf rdf:resource="http://xmlns.com/foaf/0.1/Organization"/>
     <rdfs:subClassOf rdf:resource="http://www.w3.org/ns/prov#Agent"/>
     <rdfs:subClassOf rdf:resource="http://www.w3.org/ns/prov#Location"/>
     <rdfs:subClassOf rdf:resource="http://www.opengis.net/ont/geosparql#Feature"/>
     <rdfs:subClassOf rdf:resource="https://gs1.org/voc/Organization"/>
     <rdfs:subClassOf rdf:resource="https://schema.org/Organization"/>
 </owl:Class>
 
 <owl:Class rdf:ID="BeverageProduct">
     <rdfs:subClassOf rdf:resource="http://purl.obolibrary.org/obo/FOODON_00001002"/>
     <rdfs:subClassOf rdf:resource="https://gs1.org/voc/Product"/>
     <rdfs:subClassOf rdf:resource="https://schema.org/Product"/>
     <rdfs:label xml:lang="en">Beverage</rdfs:label>
     <rdfs:label xml:lang="fr">Boisson</rdfs:label>
     <skos:definition xml:lang="en">A commercially available beverage in a packaging.</skos:definition>
     <skos:definition xml:lang="fr">Une boisson commercialiser dans un emballage.</skos:definition>
     <rdfs:subClassOf>
      <owl:Restriction rdf:about="#BeverageProductPackaging">
       <owl:onProperty rdf:resource="https://gs1.org/voc/packaging"/>
       <owl:cardinality rdf:datatype="http://www.w3.org/2001/XMLSchema#nonNegativeInteger">1</owl:cardinality>
      </owl:Restriction>
     </rdfs:subClassOf>               
     <rdfs:isDefinedBy rdf:resource="https://rdf.ag/o/beer-ONTOLOGY_DATE"/>
     <void:inDataset rdf:resource="#datasetdefinition"/>
 </owl:Class>
 
<!-- Beer Types -->
 <owl:Class rdf:ID="AmericanBeer">
     <rdfs:subClassOf rdf:resource="#NorthAmericanBeer"/>
     <foaf:name>American Beer</foaf:name>
     <foaf:name>New World Beer</foaf:name>
     <rdfs:label xml:lang="en">American Beer</rdfs:label>
     <rdfs:label xml:lang="fr">Bière Américaine</rdfs:label>
     <skos:definition xml:lang="en">This style of beer is brewed to appeal to wide range of American consumers. It includes ales and lagers, both that appeal to the American mass-market.</skos:definition>
     <skos:definition xml:lang="fr">Ce style de bière est brassé pour plaire à un large éventail de consommateurs américains. Il comprend des ales et des lagers, toutes deux qui plaisent au marché de masse américain.</skos:definition>
     <prov:hadPrimarySource rdf:resource="#BJCP2015"/>
     <rdfs:isDefinedBy rdf:resource="http://rdf.ag/o/beer-ONTOLOGY_DATE"/>
     <void:inDataset rdf:resource="#datasetdefinition"/>
 </owl:Class>
     
 <owl:Class rdf:ID="InternationalLager">
     <rdfs:subClassOf rdf:resource="#Lager"/>
     <foaf:name>International Lager</foaf:name>
     <rdfs:label xml:lang="en">International Lager</rdfs:label>
     <rdfs:label xml:lang="fr">Lager Internationale</rdfs:label>
     <skos:definition xml:lang="en">While the name implies that these lagers are sold internationally, this is not the case. This style of lager, irrespective of where it was brewed or where it is sold, matches a similar profile of lagers that popular across the masses internationally. These styles of lagers are also heavily marketed.</skos:definition>
     <skos:definition xml:lang="fr">Alors que le nom implique que ces lagers sont vendues à l'international, ce n'est pas le cas. Ce style de bière blonde, quel que soit l'endroit où elle a été brassée ou où elle est vendue, correspond à un profil similaire de bière blonde populaire à travers le monde. Ces styles de lagers sont également fortement commercialisés.</skos:definition>
     <prov:hadPrimarySource rdf:resource="#BJCP2015"/>
     <rdfs:isDefinedBy rdf:resource="http://rdf.ag/o/beer-ONTOLOGY_DATE"/>
     <void:inDataset rdf:resource="#datasetdefinition"/>
 </owl:Class>
 
 <owl:Class rdf:ID="CzechLager">
     <rdfs:subClassOf rdf:resource="#Lager"/>
     <rdfs:subClassOf rdf:resource="#EuropeanBeer"/>
     <foaf:name>Czech Lager</foaf:name>
     <rdfs:label xml:lang="en">Czech Lager</rdfs:label>
     <rdfs:label xml:lang="fr">Lager Tchèque</rdfs:label>
     <skos:definition xml:lang="en">Czech lagers are less attenuated than German lagers which results in a higher finishing gravity. They are also usually fermented at cooler temperatures (7-10˚C) and for longer and use decoction, mostly double decoction, mashes.</skos:definition>
     <skos:definition xml:lang="fr">Les lagers tchèques sont moins atténuées que les lagers allemandes, ce qui se traduit par une densité de finition plus élevée. Ils sont également généralement fermentés à des températures plus fraîches (7-10°C) et plus longtemps et utilisent des purées en décoction, principalement en double décoction.</skos:definition>
     <prov:hadPrimarySource rdf:resource="#BJCP2015"/>
     <rdfs:isDefinedBy rdf:resource="http://rdf.ag/o/beer-ONTOLOGY_DATE"/>
     <void:inDataset rdf:resource="#datasetdefinition"/>
 </owl:Class>
 
 <owl:Class rdf:ID="PaleMaltyEuropeanLager">
     <rdfs:subClassOf rdf:resource="#Lager"/>
     <rdfs:subClassOf rdf:resource="#EuropeanBeer"/>
     <foaf:name>Pale Malty European Lager</foaf:name>
     <rdfs:label xml:lang="en">Pale Malty European Lager</rdfs:label>
     <rdfs:label xml:lang="fr">Lager Européenne Pâle et Maltée</rdfs:label>
     <skos:definition xml:lang="en">This style includes mostly German lagers that use Pilsner malts and while they are malty, they are still well attenuated.</skos:definition>
     <skos:definition xml:lang="fr">Ce style comprend principalement des lagers allemandes qui utilisent des malts Pilsner et bien qu'elles soient maltées, elles sont toujours bien atténuées.</skos:definition>
     <prov:hadPrimarySource rdf:resource="#BJCP2015"/>
     <rdfs:isDefinedBy rdf:resource="http://rdf.ag/o/beer-ONTOLOGY_DATE"/>
     <void:inDataset rdf:resource="#datasetdefinition"/>
 </owl:Class>
 
 <owl:Class rdf:ID="MunichHelles">
     <rdfs:subClassOf rdf:resource="#PaleMaltyEuropeanLager"/>
     <rdfs:subClassOf rdf:resource="#GermanBeer"/>
     <foaf:name>Munich Helles</foaf:name>
     <rdfs:label xml:lang="en">Munich Helles</rdfs:label>
     <rdfs:label xml:lang="en">Helles</rdfs:label>
     <skos:definition xml:lang="en">Munich Helles is a type of light lager brewed in Germany that was created in order to compete with Czech Pilsners. This style of beer typically uses Hallertau hops and has more of an amphasis on malts than the Czech Pilsners.</skos:definition>
     <skos:definition xml:lang="fr">La Munich Helles est un type de bière lager légère brassée en Allemagne qui a été créée pour concurrencer la pilsner tchèque. Ce style de bière utilise généralement du houblon Hallertau et met davantage l'accent sur les malts que la pilsner tchèque.</skos:definition>
     <rdfs:isDefinedBy rdf:resource="http://rdf.ag/o/beer-ONTOLOGY_DATE"/>
     <void:inDataset rdf:resource="#datasetdefinition"/>
 </owl:Class>
 
 <owl:Class rdf:ID="PaleBitterEuropeanBeer">
     <rdfs:subClassOf rdf:resource="#Beer"/>
     <rdfs:subClassOf rdf:resource="#EuropeanBeer"/>
     <foaf:name>Pale Bitter European Beer</foaf:name>
     <rdfs:label xml:lang="en">Pale Bitter European Beer</rdfs:label>
     <rdfs:label xml:lang="fr">Bière Européenne Amère Pâle</rdfs:label>
     <skos:definition xml:lang="en">These beers are pale and bitter with a mild to moderately strong hoppy aroma. These beers are well attenuated and are usually lagered, or bottom-fermented.</skos:definition>
     <skos:definition xml:lang="fr">Ces bières sont pâles et amères avec un arôme de houblon doux à modérément fort. Ces bières sont bien atténuées et sont généralement lagerées ou de fermentation basse.</skos:definition>
     <prov:hadPrimarySource rdf:resource="#BJCP2015"/>
     <rdfs:isDefinedBy rdf:resource="http://rdf.ag/o/beer-ONTOLOGY_DATE"/>
     <void:inDataset rdf:resource="#datasetdefinition"/>
 </owl:Class>
 
 <owl:Class rdf:ID="AmberMaltyEuropeanLager">
     <rdfs:subClassOf rdf:resource="#Beer"/>
     <foaf:name>Amber Malty European Lager</foaf:name>
     <rdfs:label xml:lang="en">Amber Malty European Lager</rdfs:label>
     <rdfs:label xml:lang="fr">Lager Européenne Maltée Ambrée</rdfs:label>
     <skos:definition xml:lang="en">These types of beers are lagers, or bottom-fermenting beers, that are German in origin and are distinguished by their amber color and for being malty, strong and fullbodied (vollbier to starkbier).</skos:definition>
     <skos:definition xml:lang="fr">Ces types de bières sont des lagers, ou bières de fermentation basse, d'origine allemande qui se distinguent par leur couleur ambrée et par leur caractère malté, puissant et corsé (vollbier à starkbier).</skos:definition>
     <prov:hadPrimarySource rdf:resource="#BJCP2015"/>
     <rdfs:isDefinedBy rdf:resource="http://rdf.ag/o/beer-ONTOLOGY_DATE"/>
     <void:inDataset rdf:resource="#datasetdefinition"/>
 </owl:Class>
 
 <owl:Class rdf:ID="AmberBitterEuropeanBeer">
     <rdfs:subClassOf rdf:resource="#Beer"/>
     <rdfs:subClassOf rdf:resource="#EuropeanBeer"/>
     <foaf:name>Amber Bitter European Beer</foaf:name>
     <rdfs:label xml:lang="en">Amber Bitter European Beer</rdfs:label>
     <rdfs:label xml:lang="fr">Bière Européenne Ambrée Amère</rdfs:label>
     <skos:definition xml:lang="en">These beers are German or Austrian in origin, are amber colored, and range from even to bitter balanced.</skos:definition>
     <skos:definition xml:lang="fr">Ces bières sont d'origine allemande ou autrichienne, sont de couleur ambrée et vont de même à amères équilibrées.</skos:definition>
     <prov:hadPrimarySource rdf:resource="#BJCP2015"/>
     <rdfs:isDefinedBy rdf:resource="http://rdf.ag/o/beer-ONTOLOGY_DATE"/>
     <void:inDataset rdf:resource="#datasetdefinition"/>
 </owl:Class>
 
 <owl:Class rdf:ID="Altbier">
     <rdfs:subClassOf rdf:resource="#AmberBitterEuropeanBeer"/>
     <rdfs:subClassOf rdf:resource="#GermanBeer"/>
     <foaf:name>Altbier</foaf:name>
     <rdfs:label xml:lang="en">Altbier</rdfs:label>
     <rdfs:label xml:lang="fr">Altbier</rdfs:label>
     <skos:definition xml:lang="en">These beers are traditionally brewed near Düsseldorf, Germany. Altbier is an old style of beer that is typically amber colored, malty and somewhat bitter.</skos:definition>
     <skos:definition xml:lang="fr">Ces bières sont traditionnellement brassées près de Düsseldorf, en Allemagne. L'Altbier est une bière de style ancien qui est typiquement de couleur ambrée, maltée et quelque peu amère.</skos:definition>
     <prov:hadPrimarySource rdf:resource="#BJCP2015"/>
     <prov:hadPrimarySource rdf:resource="#Oliver2012"/>
     <rdfs:isDefinedBy rdf:resource="http://rdf.ag/o/beer-ONTOLOGY_DATE"/>
     <void:inDataset rdf:resource="#datasetdefinition"/>
 </owl:Class>
 
 <owl:Class rdf:ID="DarkEuropeanLager">
     <rdfs:subClassOf rdf:resource="#Lager"/>
     <rdfs:subClassOf rdf:resource="#EuropeanBeer"/>
     <foaf:name>Dark European Lager</foaf:name>
     <rdfs:label xml:lang="en">Dark European Lager</rdfs:label>
     <rdfs:label xml:lang="fr">Lager Européenne Foncée</rdfs:label>
     <skos:definition xml:lang="en">This style of beer includes strong (vollbier) lager that are darker in color than amber-brown colored beers.</skos:definition>
     <skos:definition xml:lang="fr">Ce style de bière comprend des bières blondes fortes (vollbier) de couleur plus foncée que les bières de couleur brun ambré.</skos:definition>
     <prov:hadPrimarySource rdf:resource="#BJCP2015"/>
     <rdfs:isDefinedBy rdf:resource="http://rdf.ag/o/beer-ONTOLOGY_DATE"/>
     <void:inDataset rdf:resource="#datasetdefinition"/>
 </owl:Class>
 
 <owl:Class rdf:ID="StrongEuropeanBeer">
     <rdfs:subClassOf rdf:resource="#Beer"/>
     <rdfs:subClassOf rdf:resource="#EuropeanBeer"/>
     <foaf:name>Strong European Beer</foaf:name>
     <rdfs:label xml:lang="en">Strong European Beer</rdfs:label>
     <rdfs:label xml:lang="fr">Bière Européenne Forte</rdfs:label>
     <skos:definition xml:lang="en">These are lagers from Germany and the Baltic regions of Europe and usually have higher alcohol contents and are stronger than other beers from the region. They are not limited to just dark colored beers.</skos:definition>
     <skos:definition xml:lang="fr">Ce sont des bières blondes d'Allemagne et des régions baltes d'Europe et ont généralement une teneur en alcool plus élevée et sont plus fortes que les autres bières de la région. Ils ne se limitent pas aux bières de couleur foncée.</skos:definition>
     <prov:hadPrimarySource rdf:resource="#BJCP2015"/>
     <rdfs:isDefinedBy rdf:resource="http://rdf.ag/o/beer-ONTOLOGY_DATE"/>
     <void:inDataset rdf:resource="#datasetdefinition"/>
 </owl:Class>
 
 <owl:Class rdf:ID="GermanWheatBeer">
     <rdfs:subClassOf rdf:resource="#WheatBeer"/>
     <rdfs:subClassOf rdf:resource="#GermanBeer"/>
     <foaf:name>German Wheat Beer</foaf:name>
     <rdfs:label xml:lang="en">German Wheat Beer</rdfs:label>
     <rdfs:label xml:lang="fr">Bière de Blé Allemande</rdfs:label>
     <skos:definition xml:lang="en">These wheat beers are strong and full bodied (vollbier and starkbier). They can be dark or pale colored and have no sourness to them.</skos:definition>
     <skos:definition xml:lang="fr">Ces bières de blé sont fortes et corsées (vollbier et starkbier). Ils peuvent être de couleur foncée ou pâle et n'avoir aucune aigreur.</skos:definition>
     <prov:hadPrimarySource rdf:resource="#BJCP2015"/>
     <rdfs:isDefinedBy rdf:resource="http://rdf.ag/o/beer-ONTOLOGY_DATE"/>
     <void:inDataset rdf:resource="#datasetdefinition"/>
 </owl:Class>
 
 <owl:Class rdf:ID="BritishBitter">
     <rdfs:subClassOf rdf:resource="#Beer"/>
     <rdfs:subClassOf rdf:resource="#BritishBeer"/>
     <foaf:name>British Bitter</foaf:name>
     <rdfs:label xml:lang="en">British Bitter</rdfs:label>
     <rdfs:label xml:lang="fr">Amer Britannique</rdfs:label>
     <skos:definition xml:lang="en">The beers in the style of British bitters are not reflective of the export formulations of a British Bitter, rather the 'real ale' version of this type of beer. This style covers a wide range of beers ranging from dark, sweet beers with no head to pale, hoppy and very foamy.</skos:definition>
     <skos:definition xml:lang="fr">Les bières dans le style des amères britanniques ne reflètent pas les formulations d'exportation d'une amère britannique, mais plutôt la version « vraie bière » de ce type de bière. Ce style couvre une large gamme de bières allant des bières brunes et sucrées sans mousse aux pâles, houblonnées et très mousseuses.</skos:definition>
     <prov:hadPrimarySource rdf:resource="#BJCP2015"/>
     <rdfs:isDefinedBy rdf:resource="http://rdf.ag/o/beer-ONTOLOGY_DATE"/>
     <void:inDataset rdf:resource="#datasetdefinition"/>
 </owl:Class>
 
 <owl:Class rdf:ID="PaleCommonwealthBeer">
     <rdfs:subClassOf rdf:resource="#Beer"/>
     <rdfs:subClassOf rdf:resource="#BritishBeer"/>
     <foaf:name>Pale Commonwealth Beer</foaf:name>
     <rdfs:label xml:lang="en">Pale Commonwealth Beer</rdfs:label>
     <rdfs:label xml:lang="fr">Bière Pâle du Commonwealth</rdfs:label>
     <skos:definition xml:lang="en">These beers are all from countries that once belonged to the former British Empire. They are light in color, hop forward, bitter, and moderately strong.</skos:definition>
     <skos:definition xml:lang="fr">Ces bières proviennent toutes de pays ayant appartenu à l'ancien Empire britannique. Ils sont de couleur claire, sautent en avant, amers et modérément forts.</skos:definition>
     <prov:hadPrimarySource rdf:resource="#BJCP2015"/>
     <rdfs:isDefinedBy rdf:resource="http://rdf.ag/o/beer-ONTOLOGY_DATE"/>
     <void:inDataset rdf:resource="#datasetdefinition"/>
 </owl:Class>
 
 <owl:Class rdf:ID="BrownBritishBeer">
     <rdfs:subClassOf rdf:resource="#Beer"/>
     <rdfs:subClassOf rdf:resource="#BritishBeer"/>
     <foaf:name>Brown British Beer</foaf:name>
     <rdfs:label xml:lang="en">Brown British Beer</rdfs:label>
     <rdfs:label xml:lang="fr">Bière Brune Britannique</rdfs:label>
     <skos:definition xml:lang="en">While these beers have no historic relationship with each other, they are grouped in the Brown British Beer style due to their similarites regarding their dark color, moderate strength, British origin and malty balance.</skos:definition>
     <skos:definition xml:lang="fr">Bien que ces bières n'aient aucune relation historique entre elles, elles sont regroupées dans le style Brown British Beer en raison de leurs similitudes concernant leur couleur sombre, leur force modérée, leur origine britannique et leur équilibre malté.</skos:definition>
     <prov:hadPrimarySource rdf:resource="#BJCP2015"/>
     <rdfs:isDefinedBy rdf:resource="http://rdf.ag/o/beer-ONTOLOGY_DATE"/>
     <void:inDataset rdf:resource="#datasetdefinition"/>
 </owl:Class>
 
 <owl:Class rdf:ID="ScottishBeer">
     <rdfs:subClassOf rdf:resource="#Beer"/>
     <rdfs:subClassOf rdf:resource="#BritishBeer"/>
     <foaf:name>Scottish Beer</foaf:name>
     <rdfs:label xml:lang="en">Scottish Beer</rdfs:label>
     <rdfs:label xml:lang="fr">Bière Écossaise</rdfs:label>
     <skos:definition xml:lang="en">Scottish Beers used to be described in shillings - or the price of a barrel of beer - now they are divided into three subcategories: Light, Heavy and Export. These beers are usually hop forward, using more caramelized hops, and usually have ABVs on the lower end.</skos:definition>
     <skos:definition xml:lang="fr">Les bières Écossaises étaient autrefois décrites en shillings - ou le prix d'un baril de bière - elles sont maintenant divisées en trois sous-catégories: Léger, Lourd et Exportation. Ces bières sont généralement houblonnées, utilisant des houblons plus caramélisés et ont généralement des ABV à l'extrémité inférieure.</skos:definition>
     <prov:hadPrimarySource rdf:resource="#BJCP2015"/>
     <rdfs:isDefinedBy rdf:resource="http://rdf.ag/o/beer-ONTOLOGY_DATE"/>
     <void:inDataset rdf:resource="#datasetdefinition"/>
 </owl:Class>
 
 <owl:Class rdf:ID="IrishBeer">
     <rdfs:subClassOf rdf:resource="#Beer"/>
     <rdfs:subClassOf rdf:resource="#BritishBeer"/>
     <foaf:name>Irish Beer</foaf:name>
     <rdfs:label xml:lang="en">Irish Beer</rdfs:label>
     <rdfs:label xml:lang="fr">Bière Irlandaise</rdfs:label>
     <skos:definition xml:lang="en">This style of beers contains traditional Irish top-fermenting beers that range from being amber to dark, and moderate to being slightly strong.</skos:definition>
     <skos:definition xml:lang="fr">Ce style de bières contient des bières irlandaises traditionnelles à fermentation haute qui vont d'ambrées à foncées, et modérées à légèrement fortes.</skos:definition>
     <prov:hadPrimarySource rdf:resource="#BJCP2015"/>
     <rdfs:isDefinedBy rdf:resource="http://rdf.ag/o/beer-ONTOLOGY_DATE"/>
     <void:inDataset rdf:resource="#datasetdefinition"/>
 </owl:Class>
 
 <owl:Class rdf:ID="NorthAmericanBeer">
     <rdfs:subClassOf rdf:resource="#Beer"/>
     <foaf:name>North American Beer</foaf:name>
     <rdfs:label xml:lang="en">North American Beer</rdfs:label>
     <rdfs:label xml:lang="fr">Bière Nord-Américaine</rdfs:label>
     <skos:definition xml:lang="en">Beers whose style originated from North America.</skos:definition>
     <skos:definition xml:lang="fr">Des bières dont le style est originaire d'Amérique du Nord.</skos:definition>
     <prov:hadPrimarySource rdf:resource="#AHA2021"/>
     <prov:hadPrimarySource rdf:resource="#BA2021"/>
     <rdfs:isDefinedBy rdf:resource="http://rdf.ag/o/beer-ONTOLOGY_DATE"/>
     <void:inDataset rdf:resource="#datasetdefinition"/>
 </owl:Class>
 
 <owl:Class rdf:ID="EuropeanBeer">
     <rdfs:subClassOf rdf:resource="#Beer"/>
     <foaf:name>European Beer</foaf:name>
     <rdfs:label xml:lang="en">European Beer</rdfs:label>
     <rdfs:label xml:lang="fr">Bière Européenne</rdfs:label>
     <skos:definition xml:lang="en">Beers whose style originated from Europe.</skos:definition>
     <skos:definition xml:lang="fr">Des bières dont le style est originaire d'Europe.</skos:definition>
     <prov:hadPrimarySource rdf:resource="#AHA2021"/>
     <prov:hadPrimarySource rdf:resource="#BA2021"/>
     <rdfs:isDefinedBy rdf:resource="http://rdf.ag/o/beer-ONTOLOGY_DATE"/>
     <void:inDataset rdf:resource="#datasetdefinition"/>
 </owl:Class>
 
 <owl:Class rdf:ID="BritishBeer">
     <rdfs:subClassOf rdf:resource="#EuropeanBeer"/>
     <foaf:name>British Beer</foaf:name>
     <rdfs:label xml:lang="en">British Beer</rdfs:label>
     <rdfs:label xml:lang="en">English Beer</rdfs:label>
     <rdfs:label xml:lang="fr">Bière Anglaise</rdfs:label>
     <skos:definition xml:lang="en">Beers whose style originated from Great Britain or countries that are part of the British Commonwealth.</skos:definition>
     <skos:definition xml:lang="fr">Bières dont le style est originaire de Grande-Bretagne ou de pays faisant partie du Commonwealth britannique.</skos:definition>
     <prov:hadPrimarySource rdf:resource="#AHA2021"/>
     <prov:hadPrimarySource rdf:resource="#BA2021"/>
     <rdfs:isDefinedBy rdf:resource="http://rdf.ag/o/beer-ONTOLOGY_DATE"/>
     <void:inDataset rdf:resource="#datasetdefinition"/>
 </owl:Class>
 
 <owl:Class rdf:ID="GermanBeer">
     <rdfs:subClassOf rdf:resource="#EuropeanBeer"/>
     <foaf:name>German Beer</foaf:name>
     <rdfs:label xml:lang="en">German Beer</rdfs:label>
     <rdfs:label xml:lang="fr">Bière Allemande</rdfs:label>
     <skos:definition xml:lang="en">Beers whose style originated from Germany.</skos:definition>
     <skos:definition xml:lang="fr">Bières dont le style est originaire d'Allemagne.</skos:definition>
     <prov:hadPrimarySource rdf:resource="#AHA2021"/>
     <prov:hadPrimarySource rdf:resource="#BA2021"/>
     <rdfs:isDefinedBy rdf:resource="http://rdf.ag/o/beer-ONTOLOGY_DATE"/>
     <void:inDataset rdf:resource="#datasetdefinition"/>
 </owl:Class>

 <owl:Class rdf:ID="BraggotBeer">
  <foaf:name>Braggot Beer</foaf:name>
  <rdfs:label xml:lang="en">Braggot Beer</rdfs:label>
  <rdfs:label xml:lang="fr">Bière Braggot</rdfs:label>
  <skos:definition xml:lang="en">A beer made with both malt and honey.</skos:definition>
  <skos:definition xml:lang="fr">Une bière faite avec du miel et du malt.</skos:definition> 
  <prov:hadPrimarySource rdf:resource="#BJCP2015"/>
  <rdfs:isDefinedBy rdf:resource="http://rdf.ag/o/beer-ONTOLOGY_DATE"/>
  <void:inDataset rdf:resource="#datasetdefinition"/>
  <dcterms:creator rdf:resource="#warren"/>
 </owl:Class>
 
 <owl:Class rdf:ID="DarkBritishBeer">
     <rdfs:subClassOf rdf:resource="#Stout"/>
     <rdfs:subClassOf rdf:resource="#BritishBeer"/>
     <foaf:name>Dark British Beer</foaf:name>
     <rdfs:label xml:lang="en">Dark British Beer</rdfs:label>
     <skos:definition xml:lang="en">These beers are typically strong stouts that range from being sweet to bitter. 'British' in this category refers to the broader British Isles rather than Great Britain, which is why some Irish beers are included in this beer style.</skos:definition>
     <skos:definition xml:lang="fr">Ces bières sont généralement des stouts forts qui vont du sucré à l'amer. 'Britannique' dans cette catégorie fait référence aux îles britanniques au sens large plutôt qu'à la Grande-Bretagne, c'est pourquoi certaines bières irlandaises sont incluses dans ce style de bière.</skos:definition>
     <prov:hadPrimarySource rdf:resource="#BJCP2015"/>
     <rdfs:isDefinedBy rdf:resource="http://rdf.ag/o/beer-ONTOLOGY_DATE"/>
     <void:inDataset rdf:resource="#datasetdefinition"/>
 </owl:Class>
 
 <owl:Class rdf:ID="StrongBritishAle">
     <rdfs:subClassOf rdf:resource="#Ale"/>
     <rdfs:subClassOf rdf:resource="#BritishBeer"/>
     <foaf:name>Strong British Ale</foaf:name>
     <rdfs:label xml:lang="en">Strong British Ale</rdfs:label>
     <rdfs:label xml:lang="fr">Ale Britannique Forte</rdfs:label>
     <skos:definition xml:lang="en">These beers are from the British Isles and are typically strong and non-roasty.</skos:definition>
     <skos:definition xml:lang="fr">Ces bières proviennent des îles britanniques et sont généralement fortes et non torréfiées.</skos:definition>
     <prov:hadPrimarySource rdf:resource="#BJCP2015"/>
     <rdfs:isDefinedBy rdf:resource="http://rdf.ag/o/beer-ONTOLOGY_DATE"/>
     <void:inDataset rdf:resource="#datasetdefinition"/>
 </owl:Class>
 
 <owl:Class rdf:ID="AmberandBrownAmericanBeer">
     <rdfs:subClassOf rdf:resource="#AmericanBeer"/>
     <foaf:name>Amber and Brown American Beer</foaf:name>
     <rdfs:label xml:lang="en">Amber and Brown American Beer</rdfs:label>
     <rdfs:label xml:lang="fr">Bière Américaine Ambrée et Brune</rdfs:label>
     <skos:definition xml:lang="en">These beers are warm-fermented beers that are of standard strength and range from amber to brown colored.</skos:definition>
     <skos:definition xml:lang="fr">Ces bières sont des bières à fermentation chaude qui sont de force standard et vont de l'ambre au brun.</skos:definition>
     <prov:hadPrimarySource rdf:resource="#BJCP2015"/>
     <rdfs:isDefinedBy rdf:resource="http://rdf.ag/o/beer-ONTOLOGY_DATE"/>
     <void:inDataset rdf:resource="#datasetdefinition"/>
 </owl:Class>
 
 <owl:Class rdf:ID="AmericanPorterandStout">
     <rdfs:subClassOf rdf:resource="#AmericanBeer"/>
     <foaf:name>American Porter and Stout</foaf:name>
     <rdfs:label xml:lang="en">American Porter and Stout</rdfs:label>
     <rdfs:label xml:lang="fr">Porter Américain et Stout</rdfs:label>
     <skos:definition xml:lang="en">These beers are strong, hop-centric, and roast-forward. They have been grouped together due to similar histories and flavor profiles.</skos:definition>
     <skos:definition xml:lang="fr">Ces bières sont fortes, axées sur le houblon et torréfiées. Ils ont été regroupés en raison d'histoires et de profils de saveur similaires.</skos:definition>
     <prov:hadPrimarySource rdf:resource="#BJCP2015"/>
     <rdfs:isDefinedBy rdf:resource="http://rdf.ag/o/beer-ONTOLOGY_DATE"/>
     <void:inDataset rdf:resource="#datasetdefinition"/>
 </owl:Class>
 
 <owl:Class rdf:ID="StrongAmericanAle">
     <rdfs:subClassOf rdf:resource="#Ale"/>
     <rdfs:subClassOf rdf:resource="#AmericanBeer"/>
     <foaf:name>Strong American Ale</foaf:name>
     <rdfs:label xml:lang="en">Strong American Ale</rdfs:label>
     <rdfs:label xml:lang="fr">Ale Américaine Forte</rdfs:label>
     <skos:definition xml:lang="en">These beers are characterized by their strong profiles that have high ABVs and lacking roast.</skos:definition>
     <skos:definition xml:lang="fr">Ces bières se caractérisent par leurs profils forts qui ont des ABV élevés et manquent de torréfaction.</skos:definition>
     <prov:hadPrimarySource rdf:resource="#BJCP2015"/>
     <rdfs:isDefinedBy rdf:resource="http://rdf.ag/o/beer-ONTOLOGY_DATE"/>
     <void:inDataset rdf:resource="#datasetdefinition"/>
 </owl:Class>
 
 <owl:Class rdf:ID="EuropeanSourAle">
     <rdfs:subClassOf rdf:resource="#Ale"/>
     <rdfs:subClassOf rdf:resource="#SourBeer"/>
     <rdfs:subClassOf rdf:resource="#EuropeanBeer"/>
     <foaf:name>European Sour Ale</foaf:name>
     <rdfs:label xml:lang="en">European Sour Ale</rdfs:label>
     <rdfs:label xml:lang="fr">Ale Aigre Européenn</rdfs:label>
     <skos:definition xml:lang="en">These beers represent the traditional sour beers of Europe that have a wheat base for the most part and low bitterness.</skos:definition>
     <skos:definition xml:lang="fr">Ces bières représentent les bières acidulées traditionnelles d'Europe qui ont pour la plupart une base de blé et une faible amertume.</skos:definition>
     <prov:hadPrimarySource rdf:resource="#BJCP2015"/>
     <rdfs:isDefinedBy rdf:resource="http://rdf.ag/o/beer-ONTOLOGY_DATE"/>
     <void:inDataset rdf:resource="#datasetdefinition"/>
 </owl:Class>
 
 <owl:Class rdf:ID="TrappistAle">
     <rdfs:subClassOf rdf:resource="#Ale"/>
     <foaf:name>Trappist Ale</foaf:name>
     <rdfs:label xml:lang="en">Trappist Ale</rdfs:label>
     <rdfs:label xml:lang="fr">Bière Trappiste</rdfs:label>
     <skos:definition xml:lang="en">The term 'Trappist' used to describe beer is a protected appelation  to be used only by the beer-brewing Trappists monastaries. Trappist Ales are characterized as being highly carbonated and attenuated with a strong yeast character.</skos:definition>
     <skos:definition xml:lang="fr">Le terme 'Trappiste' utilisé pour décrire la bière est une appellation protégée qui n'est utilisée que par les monastères trappistes brasseurs de bière. Les Trappist Ales sont caractérisées comme étant hautement carbonatées et atténuées avec un fort caractère de levure.</skos:definition>
     <prov:hadPrimarySource rdf:resource="#BJCP2015"/>
     <rdfs:isDefinedBy rdf:resource="http://rdf.ag/o/beer-ONTOLOGY_DATE"/>
     <void:inDataset rdf:resource="#datasetdefinition"/>
 </owl:Class>
 
 <owl:Class rdf:ID="HistoricalBeer">
     <rdfs:subClassOf rdf:resource="#Beer"/>
     <foaf:name>Historical Beer</foaf:name>
     <rdfs:label xml:lang="en">Historical Beer</rdfs:label>
     <rdfs:label xml:lang="fr">Bière Historique</rdfs:label>
     <skos:definition xml:lang="en">This category of beer styles includes beer that are recreations and rediscoveries of traditional beers but also beer styles that have died out and are no longer in production today.</skos:definition>
     <skos:definition xml:lang="fr">Cette catégorie de styles de bière comprend les bières qui sont des recréations et redécouvertes de bières traditionnelles mais aussi des styles de bière qui ont disparu et ne sont plus en production aujourd'hui.</skos:definition>
     <prov:hadPrimarySource rdf:resource="#BJCP2015"/>
     <rdfs:isDefinedBy rdf:resource="http://rdf.ag/o/beer-ONTOLOGY_DATE"/>
     <void:inDataset rdf:resource="#datasetdefinition"/>
 </owl:Class>
 
 <owl:Class rdf:ID="AmericanWildAle">
     <rdfs:subClassOf rdf:resource="#Ale"/>
     <rdfs:subClassOf rdf:resource="#AmericanBeer"/>
     <foaf:name>American Wild Ale</foaf:name>
     <rdfs:label xml:lang="en">American Wild Ale</rdfs:label>
     <rdfs:label xml:lang="fr">Ale Sauvage Américain</rdfs:label>
     <skos:definition xml:lang="en">The term 'Wild' in the name of this category has to do with the fact that the flavors of these beers are influenced more by microbial processes rather than by the traditional brewer's yeasts. These are specialty beers that cover a wide variety of styles that don't fit traditional styles but have similar fermentation ingredients and profiles.</skos:definition>
     <skos:definition xml:lang="fr">Le terme 'sauvage' dans le nom de cette catégorie est lié au fait que les saveurs de ces bières sont davantage influencées par des processus microbiens que par les levures de bière traditionnelles. Ce sont des bières de spécialité qui couvrent une grande variété de styles qui ne correspondent pas aux styles traditionnels mais qui ont des ingrédients et des profils de fermentation similaires.</skos:definition>
     <prov:hadPrimarySource rdf:resource="#BJCP2015"/>
     <rdfs:isDefinedBy rdf:resource="http://rdf.ag/o/beer-ONTOLOGY_DATE"/>
     <void:inDataset rdf:resource="#datasetdefinition"/>
 </owl:Class>
 
 <owl:Class rdf:ID="FruitBeer">
     <rdfs:subClassOf rdf:resource="#Beer"/>
     <foaf:name>Fruit Beer</foaf:name>
     <rdfs:label xml:lang="en">Fruit Beer</rdfs:label>
     <rdfs:label xml:lang="fr">Bière aux Fruits</rdfs:label>
     <skos:definition xml:lang="en">Fruit beers involve the use of fruit in the beer brewing process. It is important to note that the culinary definition of 'fruit' is used, which are plant structures that are sweet or sour, have a seed or seeds and can be eaten raw.</skos:definition>
     <skos:definition xml:lang="fr">Les bières aux fruits impliquent l'utilisation de fruits dans le processus de brassage de la bière. Il est important de noter que la définition culinaire de «fruit» est utilisée, qui sont des structures végétales aigre-douces, ont une graine ou des graines et peuvent être consommées crues.</skos:definition>
     <prov:hadPrimarySource rdf:resource="#BJCP2015"/>
     <rdfs:isDefinedBy rdf:resource="http://rdf.ag/o/beer-ONTOLOGY_DATE"/>
     <void:inDataset rdf:resource="#datasetdefinition"/>
 </owl:Class>

 <owl:Class rdf:ID="SpicedBeer">
     <rdfs:subClassOf rdf:resource="#Beer"/>
     <foaf:name>Spiced Beer</foaf:name>
     <rdfs:label xml:lang="en">Spiced Beer</rdfs:label>
     <rdfs:label xml:lang="fr">Bière Épicée</rdfs:label>
     <skos:definition xml:lang="en">These are beers that a brewed with the culinary definitions of vegetable, herbs, and spices. In this instance 'vegetable' is defined as a part of a plant that is less sweet than the fruit of a plant, savory and can sometimes be eaten raw. 'Herbs' are the leafy parts of plants used for flavoring food such as petals, flowers, and stalks. 'Spices' are the dried, non-leafy parts of plants used for flavoring and can include seeds, bark, roots and fruit.</skos:definition>
     <skos:definition xml:lang="fr">Ce sont des bières brassées avec les définitions culinaires des légumes, des herbes et des épices. Dans ce cas, le 'légume' est défini comme une partie d'une plante qui est moins sucrée que le fruit d'une plante, salée et peut parfois être consommée crue. Les 'herbes' sont les parties feuillues des plantes utilisées pour aromatiser les aliments tels que les pétales, les fleurs et les tiges. Les 'épices' sont les parties séchées et non feuillues des plantes utilisées pour aromatiser et peuvent inclure les graines, l'écorce, les racines et les fruits.</skos:definition>
     <prov:hadPrimarySource rdf:resource="#BJCP2015"/>
     <rdfs:isDefinedBy rdf:resource="http://rdf.ag/o/beer-ONTOLOGY_DATE"/>
     <void:inDataset rdf:resource="#datasetdefinition"/>
 </owl:Class>
     
 <owl:Class rdf:ID="AlternativeFermentablesBeer">
     <rdfs:subClassOf rdf:resource="#Beer"/>
     <foaf:name>Alternative Fermentables Beer</foaf:name>
     <rdfs:label xml:lang="en">Alternative Fermentables Beer</rdfs:label>
     <rdfs:label xml:lang="fr">Bière Fermentable Alternative</rdfs:label>
     <skos:definition xml:lang="en">These are specialty beers that use additional ingredients to add distinct flavoring such as grain or sugar.</skos:definition>
     <skos:definition xml:lang="fr">Ce sont des bières spéciales qui utilisent des ingrédients supplémentaires pour ajouter des arômes distincts tels que des céréales ou du sucre.</skos:definition>
     <prov:hadPrimarySource rdf:resource="#BJCP2015"/>
     <rdfs:isDefinedBy rdf:resource="http://rdf.ag/o/beer-ONTOLOGY_DATE"/>
     <void:inDataset rdf:resource="#datasetdefinition"/>
 </owl:Class>
 
 <owl:Class rdf:ID="SmokedBeer">
     <rdfs:subClassOf rdf:resource="#Beer"/>
     <foaf:name>Smoked Beer</foaf:name>
     <rdfs:label xml:lang="en">Smoked Beer</rdfs:label>
     <rdfs:label xml:lang="fr">Bière Fumée</rdfs:label>
     <skos:definition xml:lang="en">These are specialty beers that have a distinct smokey aroma.</skos:definition>
     <skos:definition xml:lang="fr">Ce sont des bières de spécialité qui ont un arôme fumé distinct.</skos:definition>
     <prov:hadPrimarySource rdf:resource="#BJCP2015"/>
     <rdfs:isDefinedBy rdf:resource="http://rdf.ag/o/beer-ONTOLOGY_DATE"/>
     <void:inDataset rdf:resource="#datasetdefinition"/>
 </owl:Class>
 
 <owl:Class rdf:ID="WoodBeer">
     <rdfs:subClassOf rdf:resource="#Beer"/>
     <foaf:name>Wood Beer</foaf:name>
     <rdfs:label xml:lang="en">Wood Beer</rdfs:label>
     <rdfs:label xml:lang="fr">Bière De Bois</rdfs:label>
     <skos:definition xml:lang="en">These are specialty beers that have a wood-aged aroma.</skos:definition>
     <skos:definition xml:lang="fr">Ce sont des bières de spécialité qui ont un arôme de bois vieilli.</skos:definition>
     <prov:hadPrimarySource rdf:resource="#BJCP2015"/>
     <rdfs:isDefinedBy rdf:resource="http://rdf.ag/o/beer-ONTOLOGY_DATE"/>
     <void:inDataset rdf:resource="#datasetdefinition"/>
 </owl:Class>
 
 <owl:Class rdf:ID="SpecialtyBeer">
     <rdfs:subClassOf rdf:resource="#Beer"/>
     <foaf:name>Specialty Beer</foaf:name>
     <rdfs:label xml:lang="en">Specialty Beer</rdfs:label>
     <rdfs:label xml:lang="en">Hybrid/Mixed Beer</rdfs:label>
     <rdfs:label xml:lang="fr">Bière de Spécialité</rdfs:label>
     <skos:definition xml:lang="en">These are specialty beers that do not fit in any other category of beer.</skos:definition>
     <skos:definition xml:lang="fr">Ce sont des bières de spécialité qui ne rentrent dans aucune autre catégorie de bière.</skos:definition>
     <prov:hadPrimarySource rdf:resource="#BJCP2015"/>
     <prov:hadPrimarySource rdf:resource="#AHA2021"/>
     <rdfs:isDefinedBy rdf:resource="http://rdf.ag/o/beer-ONTOLOGY_DATE"/>
     <void:inDataset rdf:resource="#datasetdefinition"/>
 </owl:Class>
 
 <owl:Class rdf:ID="BelgianBeer">
     <rdfs:subClassOf rdf:resource="#EuropeanBeer"/>
     <foaf:name>Belgian Beer</foaf:name>
     <rdfs:label xml:lang="en">Belgian Beer</rdfs:label>
     <rdfs:label xml:lang="en">French Beer</rdfs:label>
     <rdfs:label xml:lang="fr">Bière Belge</rdfs:label>
     <skos:definition xml:lang="en">Belgian beers are a grouping of beer styles produced in Belgium or in the Belgian style. These styles are mostly ales that use fruity yeasts and malts. French beers are also included in this categorization.</skos:definition>
     <skos:definition xml:lang="fr">Les bières belges sont un regroupement de styles de bières produits en Belgique ou dans le style belge. Ces styles sont principalement des ales qui utilisent des levures et des malts fruités. Les bières françaises sont également incluses dans cette catégorisation.</skos:definition>
     <rdfs:isDefinedBy rdf:resource="https://rdf.ag/o/beer-ONTOLOGY_DATE"/>
     <void:inDataset rdf:resource="#datasetdefinition"/>
 </owl:Class>
         
 <owl:Class rdf:ID="Ale">
     <rdfs:subClassOf rdf:resource="#Beer"/>
     <foaf:name>Ale</foaf:name>
     <rdfs:label xml:lang="en">Ale</rdfs:label>
     <skos:definition xml:lang="en">The main distinguishing feature of an ale is the type of yeast used in the brewing process, Saccharomyces cerevisiae. S. cerevisiae typically prefers a warmer brewing range and lacks the ability to metabolize the complex sugars: melibiose and raffinose.
         
         Ales are typically fermented, depending of course on the strain yeast, at 16-24˚C (60-75˚F) temperature range. Which is typically, but not exclusively, warmer than lager fermentation.
         
         Ales also do not undergo a cold-conditioning phase. However it is not uncommon for some lagers to not undergo a cold phase.</skos:definition>
     <skos:definition xml:lang="fr">La principale caractéristique distinctive d'un Ale est le type de levure utilisé dans le processus de brassage, Saccharomyces cerevisiae. S. cerevisiae préfère généralement une gamme de brassage plus chaude et n'a pas la capacité de métaboliser les sucres complexes: mélibiose et raffinose.
         
         Les Ales sont généralement fermentées, en fonction bien sûr de la souche de levure, à 16-24°C (60-75°F). Ce qui est généralement, mais pas exclusivement, plus chaud que la fermentation de lager.
         
         Les Ales ne subissent pas non plus de phase de conditionnement à froid. Cependant, il n'est pas rare que certaines lagers ne subissent pas de phase froide.</skos:definition>
     <prov:hadPrimarySource rdf:resource="#Carpenter2017"/>
     <rdfs:isDefinedBy rdf:resource="https://rdf.ag/o/beer-ONTOLOGY_DATE"/>
     <void:inDataset rdf:resource="#datasetdefinition"/>
 </owl:Class>
 
 <owl:Class rdf:ID="CreamAle">
     <rdfs:subClassOf rdf:resource="#Ale"/>
     <rdfs:subClassOf rdf:resource="#AmericanBeer"/>
     <rdfs:label xml:lang="en">Cream Ale</rdfs:label>
     <skos:definition xml:lang="en">While considered ales, cream beers more closely resemble light lagers in terms of taste. Contrary to the name, cream beers do not necessarily contain cream or other milk products or derivatives. They do however contain adjuct ingredients which could contain lactose or milk sugar but could be fruit, coffee, mint, vanilla, other grains, or even nitrogenated gas that attributes to a more 'creamy' texture. These beers are typically more alcoholic and bitter compared to other light ales.
         
         Cream ales use yeasts that are typically used for lagers, but could sometimes include yeasts for ales. Even with a lager yeast, the beer is fermented at a higher temperature, which is typical for ales.</skos:definition>
     <skos:definition xml:lang="fr">Bien que considérées comme des ales, les bières à la crème ressemblent davantage à des lagers légères en termes de goût. Contrairement à leur nom, les bières à la crème ne contiennent pas nécessairement de crème ou d'autres produits laitiers ou dérivés. Ils contiennent cependant des ingrédients adjuvants qui pourraient contenir du lactose ou du sucre de lait mais qui pourraient être des fruits, du café, de la menthe, de la vanille, d'autres céréales ou même du gaz azoté qui donne une texture plus «crémeuse». Ces bières sont généralement plus alcoolisées et amères que les autres bières légères.
         
         Les bières à la crème utilisent des levures qui sont généralement utilisées pour les bières blondes, mais peuvent parfois inclure des levures pour les bières. Même avec une levure de bière blonde, la bière est fermentée à une température plus élevée, ce qui est typique des ales.</skos:definition>
     <prov:hadPrimarySource rdf:resource="#Oliver2012"/>
     <rdfs:isDefinedBy rdf:resource="https://rdf.ag/o/beer-ONTOLOGY_DATE"/>
     <void:inDataset rdf:resource="#datasetdefinition"/>
 </owl:Class>
 
 <owl:Class rdf:ID="BelgianAle">
     <rdfs:subClassOf rdf:resource="#Ale"/>
     <rdfs:subClassOf rdf:resource="#BelgianBeer"/>
     <foaf:name>Belgian Ale</foaf:name>
     <rdfs:label xml:lang="en">Belgian Ale</rdfs:label>
     <rdfs:label xml:lang="en">French Ale</rdfs:label>
     <rdfs:label xml:lang="fr">Bière Belge</rdfs:label>
     <skos:definition xml:lang="en">Belgian Ales are flavorful Belgian and French Ales that range from being balanced to malty.</skos:definition>
     <skos:definition xml:lang="fr">Les bières belges sont des bières belges et françaises savoureuses qui vont de l'équilibre au malté.</skos:definition>
     <prov:hadPrimarySource rdf:resource="#AHA2021"/>
     <prov:hadPrimarySource rdf:resource="#BJCP2015"/>
     <rdfs:isDefinedBy rdf:resource="http://rdf.ag/o/beer-ONTOLOGY_DATE"/>
     <void:inDataset rdf:resource="#datasetdefinition"/>
 </owl:Class>
 
 <owl:Class rdf:ID="StrongBelgianAle">
     <rdfs:subClassOf rdf:resource="#BelgianAle"/>
     <foaf:name>Strong Belgian Ale</foaf:name>
     <rdfs:label xml:lang="en">Strong Belgian Ale</rdfs:label>
     <rdfs:label xml:lang="fr">Ale Belge Forte</rdfs:label>
     <skos:definition xml:lang="en">Strong Belgian Ales are the stronger versions of Belgian Ales, they rely more on yeast for their flavor rather than malts as for most Belgian Ales and generally have higher alcohol content.</skos:definition>
     <skos:definition xml:lang="fr">Les Strong Belgian Ales sont les versions les plus fortes des Belgian Ales, elles reposent davantage sur la levure pour leur saveur plutôt que sur les malts comme pour la plupart des Belges Ales et ont généralement une teneur en alcool plus élevée.</skos:definition>
     <prov:hadPrimarySource rdf:resource="#BJCP2015"/>
     <rdfs:isDefinedBy rdf:resource="http://rdf.ag/o/beer-ONTOLOGY_DATE"/>
     <skos:definition xml:lang="en">Belgian Ales are ales are that are brewed in the Belgian style.</skos:definition>
     <skos:definition xml:lang="fr">Les bières belges sont des bières brassées dans le style belge.</skos:definition>
     <rdfs:isDefinedBy rdf:resource="https://rdf.ag/o/beer-ONTOLOGY_DATE"/>
     <void:inDataset rdf:resource="#datasetdefinition"/>
 </owl:Class>
 
 <owl:Class rdf:ID="EnglishStyleAle">
     <rdfs:subClassOf rdf:resource="#Ale"/>
     <rdfs:subClassOf rdf:resource="#BritishBeer"/>
     <foaf:name>English Style Ale</foaf:name>
     <rdfs:label xml:lang="en">British Style Ale</rdfs:label>
     <rdfs:label xml:lang="en">English Style Ale</rdfs:label>
     <rdfs:label xml:lang="fr">Style Anglais</rdfs:label>
     <skos:definition xml:lang="en">English Style Ales are ales are that are brewed in the English style.</skos:definition>
     <skos:definition xml:lang="fr">Les ales à l'anglaise sont des ales brassées dans le style Anglais.</skos:definition>
     <rdfs:isDefinedBy rdf:resource="https://rdf.ag/o/beer-ONTOLOGY_DATE"/>
     <void:inDataset rdf:resource="#datasetdefinition"/>
 </owl:Class>
 
 <owl:Class rdf:ID="PaleAle">
     <rdfs:subClassOf rdf:resource="#Ale"/>
     <foaf:name>Pale Ale</foaf:name>
     <rdfs:label xml:lang="en">Pale Ale</rdfs:label>
     <rdfs:label xml:lang="en">Ale Pâle</rdfs:label>
     <rdfs:label xml:lang="fr">Une Blonde</rdfs:label>
     <skos:definition xml:lang="en">Pale Ales are a style of beer that are typically light in color, have stong hop flavors, and low in alcohol content. This umbrella term includes IPAs, APAs and English pale ales.
      
      Most Pale Ales are english-style, since it has become quite popular, many countries developed their own versions of pale ales that originated from English style of brewing beer.
      
      Samuel Allsopp in Burton, UK brewed the first pale ale for the Indian market in 1822 and it was shipped in 1823 to India which had a lasting impact that lead to the rise of India Pale Ales.
      
     Pale ales used to be called "bitter ales" in the past but now it has become three versions being "ordinary" that range in 3%-4% ABV, "special" and "extra special" that range 4.5-5% ABV.</skos:definition>
     <skos:definition xml:lang="fr">Les Pale Ales sont un style de bière généralement de couleur claire, aux saveurs de houblon fort et à faible teneur en alcool. Ce terme générique comprend les IPA, les APA et les Ales Pâle Anglaises.
         
         La plupart des Pale Ales sont de style anglais, car elles sont devenues très populaires, de nombreux pays ont développé leurs propres versions de pâles ales qui provenaient du style anglais de brassage de bière.
         
         Samuel Allsopp à Burton, au Royaume-Uni, a brassé la première Ale Pâle pour le marché indien en 1822 et elle a été expédiée en 1823 en Inde, ce qui a eu un impact durable qui a conduit à l'essor des India Pale Ales.
         
         Les ales pâles étaient autrefois appelées «bitter ales», mais maintenant elles sont devenues trois versions «ordinaires» qui vont de 3% -4% ABV, «spéciales» et «extra spéciales» qui vont de 4,5-5% ABV.</skos:definition>
     <prov:hadPrimarySource rdf:resource="#Foster2020"/>
     <prov:hadPrimarySource rdf:resource="#Foster1999"/>
     <prov:hadPrimarySource rdf:resource="#Oliver2012"/>
     <prov:hadPrimarySource rdf:resource="#Jackson1993"/>
     <rdfs:isDefinedBy rdf:resource="https://rdf.ag/o/beer-ONTOLOGY_DATE"/>
     <void:inDataset rdf:resource="#datasetdefinition"/>
 </owl:Class>
 
 <owl:Class rdf:ID="SummerAle">
     <rdfs:subClassOf rdf:resource="#Ale"/>
     <foaf:name>Summer Ale</foaf:name>
     <rdfs:label xml:lang="en">Summer Ale</rdfs:label>
     <rdfs:label xml:lang="fr">Ale d'Été</rdfs:label>
     <skos:definition xml:lang="en">Summer Ales are typically characterized as citrus-y and refreshing summer beer. They are most commonly a form of American Wheat beer or English-style summer ale, but can include other styles of ale.</skos:definition>
     <skos:definition xml:lang="fr">Les bières d'été sont généralement caractérisées comme une bière d'été aux agrumes et rafraîchissante. Ils sont le plus souvent une forme de bière de blé américaine, mais peuvent inclure d'autres styles de bière.</skos:definition>
     <rdfs:isDefinedBy rdf:resource="https://rdf.ag/o/beer-ONTOLOGY_DATE"/>
     <void:inDataset rdf:resource="#datasetdefinition"/>
 </owl:Class>

 <owl:Class rdf:ID="EnglishPaleAle">
     <rdfs:subClassOf rdf:resource="#PaleAle"/>
     <rdfs:subClassOf rdf:resource="#EnglishStyleAle"/>
     <foaf:name>English Pale Ale</foaf:name>
     <rdfs:label xml:lang="en">English Pale Ale</rdfs:label>
     <rdfs:label xml:lang="en">British Pale Ale</rdfs:label>
     <rdfs:label xml:lang="en">English-Style Pale Ale</rdfs:label>
     <skos:definition xml:lang="en">English Pale Ale is a type of pale ale that is brewed in the English style, usually more with more hop flavor and bitterness.</skos:definition>
     <skos:definition xml:lang="fr">La Pale Ale anglaise est un type de ale pâle brassée dans le style anglais, généralement plus avec plus de saveur de houblon et d'amertume.</skos:definition>
     <rdfs:isDefinedBy rdf:resource="https://rdf.ag/o/beer-ONTOLOGY_DATE"/>
     <void:inDataset rdf:resource="#datasetdefinition"/>
 </owl:Class>
 
 <owl:Class rdf:ID="IndiaPaleAle">
     <rdfs:subClassOf rdf:resource="#EnglishPaleAle"/>
     <foaf:name>India Pale Ale</foaf:name>
     <rdfs:label xml:lang="en">IPA</rdfs:label>
     <skos:definition xml:lang="en">India Pale Ale is actually a type of pale ale that is brewed in the "English" style, contrary to its name. It was originally brewed for the Indian market which is where it got its name. It's origins are still debated to this day but this beer is known for its use of English hops and yeast.</skos:definition>
     <skos:definition xml:lang="fr">L'Inde Pale Ale est en fait un type de ale pâle qui est brassée dans le style "anglais", contrairement à son nom. Il était à l'origine brassé pour le marché indien, d'où il tire son nom. Ses origines sont encore débattues à ce jour, mais cette bière est connue pour son utilisation de houblon anglais et de levure.</skos:definition>
     <prov:hadPrimarySource rdf:resource="#Craftbeer.com2020IPA"/>
     <rdfs:isDefinedBy rdf:resource="https://rdf.ag/o/beer-ONTOLOGY_DATE"/>
     <void:inDataset rdf:resource="#datasetdefinition"/>
 </owl:Class>
 
 <owl:Class rdf:ID="AmericanPaleAle">
     <rdfs:subClassOf rdf:resource="#PaleAle"/>
     <rdfs:subClassOf rdf:resource="#AmericanBeer"/>
     <foaf:name>American Pale Ale</foaf:name>
     <rdfs:label xml:lang="en">APA</rdfs:label>
     <rdfs:label xml:lang="en">American Pale Ale</rdfs:label>
     <rdfs:label xml:lang="en">Pale American Ale</rdfs:label>
     <rdfs:label xml:lang="en">New World Pale Ale</rdfs:label>
     <rdfs:label xml:lang="fr">Pale Ale Américaine</rdfs:label>
     <skos:definition xml:lang="en">American Pale Ale is based on the English Pale Ale style however rather than the woody aromas of English hops, American IPAs use American hops that are usually more citrus and piney. These ales are pale and typically of average strength and are moderately malty and bitter.</skos:definition>
     <skos:definition xml:lang="fr">L'American Pale Ale est basée sur le style English Pale Ale, mais plutôt que les arômes boisés du houblon anglais, les IPA américaines utilisent des houblons américains qui sont généralement plus d'agrumes et de pin. Ces bières sont pâles et généralement de force moyenne et sont modérément maltées et amères.</skos:definition>
     <prov:hadPrimarySource rdf:resource="#Craftbeer.com2020APA"/>
     <prov:hadPrimarySource rdf:resource="#BJCP2015"/>
     <rdfs:isDefinedBy rdf:resource="http://rdf.ag/o/beer-ONTOLOGY_DATE"/>
     <void:inDataset rdf:resource="#datasetdefinition"/>
 </owl:Class>
 
 <owl:Class rdf:ID="BarleyWine">
     <foaf:name>Barley Wine</foaf:name>
     <rdfs:label xml:lang="en">Barley Wine</rdfs:label>
     <skos:definition xml:lang="en">Contrary to their name, barley wines are not a type of wine. Barley wine is actually a type of beer with a base of barley. Barley wines have a much higher alcohol content than typical beers.</skos:definition>
     <skos:definition xml:lang="fr">Contrairement à leur nom, les vins d'orge ne sont pas un type de vin. Le vin d'orge est en fait une bière de type pf à base d'orge. Les vins d'orge ont une teneur en alcool beaucoup plus élevée que les bières typiques.</skos:definition>
     <rdfs:isDefinedBy rdf:resource="https://rdf.ag/o/beer-ONTOLOGY_DATE"/>
     <void:inDataset rdf:resource="#datasetdefinition"/>
 </owl:Class>
 
 <owl:Class rdf:ID="FarmhouseAle">
     <rdfs:subClassOf rdf:resource="#Ale"/>
     <rdfs:subClassOf rdf:resource="#BelgianBeer"/>
     <foaf:name>Farmhouse Ale</foaf:name>
     <rdfs:label xml:lang="en">Farmhouse Ale</rdfs:label>
     <rdfs:label xml:lang="fr">Ale de Ferme</rdfs:label>
     <skos:definition xml:lang="en">Farmhouse ales are traditionally brewed during the winter with leftover crops from the harvest and are drunk by seasonal farmhands, or 'saisonniers' in French, when working on the farm throughout the following season. This classification of beer encompasses a number of styles.</skos:definition>
     <skos:definition xml:lang="fr">Les bières de ferme sont traditionnellement brassées pendant l'hiver avec les restes de récolte et sont bues par les ouvriers agricoles saisonniers, ou «saisonniers» en français, lorsqu'ils travaillent à la ferme tout au long de la saison suivante. Cette classification de la bière englobe un certain nombre de styles.</skos:definition>
     <rdfs:isDefinedBy rdf:resource="https://rdf.ag/o/beer-ONTOLOGY_DATE"/>
     <void:inDataset rdf:resource="#datasetdefinition"/>
 </owl:Class>
 
 <owl:Class rdf:ID="Saison">
     <rdfs:subClassOf rdf:resource="#FarmhouseAle"/>
     <foaf:name>Saison</foaf:name>
     <rdfs:label xml:lang="en">Saison</rdfs:label>
     <rdfs:label xml:lang="fr">Saison</rdfs:label>
     <skos:definition xml:lang="en">Saison beers are seasonal beers that are typically enjoyed during the summer until the end of harvest. There are a wide variety of saisons brewed in the fasion as choosen at the brewer's discretion. Saisons are typically fruitier and lower in alcohol content than typical beers. While saisons originated in Belgium, there is increasing popularity among American craft brewers to produce their own saisons.</skos:definition>
     <skos:definition xml:lang="fr">Les bières de saison sont des bières de saison qui sont généralement appréciées pendant l'été jusqu'à la fin de la récolte. Il existe une grande variété de saisons brassées à la mode, choisies à la discrétion du brasseur. Les saisons sont généralement plus fruitées et plus faibles en alcool que les bières typiques. Alors que les saisons sont originaires de Belgique, il y a une popularité croissante parmi les brasseurs artisanaux américains pour produire leurs propres saisons.</skos:definition>
     <prov:hadPrimarySource rdf:resource="#Oliver2012"/>
     <rdfs:isDefinedBy rdf:resource="https://rdf.ag/o/beer-ONTOLOGY_DATE"/>
     <void:inDataset rdf:resource="#datasetdefinition"/>
 </owl:Class>
 
 <owl:Class rdf:ID="BDG">
     <rdfs:subClassOf rdf:resource="#FarmhouseAle"/>
     <foaf:name>Bière de Garde</foaf:name>
     <rdfs:label xml:lang="en">Bière de Garde</rdfs:label>
     <rdfs:label xml:lang="fr">Bière de Garde</rdfs:label>
     <skos:definition xml:lang="en">Similar to saison beers, bière de garde beers are seasonal beers that are typically enjoyed during the summer until the end of harvest. They were traditionally brewed in the Nord-Pas-de-Calais region of France. Saisons are typically dry and or spicy, however, unlike its cousin, bière de gardes are typically sweeter and maltier.</skos:definition>
     <skos:definition xml:lang="fr">Semblables aux bières de saison, les bières de garde sont des bières de saison qui sont généralement appréciées pendant l'été jusqu'à la fin des vendanges. Elles étaient traditionnellement brassées dans la région Nord-Pas-de-Calais en France. Les saisons sont généralement sèches et/ou épicées, cependant, contrairement à sa cousine, la bière de garde est généralement plus douce et maltée.</skos:definition>
     <rdfs:isDefinedBy rdf:resource="https://rdf.ag/o/beer-ONTOLOGY_DATE"/>
     <void:inDataset rdf:resource="#datasetdefinition"/>
 </owl:Class>
 
 <owl:Class rdf:ID="Lager">
     <foaf:name>Lager</foaf:name>
     <rdfs:label xml:lang="en">Lager</rdfs:label>
     <skos:definition xml:lang="en">Lagers are fermented with the yeast strain Saccharomyces pastorianus, which typically ferments better in colder temperatures 7-13˚C (45-55˚F) than S. cerevisiae.
         
         Lagers are also known for having a cold-conditioning phase of the brewing process, although not all lagers go through this phase.
     
         Lagers can be pale yellow, amber or dark.</skos:definition>
     <skos:definition xml:lang="fr">Les lagers sont fermentées avec la souche de levure Saccharomyces pastorianus, qui fermente généralement mieux à des températures plus froides de 7 à 13 ° C (45 à 55 ° F) que S. cerevisiae.
         
         Les lagers sont également connues pour avoir une phase de conditionnement à froid du processus de brassage, bien que toutes les lagers ne passent pas par cette phase.
         
         Les lagers peuvent être jaune pâle, ambre ou foncé.</skos:definition>
     <prov:hadPrimarySource rdf:resource="#Carpenter2017"/>
     <rdfs:isDefinedBy rdf:resource="https://rdf.ag/o/beer-ONTOLOGY_DATE"/>
     <void:inDataset rdf:resource="#datasetdefinition"/>
 </owl:Class>
 
 <owl:Class rdf:ID="Oktoberfestbier">
     <rdfs:subClassOf rdf:resource="#Lager"/>
     <rdfs:subClassOf rdf:resource="#GermanBeer"/>
     <foaf:name xml:lang="en">Oktoberfest Beer</foaf:name>
     <foaf:name xml:lang="de">Oktoberfestbier</foaf:name>
     <foaf:name>Märzenbier</foaf:name>
     <rdfs:label xml:lang="en">Oktoberfest Beer</rdfs:label>
     <rdfs:label xml:lang="en">Märzen</rdfs:label>
     <skos:definition xml:lang="en">Märzen-style beers are light lagers that are typically brewed with Vienna, Munich and sometimes Pilsner malts and traditional German hops with low alpha acid contents such as Hallertau and Tettnanger but can substituted with Mt. Hood or Saaz. The aroma of Märzen is slightly bitter and not overly hoppy so that the Vienna and Munich malt flavor is more promenant. This beer is typically higher in alcohol content than traditional German lagers at around 5-6% abv. The aroma is comparable to Vienna lager.</skos:definition>
     <skos:definition xml:lang="fr">Les bières de style Märzen sont des lagers légères qui sont généralement brassées avec des malts de Vienne, de Munich et parfois Pilsner et du houblon allemand traditionnel à faible teneur en acide alpha comme Hallertau et Tettnanger, mais peuvent être remplacés par le mont. Hood ou Saaz. L'arôme de Märzen est légèrement amer et pas trop houblonné, de sorte que la saveur du malt de Vienne et de Munich est plus prononcée. Cette bière a généralement une teneur en alcool plus élevée que les lagers allemandes traditionnelles à environ 5-6% abv. L'arôme est comparable à le Lager de Vienne.
         
         Historiquement, ce style de bière était brassé en mars, d'où le Märzen signifiant «mars» en allemand. En raison du manque de réfrigération à l'époque, le duc bavarois Albrecht V a décrété qu'aucun brassage ne devrait avoir lieu entre le 23 avril et le 29 septembre pour réduire la détérioration de la bière. Par conséquent, les bières ont été brassées en mars et mises en bière (conservées au frais) jusqu'à l'Oktoberfest. Traditionnellement, ces bières étaient plus foncées mais sont devenues de plus en plus légères pour correspondre aux goûts modernes.</skos:definition>
     <rdfs:comment xml:lang="en">According to German Law, Oktoberfestbier is legally reserved for the six breweries who are allowed to serve their beer at the Munich Oktoberfest. Those brewers are: Augustiner, Hacker-Pschorr, Hofbräuhaus, Löwenbräu, Paulaner, and Spaten. However, German Law does not extend beyond the German borders so the märzen/oktoberfest is used as a label for a beer style elsewhere, particulary among craft brewers.</rdfs:comment>
     <rdfs:comment xml:lang="fr">According to German Law, Oktoberfestbier is legally reserved for the six breweries who are allowed to serve their beer at the Munich Oktoberfest. Those brewers are: Augustiner, Hacker-Pschorr, Hofbräuhaus, Löwenbräu, Paulaner, and Spaten. However, German Law does not extend beyond the German borders so the märzen/oktoberfest is used as a label for a beer style elsewhere, particulary among craft brewers.</rdfs:comment>
     <prov:hadPrimarySource rdf:resource="#Oliver2012"/>
     <prov:hadPrimarySource rdf:resource="#BeerHQ2021"/>
     <rdfs:isDefinedBy rdf:resource="https://rdf.ag/o/beer-ONTOLOGY_DATE"/>
     <void:inDataset rdf:resource="#datasetdefinition"/>
 </owl:Class>
 
 <owl:Class rdf:ID="TraditionalOktoberfestbier">
     <rdfs:subClassOf rdf:resource="#Lager"/>
     <rdfs:subClassOf rdf:resource="#GermanBeer"/>
     <foaf:name xml:lang="en">Traditional Oktoberfest Beer</foaf:name>
     <foaf:name>Traditional Märzenbier</foaf:name>
     <rdfs:label xml:lang="en">Traditional Oktoberfest Beer</rdfs:label>
     <rdfs:label xml:lang="en">Traditional Märzenbier</rdfs:label>
     <skos:definition xml:lang="en">Historically, this style of beer was brewed in March, hence the Märzen meaning 'March' in German. Due to the lack of refrigeration at the time, the Bavarian Duke Albrecht V decreed that no brewing should occur between April 23 and September 29th to reduce beer spoilage. Therefore the beers were brewed in March and lagered (stored cool) until Oktoberfest. Traditionally these beers were darker but have now become increasing lighter to match modern tastes.
         
         The first lager that was officially labelled 'Märzenbier' was brewed in 1841 by the Spaten Brewery of Munich and was introduced at that year's Oktoberfest. In 1872 Spaten was the first to label their märzen-style lager as Oktoberfestbier, and the recipe Spaten uses today is still largely based on the one used in 1872.</skos:definition>
     <skos:definition xml:lang="fr">Historiquement, ce style de bière était brassé en mars, d'où le Märzen signifiant «mars» en allemand. En raison du manque de réfrigération à l'époque, le duc bavarois Albrecht V a décrété qu'aucun brassage ne devrait avoir lieu entre le 23 avril et le 29 septembre pour réduire la détérioration de la bière. Par conséquent, les bières ont été brassées en mars et conservées au frais jusqu'à l'Oktoberfest. Traditionnellement, ces bières étaient plus foncées mais sont devenues de plus en plus légères pour correspondre aux goûts modernes.
     
         La première lager officiellement étiquetée «Märzenbier» a été brassée en 1841 par la brasserie Spaten de Munich et a été présentée à l'Oktoberfest de cette année-là. En 1872, Spaten fut le premier à étiqueter son lager de style märzen comme Oktoberfestbier, et la recette que Spaten utilise aujourd'hui est encore largement basée sur celle utilisée en 1872.</skos:definition>
     <rdfs:comment xml:lang="en">According to German Law, Oktoberfestbier is legally reserved for the six breweries who are allowed to serve their beer at the Munich Oktoberfest. Those brewers are: Augustiner, Hacker-Pschorr, Hofbräuhaus, Löwenbräu, Paulaner, and Spaten. However, German Law does not extend beyond the German borders so the märzen/oktoberfest is used as a label for a beer style elsewhere, particulary among craft brewers.</rdfs:comment>
     <rdfs:comment xml:lang="fr">According to German Law, Oktoberfestbier is legally reserved for the six breweries who are allowed to serve their beer at the Munich Oktoberfest. Those brewers are: Augustiner, Hacker-Pschorr, Hofbräuhaus, Löwenbräu, Paulaner, and Spaten. However, German Law does not extend beyond the German borders so the märzen/oktoberfest is used as a label for a beer style elsewhere, particulary among craft brewers.</rdfs:comment>
     <prov:hadPrimarySource rdf:resource="#Oliver2012"/>
     <prov:hadPrimarySource rdf:resource="#BeerHQ2021"/>
     <rdfs:isDefinedBy rdf:resource="https://rdf.ag/o/beer-ONTOLOGY_DATE"/>
     <void:inDataset rdf:resource="#datasetdefinition"/>
 </owl:Class>
 
 <owl:Class rdf:ID="AmericanLager">
     <rdfs:subClassOf rdf:resource="#Lager"/>
     <rdfs:subClassOf rdf:resource="#AmericanBeer"/>
     <foaf:name>American Lager</foaf:name>
     <rdfs:label xml:lang="en">American Lager</rdfs:label>
     <skos:definition xml:lang="en">American lagers came about from german immigrants bringing over their brewing style while using American ingredients. This beer is typically characterized as being light in color, low in bitterness and alcohol.</skos:definition>
     <skos:definition xml:lang="fr">Les lagers américaines sont issues d'immigrants allemands apportant leur style de brassage tout en utilisant des ingrédients américains. Cette bière est généralement caractérisée comme étant de couleur claire, faible en amertume et en alcool.</skos:definition>
     <rdfs:isDefinedBy rdf:resource="https://rdf.ag/o/beer-ONTOLOGY_DATE"/>
     <void:inDataset rdf:resource="#datasetdefinition"/>
 </owl:Class>
 
 <owl:Class rdf:ID="Schwarzbier">
     <rdfs:subClassOf rdf:resource="#DarkEuropeanLager"/>
     <rdfs:subClassOf rdf:resource="#GermanBeer"/>
     <foaf:name>Schwarzbier</foaf:name>
     <rdfs:label xml:lang="en">Schwarzbier</rdfs:label>
     <skos:definition xml:lang="en">Schwarzbier is a type of German Lager that is made from roasted malts, similar to a stout, which gives it its dark coloring. Hints of chocolate or coffee can be decerned from the roasted malts used in its brewing.</skos:definition>
     <skos:definition xml:lang="fr">La Schwarzbier est un type de Lager allemande qui est fabriquée à partir de malts torréfiés, semblable à un stout, ce qui lui donne sa coloration foncée. Des notes de chocolat ou de café peuvent être déduites des malts torréfiés utilisés dans son brassage.</skos:definition>
     <rdfs:isDefinedBy rdf:resource="https://rdf.ag/o/beer-ONTOLOGY_DATE"/>
     <void:inDataset rdf:resource="#datasetdefinition"/>
 </owl:Class>
 
 <owl:Class rdf:ID="Pilsner">
     <rdfs:subClassOf rdf:resource="#Lager"/>
     <foaf:name>Pilsner</foaf:name>
     <rdfs:label xml:lang="en">Pilsner</rdfs:label>
     <skos:definition xml:lang="en">Pilsners are a type of lager that first appeared in Pilsen, Bohemia from Josef Groll. It is a light colored beer that is characterized by being refreshing and low in alcohol.</skos:definition>
     <skos:definition xml:lang="fr">Les pilsners sont un type de lager qui est apparu pour la première fois à Pilsen, en Bohême, de Josef Groll. C'est une bière de couleur claire qui se caractérise par sa fraîcheur et sa faible teneur en alcool.</skos:definition>
     <rdfs:isDefinedBy rdf:resource="https://rdf.ag/o/beer-ONTOLOGY_DATE"/>
     <void:inDataset rdf:resource="#datasetdefinition"/>
 </owl:Class>
 
 <owl:Class rdf:ID="Pilsner_GermanStyle">
     <rdfs:subClassOf rdf:resource="#Pilsner"/>
     <rdfs:subClassOf rdf:resource="#PaleEuropeanBeer"/>
     <rdfs:subClassOf rdf:resource="#GermanBeer"/>
     <foaf:name>German Style Pilsner</foaf:name>
     <rdfs:label xml:lang="en">German Style Pilsner</rdfs:label>
     <skos:definition xml:lang="en">This style pilsner is characterized from Czech pilsners by having used German pilsner malts and often one or more of the four "noble" German hops: Hallertau, Tettnanger, Spalt and Hersbrucker.</skos:definition>
     <skos:definition xml:lang="fr">Ce style pilsner se caractérise par rapport aux pilsners tchèques en ayant utilisé des malts pilsner allemands et souvent un ou plusieurs des quatre houblons allemands 'nobles': Hallertau, Tettnanger, Spalt et Hersbrucker.</skos:definition>
     <prov:hadPrimarySource rdf:resource="#Seidl2021GermanPilsner"/>
     <rdfs:isDefinedBy rdf:resource="https://rdf.ag/o/beer-ONTOLOGY_DATE"/>
     <void:inDataset rdf:resource="#datasetdefinition"/>
 </owl:Class>
 
 <owl:Class rdf:ID="Stout">
     <rdfs:subClassOf rdf:resource="#Ale"/>
     <foaf:name>Stout</foaf:name>
     <rdfs:label xml:lang="en">Stout</rdfs:label>
     <rdfs:label xml:lang="fr">Stout</rdfs:label>
     <skos:definition xml:lang="en">Stouts are a dark type of ale that use a 'smoked' or malted barley, which give its distinctive 'coffee' or 'chocolate' flavored. Stouts are similar to porters but are usually thicker and healthier.</skos:definition>
     <skos:definition xml:lang="fr">Les stouts sont un type de bière noire qui utilise une orge «fumée» ou maltée, qui donne son arôme distinctif de «café» ou de «chocolat». Les stouts sont similaires aux porteurs mais sont généralement plus épais et plus sains.</skos:definition>
     <rdfs:isDefinedBy rdf:resource="https://rdf.ag/o/beer-ONTOLOGY_DATE"/>
     <void:inDataset rdf:resource="#datasetdefinition"/>
 </owl:Class>
 
 <owl:Class rdf:ID="ImperialStout">
     <rdfs:subClassOf rdf:resource="#Stout"/>
     <rdfs:subClassOf rdf:resource="#AmericanPorterandStout"/>
     <skos:definition xml:lang="en">A very dark beer style with a high ABV. An intense and complex flavored stout that relies on roasted malts.</skos:definition>
     <skos:definition xml:lang="fr">Un style de bière très sombre avec un ABV élevé. Une stout au goût intense et complexe qui repose sur des malts torréfiés.</skos:definition>
     <rdfs:isDefinedBy rdf:resource="http://rdf.ag/o/beer-ONTOLOGY_DATE"/>
     <void:inDataset rdf:resource="#datasetdefinition"/>
 </owl:Class>
 
 <owl:Class rdf:ID="MilkStout">
     <rdfs:subClassOf rdf:resource="#Stout"/>
     <foaf:name>Milk Stout</foaf:name>
     <rdfs:label xml:lang="en">Milk Stout</rdfs:label>
     <rdfs:label xml:lang="fr">Milk Stout</rdfs:label>
     <skos:definition xml:lang="en">Milk stouts are a type of stouts that have been sweetened by the addition of milk or milk products.</skos:definition>
     <skos:definition xml:lang="fr">Les stouts de lait sont un type de stouts qui ont été édulcorés par l'ajout de lait ou de produits laitiers.</skos:definition>
     <skos:historyNote xml:lang="en">In the United Kingdom, the Food Labelling Regulations of 1996 state that milk stouts cannot be described as containing 'milk', since the milk nutrients are destroyed or transformed in the brewing process and what is left is not 'milk'.</skos:historyNote>
     <skos:historyNote xml:lang="fr">Au Royaume-Uni, le Food Labelling Regulations de 1996 stipule que les stouts de lait ne peuvent pas être décrits comme contenant du «lait», étant donné que les éléments nutritifs du lait sont détruits ou transformés dans le processus de brassage et que ce qui reste n'est pas du «lait».</skos:historyNote>
     <rdfs:comment xml:lang="en">Any stouts that that use milk or any milk product as an ingredient is an instance of this class despite the UK Food Labelling Regulations of 1996 to ensure that consumers are aware of a possibility of lactose in their beer.</rdfs:comment>
     <rdfs:comment xml:lang="fr">Toute stout qui utilise du lait ou tout produit laitier comme ingrédient est un exemple de cette classe malgré les réglementations britanniques sur l'étiquetage des aliments de 1996 pour s'assurer que les consommateurs sont conscients d'une possibilité de lactose dans leur bière.</rdfs:comment>
     <prov:hadPrimarySource rdf:resource="#UKGovLegislation1996"/>
     <rdfs:isDefinedBy rdf:resource="https://rdf.ag/o/beer-ONTOLOGY_DATE"/>
     <void:inDataset rdf:resource="#datasetdefinition"/>
 </owl:Class>
 
 <owl:Class rdf:ID="Porter">
     <foaf:name>Porter</foaf:name>
     <rdfs:label xml:lang="en">Porter</rdfs:label>
     <rdfs:label xml:lang="fr">Porter</rdfs:label>
     <skos:definition xml:lang="en">While closely related to stouts and both dark in color, porters usually use a combination of pale and dark malts.</skos:definition>
     <skos:definition xml:lang="fr">Bien que étroitement apparentés aux stouts et de couleur sombre, les porteurs utilisent généralement une combinaison de malts pâles et foncés.</skos:definition>
     <rdfs:isDefinedBy rdf:resource="https://rdf.ag/o/beer-ONTOLOGY_DATE"/>
     <void:inDataset rdf:resource="#datasetdefinition"/>
 </owl:Class>
 
 <owl:Class rdf:ID="Mead">
     <owl:disjointWith rdf:resource="#Cider"/>
     <owl:disjointWith rdf:resource="#Beer"/>
     <owl:equivalentClass rdf:resource="#http://purl.obolibrary.org/obo/FOODON_03307306"/>
     <foaf:name>Mead</foaf:name>
     <rdfs:label xml:lang="en">Mead</rdfs:label>
     <rdfs:label xml:lang="en">Honey Wine</rdfs:label>
     <rdfs:label xml:lang="fr">Hydromel</rdfs:label>
     <rdfs:comment xml:lang="en">Mead is not technically a beer since its primary source of sugar comes from honey, but for the sake of convenience this class is in the Beer Ontology.</rdfs:comment>
     <rdfs:comment xml:lang="fr">L'hydromel n'est pas techniquement une bière puisque sa principale source de sucre provient du miel, mais pour des raisons de commodité, cette classe se trouve dans l'ontologie de la bière.</rdfs:comment>
     <skos:definition xml:lang="en">Mead is one of the oldest alcoholic beverages, produced by fermenting honey (although some other ingredients like fruit can be added in as well). The alcohol content usually ranges from 5 to 20% and the flavor profile ranges from very dry to very sweet.</skos:definition>
     <skos:definition xml:lang="fr">L'hydromel est l'une des boissons alcoolisées les plus anciennes, produite par la fermentation du miel (bien que certains autres ingrédients comme les fruits puissent également être ajoutés). La teneur en alcool varie généralement de 5 à 20% et le profil de saveur varie de très sec à très sucré.</skos:definition>
     <rdfs:isDefinedBy rdf:resource="https://rdf.ag/o/beer-ONTOLOGY_DATE"/>
     <void:inDataset rdf:resource="#datasetdefinition"/>
 </owl:Class>
 
 <owl:Class rdf:ID="Cider">
     <owl:equivalentClass rdf:resource="http://purl.obolibrary.org/obo/FOODON_03301134"/>
     <owl:disjointWith rdf:resource="#Beer"/>
     <owl:disjointWith rdf:resource="#Mead"/>
     <foaf:name>Cider</foaf:name>
     <rdfs:label xml:lang="en">Cider</rdfs:label>
     <rdfs:label xml:lang="en">Hard Cider</rdfs:label> <!-- US -->
     <rdfs:label xml:lang="fr">Cidre</rdfs:label>
     <rdfs:comment xml:lang="en">In North America, particularly the US, cider is an unfermented beverage produced from crushing apples, but can be made from other fruit.
         
         While fermented crushed fruit (cider) is not a type of beer this class is in the Beer Ontology for convenience.</rdfs:comment>
     <rdfs:comment xml:lang="fr">En Amérique du Nord, en particulier aux États-Unis, le cidre est une boisson non fermentée produite à partir du broyage de pommes, mais peut être fabriqué à partir d'autres fruits.
         
         Bien que les fruits broyés fermentés (cidre) ne soient pas un type de bière, cette classe est dans l'ontologie de la bière pour plus de commodité.</rdfs:comment>
     <skos:definition xml:lang="en">Cider is made from fermenting the juice of crushed fruit, usually apples.</skos:definition>
     <skos:definition xml:lang="fr">Le cidre est fabriqué à partir de la fermentation du jus de fruits écrasés, généralement des pommes.</skos:definition>
     <rdfs:isDefinedBy rdf:resource="https://rdf.ag/o/beer-ONTOLOGY_DATE"/>
     <void:inDataset rdf:resource="#datasetdefinition"/>
 </owl:Class>
 
 <owl:Class rdf:ID="SourBeer">
     <rdfs:subClassOf rdf:resource="#Beer"/>
     <foaf:name>Sour Beer</foaf:name>
     <rdfs:label xml:lang="en">Sour Beer</rdfs:label>
     <skos:definition xml:lang="en">Sour beers are a grouping of beers that taste sour, acidic or tart. They come about from a variety of styles and ingredients. This acidity comes from the Pediococcus Lactobacillus bacteria, which produce lactic acid as well as some small amounts of acedic acid, or vinegar.</skos:definition>
     <skos:definition xml:lang="fr">Les bières aigres sont un groupe de bières au goût aigre, acide ou acidulé. Ils proviennent d'une variété de styles et d'ingrédients. Cette acidité provient de la bactérie Pediococcus Lactobacillus, qui produit de l'acide lactique ainsi que de petites quantités d'acide acédique ou de vinaigre.</skos:definition>
     <rdfs:isDefinedBy rdf:resource="https://rdf.ag/o/beer-ONTOLOGY_DATE"/>
     <void:inDataset rdf:resource="#datasetdefinition"/>
 </owl:Class>
 
 <owl:Class rdf:ID="GermanPurityLawBeer">
     <rdfs:subClassOf rdf:resource="#Beer"/>
     <rdfs:subClassOf rdf:resource="#EuropeanBeer"/>
     <rdfs:label xml:lang="en">German Purity Law Beer</rdfs:label>
     <rdfs:label xml:lang="fr">Bière Pureté Allemande</rdfs:label>
     <rdfs:label xml:lang="de">Reinheitsgebot</rdfs:label>
     <skos:definition xml:lang="en">A beer that meets the requirements of the German Beer Purity Law of 1516 where beer was made exclusively from water, barley, hops and yeast.</skos:definition>
     <skos:definition xml:lang="fr">Une bière qui répond aux exigences de la loi allemande sur la pureté de la bière de 1516, où la bière était fabriquée exclusivement à partir d'eau, d'orge, de houblon et de levure.</skos:definition>
     <rdfs:isDefinedBy rdf:resource="http://rdf.ag/o/beer-ONTOLOGY_DATE"/>
     <void:inDataset rdf:resource="#datasetdefinition"/>
     <void:inDataset rdf:resource="Sundby2013"/>
 </owl:Class>
 
 <owl:Class rdf:ID="Kolsch">
     <rdfs:subClassOf rdf:resource="#GermanPurityLawBeer"/>
     <rdfs:subClassOf rdf:resource="#PaleBitterEuropeanBeer"/>
     <rdfs:subClassOf rdf:resource="#GermanBeer"/>
     <rdfs:label xml:lang="en">Kölsch Beer</rdfs:label>
     <rdfs:label xml:lang="de">Kölsch Bier</rdfs:label>
     <skos:definition xml:lang="en">Kölsch beer is beer that has been brewed within 50 km of the city of Cologne, Germany and brewed according to the Kölsch Konvention as defined by the Kölner Brauerei-Verband, or the Cologne Brewers Association, and it also must confer to the Reinheitsgebot requirements.</skos:definition>
     <skos:definition xml:lang="fr">La bière Kölsch est une bière brassée à moins de 50 km de la ville de Cologne, en Allemagne, et brassée selon la Kölsch Konvention telle que définie par le Kölner Brauerei-Verband, ou l'Association des brasseurs de Cologne, et elle doit également répondre aux exigences Reinheitsgebot.</skos:definition>
     <rdfs:isDefinedBy rdf:resource="http://rdf.ag/o/beer-ONTOLOGY_DATE"/>
     <void:inDataset rdf:resource="#datasetdefinition"/>
 </owl:Class>
 
 <owl:Class rdf:ID="Sake">
     <rdfs:label xml:lang="en">Sake</rdfs:label>
     <rdfs:label xml:lang="en">Rice Wine</rdfs:label>
     <rdfs:label xml:lang="fr">Saké</rdfs:label>
     <skos:definition xml:lang="en">While typically referred to as 'rice wine', the sake process is similar to brewing beer. However, the Tax and Trade Bureau (TTB) classifies Sake as a wine, rather than as a beer.
         
         Sake is a traditional Japanese alcoholic drink made from four ingredients: rice, water, yeast and koji, usually served heated and has a high abv of 18-20%.</skos:definition>
     <skos:definition xml:lang="fr">Bien qu'il soit généralement appelé 'vin de riz', le processus du saké est similaire au brassage de la bière. Cependant, le Tax and Trade Bureau (TTB) classe le saké comme un vin plutôt que comme une bière.
         
         Le saké est une boisson alcoolisée traditionnelle japonaise composée de quatre ingrédients : du riz, de l'eau, de la levure et du koji, généralement servi chauffé et a un taux d'alcoolémie élevé de 18 à 20 %.</skos:definition>
     <void:inDataset rdf:resource="FDA2014"/>
     <rdfs:isDefinedBy rdf:resource="http://rdf.ag/o/beer-ONTOLOGY_DATE"/>
     <void:inDataset rdf:resource="#datasetdefinition"/>
 </owl:Class>
 
 <owl:Class rdf:ID="GlutenFreeBeer">
     <rdfs:subClassOf rdf:resource="#Beer"/>
     <skos:definition xml:lang="en">Beer that was brewed with no gluten products, specifically using gluten-free malts.</skos:definition>
     <skos:definition xml:lang="fr">Bière brassée sans produits sans gluten, en particulier avec des malts sans gluten.</skos:definition>
     <rdfs:isDefinedBy rdf:resource="http://rdf.ag/o/beer-ONTOLOGY_DATE"/>
     <void:inDataset rdf:resource="#datasetdefinition"/>
 </owl:Class>
 
 <owl:Class rdf:ID="GlutenReducedBeer">
     <rdfs:subClassOf rdf:resource="#Beer"/>
     <skos:definition xml:lang="en">Beer that was brewed with ingredients containing gluten but had undergone another process to remove the gluten. Since there are gluten ingredients involved, there might still be traces of gluten that are lower than the FDA detectable gluten amount for labelling purposes but may still be present all the same.</skos:definition>
     <skos:definition xml:lang="fr">Bière brassée avec des ingrédients contenant du gluten mais ayant subi un autre processus pour éliminer le gluten. Étant donné qu'il y a des ingrédients de gluten impliqués, il peut toujours y avoir des traces de gluten qui sont inférieures à la quantité de gluten détectable par la FDA à des fins d'étiquetage, mais qui peuvent tout de même être présentes.</skos:definition>
     <rdfs:isDefinedBy rdf:resource="http://rdf.ag/o/beer-ONTOLOGY_DATE"/>
     <void:inDataset rdf:resource="#datasetdefinition"/>
 </owl:Class>
 
 <!-- Beer Descriptors, not exactly syles of beers rather subjective descriptors for beers -->
 <owl:Class rdf:ID="LightBeer">
     <foaf:name>Light Beer</foaf:name>
     <rdfs:label xml:lang="en">Light Beer</rdfs:label>
     <rdfs:label xml:lang="fr">Bières Léger</rdfs:label>
     <skos:definition xml:lang="en">Light beers are beers that are either light in calories or light in alcohol depending on location.</skos:definition>
     <skos:definition xml:lang="fr">Les bières légères sont des bières soit légères en calories, soit légères en alcool selon l'endroit.</skos:definition>
     <rdfs:comment xml:lang="en">In Canada, 'light' refers to a beer that has an alcoholic content from 2.6 - 4.0 % alcohol per volume. While in the US it usually refers to a beer having less calories than the original version of that beer.</rdfs:comment>
     <rdfs:comment xml:lang="fr">Au Canada, le terme «léger» fait référence à une bière dont la teneur en alcool est comprise entre 2.6 - 4.0 % d'alcool par volume. Aux États-Unis, il s'agit généralement d'une bière contenant moins de calories que la version originale de cette bière.</rdfs:comment>
     <rdfs:isDefinedBy rdf:resource="https://rdf.ag/o/beer-ONTOLOGY_DATE"/>
     <void:inDataset rdf:resource="#datasetdefinition"/>
     <prov:hadPrimarySource rdf:resource="#GovernmentofCanada2020-Product-specific-information-for-beer"/>
 </owl:Class>
 
 <owl:Class rdf:ID="BlondeBeer">
     <foaf:name>Blonde Beer</foaf:name>
     <rdfs:label xml:lang="en">Blonde Beer</rdfs:label>
     <rdfs:label xml:lang="en">Blond Beer</rdfs:label>
     <rdfs:label xml:lang="en">Golden Beer</rdfs:label>
     <rdfs:label xml:lang="en">Pale Beer</rdfs:label>
     <rdfs:label xml:lang="fr">Bières Blonde</rdfs:label>
     <skos:definition xml:lang="en">Blonde or Golden beers are mostly characterized by their light coloring, which is determined by the types of malts rather than by style. Lighter malts have less maillard reactions, which produces less complexity in the flavoring. Therefore, lighter beers are better paired with more flavorful food.</skos:definition>
     <skos:definition xml:lang="fr">Les bières Blondes ou Dorées se caractérisent principalement par leur coloration claire, qui est déterminée par les types de malts plutôt que par le style. Les malts plus légers ont moins de réactions de maillard, ce qui produit moins de complexité dans l'arôme.</skos:definition>
     <prov:hadPrimarySource rdf:resource="#Daniels2000"/>
     <prov:hadPrimarySource rdf:resource="#CAMRA2021"/>
     <rdfs:isDefinedBy rdf:resource="https://rdf.ag/o/beer-ONTOLOGY_DATE"/>
     <void:inDataset rdf:resource="#datasetdefinition"/>
 </owl:Class>
 
 <owl:Class rdf:ID="AmberBeer">
     <foaf:name>Amber Beer</foaf:name>
     <rdfs:label xml:lang="en">Amber Beer</rdfs:label>
     <rdfs:label xml:lang="en">Red Beer</rdfs:label>
     <rdfs:label xml:lang="fr">Bières Ambrées</rdfs:label>
     <rdfs:label xml:lang="fr">Bières Rouges</rdfs:label>
     <skos:definition xml:lang="en">Amber, or Red beers are mostly characterized by their coloring, which is determined by the types of malts rather than by style. Amber beers are more opaque than Blonde or Pale beers but they are not as opaque as Brown beers. Darker malts undergo more mailard reactions which gives them a more complex and intense flavor profile. Hints of carmel and/or toffee can be decerned as a result of the mailard reactions.</skos:definition>
     <skos:definition xml:lang="fr">Les bières ambrées ou rouges se caractérisent principalement par leur coloration, qui est déterminée par les types de malts plutôt que par le style. Les bières ambrées sont plus opaques que les bières blondes ou pâles mais elles ne sont pas aussi opaques que les bières brunes. Les malts plus foncés subissent plus de réactions mailard, ce qui leur confère un profil de saveur plus complexe et intense. Des notes de carmel et / ou de caramel peuvent être décernées à la suite des réactions du mailard.</skos:definition>
     <rdfs:isDefinedBy rdf:resource="https://rdf.ag/o/beer-ONTOLOGY_DATE"/>
     <void:inDataset rdf:resource="#datasetdefinition"/>
     <prov:hadPrimarySource rdf:resource="#Daniels2000"/>
 </owl:Class>

 <owl:Class rdf:ID="BrownBeer">
     <foaf:name>Brown Beer</foaf:name>
     <rdfs:label xml:lang="en">Brown Beer</rdfs:label>
     <rdfs:label xml:lang="fr">Bières Brun</rdfs:label>
     <skos:definition xml:lang="en">Brown beers are mostly characterized by their coloring, which is determined by the types of malts rather than by style. Brown beers are more opaque than Amber or Red beers but they are not as opaque as Dark beers. Darker malts undergo more mailard reactions which gives them a more complex and intense flavor profile. Hints of carmel and/or toffee can be decerned as a result of the mailard reactions.</skos:definition>
     <skos:definition xml:lang="fr">Les bières brunes se caractérisent principalement par leur coloration, qui est déterminée par les types de malts plutôt que par le style. Les bières Brunes sont plus opaques que les bières Ambrées ou Rouges mais elles ne sont pas aussi opaques que les bières Foncées. Les malts plus foncés subissent plus de réactions mailard, ce qui leur confère un profil de saveur plus complexe et intense. Des notes de carmel et / ou de caramel peuvent être décernées à la suite des réactions du mailard.</skos:definition>
     <rdfs:isDefinedBy rdf:resource="https://rdf.ag/o/beer-ONTOLOGY_DATE"/>
     <void:inDataset rdf:resource="#datasetdefinition"/>
     <prov:hadPrimarySource rdf:resource="#Daniels2000"/>
 </owl:Class>
 
 <owl:Class rdf:ID="DarkBeer">
     <foaf:name>Brown Beer</foaf:name>
     <rdfs:label xml:lang="en">Dark Beer</rdfs:label>
     <rdfs:label xml:lang="fr">Bières Foncés</rdfs:label>
     <skos:definition xml:lang="en">Dark beers are mostly characterized by their coloring, which is determined by the types of malts rather than by style. Darker malts undergo more mailard reactions which gives them a more complex and intense flavor profile. Hints of carmel and/or toffee can be decerned as a result of the mailard reactions. Dark beers are the most opaque beers, due to the more mailard reactions resulting in an intense and complex flavor profile, these beers are better drunk alone so that they don't overpower the food.</skos:definition>
     <skos:definition xml:lang="fr">Les bières brunes se caractérisent principalement par leur coloration, qui est déterminée par les types de malts plutôt que par le style. Les bières Brunes sont plus opaques que les bières Ambrées ou Rouges mais elles ne sont pas aussi opaques que les bières Foncées. Les malts plus foncés subissent plus de réactions mailard, ce qui leur confère un profil de saveur plus complexe et intense. Des notes de carmel et / ou de caramel peuvent être décernées à la suite des réactions du mailard.</skos:definition>
     <rdfs:isDefinedBy rdf:resource="https://rdf.ag/o/beer-ONTOLOGY_DATE"/>
     <void:inDataset rdf:resource="#datasetdefinition"/>
     <prov:hadPrimarySource rdf:resource="#Daniels2000"/>
 </owl:Class>
 
 <owl:Class rdf:ID="BalckBeer">
     <foaf:name>Black Beer</foaf:name>
     <rdfs:label xml:lang="en">Black Beer</rdfs:label>
     <rdfs:label xml:lang="fr">Bière Noire</rdfs:label>
     <skos:definition xml:lang="en">Beers that have a very opaque, almost black coloring and typically have more complex flavors.</skos:definition>
     <skos:definition xml:lang="fr">Bières qui ont une coloration très opaque, presque noire et qui ont généralement des saveurs plus complexes.</skos:definition>
     <rdfs:isDefinedBy rdf:resource="https://rdf.ag/o/beer-ONTOLOGY_DATE"/>
     <void:inDataset rdf:resource="#datasetdefinition"/>
 </owl:Class>
 
 <owl:Class rdf:ID="RyeBeer">
     <foaf:name>Rye Beer</foaf:name>
     <rdfs:label xml:lang="en">Rye Beer</rdfs:label>
     <rdfs:label xml:lang="fr">Bière de Seigle</rdfs:label>
     <skos:definition xml:lang="en">Beers that are brewed with rye malt or in conjunction with other malted cereals.</skos:definition>
     <skos:definition xml:lang="fr">Bières brassées avec du malt de seigle ou en association avec d'autres céréales maltées.</skos:definition>
     <rdfs:isDefinedBy rdf:resource="https://rdf.ag/o/beer-ONTOLOGY_DATE"/>
     <void:inDataset rdf:resource="#datasetdefinition"/>
 </owl:Class>
 
 <owl:Class rdf:ID="DryBeer">
     <foaf:name>Dry Beer</foaf:name>
     <rdfs:label xml:lang="en">Dry Beer</rdfs:label>
     <rdfs:label xml:lang="fr">Bières Sec</rdfs:label>
     <skos:definition xml:lang="en">Beers that are considered 'dry' has nothing to do with the water content rather the amount of excess sugar in the finished product. The lack of excess sugar increases the bitterness of these beers but also reduces the aftertaste.</skos:definition>
     <skos:definition xml:lang="fr">Les bières considérées comme «sèches» n'ont rien à voir avec la teneur en eau mais plutôt avec la quantité de sucre en excès dans le produit fini. Le manque d'excès de sucre augmente l'amertume de ces bières mais réduit également l'arrière-goût.</skos:definition>
     <rdfs:isDefinedBy rdf:resource="https://rdf.ag/o/beer-ONTOLOGY_DATE"/>
     <void:inDataset rdf:resource="#datasetdefinition"/>
 </owl:Class>
 
 <owl:Class rdf:ID="LimeBeer">
     <rdfs:subClassOf rdf:resource="#FruitBeer"/>
     <foaf:name>Lime Beer</foaf:name>
     <rdfs:label xml:lang="en">Lime Beer</rdfs:label>
     <rdfs:label xml:lang="fr">Bières de Lime</rdfs:label>
     <skos:definition xml:lang="en">Beers with lime or lime-based adjuncts that have been added at any point in the brewing process.</skos:definition>
     <skos:definition xml:lang="fr">Bières avec des adjuvants à base de chaux ou à base de chaux qui ont été ajoutés à tout moment du processus de brassage.</skos:definition>
     <rdfs:isDefinedBy rdf:resource="https://rdf.ag/o/beer-ONTOLOGY_DATE"/>
     <void:inDataset rdf:resource="#datasetdefinition"/>
 </owl:Class>
 
 <owl:Class rdf:ID="HoneyBeer">
     <owl:disjointWith rdf:resource="#Mead"/>
     <foaf:name>Honey Beer</foaf:name>
     <rdfs:label xml:lang="en">Honey Beer</rdfs:label>
     <rdfs:label xml:lang="fr">Bières de Miel</rdfs:label>
     <skos:definition xml:lang="en">Beers that use honey as an equal source of sugar as malt in the brewing process.</skos:definition>
     <skos:definition xml:lang="fr">Bières qui utilisent le miel comme source égale de sucre et de malt dans le processus de brassage.</skos:definition>
     <rdfs:isDefinedBy rdf:resource="https://rdf.ag/o/beer-ONTOLOGY_DATE"/>
     <void:inDataset rdf:resource="#datasetdefinition"/>
 </owl:Class>
 
 <owl:Class rdf:ID="Radler">
     <foaf:name>Radler</foaf:name>
     <rdfs:label xml:lang="en">Radler</rdfs:label>
     <skos:definition xml:lang="en">Radlers are a beer cocktail made by combining a beer with a fruit juice or soda.</skos:definition>
     <skos:definition xml:lang="fr">Les radlers sont un cocktail de bière fait en combinant une bière avec un jus de fruit ou un soda.</skos:definition>
     <rdfs:isDefinedBy rdf:resource="https://rdf.ag/o/beer-ONTOLOGY_DATE"/>
     <void:inDataset rdf:resource="#datasetdefinition"/>
 </owl:Class>
 
 <owl:Class rdf:ID="Shandy">
     <foaf:name>Shandy</foaf:name>
     <rdfs:label xml:lang="en">Shandy</rdfs:label>
     <rdfs:label xml:lang="fr">Panaché</rdfs:label>
     <skos:definition xml:lang="en">A shandy is a type of beer cocktail that is usually half-lemonade (or limeade) and half-beer.</skos:definition>
     <skos:definition xml:lang="fr">Un panaché est un type de cocktail à la bière qui est généralement une demi-limonade (ou limeade) et une demi-bière.</skos:definition>
     <rdfs:isDefinedBy rdf:resource="https://rdf.ag/o/beer-ONTOLOGY_DATE"/>
     <void:inDataset rdf:resource="#datasetdefinition"/>
 </owl:Class>
 
 <owl:Class rdf:ID="OrganicBeer">
     <foaf:name>Organic Beer</foaf:name>
     <rdfs:label xml:lang="en">Organic Beer</rdfs:label>
     <rdfs:label xml:lang="fr">Bière Biologique</rdfs:label>
     <skos:definition xml:lang="en">Beers that use only organic ingredients.</skos:definition>
     <skos:definition xml:lang="fr">Bières qui n'utilisent que des ingrédients biologiques.</skos:definition>
     <rdfs:isDefinedBy rdf:resource="https://rdf.ag/o/beer-ONTOLOGY_DATE"/>
     <void:inDataset rdf:resource="#datasetdefinition"/>
 </owl:Class>
 
 <owl:Class rdf:ID="WheatBeer">
     <rdfs:subClassOf rdf:resource="#Beer"/>
     <foaf:name>Wheat Beer</foaf:name>
     <rdfs:label xml:lang="en">Wheat Beer</rdfs:label>
     <rdfs:label xml:lang="fr">Bière de Blé</rdfs:label>
     <skos:definition xml:lang="en">Wheat beers are characterized by having a large percentage of malted or unmalted wheat. They originated in Germany and are usually brewed in the style of pale ales.</skos:definition>
     <skos:definition xml:lang="fr">Les bières de blé sont originaires d'Allemagne et sont généralement des ales pâles. Le style Ahe se caractérise par un pourcentage élevé de blé malté ou non.</skos:definition>
     <rdfs:isDefinedBy rdf:resource="https://rdf.ag/o/beer-ONTOLOGY_DATE"/>
     <void:inDataset rdf:resource="#datasetdefinition"/>
 </owl:Class>
 
 <owl:Class rdf:ID="HefeweizenBeer">
     <rdfs:subClassOf rdf:resource="#WheatBeer"/>
     <foaf:name>Hefeweizen Beer</foaf:name>
     <rdfs:label xml:lang="en">Hefeweizen Beer</rdfs:label>
     <skos:definition xml:lang="en">Hefeweizen (translating to 'wheat beer with yeast') is a traditional Bavarian wheat beer that uses at least 50% wheat malt and a yeast with a unique aroma.</skos:definition>
     <skos:definition xml:lang="fr">La Hefeweizen (qui se traduit par « bière de blé avec levure ») est une bière de blé traditionnelle bavaroise qui utilise au moins 50 % de malt de blé et une levure à l'arôme unique.</skos:definition>
     <rdfs:isDefinedBy rdf:resource="https://rdf.ag/o/beer-ONTOLOGY_DATE"/>
     <void:inDataset rdf:resource="#datasetdefinition"/>
 </owl:Class>
 
<!-- Liquid Container -->
<owl:ObjectProperty rdf:about="https://gs1.org/voc/packaging">
    <rdfs:label xml:lang="en">In Packaging</rdfs:label>
    <rdfs:label xml:lang="fr">Conteneur</rdfs:label>
</owl:ObjectProperty>

<owl:ObjectProperty rdf:about="https://gs1.org/voc/countryOfOrigin">
    <rdfs:label xml:lang="en">Country Of Origine</rdfs:label>
    <rdfs:label xml:lang="fr">Pays D'origine</rdfs:label>
</owl:ObjectProperty>

<owl:DatatypeProperty rdf:about="#serialNumber">
 <owl:equivalentProperty rdf:resource="https://gs1.org/voc/hasSerialNumber"/>
 <owl:equivalentProperty rdf:resource="https://schema.org/serialNumber"/>
 <rdfs:label xml:lang="en">Serial Number</rdfs:label>
 <rdfs:label xml:lang="fr">Numéros de série</rdfs:label>
 <skos:definition xml:lang="en">The serial number of a product or reusable container (such as a Keg).</skos:definition>
 <skos:definition xml:lang="fr">Le numéro de série d'un produit ou d'un conteneur réutilisable (tel qu'un Fût).</skos:definition>
 <rdfs:isDefinedBy rdf:resource="https://rdf.ag/o/beer-ONTOLOGY_DATE"/>
 <void:inDataset rdf:resource="#datasetdefinition"/>
</owl:DatatypeProperty>


<owl:Class rdf:ID="LiquidContainer">
    <rdfs:subClassOf rdf:resource="https://gs1.org/voc/PackagingDetails"/>
    <rdfs:label xml:lang="en">Liquid Container</rdfs:label>
    <rdfs:label xml:lang="fr">Conteneur de Liquide</rdfs:label>
    <skos:definition xml:lang="en">A container made for holding liquids.</skos:definition>
    <skos:definition xml:lang="fr">Un récipient conçu pour contenir des liquides.</skos:definition>
    <rdfs:isDefinedBy rdf:resource="https://rdf.ag/o/beer-ONTOLOGY_DATE"/>
    <void:inDataset rdf:resource="#datasetdefinition"/>
</owl:Class>

<owl:Class rdf:ID="MultiPack">
    <rdfs:subClassOf rdf:resource="https://gs1.org/voc/PackagingDetails"/>
    <rdfs:label xml:lang="en">Aggregate Container</rdfs:label>
    <rdfs:label xml:lang="fr">Emballage groupé</rdfs:label>
    <skos:definition xml:lang="en">A container that holds multiple units of the same product.</skos:definition>
    <skos:definition xml:lang="fr">Un emballage qui contient plusieurs unités du même produit.</skos:definition>
    <rdfs:subClassOf>
     <owl:Restriction rdf:about="#ContainerContentRestriction">
      <owl:onProperty rdf:resource="#item"/>
      <owl:cardinality rdf:datatype="http://www.w3.org/2001/XMLSchema#nonNegativeInteger">1</owl:cardinality>
     </owl:Restriction>
    </rdfs:subClassOf>               
    <owl:equivalentClass>
     <owl:Restriction rdf:about="#AggregateContainerCountRestriction">
      <owl:onProperty rdf:resource="#count"/>
      <owl:someValuesFrom>
       <owl:Datatype rdf:about="#AggregateContainerNonZeroCount">
        <owl:onDatatype rdf:resource="http://www.w3.org/2001/XMLSchema#integer"/>
        <owl:withRestrictions>
         <rdf:Description rdf:about="#AggregateContainerNonZeroCountValue">
          <xsd:minInclusive rdf:datatype="http://www.w3.org/2001/XMLSchema#integer">2</xsd:minInclusive>
         </rdf:Description>
        </owl:withRestrictions>
       </owl:Datatype>
      </owl:someValuesFrom>
     </owl:Restriction>
    </owl:equivalentClass>    
    <rdfs:isDefinedBy rdf:resource="https://rdf.ag/o/beer-ONTOLOGY_DATE"/>
    <void:inDataset rdf:resource="#datasetdefinition"/>
</owl:Class>

<owl:ObjectProperty rdf:about="#item">
     <rdfs:label xml:lang="en">Item</rdfs:label>
     <rdfs:label xml:lang="fr">Item</rdfs:label>
     <skos:definition xml:lang="en">The item aggregated in this package.</skos:definition>
     <skos:definition xml:lang="fr">L'item qui est contenue dans ce packet.</skos:definition>
     <rdfs:comment xml:lang="en">Equivalent to gs1 AI (02) CONTENT.</rdfs:comment>
     <rdfs:isDefinedBy rdf:resource="https://rdf.ag/o/beer-ONTOLOGY_DATE"/>
     <void:inDataset rdf:resource="#datasetdefinition"/>
</owl:ObjectProperty>

<owl:DatatypeProperty rdf:about="#count">
    <rdfs:label xml:lang="en">Count</rdfs:label>
    <rdfs:label xml:lang="fr">Contenue</rdfs:label>
    <skos:definition xml:lang="en">The number of items aggregated in this package.</skos:definition>
     <skos:definition xml:lang="fr">Le nombre d'item qui est contenue dans ce packet.</skos:definition>
     <rdfs:comment xml:lang="en">Equivalent to gs1 AI (37) ITEM.</rdfs:comment>
     <rdfs:isDefinedBy rdf:resource="https://rdf.ag/o/beer-ONTOLOGY_DATE"/>
     <void:inDataset rdf:resource="#datasetdefinition"/>
</owl:DatatypeProperty>

<owl:Class rdf:ID="BagNBox">
    <rdf:type rdf:resource="http://purl.obolibrary.org/obo/FOODON_03490100"/>
    <rdfs:subClassOf rdf:resource="#LiquidContainer"/>
    <rdfs:label xml:lang="en">Bag in Box</rdfs:label>
    <rdfs:label xml:lang="fr">Vin en boîte</rdfs:label>
    <skos:definition xml:lang="en">A plastic bladder with an air-tight valve within a protective cardboard box.</skos:definition>
    <skos:definition xml:lang="fr">Un sac en plastique avec une valve dans une boîte en carton.</skos:definition>
    <rdfs:isDefinedBy rdf:resource="https://rdf.ag/o/beer-ONTOLOGY_DATE"/>
    <void:inDataset rdf:resource="#datasetdefinition"/>
</owl:Class>

<rdf:Description rdf:about="#bagnbox4000">
 <rdf:type rdf:resource="https://gs1.org/voc/PackagingDetails"/>
 <rdf:type rdf:resource="#LiquidContainer"/>
 <rdf:type rdf:resource="#BagNBox"/>
 <rdfs:label xml:lang="en">4000ml Bag in Box</rdfs:label>
 <rdfs:label xml:lang="fr">Vin en boîte de 4000ml</rdfs:label>
 <skos:definition xml:lang="en">A plastic bladder containing 4000ml with an air-tight valve within a protective cardboard box.</skos:definition>
 <skos:definition xml:lang="fr">Un sac en plastique contenant 4000ml avec une valve dans une boîte en carton.</skos:definition>
 <!-- Net Content -->
 <gs1:netContent>
  <gs1:QuantitativeValue rdf:about="#bagnbox4000Content">
    <rdf:type rdf:resource="http://qudt.org/1.1/schema/qudt#QuantityValue"/>
    <qudt:unit rdf:resource="http://www.qudt.org/2.1/vocab/unit/MilliL"/>
    <qudt:numericalValue rdf:datatype="http://www.w3.org/2001/XMLSchema#double">4000</qudt:numericalValue>
    <rdf:value rdf:datatype="http://www.w3.org/2001/XMLSchema#double">4000</rdf:value>
    <gs1:unitCode>MLT</gs1:unitCode>
    <gs1:value>4000</gs1:value>
  </gs1:QuantitativeValue>
 </gs1:netContent> 
 <sosa:isFeatureOfInterestOf>
  <rdf:Description rdf:about="#bagnbox4000ContentSosa">
   <rdf:type rdf:resource="http://www.w3.org/ns/sosa/Observation"/>
   <sosa:hasFeatureOfInterest rdf:resource="#bagnbox4000"/>
   <sosa:observedProperty  rdf:resource="#netcontent"/>
   <sosa:hasResult rdf:resource="#bagnbox4000Content"/>
   <sosa:hasSimpleResult rdf:datatype="http://www.qudt.org/2.1/vocab/unit/MilliM">4000</sosa:hasSimpleResult>
  </rdf:Description>
 </sosa:isFeatureOfInterestOf>
 <rdfs:isDefinedBy rdf:resource="https://rdf.ag/o/beer-ONTOLOGY_DATE"/>
 <void:inDataset rdf:resource="#datasetdefinition"/>
</rdf:Description>

<rdf:Description rdf:about="#bagnbox3000">
 <rdf:type rdf:resource="https://gs1.org/voc/PackagingDetails"/>
 <rdf:type rdf:resource="#LiquidContainer"/>
 <rdf:type rdf:resource="#BagNBox"/>
 <rdfs:label xml:lang="en">3000ml Bag in Box</rdfs:label>
 <rdfs:label xml:lang="fr">Vin en boîte de 3000ml</rdfs:label>
 <skos:definition xml:lang="en">A plastic bladder containing 3000ml with an air-tight valve within a protective cardboard box.</skos:definition>
 <skos:definition xml:lang="fr">Un sac en plastique contenant 3000ml avec une valve dans une boîte en carton.</skos:definition>
 <!-- Net Content -->
 <gs1:netContent>
  <gs1:QuantitativeValue rdf:about="#bagnbox3000Content">
    <rdf:type rdf:resource="http://qudt.org/1.1/schema/qudt#QuantityValue"/>
    <qudt:unit rdf:resource="http://www.qudt.org/2.1/vocab/unit/MilliL"/>
    <qudt:numericalValue rdf:datatype="http://www.w3.org/2001/XMLSchema#double">3000</qudt:numericalValue>
    <rdf:value rdf:datatype="http://www.w3.org/2001/XMLSchema#double">3000</rdf:value>
    <gs1:unitCode>MLT</gs1:unitCode>
    <gs1:value>3000</gs1:value>
  </gs1:QuantitativeValue>
 </gs1:netContent> 
 <sosa:isFeatureOfInterestOf>
  <rdf:Description rdf:about="#bagnbox3000ContentSosa">
   <rdf:type rdf:resource="http://www.w3.org/ns/sosa/Observation"/>
   <sosa:hasFeatureOfInterest rdf:resource="#bagnbox3000"/>
   <sosa:observedProperty  rdf:resource="#netcontent"/>
   <sosa:hasResult rdf:resource="#bagnbox3000Content"/>
   <sosa:hasSimpleResult rdf:datatype="http://www.qudt.org/2.1/vocab/unit/MilliM">3000</sosa:hasSimpleResult>
  </rdf:Description>
 </sosa:isFeatureOfInterestOf>
 <rdfs:isDefinedBy rdf:resource="https://rdf.ag/o/beer-ONTOLOGY_DATE"/>
 <void:inDataset rdf:resource="#datasetdefinition"/>
</rdf:Description>


<owl:Class rdf:ID="TetraPack">
    <rdf:type rdf:resource="http://purl.obolibrary.org/obo/FOODON_03490100"/>
    <rdfs:subClassOf rdf:resource="#LiquidContainer"/>
    <rdfs:label xml:lang="en">Tetra Pack®</rdfs:label>
    <rdfs:label xml:lang="fr">Tetra Pack®</rdfs:label>
    <skos:definition xml:lang="en">A liquid carton based container manufactured by Tetra Pack®</skos:definition>
    <skos:definition xml:lang="fr">Un emballage en carton en pour liquides forme de tétraèdre de la firme Tetra Pack®</skos:definition>
    <rdfs:isDefinedBy rdf:resource="https://rdf.ag/o/beer-ONTOLOGY_DATE"/>
    <void:inDataset rdf:resource="#datasetdefinition"/>
</owl:Class>



<owl:Class rdf:ID="Keg">
    <rdf:type rdf:resource="http://purl.obolibrary.org/obo/FOODON_03490100"/>
    <rdfs:subClassOf rdf:resource="#LiquidContainer"/>
    <rdfs:label xml:lang="en">Keg</rdfs:label>
    <rdfs:label xml:lang="fr">Fût</rdfs:label>
    <skos:definition xml:lang="en">A small barrel used to store and serve beer.</skos:definition>
    <skos:definition xml:lang="fr">Un contenant réutilisable pour entreposer et servir la bière.</skos:definition>
    <rdfs:isDefinedBy rdf:resource="https://rdf.ag/o/beer-ONTOLOGY_DATE"/>
    <void:inDataset rdf:resource="#datasetdefinition"/>
</owl:Class>

<rdf:Description rdf:about="#miniKeg">
 <rdf:type rdf:resource="#LiquidContainer"/>
 <rdf:type rdf:resource="#Keg"/>
 <rdf:type rdf:resource="https://gs1.org/voc/PackagingDetails"/>
 <rdfs:label xml:lang="en">Mini Keg</rdfs:label>
 <rdfs:label xml:lang="fr">Mini-fût</rdfs:label>
 <skos:definition xml:lang="en">Mini Keg</skos:definition>
 <skos:definition xml:lang="fr">Mini-fût</skos:definition>
 <skos:altLabel xml:lang="en">Bubba</skos:altLabel>
 <beer:nominalCapacity rdf:datatype="http://www.qudt.org/2.1/vocab/unit/MilliL">5000</beer:nominalCapacity>
 <sosa:isFeatureOfInterestOf>
  <rdf:Description rdf:about="#miniKegContentSosaML">
   <rdf:type rdf:resource="http://www.w3.org/ns/sosa/Observation"/>
   <sosa:hasFeatureOfInterest rdf:resource="#miniKeg"/>
   <sosa:observedProperty rdf:resource="#sosaNominalCapacity"/>
   <sosa:hasResult>
    <gs1:QuantitativeValue rdf:about="#miniKegContentML">
     <rdf:type rdf:resource="http://qudt.org/1.1/schema/qudt#QuantityValue"/>
     <gs1:unitCode>MLT</gs1:unitCode>
     <gs1:value>5000</gs1:value>
     <rdf:value rdf:datatype="http://www.w3.org/2001/XMLSchema#double">5000</rdf:value>
     <qudt:unit rdf:resource="http://www.qudt.org/2.1/vocab/unit/MilliL"/>
     <qudt:numericalValue rdf:datatype="http://www.w3.org/2001/XMLSchema#double">5000</qudt:numericalValue>
     <rdfs:isDefinedBy rdf:resource="https://rdf.ag/o/beer-ONTOLOGY_DATE"/>
     <void:inDataset rdf:resource="#datasetdefinition"/>
    </gs1:QuantitativeValue>
   </sosa:hasResult> 
   <sosa:hasSimpleResult rdf:datatype="http://www.qudt.org/2.1/vocab/unit/MilliM">5000</sosa:hasSimpleResult>
   <rdfs:isDefinedBy rdf:resource="https://rdf.ag/o/beer-ONTOLOGY_DATE"/>
   <void:inDataset rdf:resource="#datasetdefinition"/>
  </rdf:Description>
 </sosa:isFeatureOfInterestOf>
 <sosa:isFeatureOfInterestOf>
  <rdf:Description rdf:about="#miniKegContentSosaOZ">
   <rdf:type rdf:resource="http://www.w3.org/ns/sosa/Observation"/>
   <sosa:hasFeatureOfInterest rdf:resource="#miniKeg"/>
   <sosa:observedProperty rdf:resource="#sosaNominalCapacity"/>
   <sosa:hasResult>
   <gs1:QuantitativeValue rdf:about="#miniKegContentOZ">
    <rdf:type rdf:resource="http://qudt.org/1.1/schema/qudt#QuantityValue"/>
    <gs1:unitCode>foz_us</gs1:unitCode>
    <gs1:value>169</gs1:value>
    <rdf:value rdf:datatype="http://www.w3.org/2001/XMLSchema#double">169</rdf:value>
    <qudt:unit rdf:resource="http://www.qudt.org/2.1/vocab/unit/OZ_VOL_US"/>
    <qudt:numericalValue rdf:datatype="http://www.w3.org/2001/XMLSchema#double">169</qudt:numericalValue>
    <rdfs:isDefinedBy rdf:resource="https://rdf.ag/o/beer-ONTOLOGY_DATE"/>
    <void:inDataset rdf:resource="#datasetdefinition"/>  
   </gs1:QuantitativeValue>
   </sosa:hasResult>
   <sosa:hasSimpleResult rdf:datatype="http://www.qudt.org/2.1/vocab/unit/OZ_VOL_US">169</sosa:hasSimpleResult>
   <rdfs:isDefinedBy rdf:resource="https://rdf.ag/o/beer-ONTOLOGY_DATE"/>
   <void:inDataset rdf:resource="#datasetdefinition"/>  
 </rdf:Description>
 </sosa:isFeatureOfInterestOf>
 <!-- Net Content Gal -->
 <sosa:isFeatureOfInterestOf>
  <rdf:Description rdf:about="#miniKegContentSosaGAL">
   <rdf:type rdf:resource="http://www.w3.org/ns/sosa/Observation"/>
   <sosa:hasFeatureOfInterest rdf:resource="#miniKeg"/>
   <sosa:observedProperty rdf:resource="#netcontent"/>
   <sosa:hasResult>
    <gs1:QuantitativeValue rdf:about="#miniKegContentGal">
     <rdf:type rdf:resource="http://qudt.org/1.1/schema/qudt#QuantityValue"/>
     <gs1:unitCode>gal_us</gs1:unitCode>
     <gs1:value>1.32</gs1:value>
     <rdf:value rdf:datatype="http://www.w3.org/2001/XMLSchema#double">1.32</rdf:value>
     <qudt:unit rdf:resource="http://www.qudt.org/2.1/vocab/unit/GAL_US"/>
     <qudt:numericalValue rdf:datatype="http://www.w3.org/2001/XMLSchema#double">1.32</qudt:numericalValue>
     <rdfs:isDefinedBy rdf:resource="https://rdf.ag/o/beer-ONTOLOGY_DATE"/>
     <void:inDataset rdf:resource="#datasetdefinition"/>  
    </gs1:QuantitativeValue>
   </sosa:hasResult>
   <sosa:hasSimpleResult rdf:datatype="http://www.qudt.org/2.1/vocab/unit/GAL_US">1.32</sosa:hasSimpleResult>
   <rdfs:isDefinedBy rdf:resource="https://rdf.ag/o/beer-ONTOLOGY_DATE"/>
   <void:inDataset rdf:resource="#datasetdefinition"/>  
 </rdf:Description>
 </sosa:isFeatureOfInterestOf>

 <!-- Height MM-->
 <gs1:inPackageHeight>
  <gs1:QuantitativeValue rdf:about="#miniKegHeightMM">
   <rdf:type rdf:resource="http://qudt.org/1.1/schema/qudt#QuantityValue"/>
   <qudt:unit rdf:resource="http://www.qudt.org/2.1/vocab/unit/MilliM"/>
   <qudt:numericalValue rdf:datatype="http://www.w3.org/2001/XMLSchema#double">251</qudt:numericalValue>
   <rdf:value rdf:datatype="http://www.w3.org/2001/XMLSchema#double">251</rdf:value>
   <gs1:unitCode>MMT</gs1:unitCode>
   <gs1:value>251</gs1:value>
   <rdfs:isDefinedBy rdf:resource="https://rdf.ag/o/beer-ONTOLOGY_DATE"/>
   <void:inDataset rdf:resource="#datasetdefinition"/>
  </gs1:QuantitativeValue>
 </gs1:inPackageHeight>  
 <sosa:isFeatureOfInterestOf>
  <rdf:Description rdf:about="#miniKegHeightSosaMM">
   <rdf:type rdf:resource="http://www.w3.org/ns/sosa/Observation"/>
   <sosa:hasFeatureOfInterest rdf:resource="#miniKeg"/>
   <sosa:observedProperty  rdf:resource="#height"/>
   <sosa:hasResult rdf:resource="#miniKegHeightMM"/>
   <sosa:hasSimpleResult rdf:datatype="http://www.qudt.org/2.1/vocab/unit/MilliM">251</sosa:hasSimpleResult>
   <rdfs:isDefinedBy rdf:resource="https://rdf.ag/o/beer-ONTOLOGY_DATE"/>
   <void:inDataset rdf:resource="#datasetdefinition"/>
  </rdf:Description>
 </sosa:isFeatureOfInterestOf>
 <!-- Height IN-->
 <gs1:inPackageHeight>
  <gs1:QuantitativeValue rdf:about="#miniKegHeightIN">
   <rdf:type rdf:resource="http://qudt.org/1.1/schema/qudt#QuantityValue"/>
   <qudt:unit rdf:resource="http://www.qudt.org/2.1/vocab/unit/IN"/>
   <qudt:numericalValue rdf:datatype="http://www.w3.org/2001/XMLSchema#double">9.875</qudt:numericalValue>
   <rdf:value rdf:datatype="http://www.w3.org/2001/XMLSchema#double">9.875</rdf:value>
   <gs1:unitCode>INH</gs1:unitCode>
   <gs1:value>9.875</gs1:value>
   <rdfs:isDefinedBy rdf:resource="https://rdf.ag/o/beer-ONTOLOGY_DATE"/>
   <void:inDataset rdf:resource="#datasetdefinition"/>
  </gs1:QuantitativeValue>
 </gs1:inPackageHeight>  
 <sosa:isFeatureOfInterestOf>
  <rdf:Description rdf:about="#miniKegHeightSosaIN">
   <rdf:type rdf:resource="http://www.w3.org/ns/sosa/Observation"/>
   <sosa:hasFeatureOfInterest rdf:resource="#miniKeg"/>
   <sosa:observedProperty  rdf:resource="#height"/>
   <sosa:hasResult rdf:resource="#miniKegHeightIN"/>
   <sosa:hasSimpleResult rdf:datatype="http://www.qudt.org/2.1/vocab/unit/IN">9.875</sosa:hasSimpleResult>
   <rdfs:isDefinedBy rdf:resource="https://rdf.ag/o/beer-ONTOLOGY_DATE"/>
   <void:inDataset rdf:resource="#datasetdefinition"/>
  </rdf:Description>
 </sosa:isFeatureOfInterestOf>
 <!-- Diameter MM --> 
 <gs1:inPackageDiameter>
  <gs1:QuantitativeValue rdf:about="#miniKegDiameterMM">
   <rdf:type rdf:resource="http://qudt.org/1.1/schema/qudt#QuantityValue"/>
   <qudt:unit rdf:resource="http://www.qudt.org/2.1/vocab/unit/MilliM"/>
   <qudt:numericalValue rdf:datatype="http://www.w3.org/2001/XMLSchema#double">171</qudt:numericalValue>
   <rdf:value rdf:datatype="http://www.w3.org/2001/XMLSchema#double">171</rdf:value>
   <gs1:unitCode>MMT</gs1:unitCode>
   <gs1:value>171</gs1:value>
   <rdfs:isDefinedBy rdf:resource="https://rdf.ag/o/beer-ONTOLOGY_DATE"/>
   <void:inDataset rdf:resource="#datasetdefinition"/>
  </gs1:QuantitativeValue>
 </gs1:inPackageDiameter>
 <sosa:isFeatureOfInterestOf>
  <rdf:Description rdf:about="#miniKegDiameterSosaMM">
   <rdf:type rdf:resource="http://www.w3.org/ns/sosa/Observation"/>
   <sosa:hasFeatureOfInterest rdf:resource="#miniKeg"/>
   <sosa:observedProperty  rdf:resource="#diameter"/>
   <sosa:hasResult rdf:resource="#miniKegDiameterMM"/>
   <sosa:hasSimpleResult rdf:datatype="http://www.qudt.org/2.1/vocab/unit/MilliM">171</sosa:hasSimpleResult>
   <rdfs:isDefinedBy rdf:resource="https://rdf.ag/o/beer-ONTOLOGY_DATE"/>
   <void:inDataset rdf:resource="#datasetdefinition"/>
  </rdf:Description>
 </sosa:isFeatureOfInterestOf>
 <!-- Diameter IN --> 
 <gs1:inPackageDiameter>
  <gs1:QuantitativeValue rdf:about="#miniKegDiameterIN">
   <rdf:type rdf:resource="http://qudt.org/1.1/schema/qudt#QuantityValue"/>
   <qudt:unit rdf:resource="http://www.qudt.org/2.1/vocab/unit/IN"/>
   <qudt:numericalValue rdf:datatype="http://www.w3.org/2001/XMLSchema#double">6.750</qudt:numericalValue>
   <rdf:value rdf:datatype="http://www.w3.org/2001/XMLSchema#double">6.750</rdf:value>
   <gs1:unitCode>INH</gs1:unitCode>
   <gs1:value>6.750</gs1:value>
   <rdfs:isDefinedBy rdf:resource="https://rdf.ag/o/beer-ONTOLOGY_DATE"/>
   <void:inDataset rdf:resource="#datasetdefinition"/>
  </gs1:QuantitativeValue>
 </gs1:inPackageDiameter>
 <sosa:isFeatureOfInterestOf>
  <rdf:Description rdf:about="#miniKegDiameterSosaIN">
   <rdf:type rdf:resource="http://www.w3.org/ns/sosa/Observation"/>
   <sosa:hasFeatureOfInterest rdf:resource="#miniKeg"/>
   <sosa:observedProperty  rdf:resource="#diameter"/>
   <sosa:hasResult rdf:resource="#miniKegDiameterIN"/>
   <sosa:hasSimpleResult rdf:datatype="http://www.qudt.org/2.1/vocab/unit/IN">6.750</sosa:hasSimpleResult>
   <rdfs:isDefinedBy rdf:resource="https://rdf.ag/o/beer-ONTOLOGY_DATE"/>
   <void:inDataset rdf:resource="#datasetdefinition"/>
  </rdf:Description>
 </sosa:isFeatureOfInterestOf>
 <!-- KG Weight -->
 <schema:weight>
  <gs1:QuantitativeValue rdf:about="#miniKegWeightKG">
   <rdf:type rdf:resource="http://qudt.org/1.1/schema/qudt#QuantityValue"/>
   <qudt:unit rdf:resource="http://www.qudt.org/2.1/vocab/unit/KiloGM"/>
   <qudt:numericalValue rdf:datatype="http://www.w3.org/2001/XMLSchema#double">0.6</qudt:numericalValue>
   <rdf:value rdf:datatype="http://www.w3.org/2001/XMLSchema#double">0.6</rdf:value>
   <gs1:unitCode>KGM</gs1:unitCode>
   <gs1:value>0.6</gs1:value>
   <rdfs:isDefinedBy rdf:resource="https://rdf.ag/o/beer-ONTOLOGY_DATE"/>
   <void:inDataset rdf:resource="#datasetdefinition"/>
  </gs1:QuantitativeValue>
 </schema:weight>
 <sosa:isFeatureOfInterestOf>
  <rdf:Description rdf:about="#miniKegWeightSosaKG">
   <rdf:type rdf:resource="http://www.w3.org/ns/sosa/Observation"/>
   <sosa:hasFeatureOfInterest rdf:resource="#miniKeg"/>
   <sosa:observedProperty  rdf:resource="#grossWeight"/>
   <sosa:hasResult rdf:resource="#miniKegWeightKG"/>
   <sosa:hasSimpleResult rdf:datatype="http://www.qudt.org/2.1/vocab/unit/KiloGM">0.6</sosa:hasSimpleResult>
   <rdfs:isDefinedBy rdf:resource="https://rdf.ag/o/beer-ONTOLOGY_DATE"/>
   <void:inDataset rdf:resource="#datasetdefinition"/>
  </rdf:Description>
 </sosa:isFeatureOfInterestOf>
 <!-- LB Weight -->
 <schema:weight>
  <gs1:QuantitativeValue rdf:about="#miniKegWeightLB">
   <rdf:type rdf:resource="http://qudt.org/1.1/schema/qudt#QuantityValue"/>
   <qudt:unit rdf:resource="http://www.qudt.org/2.1/vocab/unit/LB"/>
   <qudt:numericalValue rdf:datatype="http://www.w3.org/2001/XMLSchema#double">1.4</qudt:numericalValue>
   <rdf:value rdf:datatype="http://www.w3.org/2001/XMLSchema#double">1.4</rdf:value>
   <gs1:unitCode>lbm</gs1:unitCode>
   <gs1:value>1.4</gs1:value>
   <rdfs:isDefinedBy rdf:resource="https://rdf.ag/o/beer-ONTOLOGY_DATE"/>
   <void:inDataset rdf:resource="#datasetdefinition"/>
  </gs1:QuantitativeValue>
 </schema:weight>
 <sosa:isFeatureOfInterestOf>
  <rdf:Description rdf:about="#miniKegWeightSosaLB">
   <rdf:type rdf:resource="http://www.w3.org/ns/sosa/Observation"/>
   <sosa:hasFeatureOfInterest rdf:resource="#miniKeg"/>
   <sosa:observedProperty  rdf:resource="#grossWeight"/>
   <sosa:hasResult rdf:resource="#miniKegWeightLB"/>
   <sosa:hasSimpleResult rdf:datatype="http://www.qudt.org/2.1/vocab/unit/LB">1.4</sosa:hasSimpleResult>
   <rdfs:isDefinedBy rdf:resource="https://rdf.ag/o/beer-ONTOLOGY_DATE"/>
   <void:inDataset rdf:resource="#datasetdefinition"/>
  </rdf:Description>
 </sosa:isFeatureOfInterestOf>
 <rdfs:isDefinedBy rdf:resource="https://rdf.ag/o/beer-ONTOLOGY_DATE"/>
 <void:inDataset rdf:resource="#datasetdefinition"/>
</rdf:Description>

<rdf:Description rdf:about="#miniKegGrowler">
 <rdf:type rdf:resource="#LiquidContainer"/>
 <rdf:type rdf:resource="#Keg"/>
 <rdf:type rdf:resource="https://gs1.org/voc/PackagingDetails"/>
 <rdfs:label xml:lang="en">Mini Keg Growler</rdfs:label>
 <rdfs:label xml:lang="fr">Mini-fût Growler</rdfs:label>
 <skos:definition xml:lang="en">Mini Keg 8L Growler</skos:definition>
 <skos:definition xml:lang="fr">Mini-fût 8l Growler</skos:definition>
 <beer:nominalCapacity rdf:datatype="http://www.qudt.org/2.1/vocab/unit/MilliL">8000</beer:nominalCapacity>
 <sosa:isFeatureOfInterestOf>
  <rdf:Description rdf:about="#miniKegGrowlerContentSosaML">
   <rdf:type rdf:resource="http://www.w3.org/ns/sosa/Observation"/>
   <sosa:hasFeatureOfInterest rdf:resource="#miniKegGrowler"/>
   <sosa:observedProperty rdf:resource="#sosaNominalCapacity"/>
   <sosa:hasResult>
    <gs1:QuantitativeValue rdf:about="#miniKegGrowlerContentML">
     <rdf:type rdf:resource="http://qudt.org/1.1/schema/qudt#QuantityValue"/>
     <gs1:unitCode>MLT</gs1:unitCode>
     <gs1:value>8000</gs1:value>
     <rdf:value rdf:datatype="http://www.w3.org/2001/XMLSchema#double">8000</rdf:value>
     <qudt:unit rdf:resource="http://www.qudt.org/2.1/vocab/unit/MilliL"/>
     <qudt:numericalValue rdf:datatype="http://www.w3.org/2001/XMLSchema#double">8000</qudt:numericalValue>
     <rdfs:isDefinedBy rdf:resource="https://rdf.ag/o/beer-ONTOLOGY_DATE"/>
     <void:inDataset rdf:resource="#datasetdefinition"/>
    </gs1:QuantitativeValue>
   </sosa:hasResult> 
   <sosa:hasSimpleResult rdf:datatype="http://www.qudt.org/2.1/vocab/unit/MilliM">8000</sosa:hasSimpleResult>
   <rdfs:isDefinedBy rdf:resource="https://rdf.ag/o/beer-ONTOLOGY_DATE"/>
   <void:inDataset rdf:resource="#datasetdefinition"/>
  </rdf:Description>
 </sosa:isFeatureOfInterestOf>
 <sosa:isFeatureOfInterestOf>
  <rdf:Description rdf:about="#miniKegGrowlerContentSosaOZ">
   <rdf:type rdf:resource="http://www.w3.org/ns/sosa/Observation"/>
   <sosa:hasFeatureOfInterest rdf:resource="#miniKegGrowler"/>
   <sosa:observedProperty rdf:resource="#sosaNominalCapacity"/>
   <sosa:hasResult>
   <gs1:QuantitativeValue rdf:about="#miniKegGrowlerContentOZ">
    <rdf:type rdf:resource="http://qudt.org/1.1/schema/qudt#QuantityValue"/>
    <gs1:unitCode>foz_us</gs1:unitCode>
    <gs1:value>271</gs1:value>
    <rdf:value rdf:datatype="http://www.w3.org/2001/XMLSchema#double">271</rdf:value>
    <qudt:unit rdf:resource="http://www.qudt.org/2.1/vocab/unit/OZ_VOL_US"/>
    <qudt:numericalValue rdf:datatype="http://www.w3.org/2001/XMLSchema#double">271</qudt:numericalValue>
    <rdfs:isDefinedBy rdf:resource="https://rdf.ag/o/beer-ONTOLOGY_DATE"/>
    <void:inDataset rdf:resource="#datasetdefinition"/>  
   </gs1:QuantitativeValue>
   </sosa:hasResult>
   <sosa:hasSimpleResult rdf:datatype="http://www.qudt.org/2.1/vocab/unit/OZ_VOL_US">271</sosa:hasSimpleResult>
   <rdfs:isDefinedBy rdf:resource="https://rdf.ag/o/beer-ONTOLOGY_DATE"/>
   <void:inDataset rdf:resource="#datasetdefinition"/>  
 </rdf:Description>
 </sosa:isFeatureOfInterestOf>
 <!-- Net Content Gal -->
 <sosa:isFeatureOfInterestOf>
  <rdf:Description rdf:about="#miniKegGrowlerContentSosaGAL">
   <rdf:type rdf:resource="http://www.w3.org/ns/sosa/Observation"/>
   <sosa:hasFeatureOfInterest rdf:resource="#miniKegGrowler"/>
   <sosa:observedProperty rdf:resource="#netcontent"/>
   <sosa:hasResult>
    <gs1:QuantitativeValue rdf:about="#miniKegGrowlerContentGal">
     <rdf:type rdf:resource="http://qudt.org/1.1/schema/qudt#QuantityValue"/>
     <gs1:unitCode>gal_us</gs1:unitCode>
     <gs1:value>2.11</gs1:value>
     <rdf:value rdf:datatype="http://www.w3.org/2001/XMLSchema#double">2.11</rdf:value>
     <qudt:unit rdf:resource="http://www.qudt.org/2.1/vocab/unit/GAL_US"/>
     <qudt:numericalValue rdf:datatype="http://www.w3.org/2001/XMLSchema#double">2.11</qudt:numericalValue>
     <rdfs:isDefinedBy rdf:resource="https://rdf.ag/o/beer-ONTOLOGY_DATE"/>
     <void:inDataset rdf:resource="#datasetdefinition"/>  
    </gs1:QuantitativeValue>
   </sosa:hasResult>
   <sosa:hasSimpleResult rdf:datatype="http://www.qudt.org/2.1/vocab/unit/GAL_US">2.11</sosa:hasSimpleResult>
   <rdfs:isDefinedBy rdf:resource="https://rdf.ag/o/beer-ONTOLOGY_DATE"/>
   <void:inDataset rdf:resource="#datasetdefinition"/>  
 </rdf:Description>
 </sosa:isFeatureOfInterestOf>

 <!-- Height MM-->
 <gs1:inPackageHeight>
  <gs1:QuantitativeValue rdf:about="#miniKegGrowlerHeightMM">
   <rdf:type rdf:resource="http://qudt.org/1.1/schema/qudt#QuantityValue"/>
   <qudt:unit rdf:resource="http://www.qudt.org/2.1/vocab/unit/MilliM"/>
   <qudt:numericalValue rdf:datatype="http://www.w3.org/2001/XMLSchema#double">400.05</qudt:numericalValue>
   <rdf:value rdf:datatype="http://www.w3.org/2001/XMLSchema#double">400.05</rdf:value>
   <gs1:unitCode>MMT</gs1:unitCode>
   <gs1:value>400.05</gs1:value>
   <rdfs:isDefinedBy rdf:resource="https://rdf.ag/o/beer-ONTOLOGY_DATE"/>
   <void:inDataset rdf:resource="#datasetdefinition"/>
  </gs1:QuantitativeValue>
 </gs1:inPackageHeight>  
 <sosa:isFeatureOfInterestOf>
  <rdf:Description rdf:about="#miniKegGrowlerHeightSosaMM">
   <rdf:type rdf:resource="http://www.w3.org/ns/sosa/Observation"/>
   <sosa:hasFeatureOfInterest rdf:resource="#miniKegGrowler"/>
   <sosa:observedProperty  rdf:resource="#height"/>
   <sosa:hasResult rdf:resource="#miniKegGrowlerHeightMM"/>
   <sosa:hasSimpleResult rdf:datatype="http://www.qudt.org/2.1/vocab/unit/MilliM">400.05</sosa:hasSimpleResult>
   <rdfs:isDefinedBy rdf:resource="https://rdf.ag/o/beer-ONTOLOGY_DATE"/>
   <void:inDataset rdf:resource="#datasetdefinition"/>
  </rdf:Description>
 </sosa:isFeatureOfInterestOf>
 <!-- Height IN-->
 <gs1:inPackageHeight>
  <gs1:QuantitativeValue rdf:about="#miniKegGrowlerHeightIN">
   <rdf:type rdf:resource="http://qudt.org/1.1/schema/qudt#QuantityValue"/>
   <qudt:unit rdf:resource="http://www.qudt.org/2.1/vocab/unit/IN"/>
   <qudt:numericalValue rdf:datatype="http://www.w3.org/2001/XMLSchema#double">15.75</qudt:numericalValue>
   <rdf:value rdf:datatype="http://www.w3.org/2001/XMLSchema#double">15.75</rdf:value>
   <gs1:unitCode>INH</gs1:unitCode>
   <gs1:value>15.75</gs1:value>
   <rdfs:isDefinedBy rdf:resource="https://rdf.ag/o/beer-ONTOLOGY_DATE"/>
   <void:inDataset rdf:resource="#datasetdefinition"/>
  </gs1:QuantitativeValue>
 </gs1:inPackageHeight>  
 <sosa:isFeatureOfInterestOf>
  <rdf:Description rdf:about="#miniKegGrowlerHeightSosaIN">
   <rdf:type rdf:resource="http://www.w3.org/ns/sosa/Observation"/>
   <sosa:hasFeatureOfInterest rdf:resource="#miniKegGrowler"/>
   <sosa:observedProperty  rdf:resource="#height"/>
   <sosa:hasResult rdf:resource="#miniKegGrowlerHeightIN"/>
   <sosa:hasSimpleResult rdf:datatype="http://www.qudt.org/2.1/vocab/unit/IN">15.75</sosa:hasSimpleResult>
   <rdfs:isDefinedBy rdf:resource="https://rdf.ag/o/beer-ONTOLOGY_DATE"/>
   <void:inDataset rdf:resource="#datasetdefinition"/>
  </rdf:Description>
 </sosa:isFeatureOfInterestOf>
 <!-- Diameter MM --> 
 <gs1:inPackageDiameter>
  <gs1:QuantitativeValue rdf:about="#miniKegGrowlerDiameterMM">
   <rdf:type rdf:resource="http://qudt.org/1.1/schema/qudt#QuantityValue"/>
   <qudt:unit rdf:resource="http://www.qudt.org/2.1/vocab/unit/MilliM"/>
   <qudt:numericalValue rdf:datatype="http://www.w3.org/2001/XMLSchema#double">171.45</qudt:numericalValue>
   <rdf:value rdf:datatype="http://www.w3.org/2001/XMLSchema#double">171.45</rdf:value>
   <gs1:unitCode>MMT</gs1:unitCode>
   <gs1:value>171.45</gs1:value>
   <rdfs:isDefinedBy rdf:resource="https://rdf.ag/o/beer-ONTOLOGY_DATE"/>
   <void:inDataset rdf:resource="#datasetdefinition"/>
  </gs1:QuantitativeValue>
 </gs1:inPackageDiameter>
 <sosa:isFeatureOfInterestOf>
  <rdf:Description rdf:about="#miniKegGrowlerDiameterSosaMM">
   <rdf:type rdf:resource="http://www.w3.org/ns/sosa/Observation"/>
   <sosa:hasFeatureOfInterest rdf:resource="#miniKegGrowler"/>
   <sosa:observedProperty  rdf:resource="#diameter"/>
   <sosa:hasResult rdf:resource="#miniKegGrowlerDiameterMM"/>
   <sosa:hasSimpleResult rdf:datatype="http://www.qudt.org/2.1/vocab/unit/MilliM">171.45</sosa:hasSimpleResult>
   <rdfs:isDefinedBy rdf:resource="https://rdf.ag/o/beer-ONTOLOGY_DATE"/>
   <void:inDataset rdf:resource="#datasetdefinition"/>
  </rdf:Description>
 </sosa:isFeatureOfInterestOf>
 <!-- Diameter IN --> 
 <gs1:inPackageDiameter>
  <gs1:QuantitativeValue rdf:about="#miniKegGrowlerDiameterIN">
   <rdf:type rdf:resource="http://qudt.org/1.1/schema/qudt#QuantityValue"/>
   <qudt:unit rdf:resource="http://www.qudt.org/2.1/vocab/unit/IN"/>
   <qudt:numericalValue rdf:datatype="http://www.w3.org/2001/XMLSchema#double">6.75</qudt:numericalValue>
   <rdf:value rdf:datatype="http://www.w3.org/2001/XMLSchema#double">6.75</rdf:value>
   <gs1:unitCode>INH</gs1:unitCode>
   <gs1:value>6.75</gs1:value>
   <rdfs:isDefinedBy rdf:resource="https://rdf.ag/o/beer-ONTOLOGY_DATE"/>
   <void:inDataset rdf:resource="#datasetdefinition"/>
  </gs1:QuantitativeValue>
 </gs1:inPackageDiameter>
 <sosa:isFeatureOfInterestOf>
  <rdf:Description rdf:about="#miniKegGrowlerDiameterSosaIN">
   <rdf:type rdf:resource="http://www.w3.org/ns/sosa/Observation"/>
   <sosa:hasFeatureOfInterest rdf:resource="#miniKegGrowler"/>
   <sosa:observedProperty  rdf:resource="#diameter"/>
   <sosa:hasResult rdf:resource="#miniKegGrowlerDiameterIN"/>
   <sosa:hasSimpleResult rdf:datatype="http://www.qudt.org/2.1/vocab/unit/IN">6.75</sosa:hasSimpleResult>
   <rdfs:isDefinedBy rdf:resource="https://rdf.ag/o/beer-ONTOLOGY_DATE"/>
   <void:inDataset rdf:resource="#datasetdefinition"/>
  </rdf:Description>
 </sosa:isFeatureOfInterestOf>
 <!-- KG Weight -->
 <schema:weight>
  <gs1:QuantitativeValue rdf:about="#miniKegGrowlerWeightKG">
   <rdf:type rdf:resource="http://qudt.org/1.1/schema/qudt#QuantityValue"/>
   <qudt:unit rdf:resource="http://www.qudt.org/2.1/vocab/unit/KiloGM"/>
   <qudt:numericalValue rdf:datatype="http://www.w3.org/2001/XMLSchema#double">0.7</qudt:numericalValue>
   <rdf:value rdf:datatype="http://www.w3.org/2001/XMLSchema#double">0.7</rdf:value>
   <gs1:unitCode>KGM</gs1:unitCode>
   <gs1:value>0.7</gs1:value>
   <rdfs:isDefinedBy rdf:resource="https://rdf.ag/o/beer-ONTOLOGY_DATE"/>
   <void:inDataset rdf:resource="#datasetdefinition"/>
  </gs1:QuantitativeValue>
 </schema:weight>
 <sosa:isFeatureOfInterestOf>
  <rdf:Description rdf:about="#miniKegGrowlerWeightSosaKG">
   <rdf:type rdf:resource="http://www.w3.org/ns/sosa/Observation"/>
   <sosa:hasFeatureOfInterest rdf:resource="#miniKegGrowler"/>
   <sosa:observedProperty  rdf:resource="#grossWeight"/>
   <sosa:hasResult rdf:resource="#miniKegGrowlerWeightKG"/>
   <sosa:hasSimpleResult rdf:datatype="http://www.qudt.org/2.1/vocab/unit/KiloGM">0.7</sosa:hasSimpleResult>
   <rdfs:isDefinedBy rdf:resource="https://rdf.ag/o/beer-ONTOLOGY_DATE"/>
   <void:inDataset rdf:resource="#datasetdefinition"/>
  </rdf:Description>
 </sosa:isFeatureOfInterestOf>
 <!-- LB Weight -->
 <schema:weight>
  <gs1:QuantitativeValue rdf:about="#miniKegGrowlerWeightLB">
   <rdf:type rdf:resource="http://qudt.org/1.1/schema/qudt#QuantityValue"/>
   <qudt:unit rdf:resource="http://www.qudt.org/2.1/vocab/unit/LB"/>
   <qudt:numericalValue rdf:datatype="http://www.w3.org/2001/XMLSchema#double">1.5</qudt:numericalValue>
   <rdf:value rdf:datatype="http://www.w3.org/2001/XMLSchema#double">1.5</rdf:value>
   <gs1:unitCode>lbm</gs1:unitCode>
   <gs1:value>1.5</gs1:value>
   <rdfs:isDefinedBy rdf:resource="https://rdf.ag/o/beer-ONTOLOGY_DATE"/>
   <void:inDataset rdf:resource="#datasetdefinition"/>
  </gs1:QuantitativeValue>
 </schema:weight>
 <sosa:isFeatureOfInterestOf>
  <rdf:Description rdf:about="#miniKegGrowlerWeightSosaLB">
   <rdf:type rdf:resource="http://www.w3.org/ns/sosa/Observation"/>
   <sosa:hasFeatureOfInterest rdf:resource="#miniKegGrowler"/>
   <sosa:observedProperty  rdf:resource="#grossWeight"/>
   <sosa:hasResult rdf:resource="#miniKegGrowlerWeightLB"/>
   <sosa:hasSimpleResult rdf:datatype="http://www.qudt.org/2.1/vocab/unit/LB">1.5</sosa:hasSimpleResult>
   <rdfs:isDefinedBy rdf:resource="https://rdf.ag/o/beer-ONTOLOGY_DATE"/>
   <void:inDataset rdf:resource="#datasetdefinition"/>
  </rdf:Description>
 </sosa:isFeatureOfInterestOf>
 <rdfs:isDefinedBy rdf:resource="https://rdf.ag/o/beer-ONTOLOGY_DATE"/>
 <void:inDataset rdf:resource="#datasetdefinition"/>
</rdf:Description>


<rdf:Description rdf:about="#corneliusKeg">
 <rdf:type rdf:resource="#LiquidContainer"/>
 <rdf:type rdf:resource="#Keg"/>
 <rdf:type rdf:resource="https://gs1.org/voc/PackagingDetails"/>
 <rdfs:label xml:lang="en">Cornelius Keg</rdfs:label>
 <rdfs:label xml:lang="fr">Fût Cornelius</rdfs:label>
 <skos:definition xml:lang="en">Cornelius Keg</skos:definition>
 <skos:definition xml:lang="fr">Fût Cornelius</skos:definition>
 <skos:altLabel xml:lang="en">Soda Keg</skos:altLabel>
 <beer:nominalCapacity rdf:datatype="http://www.qudt.org/2.1/vocab/unit/MilliL">18930</beer:nominalCapacity>
 <sosa:isFeatureOfInterestOf>
  <rdf:Description rdf:about="#corneliusKegContentSosaML">
   <rdf:type rdf:resource="http://www.w3.org/ns/sosa/Observation"/>
   <sosa:hasFeatureOfInterest rdf:resource="#corneliusKeg"/>
   <sosa:observedProperty rdf:resource="#sosaNominalCapacity"/>
   <sosa:hasResult>
    <gs1:QuantitativeValue rdf:about="#corneliusKegContentML">
     <rdf:type rdf:resource="http://qudt.org/1.1/schema/qudt#QuantityValue"/>
     <gs1:unitCode>MLT</gs1:unitCode>
     <gs1:value>18930</gs1:value>
     <rdf:value rdf:datatype="http://www.w3.org/2001/XMLSchema#double">18930</rdf:value>
     <qudt:unit rdf:resource="http://www.qudt.org/2.1/vocab/unit/MilliL"/>
     <qudt:numericalValue rdf:datatype="http://www.w3.org/2001/XMLSchema#double">18930</qudt:numericalValue>
     <rdfs:isDefinedBy rdf:resource="https://rdf.ag/o/beer-ONTOLOGY_DATE"/>
     <void:inDataset rdf:resource="#datasetdefinition"/>
    </gs1:QuantitativeValue>
   </sosa:hasResult> 
   <sosa:hasSimpleResult rdf:datatype="http://www.qudt.org/2.1/vocab/unit/MilliM">18930</sosa:hasSimpleResult>
   <rdfs:isDefinedBy rdf:resource="https://rdf.ag/o/beer-ONTOLOGY_DATE"/>
   <void:inDataset rdf:resource="#datasetdefinition"/>
  </rdf:Description>
 </sosa:isFeatureOfInterestOf>
 <sosa:isFeatureOfInterestOf>
  <rdf:Description rdf:about="#corneliusKegContentSosaOZ">
   <rdf:type rdf:resource="http://www.w3.org/ns/sosa/Observation"/>
   <sosa:hasFeatureOfInterest rdf:resource="#corneliusKeg"/>
   <sosa:observedProperty rdf:resource="#sosaNominalCapacity"/>
   <sosa:hasResult>
   <gs1:QuantitativeValue rdf:about="#corneliusKegContentOZ">
    <rdf:type rdf:resource="http://qudt.org/1.1/schema/qudt#QuantityValue"/>
    <gs1:unitCode>foz_us</gs1:unitCode>
    <gs1:value>640</gs1:value>
    <rdf:value rdf:datatype="http://www.w3.org/2001/XMLSchema#double">640</rdf:value>
    <qudt:unit rdf:resource="http://www.qudt.org/2.1/vocab/unit/OZ_VOL_US"/>
    <qudt:numericalValue rdf:datatype="http://www.w3.org/2001/XMLSchema#double">640</qudt:numericalValue>
    <rdfs:isDefinedBy rdf:resource="https://rdf.ag/o/beer-ONTOLOGY_DATE"/>
    <void:inDataset rdf:resource="#datasetdefinition"/>  
   </gs1:QuantitativeValue>
   </sosa:hasResult>
   <sosa:hasSimpleResult rdf:datatype="http://www.qudt.org/2.1/vocab/unit/OZ_VOL_US">640</sosa:hasSimpleResult>
   <rdfs:isDefinedBy rdf:resource="https://rdf.ag/o/beer-ONTOLOGY_DATE"/>
   <void:inDataset rdf:resource="#datasetdefinition"/>  
 </rdf:Description>
 </sosa:isFeatureOfInterestOf>
 <!-- Net Content Gal -->
 <sosa:isFeatureOfInterestOf>
  <rdf:Description rdf:about="#corneliusKegContentSosaGAL">
   <rdf:type rdf:resource="http://www.w3.org/ns/sosa/Observation"/>
   <sosa:hasFeatureOfInterest rdf:resource="#corneliusKeg"/>
   <sosa:observedProperty rdf:resource="#netcontent"/>
   <sosa:hasResult>
    <gs1:QuantitativeValue rdf:about="#corneliusKegContentGal">
     <rdf:type rdf:resource="http://qudt.org/1.1/schema/qudt#QuantityValue"/>
     <gs1:unitCode>gal_us</gs1:unitCode>
     <gs1:value>5.23</gs1:value>
     <rdf:value rdf:datatype="http://www.w3.org/2001/XMLSchema#double">5.23</rdf:value>
     <qudt:unit rdf:resource="http://www.qudt.org/2.1/vocab/unit/GAL_US"/>
     <qudt:numericalValue rdf:datatype="http://www.w3.org/2001/XMLSchema#double">5.23</qudt:numericalValue>
     <rdfs:isDefinedBy rdf:resource="https://rdf.ag/o/beer-ONTOLOGY_DATE"/>
     <void:inDataset rdf:resource="#datasetdefinition"/>  
    </gs1:QuantitativeValue>
   </sosa:hasResult>
   <sosa:hasSimpleResult rdf:datatype="http://www.qudt.org/2.1/vocab/unit/GAL_US">5.23</sosa:hasSimpleResult>
   <rdfs:isDefinedBy rdf:resource="https://rdf.ag/o/beer-ONTOLOGY_DATE"/>
   <void:inDataset rdf:resource="#datasetdefinition"/>  
 </rdf:Description>
 </sosa:isFeatureOfInterestOf>

 <!-- Height MM-->
 <gs1:inPackageHeight>
  <gs1:QuantitativeValue rdf:about="#corneliusKegHeightMM">
   <rdf:type rdf:resource="http://qudt.org/1.1/schema/qudt#QuantityValue"/>
   <qudt:unit rdf:resource="http://www.qudt.org/2.1/vocab/unit/MilliM"/>
   <qudt:numericalValue rdf:datatype="http://www.w3.org/2001/XMLSchema#double">584</qudt:numericalValue>
   <rdf:value rdf:datatype="http://www.w3.org/2001/XMLSchema#double">584</rdf:value>
   <gs1:unitCode>MMT</gs1:unitCode>
   <gs1:value>584</gs1:value>
   <rdfs:isDefinedBy rdf:resource="https://rdf.ag/o/beer-ONTOLOGY_DATE"/>
   <void:inDataset rdf:resource="#datasetdefinition"/>
  </gs1:QuantitativeValue>
 </gs1:inPackageHeight>  
 <sosa:isFeatureOfInterestOf>
  <rdf:Description rdf:about="#corneliusKegHeightSosaMM">
   <rdf:type rdf:resource="http://www.w3.org/ns/sosa/Observation"/>
   <sosa:hasFeatureOfInterest rdf:resource="#corneliusKeg"/>
   <sosa:observedProperty  rdf:resource="#height"/>
   <sosa:hasResult rdf:resource="#corneliusKegHeightMM"/>
   <sosa:hasSimpleResult rdf:datatype="http://www.qudt.org/2.1/vocab/unit/MilliM">584</sosa:hasSimpleResult>
   <rdfs:isDefinedBy rdf:resource="https://rdf.ag/o/beer-ONTOLOGY_DATE"/>
   <void:inDataset rdf:resource="#datasetdefinition"/>
  </rdf:Description>
 </sosa:isFeatureOfInterestOf>
 <!-- Height IN-->
 <gs1:inPackageHeight>
  <gs1:QuantitativeValue rdf:about="#corneliusKegHeightIN">
   <rdf:type rdf:resource="http://qudt.org/1.1/schema/qudt#QuantityValue"/>
   <qudt:unit rdf:resource="http://www.qudt.org/2.1/vocab/unit/IN"/>
   <qudt:numericalValue rdf:datatype="http://www.w3.org/2001/XMLSchema#double">23.000</qudt:numericalValue>
   <rdf:value rdf:datatype="http://www.w3.org/2001/XMLSchema#double">23.000</rdf:value>
   <gs1:unitCode>INH</gs1:unitCode>
   <gs1:value>23.000</gs1:value>
   <rdfs:isDefinedBy rdf:resource="https://rdf.ag/o/beer-ONTOLOGY_DATE"/>
   <void:inDataset rdf:resource="#datasetdefinition"/>
  </gs1:QuantitativeValue>
 </gs1:inPackageHeight>  
 <sosa:isFeatureOfInterestOf>
  <rdf:Description rdf:about="#corneliusKegHeightSosaIN">
   <rdf:type rdf:resource="http://www.w3.org/ns/sosa/Observation"/>
   <sosa:hasFeatureOfInterest rdf:resource="#corneliusKeg"/>
   <sosa:observedProperty  rdf:resource="#height"/>
   <sosa:hasResult rdf:resource="#corneliusKegHeightIN"/>
   <sosa:hasSimpleResult rdf:datatype="http://www.qudt.org/2.1/vocab/unit/IN">23.000</sosa:hasSimpleResult>
   <rdfs:isDefinedBy rdf:resource="https://rdf.ag/o/beer-ONTOLOGY_DATE"/>
   <void:inDataset rdf:resource="#datasetdefinition"/>
  </rdf:Description>
 </sosa:isFeatureOfInterestOf>
 <!-- Diameter MM --> 
 <gs1:inPackageDiameter>
  <gs1:QuantitativeValue rdf:about="#corneliusKegDiameterMM">
   <rdf:type rdf:resource="http://qudt.org/1.1/schema/qudt#QuantityValue"/>
   <qudt:unit rdf:resource="http://www.qudt.org/2.1/vocab/unit/MilliM"/>
   <qudt:numericalValue rdf:datatype="http://www.w3.org/2001/XMLSchema#double">229</qudt:numericalValue>
   <rdf:value rdf:datatype="http://www.w3.org/2001/XMLSchema#double">229</rdf:value>
   <gs1:unitCode>MMT</gs1:unitCode>
   <gs1:value>229</gs1:value>
   <rdfs:isDefinedBy rdf:resource="https://rdf.ag/o/beer-ONTOLOGY_DATE"/>
   <void:inDataset rdf:resource="#datasetdefinition"/>
  </gs1:QuantitativeValue>
 </gs1:inPackageDiameter>
 <sosa:isFeatureOfInterestOf>
  <rdf:Description rdf:about="#corneliusKegDiameterSosaMM">
   <rdf:type rdf:resource="http://www.w3.org/ns/sosa/Observation"/>
   <sosa:hasFeatureOfInterest rdf:resource="#corneliusKeg"/>
   <sosa:observedProperty  rdf:resource="#diameter"/>
   <sosa:hasResult rdf:resource="#corneliusKegDiameterMM"/>
   <sosa:hasSimpleResult rdf:datatype="http://www.qudt.org/2.1/vocab/unit/MilliM">229</sosa:hasSimpleResult>
   <rdfs:isDefinedBy rdf:resource="https://rdf.ag/o/beer-ONTOLOGY_DATE"/>
   <void:inDataset rdf:resource="#datasetdefinition"/>
  </rdf:Description>
 </sosa:isFeatureOfInterestOf>
 <!-- Diameter IN --> 
 <gs1:inPackageDiameter>
  <gs1:QuantitativeValue rdf:about="#corneliusKegDiameterIN">
   <rdf:type rdf:resource="http://qudt.org/1.1/schema/qudt#QuantityValue"/>
   <qudt:unit rdf:resource="http://www.qudt.org/2.1/vocab/unit/IN"/>
   <qudt:numericalValue rdf:datatype="http://www.w3.org/2001/XMLSchema#double">9.000</qudt:numericalValue>
   <rdf:value rdf:datatype="http://www.w3.org/2001/XMLSchema#double">9.000</rdf:value>
   <gs1:unitCode>INH</gs1:unitCode>
   <gs1:value>9.000</gs1:value>
   <rdfs:isDefinedBy rdf:resource="https://rdf.ag/o/beer-ONTOLOGY_DATE"/>
   <void:inDataset rdf:resource="#datasetdefinition"/>
  </gs1:QuantitativeValue>
 </gs1:inPackageDiameter>
 <sosa:isFeatureOfInterestOf>
  <rdf:Description rdf:about="#corneliusKegDiameterSosaIN">
   <rdf:type rdf:resource="http://www.w3.org/ns/sosa/Observation"/>
   <sosa:hasFeatureOfInterest rdf:resource="#corneliusKeg"/>
   <sosa:observedProperty  rdf:resource="#diameter"/>
   <sosa:hasResult rdf:resource="#corneliusKegDiameterIN"/>
   <sosa:hasSimpleResult rdf:datatype="http://www.qudt.org/2.1/vocab/unit/IN">9.000</sosa:hasSimpleResult>
   <rdfs:isDefinedBy rdf:resource="https://rdf.ag/o/beer-ONTOLOGY_DATE"/>
   <void:inDataset rdf:resource="#datasetdefinition"/>
  </rdf:Description>
 </sosa:isFeatureOfInterestOf>
 <!-- KG Weight -->
 <schema:weight>
  <gs1:QuantitativeValue rdf:about="#corneliusKegWeightKG">
   <rdf:type rdf:resource="http://qudt.org/1.1/schema/qudt#QuantityValue"/>
   <qudt:unit rdf:resource="http://www.qudt.org/2.1/vocab/unit/KiloGM"/>
   <qudt:numericalValue rdf:datatype="http://www.w3.org/2001/XMLSchema#double">4.1</qudt:numericalValue>
   <rdf:value rdf:datatype="http://www.w3.org/2001/XMLSchema#double">4.1</rdf:value>
   <gs1:unitCode>KGM</gs1:unitCode>
   <gs1:value>4.1</gs1:value>
   <rdfs:isDefinedBy rdf:resource="https://rdf.ag/o/beer-ONTOLOGY_DATE"/>
   <void:inDataset rdf:resource="#datasetdefinition"/>
  </gs1:QuantitativeValue>
 </schema:weight>
 <sosa:isFeatureOfInterestOf>
  <rdf:Description rdf:about="#corneliusKegWeightSosaKG">
   <rdf:type rdf:resource="http://www.w3.org/ns/sosa/Observation"/>
   <sosa:hasFeatureOfInterest rdf:resource="#corneliusKeg"/>
   <sosa:observedProperty  rdf:resource="#grossWeight"/>
   <sosa:hasResult rdf:resource="#corneliusKegWeightKG"/>
   <sosa:hasSimpleResult rdf:datatype="http://www.qudt.org/2.1/vocab/unit/KiloGM">4.1</sosa:hasSimpleResult>
   <rdfs:isDefinedBy rdf:resource="https://rdf.ag/o/beer-ONTOLOGY_DATE"/>
   <void:inDataset rdf:resource="#datasetdefinition"/>
  </rdf:Description>
 </sosa:isFeatureOfInterestOf>
 <!-- LB Weight -->
 <schema:weight>
  <gs1:QuantitativeValue rdf:about="#corneliusKegWeightLB">
   <rdf:type rdf:resource="http://qudt.org/1.1/schema/qudt#QuantityValue"/>
   <qudt:unit rdf:resource="http://www.qudt.org/2.1/vocab/unit/LB"/>
   <qudt:numericalValue rdf:datatype="http://www.w3.org/2001/XMLSchema#double">9.0</qudt:numericalValue>
   <rdf:value rdf:datatype="http://www.w3.org/2001/XMLSchema#double">9.0</rdf:value>
   <gs1:unitCode>lbm</gs1:unitCode>
   <gs1:value>9.0</gs1:value>
   <rdfs:isDefinedBy rdf:resource="https://rdf.ag/o/beer-ONTOLOGY_DATE"/>
   <void:inDataset rdf:resource="#datasetdefinition"/>
  </gs1:QuantitativeValue>
 </schema:weight>
 <sosa:isFeatureOfInterestOf>
  <rdf:Description rdf:about="#corneliusKegWeightSosaLB">
   <rdf:type rdf:resource="http://www.w3.org/ns/sosa/Observation"/>
   <sosa:hasFeatureOfInterest rdf:resource="#corneliusKeg"/>
   <sosa:observedProperty  rdf:resource="#grossWeight"/>
   <sosa:hasResult rdf:resource="#corneliusKegWeightLB"/>
   <sosa:hasSimpleResult rdf:datatype="http://www.qudt.org/2.1/vocab/unit/LB">9.0</sosa:hasSimpleResult>
   <rdfs:isDefinedBy rdf:resource="https://rdf.ag/o/beer-ONTOLOGY_DATE"/>
   <void:inDataset rdf:resource="#datasetdefinition"/>
  </rdf:Description>
 </sosa:isFeatureOfInterestOf>
 <rdfs:isDefinedBy rdf:resource="https://rdf.ag/o/beer-ONTOLOGY_DATE"/>
 <void:inDataset rdf:resource="#datasetdefinition"/>
</rdf:Description>
<rdf:Description rdf:about="#sixthBarrelKeg">
 <rdf:type rdf:resource="#LiquidContainer"/>
 <rdf:type rdf:resource="#Keg"/>
 <rdf:type rdf:resource="https://gs1.org/voc/PackagingDetails"/>
 <rdfs:label xml:lang="en">Sixth Barrel Keg</rdfs:label>
 <rdfs:label xml:lang="fr">fûts de Sixtel </rdfs:label>
 <skos:definition xml:lang="en">Sixth Barrel Keg</skos:definition>
 <skos:definition xml:lang="fr">fûts de Sixtel </skos:definition>
 <skos:altLabel xml:lang="en">Sixtel</skos:altLabel>
 <beer:nominalCapacity rdf:datatype="http://www.qudt.org/2.1/vocab/unit/MilliL">20000</beer:nominalCapacity>
 <sosa:isFeatureOfInterestOf>
  <rdf:Description rdf:about="#sixthBarrelKegContentSosaML">
   <rdf:type rdf:resource="http://www.w3.org/ns/sosa/Observation"/>
   <sosa:hasFeatureOfInterest rdf:resource="#sixthBarrelKeg"/>
   <sosa:observedProperty rdf:resource="#sosaNominalCapacity"/>
   <sosa:hasResult>
    <gs1:QuantitativeValue rdf:about="#sixthBarrelKegContentML">
     <rdf:type rdf:resource="http://qudt.org/1.1/schema/qudt#QuantityValue"/>
     <gs1:unitCode>MLT</gs1:unitCode>
     <gs1:value>20000</gs1:value>
     <rdf:value rdf:datatype="http://www.w3.org/2001/XMLSchema#double">20000</rdf:value>
     <qudt:unit rdf:resource="http://www.qudt.org/2.1/vocab/unit/MilliL"/>
     <qudt:numericalValue rdf:datatype="http://www.w3.org/2001/XMLSchema#double">20000</qudt:numericalValue>
     <rdfs:isDefinedBy rdf:resource="https://rdf.ag/o/beer-ONTOLOGY_DATE"/>
     <void:inDataset rdf:resource="#datasetdefinition"/>
    </gs1:QuantitativeValue>
   </sosa:hasResult> 
   <sosa:hasSimpleResult rdf:datatype="http://www.qudt.org/2.1/vocab/unit/MilliM">20000</sosa:hasSimpleResult>
   <rdfs:isDefinedBy rdf:resource="https://rdf.ag/o/beer-ONTOLOGY_DATE"/>
   <void:inDataset rdf:resource="#datasetdefinition"/>
  </rdf:Description>
 </sosa:isFeatureOfInterestOf>
 <sosa:isFeatureOfInterestOf>
  <rdf:Description rdf:about="#sixthBarrelKegContentSosaOZ">
   <rdf:type rdf:resource="http://www.w3.org/ns/sosa/Observation"/>
   <sosa:hasFeatureOfInterest rdf:resource="#sixthBarrelKeg"/>
   <sosa:observedProperty rdf:resource="#sosaNominalCapacity"/>
   <sosa:hasResult>
   <gs1:QuantitativeValue rdf:about="#sixthBarrelKegContentOZ">
    <rdf:type rdf:resource="http://qudt.org/1.1/schema/qudt#QuantityValue"/>
    <gs1:unitCode>foz_us</gs1:unitCode>
    <gs1:value>660</gs1:value>
    <rdf:value rdf:datatype="http://www.w3.org/2001/XMLSchema#double">660</rdf:value>
    <qudt:unit rdf:resource="http://www.qudt.org/2.1/vocab/unit/OZ_VOL_US"/>
    <qudt:numericalValue rdf:datatype="http://www.w3.org/2001/XMLSchema#double">660</qudt:numericalValue>
    <rdfs:isDefinedBy rdf:resource="https://rdf.ag/o/beer-ONTOLOGY_DATE"/>
    <void:inDataset rdf:resource="#datasetdefinition"/>  
   </gs1:QuantitativeValue>
   </sosa:hasResult>
   <sosa:hasSimpleResult rdf:datatype="http://www.qudt.org/2.1/vocab/unit/OZ_VOL_US">660</sosa:hasSimpleResult>
   <rdfs:isDefinedBy rdf:resource="https://rdf.ag/o/beer-ONTOLOGY_DATE"/>
   <void:inDataset rdf:resource="#datasetdefinition"/>  
 </rdf:Description>
 </sosa:isFeatureOfInterestOf>
 <!-- Net Content Gal -->
 <sosa:isFeatureOfInterestOf>
  <rdf:Description rdf:about="#sixthBarrelKegContentSosaGAL">
   <rdf:type rdf:resource="http://www.w3.org/ns/sosa/Observation"/>
   <sosa:hasFeatureOfInterest rdf:resource="#sixthBarrelKeg"/>
   <sosa:observedProperty rdf:resource="#netcontent"/>
   <sosa:hasResult>
    <gs1:QuantitativeValue rdf:about="#sixthBarrelKegContentGal">
     <rdf:type rdf:resource="http://qudt.org/1.1/schema/qudt#QuantityValue"/>
     <gs1:unitCode>gal_us</gs1:unitCode>
     <gs1:value>5.28</gs1:value>
     <rdf:value rdf:datatype="http://www.w3.org/2001/XMLSchema#double">5.28</rdf:value>
     <qudt:unit rdf:resource="http://www.qudt.org/2.1/vocab/unit/GAL_US"/>
     <qudt:numericalValue rdf:datatype="http://www.w3.org/2001/XMLSchema#double">5.28</qudt:numericalValue>
     <rdfs:isDefinedBy rdf:resource="https://rdf.ag/o/beer-ONTOLOGY_DATE"/>
     <void:inDataset rdf:resource="#datasetdefinition"/>  
    </gs1:QuantitativeValue>
   </sosa:hasResult>
   <sosa:hasSimpleResult rdf:datatype="http://www.qudt.org/2.1/vocab/unit/GAL_US">5.28</sosa:hasSimpleResult>
   <rdfs:isDefinedBy rdf:resource="https://rdf.ag/o/beer-ONTOLOGY_DATE"/>
   <void:inDataset rdf:resource="#datasetdefinition"/>  
 </rdf:Description>
 </sosa:isFeatureOfInterestOf>

 <!-- Height MM-->
 <gs1:inPackageHeight>
  <gs1:QuantitativeValue rdf:about="#sixthBarrelKegHeightMM">
   <rdf:type rdf:resource="http://qudt.org/1.1/schema/qudt#QuantityValue"/>
   <qudt:unit rdf:resource="http://www.qudt.org/2.1/vocab/unit/MilliM"/>
   <qudt:numericalValue rdf:datatype="http://www.w3.org/2001/XMLSchema#double">591</qudt:numericalValue>
   <rdf:value rdf:datatype="http://www.w3.org/2001/XMLSchema#double">591</rdf:value>
   <gs1:unitCode>MMT</gs1:unitCode>
   <gs1:value>591</gs1:value>
   <rdfs:isDefinedBy rdf:resource="https://rdf.ag/o/beer-ONTOLOGY_DATE"/>
   <void:inDataset rdf:resource="#datasetdefinition"/>
  </gs1:QuantitativeValue>
 </gs1:inPackageHeight>  
 <sosa:isFeatureOfInterestOf>
  <rdf:Description rdf:about="#sixthBarrelKegHeightSosaMM">
   <rdf:type rdf:resource="http://www.w3.org/ns/sosa/Observation"/>
   <sosa:hasFeatureOfInterest rdf:resource="#sixthBarrelKeg"/>
   <sosa:observedProperty  rdf:resource="#height"/>
   <sosa:hasResult rdf:resource="#sixthBarrelKegHeightMM"/>
   <sosa:hasSimpleResult rdf:datatype="http://www.qudt.org/2.1/vocab/unit/MilliM">591</sosa:hasSimpleResult>
   <rdfs:isDefinedBy rdf:resource="https://rdf.ag/o/beer-ONTOLOGY_DATE"/>
   <void:inDataset rdf:resource="#datasetdefinition"/>
  </rdf:Description>
 </sosa:isFeatureOfInterestOf>
 <!-- Height IN-->
 <gs1:inPackageHeight>
  <gs1:QuantitativeValue rdf:about="#sixthBarrelKegHeightIN">
   <rdf:type rdf:resource="http://qudt.org/1.1/schema/qudt#QuantityValue"/>
   <qudt:unit rdf:resource="http://www.qudt.org/2.1/vocab/unit/IN"/>
   <qudt:numericalValue rdf:datatype="http://www.w3.org/2001/XMLSchema#double">23.250</qudt:numericalValue>
   <rdf:value rdf:datatype="http://www.w3.org/2001/XMLSchema#double">23.250</rdf:value>
   <gs1:unitCode>INH</gs1:unitCode>
   <gs1:value>23.250</gs1:value>
   <rdfs:isDefinedBy rdf:resource="https://rdf.ag/o/beer-ONTOLOGY_DATE"/>
   <void:inDataset rdf:resource="#datasetdefinition"/>
  </gs1:QuantitativeValue>
 </gs1:inPackageHeight>  
 <sosa:isFeatureOfInterestOf>
  <rdf:Description rdf:about="#sixthBarrelKegHeightSosaIN">
   <rdf:type rdf:resource="http://www.w3.org/ns/sosa/Observation"/>
   <sosa:hasFeatureOfInterest rdf:resource="#sixthBarrelKeg"/>
   <sosa:observedProperty  rdf:resource="#height"/>
   <sosa:hasResult rdf:resource="#sixthBarrelKegHeightIN"/>
   <sosa:hasSimpleResult rdf:datatype="http://www.qudt.org/2.1/vocab/unit/IN">23.250</sosa:hasSimpleResult>
   <rdfs:isDefinedBy rdf:resource="https://rdf.ag/o/beer-ONTOLOGY_DATE"/>
   <void:inDataset rdf:resource="#datasetdefinition"/>
  </rdf:Description>
 </sosa:isFeatureOfInterestOf>
 <!-- Diameter MM --> 
 <gs1:inPackageDiameter>
  <gs1:QuantitativeValue rdf:about="#sixthBarrelKegDiameterMM">
   <rdf:type rdf:resource="http://qudt.org/1.1/schema/qudt#QuantityValue"/>
   <qudt:unit rdf:resource="http://www.qudt.org/2.1/vocab/unit/MilliM"/>
   <qudt:numericalValue rdf:datatype="http://www.w3.org/2001/XMLSchema#double">234</qudt:numericalValue>
   <rdf:value rdf:datatype="http://www.w3.org/2001/XMLSchema#double">234</rdf:value>
   <gs1:unitCode>MMT</gs1:unitCode>
   <gs1:value>234</gs1:value>
   <rdfs:isDefinedBy rdf:resource="https://rdf.ag/o/beer-ONTOLOGY_DATE"/>
   <void:inDataset rdf:resource="#datasetdefinition"/>
  </gs1:QuantitativeValue>
 </gs1:inPackageDiameter>
 <sosa:isFeatureOfInterestOf>
  <rdf:Description rdf:about="#sixthBarrelKegDiameterSosaMM">
   <rdf:type rdf:resource="http://www.w3.org/ns/sosa/Observation"/>
   <sosa:hasFeatureOfInterest rdf:resource="#sixthBarrelKeg"/>
   <sosa:observedProperty  rdf:resource="#diameter"/>
   <sosa:hasResult rdf:resource="#sixthBarrelKegDiameterMM"/>
   <sosa:hasSimpleResult rdf:datatype="http://www.qudt.org/2.1/vocab/unit/MilliM">234</sosa:hasSimpleResult>
   <rdfs:isDefinedBy rdf:resource="https://rdf.ag/o/beer-ONTOLOGY_DATE"/>
   <void:inDataset rdf:resource="#datasetdefinition"/>
  </rdf:Description>
 </sosa:isFeatureOfInterestOf>
 <!-- Diameter IN --> 
 <gs1:inPackageDiameter>
  <gs1:QuantitativeValue rdf:about="#sixthBarrelKegDiameterIN">
   <rdf:type rdf:resource="http://qudt.org/1.1/schema/qudt#QuantityValue"/>
   <qudt:unit rdf:resource="http://www.qudt.org/2.1/vocab/unit/IN"/>
   <qudt:numericalValue rdf:datatype="http://www.w3.org/2001/XMLSchema#double">9.190</qudt:numericalValue>
   <rdf:value rdf:datatype="http://www.w3.org/2001/XMLSchema#double">9.190</rdf:value>
   <gs1:unitCode>INH</gs1:unitCode>
   <gs1:value>9.190</gs1:value>
   <rdfs:isDefinedBy rdf:resource="https://rdf.ag/o/beer-ONTOLOGY_DATE"/>
   <void:inDataset rdf:resource="#datasetdefinition"/>
  </gs1:QuantitativeValue>
 </gs1:inPackageDiameter>
 <sosa:isFeatureOfInterestOf>
  <rdf:Description rdf:about="#sixthBarrelKegDiameterSosaIN">
   <rdf:type rdf:resource="http://www.w3.org/ns/sosa/Observation"/>
   <sosa:hasFeatureOfInterest rdf:resource="#sixthBarrelKeg"/>
   <sosa:observedProperty  rdf:resource="#diameter"/>
   <sosa:hasResult rdf:resource="#sixthBarrelKegDiameterIN"/>
   <sosa:hasSimpleResult rdf:datatype="http://www.qudt.org/2.1/vocab/unit/IN">9.190</sosa:hasSimpleResult>
   <rdfs:isDefinedBy rdf:resource="https://rdf.ag/o/beer-ONTOLOGY_DATE"/>
   <void:inDataset rdf:resource="#datasetdefinition"/>
  </rdf:Description>
 </sosa:isFeatureOfInterestOf>
 <!-- KG Weight -->
 <schema:weight>
  <gs1:QuantitativeValue rdf:about="#sixthBarrelKegWeightKG">
   <rdf:type rdf:resource="http://qudt.org/1.1/schema/qudt#QuantityValue"/>
   <qudt:unit rdf:resource="http://www.qudt.org/2.1/vocab/unit/KiloGM"/>
   <qudt:numericalValue rdf:datatype="http://www.w3.org/2001/XMLSchema#double">7.5</qudt:numericalValue>
   <rdf:value rdf:datatype="http://www.w3.org/2001/XMLSchema#double">7.5</rdf:value>
   <gs1:unitCode>KGM</gs1:unitCode>
   <gs1:value>7.5</gs1:value>
   <rdfs:isDefinedBy rdf:resource="https://rdf.ag/o/beer-ONTOLOGY_DATE"/>
   <void:inDataset rdf:resource="#datasetdefinition"/>
  </gs1:QuantitativeValue>
 </schema:weight>
 <sosa:isFeatureOfInterestOf>
  <rdf:Description rdf:about="#sixthBarrelKegWeightSosaKG">
   <rdf:type rdf:resource="http://www.w3.org/ns/sosa/Observation"/>
   <sosa:hasFeatureOfInterest rdf:resource="#sixthBarrelKeg"/>
   <sosa:observedProperty  rdf:resource="#grossWeight"/>
   <sosa:hasResult rdf:resource="#sixthBarrelKegWeightKG"/>
   <sosa:hasSimpleResult rdf:datatype="http://www.qudt.org/2.1/vocab/unit/KiloGM">7.5</sosa:hasSimpleResult>
   <rdfs:isDefinedBy rdf:resource="https://rdf.ag/o/beer-ONTOLOGY_DATE"/>
   <void:inDataset rdf:resource="#datasetdefinition"/>
  </rdf:Description>
 </sosa:isFeatureOfInterestOf>
 <!-- LB Weight -->
 <schema:weight>
  <gs1:QuantitativeValue rdf:about="#sixthBarrelKegWeightLB">
   <rdf:type rdf:resource="http://qudt.org/1.1/schema/qudt#QuantityValue"/>
   <qudt:unit rdf:resource="http://www.qudt.org/2.1/vocab/unit/LB"/>
   <qudt:numericalValue rdf:datatype="http://www.w3.org/2001/XMLSchema#double">16.5</qudt:numericalValue>
   <rdf:value rdf:datatype="http://www.w3.org/2001/XMLSchema#double">16.5</rdf:value>
   <gs1:unitCode>lbm</gs1:unitCode>
   <gs1:value>16.5</gs1:value>
   <rdfs:isDefinedBy rdf:resource="https://rdf.ag/o/beer-ONTOLOGY_DATE"/>
   <void:inDataset rdf:resource="#datasetdefinition"/>
  </gs1:QuantitativeValue>
 </schema:weight>
 <sosa:isFeatureOfInterestOf>
  <rdf:Description rdf:about="#sixthBarrelKegWeightSosaLB">
   <rdf:type rdf:resource="http://www.w3.org/ns/sosa/Observation"/>
   <sosa:hasFeatureOfInterest rdf:resource="#sixthBarrelKeg"/>
   <sosa:observedProperty  rdf:resource="#grossWeight"/>
   <sosa:hasResult rdf:resource="#sixthBarrelKegWeightLB"/>
   <sosa:hasSimpleResult rdf:datatype="http://www.qudt.org/2.1/vocab/unit/LB">16.5</sosa:hasSimpleResult>
   <rdfs:isDefinedBy rdf:resource="https://rdf.ag/o/beer-ONTOLOGY_DATE"/>
   <void:inDataset rdf:resource="#datasetdefinition"/>
  </rdf:Description>
 </sosa:isFeatureOfInterestOf>
 <rdfs:isDefinedBy rdf:resource="https://rdf.ag/o/beer-ONTOLOGY_DATE"/>
 <void:inDataset rdf:resource="#datasetdefinition"/>
</rdf:Description>
<rdf:Description rdf:about="#slimQuarterKeg">
 <rdf:type rdf:resource="#LiquidContainer"/>
 <rdf:type rdf:resource="#Keg"/>
 <rdf:type rdf:resource="https://gs1.org/voc/PackagingDetails"/>
 <rdfs:label xml:lang="en">Slim Quarter Keg</rdfs:label>
 <rdfs:label xml:lang="fr">Fût Mince</rdfs:label>
 <skos:definition xml:lang="en">Slim Quarter Keg</skos:definition>
 <skos:definition xml:lang="fr">Fût Mince</skos:definition>
 <skos:altLabel xml:lang="en">Slim</skos:altLabel>
 <beer:nominalCapacity rdf:datatype="http://www.qudt.org/2.1/vocab/unit/MilliL">30000</beer:nominalCapacity>
 <sosa:isFeatureOfInterestOf>
  <rdf:Description rdf:about="#slimQuarterKegContentSosaML">
   <rdf:type rdf:resource="http://www.w3.org/ns/sosa/Observation"/>
   <sosa:hasFeatureOfInterest rdf:resource="#slimQuarterKeg"/>
   <sosa:observedProperty rdf:resource="#sosaNominalCapacity"/>
   <sosa:hasResult>
    <gs1:QuantitativeValue rdf:about="#slimQuarterKegContentML">
     <rdf:type rdf:resource="http://qudt.org/1.1/schema/qudt#QuantityValue"/>
     <gs1:unitCode>MLT</gs1:unitCode>
     <gs1:value>30000</gs1:value>
     <rdf:value rdf:datatype="http://www.w3.org/2001/XMLSchema#double">30000</rdf:value>
     <qudt:unit rdf:resource="http://www.qudt.org/2.1/vocab/unit/MilliL"/>
     <qudt:numericalValue rdf:datatype="http://www.w3.org/2001/XMLSchema#double">30000</qudt:numericalValue>
     <rdfs:isDefinedBy rdf:resource="https://rdf.ag/o/beer-ONTOLOGY_DATE"/>
     <void:inDataset rdf:resource="#datasetdefinition"/>
    </gs1:QuantitativeValue>
   </sosa:hasResult> 
   <sosa:hasSimpleResult rdf:datatype="http://www.qudt.org/2.1/vocab/unit/MilliM">30000</sosa:hasSimpleResult>
   <rdfs:isDefinedBy rdf:resource="https://rdf.ag/o/beer-ONTOLOGY_DATE"/>
   <void:inDataset rdf:resource="#datasetdefinition"/>
  </rdf:Description>
 </sosa:isFeatureOfInterestOf>
 <sosa:isFeatureOfInterestOf>
  <rdf:Description rdf:about="#slimQuarterKegContentSosaOZ">
   <rdf:type rdf:resource="http://www.w3.org/ns/sosa/Observation"/>
   <sosa:hasFeatureOfInterest rdf:resource="#slimQuarterKeg"/>
   <sosa:observedProperty rdf:resource="#sosaNominalCapacity"/>
   <sosa:hasResult>
   <gs1:QuantitativeValue rdf:about="#slimQuarterKegContentOZ">
    <rdf:type rdf:resource="http://qudt.org/1.1/schema/qudt#QuantityValue"/>
    <gs1:unitCode>foz_us</gs1:unitCode>
    <gs1:value>1014</gs1:value>
    <rdf:value rdf:datatype="http://www.w3.org/2001/XMLSchema#double">1014</rdf:value>
    <qudt:unit rdf:resource="http://www.qudt.org/2.1/vocab/unit/OZ_VOL_US"/>
    <qudt:numericalValue rdf:datatype="http://www.w3.org/2001/XMLSchema#double">1014</qudt:numericalValue>
    <rdfs:isDefinedBy rdf:resource="https://rdf.ag/o/beer-ONTOLOGY_DATE"/>
    <void:inDataset rdf:resource="#datasetdefinition"/>  
   </gs1:QuantitativeValue>
   </sosa:hasResult>
   <sosa:hasSimpleResult rdf:datatype="http://www.qudt.org/2.1/vocab/unit/OZ_VOL_US">1014</sosa:hasSimpleResult>
   <rdfs:isDefinedBy rdf:resource="https://rdf.ag/o/beer-ONTOLOGY_DATE"/>
   <void:inDataset rdf:resource="#datasetdefinition"/>  
 </rdf:Description>
 </sosa:isFeatureOfInterestOf>
 <!-- Net Content Gal -->
 <sosa:isFeatureOfInterestOf>
  <rdf:Description rdf:about="#slimQuarterKegContentSosaGAL">
   <rdf:type rdf:resource="http://www.w3.org/ns/sosa/Observation"/>
   <sosa:hasFeatureOfInterest rdf:resource="#slimQuarterKeg"/>
   <sosa:observedProperty rdf:resource="#netcontent"/>
   <sosa:hasResult>
    <gs1:QuantitativeValue rdf:about="#slimQuarterKegContentGal">
     <rdf:type rdf:resource="http://qudt.org/1.1/schema/qudt#QuantityValue"/>
     <gs1:unitCode>gal_us</gs1:unitCode>
     <gs1:value>7.92</gs1:value>
     <rdf:value rdf:datatype="http://www.w3.org/2001/XMLSchema#double">7.92</rdf:value>
     <qudt:unit rdf:resource="http://www.qudt.org/2.1/vocab/unit/GAL_US"/>
     <qudt:numericalValue rdf:datatype="http://www.w3.org/2001/XMLSchema#double">7.92</qudt:numericalValue>
     <rdfs:isDefinedBy rdf:resource="https://rdf.ag/o/beer-ONTOLOGY_DATE"/>
     <void:inDataset rdf:resource="#datasetdefinition"/>  
    </gs1:QuantitativeValue>
   </sosa:hasResult>
   <sosa:hasSimpleResult rdf:datatype="http://www.qudt.org/2.1/vocab/unit/GAL_US">7.92</sosa:hasSimpleResult>
   <rdfs:isDefinedBy rdf:resource="https://rdf.ag/o/beer-ONTOLOGY_DATE"/>
   <void:inDataset rdf:resource="#datasetdefinition"/>  
 </rdf:Description>
 </sosa:isFeatureOfInterestOf>

 <!-- Height MM-->
 <gs1:inPackageHeight>
  <gs1:QuantitativeValue rdf:about="#slimQuarterKegHeightMM">
   <rdf:type rdf:resource="http://qudt.org/1.1/schema/qudt#QuantityValue"/>
   <qudt:unit rdf:resource="http://www.qudt.org/2.1/vocab/unit/MilliM"/>
   <qudt:numericalValue rdf:datatype="http://www.w3.org/2001/XMLSchema#double">594</qudt:numericalValue>
   <rdf:value rdf:datatype="http://www.w3.org/2001/XMLSchema#double">594</rdf:value>
   <gs1:unitCode>MMT</gs1:unitCode>
   <gs1:value>594</gs1:value>
   <rdfs:isDefinedBy rdf:resource="https://rdf.ag/o/beer-ONTOLOGY_DATE"/>
   <void:inDataset rdf:resource="#datasetdefinition"/>
  </gs1:QuantitativeValue>
 </gs1:inPackageHeight>  
 <sosa:isFeatureOfInterestOf>
  <rdf:Description rdf:about="#slimQuarterKegHeightSosaMM">
   <rdf:type rdf:resource="http://www.w3.org/ns/sosa/Observation"/>
   <sosa:hasFeatureOfInterest rdf:resource="#slimQuarterKeg"/>
   <sosa:observedProperty  rdf:resource="#height"/>
   <sosa:hasResult rdf:resource="#slimQuarterKegHeightMM"/>
   <sosa:hasSimpleResult rdf:datatype="http://www.qudt.org/2.1/vocab/unit/MilliM">594</sosa:hasSimpleResult>
   <rdfs:isDefinedBy rdf:resource="https://rdf.ag/o/beer-ONTOLOGY_DATE"/>
   <void:inDataset rdf:resource="#datasetdefinition"/>
  </rdf:Description>
 </sosa:isFeatureOfInterestOf>
 <!-- Height IN-->
 <gs1:inPackageHeight>
  <gs1:QuantitativeValue rdf:about="#slimQuarterKegHeightIN">
   <rdf:type rdf:resource="http://qudt.org/1.1/schema/qudt#QuantityValue"/>
   <qudt:unit rdf:resource="http://www.qudt.org/2.1/vocab/unit/IN"/>
   <qudt:numericalValue rdf:datatype="http://www.w3.org/2001/XMLSchema#double">23.400</qudt:numericalValue>
   <rdf:value rdf:datatype="http://www.w3.org/2001/XMLSchema#double">23.400</rdf:value>
   <gs1:unitCode>INH</gs1:unitCode>
   <gs1:value>23.400</gs1:value>
   <rdfs:isDefinedBy rdf:resource="https://rdf.ag/o/beer-ONTOLOGY_DATE"/>
   <void:inDataset rdf:resource="#datasetdefinition"/>
  </gs1:QuantitativeValue>
 </gs1:inPackageHeight>  
 <sosa:isFeatureOfInterestOf>
  <rdf:Description rdf:about="#slimQuarterKegHeightSosaIN">
   <rdf:type rdf:resource="http://www.w3.org/ns/sosa/Observation"/>
   <sosa:hasFeatureOfInterest rdf:resource="#slimQuarterKeg"/>
   <sosa:observedProperty  rdf:resource="#height"/>
   <sosa:hasResult rdf:resource="#slimQuarterKegHeightIN"/>
   <sosa:hasSimpleResult rdf:datatype="http://www.qudt.org/2.1/vocab/unit/IN">23.400</sosa:hasSimpleResult>
   <rdfs:isDefinedBy rdf:resource="https://rdf.ag/o/beer-ONTOLOGY_DATE"/>
   <void:inDataset rdf:resource="#datasetdefinition"/>
  </rdf:Description>
 </sosa:isFeatureOfInterestOf>
 <!-- Diameter MM --> 
 <gs1:inPackageDiameter>
  <gs1:QuantitativeValue rdf:about="#slimQuarterKegDiameterMM">
   <rdf:type rdf:resource="http://qudt.org/1.1/schema/qudt#QuantityValue"/>
   <qudt:unit rdf:resource="http://www.qudt.org/2.1/vocab/unit/MilliM"/>
   <qudt:numericalValue rdf:datatype="http://www.w3.org/2001/XMLSchema#double">286</qudt:numericalValue>
   <rdf:value rdf:datatype="http://www.w3.org/2001/XMLSchema#double">286</rdf:value>
   <gs1:unitCode>MMT</gs1:unitCode>
   <gs1:value>286</gs1:value>
   <rdfs:isDefinedBy rdf:resource="https://rdf.ag/o/beer-ONTOLOGY_DATE"/>
   <void:inDataset rdf:resource="#datasetdefinition"/>
  </gs1:QuantitativeValue>
 </gs1:inPackageDiameter>
 <sosa:isFeatureOfInterestOf>
  <rdf:Description rdf:about="#slimQuarterKegDiameterSosaMM">
   <rdf:type rdf:resource="http://www.w3.org/ns/sosa/Observation"/>
   <sosa:hasFeatureOfInterest rdf:resource="#slimQuarterKeg"/>
   <sosa:observedProperty  rdf:resource="#diameter"/>
   <sosa:hasResult rdf:resource="#slimQuarterKegDiameterMM"/>
   <sosa:hasSimpleResult rdf:datatype="http://www.qudt.org/2.1/vocab/unit/MilliM">286</sosa:hasSimpleResult>
   <rdfs:isDefinedBy rdf:resource="https://rdf.ag/o/beer-ONTOLOGY_DATE"/>
   <void:inDataset rdf:resource="#datasetdefinition"/>
  </rdf:Description>
 </sosa:isFeatureOfInterestOf>
 <!-- Diameter IN --> 
 <gs1:inPackageDiameter>
  <gs1:QuantitativeValue rdf:about="#slimQuarterKegDiameterIN">
   <rdf:type rdf:resource="http://qudt.org/1.1/schema/qudt#QuantityValue"/>
   <qudt:unit rdf:resource="http://www.qudt.org/2.1/vocab/unit/IN"/>
   <qudt:numericalValue rdf:datatype="http://www.w3.org/2001/XMLSchema#double">11.250</qudt:numericalValue>
   <rdf:value rdf:datatype="http://www.w3.org/2001/XMLSchema#double">11.250</rdf:value>
   <gs1:unitCode>INH</gs1:unitCode>
   <gs1:value>11.250</gs1:value>
   <rdfs:isDefinedBy rdf:resource="https://rdf.ag/o/beer-ONTOLOGY_DATE"/>
   <void:inDataset rdf:resource="#datasetdefinition"/>
  </gs1:QuantitativeValue>
 </gs1:inPackageDiameter>
 <sosa:isFeatureOfInterestOf>
  <rdf:Description rdf:about="#slimQuarterKegDiameterSosaIN">
   <rdf:type rdf:resource="http://www.w3.org/ns/sosa/Observation"/>
   <sosa:hasFeatureOfInterest rdf:resource="#slimQuarterKeg"/>
   <sosa:observedProperty  rdf:resource="#diameter"/>
   <sosa:hasResult rdf:resource="#slimQuarterKegDiameterIN"/>
   <sosa:hasSimpleResult rdf:datatype="http://www.qudt.org/2.1/vocab/unit/IN">11.250</sosa:hasSimpleResult>
   <rdfs:isDefinedBy rdf:resource="https://rdf.ag/o/beer-ONTOLOGY_DATE"/>
   <void:inDataset rdf:resource="#datasetdefinition"/>
  </rdf:Description>
 </sosa:isFeatureOfInterestOf>
 <!-- KG Weight -->
 <schema:weight>
  <gs1:QuantitativeValue rdf:about="#slimQuarterKegWeightKG">
   <rdf:type rdf:resource="http://qudt.org/1.1/schema/qudt#QuantityValue"/>
   <qudt:unit rdf:resource="http://www.qudt.org/2.1/vocab/unit/KiloGM"/>
   <qudt:numericalValue rdf:datatype="http://www.w3.org/2001/XMLSchema#double">11.3</qudt:numericalValue>
   <rdf:value rdf:datatype="http://www.w3.org/2001/XMLSchema#double">11.3</rdf:value>
   <gs1:unitCode>KGM</gs1:unitCode>
   <gs1:value>11.3</gs1:value>
   <rdfs:isDefinedBy rdf:resource="https://rdf.ag/o/beer-ONTOLOGY_DATE"/>
   <void:inDataset rdf:resource="#datasetdefinition"/>
  </gs1:QuantitativeValue>
 </schema:weight>
 <sosa:isFeatureOfInterestOf>
  <rdf:Description rdf:about="#slimQuarterKegWeightSosaKG">
   <rdf:type rdf:resource="http://www.w3.org/ns/sosa/Observation"/>
   <sosa:hasFeatureOfInterest rdf:resource="#slimQuarterKeg"/>
   <sosa:observedProperty  rdf:resource="#grossWeight"/>
   <sosa:hasResult rdf:resource="#slimQuarterKegWeightKG"/>
   <sosa:hasSimpleResult rdf:datatype="http://www.qudt.org/2.1/vocab/unit/KiloGM">11.3</sosa:hasSimpleResult>
   <rdfs:isDefinedBy rdf:resource="https://rdf.ag/o/beer-ONTOLOGY_DATE"/>
   <void:inDataset rdf:resource="#datasetdefinition"/>
  </rdf:Description>
 </sosa:isFeatureOfInterestOf>
 <!-- LB Weight -->
 <schema:weight>
  <gs1:QuantitativeValue rdf:about="#slimQuarterKegWeightLB">
   <rdf:type rdf:resource="http://qudt.org/1.1/schema/qudt#QuantityValue"/>
   <qudt:unit rdf:resource="http://www.qudt.org/2.1/vocab/unit/LB"/>
   <qudt:numericalValue rdf:datatype="http://www.w3.org/2001/XMLSchema#double">25.0</qudt:numericalValue>
   <rdf:value rdf:datatype="http://www.w3.org/2001/XMLSchema#double">25.0</rdf:value>
   <gs1:unitCode>lbm</gs1:unitCode>
   <gs1:value>25.0</gs1:value>
   <rdfs:isDefinedBy rdf:resource="https://rdf.ag/o/beer-ONTOLOGY_DATE"/>
   <void:inDataset rdf:resource="#datasetdefinition"/>
  </gs1:QuantitativeValue>
 </schema:weight>
 <sosa:isFeatureOfInterestOf>
  <rdf:Description rdf:about="#slimQuarterKegWeightSosaLB">
   <rdf:type rdf:resource="http://www.w3.org/ns/sosa/Observation"/>
   <sosa:hasFeatureOfInterest rdf:resource="#slimQuarterKeg"/>
   <sosa:observedProperty  rdf:resource="#grossWeight"/>
   <sosa:hasResult rdf:resource="#slimQuarterKegWeightLB"/>
   <sosa:hasSimpleResult rdf:datatype="http://www.qudt.org/2.1/vocab/unit/LB">25.0</sosa:hasSimpleResult>
   <rdfs:isDefinedBy rdf:resource="https://rdf.ag/o/beer-ONTOLOGY_DATE"/>
   <void:inDataset rdf:resource="#datasetdefinition"/>
  </rdf:Description>
 </sosa:isFeatureOfInterestOf>
 <rdfs:isDefinedBy rdf:resource="https://rdf.ag/o/beer-ONTOLOGY_DATE"/>
 <void:inDataset rdf:resource="#datasetdefinition"/>
</rdf:Description>

<rdf:Description rdf:about="#any30LKeg">
 <rdf:type rdf:resource="#LiquidContainer"/>
 <rdf:type rdf:resource="#Keg"/>
 <rdf:type rdf:resource="https://gs1.org/voc/PackagingDetails"/>
 <rdfs:label xml:lang="en">Any 30L Keg</rdfs:label>
 <rdfs:label xml:lang="fr">Fût de 30L</rdfs:label>
 <skos:definition xml:lang="en">Any 30L Keg</skos:definition>
 <skos:definition xml:lang="fr">Fût de 30L</skos:definition>
 <owl:oneOf>
  <rdf:List rdf:about="#any30LKeyList1">
   <rdf:first rdf:resource="#quarterKeg"/>
   <rdf:rest>
    <rdf:List rdf:about="#any30LKeyList2">
     <rdf:first rdf:resource="#slimQuarterKeg"/>
     <rdf:rest rdf:resource="http://www.w3.org/1999/02/22-rdf-syntax-ns#nil"/>
    </rdf:List>
   </rdf:rest>
  </rdf:List>
 </owl:oneOf>       
</rdf:Description>

<rdf:Description rdf:about="#quarerKeg">
 <rdf:type rdf:resource="#LiquidContainer"/>
 <rdf:type rdf:resource="#Keg"/>
 <rdf:type rdf:resource="https://gs1.org/voc/PackagingDetails"/>
 <rdfs:label xml:lang="en">Quarter Barrel Keg</rdfs:label>
 <rdfs:label xml:lang="fr">Quart de Fût</rdfs:label>
 <skos:definition xml:lang="en">Quarter Barrel Keg</skos:definition>
 <skos:definition xml:lang="fr">Quart de Fût</skos:definition>
 <skos:altLabel xml:lang="en">Pony Keg</skos:altLabel>
 <beer:nominalCapacity rdf:datatype="http://www.qudt.org/2.1/vocab/unit/MilliL">30000</beer:nominalCapacity>
 <sosa:isFeatureOfInterestOf>
  <rdf:Description rdf:about="#quarterKegContentSosaML">
   <rdf:type rdf:resource="http://www.w3.org/ns/sosa/Observation"/>
   <sosa:hasFeatureOfInterest rdf:resource="#quarterKeg"/>
   <sosa:observedProperty rdf:resource="#sosaNominalCapacity"/>
   <sosa:hasResult>
    <gs1:QuantitativeValue rdf:about="#quarterKegContentML">
     <rdf:type rdf:resource="http://qudt.org/1.1/schema/qudt#QuantityValue"/>
     <gs1:unitCode>MLT</gs1:unitCode>
     <gs1:value>30000</gs1:value>
     <rdf:value rdf:datatype="http://www.w3.org/2001/XMLSchema#double">30000</rdf:value>
     <qudt:unit rdf:resource="http://www.qudt.org/2.1/vocab/unit/MilliL"/>
     <qudt:numericalValue rdf:datatype="http://www.w3.org/2001/XMLSchema#double">30000</qudt:numericalValue>
     <rdfs:isDefinedBy rdf:resource="https://rdf.ag/o/beer-ONTOLOGY_DATE"/>
     <void:inDataset rdf:resource="#datasetdefinition"/>
    </gs1:QuantitativeValue>
   </sosa:hasResult> 
   <sosa:hasSimpleResult rdf:datatype="http://www.qudt.org/2.1/vocab/unit/MilliM">30000</sosa:hasSimpleResult>
   <rdfs:isDefinedBy rdf:resource="https://rdf.ag/o/beer-ONTOLOGY_DATE"/>
   <void:inDataset rdf:resource="#datasetdefinition"/>
  </rdf:Description>
 </sosa:isFeatureOfInterestOf>
 <sosa:isFeatureOfInterestOf>
  <rdf:Description rdf:about="#quarterKegContentSosaOZ">
   <rdf:type rdf:resource="http://www.w3.org/ns/sosa/Observation"/>
   <sosa:hasFeatureOfInterest rdf:resource="#quarterKeg"/>
   <sosa:observedProperty rdf:resource="#sosaNominalCapacity"/>
   <sosa:hasResult>
   <gs1:QuantitativeValue rdf:about="#quarterKegContentOZ">
    <rdf:type rdf:resource="http://qudt.org/1.1/schema/qudt#QuantityValue"/>
    <gs1:unitCode>foz_us</gs1:unitCode>
    <gs1:value>1014</gs1:value>
    <rdf:value rdf:datatype="http://www.w3.org/2001/XMLSchema#double">1014</rdf:value>
    <qudt:unit rdf:resource="http://www.qudt.org/2.1/vocab/unit/OZ_VOL_US"/>
    <qudt:numericalValue rdf:datatype="http://www.w3.org/2001/XMLSchema#double">1014</qudt:numericalValue>
    <rdfs:isDefinedBy rdf:resource="https://rdf.ag/o/beer-ONTOLOGY_DATE"/>
    <void:inDataset rdf:resource="#datasetdefinition"/>  
   </gs1:QuantitativeValue>
   </sosa:hasResult>
   <sosa:hasSimpleResult rdf:datatype="http://www.qudt.org/2.1/vocab/unit/OZ_VOL_US">1014</sosa:hasSimpleResult>
   <rdfs:isDefinedBy rdf:resource="https://rdf.ag/o/beer-ONTOLOGY_DATE"/>
   <void:inDataset rdf:resource="#datasetdefinition"/>  
 </rdf:Description>
 </sosa:isFeatureOfInterestOf>
 <!-- Net Content Gal -->
 <sosa:isFeatureOfInterestOf>
  <rdf:Description rdf:about="#quarterKegContentSosaGAL">
   <rdf:type rdf:resource="http://www.w3.org/ns/sosa/Observation"/>
   <sosa:hasFeatureOfInterest rdf:resource="#quarterKeg"/>
   <sosa:observedProperty rdf:resource="#netcontent"/>
   <sosa:hasResult>
    <gs1:QuantitativeValue rdf:about="#quarterKegContentGal">
     <rdf:type rdf:resource="http://qudt.org/1.1/schema/qudt#QuantityValue"/>
     <gs1:unitCode>gal_us</gs1:unitCode>
     <gs1:value>7.92</gs1:value>
     <rdf:value rdf:datatype="http://www.w3.org/2001/XMLSchema#double">7.92</rdf:value>
     <qudt:unit rdf:resource="http://www.qudt.org/2.1/vocab/unit/GAL_US"/>
     <qudt:numericalValue rdf:datatype="http://www.w3.org/2001/XMLSchema#double">7.92</qudt:numericalValue>
     <rdfs:isDefinedBy rdf:resource="https://rdf.ag/o/beer-ONTOLOGY_DATE"/>
     <void:inDataset rdf:resource="#datasetdefinition"/>  
    </gs1:QuantitativeValue>
   </sosa:hasResult>
   <sosa:hasSimpleResult rdf:datatype="http://www.qudt.org/2.1/vocab/unit/GAL_US">7.92</sosa:hasSimpleResult>
   <rdfs:isDefinedBy rdf:resource="https://rdf.ag/o/beer-ONTOLOGY_DATE"/>
   <void:inDataset rdf:resource="#datasetdefinition"/>  
 </rdf:Description>
 </sosa:isFeatureOfInterestOf>

 <!-- Height MM-->
 <gs1:inPackageHeight>
  <gs1:QuantitativeValue rdf:about="#quarterKegHeightMM">
   <rdf:type rdf:resource="http://qudt.org/1.1/schema/qudt#QuantityValue"/>
   <qudt:unit rdf:resource="http://www.qudt.org/2.1/vocab/unit/MilliM"/>
   <qudt:numericalValue rdf:datatype="http://www.w3.org/2001/XMLSchema#double">351</qudt:numericalValue>
   <rdf:value rdf:datatype="http://www.w3.org/2001/XMLSchema#double">351</rdf:value>
   <gs1:unitCode>MMT</gs1:unitCode>
   <gs1:value>351</gs1:value>
   <rdfs:isDefinedBy rdf:resource="https://rdf.ag/o/beer-ONTOLOGY_DATE"/>
   <void:inDataset rdf:resource="#datasetdefinition"/>
  </gs1:QuantitativeValue>
 </gs1:inPackageHeight>  
 <sosa:isFeatureOfInterestOf>
  <rdf:Description rdf:about="#quarterKegHeightSosaMM">
   <rdf:type rdf:resource="http://www.w3.org/ns/sosa/Observation"/>
   <sosa:hasFeatureOfInterest rdf:resource="#quarterKeg"/>
   <sosa:observedProperty  rdf:resource="#height"/>
   <sosa:hasResult rdf:resource="#quarterKegHeightMM"/>
   <sosa:hasSimpleResult rdf:datatype="http://www.qudt.org/2.1/vocab/unit/MilliM">351</sosa:hasSimpleResult>
   <rdfs:isDefinedBy rdf:resource="https://rdf.ag/o/beer-ONTOLOGY_DATE"/>
   <void:inDataset rdf:resource="#datasetdefinition"/>
  </rdf:Description>
 </sosa:isFeatureOfInterestOf>
 <!-- Height IN-->
 <gs1:inPackageHeight>
  <gs1:QuantitativeValue rdf:about="#quarterKegHeightIN">
   <rdf:type rdf:resource="http://qudt.org/1.1/schema/qudt#QuantityValue"/>
   <qudt:unit rdf:resource="http://www.qudt.org/2.1/vocab/unit/IN"/>
   <qudt:numericalValue rdf:datatype="http://www.w3.org/2001/XMLSchema#double">13.800</qudt:numericalValue>
   <rdf:value rdf:datatype="http://www.w3.org/2001/XMLSchema#double">13.800</rdf:value>
   <gs1:unitCode>INH</gs1:unitCode>
   <gs1:value>13.800</gs1:value>
   <rdfs:isDefinedBy rdf:resource="https://rdf.ag/o/beer-ONTOLOGY_DATE"/>
   <void:inDataset rdf:resource="#datasetdefinition"/>
  </gs1:QuantitativeValue>
 </gs1:inPackageHeight>  
 <sosa:isFeatureOfInterestOf>
  <rdf:Description rdf:about="#quarterKegHeightSosaIN">
   <rdf:type rdf:resource="http://www.w3.org/ns/sosa/Observation"/>
   <sosa:hasFeatureOfInterest rdf:resource="#quarterKeg"/>
   <sosa:observedProperty  rdf:resource="#height"/>
   <sosa:hasResult rdf:resource="#quarterKegHeightIN"/>
   <sosa:hasSimpleResult rdf:datatype="http://www.qudt.org/2.1/vocab/unit/IN">13.800</sosa:hasSimpleResult>
   <rdfs:isDefinedBy rdf:resource="https://rdf.ag/o/beer-ONTOLOGY_DATE"/>
   <void:inDataset rdf:resource="#datasetdefinition"/>
  </rdf:Description>
 </sosa:isFeatureOfInterestOf>
 <!-- Diameter MM --> 
 <gs1:inPackageDiameter>
  <gs1:QuantitativeValue rdf:about="#quarterKegDiameterMM">
   <rdf:type rdf:resource="http://qudt.org/1.1/schema/qudt#QuantityValue"/>
   <qudt:unit rdf:resource="http://www.qudt.org/2.1/vocab/unit/MilliM"/>
   <qudt:numericalValue rdf:datatype="http://www.w3.org/2001/XMLSchema#double">409</qudt:numericalValue>
   <rdf:value rdf:datatype="http://www.w3.org/2001/XMLSchema#double">409</rdf:value>
   <gs1:unitCode>MMT</gs1:unitCode>
   <gs1:value>409</gs1:value>
   <rdfs:isDefinedBy rdf:resource="https://rdf.ag/o/beer-ONTOLOGY_DATE"/>
   <void:inDataset rdf:resource="#datasetdefinition"/>
  </gs1:QuantitativeValue>
 </gs1:inPackageDiameter>
 <sosa:isFeatureOfInterestOf>
  <rdf:Description rdf:about="#quarterKegDiameterSosaMM">
   <rdf:type rdf:resource="http://www.w3.org/ns/sosa/Observation"/>
   <sosa:hasFeatureOfInterest rdf:resource="#quarterKeg"/>
   <sosa:observedProperty  rdf:resource="#diameter"/>
   <sosa:hasResult rdf:resource="#quarterKegDiameterMM"/>
   <sosa:hasSimpleResult rdf:datatype="http://www.qudt.org/2.1/vocab/unit/MilliM">409</sosa:hasSimpleResult>
   <rdfs:isDefinedBy rdf:resource="https://rdf.ag/o/beer-ONTOLOGY_DATE"/>
   <void:inDataset rdf:resource="#datasetdefinition"/>
  </rdf:Description>
 </sosa:isFeatureOfInterestOf>
 <!-- Diameter IN --> 
 <gs1:inPackageDiameter>
  <gs1:QuantitativeValue rdf:about="#quarterKegDiameterIN">
   <rdf:type rdf:resource="http://qudt.org/1.1/schema/qudt#QuantityValue"/>
   <qudt:unit rdf:resource="http://www.qudt.org/2.1/vocab/unit/IN"/>
   <qudt:numericalValue rdf:datatype="http://www.w3.org/2001/XMLSchema#double">16.120</qudt:numericalValue>
   <rdf:value rdf:datatype="http://www.w3.org/2001/XMLSchema#double">16.120</rdf:value>
   <gs1:unitCode>INH</gs1:unitCode>
   <gs1:value>16.120</gs1:value>
   <rdfs:isDefinedBy rdf:resource="https://rdf.ag/o/beer-ONTOLOGY_DATE"/>
   <void:inDataset rdf:resource="#datasetdefinition"/>
  </gs1:QuantitativeValue>
 </gs1:inPackageDiameter>
 <sosa:isFeatureOfInterestOf>
  <rdf:Description rdf:about="#quarterKegDiameterSosaIN">
   <rdf:type rdf:resource="http://www.w3.org/ns/sosa/Observation"/>
   <sosa:hasFeatureOfInterest rdf:resource="#quarterKeg"/>
   <sosa:observedProperty  rdf:resource="#diameter"/>
   <sosa:hasResult rdf:resource="#quarterKegDiameterIN"/>
   <sosa:hasSimpleResult rdf:datatype="http://www.qudt.org/2.1/vocab/unit/IN">16.120</sosa:hasSimpleResult>
   <rdfs:isDefinedBy rdf:resource="https://rdf.ag/o/beer-ONTOLOGY_DATE"/>
   <void:inDataset rdf:resource="#datasetdefinition"/>
  </rdf:Description>
 </sosa:isFeatureOfInterestOf>
 <!-- KG Weight -->
 <schema:weight>
  <gs1:QuantitativeValue rdf:about="#quarterKegWeightKG">
   <rdf:type rdf:resource="http://qudt.org/1.1/schema/qudt#QuantityValue"/>
   <qudt:unit rdf:resource="http://www.qudt.org/2.1/vocab/unit/KiloGM"/>
   <qudt:numericalValue rdf:datatype="http://www.w3.org/2001/XMLSchema#double">11.3</qudt:numericalValue>
   <rdf:value rdf:datatype="http://www.w3.org/2001/XMLSchema#double">11.3</rdf:value>
   <gs1:unitCode>KGM</gs1:unitCode>
   <gs1:value>11.3</gs1:value>
   <rdfs:isDefinedBy rdf:resource="https://rdf.ag/o/beer-ONTOLOGY_DATE"/>
   <void:inDataset rdf:resource="#datasetdefinition"/>
  </gs1:QuantitativeValue>
 </schema:weight>
 <sosa:isFeatureOfInterestOf>
  <rdf:Description rdf:about="#quarterKegWeightSosaKG">
   <rdf:type rdf:resource="http://www.w3.org/ns/sosa/Observation"/>
   <sosa:hasFeatureOfInterest rdf:resource="#quarterKeg"/>
   <sosa:observedProperty  rdf:resource="#grossWeight"/>
   <sosa:hasResult rdf:resource="#quarterKegWeightKG"/>
   <sosa:hasSimpleResult rdf:datatype="http://www.qudt.org/2.1/vocab/unit/KiloGM">11.3</sosa:hasSimpleResult>
   <rdfs:isDefinedBy rdf:resource="https://rdf.ag/o/beer-ONTOLOGY_DATE"/>
   <void:inDataset rdf:resource="#datasetdefinition"/>
  </rdf:Description>
 </sosa:isFeatureOfInterestOf>
 <!-- LB Weight -->
 <schema:weight>
  <gs1:QuantitativeValue rdf:about="#quarterKegWeightLB">
   <rdf:type rdf:resource="http://qudt.org/1.1/schema/qudt#QuantityValue"/>
   <qudt:unit rdf:resource="http://www.qudt.org/2.1/vocab/unit/LB"/>
   <qudt:numericalValue rdf:datatype="http://www.w3.org/2001/XMLSchema#double">25.0</qudt:numericalValue>
   <rdf:value rdf:datatype="http://www.w3.org/2001/XMLSchema#double">25.0</rdf:value>
   <gs1:unitCode>lbm</gs1:unitCode>
   <gs1:value>25.0</gs1:value>
   <rdfs:isDefinedBy rdf:resource="https://rdf.ag/o/beer-ONTOLOGY_DATE"/>
   <void:inDataset rdf:resource="#datasetdefinition"/>
  </gs1:QuantitativeValue>
 </schema:weight>
 <sosa:isFeatureOfInterestOf>
  <rdf:Description rdf:about="#quarterKegWeightSosaLB">
   <rdf:type rdf:resource="http://www.w3.org/ns/sosa/Observation"/>
   <sosa:hasFeatureOfInterest rdf:resource="#quarterKeg"/>
   <sosa:observedProperty  rdf:resource="#grossWeight"/>
   <sosa:hasResult rdf:resource="#quarterKegWeightLB"/>
   <sosa:hasSimpleResult rdf:datatype="http://www.qudt.org/2.1/vocab/unit/LB">25.0</sosa:hasSimpleResult>
   <rdfs:isDefinedBy rdf:resource="https://rdf.ag/o/beer-ONTOLOGY_DATE"/>
   <void:inDataset rdf:resource="#datasetdefinition"/>
  </rdf:Description>
 </sosa:isFeatureOfInterestOf>
 <rdfs:isDefinedBy rdf:resource="https://rdf.ag/o/beer-ONTOLOGY_DATE"/>
 <void:inDataset rdf:resource="#datasetdefinition"/>
</rdf:Description>
<rdf:Description rdf:about="#halfBarrelKeg">
 <rdf:type rdf:resource="#LiquidContainer"/>
 <rdf:type rdf:resource="#Keg"/>
 <rdf:type rdf:resource="https://gs1.org/voc/PackagingDetails"/>
 <rdfs:label xml:lang="en">Half Barrel Keg</rdfs:label>
 <rdfs:label xml:lang="fr">Demi Fût</rdfs:label>
 <skos:definition xml:lang="en">Half Barrel Keg</skos:definition>
 <skos:definition xml:lang="fr">Demi Fût</skos:definition>
 <beer:nominalCapacity rdf:datatype="http://www.qudt.org/2.1/vocab/unit/MilliL">58600</beer:nominalCapacity>
 <sosa:isFeatureOfInterestOf>
  <rdf:Description rdf:about="#halfBarrelKegContentSosaML">
   <rdf:type rdf:resource="http://www.w3.org/ns/sosa/Observation"/>
   <sosa:hasFeatureOfInterest rdf:resource="#halfBarrelKeg"/>
   <sosa:observedProperty rdf:resource="#sosaNominalCapacity"/>
   <sosa:hasResult>
    <gs1:QuantitativeValue rdf:about="#halfBarrelKegContentML">
     <rdf:type rdf:resource="http://qudt.org/1.1/schema/qudt#QuantityValue"/>
     <gs1:unitCode>MLT</gs1:unitCode>
     <gs1:value>58600</gs1:value>
     <rdf:value rdf:datatype="http://www.w3.org/2001/XMLSchema#double">58600</rdf:value>
     <qudt:unit rdf:resource="http://www.qudt.org/2.1/vocab/unit/MilliL"/>
     <qudt:numericalValue rdf:datatype="http://www.w3.org/2001/XMLSchema#double">58600</qudt:numericalValue>
     <rdfs:isDefinedBy rdf:resource="https://rdf.ag/o/beer-ONTOLOGY_DATE"/>
     <void:inDataset rdf:resource="#datasetdefinition"/>
    </gs1:QuantitativeValue>
   </sosa:hasResult> 
   <sosa:hasSimpleResult rdf:datatype="http://www.qudt.org/2.1/vocab/unit/MilliM">58600</sosa:hasSimpleResult>
   <rdfs:isDefinedBy rdf:resource="https://rdf.ag/o/beer-ONTOLOGY_DATE"/>
   <void:inDataset rdf:resource="#datasetdefinition"/>
  </rdf:Description>
 </sosa:isFeatureOfInterestOf>
 <sosa:isFeatureOfInterestOf>
  <rdf:Description rdf:about="#halfBarrelKegContentSosaOZ">
   <rdf:type rdf:resource="http://www.w3.org/ns/sosa/Observation"/>
   <sosa:hasFeatureOfInterest rdf:resource="#halfBarrelKeg"/>
   <sosa:observedProperty rdf:resource="#sosaNominalCapacity"/>
   <sosa:hasResult>
   <gs1:QuantitativeValue rdf:about="#halfBarrelKegContentOZ">
    <rdf:type rdf:resource="http://qudt.org/1.1/schema/qudt#QuantityValue"/>
    <gs1:unitCode>foz_us</gs1:unitCode>
    <gs1:value>1981</gs1:value>
    <rdf:value rdf:datatype="http://www.w3.org/2001/XMLSchema#double">1981</rdf:value>
    <qudt:unit rdf:resource="http://www.qudt.org/2.1/vocab/unit/OZ_VOL_US"/>
    <qudt:numericalValue rdf:datatype="http://www.w3.org/2001/XMLSchema#double">1981</qudt:numericalValue>
    <rdfs:isDefinedBy rdf:resource="https://rdf.ag/o/beer-ONTOLOGY_DATE"/>
    <void:inDataset rdf:resource="#datasetdefinition"/>  
   </gs1:QuantitativeValue>
   </sosa:hasResult>
   <sosa:hasSimpleResult rdf:datatype="http://www.qudt.org/2.1/vocab/unit/OZ_VOL_US">1981</sosa:hasSimpleResult>
   <rdfs:isDefinedBy rdf:resource="https://rdf.ag/o/beer-ONTOLOGY_DATE"/>
   <void:inDataset rdf:resource="#datasetdefinition"/>  
 </rdf:Description>
 </sosa:isFeatureOfInterestOf>
 <!-- Net Content Gal -->
 <sosa:isFeatureOfInterestOf>
  <rdf:Description rdf:about="#halfBarrelKegContentSosaGAL">
   <rdf:type rdf:resource="http://www.w3.org/ns/sosa/Observation"/>
   <sosa:hasFeatureOfInterest rdf:resource="#halfBarrelKeg"/>
   <sosa:observedProperty rdf:resource="#netcontent"/>
   <sosa:hasResult>
    <gs1:QuantitativeValue rdf:about="#halfBarrelKegContentGal">
     <rdf:type rdf:resource="http://qudt.org/1.1/schema/qudt#QuantityValue"/>
     <gs1:unitCode>gal_us</gs1:unitCode>
     <gs1:value>15.47</gs1:value>
     <rdf:value rdf:datatype="http://www.w3.org/2001/XMLSchema#double">15.47</rdf:value>
     <qudt:unit rdf:resource="http://www.qudt.org/2.1/vocab/unit/GAL_US"/>
     <qudt:numericalValue rdf:datatype="http://www.w3.org/2001/XMLSchema#double">15.47</qudt:numericalValue>
     <rdfs:isDefinedBy rdf:resource="https://rdf.ag/o/beer-ONTOLOGY_DATE"/>
     <void:inDataset rdf:resource="#datasetdefinition"/>  
    </gs1:QuantitativeValue>
   </sosa:hasResult>
   <sosa:hasSimpleResult rdf:datatype="http://www.qudt.org/2.1/vocab/unit/GAL_US">15.47</sosa:hasSimpleResult>
   <rdfs:isDefinedBy rdf:resource="https://rdf.ag/o/beer-ONTOLOGY_DATE"/>
   <void:inDataset rdf:resource="#datasetdefinition"/>  
 </rdf:Description>
 </sosa:isFeatureOfInterestOf>

 <!-- Height MM-->
 <gs1:inPackageHeight>
  <gs1:QuantitativeValue rdf:about="#halfBarrelKegHeightMM">
   <rdf:type rdf:resource="http://qudt.org/1.1/schema/qudt#QuantityValue"/>
   <qudt:unit rdf:resource="http://www.qudt.org/2.1/vocab/unit/MilliM"/>
   <qudt:numericalValue rdf:datatype="http://www.w3.org/2001/XMLSchema#double">592</qudt:numericalValue>
   <rdf:value rdf:datatype="http://www.w3.org/2001/XMLSchema#double">592</rdf:value>
   <gs1:unitCode>MMT</gs1:unitCode>
   <gs1:value>592</gs1:value>
   <rdfs:isDefinedBy rdf:resource="https://rdf.ag/o/beer-ONTOLOGY_DATE"/>
   <void:inDataset rdf:resource="#datasetdefinition"/>
  </gs1:QuantitativeValue>
 </gs1:inPackageHeight>  
 <sosa:isFeatureOfInterestOf>
  <rdf:Description rdf:about="#halfBarrelKegHeightSosaMM">
   <rdf:type rdf:resource="http://www.w3.org/ns/sosa/Observation"/>
   <sosa:hasFeatureOfInterest rdf:resource="#halfBarrelKeg"/>
   <sosa:observedProperty  rdf:resource="#height"/>
   <sosa:hasResult rdf:resource="#halfBarrelKegHeightMM"/>
   <sosa:hasSimpleResult rdf:datatype="http://www.qudt.org/2.1/vocab/unit/MilliM">592</sosa:hasSimpleResult>
   <rdfs:isDefinedBy rdf:resource="https://rdf.ag/o/beer-ONTOLOGY_DATE"/>
   <void:inDataset rdf:resource="#datasetdefinition"/>
  </rdf:Description>
 </sosa:isFeatureOfInterestOf>
 <!-- Height IN-->
 <gs1:inPackageHeight>
  <gs1:QuantitativeValue rdf:about="#halfBarrelKegHeightIN">
   <rdf:type rdf:resource="http://qudt.org/1.1/schema/qudt#QuantityValue"/>
   <qudt:unit rdf:resource="http://www.qudt.org/2.1/vocab/unit/IN"/>
   <qudt:numericalValue rdf:datatype="http://www.w3.org/2001/XMLSchema#double">23.300</qudt:numericalValue>
   <rdf:value rdf:datatype="http://www.w3.org/2001/XMLSchema#double">23.300</rdf:value>
   <gs1:unitCode>INH</gs1:unitCode>
   <gs1:value>23.300</gs1:value>
   <rdfs:isDefinedBy rdf:resource="https://rdf.ag/o/beer-ONTOLOGY_DATE"/>
   <void:inDataset rdf:resource="#datasetdefinition"/>
  </gs1:QuantitativeValue>
 </gs1:inPackageHeight>  
 <sosa:isFeatureOfInterestOf>
  <rdf:Description rdf:about="#halfBarrelKegHeightSosaIN">
   <rdf:type rdf:resource="http://www.w3.org/ns/sosa/Observation"/>
   <sosa:hasFeatureOfInterest rdf:resource="#halfBarrelKeg"/>
   <sosa:observedProperty  rdf:resource="#height"/>
   <sosa:hasResult rdf:resource="#halfBarrelKegHeightIN"/>
   <sosa:hasSimpleResult rdf:datatype="http://www.qudt.org/2.1/vocab/unit/IN">23.300</sosa:hasSimpleResult>
   <rdfs:isDefinedBy rdf:resource="https://rdf.ag/o/beer-ONTOLOGY_DATE"/>
   <void:inDataset rdf:resource="#datasetdefinition"/>
  </rdf:Description>
 </sosa:isFeatureOfInterestOf>
 <!-- Diameter MM --> 
 <gs1:inPackageDiameter>
  <gs1:QuantitativeValue rdf:about="#halfBarrelKegDiameterMM">
   <rdf:type rdf:resource="http://qudt.org/1.1/schema/qudt#QuantityValue"/>
   <qudt:unit rdf:resource="http://www.qudt.org/2.1/vocab/unit/MilliM"/>
   <qudt:numericalValue rdf:datatype="http://www.w3.org/2001/XMLSchema#double">409</qudt:numericalValue>
   <rdf:value rdf:datatype="http://www.w3.org/2001/XMLSchema#double">409</rdf:value>
   <gs1:unitCode>MMT</gs1:unitCode>
   <gs1:value>409</gs1:value>
   <rdfs:isDefinedBy rdf:resource="https://rdf.ag/o/beer-ONTOLOGY_DATE"/>
   <void:inDataset rdf:resource="#datasetdefinition"/>
  </gs1:QuantitativeValue>
 </gs1:inPackageDiameter>
 <sosa:isFeatureOfInterestOf>
  <rdf:Description rdf:about="#halfBarrelKegDiameterSosaMM">
   <rdf:type rdf:resource="http://www.w3.org/ns/sosa/Observation"/>
   <sosa:hasFeatureOfInterest rdf:resource="#halfBarrelKeg"/>
   <sosa:observedProperty  rdf:resource="#diameter"/>
   <sosa:hasResult rdf:resource="#halfBarrelKegDiameterMM"/>
   <sosa:hasSimpleResult rdf:datatype="http://www.qudt.org/2.1/vocab/unit/MilliM">409</sosa:hasSimpleResult>
   <rdfs:isDefinedBy rdf:resource="https://rdf.ag/o/beer-ONTOLOGY_DATE"/>
   <void:inDataset rdf:resource="#datasetdefinition"/>
  </rdf:Description>
 </sosa:isFeatureOfInterestOf>
 <!-- Diameter IN --> 
 <gs1:inPackageDiameter>
  <gs1:QuantitativeValue rdf:about="#halfBarrelKegDiameterIN">
   <rdf:type rdf:resource="http://qudt.org/1.1/schema/qudt#QuantityValue"/>
   <qudt:unit rdf:resource="http://www.qudt.org/2.1/vocab/unit/IN"/>
   <qudt:numericalValue rdf:datatype="http://www.w3.org/2001/XMLSchema#double">16.120</qudt:numericalValue>
   <rdf:value rdf:datatype="http://www.w3.org/2001/XMLSchema#double">16.120</rdf:value>
   <gs1:unitCode>INH</gs1:unitCode>
   <gs1:value>16.120</gs1:value>
   <rdfs:isDefinedBy rdf:resource="https://rdf.ag/o/beer-ONTOLOGY_DATE"/>
   <void:inDataset rdf:resource="#datasetdefinition"/>
  </gs1:QuantitativeValue>
 </gs1:inPackageDiameter>
 <sosa:isFeatureOfInterestOf>
  <rdf:Description rdf:about="#halfBarrelKegDiameterSosaIN">
   <rdf:type rdf:resource="http://www.w3.org/ns/sosa/Observation"/>
   <sosa:hasFeatureOfInterest rdf:resource="#halfBarrelKeg"/>
   <sosa:observedProperty  rdf:resource="#diameter"/>
   <sosa:hasResult rdf:resource="#halfBarrelKegDiameterIN"/>
   <sosa:hasSimpleResult rdf:datatype="http://www.qudt.org/2.1/vocab/unit/IN">16.120</sosa:hasSimpleResult>
   <rdfs:isDefinedBy rdf:resource="https://rdf.ag/o/beer-ONTOLOGY_DATE"/>
   <void:inDataset rdf:resource="#datasetdefinition"/>
  </rdf:Description>
 </sosa:isFeatureOfInterestOf>
 <!-- KG Weight -->
 <schema:weight>
  <gs1:QuantitativeValue rdf:about="#halfBarrelKegWeightKG">
   <rdf:type rdf:resource="http://qudt.org/1.1/schema/qudt#QuantityValue"/>
   <qudt:unit rdf:resource="http://www.qudt.org/2.1/vocab/unit/KiloGM"/>
   <qudt:numericalValue rdf:datatype="http://www.w3.org/2001/XMLSchema#double">13.6</qudt:numericalValue>
   <rdf:value rdf:datatype="http://www.w3.org/2001/XMLSchema#double">13.6</rdf:value>
   <gs1:unitCode>KGM</gs1:unitCode>
   <gs1:value>13.6</gs1:value>
   <rdfs:isDefinedBy rdf:resource="https://rdf.ag/o/beer-ONTOLOGY_DATE"/>
   <void:inDataset rdf:resource="#datasetdefinition"/>
  </gs1:QuantitativeValue>
 </schema:weight>
 <sosa:isFeatureOfInterestOf>
  <rdf:Description rdf:about="#halfBarrelKegWeightSosaKG">
   <rdf:type rdf:resource="http://www.w3.org/ns/sosa/Observation"/>
   <sosa:hasFeatureOfInterest rdf:resource="#halfBarrelKeg"/>
   <sosa:observedProperty  rdf:resource="#grossWeight"/>
   <sosa:hasResult rdf:resource="#halfBarrelKegWeightKG"/>
   <sosa:hasSimpleResult rdf:datatype="http://www.qudt.org/2.1/vocab/unit/KiloGM">13.6</sosa:hasSimpleResult>
   <rdfs:isDefinedBy rdf:resource="https://rdf.ag/o/beer-ONTOLOGY_DATE"/>
   <void:inDataset rdf:resource="#datasetdefinition"/>
  </rdf:Description>
 </sosa:isFeatureOfInterestOf>
 <!-- LB Weight -->
 <schema:weight>
  <gs1:QuantitativeValue rdf:about="#halfBarrelKegWeightLB">
   <rdf:type rdf:resource="http://qudt.org/1.1/schema/qudt#QuantityValue"/>
   <qudt:unit rdf:resource="http://www.qudt.org/2.1/vocab/unit/LB"/>
   <qudt:numericalValue rdf:datatype="http://www.w3.org/2001/XMLSchema#double">30.0</qudt:numericalValue>
   <rdf:value rdf:datatype="http://www.w3.org/2001/XMLSchema#double">30.0</rdf:value>
   <gs1:unitCode>lbm</gs1:unitCode>
   <gs1:value>30.0</gs1:value>
   <rdfs:isDefinedBy rdf:resource="https://rdf.ag/o/beer-ONTOLOGY_DATE"/>
   <void:inDataset rdf:resource="#datasetdefinition"/>
  </gs1:QuantitativeValue>
 </schema:weight>
 <sosa:isFeatureOfInterestOf>
  <rdf:Description rdf:about="#halfBarrelKegWeightSosaLB">
   <rdf:type rdf:resource="http://www.w3.org/ns/sosa/Observation"/>
   <sosa:hasFeatureOfInterest rdf:resource="#halfBarrelKeg"/>
   <sosa:observedProperty  rdf:resource="#grossWeight"/>
   <sosa:hasResult rdf:resource="#halfBarrelKegWeightLB"/>
   <sosa:hasSimpleResult rdf:datatype="http://www.qudt.org/2.1/vocab/unit/LB">30.0</sosa:hasSimpleResult>
   <rdfs:isDefinedBy rdf:resource="https://rdf.ag/o/beer-ONTOLOGY_DATE"/>
   <void:inDataset rdf:resource="#datasetdefinition"/>
  </rdf:Description>
 </sosa:isFeatureOfInterestOf>
 <rdfs:isDefinedBy rdf:resource="https://rdf.ag/o/beer-ONTOLOGY_DATE"/>
 <void:inDataset rdf:resource="#datasetdefinition"/>
</rdf:Description>
<rdf:Description rdf:about="#D201">
 <rdf:type rdf:resource="#LiquidContainer"/>
 <rdf:type rdf:resource="#Keg"/>
 <rdf:type rdf:resource="https://gs1.org/voc/PackagingDetails"/>
 <rdfs:label xml:lang="en">German DIN201</rdfs:label>
 <rdfs:label xml:lang="fr">Fût DIN201</rdfs:label>
 <skos:definition xml:lang="en">German DIN201</skos:definition>
 <skos:definition xml:lang="fr">Fût DIN201</skos:definition>
 <skos:altLabel xml:lang="en">DIN201</skos:altLabel>
 <beer:nominalCapacity rdf:datatype="http://www.qudt.org/2.1/vocab/unit/MilliL">20200</beer:nominalCapacity>
 <sosa:isFeatureOfInterestOf>
  <rdf:Description rdf:about="#D201ContentSosaML">
   <rdf:type rdf:resource="http://www.w3.org/ns/sosa/Observation"/>
   <sosa:hasFeatureOfInterest rdf:resource="#D201"/>
   <sosa:observedProperty rdf:resource="#sosaNominalCapacity"/>
   <sosa:hasResult>
    <gs1:QuantitativeValue rdf:about="#D201ContentML">
     <rdf:type rdf:resource="http://qudt.org/1.1/schema/qudt#QuantityValue"/>
     <gs1:unitCode>MLT</gs1:unitCode>
     <gs1:value>20200</gs1:value>
     <rdf:value rdf:datatype="http://www.w3.org/2001/XMLSchema#double">20200</rdf:value>
     <qudt:unit rdf:resource="http://www.qudt.org/2.1/vocab/unit/MilliL"/>
     <qudt:numericalValue rdf:datatype="http://www.w3.org/2001/XMLSchema#double">20200</qudt:numericalValue>
     <rdfs:isDefinedBy rdf:resource="https://rdf.ag/o/beer-ONTOLOGY_DATE"/>
     <void:inDataset rdf:resource="#datasetdefinition"/>
    </gs1:QuantitativeValue>
   </sosa:hasResult> 
   <sosa:hasSimpleResult rdf:datatype="http://www.qudt.org/2.1/vocab/unit/MilliM">20200</sosa:hasSimpleResult>
   <rdfs:isDefinedBy rdf:resource="https://rdf.ag/o/beer-ONTOLOGY_DATE"/>
   <void:inDataset rdf:resource="#datasetdefinition"/>
  </rdf:Description>
 </sosa:isFeatureOfInterestOf>
 <sosa:isFeatureOfInterestOf>
  <rdf:Description rdf:about="#D201ContentSosaOZ">
   <rdf:type rdf:resource="http://www.w3.org/ns/sosa/Observation"/>
   <sosa:hasFeatureOfInterest rdf:resource="#D201"/>
   <sosa:observedProperty rdf:resource="#sosaNominalCapacity"/>
   <sosa:hasResult>
   <gs1:QuantitativeValue rdf:about="#D201ContentOZ">
    <rdf:type rdf:resource="http://qudt.org/1.1/schema/qudt#QuantityValue"/>
    <gs1:unitCode>foz_us</gs1:unitCode>
    <gs1:value>676</gs1:value>
    <rdf:value rdf:datatype="http://www.w3.org/2001/XMLSchema#double">676</rdf:value>
    <qudt:unit rdf:resource="http://www.qudt.org/2.1/vocab/unit/OZ_VOL_US"/>
    <qudt:numericalValue rdf:datatype="http://www.w3.org/2001/XMLSchema#double">676</qudt:numericalValue>
    <rdfs:isDefinedBy rdf:resource="https://rdf.ag/o/beer-ONTOLOGY_DATE"/>
    <void:inDataset rdf:resource="#datasetdefinition"/>  
   </gs1:QuantitativeValue>
   </sosa:hasResult>
   <sosa:hasSimpleResult rdf:datatype="http://www.qudt.org/2.1/vocab/unit/OZ_VOL_US">676</sosa:hasSimpleResult>
   <rdfs:isDefinedBy rdf:resource="https://rdf.ag/o/beer-ONTOLOGY_DATE"/>
   <void:inDataset rdf:resource="#datasetdefinition"/>  
 </rdf:Description>
 </sosa:isFeatureOfInterestOf>
 <!-- Net Content Gal -->
 <sosa:isFeatureOfInterestOf>
  <rdf:Description rdf:about="#D201ContentSosaGAL">
   <rdf:type rdf:resource="http://www.w3.org/ns/sosa/Observation"/>
   <sosa:hasFeatureOfInterest rdf:resource="#D201"/>
   <sosa:observedProperty rdf:resource="#netcontent"/>
   <sosa:hasResult>
    <gs1:QuantitativeValue rdf:about="#D201ContentGal">
     <rdf:type rdf:resource="http://qudt.org/1.1/schema/qudt#QuantityValue"/>
     <gs1:unitCode>gal_us</gs1:unitCode>
     <gs1:value>5.28</gs1:value>
     <rdf:value rdf:datatype="http://www.w3.org/2001/XMLSchema#double">5.28</rdf:value>
     <qudt:unit rdf:resource="http://www.qudt.org/2.1/vocab/unit/GAL_US"/>
     <qudt:numericalValue rdf:datatype="http://www.w3.org/2001/XMLSchema#double">5.28</qudt:numericalValue>
     <rdfs:isDefinedBy rdf:resource="https://rdf.ag/o/beer-ONTOLOGY_DATE"/>
     <void:inDataset rdf:resource="#datasetdefinition"/>  
    </gs1:QuantitativeValue>
   </sosa:hasResult>
   <sosa:hasSimpleResult rdf:datatype="http://www.qudt.org/2.1/vocab/unit/GAL_US">5.28</sosa:hasSimpleResult>
   <rdfs:isDefinedBy rdf:resource="https://rdf.ag/o/beer-ONTOLOGY_DATE"/>
   <void:inDataset rdf:resource="#datasetdefinition"/>  
 </rdf:Description>
 </sosa:isFeatureOfInterestOf>

 <!-- Height MM-->
 <gs1:inPackageHeight>
  <gs1:QuantitativeValue rdf:about="#D201HeightMM">
   <rdf:type rdf:resource="http://qudt.org/1.1/schema/qudt#QuantityValue"/>
   <qudt:unit rdf:resource="http://www.qudt.org/2.1/vocab/unit/MilliM"/>
   <qudt:numericalValue rdf:datatype="http://www.w3.org/2001/XMLSchema#double">310</qudt:numericalValue>
   <rdf:value rdf:datatype="http://www.w3.org/2001/XMLSchema#double">310</rdf:value>
   <gs1:unitCode>MMT</gs1:unitCode>
   <gs1:value>310</gs1:value>
   <rdfs:isDefinedBy rdf:resource="https://rdf.ag/o/beer-ONTOLOGY_DATE"/>
   <void:inDataset rdf:resource="#datasetdefinition"/>
  </gs1:QuantitativeValue>
 </gs1:inPackageHeight>  
 <sosa:isFeatureOfInterestOf>
  <rdf:Description rdf:about="#D201HeightSosaMM">
   <rdf:type rdf:resource="http://www.w3.org/ns/sosa/Observation"/>
   <sosa:hasFeatureOfInterest rdf:resource="#D201"/>
   <sosa:observedProperty  rdf:resource="#height"/>
   <sosa:hasResult rdf:resource="#D201HeightMM"/>
   <sosa:hasSimpleResult rdf:datatype="http://www.qudt.org/2.1/vocab/unit/MilliM">310</sosa:hasSimpleResult>
   <rdfs:isDefinedBy rdf:resource="https://rdf.ag/o/beer-ONTOLOGY_DATE"/>
   <void:inDataset rdf:resource="#datasetdefinition"/>
  </rdf:Description>
 </sosa:isFeatureOfInterestOf>
 <!-- Height IN-->
 <gs1:inPackageHeight>
  <gs1:QuantitativeValue rdf:about="#D201HeightIN">
   <rdf:type rdf:resource="http://qudt.org/1.1/schema/qudt#QuantityValue"/>
   <qudt:unit rdf:resource="http://www.qudt.org/2.1/vocab/unit/IN"/>
   <qudt:numericalValue rdf:datatype="http://www.w3.org/2001/XMLSchema#double">12.205</qudt:numericalValue>
   <rdf:value rdf:datatype="http://www.w3.org/2001/XMLSchema#double">12.205</rdf:value>
   <gs1:unitCode>INH</gs1:unitCode>
   <gs1:value>12.205</gs1:value>
   <rdfs:isDefinedBy rdf:resource="https://rdf.ag/o/beer-ONTOLOGY_DATE"/>
   <void:inDataset rdf:resource="#datasetdefinition"/>
  </gs1:QuantitativeValue>
 </gs1:inPackageHeight>  
 <sosa:isFeatureOfInterestOf>
  <rdf:Description rdf:about="#D201HeightSosaIN">
   <rdf:type rdf:resource="http://www.w3.org/ns/sosa/Observation"/>
   <sosa:hasFeatureOfInterest rdf:resource="#D201"/>
   <sosa:observedProperty  rdf:resource="#height"/>
   <sosa:hasResult rdf:resource="#D201HeightIN"/>
   <sosa:hasSimpleResult rdf:datatype="http://www.qudt.org/2.1/vocab/unit/IN">12.205</sosa:hasSimpleResult>
   <rdfs:isDefinedBy rdf:resource="https://rdf.ag/o/beer-ONTOLOGY_DATE"/>
   <void:inDataset rdf:resource="#datasetdefinition"/>
  </rdf:Description>
 </sosa:isFeatureOfInterestOf>
 <!-- Diameter MM --> 
 <gs1:inPackageDiameter>
  <gs1:QuantitativeValue rdf:about="#D201DiameterMM">
   <rdf:type rdf:resource="http://qudt.org/1.1/schema/qudt#QuantityValue"/>
   <qudt:unit rdf:resource="http://www.qudt.org/2.1/vocab/unit/MilliM"/>
   <qudt:numericalValue rdf:datatype="http://www.w3.org/2001/XMLSchema#double">363</qudt:numericalValue>
   <rdf:value rdf:datatype="http://www.w3.org/2001/XMLSchema#double">363</rdf:value>
   <gs1:unitCode>MMT</gs1:unitCode>
   <gs1:value>363</gs1:value>
   <rdfs:isDefinedBy rdf:resource="https://rdf.ag/o/beer-ONTOLOGY_DATE"/>
   <void:inDataset rdf:resource="#datasetdefinition"/>
  </gs1:QuantitativeValue>
 </gs1:inPackageDiameter>
 <sosa:isFeatureOfInterestOf>
  <rdf:Description rdf:about="#D201DiameterSosaMM">
   <rdf:type rdf:resource="http://www.w3.org/ns/sosa/Observation"/>
   <sosa:hasFeatureOfInterest rdf:resource="#D201"/>
   <sosa:observedProperty  rdf:resource="#diameter"/>
   <sosa:hasResult rdf:resource="#D201DiameterMM"/>
   <sosa:hasSimpleResult rdf:datatype="http://www.qudt.org/2.1/vocab/unit/MilliM">363</sosa:hasSimpleResult>
   <rdfs:isDefinedBy rdf:resource="https://rdf.ag/o/beer-ONTOLOGY_DATE"/>
   <void:inDataset rdf:resource="#datasetdefinition"/>
  </rdf:Description>
 </sosa:isFeatureOfInterestOf>
 <!-- Diameter IN --> 
 <gs1:inPackageDiameter>
  <gs1:QuantitativeValue rdf:about="#D201DiameterIN">
   <rdf:type rdf:resource="http://qudt.org/1.1/schema/qudt#QuantityValue"/>
   <qudt:unit rdf:resource="http://www.qudt.org/2.1/vocab/unit/IN"/>
   <qudt:numericalValue rdf:datatype="http://www.w3.org/2001/XMLSchema#double">14.291</qudt:numericalValue>
   <rdf:value rdf:datatype="http://www.w3.org/2001/XMLSchema#double">14.291</rdf:value>
   <gs1:unitCode>INH</gs1:unitCode>
   <gs1:value>14.291</gs1:value>
   <rdfs:isDefinedBy rdf:resource="https://rdf.ag/o/beer-ONTOLOGY_DATE"/>
   <void:inDataset rdf:resource="#datasetdefinition"/>
  </gs1:QuantitativeValue>
 </gs1:inPackageDiameter>
 <sosa:isFeatureOfInterestOf>
  <rdf:Description rdf:about="#D201DiameterSosaIN">
   <rdf:type rdf:resource="http://www.w3.org/ns/sosa/Observation"/>
   <sosa:hasFeatureOfInterest rdf:resource="#D201"/>
   <sosa:observedProperty  rdf:resource="#diameter"/>
   <sosa:hasResult rdf:resource="#D201DiameterIN"/>
   <sosa:hasSimpleResult rdf:datatype="http://www.qudt.org/2.1/vocab/unit/IN">14.291</sosa:hasSimpleResult>
   <rdfs:isDefinedBy rdf:resource="https://rdf.ag/o/beer-ONTOLOGY_DATE"/>
   <void:inDataset rdf:resource="#datasetdefinition"/>
  </rdf:Description>
 </sosa:isFeatureOfInterestOf>
 <!-- KG Weight -->
 <schema:weight>
  <gs1:QuantitativeValue rdf:about="#D201WeightKG">
   <rdf:type rdf:resource="http://qudt.org/1.1/schema/qudt#QuantityValue"/>
   <qudt:unit rdf:resource="http://www.qudt.org/2.1/vocab/unit/KiloGM"/>
   <qudt:numericalValue rdf:datatype="http://www.w3.org/2001/XMLSchema#double">7.3</qudt:numericalValue>
   <rdf:value rdf:datatype="http://www.w3.org/2001/XMLSchema#double">7.3</rdf:value>
   <gs1:unitCode>KGM</gs1:unitCode>
   <gs1:value>7.3</gs1:value>
   <rdfs:isDefinedBy rdf:resource="https://rdf.ag/o/beer-ONTOLOGY_DATE"/>
   <void:inDataset rdf:resource="#datasetdefinition"/>
  </gs1:QuantitativeValue>
 </schema:weight>
 <sosa:isFeatureOfInterestOf>
  <rdf:Description rdf:about="#D201WeightSosaKG">
   <rdf:type rdf:resource="http://www.w3.org/ns/sosa/Observation"/>
   <sosa:hasFeatureOfInterest rdf:resource="#D201"/>
   <sosa:observedProperty  rdf:resource="#grossWeight"/>
   <sosa:hasResult rdf:resource="#D201WeightKG"/>
   <sosa:hasSimpleResult rdf:datatype="http://www.qudt.org/2.1/vocab/unit/KiloGM">7.3</sosa:hasSimpleResult>
   <rdfs:isDefinedBy rdf:resource="https://rdf.ag/o/beer-ONTOLOGY_DATE"/>
   <void:inDataset rdf:resource="#datasetdefinition"/>
  </rdf:Description>
 </sosa:isFeatureOfInterestOf>
 <!-- LB Weight -->
 <schema:weight>
  <gs1:QuantitativeValue rdf:about="#D201WeightLB">
   <rdf:type rdf:resource="http://qudt.org/1.1/schema/qudt#QuantityValue"/>
   <qudt:unit rdf:resource="http://www.qudt.org/2.1/vocab/unit/LB"/>
   <qudt:numericalValue rdf:datatype="http://www.w3.org/2001/XMLSchema#double">16.1</qudt:numericalValue>
   <rdf:value rdf:datatype="http://www.w3.org/2001/XMLSchema#double">16.1</rdf:value>
   <gs1:unitCode>lbm</gs1:unitCode>
   <gs1:value>16.1</gs1:value>
   <rdfs:isDefinedBy rdf:resource="https://rdf.ag/o/beer-ONTOLOGY_DATE"/>
   <void:inDataset rdf:resource="#datasetdefinition"/>
  </gs1:QuantitativeValue>
 </schema:weight>
 <sosa:isFeatureOfInterestOf>
  <rdf:Description rdf:about="#D201WeightSosaLB">
   <rdf:type rdf:resource="http://www.w3.org/ns/sosa/Observation"/>
   <sosa:hasFeatureOfInterest rdf:resource="#D201"/>
   <sosa:observedProperty  rdf:resource="#grossWeight"/>
   <sosa:hasResult rdf:resource="#D201WeightLB"/>
   <sosa:hasSimpleResult rdf:datatype="http://www.qudt.org/2.1/vocab/unit/LB">16.1</sosa:hasSimpleResult>
   <rdfs:isDefinedBy rdf:resource="https://rdf.ag/o/beer-ONTOLOGY_DATE"/>
   <void:inDataset rdf:resource="#datasetdefinition"/>
  </rdf:Description>
 </sosa:isFeatureOfInterestOf>
 <rdfs:isDefinedBy rdf:resource="https://rdf.ag/o/beer-ONTOLOGY_DATE"/>
 <void:inDataset rdf:resource="#datasetdefinition"/>
</rdf:Description>
<rdf:Description rdf:about="#D251">
 <rdf:type rdf:resource="#LiquidContainer"/>
 <rdf:type rdf:resource="#Keg"/>
 <rdf:type rdf:resource="https://gs1.org/voc/PackagingDetails"/>
 <rdfs:label xml:lang="en">German DIN251</rdfs:label>
 <rdfs:label xml:lang="fr">Fût DIN251</rdfs:label>
 <skos:definition xml:lang="en">German DIN251</skos:definition>
 <skos:definition xml:lang="fr">Fût DIN251</skos:definition>
 <skos:altLabel xml:lang="en">DIN251</skos:altLabel>
 <beer:nominalCapacity rdf:datatype="http://www.qudt.org/2.1/vocab/unit/MilliL">25200</beer:nominalCapacity>
 <sosa:isFeatureOfInterestOf>
  <rdf:Description rdf:about="#D251ContentSosaML">
   <rdf:type rdf:resource="http://www.w3.org/ns/sosa/Observation"/>
   <sosa:hasFeatureOfInterest rdf:resource="#D251"/>
   <sosa:observedProperty rdf:resource="#sosaNominalCapacity"/>
   <sosa:hasResult>
    <gs1:QuantitativeValue rdf:about="#D251ContentML">
     <rdf:type rdf:resource="http://qudt.org/1.1/schema/qudt#QuantityValue"/>
     <gs1:unitCode>MLT</gs1:unitCode>
     <gs1:value>25200</gs1:value>
     <rdf:value rdf:datatype="http://www.w3.org/2001/XMLSchema#double">25200</rdf:value>
     <qudt:unit rdf:resource="http://www.qudt.org/2.1/vocab/unit/MilliL"/>
     <qudt:numericalValue rdf:datatype="http://www.w3.org/2001/XMLSchema#double">25200</qudt:numericalValue>
     <rdfs:isDefinedBy rdf:resource="https://rdf.ag/o/beer-ONTOLOGY_DATE"/>
     <void:inDataset rdf:resource="#datasetdefinition"/>
    </gs1:QuantitativeValue>
   </sosa:hasResult> 
   <sosa:hasSimpleResult rdf:datatype="http://www.qudt.org/2.1/vocab/unit/MilliM">25200</sosa:hasSimpleResult>
   <rdfs:isDefinedBy rdf:resource="https://rdf.ag/o/beer-ONTOLOGY_DATE"/>
   <void:inDataset rdf:resource="#datasetdefinition"/>
  </rdf:Description>
 </sosa:isFeatureOfInterestOf>
 <sosa:isFeatureOfInterestOf>
  <rdf:Description rdf:about="#D251ContentSosaOZ">
   <rdf:type rdf:resource="http://www.w3.org/ns/sosa/Observation"/>
   <sosa:hasFeatureOfInterest rdf:resource="#D251"/>
   <sosa:observedProperty rdf:resource="#sosaNominalCapacity"/>
   <sosa:hasResult>
   <gs1:QuantitativeValue rdf:about="#D251ContentOZ">
    <rdf:type rdf:resource="http://qudt.org/1.1/schema/qudt#QuantityValue"/>
    <gs1:unitCode>foz_us</gs1:unitCode>
    <gs1:value>845</gs1:value>
    <rdf:value rdf:datatype="http://www.w3.org/2001/XMLSchema#double">845</rdf:value>
    <qudt:unit rdf:resource="http://www.qudt.org/2.1/vocab/unit/OZ_VOL_US"/>
    <qudt:numericalValue rdf:datatype="http://www.w3.org/2001/XMLSchema#double">845</qudt:numericalValue>
    <rdfs:isDefinedBy rdf:resource="https://rdf.ag/o/beer-ONTOLOGY_DATE"/>
    <void:inDataset rdf:resource="#datasetdefinition"/>  
   </gs1:QuantitativeValue>
   </sosa:hasResult>
   <sosa:hasSimpleResult rdf:datatype="http://www.qudt.org/2.1/vocab/unit/OZ_VOL_US">845</sosa:hasSimpleResult>
   <rdfs:isDefinedBy rdf:resource="https://rdf.ag/o/beer-ONTOLOGY_DATE"/>
   <void:inDataset rdf:resource="#datasetdefinition"/>  
 </rdf:Description>
 </sosa:isFeatureOfInterestOf>
 <!-- Net Content Gal -->
 <sosa:isFeatureOfInterestOf>
  <rdf:Description rdf:about="#D251ContentSosaGAL">
   <rdf:type rdf:resource="http://www.w3.org/ns/sosa/Observation"/>
   <sosa:hasFeatureOfInterest rdf:resource="#D251"/>
   <sosa:observedProperty rdf:resource="#netcontent"/>
   <sosa:hasResult>
    <gs1:QuantitativeValue rdf:about="#D251ContentGal">
     <rdf:type rdf:resource="http://qudt.org/1.1/schema/qudt#QuantityValue"/>
     <gs1:unitCode>gal_us</gs1:unitCode>
     <gs1:value>6.60</gs1:value>
     <rdf:value rdf:datatype="http://www.w3.org/2001/XMLSchema#double">6.60</rdf:value>
     <qudt:unit rdf:resource="http://www.qudt.org/2.1/vocab/unit/GAL_US"/>
     <qudt:numericalValue rdf:datatype="http://www.w3.org/2001/XMLSchema#double">6.60</qudt:numericalValue>
     <rdfs:isDefinedBy rdf:resource="https://rdf.ag/o/beer-ONTOLOGY_DATE"/>
     <void:inDataset rdf:resource="#datasetdefinition"/>  
    </gs1:QuantitativeValue>
   </sosa:hasResult>
   <sosa:hasSimpleResult rdf:datatype="http://www.qudt.org/2.1/vocab/unit/GAL_US">6.60</sosa:hasSimpleResult>
   <rdfs:isDefinedBy rdf:resource="https://rdf.ag/o/beer-ONTOLOGY_DATE"/>
   <void:inDataset rdf:resource="#datasetdefinition"/>  
 </rdf:Description>
 </sosa:isFeatureOfInterestOf>

 <!-- Height MM-->
 <gs1:inPackageHeight>
  <gs1:QuantitativeValue rdf:about="#D251HeightMM">
   <rdf:type rdf:resource="http://qudt.org/1.1/schema/qudt#QuantityValue"/>
   <qudt:unit rdf:resource="http://www.qudt.org/2.1/vocab/unit/MilliM"/>
   <qudt:numericalValue rdf:datatype="http://www.w3.org/2001/XMLSchema#double">360</qudt:numericalValue>
   <rdf:value rdf:datatype="http://www.w3.org/2001/XMLSchema#double">360</rdf:value>
   <gs1:unitCode>MMT</gs1:unitCode>
   <gs1:value>360</gs1:value>
   <rdfs:isDefinedBy rdf:resource="https://rdf.ag/o/beer-ONTOLOGY_DATE"/>
   <void:inDataset rdf:resource="#datasetdefinition"/>
  </gs1:QuantitativeValue>
 </gs1:inPackageHeight>  
 <sosa:isFeatureOfInterestOf>
  <rdf:Description rdf:about="#D251HeightSosaMM">
   <rdf:type rdf:resource="http://www.w3.org/ns/sosa/Observation"/>
   <sosa:hasFeatureOfInterest rdf:resource="#D251"/>
   <sosa:observedProperty  rdf:resource="#height"/>
   <sosa:hasResult rdf:resource="#D251HeightMM"/>
   <sosa:hasSimpleResult rdf:datatype="http://www.qudt.org/2.1/vocab/unit/MilliM">360</sosa:hasSimpleResult>
   <rdfs:isDefinedBy rdf:resource="https://rdf.ag/o/beer-ONTOLOGY_DATE"/>
   <void:inDataset rdf:resource="#datasetdefinition"/>
  </rdf:Description>
 </sosa:isFeatureOfInterestOf>
 <!-- Height IN-->
 <gs1:inPackageHeight>
  <gs1:QuantitativeValue rdf:about="#D251HeightIN">
   <rdf:type rdf:resource="http://qudt.org/1.1/schema/qudt#QuantityValue"/>
   <qudt:unit rdf:resource="http://www.qudt.org/2.1/vocab/unit/IN"/>
   <qudt:numericalValue rdf:datatype="http://www.w3.org/2001/XMLSchema#double">14.173</qudt:numericalValue>
   <rdf:value rdf:datatype="http://www.w3.org/2001/XMLSchema#double">14.173</rdf:value>
   <gs1:unitCode>INH</gs1:unitCode>
   <gs1:value>14.173</gs1:value>
   <rdfs:isDefinedBy rdf:resource="https://rdf.ag/o/beer-ONTOLOGY_DATE"/>
   <void:inDataset rdf:resource="#datasetdefinition"/>
  </gs1:QuantitativeValue>
 </gs1:inPackageHeight>  
 <sosa:isFeatureOfInterestOf>
  <rdf:Description rdf:about="#D251HeightSosaIN">
   <rdf:type rdf:resource="http://www.w3.org/ns/sosa/Observation"/>
   <sosa:hasFeatureOfInterest rdf:resource="#D251"/>
   <sosa:observedProperty  rdf:resource="#height"/>
   <sosa:hasResult rdf:resource="#D251HeightIN"/>
   <sosa:hasSimpleResult rdf:datatype="http://www.qudt.org/2.1/vocab/unit/IN">14.173</sosa:hasSimpleResult>
   <rdfs:isDefinedBy rdf:resource="https://rdf.ag/o/beer-ONTOLOGY_DATE"/>
   <void:inDataset rdf:resource="#datasetdefinition"/>
  </rdf:Description>
 </sosa:isFeatureOfInterestOf>
 <!-- Diameter MM --> 
 <gs1:inPackageDiameter>
  <gs1:QuantitativeValue rdf:about="#D251DiameterMM">
   <rdf:type rdf:resource="http://qudt.org/1.1/schema/qudt#QuantityValue"/>
   <qudt:unit rdf:resource="http://www.qudt.org/2.1/vocab/unit/MilliM"/>
   <qudt:numericalValue rdf:datatype="http://www.w3.org/2001/XMLSchema#double">363</qudt:numericalValue>
   <rdf:value rdf:datatype="http://www.w3.org/2001/XMLSchema#double">363</rdf:value>
   <gs1:unitCode>MMT</gs1:unitCode>
   <gs1:value>363</gs1:value>
   <rdfs:isDefinedBy rdf:resource="https://rdf.ag/o/beer-ONTOLOGY_DATE"/>
   <void:inDataset rdf:resource="#datasetdefinition"/>
  </gs1:QuantitativeValue>
 </gs1:inPackageDiameter>
 <sosa:isFeatureOfInterestOf>
  <rdf:Description rdf:about="#D251DiameterSosaMM">
   <rdf:type rdf:resource="http://www.w3.org/ns/sosa/Observation"/>
   <sosa:hasFeatureOfInterest rdf:resource="#D251"/>
   <sosa:observedProperty  rdf:resource="#diameter"/>
   <sosa:hasResult rdf:resource="#D251DiameterMM"/>
   <sosa:hasSimpleResult rdf:datatype="http://www.qudt.org/2.1/vocab/unit/MilliM">363</sosa:hasSimpleResult>
   <rdfs:isDefinedBy rdf:resource="https://rdf.ag/o/beer-ONTOLOGY_DATE"/>
   <void:inDataset rdf:resource="#datasetdefinition"/>
  </rdf:Description>
 </sosa:isFeatureOfInterestOf>
 <!-- Diameter IN --> 
 <gs1:inPackageDiameter>
  <gs1:QuantitativeValue rdf:about="#D251DiameterIN">
   <rdf:type rdf:resource="http://qudt.org/1.1/schema/qudt#QuantityValue"/>
   <qudt:unit rdf:resource="http://www.qudt.org/2.1/vocab/unit/IN"/>
   <qudt:numericalValue rdf:datatype="http://www.w3.org/2001/XMLSchema#double">14.291</qudt:numericalValue>
   <rdf:value rdf:datatype="http://www.w3.org/2001/XMLSchema#double">14.291</rdf:value>
   <gs1:unitCode>INH</gs1:unitCode>
   <gs1:value>14.291</gs1:value>
   <rdfs:isDefinedBy rdf:resource="https://rdf.ag/o/beer-ONTOLOGY_DATE"/>
   <void:inDataset rdf:resource="#datasetdefinition"/>
  </gs1:QuantitativeValue>
 </gs1:inPackageDiameter>
 <sosa:isFeatureOfInterestOf>
  <rdf:Description rdf:about="#D251DiameterSosaIN">
   <rdf:type rdf:resource="http://www.w3.org/ns/sosa/Observation"/>
   <sosa:hasFeatureOfInterest rdf:resource="#D251"/>
   <sosa:observedProperty  rdf:resource="#diameter"/>
   <sosa:hasResult rdf:resource="#D251DiameterIN"/>
   <sosa:hasSimpleResult rdf:datatype="http://www.qudt.org/2.1/vocab/unit/IN">14.291</sosa:hasSimpleResult>
   <rdfs:isDefinedBy rdf:resource="https://rdf.ag/o/beer-ONTOLOGY_DATE"/>
   <void:inDataset rdf:resource="#datasetdefinition"/>
  </rdf:Description>
 </sosa:isFeatureOfInterestOf>
 <!-- KG Weight -->
 <schema:weight>
  <gs1:QuantitativeValue rdf:about="#D251WeightKG">
   <rdf:type rdf:resource="http://qudt.org/1.1/schema/qudt#QuantityValue"/>
   <qudt:unit rdf:resource="http://www.qudt.org/2.1/vocab/unit/KiloGM"/>
   <qudt:numericalValue rdf:datatype="http://www.w3.org/2001/XMLSchema#double">8.5</qudt:numericalValue>
   <rdf:value rdf:datatype="http://www.w3.org/2001/XMLSchema#double">8.5</rdf:value>
   <gs1:unitCode>KGM</gs1:unitCode>
   <gs1:value>8.5</gs1:value>
   <rdfs:isDefinedBy rdf:resource="https://rdf.ag/o/beer-ONTOLOGY_DATE"/>
   <void:inDataset rdf:resource="#datasetdefinition"/>
  </gs1:QuantitativeValue>
 </schema:weight>
 <sosa:isFeatureOfInterestOf>
  <rdf:Description rdf:about="#D251WeightSosaKG">
   <rdf:type rdf:resource="http://www.w3.org/ns/sosa/Observation"/>
   <sosa:hasFeatureOfInterest rdf:resource="#D251"/>
   <sosa:observedProperty  rdf:resource="#grossWeight"/>
   <sosa:hasResult rdf:resource="#D251WeightKG"/>
   <sosa:hasSimpleResult rdf:datatype="http://www.qudt.org/2.1/vocab/unit/KiloGM">8.5</sosa:hasSimpleResult>
   <rdfs:isDefinedBy rdf:resource="https://rdf.ag/o/beer-ONTOLOGY_DATE"/>
   <void:inDataset rdf:resource="#datasetdefinition"/>
  </rdf:Description>
 </sosa:isFeatureOfInterestOf>
 <!-- LB Weight -->
 <schema:weight>
  <gs1:QuantitativeValue rdf:about="#D251WeightLB">
   <rdf:type rdf:resource="http://qudt.org/1.1/schema/qudt#QuantityValue"/>
   <qudt:unit rdf:resource="http://www.qudt.org/2.1/vocab/unit/LB"/>
   <qudt:numericalValue rdf:datatype="http://www.w3.org/2001/XMLSchema#double">18.7</qudt:numericalValue>
   <rdf:value rdf:datatype="http://www.w3.org/2001/XMLSchema#double">18.7</rdf:value>
   <gs1:unitCode>lbm</gs1:unitCode>
   <gs1:value>18.7</gs1:value>
   <rdfs:isDefinedBy rdf:resource="https://rdf.ag/o/beer-ONTOLOGY_DATE"/>
   <void:inDataset rdf:resource="#datasetdefinition"/>
  </gs1:QuantitativeValue>
 </schema:weight>
 <sosa:isFeatureOfInterestOf>
  <rdf:Description rdf:about="#D251WeightSosaLB">
   <rdf:type rdf:resource="http://www.w3.org/ns/sosa/Observation"/>
   <sosa:hasFeatureOfInterest rdf:resource="#D251"/>
   <sosa:observedProperty  rdf:resource="#grossWeight"/>
   <sosa:hasResult rdf:resource="#D251WeightLB"/>
   <sosa:hasSimpleResult rdf:datatype="http://www.qudt.org/2.1/vocab/unit/LB">18.7</sosa:hasSimpleResult>
   <rdfs:isDefinedBy rdf:resource="https://rdf.ag/o/beer-ONTOLOGY_DATE"/>
   <void:inDataset rdf:resource="#datasetdefinition"/>
  </rdf:Description>
 </sosa:isFeatureOfInterestOf>
 <rdfs:isDefinedBy rdf:resource="https://rdf.ag/o/beer-ONTOLOGY_DATE"/>
 <void:inDataset rdf:resource="#datasetdefinition"/>
</rdf:Description>
<rdf:Description rdf:about="#D301">
 <rdf:type rdf:resource="#LiquidContainer"/>
 <rdf:type rdf:resource="#Keg"/>
 <rdf:type rdf:resource="https://gs1.org/voc/PackagingDetails"/>
 <rdfs:label xml:lang="en">German DIN301</rdfs:label>
 <rdfs:label xml:lang="fr">Fût DIN301</rdfs:label>
 <skos:definition xml:lang="en">German DIN301</skos:definition>
 <skos:definition xml:lang="fr">Fût DIN301</skos:definition>
 <skos:altLabel xml:lang="en">DIN301</skos:altLabel>
 <beer:nominalCapacity rdf:datatype="http://www.qudt.org/2.1/vocab/unit/MilliL">30200</beer:nominalCapacity>
 <sosa:isFeatureOfInterestOf>
  <rdf:Description rdf:about="#D301ContentSosaML">
   <rdf:type rdf:resource="http://www.w3.org/ns/sosa/Observation"/>
   <sosa:hasFeatureOfInterest rdf:resource="#D301"/>
   <sosa:observedProperty rdf:resource="#sosaNominalCapacity"/>
   <sosa:hasResult>
    <gs1:QuantitativeValue rdf:about="#D301ContentML">
     <rdf:type rdf:resource="http://qudt.org/1.1/schema/qudt#QuantityValue"/>
     <gs1:unitCode>MLT</gs1:unitCode>
     <gs1:value>30200</gs1:value>
     <rdf:value rdf:datatype="http://www.w3.org/2001/XMLSchema#double">30200</rdf:value>
     <qudt:unit rdf:resource="http://www.qudt.org/2.1/vocab/unit/MilliL"/>
     <qudt:numericalValue rdf:datatype="http://www.w3.org/2001/XMLSchema#double">30200</qudt:numericalValue>
     <rdfs:isDefinedBy rdf:resource="https://rdf.ag/o/beer-ONTOLOGY_DATE"/>
     <void:inDataset rdf:resource="#datasetdefinition"/>
    </gs1:QuantitativeValue>
   </sosa:hasResult> 
   <sosa:hasSimpleResult rdf:datatype="http://www.qudt.org/2.1/vocab/unit/MilliM">30200</sosa:hasSimpleResult>
   <rdfs:isDefinedBy rdf:resource="https://rdf.ag/o/beer-ONTOLOGY_DATE"/>
   <void:inDataset rdf:resource="#datasetdefinition"/>
  </rdf:Description>
 </sosa:isFeatureOfInterestOf>
 <sosa:isFeatureOfInterestOf>
  <rdf:Description rdf:about="#D301ContentSosaOZ">
   <rdf:type rdf:resource="http://www.w3.org/ns/sosa/Observation"/>
   <sosa:hasFeatureOfInterest rdf:resource="#D301"/>
   <sosa:observedProperty rdf:resource="#sosaNominalCapacity"/>
   <sosa:hasResult>
   <gs1:QuantitativeValue rdf:about="#D301ContentOZ">
    <rdf:type rdf:resource="http://qudt.org/1.1/schema/qudt#QuantityValue"/>
    <gs1:unitCode>foz_us</gs1:unitCode>
    <gs1:value>1014</gs1:value>
    <rdf:value rdf:datatype="http://www.w3.org/2001/XMLSchema#double">1014</rdf:value>
    <qudt:unit rdf:resource="http://www.qudt.org/2.1/vocab/unit/OZ_VOL_US"/>
    <qudt:numericalValue rdf:datatype="http://www.w3.org/2001/XMLSchema#double">1014</qudt:numericalValue>
    <rdfs:isDefinedBy rdf:resource="https://rdf.ag/o/beer-ONTOLOGY_DATE"/>
    <void:inDataset rdf:resource="#datasetdefinition"/>  
   </gs1:QuantitativeValue>
   </sosa:hasResult>
   <sosa:hasSimpleResult rdf:datatype="http://www.qudt.org/2.1/vocab/unit/OZ_VOL_US">1014</sosa:hasSimpleResult>
   <rdfs:isDefinedBy rdf:resource="https://rdf.ag/o/beer-ONTOLOGY_DATE"/>
   <void:inDataset rdf:resource="#datasetdefinition"/>  
 </rdf:Description>
 </sosa:isFeatureOfInterestOf>
 <!-- Net Content Gal -->
 <sosa:isFeatureOfInterestOf>
  <rdf:Description rdf:about="#D301ContentSosaGAL">
   <rdf:type rdf:resource="http://www.w3.org/ns/sosa/Observation"/>
   <sosa:hasFeatureOfInterest rdf:resource="#D301"/>
   <sosa:observedProperty rdf:resource="#netcontent"/>
   <sosa:hasResult>
    <gs1:QuantitativeValue rdf:about="#D301ContentGal">
     <rdf:type rdf:resource="http://qudt.org/1.1/schema/qudt#QuantityValue"/>
     <gs1:unitCode>gal_us</gs1:unitCode>
     <gs1:value>7.92</gs1:value>
     <rdf:value rdf:datatype="http://www.w3.org/2001/XMLSchema#double">7.92</rdf:value>
     <qudt:unit rdf:resource="http://www.qudt.org/2.1/vocab/unit/GAL_US"/>
     <qudt:numericalValue rdf:datatype="http://www.w3.org/2001/XMLSchema#double">7.92</qudt:numericalValue>
     <rdfs:isDefinedBy rdf:resource="https://rdf.ag/o/beer-ONTOLOGY_DATE"/>
     <void:inDataset rdf:resource="#datasetdefinition"/>  
    </gs1:QuantitativeValue>
   </sosa:hasResult>
   <sosa:hasSimpleResult rdf:datatype="http://www.qudt.org/2.1/vocab/unit/GAL_US">7.92</sosa:hasSimpleResult>
   <rdfs:isDefinedBy rdf:resource="https://rdf.ag/o/beer-ONTOLOGY_DATE"/>
   <void:inDataset rdf:resource="#datasetdefinition"/>  
 </rdf:Description>
 </sosa:isFeatureOfInterestOf>

 <!-- Height MM-->
 <gs1:inPackageHeight>
  <gs1:QuantitativeValue rdf:about="#D301HeightMM">
   <rdf:type rdf:resource="http://qudt.org/1.1/schema/qudt#QuantityValue"/>
   <qudt:unit rdf:resource="http://www.qudt.org/2.1/vocab/unit/MilliM"/>
   <qudt:numericalValue rdf:datatype="http://www.w3.org/2001/XMLSchema#double">404</qudt:numericalValue>
   <rdf:value rdf:datatype="http://www.w3.org/2001/XMLSchema#double">404</rdf:value>
   <gs1:unitCode>MMT</gs1:unitCode>
   <gs1:value>404</gs1:value>
   <rdfs:isDefinedBy rdf:resource="https://rdf.ag/o/beer-ONTOLOGY_DATE"/>
   <void:inDataset rdf:resource="#datasetdefinition"/>
  </gs1:QuantitativeValue>
 </gs1:inPackageHeight>  
 <sosa:isFeatureOfInterestOf>
  <rdf:Description rdf:about="#D301HeightSosaMM">
   <rdf:type rdf:resource="http://www.w3.org/ns/sosa/Observation"/>
   <sosa:hasFeatureOfInterest rdf:resource="#D301"/>
   <sosa:observedProperty  rdf:resource="#height"/>
   <sosa:hasResult rdf:resource="#D301HeightMM"/>
   <sosa:hasSimpleResult rdf:datatype="http://www.qudt.org/2.1/vocab/unit/MilliM">404</sosa:hasSimpleResult>
   <rdfs:isDefinedBy rdf:resource="https://rdf.ag/o/beer-ONTOLOGY_DATE"/>
   <void:inDataset rdf:resource="#datasetdefinition"/>
  </rdf:Description>
 </sosa:isFeatureOfInterestOf>
 <!-- Height IN-->
 <gs1:inPackageHeight>
  <gs1:QuantitativeValue rdf:about="#D301HeightIN">
   <rdf:type rdf:resource="http://qudt.org/1.1/schema/qudt#QuantityValue"/>
   <qudt:unit rdf:resource="http://www.qudt.org/2.1/vocab/unit/IN"/>
   <qudt:numericalValue rdf:datatype="http://www.w3.org/2001/XMLSchema#double">15.906</qudt:numericalValue>
   <rdf:value rdf:datatype="http://www.w3.org/2001/XMLSchema#double">15.906</rdf:value>
   <gs1:unitCode>INH</gs1:unitCode>
   <gs1:value>15.906</gs1:value>
   <rdfs:isDefinedBy rdf:resource="https://rdf.ag/o/beer-ONTOLOGY_DATE"/>
   <void:inDataset rdf:resource="#datasetdefinition"/>
  </gs1:QuantitativeValue>
 </gs1:inPackageHeight>  
 <sosa:isFeatureOfInterestOf>
  <rdf:Description rdf:about="#D301HeightSosaIN">
   <rdf:type rdf:resource="http://www.w3.org/ns/sosa/Observation"/>
   <sosa:hasFeatureOfInterest rdf:resource="#D301"/>
   <sosa:observedProperty  rdf:resource="#height"/>
   <sosa:hasResult rdf:resource="#D301HeightIN"/>
   <sosa:hasSimpleResult rdf:datatype="http://www.qudt.org/2.1/vocab/unit/IN">15.906</sosa:hasSimpleResult>
   <rdfs:isDefinedBy rdf:resource="https://rdf.ag/o/beer-ONTOLOGY_DATE"/>
   <void:inDataset rdf:resource="#datasetdefinition"/>
  </rdf:Description>
 </sosa:isFeatureOfInterestOf>
 <!-- Diameter MM --> 
 <gs1:inPackageDiameter>
  <gs1:QuantitativeValue rdf:about="#D301DiameterMM">
   <rdf:type rdf:resource="http://qudt.org/1.1/schema/qudt#QuantityValue"/>
   <qudt:unit rdf:resource="http://www.qudt.org/2.1/vocab/unit/MilliM"/>
   <qudt:numericalValue rdf:datatype="http://www.w3.org/2001/XMLSchema#double">381</qudt:numericalValue>
   <rdf:value rdf:datatype="http://www.w3.org/2001/XMLSchema#double">381</rdf:value>
   <gs1:unitCode>MMT</gs1:unitCode>
   <gs1:value>381</gs1:value>
   <rdfs:isDefinedBy rdf:resource="https://rdf.ag/o/beer-ONTOLOGY_DATE"/>
   <void:inDataset rdf:resource="#datasetdefinition"/>
  </gs1:QuantitativeValue>
 </gs1:inPackageDiameter>
 <sosa:isFeatureOfInterestOf>
  <rdf:Description rdf:about="#D301DiameterSosaMM">
   <rdf:type rdf:resource="http://www.w3.org/ns/sosa/Observation"/>
   <sosa:hasFeatureOfInterest rdf:resource="#D301"/>
   <sosa:observedProperty  rdf:resource="#diameter"/>
   <sosa:hasResult rdf:resource="#D301DiameterMM"/>
   <sosa:hasSimpleResult rdf:datatype="http://www.qudt.org/2.1/vocab/unit/MilliM">381</sosa:hasSimpleResult>
   <rdfs:isDefinedBy rdf:resource="https://rdf.ag/o/beer-ONTOLOGY_DATE"/>
   <void:inDataset rdf:resource="#datasetdefinition"/>
  </rdf:Description>
 </sosa:isFeatureOfInterestOf>
 <!-- Diameter IN --> 
 <gs1:inPackageDiameter>
  <gs1:QuantitativeValue rdf:about="#D301DiameterIN">
   <rdf:type rdf:resource="http://qudt.org/1.1/schema/qudt#QuantityValue"/>
   <qudt:unit rdf:resource="http://www.qudt.org/2.1/vocab/unit/IN"/>
   <qudt:numericalValue rdf:datatype="http://www.w3.org/2001/XMLSchema#double">15.000</qudt:numericalValue>
   <rdf:value rdf:datatype="http://www.w3.org/2001/XMLSchema#double">15.000</rdf:value>
   <gs1:unitCode>INH</gs1:unitCode>
   <gs1:value>15.000</gs1:value>
   <rdfs:isDefinedBy rdf:resource="https://rdf.ag/o/beer-ONTOLOGY_DATE"/>
   <void:inDataset rdf:resource="#datasetdefinition"/>
  </gs1:QuantitativeValue>
 </gs1:inPackageDiameter>
 <sosa:isFeatureOfInterestOf>
  <rdf:Description rdf:about="#D301DiameterSosaIN">
   <rdf:type rdf:resource="http://www.w3.org/ns/sosa/Observation"/>
   <sosa:hasFeatureOfInterest rdf:resource="#D301"/>
   <sosa:observedProperty  rdf:resource="#diameter"/>
   <sosa:hasResult rdf:resource="#D301DiameterIN"/>
   <sosa:hasSimpleResult rdf:datatype="http://www.qudt.org/2.1/vocab/unit/IN">15.000</sosa:hasSimpleResult>
   <rdfs:isDefinedBy rdf:resource="https://rdf.ag/o/beer-ONTOLOGY_DATE"/>
   <void:inDataset rdf:resource="#datasetdefinition"/>
  </rdf:Description>
 </sosa:isFeatureOfInterestOf>
 <!-- KG Weight -->
 <schema:weight>
  <gs1:QuantitativeValue rdf:about="#D301WeightKG">
   <rdf:type rdf:resource="http://qudt.org/1.1/schema/qudt#QuantityValue"/>
   <qudt:unit rdf:resource="http://www.qudt.org/2.1/vocab/unit/KiloGM"/>
   <qudt:numericalValue rdf:datatype="http://www.w3.org/2001/XMLSchema#double">8.9</qudt:numericalValue>
   <rdf:value rdf:datatype="http://www.w3.org/2001/XMLSchema#double">8.9</rdf:value>
   <gs1:unitCode>KGM</gs1:unitCode>
   <gs1:value>8.9</gs1:value>
   <rdfs:isDefinedBy rdf:resource="https://rdf.ag/o/beer-ONTOLOGY_DATE"/>
   <void:inDataset rdf:resource="#datasetdefinition"/>
  </gs1:QuantitativeValue>
 </schema:weight>
 <sosa:isFeatureOfInterestOf>
  <rdf:Description rdf:about="#D301WeightSosaKG">
   <rdf:type rdf:resource="http://www.w3.org/ns/sosa/Observation"/>
   <sosa:hasFeatureOfInterest rdf:resource="#D301"/>
   <sosa:observedProperty  rdf:resource="#grossWeight"/>
   <sosa:hasResult rdf:resource="#D301WeightKG"/>
   <sosa:hasSimpleResult rdf:datatype="http://www.qudt.org/2.1/vocab/unit/KiloGM">8.9</sosa:hasSimpleResult>
   <rdfs:isDefinedBy rdf:resource="https://rdf.ag/o/beer-ONTOLOGY_DATE"/>
   <void:inDataset rdf:resource="#datasetdefinition"/>
  </rdf:Description>
 </sosa:isFeatureOfInterestOf>
 <!-- LB Weight -->
 <schema:weight>
  <gs1:QuantitativeValue rdf:about="#D301WeightLB">
   <rdf:type rdf:resource="http://qudt.org/1.1/schema/qudt#QuantityValue"/>
   <qudt:unit rdf:resource="http://www.qudt.org/2.1/vocab/unit/LB"/>
   <qudt:numericalValue rdf:datatype="http://www.w3.org/2001/XMLSchema#double">19.6</qudt:numericalValue>
   <rdf:value rdf:datatype="http://www.w3.org/2001/XMLSchema#double">19.6</rdf:value>
   <gs1:unitCode>lbm</gs1:unitCode>
   <gs1:value>19.6</gs1:value>
   <rdfs:isDefinedBy rdf:resource="https://rdf.ag/o/beer-ONTOLOGY_DATE"/>
   <void:inDataset rdf:resource="#datasetdefinition"/>
  </gs1:QuantitativeValue>
 </schema:weight>
 <sosa:isFeatureOfInterestOf>
  <rdf:Description rdf:about="#D301WeightSosaLB">
   <rdf:type rdf:resource="http://www.w3.org/ns/sosa/Observation"/>
   <sosa:hasFeatureOfInterest rdf:resource="#D301"/>
   <sosa:observedProperty  rdf:resource="#grossWeight"/>
   <sosa:hasResult rdf:resource="#D301WeightLB"/>
   <sosa:hasSimpleResult rdf:datatype="http://www.qudt.org/2.1/vocab/unit/LB">19.6</sosa:hasSimpleResult>
   <rdfs:isDefinedBy rdf:resource="https://rdf.ag/o/beer-ONTOLOGY_DATE"/>
   <void:inDataset rdf:resource="#datasetdefinition"/>
  </rdf:Description>
 </sosa:isFeatureOfInterestOf>
 <rdfs:isDefinedBy rdf:resource="https://rdf.ag/o/beer-ONTOLOGY_DATE"/>
 <void:inDataset rdf:resource="#datasetdefinition"/>
</rdf:Description>
<rdf:Description rdf:about="#D501">
 <rdf:type rdf:resource="#LiquidContainer"/>
 <rdf:type rdf:resource="#Keg"/>
 <rdf:type rdf:resource="https://gs1.org/voc/PackagingDetails"/>
 <rdfs:label xml:lang="en">German DIN501</rdfs:label>
 <rdfs:label xml:lang="fr">Fût DIN501</rdfs:label>
 <skos:definition xml:lang="en">German DIN501</skos:definition>
 <skos:definition xml:lang="fr">Fût DIN501</skos:definition>
 <skos:altLabel xml:lang="en">DIN501</skos:altLabel>
 <beer:nominalCapacity rdf:datatype="http://www.qudt.org/2.1/vocab/unit/MilliL">50200</beer:nominalCapacity>
 <sosa:isFeatureOfInterestOf>
  <rdf:Description rdf:about="#D501ContentSosaML">
   <rdf:type rdf:resource="http://www.w3.org/ns/sosa/Observation"/>
   <sosa:hasFeatureOfInterest rdf:resource="#D501"/>
   <sosa:observedProperty rdf:resource="#sosaNominalCapacity"/>
   <sosa:hasResult>
    <gs1:QuantitativeValue rdf:about="#D501ContentML">
     <rdf:type rdf:resource="http://qudt.org/1.1/schema/qudt#QuantityValue"/>
     <gs1:unitCode>MLT</gs1:unitCode>
     <gs1:value>50200</gs1:value>
     <rdf:value rdf:datatype="http://www.w3.org/2001/XMLSchema#double">50200</rdf:value>
     <qudt:unit rdf:resource="http://www.qudt.org/2.1/vocab/unit/MilliL"/>
     <qudt:numericalValue rdf:datatype="http://www.w3.org/2001/XMLSchema#double">50200</qudt:numericalValue>
     <rdfs:isDefinedBy rdf:resource="https://rdf.ag/o/beer-ONTOLOGY_DATE"/>
     <void:inDataset rdf:resource="#datasetdefinition"/>
    </gs1:QuantitativeValue>
   </sosa:hasResult> 
   <sosa:hasSimpleResult rdf:datatype="http://www.qudt.org/2.1/vocab/unit/MilliM">50200</sosa:hasSimpleResult>
   <rdfs:isDefinedBy rdf:resource="https://rdf.ag/o/beer-ONTOLOGY_DATE"/>
   <void:inDataset rdf:resource="#datasetdefinition"/>
  </rdf:Description>
 </sosa:isFeatureOfInterestOf>
 <sosa:isFeatureOfInterestOf>
  <rdf:Description rdf:about="#D501ContentSosaOZ">
   <rdf:type rdf:resource="http://www.w3.org/ns/sosa/Observation"/>
   <sosa:hasFeatureOfInterest rdf:resource="#D501"/>
   <sosa:observedProperty rdf:resource="#sosaNominalCapacity"/>
   <sosa:hasResult>
   <gs1:QuantitativeValue rdf:about="#D501ContentOZ">
    <rdf:type rdf:resource="http://qudt.org/1.1/schema/qudt#QuantityValue"/>
    <gs1:unitCode>foz_us</gs1:unitCode>
    <gs1:value>1690</gs1:value>
    <rdf:value rdf:datatype="http://www.w3.org/2001/XMLSchema#double">1690</rdf:value>
    <qudt:unit rdf:resource="http://www.qudt.org/2.1/vocab/unit/OZ_VOL_US"/>
    <qudt:numericalValue rdf:datatype="http://www.w3.org/2001/XMLSchema#double">1690</qudt:numericalValue>
    <rdfs:isDefinedBy rdf:resource="https://rdf.ag/o/beer-ONTOLOGY_DATE"/>
    <void:inDataset rdf:resource="#datasetdefinition"/>  
   </gs1:QuantitativeValue>
   </sosa:hasResult>
   <sosa:hasSimpleResult rdf:datatype="http://www.qudt.org/2.1/vocab/unit/OZ_VOL_US">1690</sosa:hasSimpleResult>
   <rdfs:isDefinedBy rdf:resource="https://rdf.ag/o/beer-ONTOLOGY_DATE"/>
   <void:inDataset rdf:resource="#datasetdefinition"/>  
 </rdf:Description>
 </sosa:isFeatureOfInterestOf>
 <!-- Net Content Gal -->
 <sosa:isFeatureOfInterestOf>
  <rdf:Description rdf:about="#D501ContentSosaGAL">
   <rdf:type rdf:resource="http://www.w3.org/ns/sosa/Observation"/>
   <sosa:hasFeatureOfInterest rdf:resource="#D501"/>
   <sosa:observedProperty rdf:resource="#netcontent"/>
   <sosa:hasResult>
    <gs1:QuantitativeValue rdf:about="#D501ContentGal">
     <rdf:type rdf:resource="http://qudt.org/1.1/schema/qudt#QuantityValue"/>
     <gs1:unitCode>gal_us</gs1:unitCode>
     <gs1:value>13.20</gs1:value>
     <rdf:value rdf:datatype="http://www.w3.org/2001/XMLSchema#double">13.20</rdf:value>
     <qudt:unit rdf:resource="http://www.qudt.org/2.1/vocab/unit/GAL_US"/>
     <qudt:numericalValue rdf:datatype="http://www.w3.org/2001/XMLSchema#double">13.20</qudt:numericalValue>
     <rdfs:isDefinedBy rdf:resource="https://rdf.ag/o/beer-ONTOLOGY_DATE"/>
     <void:inDataset rdf:resource="#datasetdefinition"/>  
    </gs1:QuantitativeValue>
   </sosa:hasResult>
   <sosa:hasSimpleResult rdf:datatype="http://www.qudt.org/2.1/vocab/unit/GAL_US">13.20</sosa:hasSimpleResult>
   <rdfs:isDefinedBy rdf:resource="https://rdf.ag/o/beer-ONTOLOGY_DATE"/>
   <void:inDataset rdf:resource="#datasetdefinition"/>  
 </rdf:Description>
 </sosa:isFeatureOfInterestOf>

 <!-- Height MM-->
 <gs1:inPackageHeight>
  <gs1:QuantitativeValue rdf:about="#D501HeightMM">
   <rdf:type rdf:resource="http://qudt.org/1.1/schema/qudt#QuantityValue"/>
   <qudt:unit rdf:resource="http://www.qudt.org/2.1/vocab/unit/MilliM"/>
   <qudt:numericalValue rdf:datatype="http://www.w3.org/2001/XMLSchema#double">600</qudt:numericalValue>
   <rdf:value rdf:datatype="http://www.w3.org/2001/XMLSchema#double">600</rdf:value>
   <gs1:unitCode>MMT</gs1:unitCode>
   <gs1:value>600</gs1:value>
   <rdfs:isDefinedBy rdf:resource="https://rdf.ag/o/beer-ONTOLOGY_DATE"/>
   <void:inDataset rdf:resource="#datasetdefinition"/>
  </gs1:QuantitativeValue>
 </gs1:inPackageHeight>  
 <sosa:isFeatureOfInterestOf>
  <rdf:Description rdf:about="#D501HeightSosaMM">
   <rdf:type rdf:resource="http://www.w3.org/ns/sosa/Observation"/>
   <sosa:hasFeatureOfInterest rdf:resource="#D501"/>
   <sosa:observedProperty  rdf:resource="#height"/>
   <sosa:hasResult rdf:resource="#D501HeightMM"/>
   <sosa:hasSimpleResult rdf:datatype="http://www.qudt.org/2.1/vocab/unit/MilliM">600</sosa:hasSimpleResult>
   <rdfs:isDefinedBy rdf:resource="https://rdf.ag/o/beer-ONTOLOGY_DATE"/>
   <void:inDataset rdf:resource="#datasetdefinition"/>
  </rdf:Description>
 </sosa:isFeatureOfInterestOf>
 <!-- Height IN-->
 <gs1:inPackageHeight>
  <gs1:QuantitativeValue rdf:about="#D501HeightIN">
   <rdf:type rdf:resource="http://qudt.org/1.1/schema/qudt#QuantityValue"/>
   <qudt:unit rdf:resource="http://www.qudt.org/2.1/vocab/unit/IN"/>
   <qudt:numericalValue rdf:datatype="http://www.w3.org/2001/XMLSchema#double">23.622</qudt:numericalValue>
   <rdf:value rdf:datatype="http://www.w3.org/2001/XMLSchema#double">23.622</rdf:value>
   <gs1:unitCode>INH</gs1:unitCode>
   <gs1:value>23.622</gs1:value>
   <rdfs:isDefinedBy rdf:resource="https://rdf.ag/o/beer-ONTOLOGY_DATE"/>
   <void:inDataset rdf:resource="#datasetdefinition"/>
  </gs1:QuantitativeValue>
 </gs1:inPackageHeight>  
 <sosa:isFeatureOfInterestOf>
  <rdf:Description rdf:about="#D501HeightSosaIN">
   <rdf:type rdf:resource="http://www.w3.org/ns/sosa/Observation"/>
   <sosa:hasFeatureOfInterest rdf:resource="#D501"/>
   <sosa:observedProperty  rdf:resource="#height"/>
   <sosa:hasResult rdf:resource="#D501HeightIN"/>
   <sosa:hasSimpleResult rdf:datatype="http://www.qudt.org/2.1/vocab/unit/IN">23.622</sosa:hasSimpleResult>
   <rdfs:isDefinedBy rdf:resource="https://rdf.ag/o/beer-ONTOLOGY_DATE"/>
   <void:inDataset rdf:resource="#datasetdefinition"/>
  </rdf:Description>
 </sosa:isFeatureOfInterestOf>
 <!-- Diameter MM --> 
 <gs1:inPackageDiameter>
  <gs1:QuantitativeValue rdf:about="#D501DiameterMM">
   <rdf:type rdf:resource="http://qudt.org/1.1/schema/qudt#QuantityValue"/>
   <qudt:unit rdf:resource="http://www.qudt.org/2.1/vocab/unit/MilliM"/>
   <qudt:numericalValue rdf:datatype="http://www.w3.org/2001/XMLSchema#double">381</qudt:numericalValue>
   <rdf:value rdf:datatype="http://www.w3.org/2001/XMLSchema#double">381</rdf:value>
   <gs1:unitCode>MMT</gs1:unitCode>
   <gs1:value>381</gs1:value>
   <rdfs:isDefinedBy rdf:resource="https://rdf.ag/o/beer-ONTOLOGY_DATE"/>
   <void:inDataset rdf:resource="#datasetdefinition"/>
  </gs1:QuantitativeValue>
 </gs1:inPackageDiameter>
 <sosa:isFeatureOfInterestOf>
  <rdf:Description rdf:about="#D501DiameterSosaMM">
   <rdf:type rdf:resource="http://www.w3.org/ns/sosa/Observation"/>
   <sosa:hasFeatureOfInterest rdf:resource="#D501"/>
   <sosa:observedProperty  rdf:resource="#diameter"/>
   <sosa:hasResult rdf:resource="#D501DiameterMM"/>
   <sosa:hasSimpleResult rdf:datatype="http://www.qudt.org/2.1/vocab/unit/MilliM">381</sosa:hasSimpleResult>
   <rdfs:isDefinedBy rdf:resource="https://rdf.ag/o/beer-ONTOLOGY_DATE"/>
   <void:inDataset rdf:resource="#datasetdefinition"/>
  </rdf:Description>
 </sosa:isFeatureOfInterestOf>
 <!-- Diameter IN --> 
 <gs1:inPackageDiameter>
  <gs1:QuantitativeValue rdf:about="#D501DiameterIN">
   <rdf:type rdf:resource="http://qudt.org/1.1/schema/qudt#QuantityValue"/>
   <qudt:unit rdf:resource="http://www.qudt.org/2.1/vocab/unit/IN"/>
   <qudt:numericalValue rdf:datatype="http://www.w3.org/2001/XMLSchema#double">15.000</qudt:numericalValue>
   <rdf:value rdf:datatype="http://www.w3.org/2001/XMLSchema#double">15.000</rdf:value>
   <gs1:unitCode>INH</gs1:unitCode>
   <gs1:value>15.000</gs1:value>
   <rdfs:isDefinedBy rdf:resource="https://rdf.ag/o/beer-ONTOLOGY_DATE"/>
   <void:inDataset rdf:resource="#datasetdefinition"/>
  </gs1:QuantitativeValue>
 </gs1:inPackageDiameter>
 <sosa:isFeatureOfInterestOf>
  <rdf:Description rdf:about="#D501DiameterSosaIN">
   <rdf:type rdf:resource="http://www.w3.org/ns/sosa/Observation"/>
   <sosa:hasFeatureOfInterest rdf:resource="#D501"/>
   <sosa:observedProperty  rdf:resource="#diameter"/>
   <sosa:hasResult rdf:resource="#D501DiameterIN"/>
   <sosa:hasSimpleResult rdf:datatype="http://www.qudt.org/2.1/vocab/unit/IN">15.000</sosa:hasSimpleResult>
   <rdfs:isDefinedBy rdf:resource="https://rdf.ag/o/beer-ONTOLOGY_DATE"/>
   <void:inDataset rdf:resource="#datasetdefinition"/>
  </rdf:Description>
 </sosa:isFeatureOfInterestOf>
 <!-- KG Weight -->
 <schema:weight>
  <gs1:QuantitativeValue rdf:about="#D501WeightKG">
   <rdf:type rdf:resource="http://qudt.org/1.1/schema/qudt#QuantityValue"/>
   <qudt:unit rdf:resource="http://www.qudt.org/2.1/vocab/unit/KiloGM"/>
   <qudt:numericalValue rdf:datatype="http://www.w3.org/2001/XMLSchema#double">11.1</qudt:numericalValue>
   <rdf:value rdf:datatype="http://www.w3.org/2001/XMLSchema#double">11.1</rdf:value>
   <gs1:unitCode>KGM</gs1:unitCode>
   <gs1:value>11.1</gs1:value>
   <rdfs:isDefinedBy rdf:resource="https://rdf.ag/o/beer-ONTOLOGY_DATE"/>
   <void:inDataset rdf:resource="#datasetdefinition"/>
  </gs1:QuantitativeValue>
 </schema:weight>
 <sosa:isFeatureOfInterestOf>
  <rdf:Description rdf:about="#D501WeightSosaKG">
   <rdf:type rdf:resource="http://www.w3.org/ns/sosa/Observation"/>
   <sosa:hasFeatureOfInterest rdf:resource="#D501"/>
   <sosa:observedProperty  rdf:resource="#grossWeight"/>
   <sosa:hasResult rdf:resource="#D501WeightKG"/>
   <sosa:hasSimpleResult rdf:datatype="http://www.qudt.org/2.1/vocab/unit/KiloGM">11.1</sosa:hasSimpleResult>
   <rdfs:isDefinedBy rdf:resource="https://rdf.ag/o/beer-ONTOLOGY_DATE"/>
   <void:inDataset rdf:resource="#datasetdefinition"/>
  </rdf:Description>
 </sosa:isFeatureOfInterestOf>
 <!-- LB Weight -->
 <schema:weight>
  <gs1:QuantitativeValue rdf:about="#D501WeightLB">
   <rdf:type rdf:resource="http://qudt.org/1.1/schema/qudt#QuantityValue"/>
   <qudt:unit rdf:resource="http://www.qudt.org/2.1/vocab/unit/LB"/>
   <qudt:numericalValue rdf:datatype="http://www.w3.org/2001/XMLSchema#double">24.5</qudt:numericalValue>
   <rdf:value rdf:datatype="http://www.w3.org/2001/XMLSchema#double">24.5</rdf:value>
   <gs1:unitCode>lbm</gs1:unitCode>
   <gs1:value>24.5</gs1:value>
   <rdfs:isDefinedBy rdf:resource="https://rdf.ag/o/beer-ONTOLOGY_DATE"/>
   <void:inDataset rdf:resource="#datasetdefinition"/>
  </gs1:QuantitativeValue>
 </schema:weight>
 <sosa:isFeatureOfInterestOf>
  <rdf:Description rdf:about="#D501WeightSosaLB">
   <rdf:type rdf:resource="http://www.w3.org/ns/sosa/Observation"/>
   <sosa:hasFeatureOfInterest rdf:resource="#D501"/>
   <sosa:observedProperty  rdf:resource="#grossWeight"/>
   <sosa:hasResult rdf:resource="#D501WeightLB"/>
   <sosa:hasSimpleResult rdf:datatype="http://www.qudt.org/2.1/vocab/unit/LB">24.5</sosa:hasSimpleResult>
   <rdfs:isDefinedBy rdf:resource="https://rdf.ag/o/beer-ONTOLOGY_DATE"/>
   <void:inDataset rdf:resource="#datasetdefinition"/>
  </rdf:Description>
 </sosa:isFeatureOfInterestOf>
 <rdfs:isDefinedBy rdf:resource="https://rdf.ag/o/beer-ONTOLOGY_DATE"/>
 <void:inDataset rdf:resource="#datasetdefinition"/>
</rdf:Description>
<rdf:Description rdf:about="#Euro20">
 <rdf:type rdf:resource="#LiquidContainer"/>
 <rdf:type rdf:resource="#Keg"/>
 <rdf:type rdf:resource="https://gs1.org/voc/PackagingDetails"/>
 <rdfs:label xml:lang="en">European 20L Keg</rdfs:label>
 <rdfs:label xml:lang="fr">Fût Européen 20L</rdfs:label>
 <skos:definition xml:lang="en">European 20L Keg</skos:definition>
 <skos:definition xml:lang="fr">Fût Européen 20L</skos:definition>
 <beer:nominalCapacity rdf:datatype="http://www.qudt.org/2.1/vocab/unit/MilliL">20000</beer:nominalCapacity>
 <sosa:isFeatureOfInterestOf>
  <rdf:Description rdf:about="#Euro20ContentSosaML">
   <rdf:type rdf:resource="http://www.w3.org/ns/sosa/Observation"/>
   <sosa:hasFeatureOfInterest rdf:resource="#Euro20"/>
   <sosa:observedProperty rdf:resource="#sosaNominalCapacity"/>
   <sosa:hasResult>
    <gs1:QuantitativeValue rdf:about="#Euro20ContentML">
     <rdf:type rdf:resource="http://qudt.org/1.1/schema/qudt#QuantityValue"/>
     <gs1:unitCode>MLT</gs1:unitCode>
     <gs1:value>20000</gs1:value>
     <rdf:value rdf:datatype="http://www.w3.org/2001/XMLSchema#double">20000</rdf:value>
     <qudt:unit rdf:resource="http://www.qudt.org/2.1/vocab/unit/MilliL"/>
     <qudt:numericalValue rdf:datatype="http://www.w3.org/2001/XMLSchema#double">20000</qudt:numericalValue>
     <rdfs:isDefinedBy rdf:resource="https://rdf.ag/o/beer-ONTOLOGY_DATE"/>
     <void:inDataset rdf:resource="#datasetdefinition"/>
    </gs1:QuantitativeValue>
   </sosa:hasResult> 
   <sosa:hasSimpleResult rdf:datatype="http://www.qudt.org/2.1/vocab/unit/MilliM">20000</sosa:hasSimpleResult>
   <rdfs:isDefinedBy rdf:resource="https://rdf.ag/o/beer-ONTOLOGY_DATE"/>
   <void:inDataset rdf:resource="#datasetdefinition"/>
  </rdf:Description>
 </sosa:isFeatureOfInterestOf>
 <sosa:isFeatureOfInterestOf>
  <rdf:Description rdf:about="#Euro20ContentSosaOZ">
   <rdf:type rdf:resource="http://www.w3.org/ns/sosa/Observation"/>
   <sosa:hasFeatureOfInterest rdf:resource="#Euro20"/>
   <sosa:observedProperty rdf:resource="#sosaNominalCapacity"/>
   <sosa:hasResult>
   <gs1:QuantitativeValue rdf:about="#Euro20ContentOZ">
    <rdf:type rdf:resource="http://qudt.org/1.1/schema/qudt#QuantityValue"/>
    <gs1:unitCode>foz_us</gs1:unitCode>
    <gs1:value>563</gs1:value>
    <rdf:value rdf:datatype="http://www.w3.org/2001/XMLSchema#double">563</rdf:value>
    <qudt:unit rdf:resource="http://www.qudt.org/2.1/vocab/unit/OZ_VOL_US"/>
    <qudt:numericalValue rdf:datatype="http://www.w3.org/2001/XMLSchema#double">563</qudt:numericalValue>
    <rdfs:isDefinedBy rdf:resource="https://rdf.ag/o/beer-ONTOLOGY_DATE"/>
    <void:inDataset rdf:resource="#datasetdefinition"/>  
   </gs1:QuantitativeValue>
   </sosa:hasResult>
   <sosa:hasSimpleResult rdf:datatype="http://www.qudt.org/2.1/vocab/unit/OZ_VOL_US">563</sosa:hasSimpleResult>
   <rdfs:isDefinedBy rdf:resource="https://rdf.ag/o/beer-ONTOLOGY_DATE"/>
   <void:inDataset rdf:resource="#datasetdefinition"/>  
 </rdf:Description>
 </sosa:isFeatureOfInterestOf>
 <!-- Net Content Gal -->
 <sosa:isFeatureOfInterestOf>
  <rdf:Description rdf:about="#Euro20ContentSosaGAL">
   <rdf:type rdf:resource="http://www.w3.org/ns/sosa/Observation"/>
   <sosa:hasFeatureOfInterest rdf:resource="#Euro20"/>
   <sosa:observedProperty rdf:resource="#netcontent"/>
   <sosa:hasResult>
    <gs1:QuantitativeValue rdf:about="#Euro20ContentGal">
     <rdf:type rdf:resource="http://qudt.org/1.1/schema/qudt#QuantityValue"/>
     <gs1:unitCode>gal_us</gs1:unitCode>
     <gs1:value>4.40</gs1:value>
     <rdf:value rdf:datatype="http://www.w3.org/2001/XMLSchema#double">4.40</rdf:value>
     <qudt:unit rdf:resource="http://www.qudt.org/2.1/vocab/unit/GAL_US"/>
     <qudt:numericalValue rdf:datatype="http://www.w3.org/2001/XMLSchema#double">4.40</qudt:numericalValue>
     <rdfs:isDefinedBy rdf:resource="https://rdf.ag/o/beer-ONTOLOGY_DATE"/>
     <void:inDataset rdf:resource="#datasetdefinition"/>  
    </gs1:QuantitativeValue>
   </sosa:hasResult>
   <sosa:hasSimpleResult rdf:datatype="http://www.qudt.org/2.1/vocab/unit/GAL_US">4.40</sosa:hasSimpleResult>
   <rdfs:isDefinedBy rdf:resource="https://rdf.ag/o/beer-ONTOLOGY_DATE"/>
   <void:inDataset rdf:resource="#datasetdefinition"/>  
 </rdf:Description>
 </sosa:isFeatureOfInterestOf>

 <!-- Height MM-->
 <gs1:inPackageHeight>
  <gs1:QuantitativeValue rdf:about="#Euro20HeightMM">
   <rdf:type rdf:resource="http://qudt.org/1.1/schema/qudt#QuantityValue"/>
   <qudt:unit rdf:resource="http://www.qudt.org/2.1/vocab/unit/MilliM"/>
   <qudt:numericalValue rdf:datatype="http://www.w3.org/2001/XMLSchema#double">216</qudt:numericalValue>
   <rdf:value rdf:datatype="http://www.w3.org/2001/XMLSchema#double">216</rdf:value>
   <gs1:unitCode>MMT</gs1:unitCode>
   <gs1:value>216</gs1:value>
   <rdfs:isDefinedBy rdf:resource="https://rdf.ag/o/beer-ONTOLOGY_DATE"/>
   <void:inDataset rdf:resource="#datasetdefinition"/>
  </gs1:QuantitativeValue>
 </gs1:inPackageHeight>  
 <sosa:isFeatureOfInterestOf>
  <rdf:Description rdf:about="#Euro20HeightSosaMM">
   <rdf:type rdf:resource="http://www.w3.org/ns/sosa/Observation"/>
   <sosa:hasFeatureOfInterest rdf:resource="#Euro20"/>
   <sosa:observedProperty  rdf:resource="#height"/>
   <sosa:hasResult rdf:resource="#Euro20HeightMM"/>
   <sosa:hasSimpleResult rdf:datatype="http://www.qudt.org/2.1/vocab/unit/MilliM">216</sosa:hasSimpleResult>
   <rdfs:isDefinedBy rdf:resource="https://rdf.ag/o/beer-ONTOLOGY_DATE"/>
   <void:inDataset rdf:resource="#datasetdefinition"/>
  </rdf:Description>
 </sosa:isFeatureOfInterestOf>
 <!-- Height IN-->
 <gs1:inPackageHeight>
  <gs1:QuantitativeValue rdf:about="#Euro20HeightIN">
   <rdf:type rdf:resource="http://qudt.org/1.1/schema/qudt#QuantityValue"/>
   <qudt:unit rdf:resource="http://www.qudt.org/2.1/vocab/unit/IN"/>
   <qudt:numericalValue rdf:datatype="http://www.w3.org/2001/XMLSchema#double">8.504</qudt:numericalValue>
   <rdf:value rdf:datatype="http://www.w3.org/2001/XMLSchema#double">8.504</rdf:value>
   <gs1:unitCode>INH</gs1:unitCode>
   <gs1:value>8.504</gs1:value>
   <rdfs:isDefinedBy rdf:resource="https://rdf.ag/o/beer-ONTOLOGY_DATE"/>
   <void:inDataset rdf:resource="#datasetdefinition"/>
  </gs1:QuantitativeValue>
 </gs1:inPackageHeight>  
 <sosa:isFeatureOfInterestOf>
  <rdf:Description rdf:about="#Euro20HeightSosaIN">
   <rdf:type rdf:resource="http://www.w3.org/ns/sosa/Observation"/>
   <sosa:hasFeatureOfInterest rdf:resource="#Euro20"/>
   <sosa:observedProperty  rdf:resource="#height"/>
   <sosa:hasResult rdf:resource="#Euro20HeightIN"/>
   <sosa:hasSimpleResult rdf:datatype="http://www.qudt.org/2.1/vocab/unit/IN">8.504</sosa:hasSimpleResult>
   <rdfs:isDefinedBy rdf:resource="https://rdf.ag/o/beer-ONTOLOGY_DATE"/>
   <void:inDataset rdf:resource="#datasetdefinition"/>
  </rdf:Description>
 </sosa:isFeatureOfInterestOf>
 <!-- Diameter MM --> 
 <gs1:inPackageDiameter>
  <gs1:QuantitativeValue rdf:about="#Euro20DiameterMM">
   <rdf:type rdf:resource="http://qudt.org/1.1/schema/qudt#QuantityValue"/>
   <qudt:unit rdf:resource="http://www.qudt.org/2.1/vocab/unit/MilliM"/>
   <qudt:numericalValue rdf:datatype="http://www.w3.org/2001/XMLSchema#double">395</qudt:numericalValue>
   <rdf:value rdf:datatype="http://www.w3.org/2001/XMLSchema#double">395</rdf:value>
   <gs1:unitCode>MMT</gs1:unitCode>
   <gs1:value>395</gs1:value>
   <rdfs:isDefinedBy rdf:resource="https://rdf.ag/o/beer-ONTOLOGY_DATE"/>
   <void:inDataset rdf:resource="#datasetdefinition"/>
  </gs1:QuantitativeValue>
 </gs1:inPackageDiameter>
 <sosa:isFeatureOfInterestOf>
  <rdf:Description rdf:about="#Euro20DiameterSosaMM">
   <rdf:type rdf:resource="http://www.w3.org/ns/sosa/Observation"/>
   <sosa:hasFeatureOfInterest rdf:resource="#Euro20"/>
   <sosa:observedProperty  rdf:resource="#diameter"/>
   <sosa:hasResult rdf:resource="#Euro20DiameterMM"/>
   <sosa:hasSimpleResult rdf:datatype="http://www.qudt.org/2.1/vocab/unit/MilliM">395</sosa:hasSimpleResult>
   <rdfs:isDefinedBy rdf:resource="https://rdf.ag/o/beer-ONTOLOGY_DATE"/>
   <void:inDataset rdf:resource="#datasetdefinition"/>
  </rdf:Description>
 </sosa:isFeatureOfInterestOf>
 <!-- Diameter IN --> 
 <gs1:inPackageDiameter>
  <gs1:QuantitativeValue rdf:about="#Euro20DiameterIN">
   <rdf:type rdf:resource="http://qudt.org/1.1/schema/qudt#QuantityValue"/>
   <qudt:unit rdf:resource="http://www.qudt.org/2.1/vocab/unit/IN"/>
   <qudt:numericalValue rdf:datatype="http://www.w3.org/2001/XMLSchema#double">15.551</qudt:numericalValue>
   <rdf:value rdf:datatype="http://www.w3.org/2001/XMLSchema#double">15.551</rdf:value>
   <gs1:unitCode>INH</gs1:unitCode>
   <gs1:value>15.551</gs1:value>
   <rdfs:isDefinedBy rdf:resource="https://rdf.ag/o/beer-ONTOLOGY_DATE"/>
   <void:inDataset rdf:resource="#datasetdefinition"/>
  </gs1:QuantitativeValue>
 </gs1:inPackageDiameter>
 <sosa:isFeatureOfInterestOf>
  <rdf:Description rdf:about="#Euro20DiameterSosaIN">
   <rdf:type rdf:resource="http://www.w3.org/ns/sosa/Observation"/>
   <sosa:hasFeatureOfInterest rdf:resource="#Euro20"/>
   <sosa:observedProperty  rdf:resource="#diameter"/>
   <sosa:hasResult rdf:resource="#Euro20DiameterIN"/>
   <sosa:hasSimpleResult rdf:datatype="http://www.qudt.org/2.1/vocab/unit/IN">15.551</sosa:hasSimpleResult>
   <rdfs:isDefinedBy rdf:resource="https://rdf.ag/o/beer-ONTOLOGY_DATE"/>
   <void:inDataset rdf:resource="#datasetdefinition"/>
  </rdf:Description>
 </sosa:isFeatureOfInterestOf>
 <!-- KG Weight -->
 <schema:weight>
  <gs1:QuantitativeValue rdf:about="#Euro20WeightKG">
   <rdf:type rdf:resource="http://qudt.org/1.1/schema/qudt#QuantityValue"/>
   <qudt:unit rdf:resource="http://www.qudt.org/2.1/vocab/unit/KiloGM"/>
   <qudt:numericalValue rdf:datatype="http://www.w3.org/2001/XMLSchema#double">8.6</qudt:numericalValue>
   <rdf:value rdf:datatype="http://www.w3.org/2001/XMLSchema#double">8.6</rdf:value>
   <gs1:unitCode>KGM</gs1:unitCode>
   <gs1:value>8.6</gs1:value>
   <rdfs:isDefinedBy rdf:resource="https://rdf.ag/o/beer-ONTOLOGY_DATE"/>
   <void:inDataset rdf:resource="#datasetdefinition"/>
  </gs1:QuantitativeValue>
 </schema:weight>
 <sosa:isFeatureOfInterestOf>
  <rdf:Description rdf:about="#Euro20WeightSosaKG">
   <rdf:type rdf:resource="http://www.w3.org/ns/sosa/Observation"/>
   <sosa:hasFeatureOfInterest rdf:resource="#Euro20"/>
   <sosa:observedProperty  rdf:resource="#grossWeight"/>
   <sosa:hasResult rdf:resource="#Euro20WeightKG"/>
   <sosa:hasSimpleResult rdf:datatype="http://www.qudt.org/2.1/vocab/unit/KiloGM">8.6</sosa:hasSimpleResult>
   <rdfs:isDefinedBy rdf:resource="https://rdf.ag/o/beer-ONTOLOGY_DATE"/>
   <void:inDataset rdf:resource="#datasetdefinition"/>
  </rdf:Description>
 </sosa:isFeatureOfInterestOf>
 <!-- LB Weight -->
 <schema:weight>
  <gs1:QuantitativeValue rdf:about="#Euro20WeightLB">
   <rdf:type rdf:resource="http://qudt.org/1.1/schema/qudt#QuantityValue"/>
   <qudt:unit rdf:resource="http://www.qudt.org/2.1/vocab/unit/LB"/>
   <qudt:numericalValue rdf:datatype="http://www.w3.org/2001/XMLSchema#double">19.0</qudt:numericalValue>
   <rdf:value rdf:datatype="http://www.w3.org/2001/XMLSchema#double">19.0</rdf:value>
   <gs1:unitCode>lbm</gs1:unitCode>
   <gs1:value>19.0</gs1:value>
   <rdfs:isDefinedBy rdf:resource="https://rdf.ag/o/beer-ONTOLOGY_DATE"/>
   <void:inDataset rdf:resource="#datasetdefinition"/>
  </gs1:QuantitativeValue>
 </schema:weight>
 <sosa:isFeatureOfInterestOf>
  <rdf:Description rdf:about="#Euro20WeightSosaLB">
   <rdf:type rdf:resource="http://www.w3.org/ns/sosa/Observation"/>
   <sosa:hasFeatureOfInterest rdf:resource="#Euro20"/>
   <sosa:observedProperty  rdf:resource="#grossWeight"/>
   <sosa:hasResult rdf:resource="#Euro20WeightLB"/>
   <sosa:hasSimpleResult rdf:datatype="http://www.qudt.org/2.1/vocab/unit/LB">19.0</sosa:hasSimpleResult>
   <rdfs:isDefinedBy rdf:resource="https://rdf.ag/o/beer-ONTOLOGY_DATE"/>
   <void:inDataset rdf:resource="#datasetdefinition"/>
  </rdf:Description>
 </sosa:isFeatureOfInterestOf>
 <rdfs:isDefinedBy rdf:resource="https://rdf.ag/o/beer-ONTOLOGY_DATE"/>
 <void:inDataset rdf:resource="#datasetdefinition"/>
</rdf:Description>
<rdf:Description rdf:about="#Euro25">
 <rdf:type rdf:resource="#LiquidContainer"/>
 <rdf:type rdf:resource="#Keg"/>
 <rdf:type rdf:resource="https://gs1.org/voc/PackagingDetails"/>
 <rdfs:label xml:lang="en">European 25L Keg</rdfs:label>
 <rdfs:label xml:lang="fr">Fût Européen 25L</rdfs:label>
 <skos:definition xml:lang="en">European 25L Keg</skos:definition>
 <skos:definition xml:lang="fr">Fût Européen 25L</skos:definition>
 <beer:nominalCapacity rdf:datatype="http://www.qudt.org/2.1/vocab/unit/MilliL">25000</beer:nominalCapacity>
 <sosa:isFeatureOfInterestOf>
  <rdf:Description rdf:about="#Euro25ContentSosaML">
   <rdf:type rdf:resource="http://www.w3.org/ns/sosa/Observation"/>
   <sosa:hasFeatureOfInterest rdf:resource="#Euro25"/>
   <sosa:observedProperty rdf:resource="#sosaNominalCapacity"/>
   <sosa:hasResult>
    <gs1:QuantitativeValue rdf:about="#Euro25ContentML">
     <rdf:type rdf:resource="http://qudt.org/1.1/schema/qudt#QuantityValue"/>
     <gs1:unitCode>MLT</gs1:unitCode>
     <gs1:value>25000</gs1:value>
     <rdf:value rdf:datatype="http://www.w3.org/2001/XMLSchema#double">25000</rdf:value>
     <qudt:unit rdf:resource="http://www.qudt.org/2.1/vocab/unit/MilliL"/>
     <qudt:numericalValue rdf:datatype="http://www.w3.org/2001/XMLSchema#double">25000</qudt:numericalValue>
     <rdfs:isDefinedBy rdf:resource="https://rdf.ag/o/beer-ONTOLOGY_DATE"/>
     <void:inDataset rdf:resource="#datasetdefinition"/>
    </gs1:QuantitativeValue>
   </sosa:hasResult> 
   <sosa:hasSimpleResult rdf:datatype="http://www.qudt.org/2.1/vocab/unit/MilliM">25000</sosa:hasSimpleResult>
   <rdfs:isDefinedBy rdf:resource="https://rdf.ag/o/beer-ONTOLOGY_DATE"/>
   <void:inDataset rdf:resource="#datasetdefinition"/>
  </rdf:Description>
 </sosa:isFeatureOfInterestOf>
 <sosa:isFeatureOfInterestOf>
  <rdf:Description rdf:about="#Euro25ContentSosaOZ">
   <rdf:type rdf:resource="http://www.w3.org/ns/sosa/Observation"/>
   <sosa:hasFeatureOfInterest rdf:resource="#Euro25"/>
   <sosa:observedProperty rdf:resource="#sosaNominalCapacity"/>
   <sosa:hasResult>
   <gs1:QuantitativeValue rdf:about="#Euro25ContentOZ">
    <rdf:type rdf:resource="http://qudt.org/1.1/schema/qudt#QuantityValue"/>
    <gs1:unitCode>foz_us</gs1:unitCode>
    <gs1:value>704</gs1:value>
    <rdf:value rdf:datatype="http://www.w3.org/2001/XMLSchema#double">704</rdf:value>
    <qudt:unit rdf:resource="http://www.qudt.org/2.1/vocab/unit/OZ_VOL_US"/>
    <qudt:numericalValue rdf:datatype="http://www.w3.org/2001/XMLSchema#double">704</qudt:numericalValue>
    <rdfs:isDefinedBy rdf:resource="https://rdf.ag/o/beer-ONTOLOGY_DATE"/>
    <void:inDataset rdf:resource="#datasetdefinition"/>  
   </gs1:QuantitativeValue>
   </sosa:hasResult>
   <sosa:hasSimpleResult rdf:datatype="http://www.qudt.org/2.1/vocab/unit/OZ_VOL_US">704</sosa:hasSimpleResult>
   <rdfs:isDefinedBy rdf:resource="https://rdf.ag/o/beer-ONTOLOGY_DATE"/>
   <void:inDataset rdf:resource="#datasetdefinition"/>  
 </rdf:Description>
 </sosa:isFeatureOfInterestOf>
 <!-- Net Content Gal -->
 <sosa:isFeatureOfInterestOf>
  <rdf:Description rdf:about="#Euro25ContentSosaGAL">
   <rdf:type rdf:resource="http://www.w3.org/ns/sosa/Observation"/>
   <sosa:hasFeatureOfInterest rdf:resource="#Euro25"/>
   <sosa:observedProperty rdf:resource="#netcontent"/>
   <sosa:hasResult>
    <gs1:QuantitativeValue rdf:about="#Euro25ContentGal">
     <rdf:type rdf:resource="http://qudt.org/1.1/schema/qudt#QuantityValue"/>
     <gs1:unitCode>gal_us</gs1:unitCode>
     <gs1:value>5.50</gs1:value>
     <rdf:value rdf:datatype="http://www.w3.org/2001/XMLSchema#double">5.50</rdf:value>
     <qudt:unit rdf:resource="http://www.qudt.org/2.1/vocab/unit/GAL_US"/>
     <qudt:numericalValue rdf:datatype="http://www.w3.org/2001/XMLSchema#double">5.50</qudt:numericalValue>
     <rdfs:isDefinedBy rdf:resource="https://rdf.ag/o/beer-ONTOLOGY_DATE"/>
     <void:inDataset rdf:resource="#datasetdefinition"/>  
    </gs1:QuantitativeValue>
   </sosa:hasResult>
   <sosa:hasSimpleResult rdf:datatype="http://www.qudt.org/2.1/vocab/unit/GAL_US">5.50</sosa:hasSimpleResult>
   <rdfs:isDefinedBy rdf:resource="https://rdf.ag/o/beer-ONTOLOGY_DATE"/>
   <void:inDataset rdf:resource="#datasetdefinition"/>  
 </rdf:Description>
 </sosa:isFeatureOfInterestOf>

 <!-- Height MM-->
 <gs1:inPackageHeight>
  <gs1:QuantitativeValue rdf:about="#Euro25HeightMM">
   <rdf:type rdf:resource="http://qudt.org/1.1/schema/qudt#QuantityValue"/>
   <qudt:unit rdf:resource="http://www.qudt.org/2.1/vocab/unit/MilliM"/>
   <qudt:numericalValue rdf:datatype="http://www.w3.org/2001/XMLSchema#double">327</qudt:numericalValue>
   <rdf:value rdf:datatype="http://www.w3.org/2001/XMLSchema#double">327</rdf:value>
   <gs1:unitCode>MMT</gs1:unitCode>
   <gs1:value>327</gs1:value>
   <rdfs:isDefinedBy rdf:resource="https://rdf.ag/o/beer-ONTOLOGY_DATE"/>
   <void:inDataset rdf:resource="#datasetdefinition"/>
  </gs1:QuantitativeValue>
 </gs1:inPackageHeight>  
 <sosa:isFeatureOfInterestOf>
  <rdf:Description rdf:about="#Euro25HeightSosaMM">
   <rdf:type rdf:resource="http://www.w3.org/ns/sosa/Observation"/>
   <sosa:hasFeatureOfInterest rdf:resource="#Euro25"/>
   <sosa:observedProperty  rdf:resource="#height"/>
   <sosa:hasResult rdf:resource="#Euro25HeightMM"/>
   <sosa:hasSimpleResult rdf:datatype="http://www.qudt.org/2.1/vocab/unit/MilliM">327</sosa:hasSimpleResult>
   <rdfs:isDefinedBy rdf:resource="https://rdf.ag/o/beer-ONTOLOGY_DATE"/>
   <void:inDataset rdf:resource="#datasetdefinition"/>
  </rdf:Description>
 </sosa:isFeatureOfInterestOf>
 <!-- Height IN-->
 <gs1:inPackageHeight>
  <gs1:QuantitativeValue rdf:about="#Euro25HeightIN">
   <rdf:type rdf:resource="http://qudt.org/1.1/schema/qudt#QuantityValue"/>
   <qudt:unit rdf:resource="http://www.qudt.org/2.1/vocab/unit/IN"/>
   <qudt:numericalValue rdf:datatype="http://www.w3.org/2001/XMLSchema#double">12.874</qudt:numericalValue>
   <rdf:value rdf:datatype="http://www.w3.org/2001/XMLSchema#double">12.874</rdf:value>
   <gs1:unitCode>INH</gs1:unitCode>
   <gs1:value>12.874</gs1:value>
   <rdfs:isDefinedBy rdf:resource="https://rdf.ag/o/beer-ONTOLOGY_DATE"/>
   <void:inDataset rdf:resource="#datasetdefinition"/>
  </gs1:QuantitativeValue>
 </gs1:inPackageHeight>  
 <sosa:isFeatureOfInterestOf>
  <rdf:Description rdf:about="#Euro25HeightSosaIN">
   <rdf:type rdf:resource="http://www.w3.org/ns/sosa/Observation"/>
   <sosa:hasFeatureOfInterest rdf:resource="#Euro25"/>
   <sosa:observedProperty  rdf:resource="#height"/>
   <sosa:hasResult rdf:resource="#Euro25HeightIN"/>
   <sosa:hasSimpleResult rdf:datatype="http://www.qudt.org/2.1/vocab/unit/IN">12.874</sosa:hasSimpleResult>
   <rdfs:isDefinedBy rdf:resource="https://rdf.ag/o/beer-ONTOLOGY_DATE"/>
   <void:inDataset rdf:resource="#datasetdefinition"/>
  </rdf:Description>
 </sosa:isFeatureOfInterestOf>
 <!-- Diameter MM --> 
 <gs1:inPackageDiameter>
  <gs1:QuantitativeValue rdf:about="#Euro25DiameterMM">
   <rdf:type rdf:resource="http://qudt.org/1.1/schema/qudt#QuantityValue"/>
   <qudt:unit rdf:resource="http://www.qudt.org/2.1/vocab/unit/MilliM"/>
   <qudt:numericalValue rdf:datatype="http://www.w3.org/2001/XMLSchema#double">395</qudt:numericalValue>
   <rdf:value rdf:datatype="http://www.w3.org/2001/XMLSchema#double">395</rdf:value>
   <gs1:unitCode>MMT</gs1:unitCode>
   <gs1:value>395</gs1:value>
   <rdfs:isDefinedBy rdf:resource="https://rdf.ag/o/beer-ONTOLOGY_DATE"/>
   <void:inDataset rdf:resource="#datasetdefinition"/>
  </gs1:QuantitativeValue>
 </gs1:inPackageDiameter>
 <sosa:isFeatureOfInterestOf>
  <rdf:Description rdf:about="#Euro25DiameterSosaMM">
   <rdf:type rdf:resource="http://www.w3.org/ns/sosa/Observation"/>
   <sosa:hasFeatureOfInterest rdf:resource="#Euro25"/>
   <sosa:observedProperty  rdf:resource="#diameter"/>
   <sosa:hasResult rdf:resource="#Euro25DiameterMM"/>
   <sosa:hasSimpleResult rdf:datatype="http://www.qudt.org/2.1/vocab/unit/MilliM">395</sosa:hasSimpleResult>
   <rdfs:isDefinedBy rdf:resource="https://rdf.ag/o/beer-ONTOLOGY_DATE"/>
   <void:inDataset rdf:resource="#datasetdefinition"/>
  </rdf:Description>
 </sosa:isFeatureOfInterestOf>
 <!-- Diameter IN --> 
 <gs1:inPackageDiameter>
  <gs1:QuantitativeValue rdf:about="#Euro25DiameterIN">
   <rdf:type rdf:resource="http://qudt.org/1.1/schema/qudt#QuantityValue"/>
   <qudt:unit rdf:resource="http://www.qudt.org/2.1/vocab/unit/IN"/>
   <qudt:numericalValue rdf:datatype="http://www.w3.org/2001/XMLSchema#double">15.551</qudt:numericalValue>
   <rdf:value rdf:datatype="http://www.w3.org/2001/XMLSchema#double">15.551</rdf:value>
   <gs1:unitCode>INH</gs1:unitCode>
   <gs1:value>15.551</gs1:value>
   <rdfs:isDefinedBy rdf:resource="https://rdf.ag/o/beer-ONTOLOGY_DATE"/>
   <void:inDataset rdf:resource="#datasetdefinition"/>
  </gs1:QuantitativeValue>
 </gs1:inPackageDiameter>
 <sosa:isFeatureOfInterestOf>
  <rdf:Description rdf:about="#Euro25DiameterSosaIN">
   <rdf:type rdf:resource="http://www.w3.org/ns/sosa/Observation"/>
   <sosa:hasFeatureOfInterest rdf:resource="#Euro25"/>
   <sosa:observedProperty  rdf:resource="#diameter"/>
   <sosa:hasResult rdf:resource="#Euro25DiameterIN"/>
   <sosa:hasSimpleResult rdf:datatype="http://www.qudt.org/2.1/vocab/unit/IN">15.551</sosa:hasSimpleResult>
   <rdfs:isDefinedBy rdf:resource="https://rdf.ag/o/beer-ONTOLOGY_DATE"/>
   <void:inDataset rdf:resource="#datasetdefinition"/>
  </rdf:Description>
 </sosa:isFeatureOfInterestOf>
 <!-- KG Weight -->
 <schema:weight>
  <gs1:QuantitativeValue rdf:about="#Euro25WeightKG">
   <rdf:type rdf:resource="http://qudt.org/1.1/schema/qudt#QuantityValue"/>
   <qudt:unit rdf:resource="http://www.qudt.org/2.1/vocab/unit/KiloGM"/>
   <qudt:numericalValue rdf:datatype="http://www.w3.org/2001/XMLSchema#double">8.9</qudt:numericalValue>
   <rdf:value rdf:datatype="http://www.w3.org/2001/XMLSchema#double">8.9</rdf:value>
   <gs1:unitCode>KGM</gs1:unitCode>
   <gs1:value>8.9</gs1:value>
   <rdfs:isDefinedBy rdf:resource="https://rdf.ag/o/beer-ONTOLOGY_DATE"/>
   <void:inDataset rdf:resource="#datasetdefinition"/>
  </gs1:QuantitativeValue>
 </schema:weight>
 <sosa:isFeatureOfInterestOf>
  <rdf:Description rdf:about="#Euro25WeightSosaKG">
   <rdf:type rdf:resource="http://www.w3.org/ns/sosa/Observation"/>
   <sosa:hasFeatureOfInterest rdf:resource="#Euro25"/>
   <sosa:observedProperty  rdf:resource="#grossWeight"/>
   <sosa:hasResult rdf:resource="#Euro25WeightKG"/>
   <sosa:hasSimpleResult rdf:datatype="http://www.qudt.org/2.1/vocab/unit/KiloGM">8.9</sosa:hasSimpleResult>
   <rdfs:isDefinedBy rdf:resource="https://rdf.ag/o/beer-ONTOLOGY_DATE"/>
   <void:inDataset rdf:resource="#datasetdefinition"/>
  </rdf:Description>
 </sosa:isFeatureOfInterestOf>
 <!-- LB Weight -->
 <schema:weight>
  <gs1:QuantitativeValue rdf:about="#Euro25WeightLB">
   <rdf:type rdf:resource="http://qudt.org/1.1/schema/qudt#QuantityValue"/>
   <qudt:unit rdf:resource="http://www.qudt.org/2.1/vocab/unit/LB"/>
   <qudt:numericalValue rdf:datatype="http://www.w3.org/2001/XMLSchema#double">19.6</qudt:numericalValue>
   <rdf:value rdf:datatype="http://www.w3.org/2001/XMLSchema#double">19.6</rdf:value>
   <gs1:unitCode>lbm</gs1:unitCode>
   <gs1:value>19.6</gs1:value>
   <rdfs:isDefinedBy rdf:resource="https://rdf.ag/o/beer-ONTOLOGY_DATE"/>
   <void:inDataset rdf:resource="#datasetdefinition"/>
  </gs1:QuantitativeValue>
 </schema:weight>
 <sosa:isFeatureOfInterestOf>
  <rdf:Description rdf:about="#Euro25WeightSosaLB">
   <rdf:type rdf:resource="http://www.w3.org/ns/sosa/Observation"/>
   <sosa:hasFeatureOfInterest rdf:resource="#Euro25"/>
   <sosa:observedProperty  rdf:resource="#grossWeight"/>
   <sosa:hasResult rdf:resource="#Euro25WeightLB"/>
   <sosa:hasSimpleResult rdf:datatype="http://www.qudt.org/2.1/vocab/unit/LB">19.6</sosa:hasSimpleResult>
   <rdfs:isDefinedBy rdf:resource="https://rdf.ag/o/beer-ONTOLOGY_DATE"/>
   <void:inDataset rdf:resource="#datasetdefinition"/>
  </rdf:Description>
 </sosa:isFeatureOfInterestOf>
 <rdfs:isDefinedBy rdf:resource="https://rdf.ag/o/beer-ONTOLOGY_DATE"/>
 <void:inDataset rdf:resource="#datasetdefinition"/>
</rdf:Description>
<rdf:Description rdf:about="#Euro30">
 <rdf:type rdf:resource="#LiquidContainer"/>
 <rdf:type rdf:resource="#Keg"/>
 <rdf:type rdf:resource="https://gs1.org/voc/PackagingDetails"/>
 <rdfs:label xml:lang="en">European 30L Keg</rdfs:label>
 <rdfs:label xml:lang="fr">Fût Européen 30L</rdfs:label>
 <skos:definition xml:lang="en">European 30L Keg</skos:definition>
 <skos:definition xml:lang="fr">Fût Européen 30L</skos:definition>
 <beer:nominalCapacity rdf:datatype="http://www.qudt.org/2.1/vocab/unit/MilliL">30000</beer:nominalCapacity>
 <sosa:isFeatureOfInterestOf>
  <rdf:Description rdf:about="#Euro30ContentSosaML">
   <rdf:type rdf:resource="http://www.w3.org/ns/sosa/Observation"/>
   <sosa:hasFeatureOfInterest rdf:resource="#Euro30"/>
   <sosa:observedProperty rdf:resource="#sosaNominalCapacity"/>
   <sosa:hasResult>
    <gs1:QuantitativeValue rdf:about="#Euro30ContentML">
     <rdf:type rdf:resource="http://qudt.org/1.1/schema/qudt#QuantityValue"/>
     <gs1:unitCode>MLT</gs1:unitCode>
     <gs1:value>30000</gs1:value>
     <rdf:value rdf:datatype="http://www.w3.org/2001/XMLSchema#double">30000</rdf:value>
     <qudt:unit rdf:resource="http://www.qudt.org/2.1/vocab/unit/MilliL"/>
     <qudt:numericalValue rdf:datatype="http://www.w3.org/2001/XMLSchema#double">30000</qudt:numericalValue>
     <rdfs:isDefinedBy rdf:resource="https://rdf.ag/o/beer-ONTOLOGY_DATE"/>
     <void:inDataset rdf:resource="#datasetdefinition"/>
    </gs1:QuantitativeValue>
   </sosa:hasResult> 
   <sosa:hasSimpleResult rdf:datatype="http://www.qudt.org/2.1/vocab/unit/MilliM">30000</sosa:hasSimpleResult>
   <rdfs:isDefinedBy rdf:resource="https://rdf.ag/o/beer-ONTOLOGY_DATE"/>
   <void:inDataset rdf:resource="#datasetdefinition"/>
  </rdf:Description>
 </sosa:isFeatureOfInterestOf>
 <sosa:isFeatureOfInterestOf>
  <rdf:Description rdf:about="#Euro30ContentSosaOZ">
   <rdf:type rdf:resource="http://www.w3.org/ns/sosa/Observation"/>
   <sosa:hasFeatureOfInterest rdf:resource="#Euro30"/>
   <sosa:observedProperty rdf:resource="#sosaNominalCapacity"/>
   <sosa:hasResult>
   <gs1:QuantitativeValue rdf:about="#Euro30ContentOZ">
    <rdf:type rdf:resource="http://qudt.org/1.1/schema/qudt#QuantityValue"/>
    <gs1:unitCode>foz_us</gs1:unitCode>
    <gs1:value>845</gs1:value>
    <rdf:value rdf:datatype="http://www.w3.org/2001/XMLSchema#double">845</rdf:value>
    <qudt:unit rdf:resource="http://www.qudt.org/2.1/vocab/unit/OZ_VOL_US"/>
    <qudt:numericalValue rdf:datatype="http://www.w3.org/2001/XMLSchema#double">845</qudt:numericalValue>
    <rdfs:isDefinedBy rdf:resource="https://rdf.ag/o/beer-ONTOLOGY_DATE"/>
    <void:inDataset rdf:resource="#datasetdefinition"/>  
   </gs1:QuantitativeValue>
   </sosa:hasResult>
   <sosa:hasSimpleResult rdf:datatype="http://www.qudt.org/2.1/vocab/unit/OZ_VOL_US">845</sosa:hasSimpleResult>
   <rdfs:isDefinedBy rdf:resource="https://rdf.ag/o/beer-ONTOLOGY_DATE"/>
   <void:inDataset rdf:resource="#datasetdefinition"/>  
 </rdf:Description>
 </sosa:isFeatureOfInterestOf>
 <!-- Net Content Gal -->
 <sosa:isFeatureOfInterestOf>
  <rdf:Description rdf:about="#Euro30ContentSosaGAL">
   <rdf:type rdf:resource="http://www.w3.org/ns/sosa/Observation"/>
   <sosa:hasFeatureOfInterest rdf:resource="#Euro30"/>
   <sosa:observedProperty rdf:resource="#netcontent"/>
   <sosa:hasResult>
    <gs1:QuantitativeValue rdf:about="#Euro30ContentGal">
     <rdf:type rdf:resource="http://qudt.org/1.1/schema/qudt#QuantityValue"/>
     <gs1:unitCode>gal_us</gs1:unitCode>
     <gs1:value>6.60</gs1:value>
     <rdf:value rdf:datatype="http://www.w3.org/2001/XMLSchema#double">6.60</rdf:value>
     <qudt:unit rdf:resource="http://www.qudt.org/2.1/vocab/unit/GAL_US"/>
     <qudt:numericalValue rdf:datatype="http://www.w3.org/2001/XMLSchema#double">6.60</qudt:numericalValue>
     <rdfs:isDefinedBy rdf:resource="https://rdf.ag/o/beer-ONTOLOGY_DATE"/>
     <void:inDataset rdf:resource="#datasetdefinition"/>  
    </gs1:QuantitativeValue>
   </sosa:hasResult>
   <sosa:hasSimpleResult rdf:datatype="http://www.qudt.org/2.1/vocab/unit/GAL_US">6.60</sosa:hasSimpleResult>
   <rdfs:isDefinedBy rdf:resource="https://rdf.ag/o/beer-ONTOLOGY_DATE"/>
   <void:inDataset rdf:resource="#datasetdefinition"/>  
 </rdf:Description>
 </sosa:isFeatureOfInterestOf>

 <!-- Height MM-->
 <gs1:inPackageHeight>
  <gs1:QuantitativeValue rdf:about="#Euro30HeightMM">
   <rdf:type rdf:resource="http://qudt.org/1.1/schema/qudt#QuantityValue"/>
   <qudt:unit rdf:resource="http://www.qudt.org/2.1/vocab/unit/MilliM"/>
   <qudt:numericalValue rdf:datatype="http://www.w3.org/2001/XMLSchema#double">365</qudt:numericalValue>
   <rdf:value rdf:datatype="http://www.w3.org/2001/XMLSchema#double">365</rdf:value>
   <gs1:unitCode>MMT</gs1:unitCode>
   <gs1:value>365</gs1:value>
   <rdfs:isDefinedBy rdf:resource="https://rdf.ag/o/beer-ONTOLOGY_DATE"/>
   <void:inDataset rdf:resource="#datasetdefinition"/>
  </gs1:QuantitativeValue>
 </gs1:inPackageHeight>  
 <sosa:isFeatureOfInterestOf>
  <rdf:Description rdf:about="#Euro30HeightSosaMM">
   <rdf:type rdf:resource="http://www.w3.org/ns/sosa/Observation"/>
   <sosa:hasFeatureOfInterest rdf:resource="#Euro30"/>
   <sosa:observedProperty  rdf:resource="#height"/>
   <sosa:hasResult rdf:resource="#Euro30HeightMM"/>
   <sosa:hasSimpleResult rdf:datatype="http://www.qudt.org/2.1/vocab/unit/MilliM">365</sosa:hasSimpleResult>
   <rdfs:isDefinedBy rdf:resource="https://rdf.ag/o/beer-ONTOLOGY_DATE"/>
   <void:inDataset rdf:resource="#datasetdefinition"/>
  </rdf:Description>
 </sosa:isFeatureOfInterestOf>
 <!-- Height IN-->
 <gs1:inPackageHeight>
  <gs1:QuantitativeValue rdf:about="#Euro30HeightIN">
   <rdf:type rdf:resource="http://qudt.org/1.1/schema/qudt#QuantityValue"/>
   <qudt:unit rdf:resource="http://www.qudt.org/2.1/vocab/unit/IN"/>
   <qudt:numericalValue rdf:datatype="http://www.w3.org/2001/XMLSchema#double">14.370</qudt:numericalValue>
   <rdf:value rdf:datatype="http://www.w3.org/2001/XMLSchema#double">14.370</rdf:value>
   <gs1:unitCode>INH</gs1:unitCode>
   <gs1:value>14.370</gs1:value>
   <rdfs:isDefinedBy rdf:resource="https://rdf.ag/o/beer-ONTOLOGY_DATE"/>
   <void:inDataset rdf:resource="#datasetdefinition"/>
  </gs1:QuantitativeValue>
 </gs1:inPackageHeight>  
 <sosa:isFeatureOfInterestOf>
  <rdf:Description rdf:about="#Euro30HeightSosaIN">
   <rdf:type rdf:resource="http://www.w3.org/ns/sosa/Observation"/>
   <sosa:hasFeatureOfInterest rdf:resource="#Euro30"/>
   <sosa:observedProperty  rdf:resource="#height"/>
   <sosa:hasResult rdf:resource="#Euro30HeightIN"/>
   <sosa:hasSimpleResult rdf:datatype="http://www.qudt.org/2.1/vocab/unit/IN">14.370</sosa:hasSimpleResult>
   <rdfs:isDefinedBy rdf:resource="https://rdf.ag/o/beer-ONTOLOGY_DATE"/>
   <void:inDataset rdf:resource="#datasetdefinition"/>
  </rdf:Description>
 </sosa:isFeatureOfInterestOf>
 <!-- Diameter MM --> 
 <gs1:inPackageDiameter>
  <gs1:QuantitativeValue rdf:about="#Euro30DiameterMM">
   <rdf:type rdf:resource="http://qudt.org/1.1/schema/qudt#QuantityValue"/>
   <qudt:unit rdf:resource="http://www.qudt.org/2.1/vocab/unit/MilliM"/>
   <qudt:numericalValue rdf:datatype="http://www.w3.org/2001/XMLSchema#double">408</qudt:numericalValue>
   <rdf:value rdf:datatype="http://www.w3.org/2001/XMLSchema#double">408</rdf:value>
   <gs1:unitCode>MMT</gs1:unitCode>
   <gs1:value>408</gs1:value>
   <rdfs:isDefinedBy rdf:resource="https://rdf.ag/o/beer-ONTOLOGY_DATE"/>
   <void:inDataset rdf:resource="#datasetdefinition"/>
  </gs1:QuantitativeValue>
 </gs1:inPackageDiameter>
 <sosa:isFeatureOfInterestOf>
  <rdf:Description rdf:about="#Euro30DiameterSosaMM">
   <rdf:type rdf:resource="http://www.w3.org/ns/sosa/Observation"/>
   <sosa:hasFeatureOfInterest rdf:resource="#Euro30"/>
   <sosa:observedProperty  rdf:resource="#diameter"/>
   <sosa:hasResult rdf:resource="#Euro30DiameterMM"/>
   <sosa:hasSimpleResult rdf:datatype="http://www.qudt.org/2.1/vocab/unit/MilliM">408</sosa:hasSimpleResult>
   <rdfs:isDefinedBy rdf:resource="https://rdf.ag/o/beer-ONTOLOGY_DATE"/>
   <void:inDataset rdf:resource="#datasetdefinition"/>
  </rdf:Description>
 </sosa:isFeatureOfInterestOf>
 <!-- Diameter IN --> 
 <gs1:inPackageDiameter>
  <gs1:QuantitativeValue rdf:about="#Euro30DiameterIN">
   <rdf:type rdf:resource="http://qudt.org/1.1/schema/qudt#QuantityValue"/>
   <qudt:unit rdf:resource="http://www.qudt.org/2.1/vocab/unit/IN"/>
   <qudt:numericalValue rdf:datatype="http://www.w3.org/2001/XMLSchema#double">16.063</qudt:numericalValue>
   <rdf:value rdf:datatype="http://www.w3.org/2001/XMLSchema#double">16.063</rdf:value>
   <gs1:unitCode>INH</gs1:unitCode>
   <gs1:value>16.063</gs1:value>
   <rdfs:isDefinedBy rdf:resource="https://rdf.ag/o/beer-ONTOLOGY_DATE"/>
   <void:inDataset rdf:resource="#datasetdefinition"/>
  </gs1:QuantitativeValue>
 </gs1:inPackageDiameter>
 <sosa:isFeatureOfInterestOf>
  <rdf:Description rdf:about="#Euro30DiameterSosaIN">
   <rdf:type rdf:resource="http://www.w3.org/ns/sosa/Observation"/>
   <sosa:hasFeatureOfInterest rdf:resource="#Euro30"/>
   <sosa:observedProperty  rdf:resource="#diameter"/>
   <sosa:hasResult rdf:resource="#Euro30DiameterIN"/>
   <sosa:hasSimpleResult rdf:datatype="http://www.qudt.org/2.1/vocab/unit/IN">16.063</sosa:hasSimpleResult>
   <rdfs:isDefinedBy rdf:resource="https://rdf.ag/o/beer-ONTOLOGY_DATE"/>
   <void:inDataset rdf:resource="#datasetdefinition"/>
  </rdf:Description>
 </sosa:isFeatureOfInterestOf>
 <!-- KG Weight -->
 <schema:weight>
  <gs1:QuantitativeValue rdf:about="#Euro30WeightKG">
   <rdf:type rdf:resource="http://qudt.org/1.1/schema/qudt#QuantityValue"/>
   <qudt:unit rdf:resource="http://www.qudt.org/2.1/vocab/unit/KiloGM"/>
   <qudt:numericalValue rdf:datatype="http://www.w3.org/2001/XMLSchema#double">9.5</qudt:numericalValue>
   <rdf:value rdf:datatype="http://www.w3.org/2001/XMLSchema#double">9.5</rdf:value>
   <gs1:unitCode>KGM</gs1:unitCode>
   <gs1:value>9.5</gs1:value>
   <rdfs:isDefinedBy rdf:resource="https://rdf.ag/o/beer-ONTOLOGY_DATE"/>
   <void:inDataset rdf:resource="#datasetdefinition"/>
  </gs1:QuantitativeValue>
 </schema:weight>
 <sosa:isFeatureOfInterestOf>
  <rdf:Description rdf:about="#Euro30WeightSosaKG">
   <rdf:type rdf:resource="http://www.w3.org/ns/sosa/Observation"/>
   <sosa:hasFeatureOfInterest rdf:resource="#Euro30"/>
   <sosa:observedProperty  rdf:resource="#grossWeight"/>
   <sosa:hasResult rdf:resource="#Euro30WeightKG"/>
   <sosa:hasSimpleResult rdf:datatype="http://www.qudt.org/2.1/vocab/unit/KiloGM">9.5</sosa:hasSimpleResult>
   <rdfs:isDefinedBy rdf:resource="https://rdf.ag/o/beer-ONTOLOGY_DATE"/>
   <void:inDataset rdf:resource="#datasetdefinition"/>
  </rdf:Description>
 </sosa:isFeatureOfInterestOf>
 <!-- LB Weight -->
 <schema:weight>
  <gs1:QuantitativeValue rdf:about="#Euro30WeightLB">
   <rdf:type rdf:resource="http://qudt.org/1.1/schema/qudt#QuantityValue"/>
   <qudt:unit rdf:resource="http://www.qudt.org/2.1/vocab/unit/LB"/>
   <qudt:numericalValue rdf:datatype="http://www.w3.org/2001/XMLSchema#double">20.9</qudt:numericalValue>
   <rdf:value rdf:datatype="http://www.w3.org/2001/XMLSchema#double">20.9</rdf:value>
   <gs1:unitCode>lbm</gs1:unitCode>
   <gs1:value>20.9</gs1:value>
   <rdfs:isDefinedBy rdf:resource="https://rdf.ag/o/beer-ONTOLOGY_DATE"/>
   <void:inDataset rdf:resource="#datasetdefinition"/>
  </gs1:QuantitativeValue>
 </schema:weight>
 <sosa:isFeatureOfInterestOf>
  <rdf:Description rdf:about="#Euro30WeightSosaLB">
   <rdf:type rdf:resource="http://www.w3.org/ns/sosa/Observation"/>
   <sosa:hasFeatureOfInterest rdf:resource="#Euro30"/>
   <sosa:observedProperty  rdf:resource="#grossWeight"/>
   <sosa:hasResult rdf:resource="#Euro30WeightLB"/>
   <sosa:hasSimpleResult rdf:datatype="http://www.qudt.org/2.1/vocab/unit/LB">20.9</sosa:hasSimpleResult>
   <rdfs:isDefinedBy rdf:resource="https://rdf.ag/o/beer-ONTOLOGY_DATE"/>
   <void:inDataset rdf:resource="#datasetdefinition"/>
  </rdf:Description>
 </sosa:isFeatureOfInterestOf>
 <rdfs:isDefinedBy rdf:resource="https://rdf.ag/o/beer-ONTOLOGY_DATE"/>
 <void:inDataset rdf:resource="#datasetdefinition"/>
</rdf:Description>
<rdf:Description rdf:about="#Euro50">
 <rdf:type rdf:resource="#LiquidContainer"/>
 <rdf:type rdf:resource="#Keg"/>
 <rdf:type rdf:resource="https://gs1.org/voc/PackagingDetails"/>
 <rdfs:label xml:lang="en">European 50L Keg</rdfs:label>
 <rdfs:label xml:lang="fr">Fût Européen 50L</rdfs:label>
 <skos:definition xml:lang="en">European 50L Keg</skos:definition>
 <skos:definition xml:lang="fr">Fût Européen 50L</skos:definition>
 <skos:altLabel xml:lang="en">Import Keg</skos:altLabel>
 <beer:nominalCapacity rdf:datatype="http://www.qudt.org/2.1/vocab/unit/MilliL">50000</beer:nominalCapacity>
 <sosa:isFeatureOfInterestOf>
  <rdf:Description rdf:about="#Euro50ContentSosaML">
   <rdf:type rdf:resource="http://www.w3.org/ns/sosa/Observation"/>
   <sosa:hasFeatureOfInterest rdf:resource="#Euro50"/>
   <sosa:observedProperty rdf:resource="#sosaNominalCapacity"/>
   <sosa:hasResult>
    <gs1:QuantitativeValue rdf:about="#Euro50ContentML">
     <rdf:type rdf:resource="http://qudt.org/1.1/schema/qudt#QuantityValue"/>
     <gs1:unitCode>MLT</gs1:unitCode>
     <gs1:value>50000</gs1:value>
     <rdf:value rdf:datatype="http://www.w3.org/2001/XMLSchema#double">50000</rdf:value>
     <qudt:unit rdf:resource="http://www.qudt.org/2.1/vocab/unit/MilliL"/>
     <qudt:numericalValue rdf:datatype="http://www.w3.org/2001/XMLSchema#double">50000</qudt:numericalValue>
     <rdfs:isDefinedBy rdf:resource="https://rdf.ag/o/beer-ONTOLOGY_DATE"/>
     <void:inDataset rdf:resource="#datasetdefinition"/>
    </gs1:QuantitativeValue>
   </sosa:hasResult> 
   <sosa:hasSimpleResult rdf:datatype="http://www.qudt.org/2.1/vocab/unit/MilliM">50000</sosa:hasSimpleResult>
   <rdfs:isDefinedBy rdf:resource="https://rdf.ag/o/beer-ONTOLOGY_DATE"/>
   <void:inDataset rdf:resource="#datasetdefinition"/>
  </rdf:Description>
 </sosa:isFeatureOfInterestOf>
 <sosa:isFeatureOfInterestOf>
  <rdf:Description rdf:about="#Euro50ContentSosaOZ">
   <rdf:type rdf:resource="http://www.w3.org/ns/sosa/Observation"/>
   <sosa:hasFeatureOfInterest rdf:resource="#Euro50"/>
   <sosa:observedProperty rdf:resource="#sosaNominalCapacity"/>
   <sosa:hasResult>
   <gs1:QuantitativeValue rdf:about="#Euro50ContentOZ">
    <rdf:type rdf:resource="http://qudt.org/1.1/schema/qudt#QuantityValue"/>
    <gs1:unitCode>foz_us</gs1:unitCode>
    <gs1:value>1665</gs1:value>
    <rdf:value rdf:datatype="http://www.w3.org/2001/XMLSchema#double">1665</rdf:value>
    <qudt:unit rdf:resource="http://www.qudt.org/2.1/vocab/unit/OZ_VOL_US"/>
    <qudt:numericalValue rdf:datatype="http://www.w3.org/2001/XMLSchema#double">1665</qudt:numericalValue>
    <rdfs:isDefinedBy rdf:resource="https://rdf.ag/o/beer-ONTOLOGY_DATE"/>
    <void:inDataset rdf:resource="#datasetdefinition"/>  
   </gs1:QuantitativeValue>
   </sosa:hasResult>
   <sosa:hasSimpleResult rdf:datatype="http://www.qudt.org/2.1/vocab/unit/OZ_VOL_US">1665</sosa:hasSimpleResult>
   <rdfs:isDefinedBy rdf:resource="https://rdf.ag/o/beer-ONTOLOGY_DATE"/>
   <void:inDataset rdf:resource="#datasetdefinition"/>  
 </rdf:Description>
 </sosa:isFeatureOfInterestOf>
 <!-- Net Content Gal -->
 <sosa:isFeatureOfInterestOf>
  <rdf:Description rdf:about="#Euro50ContentSosaGAL">
   <rdf:type rdf:resource="http://www.w3.org/ns/sosa/Observation"/>
   <sosa:hasFeatureOfInterest rdf:resource="#Euro50"/>
   <sosa:observedProperty rdf:resource="#netcontent"/>
   <sosa:hasResult>
    <gs1:QuantitativeValue rdf:about="#Euro50ContentGal">
     <rdf:type rdf:resource="http://qudt.org/1.1/schema/qudt#QuantityValue"/>
     <gs1:unitCode>gal_us</gs1:unitCode>
     <gs1:value>13.00</gs1:value>
     <rdf:value rdf:datatype="http://www.w3.org/2001/XMLSchema#double">13.00</rdf:value>
     <qudt:unit rdf:resource="http://www.qudt.org/2.1/vocab/unit/GAL_US"/>
     <qudt:numericalValue rdf:datatype="http://www.w3.org/2001/XMLSchema#double">13.00</qudt:numericalValue>
     <rdfs:isDefinedBy rdf:resource="https://rdf.ag/o/beer-ONTOLOGY_DATE"/>
     <void:inDataset rdf:resource="#datasetdefinition"/>  
    </gs1:QuantitativeValue>
   </sosa:hasResult>
   <sosa:hasSimpleResult rdf:datatype="http://www.qudt.org/2.1/vocab/unit/GAL_US">13.00</sosa:hasSimpleResult>
   <rdfs:isDefinedBy rdf:resource="https://rdf.ag/o/beer-ONTOLOGY_DATE"/>
   <void:inDataset rdf:resource="#datasetdefinition"/>  
 </rdf:Description>
 </sosa:isFeatureOfInterestOf>

 <!-- Height MM-->
 <gs1:inPackageHeight>
  <gs1:QuantitativeValue rdf:about="#Euro50HeightMM">
   <rdf:type rdf:resource="http://qudt.org/1.1/schema/qudt#QuantityValue"/>
   <qudt:unit rdf:resource="http://www.qudt.org/2.1/vocab/unit/MilliM"/>
   <qudt:numericalValue rdf:datatype="http://www.w3.org/2001/XMLSchema#double">532</qudt:numericalValue>
   <rdf:value rdf:datatype="http://www.w3.org/2001/XMLSchema#double">532</rdf:value>
   <gs1:unitCode>MMT</gs1:unitCode>
   <gs1:value>532</gs1:value>
   <rdfs:isDefinedBy rdf:resource="https://rdf.ag/o/beer-ONTOLOGY_DATE"/>
   <void:inDataset rdf:resource="#datasetdefinition"/>
  </gs1:QuantitativeValue>
 </gs1:inPackageHeight>  
 <sosa:isFeatureOfInterestOf>
  <rdf:Description rdf:about="#Euro50HeightSosaMM">
   <rdf:type rdf:resource="http://www.w3.org/ns/sosa/Observation"/>
   <sosa:hasFeatureOfInterest rdf:resource="#Euro50"/>
   <sosa:observedProperty  rdf:resource="#height"/>
   <sosa:hasResult rdf:resource="#Euro50HeightMM"/>
   <sosa:hasSimpleResult rdf:datatype="http://www.qudt.org/2.1/vocab/unit/MilliM">532</sosa:hasSimpleResult>
   <rdfs:isDefinedBy rdf:resource="https://rdf.ag/o/beer-ONTOLOGY_DATE"/>
   <void:inDataset rdf:resource="#datasetdefinition"/>
  </rdf:Description>
 </sosa:isFeatureOfInterestOf>
 <!-- Height IN-->
 <gs1:inPackageHeight>
  <gs1:QuantitativeValue rdf:about="#Euro50HeightIN">
   <rdf:type rdf:resource="http://qudt.org/1.1/schema/qudt#QuantityValue"/>
   <qudt:unit rdf:resource="http://www.qudt.org/2.1/vocab/unit/IN"/>
   <qudt:numericalValue rdf:datatype="http://www.w3.org/2001/XMLSchema#double">20.940</qudt:numericalValue>
   <rdf:value rdf:datatype="http://www.w3.org/2001/XMLSchema#double">20.940</rdf:value>
   <gs1:unitCode>INH</gs1:unitCode>
   <gs1:value>20.940</gs1:value>
   <rdfs:isDefinedBy rdf:resource="https://rdf.ag/o/beer-ONTOLOGY_DATE"/>
   <void:inDataset rdf:resource="#datasetdefinition"/>
  </gs1:QuantitativeValue>
 </gs1:inPackageHeight>  
 <sosa:isFeatureOfInterestOf>
  <rdf:Description rdf:about="#Euro50HeightSosaIN">
   <rdf:type rdf:resource="http://www.w3.org/ns/sosa/Observation"/>
   <sosa:hasFeatureOfInterest rdf:resource="#Euro50"/>
   <sosa:observedProperty  rdf:resource="#height"/>
   <sosa:hasResult rdf:resource="#Euro50HeightIN"/>
   <sosa:hasSimpleResult rdf:datatype="http://www.qudt.org/2.1/vocab/unit/IN">20.940</sosa:hasSimpleResult>
   <rdfs:isDefinedBy rdf:resource="https://rdf.ag/o/beer-ONTOLOGY_DATE"/>
   <void:inDataset rdf:resource="#datasetdefinition"/>
  </rdf:Description>
 </sosa:isFeatureOfInterestOf>
 <!-- Diameter MM --> 
 <gs1:inPackageDiameter>
  <gs1:QuantitativeValue rdf:about="#Euro50DiameterMM">
   <rdf:type rdf:resource="http://qudt.org/1.1/schema/qudt#QuantityValue"/>
   <qudt:unit rdf:resource="http://www.qudt.org/2.1/vocab/unit/MilliM"/>
   <qudt:numericalValue rdf:datatype="http://www.w3.org/2001/XMLSchema#double">408</qudt:numericalValue>
   <rdf:value rdf:datatype="http://www.w3.org/2001/XMLSchema#double">408</rdf:value>
   <gs1:unitCode>MMT</gs1:unitCode>
   <gs1:value>408</gs1:value>
   <rdfs:isDefinedBy rdf:resource="https://rdf.ag/o/beer-ONTOLOGY_DATE"/>
   <void:inDataset rdf:resource="#datasetdefinition"/>
  </gs1:QuantitativeValue>
 </gs1:inPackageDiameter>
 <sosa:isFeatureOfInterestOf>
  <rdf:Description rdf:about="#Euro50DiameterSosaMM">
   <rdf:type rdf:resource="http://www.w3.org/ns/sosa/Observation"/>
   <sosa:hasFeatureOfInterest rdf:resource="#Euro50"/>
   <sosa:observedProperty  rdf:resource="#diameter"/>
   <sosa:hasResult rdf:resource="#Euro50DiameterMM"/>
   <sosa:hasSimpleResult rdf:datatype="http://www.qudt.org/2.1/vocab/unit/MilliM">408</sosa:hasSimpleResult>
   <rdfs:isDefinedBy rdf:resource="https://rdf.ag/o/beer-ONTOLOGY_DATE"/>
   <void:inDataset rdf:resource="#datasetdefinition"/>
  </rdf:Description>
 </sosa:isFeatureOfInterestOf>
 <!-- Diameter IN --> 
 <gs1:inPackageDiameter>
  <gs1:QuantitativeValue rdf:about="#Euro50DiameterIN">
   <rdf:type rdf:resource="http://qudt.org/1.1/schema/qudt#QuantityValue"/>
   <qudt:unit rdf:resource="http://www.qudt.org/2.1/vocab/unit/IN"/>
   <qudt:numericalValue rdf:datatype="http://www.w3.org/2001/XMLSchema#double">16.060</qudt:numericalValue>
   <rdf:value rdf:datatype="http://www.w3.org/2001/XMLSchema#double">16.060</rdf:value>
   <gs1:unitCode>INH</gs1:unitCode>
   <gs1:value>16.060</gs1:value>
   <rdfs:isDefinedBy rdf:resource="https://rdf.ag/o/beer-ONTOLOGY_DATE"/>
   <void:inDataset rdf:resource="#datasetdefinition"/>
  </gs1:QuantitativeValue>
 </gs1:inPackageDiameter>
 <sosa:isFeatureOfInterestOf>
  <rdf:Description rdf:about="#Euro50DiameterSosaIN">
   <rdf:type rdf:resource="http://www.w3.org/ns/sosa/Observation"/>
   <sosa:hasFeatureOfInterest rdf:resource="#Euro50"/>
   <sosa:observedProperty  rdf:resource="#diameter"/>
   <sosa:hasResult rdf:resource="#Euro50DiameterIN"/>
   <sosa:hasSimpleResult rdf:datatype="http://www.qudt.org/2.1/vocab/unit/IN">16.060</sosa:hasSimpleResult>
   <rdfs:isDefinedBy rdf:resource="https://rdf.ag/o/beer-ONTOLOGY_DATE"/>
   <void:inDataset rdf:resource="#datasetdefinition"/>
  </rdf:Description>
 </sosa:isFeatureOfInterestOf>
 <!-- KG Weight -->
 <schema:weight>
  <gs1:QuantitativeValue rdf:about="#Euro50WeightKG">
   <rdf:type rdf:resource="http://qudt.org/1.1/schema/qudt#QuantityValue"/>
   <qudt:unit rdf:resource="http://www.qudt.org/2.1/vocab/unit/KiloGM"/>
   <qudt:numericalValue rdf:datatype="http://www.w3.org/2001/XMLSchema#double">12.7</qudt:numericalValue>
   <rdf:value rdf:datatype="http://www.w3.org/2001/XMLSchema#double">12.7</rdf:value>
   <gs1:unitCode>KGM</gs1:unitCode>
   <gs1:value>12.7</gs1:value>
   <rdfs:isDefinedBy rdf:resource="https://rdf.ag/o/beer-ONTOLOGY_DATE"/>
   <void:inDataset rdf:resource="#datasetdefinition"/>
  </gs1:QuantitativeValue>
 </schema:weight>
 <sosa:isFeatureOfInterestOf>
  <rdf:Description rdf:about="#Euro50WeightSosaKG">
   <rdf:type rdf:resource="http://www.w3.org/ns/sosa/Observation"/>
   <sosa:hasFeatureOfInterest rdf:resource="#Euro50"/>
   <sosa:observedProperty  rdf:resource="#grossWeight"/>
   <sosa:hasResult rdf:resource="#Euro50WeightKG"/>
   <sosa:hasSimpleResult rdf:datatype="http://www.qudt.org/2.1/vocab/unit/KiloGM">12.7</sosa:hasSimpleResult>
   <rdfs:isDefinedBy rdf:resource="https://rdf.ag/o/beer-ONTOLOGY_DATE"/>
   <void:inDataset rdf:resource="#datasetdefinition"/>
  </rdf:Description>
 </sosa:isFeatureOfInterestOf>
 <!-- LB Weight -->
 <schema:weight>
  <gs1:QuantitativeValue rdf:about="#Euro50WeightLB">
   <rdf:type rdf:resource="http://qudt.org/1.1/schema/qudt#QuantityValue"/>
   <qudt:unit rdf:resource="http://www.qudt.org/2.1/vocab/unit/LB"/>
   <qudt:numericalValue rdf:datatype="http://www.w3.org/2001/XMLSchema#double">28.0</qudt:numericalValue>
   <rdf:value rdf:datatype="http://www.w3.org/2001/XMLSchema#double">28.0</rdf:value>
   <gs1:unitCode>lbm</gs1:unitCode>
   <gs1:value>28.0</gs1:value>
   <rdfs:isDefinedBy rdf:resource="https://rdf.ag/o/beer-ONTOLOGY_DATE"/>
   <void:inDataset rdf:resource="#datasetdefinition"/>
  </gs1:QuantitativeValue>
 </schema:weight>
 <sosa:isFeatureOfInterestOf>
  <rdf:Description rdf:about="#Euro50WeightSosaLB">
   <rdf:type rdf:resource="http://www.w3.org/ns/sosa/Observation"/>
   <sosa:hasFeatureOfInterest rdf:resource="#Euro50"/>
   <sosa:observedProperty  rdf:resource="#grossWeight"/>
   <sosa:hasResult rdf:resource="#Euro50WeightLB"/>
   <sosa:hasSimpleResult rdf:datatype="http://www.qudt.org/2.1/vocab/unit/LB">28.0</sosa:hasSimpleResult>
   <rdfs:isDefinedBy rdf:resource="https://rdf.ag/o/beer-ONTOLOGY_DATE"/>
   <void:inDataset rdf:resource="#datasetdefinition"/>
  </rdf:Description>
 </sosa:isFeatureOfInterestOf>
 <rdfs:isDefinedBy rdf:resource="https://rdf.ag/o/beer-ONTOLOGY_DATE"/>
 <void:inDataset rdf:resource="#datasetdefinition"/>
</rdf:Description>


<owl:Class rdf:ID="BeverageBottle">
    <rdfs:subClassOf rdf:resource="https://gs1.org/voc/PackagingDetails"/>
    <owl:equivalentClass rdf:resource="http://purl.obolibrary.org/obo/FOODON_03490214"/>
    <rdfs:subClassOf rdf:resource="#LiquidContainer"/>
    <rdfs:label xml:lang="en">Bottle</rdfs:label>
    <rdfs:label xml:lang="fr">Bouteille</rdfs:label>
    <skos:definition xml:lang="en">A container that is usually round and made of glass that has a narrow mouth for serving.</skos:definition>
    <skos:definition xml:lang="fr">Un récipient généralement cylindrique à sa base et en verre, resserré à son sommet.</skos:definition>
    <rdfs:isDefinedBy rdf:resource="https://rdf.ag/o/beer-ONTOLOGY_DATE"/>
    <void:inDataset rdf:resource="#datasetdefinition"/>
</owl:Class>
    
<owl:Class rdf:ID="BeverageCan">
    <owl:equivalentClass rdf:resource="http://purl.obolibrary.org/obo/FOODON_03490204"/>
    <rdfs:subClassOf rdf:resource="#LiquidContainer"/>
    <rdfs:label xml:lang="en">Beverage Can</rdfs:label>
    <rdfs:label xml:lang="fr">Canette</rdfs:label>
    <skos:definition xml:lang="en">A cylindrical metal container mean to hold a liquid.</skos:definition>
    <skos:definition xml:lang="fr">Un contenant métallique pour contenir un liquide.</skos:definition>
    <rdfs:isDefinedBy rdf:resource="https://rdf.ag/o/beer-ONTOLOGY_DATE"/>
    <void:inDataset rdf:resource="#datasetdefinition"/>
</owl:Class>

<rdf:Description rdf:about="#can355ml">
 <rdf:type rdf:resource="#LiquidContainer"/>
 <rdf:type rdf:resource="#BeverageCan"/>
 <rdf:type rdf:resource="https://gs1.org/voc/PackagingDetails"/>
 <rdfs:label xml:lang="en">Any 355ml Can</rdfs:label>
 <rdfs:label xml:lang="fr">Canette à Boisson Métallique, 355ml</rdfs:label>
 <skos:definition xml:lang="en">Any 355ml Can</skos:definition>
 <skos:definition xml:lang="fr">Canette à Boisson Métallique, 355ml</skos:definition>
 <owl:oneOf>
  <rdf:List rdf:about="#can350mlList1">
   <rdf:first rdf:resource="#can355ml204202"/>
   <rdf:rest>
    <rdf:List rdf:about="#can350mlList2">
     <rdf:first rdf:resource="#can355ml207202"/>
     <rdf:rest>
      <rdf:List rdf:about="#can350mlList3">
       <rdf:first rdf:resource="#can355ml211202"/>
       <rdf:rest>
        <rdf:List rdf:about="#can350mlList4">
         <rdf:first rdf:resource="#can355ml-211202413"/>
         <rdf:rest rdf:resource="http://www.w3.org/1999/02/22-rdf-syntax-ns#nil"/>
        </rdf:List>
       </rdf:rest>
      </rdf:List>
     </rdf:rest>
    </rdf:List> 
   </rdf:rest>
  </rdf:List>
 </owl:oneOf>       
</rdf:Description>

<rdf:Description rdf:about="#can355ml204202">
 <rdf:type rdf:resource="https://gs1.org/voc/PackagingDetails"/>
 <rdf:type rdf:resource="#LiquidContainer"/>
 <rdf:type rdf:resource="#BeverageCan"/>
 <rdfs:label xml:lang="en">12oz/355ml Metal Beverage Can</rdfs:label>
 <rdfs:label xml:lang="fr">Canette à Boisson Métallique, 12oz/355ml</rdfs:label>
 <skos:definition xml:lang="en">A one time use 12oz/355ml metal container meant to hold a liquid, commonly referred to as Sleek 204 202 (Height 602).</skos:definition>
 <skos:definition xml:lang="fr">Un contenant non-réutilisable métallique de 12oz/355ml pour contenir un liquide, souvent appeler Sleek 204 202 (Hauteur 602).</skos:definition>
 <!-- Net Content -->
 <gs1:netContent>
  <gs1:QuantitativeValue rdf:about="#can355ml204202-Content">
    <rdf:type rdf:resource="http://qudt.org/1.1/schema/qudt#QuantityValue"/>
    <qudt:unit rdf:resource="http://www.qudt.org/2.1/vocab/unit/MilliL"/>
    <qudt:numericalValue rdf:datatype="http://www.w3.org/2001/XMLSchema#double">355</qudt:numericalValue>
    <rdf:value rdf:datatype="http://www.w3.org/2001/XMLSchema#double">355</rdf:value>
    <gs1:unitCode>MLT</gs1:unitCode>
    <gs1:value>355</gs1:value>
  </gs1:QuantitativeValue>
 </gs1:netContent> 
 <sosa:isFeatureOfInterestOf>
  <rdf:Description rdf:about="#can355ml204202-ContentSosa">
   <rdf:type rdf:resource="http://www.w3.org/ns/sosa/Observation"/>
   <sosa:hasFeatureOfInterest rdf:resource="#can355ml204202"/>
   <sosa:observedProperty  rdf:resource="#netcontent"/>
   <sosa:hasResult rdf:resource="#can355ml204202-Content"/>
   <sosa:hasSimpleResult rdf:datatype="http://www.qudt.org/2.1/vocab/unit/MilliM">355</sosa:hasSimpleResult>
  </rdf:Description>
 </sosa:isFeatureOfInterestOf>
 <!-- Height -->
 <gs1:inPackageHeight>
  <gs1:QuantitativeValue rdf:about="#can355ml204202-Height">
   <rdf:type rdf:resource="http://qudt.org/1.1/schema/qudt#QuantityValue"/>
   <qudt:unit rdf:resource="http://www.qudt.org/2.1/vocab/unit/MilliM"/>
   <qudt:numericalValue rdf:datatype="http://www.w3.org/2001/XMLSchema#double">155.4</qudt:numericalValue>
   <rdf:value rdf:datatype="http://www.w3.org/2001/XMLSchema#double">155.4</rdf:value>
   <gs1:unitCode>MMT</gs1:unitCode>
   <gs1:value>155.4</gs1:value>
  </gs1:QuantitativeValue>
 </gs1:inPackageHeight>  
 <sosa:isFeatureOfInterestOf>
  <rdf:Description rdf:about="#can355ml204202-HeightSosa">
   <rdf:type rdf:resource="http://www.w3.org/ns/sosa/Observation"/>
   <sosa:hasFeatureOfInterest rdf:resource="#can355ml204202"/>
   <sosa:observedProperty  rdf:resource="#height"/>
   <sosa:hasResult rdf:resource="#can355ml204202-Height"/>
   <sosa:hasSimpleResult rdf:datatype="http://www.qudt.org/2.1/vocab/unit/MilliM">155.4</sosa:hasSimpleResult>
  </rdf:Description>
 </sosa:isFeatureOfInterestOf>
 <!-- Diameter --> 
 <gs1:inPackageDiameter>
  <gs1:QuantitativeValue rdf:about="#can355ml204202-Diameter">
   <rdf:type rdf:resource="http://qudt.org/1.1/schema/qudt#QuantityValue"/>
   <qudt:unit rdf:resource="http://www.qudt.org/2.1/vocab/unit/MilliM"/>
   <qudt:numericalValue rdf:datatype="http://www.w3.org/2001/XMLSchema#double">57.5</qudt:numericalValue>
   <rdf:value rdf:datatype="http://www.w3.org/2001/XMLSchema#double">57.5</rdf:value>
   <gs1:unitCode>MMT</gs1:unitCode>
   <gs1:value>57.5</gs1:value>
  </gs1:QuantitativeValue>
 </gs1:inPackageDiameter>
 <sosa:isFeatureOfInterestOf>
  <rdf:Description rdf:about="#can355ml204202-DiameterSosa">
   <rdf:type rdf:resource="http://www.w3.org/ns/sosa/Observation"/>
   <sosa:hasFeatureOfInterest rdf:resource="#can355ml204202"/>
   <sosa:observedProperty  rdf:resource="#diameter"/>
   <sosa:hasResult rdf:resource="#can355ml204202-Diameter"/>
   <sosa:hasSimpleResult rdf:datatype="http://www.qudt.org/2.1/vocab/unit/MilliM">57.5</sosa:hasSimpleResult>
  </rdf:Description>
 </sosa:isFeatureOfInterestOf>
 <sosa:isFeatureOfInterestOf>
  <rdf:Description rdf:about="#can355ml204202-EndDiameterSosa">
   <rdf:type rdf:resource="http://www.w3.org/ns/sosa/Observation"/>
   <sosa:hasFeatureOfInterest rdf:resource="#can355ml204202"/>
   <sosa:observedProperty  rdf:resource="#endDiameter"/>
   <sosa:hasResult>
    <gs1:QuantitativeValue rdf:about="#can355ml204202-EndDiameter">
     <rdf:type rdf:resource="http://qudt.org/1.1/schema/qudt#QuantityValue"/>
     <qudt:unit rdf:resource="http://www.qudt.org/2.1/vocab/unit/MilliM"/>
     <qudt:numericalValue rdf:datatype="http://www.w3.org/2001/XMLSchema#double">53.55</qudt:numericalValue>
     <rdf:value rdf:datatype="http://www.w3.org/2001/XMLSchema#double">53.55</rdf:value>
     <gs1:unitCode>MMT</gs1:unitCode>
     <gs1:value>53.55</gs1:value>
    </gs1:QuantitativeValue>
   </sosa:hasResult>
   <sosa:hasSimpleResult rdf:datatype="http://www.qudt.org/2.1/vocab/unit/MilliM">53.55</sosa:hasSimpleResult>
  </rdf:Description>
 </sosa:isFeatureOfInterestOf>
 <rdfs:isDefinedBy rdf:resource="https://rdf.ag/o/beer-ONTOLOGY_DATE"/>
 <void:inDataset rdf:resource="#datasetdefinition"/>
</rdf:Description>


<rdf:Description rdf:about="#can355ml207202">
 <rdf:type rdf:resource="https://gs1.org/voc/PackagingDetails"/>
 <rdf:type rdf:resource="#LiquidContainer"/>
 <rdf:type rdf:resource="#BeverageCan"/>
 <rdfs:label xml:lang="en">12oz/355ml Metal Beverage Can</rdfs:label>
 <rdfs:label xml:lang="fr">Canette à Boisson Métallique, 12oz/355ml</rdfs:label>
 <skos:definition xml:lang="en">A one time use 12oz/355ml metal container meant to hold a liquid, commonly referred to as Sleek 207 202 (Height 510).</skos:definition>
 <skos:definition xml:lang="fr">Un contenant non-réutilisable métallique de 12oz/355ml pour contenir un liquide, souvent appeler Sleek 207 202 (Hauteur 510).</skos:definition>
 <!-- Net Content -->
 <gs1:netContent>
  <gs1:QuantitativeValue rdf:about="#can355ml207202-Content">
    <rdf:type rdf:resource="http://qudt.org/1.1/schema/qudt#QuantityValue"/>
    <qudt:unit rdf:resource="http://www.qudt.org/2.1/vocab/unit/MilliL"/>
    <qudt:numericalValue rdf:datatype="http://www.w3.org/2001/XMLSchema#double">355</qudt:numericalValue>
    <rdf:value rdf:datatype="http://www.w3.org/2001/XMLSchema#double">355</rdf:value>
    <gs1:unitCode>MLT</gs1:unitCode>
    <gs1:value>355</gs1:value>
  </gs1:QuantitativeValue>
 </gs1:netContent> 
 <sosa:isFeatureOfInterestOf>
  <rdf:Description rdf:about="#can355ml207202-ContentSosa">
   <rdf:type rdf:resource="http://www.w3.org/ns/sosa/Observation"/>
   <sosa:hasFeatureOfInterest rdf:resource="#can355ml207202"/>
   <sosa:observedProperty  rdf:resource="#netcontent"/>
   <sosa:hasResult rdf:resource="#can355ml207202-Content"/>
   <sosa:hasSimpleResult rdf:datatype="http://www.qudt.org/2.1/vocab/unit/MilliM">355</sosa:hasSimpleResult>
  </rdf:Description>
 </sosa:isFeatureOfInterestOf>
 <!-- Height -->
 <gs1:inPackageHeight>
  <gs1:QuantitativeValue rdf:about="#can355ml207202-Height">
   <rdf:type rdf:resource="http://qudt.org/1.1/schema/qudt#QuantityValue"/>
   <qudt:unit rdf:resource="http://www.qudt.org/2.1/vocab/unit/MilliM"/>
   <qudt:numericalValue rdf:datatype="http://www.w3.org/2001/XMLSchema#double">143</qudt:numericalValue>
   <rdf:value rdf:datatype="http://www.w3.org/2001/XMLSchema#double">143</rdf:value>
   <gs1:unitCode>MMT</gs1:unitCode>
   <gs1:value>143</gs1:value>
  </gs1:QuantitativeValue>
 </gs1:inPackageHeight>  
 <sosa:isFeatureOfInterestOf>
  <rdf:Description rdf:about="#can355ml207202-HeightSosa">
   <rdf:type rdf:resource="http://www.w3.org/ns/sosa/Observation"/>
   <sosa:hasFeatureOfInterest rdf:resource="#can355ml207202"/>
   <sosa:observedProperty  rdf:resource="#height"/>
   <sosa:hasResult rdf:resource="#can355ml207202-Height"/>
   <sosa:hasSimpleResult rdf:datatype="http://www.qudt.org/2.1/vocab/unit/MilliM">143</sosa:hasSimpleResult>
  </rdf:Description>
 </sosa:isFeatureOfInterestOf>
 <!-- Diameter --> 
 <gs1:inPackageDiameter>
  <gs1:QuantitativeValue rdf:about="#can355ml207202-Diameter">
   <rdf:type rdf:resource="http://qudt.org/1.1/schema/qudt#QuantityValue"/>
   <qudt:unit rdf:resource="http://www.qudt.org/2.1/vocab/unit/MilliM"/>
   <qudt:numericalValue rdf:datatype="http://www.w3.org/2001/XMLSchema#double">60.1</qudt:numericalValue>
   <rdf:value rdf:datatype="http://www.w3.org/2001/XMLSchema#double">60.1</rdf:value>
   <gs1:unitCode>MMT</gs1:unitCode>
   <gs1:value>60.1</gs1:value>
  </gs1:QuantitativeValue>
 </gs1:inPackageDiameter>
 <sosa:isFeatureOfInterestOf>
  <rdf:Description rdf:about="#can355ml207202-DiameterSosa">
   <rdf:type rdf:resource="http://www.w3.org/ns/sosa/Observation"/>
   <sosa:hasFeatureOfInterest rdf:resource="#can355ml207202"/>
   <sosa:observedProperty  rdf:resource="#diameter"/>
   <sosa:hasResult rdf:resource="#can355ml207202-Diameter"/>
   <sosa:hasSimpleResult rdf:datatype="http://www.qudt.org/2.1/vocab/unit/MilliM">60.1</sosa:hasSimpleResult>
  </rdf:Description>
 </sosa:isFeatureOfInterestOf>
 <sosa:isFeatureOfInterestOf>
  <rdf:Description rdf:about="#can355ml207202-EndDiameterSosa">
   <rdf:type rdf:resource="http://www.w3.org/ns/sosa/Observation"/>
   <sosa:hasFeatureOfInterest rdf:resource="#can355ml207202"/>
   <sosa:observedProperty  rdf:resource="#endDiameter"/>
   <sosa:hasResult>
    <gs1:QuantitativeValue rdf:about="#can355ml207202-EndDiameter">
     <rdf:type rdf:resource="http://qudt.org/1.1/schema/qudt#QuantityValue"/>
     <qudt:unit rdf:resource="http://www.qudt.org/2.1/vocab/unit/MilliM"/>
     <qudt:numericalValue rdf:datatype="http://www.w3.org/2001/XMLSchema#double">53.55</qudt:numericalValue>
     <rdf:value rdf:datatype="http://www.w3.org/2001/XMLSchema#double">53.55</rdf:value>
     <gs1:unitCode>MMT</gs1:unitCode>
     <gs1:value>53.55</gs1:value>
    </gs1:QuantitativeValue>
   </sosa:hasResult>
   <sosa:hasSimpleResult rdf:datatype="http://www.qudt.org/2.1/vocab/unit/MilliM">53.55</sosa:hasSimpleResult>
  </rdf:Description>
 </sosa:isFeatureOfInterestOf>
 <rdfs:isDefinedBy rdf:resource="https://rdf.ag/o/beer-ONTOLOGY_DATE"/>
 <void:inDataset rdf:resource="#datasetdefinition"/>
</rdf:Description>


<rdf:Description rdf:about="#can355ml211202">
 <rdf:type rdf:resource="https://gs1.org/voc/PackagingDetails"/>
 <rdf:type rdf:resource="#LiquidContainer"/>
 <rdf:type rdf:resource="#BeverageCan"/>
 <rdfs:label xml:lang="en">12oz/355ml Metal Beverage Can</rdfs:label>
 <rdfs:label xml:lang="fr">Canette à Boisson Métallique, 12oz/355ml</rdfs:label>
 <skos:definition xml:lang="en">A one time use 12oz/355ml metal container meant to hold a liquid, commonly referred to as Sleek 211-202 (Height 413).</skos:definition>
 <skos:definition xml:lang="fr">Un contenant non-réutilisable métallique de 12oz/355ml pour contenir un liquide, souvent appeler Sleek 211-202 (Hauteur 413).</skos:definition>
 <!-- Net Content -->
 <gs1:netContent>
  <gs1:QuantitativeValue rdf:about="#can355ml211202-Content">
    <rdf:type rdf:resource="http://qudt.org/1.1/schema/qudt#QuantityValue"/>
    <qudt:unit rdf:resource="http://www.qudt.org/2.1/vocab/unit/MilliL"/>
    <qudt:numericalValue rdf:datatype="http://www.w3.org/2001/XMLSchema#double">355</qudt:numericalValue>
    <rdf:value rdf:datatype="http://www.w3.org/2001/XMLSchema#double">355</rdf:value>
    <gs1:unitCode>MLT</gs1:unitCode>
    <gs1:value>355</gs1:value>
  </gs1:QuantitativeValue>
 </gs1:netContent> 
 <sosa:isFeatureOfInterestOf>
  <rdf:Description rdf:about="#can355ml211202-ContentSosa">
   <rdf:type rdf:resource="http://www.w3.org/ns/sosa/Observation"/>
   <sosa:hasFeatureOfInterest rdf:resource="#can355ml211202"/>
   <sosa:observedProperty  rdf:resource="#netcontent"/>
   <sosa:hasResult rdf:resource="#can355ml211202-Content"/>
   <sosa:hasSimpleResult rdf:datatype="http://www.qudt.org/2.1/vocab/unit/MilliM">355</sosa:hasSimpleResult>
  </rdf:Description>
 </sosa:isFeatureOfInterestOf>
 <!-- Height -->
 <gs1:inPackageHeight>
  <gs1:QuantitativeValue rdf:about="#can355ml211202-Height">
   <rdf:type rdf:resource="http://qudt.org/1.1/schema/qudt#QuantityValue"/>
   <qudt:unit rdf:resource="http://www.qudt.org/2.1/vocab/unit/MilliM"/>
   <qudt:numericalValue rdf:datatype="http://www.w3.org/2001/XMLSchema#double">122.4</qudt:numericalValue>
   <rdf:value rdf:datatype="http://www.w3.org/2001/XMLSchema#double">122.4</rdf:value>
   <gs1:unitCode>MMT</gs1:unitCode>
   <gs1:value>122.4</gs1:value>
  </gs1:QuantitativeValue>
 </gs1:inPackageHeight>  
 <sosa:isFeatureOfInterestOf>
  <rdf:Description rdf:about="#can355ml211202-HeightSosa">
   <rdf:type rdf:resource="http://www.w3.org/ns/sosa/Observation"/>
   <sosa:hasFeatureOfInterest rdf:resource="#can355ml211202"/>
   <sosa:observedProperty  rdf:resource="#height"/>
   <sosa:hasResult rdf:resource="#can355ml211202-Height"/>
   <sosa:hasSimpleResult rdf:datatype="http://www.qudt.org/2.1/vocab/unit/MilliM">122.4</sosa:hasSimpleResult>
  </rdf:Description>
 </sosa:isFeatureOfInterestOf>
 <!-- Diameter --> 
 <gs1:inPackageDiameter>
  <gs1:QuantitativeValue rdf:about="#can355ml211202-Diameter">
   <rdf:type rdf:resource="http://qudt.org/1.1/schema/qudt#QuantityValue"/>
   <qudt:unit rdf:resource="http://www.qudt.org/2.1/vocab/unit/MilliM"/>
   <qudt:numericalValue rdf:datatype="http://www.w3.org/2001/XMLSchema#double">66</qudt:numericalValue>
   <rdf:value rdf:datatype="http://www.w3.org/2001/XMLSchema#double">66</rdf:value>
   <gs1:unitCode>MMT</gs1:unitCode>
   <gs1:value>66</gs1:value>
  </gs1:QuantitativeValue>
 </gs1:inPackageDiameter>
 <sosa:isFeatureOfInterestOf>
  <rdf:Description rdf:about="#can355ml211202-DiameterSosa">
   <rdf:type rdf:resource="http://www.w3.org/ns/sosa/Observation"/>
   <sosa:hasFeatureOfInterest rdf:resource="#can355ml211202"/>
   <sosa:observedProperty  rdf:resource="#diameter"/>
   <sosa:hasResult rdf:resource="#can355ml211202-Diameter"/>
   <sosa:hasSimpleResult rdf:datatype="http://www.qudt.org/2.1/vocab/unit/MilliM">66</sosa:hasSimpleResult>
  </rdf:Description>
 </sosa:isFeatureOfInterestOf>
 <sosa:isFeatureOfInterestOf>
  <rdf:Description rdf:about="#can355ml211202-EndDiameterSosa">
   <rdf:type rdf:resource="http://www.w3.org/ns/sosa/Observation"/>
   <sosa:hasFeatureOfInterest rdf:resource="#can355ml211202"/>
   <sosa:observedProperty  rdf:resource="#endDiameter"/>
   <sosa:hasResult>
    <gs1:QuantitativeValue rdf:about="#can355ml211202-EndDiameter">
     <rdf:type rdf:resource="http://qudt.org/1.1/schema/qudt#QuantityValue"/>
     <qudt:unit rdf:resource="http://www.qudt.org/2.1/vocab/unit/MilliM"/>
     <qudt:numericalValue rdf:datatype="http://www.w3.org/2001/XMLSchema#double">53.55</qudt:numericalValue>
     <rdf:value rdf:datatype="http://www.w3.org/2001/XMLSchema#double">53.55</rdf:value>
     <gs1:unitCode>MMT</gs1:unitCode>
     <gs1:value>53.55</gs1:value>
    </gs1:QuantitativeValue>
   </sosa:hasResult>
   <sosa:hasSimpleResult rdf:datatype="http://www.qudt.org/2.1/vocab/unit/MilliM">53.55</sosa:hasSimpleResult>
  </rdf:Description>
 </sosa:isFeatureOfInterestOf>
 <rdfs:isDefinedBy rdf:resource="https://rdf.ag/o/beer-ONTOLOGY_DATE"/>
 <void:inDataset rdf:resource="#datasetdefinition"/>
</rdf:Description>



<rdf:Description rdf:about="#can355ml-211202413">
 <rdf:type rdf:resource="https://gs1.org/voc/PackagingDetails"/>
 <rdf:type rdf:resource="#LiquidContainer"/>
 <rdf:type rdf:resource="#BeverageCan"/>
 <rdfs:label xml:lang="en">12oz/355ml Metal Beverage Can</rdfs:label>
 <rdfs:label xml:lang="fr">Canette à Boisson Métallique, 12oz/355ml</rdfs:label>
 <skos:definition xml:lang="en">A one time use 12oz/355ml metal container meant to hold a liquid, commonly referred to as 202-211 (413 Height).</skos:definition>
 <skos:definition xml:lang="fr">Un contenant non-réutilisable métallique de 12oz/355ml pour contenir un liquide, souvent appeler 202-211 (Hauteur 413).</skos:definition>
 <!-- Net Content -->
 <gs1:netContent>
  <gs1:QuantitativeValue rdf:about="#can355ml-211202413-Content">
    <rdf:type rdf:resource="http://qudt.org/1.1/schema/qudt#QuantityValue"/>
    <gs1:unitCode>MLT</gs1:unitCode>
    <gs1:value>355</gs1:value>
    <rdf:value rdf:datatype="http://www.w3.org/2001/XMLSchema#double">355</rdf:value>
    <qudt:unit rdf:resource="http://www.qudt.org/2.1/vocab/unit/MilliL"/>
    <qudt:numericalValue rdf:datatype="http://www.w3.org/2001/XMLSchema#double">355</qudt:numericalValue>
  </gs1:QuantitativeValue>
 </gs1:netContent> 
 <sosa:isFeatureOfInterestOf>
  <rdf:Description rdf:about="#can355ml-211202413-ContentSosa">
   <rdf:type rdf:resource="http://www.w3.org/ns/sosa/Observation"/>
   <sosa:hasFeatureOfInterest rdf:resource="#can355ml-211202413"/>
   <sosa:observedProperty  rdf:resource="#netcontent"/>
   <sosa:hasResult rdf:resource="#can355ml-211202413-Content"/>
   <sosa:hasSimpleResult rdf:datatype="http://www.qudt.org/2.1/vocab/unit/MilliM">355</sosa:hasSimpleResult>
  </rdf:Description>
 </sosa:isFeatureOfInterestOf>
 <!-- Height -->
 <gs1:inPackageHeight>
  <gs1:QuantitativeValue rdf:about="#can355ml-211202413-Height">
   <rdf:type rdf:resource="http://qudt.org/1.1/schema/qudt#QuantityValue"/>
   <qudt:unit rdf:resource="http://www.qudt.org/2.1/vocab/unit/MilliM"/>
   <qudt:numericalValue rdf:datatype="http://www.w3.org/2001/XMLSchema#double">115.0</qudt:numericalValue>
   <rdf:value rdf:datatype="http://www.w3.org/2001/XMLSchema#double">115.0</rdf:value>
   <gs1:unitCode>MMT</gs1:unitCode>
   <gs1:value>115.0</gs1:value>
  </gs1:QuantitativeValue>
 </gs1:inPackageHeight>  
 <sosa:isFeatureOfInterestOf>
  <rdf:Description rdf:about="#can355ml-211202413-HeightSosa">
   <rdf:type rdf:resource="http://www.w3.org/ns/sosa/Observation"/>
   <sosa:hasFeatureOfInterest rdf:resource="#can355ml-211202413"/>
   <sosa:observedProperty  rdf:resource="#height"/>
   <sosa:hasResult rdf:resource="#can355ml-211202413-Height"/>
   <sosa:hasSimpleResult rdf:datatype="http://www.qudt.org/2.1/vocab/unit/MilliM">115.0</sosa:hasSimpleResult>
  </rdf:Description>
 </sosa:isFeatureOfInterestOf>
 <!-- Diameter --> 
 <gs1:inPackageDiameter>
  <gs1:QuantitativeValue rdf:about="#can355ml-211202413-Diameter">
   <rdf:type rdf:resource="http://qudt.org/1.1/schema/qudt#QuantityValue"/>
   <qudt:unit rdf:resource="http://www.qudt.org/2.1/vocab/unit/MilliM"/>
   <qudt:numericalValue rdf:datatype="http://www.w3.org/2001/XMLSchema#double">68.262</qudt:numericalValue>
   <rdf:value rdf:datatype="http://www.w3.org/2001/XMLSchema#double">68.262</rdf:value>
   <gs1:unitCode>MMT</gs1:unitCode>
   <gs1:value>68.262</gs1:value>
  </gs1:QuantitativeValue>
 </gs1:inPackageDiameter>
 <sosa:isFeatureOfInterestOf>
  <rdf:Description rdf:about="#can355ml-211202413-DiameterSosa">
   <rdf:type rdf:resource="http://www.w3.org/ns/sosa/Observation"/>
   <sosa:hasFeatureOfInterest rdf:resource="#can355ml-211202413"/>
   <sosa:observedProperty  rdf:resource="#diameter"/>
   <sosa:hasResult rdf:resource="#can355ml-211202413-Diameter"/>
   <sosa:hasSimpleResult rdf:datatype="http://www.qudt.org/2.1/vocab/unit/MilliM">68.252</sosa:hasSimpleResult>
  </rdf:Description>
 </sosa:isFeatureOfInterestOf>
 <sosa:isFeatureOfInterestOf>
  <rdf:Description rdf:about="#can355ml-211202413-EndDiameterSosa">
   <rdf:type rdf:resource="http://www.w3.org/ns/sosa/Observation"/>
   <sosa:hasFeatureOfInterest rdf:resource="#can355ml-211202413"/>
   <sosa:observedProperty  rdf:resource="#endDiameter"/>
   <sosa:hasResult>
    <gs1:QuantitativeValue rdf:about="#can355ml-211202413-EndDiameter">
     <rdf:type rdf:resource="http://qudt.org/1.1/schema/qudt#QuantityValue"/>
     <qudt:unit rdf:resource="http://www.qudt.org/2.1/vocab/unit/MilliM"/>
     <qudt:numericalValue rdf:datatype="http://www.w3.org/2001/XMLSchema#double">55.033164</qudt:numericalValue>
     <rdf:value rdf:datatype="http://www.w3.org/2001/XMLSchema#double">55.033164</rdf:value>
     <gs1:unitCode>MMT</gs1:unitCode>
     <gs1:value>55.033164</gs1:value>
    </gs1:QuantitativeValue>
   </sosa:hasResult>
   <sosa:hasSimpleResult rdf:datatype="http://www.qudt.org/2.1/vocab/unit/MilliM">55.033164</sosa:hasSimpleResult>
  </rdf:Description>
 </sosa:isFeatureOfInterestOf> 
 <rdfs:isDefinedBy rdf:resource="https://rdf.ag/o/beer-ONTOLOGY_DATE"/>
 <void:inDataset rdf:resource="#datasetdefinition"/>
</rdf:Description>

<rdf:Description rdf:about="#can473">
 <rdf:type rdf:resource="https://gs1.org/voc/PackagingDetails"/>
 <rdf:type rdf:resource="#LiquidContainer"/>
 <rdf:type rdf:resource="#BeverageCan"/>
 <rdfs:label xml:lang="en">16oz/473ml Metal Beverage Can</rdfs:label>
 <rdfs:label xml:lang="fr">Canette à Boisson Métallique, 16oz/473ml</rdfs:label>
 <skos:definition xml:lang="en">A one time use 16oz/473ml metal container meant to hold a liquid, commonly referred to as 202-211 (Height 603).</skos:definition>
 <skos:definition xml:lang="fr">Un contenant non-réutilisable métallique de 16oz/473ml pour contenir un liquide, souvent appeler 202-211 (Hauteur 603).</skos:definition>
 <!-- Net Content -->
 <gs1:netContent>
  <gs1:QuantitativeValue rdf:about="#can473Content">
    <rdf:type rdf:resource="http://qudt.org/1.1/schema/qudt#QuantityValue"/>
    <qudt:unit rdf:resource="http://www.qudt.org/2.1/vocab/unit/MilliL"/>
    <qudt:numericalValue rdf:datatype="http://www.w3.org/2001/XMLSchema#double">473</qudt:numericalValue>
    <rdf:value rdf:datatype="http://www.w3.org/2001/XMLSchema#double">473</rdf:value>
    <gs1:unitCode>MLT</gs1:unitCode>
    <gs1:value>473</gs1:value>
  </gs1:QuantitativeValue>
 </gs1:netContent> 
 <sosa:isFeatureOfInterestOf>
  <rdf:Description rdf:about="#can473ContentSosa">
   <rdf:type rdf:resource="http://www.w3.org/ns/sosa/Observation"/>
   <sosa:hasFeatureOfInterest rdf:resource="#can473"/>
   <sosa:observedProperty  rdf:resource="#netcontent"/>
   <sosa:hasResult rdf:resource="#can473Content"/>
   <sosa:hasSimpleResult rdf:datatype="http://www.qudt.org/2.1/vocab/unit/MilliM">473</sosa:hasSimpleResult>
  </rdf:Description>
 </sosa:isFeatureOfInterestOf>
 <!-- Height -->
 <gs1:inPackageHeight>
  <gs1:QuantitativeValue rdf:about="#can473Height">
   <rdf:type rdf:resource="http://qudt.org/1.1/schema/qudt#QuantityValue"/>
   <qudt:unit rdf:resource="http://www.qudt.org/2.1/vocab/unit/MilliM"/>
   <qudt:numericalValue rdf:datatype="http://www.w3.org/2001/XMLSchema#double">158.75</qudt:numericalValue>
   <rdf:value rdf:datatype="http://www.w3.org/2001/XMLSchema#double">158.75</rdf:value>
   <gs1:unitCode>MMT</gs1:unitCode>
   <gs1:value>158.75</gs1:value>
  </gs1:QuantitativeValue>
 </gs1:inPackageHeight>  
 <sosa:isFeatureOfInterestOf>
  <rdf:Description rdf:about="#can473HeightSosa">
   <rdf:type rdf:resource="http://www.w3.org/ns/sosa/Observation"/>
   <sosa:hasFeatureOfInterest rdf:resource="#can473"/>
   <sosa:observedProperty  rdf:resource="#height"/>
   <sosa:hasResult rdf:resource="#can473Height"/>
   <sosa:hasSimpleResult rdf:datatype="http://www.qudt.org/2.1/vocab/unit/MilliM">158.75</sosa:hasSimpleResult>
  </rdf:Description>
 </sosa:isFeatureOfInterestOf>
 <!-- Diameter --> 
 <gs1:inPackageDiameter>
  <gs1:QuantitativeValue rdf:about="#can473Diameter">
   <rdf:type rdf:resource="http://qudt.org/1.1/schema/qudt#QuantityValue"/>
   <qudt:unit rdf:resource="http://www.qudt.org/2.1/vocab/unit/MilliM"/>
   <qudt:numericalValue rdf:datatype="http://www.w3.org/2001/XMLSchema#double">68.262</qudt:numericalValue>
   <rdf:value rdf:datatype="http://www.w3.org/2001/XMLSchema#double">68.262</rdf:value>
   <gs1:unitCode>MMT</gs1:unitCode>
   <gs1:value>68.262</gs1:value>
  </gs1:QuantitativeValue>
 </gs1:inPackageDiameter>
 <sosa:isFeatureOfInterestOf>
  <rdf:Description rdf:about="#can473DiameterSosa">
   <rdf:type rdf:resource="http://www.w3.org/ns/sosa/Observation"/>
   <sosa:hasFeatureOfInterest rdf:resource="#can473"/>
   <sosa:observedProperty  rdf:resource="#diameter"/>
   <sosa:hasResult rdf:resource="#can473Diameter"/>
   <sosa:hasSimpleResult rdf:datatype="http://www.qudt.org/2.1/vocab/unit/MilliM">68.262</sosa:hasSimpleResult>
  </rdf:Description>
 </sosa:isFeatureOfInterestOf>
 <sosa:isFeatureOfInterestOf>
  <rdf:Description rdf:about="#can473EndDiameterSosa">
   <rdf:type rdf:resource="http://www.w3.org/ns/sosa/Observation"/>
   <sosa:hasFeatureOfInterest rdf:resource="#can473"/>
   <sosa:observedProperty  rdf:resource="#endDiameter"/>
   <sosa:hasResult>
    <gs1:QuantitativeValue rdf:about="#can473EndDiameter">
     <rdf:type rdf:resource="http://qudt.org/1.1/schema/qudt#QuantityValue"/>
     <qudt:unit rdf:resource="http://www.qudt.org/2.1/vocab/unit/MilliM"/>
     <qudt:numericalValue rdf:datatype="http://www.w3.org/2001/XMLSchema#double">55.033164</qudt:numericalValue>
     <rdf:value rdf:datatype="http://www.w3.org/2001/XMLSchema#double">55.033164</rdf:value>
     <gs1:unitCode>MMT</gs1:unitCode>
     <gs1:value>55.033164</gs1:value>
    </gs1:QuantitativeValue>
   </sosa:hasResult>
   <sosa:hasSimpleResult rdf:datatype="http://www.qudt.org/2.1/vocab/unit/MilliM">55.033164</sosa:hasSimpleResult>
  </rdf:Description>
 </sosa:isFeatureOfInterestOf>
 <rdfs:isDefinedBy rdf:resource="https://rdf.ag/o/beer-ONTOLOGY_DATE"/>
 <void:inDataset rdf:resource="#datasetdefinition"/>
</rdf:Description>

<rdf:Description rdf:about="#can500ml">
 <rdf:type rdf:resource="#LiquidContainer"/>
 <rdf:type rdf:resource="#BeverageCan"/>
 <rdf:type rdf:resource="https://gs1.org/voc/PackagingDetails"/>
 <rdfs:label xml:lang="en">Any 500ml Can</rdfs:label>
 <rdfs:label xml:lang="fr">Canette à Boisson Métallique, 500ml</rdfs:label>
 <skos:definition xml:lang="en">Any 500ml Can</skos:definition>
 <skos:definition xml:lang="fr">Canette à Boisson Métallique, 500ml</skos:definition>
 <owl:oneOf>
  <rdf:List rdf:about="#can500mlList1">
   <rdf:first rdf:resource="#can500ml211206"/>
   <rdf:rest>
    <rdf:List rdf:about="#can500mlList2">
     <rdf:first rdf:resource="#can500ml211202673"/>
     <rdf:rest rdf:resource="http://www.w3.org/1999/02/22-rdf-syntax-ns#nil"/>
    </rdf:List>
   </rdf:rest>
  </rdf:List>
 </owl:oneOf>       
</rdf:Description>


<rdf:Description rdf:about="#can500ml211206">
 <rdf:type rdf:resource="https://gs1.org/voc/PackagingDetails"/>
 <rdf:type rdf:resource="#LiquidContainer"/>
 <rdf:type rdf:resource="#BeverageCan"/>
 <rdfs:label xml:lang="en">16.9oz/500ml Metal Beverage Can</rdfs:label>
 <rdfs:label xml:lang="fr">Canette à Boisson Métallique, 16.9oz/500ml</rdfs:label>
 <skos:definition xml:lang="en">A one time use 16.9oz/500ml metal container meant to hold a liquid, commonly referred to as Standard 211 206 (Height 673).</skos:definition>
 <skos:definition xml:lang="fr">Un contenant non-réutilisable métallique de 16.9oz/500ml pour contenir un liquide, souvent appeler Standard 211 206 (Hauteur 673).</skos:definition>
 <!-- Net Content -->
 <gs1:netContent>
  <gs1:QuantitativeValue rdf:about="#can500ml211206-Content">
    <rdf:type rdf:resource="http://qudt.org/1.1/schema/qudt#QuantityValue"/>
    <qudt:unit rdf:resource="http://www.qudt.org/2.1/vocab/unit/MilliL"/>
    <qudt:numericalValue rdf:datatype="http://www.w3.org/2001/XMLSchema#double">500</qudt:numericalValue>
    <rdf:value rdf:datatype="http://www.w3.org/2001/XMLSchema#double">500</rdf:value>
    <gs1:unitCode>MLT</gs1:unitCode>
    <gs1:value>500</gs1:value>
  </gs1:QuantitativeValue>
 </gs1:netContent> 
 <sosa:isFeatureOfInterestOf>
  <rdf:Description rdf:about="#can500ml211206-ContentSosa">
   <rdf:type rdf:resource="http://www.w3.org/ns/sosa/Observation"/>
   <sosa:hasFeatureOfInterest rdf:resource="#can500ml211206"/>
   <sosa:observedProperty  rdf:resource="#netcontent"/>
   <sosa:hasResult rdf:resource="#can500ml211206-Content"/>
   <sosa:hasSimpleResult rdf:datatype="http://www.qudt.org/2.1/vocab/unit/MilliM">500</sosa:hasSimpleResult>
  </rdf:Description>
 </sosa:isFeatureOfInterestOf>
 <!-- Height -->
 <gs1:inPackageHeight>
  <gs1:QuantitativeValue rdf:about="#can500ml211206-Height">
   <rdf:type rdf:resource="http://qudt.org/1.1/schema/qudt#QuantityValue"/>
   <qudt:unit rdf:resource="http://www.qudt.org/2.1/vocab/unit/MilliM"/>
   <qudt:numericalValue rdf:datatype="http://www.w3.org/2001/XMLSchema#double">168</qudt:numericalValue>
   <rdf:value rdf:datatype="http://www.w3.org/2001/XMLSchema#double">168</rdf:value>
   <gs1:unitCode>MMT</gs1:unitCode>
   <gs1:value>168</gs1:value>
  </gs1:QuantitativeValue>
 </gs1:inPackageHeight>  
 <sosa:isFeatureOfInterestOf>
  <rdf:Description rdf:about="#can500ml211206-HeightSosa">
   <rdf:type rdf:resource="http://www.w3.org/ns/sosa/Observation"/>
   <sosa:hasFeatureOfInterest rdf:resource="#can500ml211206"/>
   <sosa:observedProperty  rdf:resource="#height"/>
   <sosa:hasResult rdf:resource="#can500ml211206-Height"/>
   <sosa:hasSimpleResult rdf:datatype="http://www.qudt.org/2.1/vocab/unit/MilliM">168</sosa:hasSimpleResult>
  </rdf:Description>
 </sosa:isFeatureOfInterestOf>
 <!-- Diameter --> 
 <gs1:inPackageDiameter>
  <gs1:QuantitativeValue rdf:about="#can500ml211206-Diameter">
   <rdf:type rdf:resource="http://qudt.org/1.1/schema/qudt#QuantityValue"/>
   <qudt:unit rdf:resource="http://www.qudt.org/2.1/vocab/unit/MilliM"/>
   <qudt:numericalValue rdf:datatype="http://www.w3.org/2001/XMLSchema#double">66</qudt:numericalValue>
   <rdf:value rdf:datatype="http://www.w3.org/2001/XMLSchema#double">66</rdf:value>
   <gs1:unitCode>MMT</gs1:unitCode>
   <gs1:value>66</gs1:value>
  </gs1:QuantitativeValue>
 </gs1:inPackageDiameter>
 <sosa:isFeatureOfInterestOf>
  <rdf:Description rdf:about="#can500ml211206-DiameterSosa">
   <rdf:type rdf:resource="http://www.w3.org/ns/sosa/Observation"/>
   <sosa:hasFeatureOfInterest rdf:resource="#can500ml211206"/>
   <sosa:observedProperty  rdf:resource="#diameter"/>
   <sosa:hasResult rdf:resource="#can500ml211206-Diameter"/>
   <sosa:hasSimpleResult rdf:datatype="http://www.qudt.org/2.1/vocab/unit/MilliM">66</sosa:hasSimpleResult>
  </rdf:Description>
 </sosa:isFeatureOfInterestOf>
 <sosa:isFeatureOfInterestOf>
  <rdf:Description rdf:about="#can500ml211206-EndDiameterSosa">
   <rdf:type rdf:resource="http://www.w3.org/ns/sosa/Observation"/>
   <sosa:hasFeatureOfInterest rdf:resource="#can500ml211206"/>
   <sosa:observedProperty  rdf:resource="#endDiameter"/>
   <sosa:hasResult>
    <gs1:QuantitativeValue rdf:about="#can500ml211206-EndDiameter">
     <rdf:type rdf:resource="http://qudt.org/1.1/schema/qudt#QuantityValue"/>
     <qudt:unit rdf:resource="http://www.qudt.org/2.1/vocab/unit/MilliM"/>
     <qudt:numericalValue rdf:datatype="http://www.w3.org/2001/XMLSchema#double">59.85</qudt:numericalValue>
     <rdf:value rdf:datatype="http://www.w3.org/2001/XMLSchema#double">59.85</rdf:value>
     <gs1:unitCode>MMT</gs1:unitCode>
     <gs1:value>59.85</gs1:value>
    </gs1:QuantitativeValue>
   </sosa:hasResult>
   <sosa:hasSimpleResult rdf:datatype="http://www.qudt.org/2.1/vocab/unit/MilliM">59.85</sosa:hasSimpleResult>
  </rdf:Description>
 </sosa:isFeatureOfInterestOf>
 <rdfs:isDefinedBy rdf:resource="https://rdf.ag/o/beer-ONTOLOGY_DATE"/>
 <void:inDataset rdf:resource="#datasetdefinition"/>
</rdf:Description>



<rdf:Description rdf:about="#can500ml211202673">
 <rdf:type rdf:resource="https://gs1.org/voc/PackagingDetails"/>
 <rdf:type rdf:resource="#LiquidContainer"/>
 <rdf:type rdf:resource="#BeverageCan"/>
 <rdfs:label xml:lang="en">16.9oz/500ml Metal Beverage Can</rdfs:label>
 <rdfs:label xml:lang="fr">Canette à Boisson Métallique, 16.9oz/500ml</rdfs:label>
 <skos:definition xml:lang="en">A one time use 16.9oz/500ml metal container meant to hold a liquid, commonly referred to as 202-211 (Height 603).</skos:definition>
 <skos:definition xml:lang="fr">Un contenant non-réutilisable métallique de 16.9oz/500ml pour contenir un liquide, souvent appeler 202-211 (Hauteur 603).</skos:definition>
 <!-- Net Content -->
 <gs1:netContent>
  <gs1:QuantitativeValue rdf:about="#can500ml211202673-Content">
    <rdf:type rdf:resource="http://qudt.org/1.1/schema/qudt#QuantityValue"/>
    <qudt:unit rdf:resource="http://www.qudt.org/2.1/vocab/unit/MilliL"/>
    <qudt:numericalValue rdf:datatype="http://www.w3.org/2001/XMLSchema#double">500</qudt:numericalValue>
    <rdf:value rdf:datatype="http://www.w3.org/2001/XMLSchema#double">500</rdf:value>
    <gs1:unitCode>MLT</gs1:unitCode>
    <gs1:value>500</gs1:value>
  </gs1:QuantitativeValue>
 </gs1:netContent> 
 <sosa:isFeatureOfInterestOf>
  <rdf:Description rdf:about="#can500ml211202673-ContentSosa">
   <rdf:type rdf:resource="http://www.w3.org/ns/sosa/Observation"/>
   <sosa:hasFeatureOfInterest rdf:resource="#can500ml211202673"/>
   <sosa:observedProperty  rdf:resource="#netcontent"/>
   <sosa:hasResult rdf:resource="#can500ml211202673-Content"/>
   <sosa:hasSimpleResult rdf:datatype="http://www.qudt.org/2.1/vocab/unit/MilliM">500</sosa:hasSimpleResult>
  </rdf:Description>
 </sosa:isFeatureOfInterestOf>
 <!-- Height -->
 <gs1:inPackageHeight>
  <gs1:QuantitativeValue rdf:about="#can500ml211202673-Height">
   <rdf:type rdf:resource="http://qudt.org/1.1/schema/qudt#QuantityValue"/>
   <qudt:unit rdf:resource="http://www.qudt.org/2.1/vocab/unit/MilliM"/>
   <qudt:numericalValue rdf:datatype="http://www.w3.org/2001/XMLSchema#double">168</qudt:numericalValue>
   <rdf:value rdf:datatype="http://www.w3.org/2001/XMLSchema#double">168</rdf:value>
   <gs1:unitCode>MMT</gs1:unitCode>
   <gs1:value>168</gs1:value>
  </gs1:QuantitativeValue>
 </gs1:inPackageHeight>  
 <sosa:isFeatureOfInterestOf>
  <rdf:Description rdf:about="#can500ml211202673-HeightSosa">
   <rdf:type rdf:resource="http://www.w3.org/ns/sosa/Observation"/>
   <sosa:hasFeatureOfInterest rdf:resource="#can500ml211202673"/>
   <sosa:observedProperty  rdf:resource="#height"/>
   <sosa:hasResult rdf:resource="#can500ml211202673-Height"/>
   <sosa:hasSimpleResult rdf:datatype="http://www.qudt.org/2.1/vocab/unit/MilliM">168</sosa:hasSimpleResult>
  </rdf:Description>
 </sosa:isFeatureOfInterestOf>
 <!-- Diameter --> 
 <gs1:inPackageDiameter>
  <gs1:QuantitativeValue rdf:about="#can500ml211202673-Diameter">
   <rdf:type rdf:resource="http://qudt.org/1.1/schema/qudt#QuantityValue"/>
   <qudt:unit rdf:resource="http://www.qudt.org/2.1/vocab/unit/MilliM"/>
   <qudt:numericalValue rdf:datatype="http://www.w3.org/2001/XMLSchema#double">68.262</qudt:numericalValue>
   <rdf:value rdf:datatype="http://www.w3.org/2001/XMLSchema#double">68.262</rdf:value>
   <gs1:unitCode>MMT</gs1:unitCode>
   <gs1:value>68.262</gs1:value>
  </gs1:QuantitativeValue>
 </gs1:inPackageDiameter>
 <sosa:isFeatureOfInterestOf>
  <rdf:Description rdf:about="#can500ml211202673-DiameterSosa">
   <rdf:type rdf:resource="http://www.w3.org/ns/sosa/Observation"/>
   <sosa:hasFeatureOfInterest rdf:resource="#can500ml211202673"/>
   <sosa:observedProperty  rdf:resource="#diameter"/>
   <sosa:hasResult rdf:resource="#can500ml211202673-Diameter"/>
   <sosa:hasSimpleResult rdf:datatype="http://www.qudt.org/2.1/vocab/unit/MilliM">68.262</sosa:hasSimpleResult>
  </rdf:Description>
 </sosa:isFeatureOfInterestOf>
 <sosa:isFeatureOfInterestOf>
  <rdf:Description rdf:about="#can500ml211202673-EndDiameterSosa">
   <rdf:type rdf:resource="http://www.w3.org/ns/sosa/Observation"/>
   <sosa:hasFeatureOfInterest rdf:resource="#can500ml211202673"/>
   <sosa:observedProperty  rdf:resource="#endDiameter"/>
   <sosa:hasResult>
    <gs1:QuantitativeValue rdf:about="#can500ml211202673-EndDiameter">
     <rdf:type rdf:resource="http://qudt.org/1.1/schema/qudt#QuantityValue"/>
     <qudt:unit rdf:resource="http://www.qudt.org/2.1/vocab/unit/MilliM"/>
     <qudt:numericalValue rdf:datatype="http://www.w3.org/2001/XMLSchema#double">55.033164</qudt:numericalValue>
     <rdf:value rdf:datatype="http://www.w3.org/2001/XMLSchema#double">55.033164</rdf:value>
     <gs1:unitCode>MMT</gs1:unitCode>
     <gs1:value>55.033164</gs1:value>
    </gs1:QuantitativeValue>
   </sosa:hasResult>
   <sosa:hasSimpleResult rdf:datatype="http://www.qudt.org/2.1/vocab/unit/MilliM">55.033164</sosa:hasSimpleResult>
  </rdf:Description>
 </sosa:isFeatureOfInterestOf>
 <rdfs:isDefinedBy rdf:resource="https://rdf.ag/o/beer-ONTOLOGY_DATE"/>
 <void:inDataset rdf:resource="#datasetdefinition"/>
</rdf:Description>

<rdf:Description rdf:about="#can163ml">
 <rdf:type rdf:resource="https://gs1.org/voc/PackagingDetails"/>
 <rdf:type rdf:resource="#LiquidContainer"/>
 <rdf:type rdf:resource="#BeverageCan"/>
 <rdfs:label xml:lang="en">5.5oz/163ml Metal Beverage Can</rdfs:label>
 <rdfs:label xml:lang="fr">Canette à Boisson Métallique, 5.5oz/163ml</rdfs:label>
 <skos:definition xml:lang="en">A one time use 5.5oz/163ml metal container meant to hold a liquid, commonly referred to as Slim 202-200 (Height 312).</skos:definition>
 <skos:definition xml:lang="fr">Un contenant non-réutilisable métallique de 5.5oz/163ml pour contenir un liquide, souvent appeler Slim 202-200 (Hauteur 312).</skos:definition>
 <!-- Net Content -->
 <gs1:netContent>
  <gs1:QuantitativeValue rdf:about="#can163ml-Content">
    <rdf:type rdf:resource="http://qudt.org/1.1/schema/qudt#QuantityValue"/>
    <qudt:unit rdf:resource="http://www.qudt.org/2.1/vocab/unit/MilliL"/>
    <qudt:numericalValue rdf:datatype="http://www.w3.org/2001/XMLSchema#double">163</qudt:numericalValue>
    <rdf:value rdf:datatype="http://www.w3.org/2001/XMLSchema#double">163</rdf:value>
    <gs1:unitCode>MLT</gs1:unitCode>
    <gs1:value>163</gs1:value>
  </gs1:QuantitativeValue>
 </gs1:netContent> 
 <sosa:isFeatureOfInterestOf>
  <rdf:Description rdf:about="#can163ml-ContentSosa">
   <rdf:type rdf:resource="http://www.w3.org/ns/sosa/Observation"/>
   <sosa:hasFeatureOfInterest rdf:resource="#can163ml"/>
   <sosa:observedProperty  rdf:resource="#netcontent"/>
   <sosa:hasResult rdf:resource="#can163ml-Content"/>
   <sosa:hasSimpleResult rdf:datatype="http://www.qudt.org/2.1/vocab/unit/MilliM">163</sosa:hasSimpleResult>
  </rdf:Description>
 </sosa:isFeatureOfInterestOf>
 <!-- Height -->
 <gs1:inPackageHeight>
  <gs1:QuantitativeValue rdf:about="#can163ml-Height">
   <rdf:type rdf:resource="http://qudt.org/1.1/schema/qudt#QuantityValue"/>
   <qudt:unit rdf:resource="http://www.qudt.org/2.1/vocab/unit/MilliM"/>
   <qudt:numericalValue rdf:datatype="http://www.w3.org/2001/XMLSchema#double">95.2</qudt:numericalValue>
   <rdf:value rdf:datatype="http://www.w3.org/2001/XMLSchema#double">95.2</rdf:value>
   <gs1:unitCode>MMT</gs1:unitCode>
   <gs1:value>95.2</gs1:value>
  </gs1:QuantitativeValue>
 </gs1:inPackageHeight>  
 <sosa:isFeatureOfInterestOf>
  <rdf:Description rdf:about="#can163ml-HeightSosa">
   <rdf:type rdf:resource="http://www.w3.org/ns/sosa/Observation"/>
   <sosa:hasFeatureOfInterest rdf:resource="#can163ml"/>
   <sosa:observedProperty  rdf:resource="#height"/>
   <sosa:hasResult rdf:resource="#can163ml-Height"/>
   <sosa:hasSimpleResult rdf:datatype="http://www.qudt.org/2.1/vocab/unit/MilliM">95.2</sosa:hasSimpleResult>
  </rdf:Description>
 </sosa:isFeatureOfInterestOf>
 <!-- Diameter --> 
 <gs1:inPackageDiameter>
  <gs1:QuantitativeValue rdf:about="#can163ml-Diameter">
   <rdf:type rdf:resource="http://qudt.org/1.1/schema/qudt#QuantityValue"/>
   <qudt:unit rdf:resource="http://www.qudt.org/2.1/vocab/unit/MilliM"/>
   <qudt:numericalValue rdf:datatype="http://www.w3.org/2001/XMLSchema#double">52.8</qudt:numericalValue>
   <rdf:value rdf:datatype="http://www.w3.org/2001/XMLSchema#double">52.8</rdf:value>
   <gs1:unitCode>MMT</gs1:unitCode>
   <gs1:value>52.8</gs1:value>
  </gs1:QuantitativeValue>
 </gs1:inPackageDiameter>
 <sosa:isFeatureOfInterestOf>
  <rdf:Description rdf:about="#can163ml-DiameterSosa">
   <rdf:type rdf:resource="http://www.w3.org/ns/sosa/Observation"/>
   <sosa:hasFeatureOfInterest rdf:resource="#can163ml"/>
   <sosa:observedProperty  rdf:resource="#diameter"/>
   <sosa:hasResult rdf:resource="#can163ml-Diameter"/>
   <sosa:hasSimpleResult rdf:datatype="http://www.qudt.org/2.1/vocab/unit/MilliM">52.8</sosa:hasSimpleResult>
  </rdf:Description>
 </sosa:isFeatureOfInterestOf>
 <sosa:isFeatureOfInterestOf>
  <rdf:Description rdf:about="#can163ml-EndDiameterSosa">
   <rdf:type rdf:resource="http://www.w3.org/ns/sosa/Observation"/>
   <sosa:hasFeatureOfInterest rdf:resource="#can163ml"/>
   <sosa:observedProperty  rdf:resource="#endDiameter"/>
   <sosa:hasResult>
    <gs1:QuantitativeValue rdf:about="#can163ml-EndDiameter">
     <rdf:type rdf:resource="http://qudt.org/1.1/schema/qudt#QuantityValue"/>
     <qudt:unit rdf:resource="http://www.qudt.org/2.1/vocab/unit/MilliM"/>
     <qudt:numericalValue rdf:datatype="http://www.w3.org/2001/XMLSchema#double">50.4</qudt:numericalValue>
     <rdf:value rdf:datatype="http://www.w3.org/2001/XMLSchema#double">50.4</rdf:value>
     <gs1:unitCode>MMT</gs1:unitCode>
     <gs1:value>50.4</gs1:value>
    </gs1:QuantitativeValue>
   </sosa:hasResult>
   <sosa:hasSimpleResult rdf:datatype="http://www.qudt.org/2.1/vocab/unit/MilliM">50.4</sosa:hasSimpleResult>
  </rdf:Description>
 </sosa:isFeatureOfInterestOf>
 <rdfs:isDefinedBy rdf:resource="https://rdf.ag/o/beer-ONTOLOGY_DATE"/>
 <void:inDataset rdf:resource="#datasetdefinition"/>
</rdf:Description>

<rdf:Description rdf:about="#can187ml">
 <rdf:type rdf:resource="https://gs1.org/voc/PackagingDetails"/>
 <rdf:type rdf:resource="#LiquidContainer"/>
 <rdf:type rdf:resource="#BeverageCan"/>
 <rdfs:label xml:lang="en">6.3oz/187ml Metal Beverage Can</rdfs:label>
 <rdfs:label xml:lang="fr">Canette à Boisson Métallique, 6.3oz/187ml</rdfs:label>
 <skos:definition xml:lang="en">A one time use 6.3oz/187ml metal container meant to hold a liquid, commonly referred to as Slim 202-200 (Height 401).</skos:definition>
 <skos:definition xml:lang="fr">Un contenant non-réutilisable métallique de 6.3oz/187ml pour contenir un liquide, souvent appeler Slim 202-200 (Hauteur 401).</skos:definition>
 <!-- Net Content -->
 <gs1:netContent>
  <gs1:QuantitativeValue rdf:about="#can187ml-Content">
    <rdf:type rdf:resource="http://qudt.org/1.1/schema/qudt#QuantityValue"/>
    <qudt:unit rdf:resource="http://www.qudt.org/2.1/vocab/unit/MilliL"/>
    <qudt:numericalValue rdf:datatype="http://www.w3.org/2001/XMLSchema#double">187</qudt:numericalValue>
    <rdf:value rdf:datatype="http://www.w3.org/2001/XMLSchema#double">187</rdf:value>
    <gs1:unitCode>MLT</gs1:unitCode>
    <gs1:value>187</gs1:value>
  </gs1:QuantitativeValue>
 </gs1:netContent> 
 <sosa:isFeatureOfInterestOf>
  <rdf:Description rdf:about="#can187ml-ContentSosa">
   <rdf:type rdf:resource="http://www.w3.org/ns/sosa/Observation"/>
   <sosa:hasFeatureOfInterest rdf:resource="#can187ml"/>
   <sosa:observedProperty  rdf:resource="#netcontent"/>
   <sosa:hasResult rdf:resource="#can187ml-Content"/>
   <sosa:hasSimpleResult rdf:datatype="http://www.qudt.org/2.1/vocab/unit/MilliM">187</sosa:hasSimpleResult>
  </rdf:Description>
 </sosa:isFeatureOfInterestOf>
 <!-- Height -->
 <gs1:inPackageHeight>
  <gs1:QuantitativeValue rdf:about="#can187ml-Height">
   <rdf:type rdf:resource="http://qudt.org/1.1/schema/qudt#QuantityValue"/>
   <qudt:unit rdf:resource="http://www.qudt.org/2.1/vocab/unit/MilliM"/>
   <qudt:numericalValue rdf:datatype="http://www.w3.org/2001/XMLSchema#double">102.6</qudt:numericalValue>
   <rdf:value rdf:datatype="http://www.w3.org/2001/XMLSchema#double">102.6</rdf:value>
   <gs1:unitCode>MMT</gs1:unitCode>
   <gs1:value>102.6</gs1:value>
  </gs1:QuantitativeValue>
 </gs1:inPackageHeight>  
 <sosa:isFeatureOfInterestOf>
  <rdf:Description rdf:about="#can187ml-HeightSosa">
   <rdf:type rdf:resource="http://www.w3.org/ns/sosa/Observation"/>
   <sosa:hasFeatureOfInterest rdf:resource="#can187ml"/>
   <sosa:observedProperty  rdf:resource="#height"/>
   <sosa:hasResult rdf:resource="#can187ml-Height"/>
   <sosa:hasSimpleResult rdf:datatype="http://www.qudt.org/2.1/vocab/unit/MilliM">102.6</sosa:hasSimpleResult>
  </rdf:Description>
 </sosa:isFeatureOfInterestOf>
 <!-- Diameter --> 
 <gs1:inPackageDiameter>
  <gs1:QuantitativeValue rdf:about="#can187ml-Diameter">
   <rdf:type rdf:resource="http://qudt.org/1.1/schema/qudt#QuantityValue"/>
   <qudt:unit rdf:resource="http://www.qudt.org/2.1/vocab/unit/MilliM"/>
   <qudt:numericalValue rdf:datatype="http://www.w3.org/2001/XMLSchema#double">52.8</qudt:numericalValue>
   <rdf:value rdf:datatype="http://www.w3.org/2001/XMLSchema#double">52.8</rdf:value>
   <gs1:unitCode>MMT</gs1:unitCode>
   <gs1:value>52.8</gs1:value>
  </gs1:QuantitativeValue>
 </gs1:inPackageDiameter>
 <sosa:isFeatureOfInterestOf>
  <rdf:Description rdf:about="#can187ml-DiameterSosa">
   <rdf:type rdf:resource="http://www.w3.org/ns/sosa/Observation"/>
   <sosa:hasFeatureOfInterest rdf:resource="#can187ml"/>
   <sosa:observedProperty  rdf:resource="#diameter"/>
   <sosa:hasResult rdf:resource="#can187ml-Diameter"/>
   <sosa:hasSimpleResult rdf:datatype="http://www.qudt.org/2.1/vocab/unit/MilliM">52.8</sosa:hasSimpleResult>
  </rdf:Description>
 </sosa:isFeatureOfInterestOf>
 <sosa:isFeatureOfInterestOf>
  <rdf:Description rdf:about="#can187ml-EndDiameterSosa">
   <rdf:type rdf:resource="http://www.w3.org/ns/sosa/Observation"/>
   <sosa:hasFeatureOfInterest rdf:resource="#can187ml"/>
   <sosa:observedProperty  rdf:resource="#endDiameter"/>
   <sosa:hasResult>
    <gs1:QuantitativeValue rdf:about="#can187ml-EndDiameter">
     <rdf:type rdf:resource="http://qudt.org/1.1/schema/qudt#QuantityValue"/>
     <qudt:unit rdf:resource="http://www.qudt.org/2.1/vocab/unit/MilliM"/>
     <qudt:numericalValue rdf:datatype="http://www.w3.org/2001/XMLSchema#double">50.4</qudt:numericalValue>
     <rdf:value rdf:datatype="http://www.w3.org/2001/XMLSchema#double">50.4</rdf:value>
     <gs1:unitCode>MMT</gs1:unitCode>
     <gs1:value>50.4</gs1:value>
    </gs1:QuantitativeValue>
   </sosa:hasResult>
   <sosa:hasSimpleResult rdf:datatype="http://www.qudt.org/2.1/vocab/unit/MilliM">50.4</sosa:hasSimpleResult>
  </rdf:Description>
 </sosa:isFeatureOfInterestOf>
 <rdfs:isDefinedBy rdf:resource="https://rdf.ag/o/beer-ONTOLOGY_DATE"/>
 <void:inDataset rdf:resource="#datasetdefinition"/>
</rdf:Description>

<rdf:Description rdf:about="#can200ml">
 <rdf:type rdf:resource="https://gs1.org/voc/PackagingDetails"/>
 <rdf:type rdf:resource="#LiquidContainer"/>
 <rdf:type rdf:resource="#BeverageCan"/>
 <rdfs:label xml:lang="en">6.8oz/200ml Metal Beverage Can</rdfs:label>
 <rdfs:label xml:lang="fr">Canette à Boisson Métallique, 6.8oz/200ml</rdfs:label>
 <skos:definition xml:lang="en">A one time use 6.8oz/200ml metal container meant to hold a liquid, commonly referred to as Slim 202-200 (Height 405).</skos:definition>
 <skos:definition xml:lang="fr">Un contenant non-réutilisable métallique de 6.8oz/200ml pour contenir un liquide, souvent appeler Slim 202-200 (Hauteur 405).</skos:definition>
 <!-- Net Content -->
 <gs1:netContent>
  <gs1:QuantitativeValue rdf:about="#can200ml-Content">
    <rdf:type rdf:resource="http://qudt.org/1.1/schema/qudt#QuantityValue"/>
    <qudt:unit rdf:resource="http://www.qudt.org/2.1/vocab/unit/MilliL"/>
    <qudt:numericalValue rdf:datatype="http://www.w3.org/2001/XMLSchema#double">200</qudt:numericalValue>
    <rdf:value rdf:datatype="http://www.w3.org/2001/XMLSchema#double">200</rdf:value>
    <gs1:unitCode>MLT</gs1:unitCode>
    <gs1:value>200</gs1:value>
  </gs1:QuantitativeValue>
 </gs1:netContent> 
 <sosa:isFeatureOfInterestOf>
  <rdf:Description rdf:about="#can200ml-ContentSosa">
   <rdf:type rdf:resource="http://www.w3.org/ns/sosa/Observation"/>
   <sosa:hasFeatureOfInterest rdf:resource="#can200ml"/>
   <sosa:observedProperty  rdf:resource="#netcontent"/>
   <sosa:hasResult rdf:resource="#can200ml-Content"/>
   <sosa:hasSimpleResult rdf:datatype="http://www.qudt.org/2.1/vocab/unit/MilliM">200</sosa:hasSimpleResult>
  </rdf:Description>
 </sosa:isFeatureOfInterestOf>
 <!-- Height -->
 <gs1:inPackageHeight>
  <gs1:QuantitativeValue rdf:about="#can200ml-Height">
   <rdf:type rdf:resource="http://qudt.org/1.1/schema/qudt#QuantityValue"/>
   <qudt:unit rdf:resource="http://www.qudt.org/2.1/vocab/unit/MilliM"/>
   <qudt:numericalValue rdf:datatype="http://www.w3.org/2001/XMLSchema#double">109.4</qudt:numericalValue>
   <rdf:value rdf:datatype="http://www.w3.org/2001/XMLSchema#double">109.4</rdf:value>
   <gs1:unitCode>MMT</gs1:unitCode>
   <gs1:value>109.4</gs1:value>
  </gs1:QuantitativeValue>
 </gs1:inPackageHeight>  
 <sosa:isFeatureOfInterestOf>
  <rdf:Description rdf:about="#can200ml-HeightSosa">
   <rdf:type rdf:resource="http://www.w3.org/ns/sosa/Observation"/>
   <sosa:hasFeatureOfInterest rdf:resource="#can200ml"/>
   <sosa:observedProperty  rdf:resource="#height"/>
   <sosa:hasResult rdf:resource="#can200ml-Height"/>
   <sosa:hasSimpleResult rdf:datatype="http://www.qudt.org/2.1/vocab/unit/MilliM">109.4</sosa:hasSimpleResult>
  </rdf:Description>
 </sosa:isFeatureOfInterestOf>
 <!-- Diameter --> 
 <gs1:inPackageDiameter>
  <gs1:QuantitativeValue rdf:about="#can200ml-Diameter">
   <rdf:type rdf:resource="http://qudt.org/1.1/schema/qudt#QuantityValue"/>
   <qudt:unit rdf:resource="http://www.qudt.org/2.1/vocab/unit/MilliM"/>
   <qudt:numericalValue rdf:datatype="http://www.w3.org/2001/XMLSchema#double">52.8</qudt:numericalValue>
   <rdf:value rdf:datatype="http://www.w3.org/2001/XMLSchema#double">52.8</rdf:value>
   <gs1:unitCode>MMT</gs1:unitCode>
   <gs1:value>52.8</gs1:value>
  </gs1:QuantitativeValue>
 </gs1:inPackageDiameter>
 <sosa:isFeatureOfInterestOf>
  <rdf:Description rdf:about="#can200ml-DiameterSosa">
   <rdf:type rdf:resource="http://www.w3.org/ns/sosa/Observation"/>
   <sosa:hasFeatureOfInterest rdf:resource="#can200ml"/>
   <sosa:observedProperty  rdf:resource="#diameter"/>
   <sosa:hasResult rdf:resource="#can200ml-Diameter"/>
   <sosa:hasSimpleResult rdf:datatype="http://www.qudt.org/2.1/vocab/unit/MilliM">52.8</sosa:hasSimpleResult>
  </rdf:Description>
 </sosa:isFeatureOfInterestOf>
 <sosa:isFeatureOfInterestOf>
  <rdf:Description rdf:about="#can200ml-EndDiameterSosa">
   <rdf:type rdf:resource="http://www.w3.org/ns/sosa/Observation"/>
   <sosa:hasFeatureOfInterest rdf:resource="#can200ml"/>
   <sosa:observedProperty  rdf:resource="#endDiameter"/>
   <sosa:hasResult>
    <gs1:QuantitativeValue rdf:about="#can200ml-EndDiameter">
     <rdf:type rdf:resource="http://qudt.org/1.1/schema/qudt#QuantityValue"/>
     <qudt:unit rdf:resource="http://www.qudt.org/2.1/vocab/unit/MilliM"/>
     <qudt:numericalValue rdf:datatype="http://www.w3.org/2001/XMLSchema#double">50.4</qudt:numericalValue>
     <rdf:value rdf:datatype="http://www.w3.org/2001/XMLSchema#double">50.4</rdf:value>
     <gs1:unitCode>MMT</gs1:unitCode>
     <gs1:value>50.4</gs1:value>
    </gs1:QuantitativeValue>
   </sosa:hasResult>
   <sosa:hasSimpleResult rdf:datatype="http://www.qudt.org/2.1/vocab/unit/MilliM">50.4</sosa:hasSimpleResult>
  </rdf:Description>
 </sosa:isFeatureOfInterestOf>
 <rdfs:isDefinedBy rdf:resource="https://rdf.ag/o/beer-ONTOLOGY_DATE"/>
 <void:inDataset rdf:resource="#datasetdefinition"/>
</rdf:Description>

<rdf:Description rdf:about="#can222ml">
 <rdf:type rdf:resource="https://gs1.org/voc/PackagingDetails"/>
 <rdf:type rdf:resource="#LiquidContainer"/>
 <rdf:type rdf:resource="#BeverageCan"/>
 <rdfs:label xml:lang="en">7.5oz/222ml Metal Beverage Can</rdfs:label>
 <rdfs:label xml:lang="fr">Canette à Boisson Métallique, 7.5oz/222ml</rdfs:label>
 <skos:definition xml:lang="en">A one time use 7.5oz/222ml metal container meant to hold a liquid, commonly referred to as Sleek 204-202 (Height 402).</skos:definition>
 <skos:definition xml:lang="fr">Un contenant non-réutilisable métallique de 7.5oz/222ml pour contenir un liquide, souvent appeler Sleek 204-202 (Hauteur 402).</skos:definition>
 <!-- Net Content -->
 <gs1:netContent>
  <gs1:QuantitativeValue rdf:about="#can222ml-Content">
    <rdf:type rdf:resource="http://qudt.org/1.1/schema/qudt#QuantityValue"/>
    <qudt:unit rdf:resource="http://www.qudt.org/2.1/vocab/unit/MilliL"/>
    <qudt:numericalValue rdf:datatype="http://www.w3.org/2001/XMLSchema#double">222</qudt:numericalValue>
    <rdf:value rdf:datatype="http://www.w3.org/2001/XMLSchema#double">222</rdf:value>
    <gs1:unitCode>MLT</gs1:unitCode>
    <gs1:value>222</gs1:value>
  </gs1:QuantitativeValue>
 </gs1:netContent> 
 <sosa:isFeatureOfInterestOf>
  <rdf:Description rdf:about="#can222ml-ContentSosa">
   <rdf:type rdf:resource="http://www.w3.org/ns/sosa/Observation"/>
   <sosa:hasFeatureOfInterest rdf:resource="#can222ml"/>
   <sosa:observedProperty  rdf:resource="#netcontent"/>
   <sosa:hasResult rdf:resource="#can222ml-Content"/>
   <sosa:hasSimpleResult rdf:datatype="http://www.qudt.org/2.1/vocab/unit/MilliM">222</sosa:hasSimpleResult>
  </rdf:Description>
 </sosa:isFeatureOfInterestOf>
 <!-- Height -->
 <gs1:inPackageHeight>
  <gs1:QuantitativeValue rdf:about="#can222ml-Height">
   <rdf:type rdf:resource="http://qudt.org/1.1/schema/qudt#QuantityValue"/>
   <qudt:unit rdf:resource="http://www.qudt.org/2.1/vocab/unit/MilliM"/>
   <qudt:numericalValue rdf:datatype="http://www.w3.org/2001/XMLSchema#double">105</qudt:numericalValue>
   <rdf:value rdf:datatype="http://www.w3.org/2001/XMLSchema#double">105</rdf:value>
   <gs1:unitCode>MMT</gs1:unitCode>
   <gs1:value>105</gs1:value>
  </gs1:QuantitativeValue>
 </gs1:inPackageHeight>  
 <sosa:isFeatureOfInterestOf>
  <rdf:Description rdf:about="#can222ml-HeightSosa">
   <rdf:type rdf:resource="http://www.w3.org/ns/sosa/Observation"/>
   <sosa:hasFeatureOfInterest rdf:resource="#can222ml"/>
   <sosa:observedProperty  rdf:resource="#height"/>
   <sosa:hasResult rdf:resource="#can222ml-Height"/>
   <sosa:hasSimpleResult rdf:datatype="http://www.qudt.org/2.1/vocab/unit/MilliM">105</sosa:hasSimpleResult>
  </rdf:Description>
 </sosa:isFeatureOfInterestOf>
 <!-- Diameter --> 
 <gs1:inPackageDiameter>
  <gs1:QuantitativeValue rdf:about="#can222ml-Diameter">
   <rdf:type rdf:resource="http://qudt.org/1.1/schema/qudt#QuantityValue"/>
   <qudt:unit rdf:resource="http://www.qudt.org/2.1/vocab/unit/MilliM"/>
   <qudt:numericalValue rdf:datatype="http://www.w3.org/2001/XMLSchema#double">56.7</qudt:numericalValue>
   <rdf:value rdf:datatype="http://www.w3.org/2001/XMLSchema#double">56.7</rdf:value>
   <gs1:unitCode>MMT</gs1:unitCode>
   <gs1:value>56.7</gs1:value>
  </gs1:QuantitativeValue>
 </gs1:inPackageDiameter>
 <sosa:isFeatureOfInterestOf>
  <rdf:Description rdf:about="#can222ml-DiameterSosa">
   <rdf:type rdf:resource="http://www.w3.org/ns/sosa/Observation"/>
   <sosa:hasFeatureOfInterest rdf:resource="#can222ml"/>
   <sosa:observedProperty  rdf:resource="#diameter"/>
   <sosa:hasResult rdf:resource="#can222ml-Diameter"/>
   <sosa:hasSimpleResult rdf:datatype="http://www.qudt.org/2.1/vocab/unit/MilliM">56.7</sosa:hasSimpleResult>
  </rdf:Description>
 </sosa:isFeatureOfInterestOf>
 <sosa:isFeatureOfInterestOf>
  <rdf:Description rdf:about="#can222ml-EndDiameterSosa">
   <rdf:type rdf:resource="http://www.w3.org/ns/sosa/Observation"/>
   <sosa:hasFeatureOfInterest rdf:resource="#can222ml"/>
   <sosa:observedProperty  rdf:resource="#endDiameter"/>
   <sosa:hasResult>
    <gs1:QuantitativeValue rdf:about="#can222ml-EndDiameter">
     <rdf:type rdf:resource="http://qudt.org/1.1/schema/qudt#QuantityValue"/>
     <qudt:unit rdf:resource="http://www.qudt.org/2.1/vocab/unit/MilliM"/>
     <qudt:numericalValue rdf:datatype="http://www.w3.org/2001/XMLSchema#double">53.55</qudt:numericalValue>
     <rdf:value rdf:datatype="http://www.w3.org/2001/XMLSchema#double">53.55</rdf:value>
     <gs1:unitCode>MMT</gs1:unitCode>
     <gs1:value>53.55</gs1:value>
    </gs1:QuantitativeValue>
   </sosa:hasResult>
   <sosa:hasSimpleResult rdf:datatype="http://www.qudt.org/2.1/vocab/unit/MilliM">53.55</sosa:hasSimpleResult>
  </rdf:Description>
 </sosa:isFeatureOfInterestOf>
 <rdfs:isDefinedBy rdf:resource="https://rdf.ag/o/beer-ONTOLOGY_DATE"/>
 <void:inDataset rdf:resource="#datasetdefinition"/>
</rdf:Description>

<rdf:Description rdf:about="#can236ml">
 <rdf:type rdf:resource="https://gs1.org/voc/PackagingDetails"/>
 <rdf:type rdf:resource="#LiquidContainer"/>
 <rdf:type rdf:resource="#BeverageCan"/>
 <rdfs:label xml:lang="en">8oz/236ml Metal Beverage Can</rdfs:label>
 <rdfs:label xml:lang="fr">Canette à Boisson Métallique, 8oz/236ml</rdfs:label>
 <skos:definition xml:lang="en">A one time use 8oz/236ml metal container meant to hold a liquid, commonly referred to as 204 (Height 405).</skos:definition>
 <skos:definition xml:lang="fr">Un contenant non-réutilisable métallique de 8oz/236ml pour contenir un liquide, souvent appeler 204 (Hauteur 405).</skos:definition>
 <!-- Net Content -->
 <gs1:netContent>
  <gs1:QuantitativeValue rdf:about="#can236ml-Content">
    <rdf:type rdf:resource="http://qudt.org/1.1/schema/qudt#QuantityValue"/>
    <qudt:unit rdf:resource="http://www.qudt.org/2.1/vocab/unit/MilliL"/>
    <qudt:numericalValue rdf:datatype="http://www.w3.org/2001/XMLSchema#double">236</qudt:numericalValue>
    <rdf:value rdf:datatype="http://www.w3.org/2001/XMLSchema#double">236</rdf:value>
    <gs1:unitCode>MLT</gs1:unitCode>
    <gs1:value>236</gs1:value>
  </gs1:QuantitativeValue>
 </gs1:netContent> 
 <sosa:isFeatureOfInterestOf>
  <rdf:Description rdf:about="#can236ml-ContentSosa">
   <rdf:type rdf:resource="http://www.w3.org/ns/sosa/Observation"/>
   <sosa:hasFeatureOfInterest rdf:resource="#can236ml"/>
   <sosa:observedProperty  rdf:resource="#netcontent"/>
   <sosa:hasResult rdf:resource="#can236ml-Content"/>
   <sosa:hasSimpleResult rdf:datatype="http://www.qudt.org/2.1/vocab/unit/MilliM">236</sosa:hasSimpleResult>
  </rdf:Description>
 </sosa:isFeatureOfInterestOf>
 <!-- Height -->
 <gs1:inPackageHeight>
  <gs1:QuantitativeValue rdf:about="#can236ml-Height">
   <rdf:type rdf:resource="http://qudt.org/1.1/schema/qudt#QuantityValue"/>
   <qudt:unit rdf:resource="http://www.qudt.org/2.1/vocab/unit/MilliM"/>
   <qudt:numericalValue rdf:datatype="http://www.w3.org/2001/XMLSchema#double">109.4</qudt:numericalValue>
   <rdf:value rdf:datatype="http://www.w3.org/2001/XMLSchema#double">109.4</rdf:value>
   <gs1:unitCode>MMT</gs1:unitCode>
   <gs1:value>109.4</gs1:value>
  </gs1:QuantitativeValue>
 </gs1:inPackageHeight>  
 <sosa:isFeatureOfInterestOf>
  <rdf:Description rdf:about="#can236ml-HeightSosa">
   <rdf:type rdf:resource="http://www.w3.org/ns/sosa/Observation"/>
   <sosa:hasFeatureOfInterest rdf:resource="#can236ml"/>
   <sosa:observedProperty  rdf:resource="#height"/>
   <sosa:hasResult rdf:resource="#can236ml-Height"/>
   <sosa:hasSimpleResult rdf:datatype="http://www.qudt.org/2.1/vocab/unit/MilliM">109.4</sosa:hasSimpleResult>
  </rdf:Description>
 </sosa:isFeatureOfInterestOf>
 <!-- Diameter --> 
 <gs1:inPackageDiameter>
  <gs1:QuantitativeValue rdf:about="#can236ml-Diameter">
   <rdf:type rdf:resource="http://qudt.org/1.1/schema/qudt#QuantityValue"/>
   <qudt:unit rdf:resource="http://www.qudt.org/2.1/vocab/unit/MilliM"/>
   <qudt:numericalValue rdf:datatype="http://www.w3.org/2001/XMLSchema#double">56.7</qudt:numericalValue>
   <rdf:value rdf:datatype="http://www.w3.org/2001/XMLSchema#double">56.7</rdf:value>
   <gs1:unitCode>MMT</gs1:unitCode>
   <gs1:value>56.7</gs1:value>
  </gs1:QuantitativeValue>
 </gs1:inPackageDiameter>
 <sosa:isFeatureOfInterestOf>
  <rdf:Description rdf:about="#can236ml-DiameterSosa">
   <rdf:type rdf:resource="http://www.w3.org/ns/sosa/Observation"/>
   <sosa:hasFeatureOfInterest rdf:resource="#can236ml"/>
   <sosa:observedProperty  rdf:resource="#diameter"/>
   <sosa:hasResult rdf:resource="#can236ml-Diameter"/>
   <sosa:hasSimpleResult rdf:datatype="http://www.qudt.org/2.1/vocab/unit/MilliM">56.7</sosa:hasSimpleResult>
  </rdf:Description>
 </sosa:isFeatureOfInterestOf>
 <rdfs:isDefinedBy rdf:resource="https://rdf.ag/o/beer-ONTOLOGY_DATE"/>
 <void:inDataset rdf:resource="#datasetdefinition"/>
</rdf:Description>

<rdf:Description rdf:about="#can237ml">
 <rdf:type rdf:resource="#LiquidContainer"/>
 <rdf:type rdf:resource="#BeverageCan"/>
 <rdf:type rdf:resource="https://gs1.org/voc/PackagingDetails"/>
 <rdfs:label xml:lang="en">Any 237ml Can</rdfs:label>
 <rdfs:label xml:lang="fr">Canette à Boisson Métallique, 237ml</rdfs:label>
 <skos:definition xml:lang="en">Any 237ml Can</skos:definition>
 <skos:definition xml:lang="fr">Canette à Boisson Métallique, 237ml</skos:definition>
 <owl:oneOf>
  <rdf:List rdf:about="#can237mlList1">
   <rdf:first rdf:resource="#can237ml204"/>
   <rdf:rest>
    <rdf:List rdf:about="#can237mlList2">
     <rdf:first rdf:resource="#can237ml211"/>
     <rdf:rest rdf:resource="http://www.w3.org/1999/02/22-rdf-syntax-ns#nil"/>
    </rdf:List>
   </rdf:rest>
  </rdf:List>
 </owl:oneOf>       
</rdf:Description>

<rdf:Description rdf:about="#can237ml204">
 <rdf:type rdf:resource="https://gs1.org/voc/PackagingDetails"/>
 <rdf:type rdf:resource="#LiquidContainer"/>
 <rdf:type rdf:resource="#BeverageCan"/>
 <rdfs:label xml:lang="en">8oz/237ml Metal Beverage Can</rdfs:label>
 <rdfs:label xml:lang="fr">Canette à Boisson Métallique, 8oz/237ml</rdfs:label>
 <skos:definition xml:lang="en">A one time use 8oz/237ml metal container meant to hold a liquid, commonly referred to as Sleek 204.5 (Height 405).</skos:definition>
 <skos:definition xml:lang="fr">Un contenant non-réutilisable métallique de 8oz/237ml pour contenir un liquide, souvent appeler Sleek 204.5 (Hauteur 405).</skos:definition>
 <!-- Net Content -->
 <gs1:netContent>
  <gs1:QuantitativeValue rdf:about="#can237ml204-Content">
    <rdf:type rdf:resource="http://qudt.org/1.1/schema/qudt#QuantityValue"/>
    <qudt:unit rdf:resource="http://www.qudt.org/2.1/vocab/unit/MilliL"/>
    <qudt:numericalValue rdf:datatype="http://www.w3.org/2001/XMLSchema#double">237</qudt:numericalValue>
    <rdf:value rdf:datatype="http://www.w3.org/2001/XMLSchema#double">237</rdf:value>
    <gs1:unitCode>MLT</gs1:unitCode>
    <gs1:value>237</gs1:value>
  </gs1:QuantitativeValue>
 </gs1:netContent> 
 <sosa:isFeatureOfInterestOf>
  <rdf:Description rdf:about="#can237ml204-ContentSosa">
   <rdf:type rdf:resource="http://www.w3.org/ns/sosa/Observation"/>
   <sosa:hasFeatureOfInterest rdf:resource="#can237ml204"/>
   <sosa:observedProperty  rdf:resource="#netcontent"/>
   <sosa:hasResult rdf:resource="#can237ml204-Content"/>
   <sosa:hasSimpleResult rdf:datatype="http://www.qudt.org/2.1/vocab/unit/MilliM">237</sosa:hasSimpleResult>
  </rdf:Description>
 </sosa:isFeatureOfInterestOf>
 <!-- Height -->
 <gs1:inPackageHeight>
  <gs1:QuantitativeValue rdf:about="#can237ml204-Height">
   <rdf:type rdf:resource="http://qudt.org/1.1/schema/qudt#QuantityValue"/>
   <qudt:unit rdf:resource="http://www.qudt.org/2.1/vocab/unit/MilliM"/>
   <qudt:numericalValue rdf:datatype="http://www.w3.org/2001/XMLSchema#double">109.4</qudt:numericalValue>
   <rdf:value rdf:datatype="http://www.w3.org/2001/XMLSchema#double">109.4</rdf:value>
   <gs1:unitCode>MMT</gs1:unitCode>
   <gs1:value>109.4</gs1:value>
  </gs1:QuantitativeValue>
 </gs1:inPackageHeight>  
 <sosa:isFeatureOfInterestOf>
  <rdf:Description rdf:about="#can237ml204-HeightSosa">
   <rdf:type rdf:resource="http://www.w3.org/ns/sosa/Observation"/>
   <sosa:hasFeatureOfInterest rdf:resource="#can237ml204"/>
   <sosa:observedProperty  rdf:resource="#height"/>
   <sosa:hasResult rdf:resource="#can237ml204-Height"/>
   <sosa:hasSimpleResult rdf:datatype="http://www.qudt.org/2.1/vocab/unit/MilliM">109.4</sosa:hasSimpleResult>
  </rdf:Description>
 </sosa:isFeatureOfInterestOf>
 <!-- Diameter --> 
 <gs1:inPackageDiameter>
  <gs1:QuantitativeValue rdf:about="#can237ml204-Diameter">
   <rdf:type rdf:resource="http://qudt.org/1.1/schema/qudt#QuantityValue"/>
   <qudt:unit rdf:resource="http://www.qudt.org/2.1/vocab/unit/MilliM"/>
   <qudt:numericalValue rdf:datatype="http://www.w3.org/2001/XMLSchema#double">75.5</qudt:numericalValue>
   <rdf:value rdf:datatype="http://www.w3.org/2001/XMLSchema#double">75.5</rdf:value>
   <gs1:unitCode>MMT</gs1:unitCode>
   <gs1:value>75.5</gs1:value>
  </gs1:QuantitativeValue>
 </gs1:inPackageDiameter>
 <sosa:isFeatureOfInterestOf>
  <rdf:Description rdf:about="#can237ml204-DiameterSosa">
   <rdf:type rdf:resource="http://www.w3.org/ns/sosa/Observation"/>
   <sosa:hasFeatureOfInterest rdf:resource="#can237ml204"/>
   <sosa:observedProperty  rdf:resource="#diameter"/>
   <sosa:hasResult rdf:resource="#can237ml204-Diameter"/>
   <sosa:hasSimpleResult rdf:datatype="http://www.qudt.org/2.1/vocab/unit/MilliM">75.5</sosa:hasSimpleResult>
  </rdf:Description>
 </sosa:isFeatureOfInterestOf>
 <rdfs:isDefinedBy rdf:resource="https://rdf.ag/o/beer-ONTOLOGY_DATE"/>
 <void:inDataset rdf:resource="#datasetdefinition"/>
</rdf:Description>


<rdf:Description rdf:about="#can237ml211">
 <rdf:type rdf:resource="https://gs1.org/voc/PackagingDetails"/>
 <rdf:type rdf:resource="#LiquidContainer"/>
 <rdf:type rdf:resource="#BeverageCan"/>
 <rdfs:label xml:lang="en">8oz/237ml Metal Beverage Can</rdfs:label>
 <rdfs:label xml:lang="fr">Canette à Boisson Métallique, 8oz/237ml</rdfs:label>
 <skos:definition xml:lang="en">A one time use 8oz/237ml metal container meant to hold a liquid, commonly referred to as Stubby 211 (Height 307).</skos:definition>
 <skos:definition xml:lang="fr">Un contenant non-réutilisable métallique de 8oz/237ml pour contenir un liquide, souvent appeler Stubby 211 (Hauteur 307).</skos:definition>
 <!-- Net Content -->
 <gs1:netContent>
  <gs1:QuantitativeValue rdf:about="#can237ml211-Content">
    <rdf:type rdf:resource="http://qudt.org/1.1/schema/qudt#QuantityValue"/>
    <qudt:unit rdf:resource="http://www.qudt.org/2.1/vocab/unit/MilliL"/>
    <qudt:numericalValue rdf:datatype="http://www.w3.org/2001/XMLSchema#double">237</qudt:numericalValue>
    <rdf:value rdf:datatype="http://www.w3.org/2001/XMLSchema#double">237</rdf:value>
    <gs1:unitCode>MLT</gs1:unitCode>
    <gs1:value>237</gs1:value>
  </gs1:QuantitativeValue>
 </gs1:netContent> 
 <sosa:isFeatureOfInterestOf>
  <rdf:Description rdf:about="#can237ml211-ContentSosa">
   <rdf:type rdf:resource="http://www.w3.org/ns/sosa/Observation"/>
   <sosa:hasFeatureOfInterest rdf:resource="#can237ml211"/>
   <sosa:observedProperty  rdf:resource="#netcontent"/>
   <sosa:hasResult rdf:resource="#can237ml211-Content"/>
   <sosa:hasSimpleResult rdf:datatype="http://www.qudt.org/2.1/vocab/unit/MilliM">237</sosa:hasSimpleResult>
  </rdf:Description>
 </sosa:isFeatureOfInterestOf>
 <!-- Height -->
 <gs1:inPackageHeight>
  <gs1:QuantitativeValue rdf:about="#can237ml211-Height">
   <rdf:type rdf:resource="http://qudt.org/1.1/schema/qudt#QuantityValue"/>
   <qudt:unit rdf:resource="http://www.qudt.org/2.1/vocab/unit/MilliM"/>
   <qudt:numericalValue rdf:datatype="http://www.w3.org/2001/XMLSchema#double">87.8</qudt:numericalValue>
   <rdf:value rdf:datatype="http://www.w3.org/2001/XMLSchema#double">87.8</rdf:value>
   <gs1:unitCode>MMT</gs1:unitCode>
   <gs1:value>87.8</gs1:value>
  </gs1:QuantitativeValue>
 </gs1:inPackageHeight>  
 <sosa:isFeatureOfInterestOf>
  <rdf:Description rdf:about="#can237ml211-HeightSosa">
   <rdf:type rdf:resource="http://www.w3.org/ns/sosa/Observation"/>
   <sosa:hasFeatureOfInterest rdf:resource="#can237ml211"/>
   <sosa:observedProperty  rdf:resource="#height"/>
   <sosa:hasResult rdf:resource="#can237ml211-Height"/>
   <sosa:hasSimpleResult rdf:datatype="http://www.qudt.org/2.1/vocab/unit/MilliM">87.8</sosa:hasSimpleResult>
  </rdf:Description>
 </sosa:isFeatureOfInterestOf>
 <!-- Diameter --> 
 <gs1:inPackageDiameter>
  <gs1:QuantitativeValue rdf:about="#can237ml211-Diameter">
   <rdf:type rdf:resource="http://qudt.org/1.1/schema/qudt#QuantityValue"/>
   <qudt:unit rdf:resource="http://www.qudt.org/2.1/vocab/unit/MilliM"/>
   <qudt:numericalValue rdf:datatype="http://www.w3.org/2001/XMLSchema#double">66</qudt:numericalValue>
   <rdf:value rdf:datatype="http://www.w3.org/2001/XMLSchema#double">66</rdf:value>
   <gs1:unitCode>MMT</gs1:unitCode>
   <gs1:value>66</gs1:value>
  </gs1:QuantitativeValue>
 </gs1:inPackageDiameter>
 <sosa:isFeatureOfInterestOf>
  <rdf:Description rdf:about="#can237ml211-DiameterSosa">
   <rdf:type rdf:resource="http://www.w3.org/ns/sosa/Observation"/>
   <sosa:hasFeatureOfInterest rdf:resource="#can237ml211"/>
   <sosa:observedProperty  rdf:resource="#diameter"/>
   <sosa:hasResult rdf:resource="#can237ml211-Diameter"/>
   <sosa:hasSimpleResult rdf:datatype="http://www.qudt.org/2.1/vocab/unit/MilliM">66</sosa:hasSimpleResult>
  </rdf:Description>
 </sosa:isFeatureOfInterestOf>
 <rdfs:isDefinedBy rdf:resource="https://rdf.ag/o/beer-ONTOLOGY_DATE"/>
 <void:inDataset rdf:resource="#datasetdefinition"/>
</rdf:Description>

<rdf:Description rdf:about="#can250ml">
 <rdf:type rdf:resource="#LiquidContainer"/>
 <rdf:type rdf:resource="#BeverageCan"/>
 <rdf:type rdf:resource="https://gs1.org/voc/PackagingDetails"/>
 <rdfs:label xml:lang="en">Any 250ml Can</rdfs:label>
 <rdfs:label xml:lang="fr">Canette à Boisson Métallique, 250ml</rdfs:label>
 <skos:definition xml:lang="en">Any 250ml Can</skos:definition>
 <skos:definition xml:lang="fr">Canette à Boisson Métallique, 250ml</skos:definition>
 <owl:oneOf>
  <rdf:List rdf:about="#can250mlList1">
   <rdf:first rdf:resource="#can250ml204202407"/>
   <rdf:rest>
    <rdf:List rdf:about="#can250mlList2">
     <rdf:first rdf:resource="#can250ml202200510"/>
     <rdf:rest>
      <rdf:List rdf:about="#can250mlList3">
       <rdf:first rdf:resource="#can250ml211202307"/>
       <rdf:rest>
        <rdf:List rdf:about="#can250mlList4">
         <rdf:first rdf:resource="#can250ml211202307-s"/>
         <rdf:rest>
          <rdf:List rdf:about="#can250mlList5">
           <rdf:first rdf:resource="#can250ml211206307"/>
           <rdf:rest rdf:resource="http://www.w3.org/1999/02/22-rdf-syntax-ns#nil"/>
          </rdf:List>
         </rdf:rest>
        </rdf:List>
       </rdf:rest>
      </rdf:List>
     </rdf:rest>
    </rdf:List> 
   </rdf:rest>
  </rdf:List>
 </owl:oneOf>       
</rdf:Description>

<rdf:Description rdf:about="#can250ml204202407">
 <rdf:type rdf:resource="https://gs1.org/voc/PackagingDetails"/>
 <rdf:type rdf:resource="#LiquidContainer"/>
 <rdf:type rdf:resource="#BeverageCan"/>
 <rdfs:label xml:lang="en">8.4oz/250ml Metal Beverage Can</rdfs:label>
 <rdfs:label xml:lang="fr">Canette à Boisson Métallique, 8.4oz/250ml</rdfs:label>
 <skos:definition xml:lang="en">A one time use 8.4oz/250ml metal container meant to hold a liquid, commonly referred to as Sleek 204-202 (Height 407).</skos:definition>
 <skos:definition xml:lang="fr">Un contenant non-réutilisable métallique de 8.4oz/250ml pour contenir un liquide, souvent appeler Sleek 204-202 (Hauteur 407).</skos:definition>
 <!-- Net Content -->
 <gs1:netContent>
  <gs1:QuantitativeValue rdf:about="#can250ml204202407-Content">
    <rdf:type rdf:resource="http://qudt.org/1.1/schema/qudt#QuantityValue"/>
    <qudt:unit rdf:resource="http://www.qudt.org/2.1/vocab/unit/MilliL"/>
    <qudt:numericalValue rdf:datatype="http://www.w3.org/2001/XMLSchema#double">250</qudt:numericalValue>
    <rdf:value rdf:datatype="http://www.w3.org/2001/XMLSchema#double">250</rdf:value>
    <gs1:unitCode>MLT</gs1:unitCode>
    <gs1:value>250</gs1:value>
  </gs1:QuantitativeValue>
 </gs1:netContent> 
 <sosa:isFeatureOfInterestOf>
  <rdf:Description rdf:about="#can250ml204202407-ContentSosa">
   <rdf:type rdf:resource="http://www.w3.org/ns/sosa/Observation"/>
   <sosa:hasFeatureOfInterest rdf:resource="#can250ml204202407"/>
   <sosa:observedProperty  rdf:resource="#netcontent"/>
   <sosa:hasResult rdf:resource="#can250ml204202407-Content"/>
   <sosa:hasSimpleResult rdf:datatype="http://www.qudt.org/2.1/vocab/unit/MilliM">250</sosa:hasSimpleResult>
  </rdf:Description>
 </sosa:isFeatureOfInterestOf>
 <!-- Height -->
 <gs1:inPackageHeight>
  <gs1:QuantitativeValue rdf:about="#can250ml204202407-Height">
   <rdf:type rdf:resource="http://qudt.org/1.1/schema/qudt#QuantityValue"/>
   <qudt:unit rdf:resource="http://www.qudt.org/2.1/vocab/unit/MilliM"/>
   <qudt:numericalValue rdf:datatype="http://www.w3.org/2001/XMLSchema#double">114</qudt:numericalValue>
   <rdf:value rdf:datatype="http://www.w3.org/2001/XMLSchema#double">114</rdf:value>
   <gs1:unitCode>MMT</gs1:unitCode>
   <gs1:value>114</gs1:value>
  </gs1:QuantitativeValue>
 </gs1:inPackageHeight>  
 <sosa:isFeatureOfInterestOf>
  <rdf:Description rdf:about="#can250ml204202407-HeightSosa">
   <rdf:type rdf:resource="http://www.w3.org/ns/sosa/Observation"/>
   <sosa:hasFeatureOfInterest rdf:resource="#can250ml204202407"/>
   <sosa:observedProperty  rdf:resource="#height"/>
   <sosa:hasResult rdf:resource="#can250ml204202407-Height"/>
   <sosa:hasSimpleResult rdf:datatype="http://www.qudt.org/2.1/vocab/unit/MilliM">114</sosa:hasSimpleResult>
  </rdf:Description>
 </sosa:isFeatureOfInterestOf>
 <!-- Diameter --> 
 <gs1:inPackageDiameter>
  <gs1:QuantitativeValue rdf:about="#can250ml204202407-Diameter">
   <rdf:type rdf:resource="http://qudt.org/1.1/schema/qudt#QuantityValue"/>
   <qudt:unit rdf:resource="http://www.qudt.org/2.1/vocab/unit/MilliM"/>
   <qudt:numericalValue rdf:datatype="http://www.w3.org/2001/XMLSchema#double">56.7</qudt:numericalValue>
   <rdf:value rdf:datatype="http://www.w3.org/2001/XMLSchema#double">56.7</rdf:value>
   <gs1:unitCode>MMT</gs1:unitCode>
   <gs1:value>56.7</gs1:value>
  </gs1:QuantitativeValue>
 </gs1:inPackageDiameter>
 <sosa:isFeatureOfInterestOf>
  <rdf:Description rdf:about="#can250ml204202407-DiameterSosa">
   <rdf:type rdf:resource="http://www.w3.org/ns/sosa/Observation"/>
   <sosa:hasFeatureOfInterest rdf:resource="#can250ml204202407"/>
   <sosa:observedProperty  rdf:resource="#diameter"/>
   <sosa:hasResult rdf:resource="#can250ml204202407-Diameter"/>
   <sosa:hasSimpleResult rdf:datatype="http://www.qudt.org/2.1/vocab/unit/MilliM">56.7</sosa:hasSimpleResult>
  </rdf:Description>
 </sosa:isFeatureOfInterestOf>
 <sosa:isFeatureOfInterestOf>
  <rdf:Description rdf:about="#can250ml204202407-EndDiameterSosa">
   <rdf:type rdf:resource="http://www.w3.org/ns/sosa/Observation"/>
   <sosa:hasFeatureOfInterest rdf:resource="#can250ml204202407"/>
   <sosa:observedProperty  rdf:resource="#endDiameter"/>
   <sosa:hasResult>
    <gs1:QuantitativeValue rdf:about="#can250ml204202407-EndDiameter">
     <rdf:type rdf:resource="http://qudt.org/1.1/schema/qudt#QuantityValue"/>
     <qudt:unit rdf:resource="http://www.qudt.org/2.1/vocab/unit/MilliM"/>
     <qudt:numericalValue rdf:datatype="http://www.w3.org/2001/XMLSchema#double">53.55</qudt:numericalValue>
     <rdf:value rdf:datatype="http://www.w3.org/2001/XMLSchema#double">53.55</rdf:value>
     <gs1:unitCode>MMT</gs1:unitCode>
     <gs1:value>53.55</gs1:value>
    </gs1:QuantitativeValue>
   </sosa:hasResult>
   <sosa:hasSimpleResult rdf:datatype="http://www.qudt.org/2.1/vocab/unit/MilliM">53.55</sosa:hasSimpleResult>
  </rdf:Description>
 </sosa:isFeatureOfInterestOf>
 <rdfs:isDefinedBy rdf:resource="https://rdf.ag/o/beer-ONTOLOGY_DATE"/>
 <void:inDataset rdf:resource="#datasetdefinition"/>
</rdf:Description>


<rdf:Description rdf:about="#can250ml202200510">
 <rdf:type rdf:resource="https://gs1.org/voc/PackagingDetails"/>
 <rdf:type rdf:resource="#LiquidContainer"/>
 <rdf:type rdf:resource="#BeverageCan"/>
 <rdfs:label xml:lang="en">8.4oz/250ml Metal Beverage Can</rdfs:label>
 <rdfs:label xml:lang="fr">Canette à Boisson Métallique, 8.4oz/250ml</rdfs:label>
 <skos:definition xml:lang="en">A one time use 8.4oz/250ml metal container meant to hold a liquid, commonly referred to as Slim 202-200 (Height 510).</skos:definition>
 <skos:definition xml:lang="fr">Un contenant non-réutilisable métallique de 8.4oz/250ml pour contenir un liquide, souvent appeler Slim 202-200 (Hauteur 510).</skos:definition>
 <!-- Net Content -->
 <gs1:netContent>
  <gs1:QuantitativeValue rdf:about="#can250ml202200510-Content">
    <rdf:type rdf:resource="http://qudt.org/1.1/schema/qudt#QuantityValue"/>
    <qudt:unit rdf:resource="http://www.qudt.org/2.1/vocab/unit/MilliL"/>
    <qudt:numericalValue rdf:datatype="http://www.w3.org/2001/XMLSchema#double">250</qudt:numericalValue>
    <rdf:value rdf:datatype="http://www.w3.org/2001/XMLSchema#double">250</rdf:value>
    <gs1:unitCode>MLT</gs1:unitCode>
    <gs1:value>250</gs1:value>
  </gs1:QuantitativeValue>
 </gs1:netContent> 
 <sosa:isFeatureOfInterestOf>
  <rdf:Description rdf:about="#can250ml202200510-ContentSosa">
   <rdf:type rdf:resource="http://www.w3.org/ns/sosa/Observation"/>
   <sosa:hasFeatureOfInterest rdf:resource="#can250ml202200510"/>
   <sosa:observedProperty  rdf:resource="#netcontent"/>
   <sosa:hasResult rdf:resource="#can250ml202200510-Content"/>
   <sosa:hasSimpleResult rdf:datatype="http://www.qudt.org/2.1/vocab/unit/MilliM">250</sosa:hasSimpleResult>
  </rdf:Description>
 </sosa:isFeatureOfInterestOf>
 <!-- Height -->
 <gs1:inPackageHeight>
  <gs1:QuantitativeValue rdf:about="#can250ml202200510-Height">
   <rdf:type rdf:resource="http://qudt.org/1.1/schema/qudt#QuantityValue"/>
   <qudt:unit rdf:resource="http://www.qudt.org/2.1/vocab/unit/MilliM"/>
   <qudt:numericalValue rdf:datatype="http://www.w3.org/2001/XMLSchema#double">143</qudt:numericalValue>
   <rdf:value rdf:datatype="http://www.w3.org/2001/XMLSchema#double">143</rdf:value>
   <gs1:unitCode>MMT</gs1:unitCode>
   <gs1:value>143</gs1:value>
  </gs1:QuantitativeValue>
 </gs1:inPackageHeight>  
 <sosa:isFeatureOfInterestOf>
  <rdf:Description rdf:about="#can250ml202200510-HeightSosa">
   <rdf:type rdf:resource="http://www.w3.org/ns/sosa/Observation"/>
   <sosa:hasFeatureOfInterest rdf:resource="#can250ml202200510"/>
   <sosa:observedProperty  rdf:resource="#height"/>
   <sosa:hasResult rdf:resource="#can250ml202200510-Height"/>
   <sosa:hasSimpleResult rdf:datatype="http://www.qudt.org/2.1/vocab/unit/MilliM">143</sosa:hasSimpleResult>
  </rdf:Description>
 </sosa:isFeatureOfInterestOf>
 <!-- Diameter --> 
 <gs1:inPackageDiameter>
  <gs1:QuantitativeValue rdf:about="#can250ml202200510-Diameter">
   <rdf:type rdf:resource="http://qudt.org/1.1/schema/qudt#QuantityValue"/>
   <qudt:unit rdf:resource="http://www.qudt.org/2.1/vocab/unit/MilliM"/>
   <qudt:numericalValue rdf:datatype="http://www.w3.org/2001/XMLSchema#double">52.8</qudt:numericalValue>
   <rdf:value rdf:datatype="http://www.w3.org/2001/XMLSchema#double">52.8</rdf:value>
   <gs1:unitCode>MMT</gs1:unitCode>
   <gs1:value>52.8</gs1:value>
  </gs1:QuantitativeValue>
 </gs1:inPackageDiameter>
 <sosa:isFeatureOfInterestOf>
  <rdf:Description rdf:about="#can250ml202200510-DiameterSosa">
   <rdf:type rdf:resource="http://www.w3.org/ns/sosa/Observation"/>
   <sosa:hasFeatureOfInterest rdf:resource="#can250ml202200510"/>
   <sosa:observedProperty  rdf:resource="#diameter"/>
   <sosa:hasResult rdf:resource="#can250ml202200510-Diameter"/>
   <sosa:hasSimpleResult rdf:datatype="http://www.qudt.org/2.1/vocab/unit/MilliM">52.8</sosa:hasSimpleResult>
  </rdf:Description>
 </sosa:isFeatureOfInterestOf>
 <sosa:isFeatureOfInterestOf>
  <rdf:Description rdf:about="#can250ml202200510-EndDiameterSosa">
   <rdf:type rdf:resource="http://www.w3.org/ns/sosa/Observation"/>
   <sosa:hasFeatureOfInterest rdf:resource="#can250ml202200510"/>
   <sosa:observedProperty  rdf:resource="#endDiameter"/>
   <sosa:hasResult>
    <gs1:QuantitativeValue rdf:about="#can250ml202200510-EndDiameter">
     <rdf:type rdf:resource="http://qudt.org/1.1/schema/qudt#QuantityValue"/>
     <qudt:unit rdf:resource="http://www.qudt.org/2.1/vocab/unit/MilliM"/>
     <qudt:numericalValue rdf:datatype="http://www.w3.org/2001/XMLSchema#double">50.4</qudt:numericalValue>
     <rdf:value rdf:datatype="http://www.w3.org/2001/XMLSchema#double">50.4</rdf:value>
     <gs1:unitCode>MMT</gs1:unitCode>
     <gs1:value>50.4</gs1:value>
    </gs1:QuantitativeValue>
   </sosa:hasResult>
   <sosa:hasSimpleResult rdf:datatype="http://www.qudt.org/2.1/vocab/unit/MilliM">50.4</sosa:hasSimpleResult>
  </rdf:Description>
 </sosa:isFeatureOfInterestOf>
 <rdfs:isDefinedBy rdf:resource="https://rdf.ag/o/beer-ONTOLOGY_DATE"/>
 <void:inDataset rdf:resource="#datasetdefinition"/>
</rdf:Description>


<rdf:Description rdf:about="#can250ml211202307">
 <rdf:type rdf:resource="https://gs1.org/voc/PackagingDetails"/>
 <rdf:type rdf:resource="#LiquidContainer"/>
 <rdf:type rdf:resource="#BeverageCan"/>
 <rdfs:label xml:lang="en">8.4oz/250ml Metal Beverage Can</rdfs:label>
 <rdfs:label xml:lang="fr">Canette à Boisson Métallique, 8.4oz/250ml</rdfs:label>
 <skos:definition xml:lang="en">A one time use 8.4oz/250ml metal container meant to hold a liquid, commonly referred to as Standard 211-202 (Height 307).</skos:definition>
 <skos:definition xml:lang="fr">Un contenant non-réutilisable métallique de 8.4oz/250ml pour contenir un liquide, souvent appeler Standard 211-202 (Hauteur 307).</skos:definition>
 <!-- Net Content -->
 <gs1:netContent>
  <gs1:QuantitativeValue rdf:about="#can250ml211202307-Content">
    <rdf:type rdf:resource="http://qudt.org/1.1/schema/qudt#QuantityValue"/>
    <qudt:unit rdf:resource="http://www.qudt.org/2.1/vocab/unit/MilliL"/>
    <qudt:numericalValue rdf:datatype="http://www.w3.org/2001/XMLSchema#double">250</qudt:numericalValue>
    <rdf:value rdf:datatype="http://www.w3.org/2001/XMLSchema#double">250</rdf:value>
    <gs1:unitCode>MLT</gs1:unitCode>
    <gs1:value>250</gs1:value>
  </gs1:QuantitativeValue>
 </gs1:netContent> 
 <sosa:isFeatureOfInterestOf>
  <rdf:Description rdf:about="#can250ml211202307-ContentSosa">
   <rdf:type rdf:resource="http://www.w3.org/ns/sosa/Observation"/>
   <sosa:hasFeatureOfInterest rdf:resource="#can250ml211202307"/>
   <sosa:observedProperty  rdf:resource="#netcontent"/>
   <sosa:hasResult rdf:resource="#can250ml211202307-Content"/>
   <sosa:hasSimpleResult rdf:datatype="http://www.qudt.org/2.1/vocab/unit/MilliM">250</sosa:hasSimpleResult>
  </rdf:Description>
 </sosa:isFeatureOfInterestOf>
 <!-- Height -->
 <gs1:inPackageHeight>
  <gs1:QuantitativeValue rdf:about="#can250ml211202307-Height">
   <rdf:type rdf:resource="http://qudt.org/1.1/schema/qudt#QuantityValue"/>
   <qudt:unit rdf:resource="http://www.qudt.org/2.1/vocab/unit/MilliM"/>
   <qudt:numericalValue rdf:datatype="http://www.w3.org/2001/XMLSchema#double">91.6</qudt:numericalValue>
   <rdf:value rdf:datatype="http://www.w3.org/2001/XMLSchema#double">91.6</rdf:value>
   <gs1:unitCode>MMT</gs1:unitCode>
   <gs1:value>91.6</gs1:value>
  </gs1:QuantitativeValue>
 </gs1:inPackageHeight>  
 <sosa:isFeatureOfInterestOf>
  <rdf:Description rdf:about="#can250ml211202307-HeightSosa">
   <rdf:type rdf:resource="http://www.w3.org/ns/sosa/Observation"/>
   <sosa:hasFeatureOfInterest rdf:resource="#can250ml211202307"/>
   <sosa:observedProperty  rdf:resource="#height"/>
   <sosa:hasResult rdf:resource="#can250ml211202307-Height"/>
   <sosa:hasSimpleResult rdf:datatype="http://www.qudt.org/2.1/vocab/unit/MilliM">91.6</sosa:hasSimpleResult>
  </rdf:Description>
 </sosa:isFeatureOfInterestOf>
 <!-- Diameter --> 
 <gs1:inPackageDiameter>
  <gs1:QuantitativeValue rdf:about="#can250ml211202307-Diameter">
   <rdf:type rdf:resource="http://qudt.org/1.1/schema/qudt#QuantityValue"/>
   <qudt:unit rdf:resource="http://www.qudt.org/2.1/vocab/unit/MilliM"/>
   <qudt:numericalValue rdf:datatype="http://www.w3.org/2001/XMLSchema#double">66</qudt:numericalValue>
   <rdf:value rdf:datatype="http://www.w3.org/2001/XMLSchema#double">66</rdf:value>
   <gs1:unitCode>MMT</gs1:unitCode>
   <gs1:value>66</gs1:value>
  </gs1:QuantitativeValue>
 </gs1:inPackageDiameter>
 <sosa:isFeatureOfInterestOf>
  <rdf:Description rdf:about="#can250ml211202307-DiameterSosa">
   <rdf:type rdf:resource="http://www.w3.org/ns/sosa/Observation"/>
   <sosa:hasFeatureOfInterest rdf:resource="#can250ml211202307"/>
   <sosa:observedProperty  rdf:resource="#diameter"/>
   <sosa:hasResult rdf:resource="#can250ml211202307-Diameter"/>
   <sosa:hasSimpleResult rdf:datatype="http://www.qudt.org/2.1/vocab/unit/MilliM">66</sosa:hasSimpleResult>
  </rdf:Description>
 </sosa:isFeatureOfInterestOf>
 <sosa:isFeatureOfInterestOf>
  <rdf:Description rdf:about="#can250ml211202307-EndDiameterSosa">
   <rdf:type rdf:resource="http://www.w3.org/ns/sosa/Observation"/>
   <sosa:hasFeatureOfInterest rdf:resource="#can250ml211202307"/>
   <sosa:observedProperty  rdf:resource="#endDiameter"/>
   <sosa:hasResult>
    <gs1:QuantitativeValue rdf:about="#can250ml211202307-EndDiameter">
     <rdf:type rdf:resource="http://qudt.org/1.1/schema/qudt#QuantityValue"/>
     <qudt:unit rdf:resource="http://www.qudt.org/2.1/vocab/unit/MilliM"/>
     <qudt:numericalValue rdf:datatype="http://www.w3.org/2001/XMLSchema#double">53.55</qudt:numericalValue>
     <rdf:value rdf:datatype="http://www.w3.org/2001/XMLSchema#double">53.55</rdf:value>
     <gs1:unitCode>MMT</gs1:unitCode>
     <gs1:value>53.55</gs1:value>
    </gs1:QuantitativeValue>
   </sosa:hasResult>
   <sosa:hasSimpleResult rdf:datatype="http://www.qudt.org/2.1/vocab/unit/MilliM">53.55</sosa:hasSimpleResult>
  </rdf:Description>
 </sosa:isFeatureOfInterestOf>
 <rdfs:isDefinedBy rdf:resource="https://rdf.ag/o/beer-ONTOLOGY_DATE"/>
 <void:inDataset rdf:resource="#datasetdefinition"/>
</rdf:Description>


<rdf:Description rdf:about="#can250ml211202307-s">
 <rdf:type rdf:resource="https://gs1.org/voc/PackagingDetails"/>
 <rdf:type rdf:resource="#LiquidContainer"/>
 <rdf:type rdf:resource="#BeverageCan"/>
 <rdfs:label xml:lang="en">8.4oz/250ml Metal Beverage Can</rdfs:label>
 <rdfs:label xml:lang="fr">Canette à Boisson Métallique, 8.4oz/250ml</rdfs:label>
 <skos:definition xml:lang="en">A one time use 8.4oz/250ml metal container meant to hold a liquid, commonly referred to as Stubby 211-202 (Height 307).</skos:definition>
 <skos:definition xml:lang="fr">Un contenant non-réutilisable métallique de 8.4oz/250ml pour contenir un liquide, souvent appeler Stubby 211-202 (Hauteur 307).</skos:definition>
 <!-- Net Content -->
 <gs1:netContent>
  <gs1:QuantitativeValue rdf:about="#can250ml211202307-s-Content">
    <rdf:type rdf:resource="http://qudt.org/1.1/schema/qudt#QuantityValue"/>
    <qudt:unit rdf:resource="http://www.qudt.org/2.1/vocab/unit/MilliL"/>
    <qudt:numericalValue rdf:datatype="http://www.w3.org/2001/XMLSchema#double">250</qudt:numericalValue>
    <rdf:value rdf:datatype="http://www.w3.org/2001/XMLSchema#double">250</rdf:value>
    <gs1:unitCode>MLT</gs1:unitCode>
    <gs1:value>250</gs1:value>
  </gs1:QuantitativeValue>
 </gs1:netContent> 
 <sosa:isFeatureOfInterestOf>
  <rdf:Description rdf:about="#can250ml211202307-s-ContentSosa">
   <rdf:type rdf:resource="http://www.w3.org/ns/sosa/Observation"/>
   <sosa:hasFeatureOfInterest rdf:resource="#can250ml211202307-s"/>
   <sosa:observedProperty  rdf:resource="#netcontent"/>
   <sosa:hasResult rdf:resource="#can250ml211202307-s-Content"/>
   <sosa:hasSimpleResult rdf:datatype="http://www.qudt.org/2.1/vocab/unit/MilliM">250</sosa:hasSimpleResult>
  </rdf:Description>
 </sosa:isFeatureOfInterestOf>
 <!-- Height -->
 <gs1:inPackageHeight>
  <gs1:QuantitativeValue rdf:about="#can250ml211202307-s-Height">
   <rdf:type rdf:resource="http://qudt.org/1.1/schema/qudt#QuantityValue"/>
   <qudt:unit rdf:resource="http://www.qudt.org/2.1/vocab/unit/MilliM"/>
   <qudt:numericalValue rdf:datatype="http://www.w3.org/2001/XMLSchema#double">91.6</qudt:numericalValue>
   <rdf:value rdf:datatype="http://www.w3.org/2001/XMLSchema#double">91.6</rdf:value>
   <gs1:unitCode>MMT</gs1:unitCode>
   <gs1:value>91.6</gs1:value>
  </gs1:QuantitativeValue>
 </gs1:inPackageHeight>  
 <sosa:isFeatureOfInterestOf>
  <rdf:Description rdf:about="#can250ml211202307-s-HeightSosa">
   <rdf:type rdf:resource="http://www.w3.org/ns/sosa/Observation"/>
   <sosa:hasFeatureOfInterest rdf:resource="#can250ml211202307-s"/>
   <sosa:observedProperty  rdf:resource="#height"/>
   <sosa:hasResult rdf:resource="#can250ml211202307-s-Height"/>
   <sosa:hasSimpleResult rdf:datatype="http://www.qudt.org/2.1/vocab/unit/MilliM">91.6</sosa:hasSimpleResult>
  </rdf:Description>
 </sosa:isFeatureOfInterestOf>
 <!-- Diameter --> 
 <gs1:inPackageDiameter>
  <gs1:QuantitativeValue rdf:about="#can250ml211202307-s-Diameter">
   <rdf:type rdf:resource="http://qudt.org/1.1/schema/qudt#QuantityValue"/>
   <qudt:unit rdf:resource="http://www.qudt.org/2.1/vocab/unit/MilliM"/>
   <qudt:numericalValue rdf:datatype="http://www.w3.org/2001/XMLSchema#double">66</qudt:numericalValue>
   <rdf:value rdf:datatype="http://www.w3.org/2001/XMLSchema#double">66</rdf:value>
   <gs1:unitCode>MMT</gs1:unitCode>
   <gs1:value>66</gs1:value>
  </gs1:QuantitativeValue>
 </gs1:inPackageDiameter>
 <sosa:isFeatureOfInterestOf>
  <rdf:Description rdf:about="#can250ml211202307-s-DiameterSosa">
   <rdf:type rdf:resource="http://www.w3.org/ns/sosa/Observation"/>
   <sosa:hasFeatureOfInterest rdf:resource="#can250ml211202307-s"/>
   <sosa:observedProperty  rdf:resource="#diameter"/>
   <sosa:hasResult rdf:resource="#can250ml211202307-s-Diameter"/>
   <sosa:hasSimpleResult rdf:datatype="http://www.qudt.org/2.1/vocab/unit/MilliM">66</sosa:hasSimpleResult>
  </rdf:Description>
 </sosa:isFeatureOfInterestOf>
 <sosa:isFeatureOfInterestOf>
  <rdf:Description rdf:about="#can250ml211202307-s-EndDiameterSosa">
   <rdf:type rdf:resource="http://www.w3.org/ns/sosa/Observation"/>
   <sosa:hasFeatureOfInterest rdf:resource="#can250ml211202307-s"/>
   <sosa:observedProperty  rdf:resource="#endDiameter"/>
   <sosa:hasResult>
    <gs1:QuantitativeValue rdf:about="#can250ml211202307-s-EndDiameter">
     <rdf:type rdf:resource="http://qudt.org/1.1/schema/qudt#QuantityValue"/>
     <qudt:unit rdf:resource="http://www.qudt.org/2.1/vocab/unit/MilliM"/>
     <qudt:numericalValue rdf:datatype="http://www.w3.org/2001/XMLSchema#double">53.55</qudt:numericalValue>
     <rdf:value rdf:datatype="http://www.w3.org/2001/XMLSchema#double">53.55</rdf:value>
     <gs1:unitCode>MMT</gs1:unitCode>
     <gs1:value>53.55</gs1:value>
    </gs1:QuantitativeValue>
   </sosa:hasResult>
   <sosa:hasSimpleResult rdf:datatype="http://www.qudt.org/2.1/vocab/unit/MilliM">53.55</sosa:hasSimpleResult>
  </rdf:Description>
 </sosa:isFeatureOfInterestOf>
 <rdfs:isDefinedBy rdf:resource="https://rdf.ag/o/beer-ONTOLOGY_DATE"/>
 <void:inDataset rdf:resource="#datasetdefinition"/>
</rdf:Description>


<rdf:Description rdf:about="#can250ml211206307">
 <rdf:type rdf:resource="https://gs1.org/voc/PackagingDetails"/>
 <rdf:type rdf:resource="#LiquidContainer"/>
 <rdf:type rdf:resource="#BeverageCan"/>
 <rdfs:label xml:lang="en">8.4oz/250ml Metal Beverage Can</rdfs:label>
 <rdfs:label xml:lang="fr">Canette à Boisson Métallique, 8.4oz/250ml</rdfs:label>
 <skos:definition xml:lang="en">A one time use 8.4oz/250ml metal container meant to hold a liquid, commonly referred to as Stubby 211-206 (Height 307).</skos:definition>
 <skos:definition xml:lang="fr">Un contenant non-réutilisable métallique de 8.4oz/250ml pour contenir un liquide, souvent appeler Stubby 211-206 (Hauteur 307).</skos:definition>
 <!-- Net Content -->
 <gs1:netContent>
  <gs1:QuantitativeValue rdf:about="#can250ml211206307-Content">
    <rdf:type rdf:resource="http://qudt.org/1.1/schema/qudt#QuantityValue"/>
    <qudt:unit rdf:resource="http://www.qudt.org/2.1/vocab/unit/MilliL"/>
    <qudt:numericalValue rdf:datatype="http://www.w3.org/2001/XMLSchema#double">250</qudt:numericalValue>
    <rdf:value rdf:datatype="http://www.w3.org/2001/XMLSchema#double">250</rdf:value>
    <gs1:unitCode>MLT</gs1:unitCode>
    <gs1:value>250</gs1:value>
  </gs1:QuantitativeValue>
 </gs1:netContent> 
 <sosa:isFeatureOfInterestOf>
  <rdf:Description rdf:about="#can250ml211206307-ContentSosa">
   <rdf:type rdf:resource="http://www.w3.org/ns/sosa/Observation"/>
   <sosa:hasFeatureOfInterest rdf:resource="#can250ml211206307"/>
   <sosa:observedProperty  rdf:resource="#netcontent"/>
   <sosa:hasResult rdf:resource="#can250ml211206307-Content"/>
   <sosa:hasSimpleResult rdf:datatype="http://www.qudt.org/2.1/vocab/unit/MilliM">250</sosa:hasSimpleResult>
  </rdf:Description>
 </sosa:isFeatureOfInterestOf>
 <!-- Height -->
 <gs1:inPackageHeight>
  <gs1:QuantitativeValue rdf:about="#can250ml211206307-Height">
   <rdf:type rdf:resource="http://qudt.org/1.1/schema/qudt#QuantityValue"/>
   <qudt:unit rdf:resource="http://www.qudt.org/2.1/vocab/unit/MilliM"/>
   <qudt:numericalValue rdf:datatype="http://www.w3.org/2001/XMLSchema#double">91.6</qudt:numericalValue>
   <rdf:value rdf:datatype="http://www.w3.org/2001/XMLSchema#double">91.6</rdf:value>
   <gs1:unitCode>MMT</gs1:unitCode>
   <gs1:value>91.6</gs1:value>
  </gs1:QuantitativeValue>
 </gs1:inPackageHeight>  
 <sosa:isFeatureOfInterestOf>
  <rdf:Description rdf:about="#can250ml211206307-HeightSosa">
   <rdf:type rdf:resource="http://www.w3.org/ns/sosa/Observation"/>
   <sosa:hasFeatureOfInterest rdf:resource="#can250ml211206307"/>
   <sosa:observedProperty  rdf:resource="#height"/>
   <sosa:hasResult rdf:resource="#can250ml211206307-Height"/>
   <sosa:hasSimpleResult rdf:datatype="http://www.qudt.org/2.1/vocab/unit/MilliM">91.6</sosa:hasSimpleResult>
  </rdf:Description>
 </sosa:isFeatureOfInterestOf>
 <!-- Diameter --> 
 <gs1:inPackageDiameter>
  <gs1:QuantitativeValue rdf:about="#can250ml211206307-Diameter">
   <rdf:type rdf:resource="http://qudt.org/1.1/schema/qudt#QuantityValue"/>
   <qudt:unit rdf:resource="http://www.qudt.org/2.1/vocab/unit/MilliM"/>
   <qudt:numericalValue rdf:datatype="http://www.w3.org/2001/XMLSchema#double">66</qudt:numericalValue>
   <rdf:value rdf:datatype="http://www.w3.org/2001/XMLSchema#double">66</rdf:value>
   <gs1:unitCode>MMT</gs1:unitCode>
   <gs1:value>66</gs1:value>
  </gs1:QuantitativeValue>
 </gs1:inPackageDiameter>
 <sosa:isFeatureOfInterestOf>
  <rdf:Description rdf:about="#can250ml211206307-DiameterSosa">
   <rdf:type rdf:resource="http://www.w3.org/ns/sosa/Observation"/>
   <sosa:hasFeatureOfInterest rdf:resource="#can250ml211206307"/>
   <sosa:observedProperty  rdf:resource="#diameter"/>
   <sosa:hasResult rdf:resource="#can250ml211206307-Diameter"/>
   <sosa:hasSimpleResult rdf:datatype="http://www.qudt.org/2.1/vocab/unit/MilliM">66</sosa:hasSimpleResult>
  </rdf:Description>
 </sosa:isFeatureOfInterestOf>
 <sosa:isFeatureOfInterestOf>
  <rdf:Description rdf:about="#can250ml211206307-EndDiameterSosa">
   <rdf:type rdf:resource="http://www.w3.org/ns/sosa/Observation"/>
   <sosa:hasFeatureOfInterest rdf:resource="#can250ml211206307"/>
   <sosa:observedProperty  rdf:resource="#endDiameter"/>
   <sosa:hasResult>
    <gs1:QuantitativeValue rdf:about="#can250ml211206307-EndDiameter">
     <rdf:type rdf:resource="http://qudt.org/1.1/schema/qudt#QuantityValue"/>
     <qudt:unit rdf:resource="http://www.qudt.org/2.1/vocab/unit/MilliM"/>
     <qudt:numericalValue rdf:datatype="http://www.w3.org/2001/XMLSchema#double">59.85</qudt:numericalValue>
     <rdf:value rdf:datatype="http://www.w3.org/2001/XMLSchema#double">59.85</rdf:value>
     <gs1:unitCode>MMT</gs1:unitCode>
     <gs1:value>59.85</gs1:value>
    </gs1:QuantitativeValue>
   </sosa:hasResult>
   <sosa:hasSimpleResult rdf:datatype="http://www.qudt.org/2.1/vocab/unit/MilliM">59.85</sosa:hasSimpleResult>
  </rdf:Description>
 </sosa:isFeatureOfInterestOf>
 <rdfs:isDefinedBy rdf:resource="https://rdf.ag/o/beer-ONTOLOGY_DATE"/>
 <void:inDataset rdf:resource="#datasetdefinition"/>
</rdf:Description>


<rdf:Description rdf:about="#can296ml">
 <rdf:type rdf:resource="https://gs1.org/voc/PackagingDetails"/>
 <rdf:type rdf:resource="#LiquidContainer"/>
 <rdf:type rdf:resource="#BeverageCan"/>
 <rdfs:label xml:lang="en">10oz/296ml Metal Beverage Can</rdfs:label>
 <rdfs:label xml:lang="fr">Canette à Boisson Métallique, 10oz/296ml</rdfs:label>
 <skos:definition xml:lang="en">A one time use 10oz/296ml metal container meant to hold a liquid, commonly referred to as Super Sleek 207.5-202 (Height 413).</skos:definition>
 <skos:definition xml:lang="fr">Un contenant non-réutilisable métallique de 10oz/296ml pour contenir un liquide, souvent appeler Super Sleek 207.5-202 (Hauteur 413).</skos:definition>
 <!-- Net Content -->
 <gs1:netContent>
  <gs1:QuantitativeValue rdf:about="#can296ml-Content">
    <rdf:type rdf:resource="http://qudt.org/1.1/schema/qudt#QuantityValue"/>
    <qudt:unit rdf:resource="http://www.qudt.org/2.1/vocab/unit/MilliL"/>
    <qudt:numericalValue rdf:datatype="http://www.w3.org/2001/XMLSchema#double">296</qudt:numericalValue>
    <rdf:value rdf:datatype="http://www.w3.org/2001/XMLSchema#double">296</rdf:value>
    <gs1:unitCode>MLT</gs1:unitCode>
    <gs1:value>296</gs1:value>
  </gs1:QuantitativeValue>
 </gs1:netContent> 
 <sosa:isFeatureOfInterestOf>
  <rdf:Description rdf:about="#can296ml-ContentSosa">
   <rdf:type rdf:resource="http://www.w3.org/ns/sosa/Observation"/>
   <sosa:hasFeatureOfInterest rdf:resource="#can296ml"/>
   <sosa:observedProperty  rdf:resource="#netcontent"/>
   <sosa:hasResult rdf:resource="#can296ml-Content"/>
   <sosa:hasSimpleResult rdf:datatype="http://www.qudt.org/2.1/vocab/unit/MilliM">296</sosa:hasSimpleResult>
  </rdf:Description>
 </sosa:isFeatureOfInterestOf>
 <!-- Height -->
 <gs1:inPackageHeight>
  <gs1:QuantitativeValue rdf:about="#can296ml-Height">
   <rdf:type rdf:resource="http://qudt.org/1.1/schema/qudt#QuantityValue"/>
   <qudt:unit rdf:resource="http://www.qudt.org/2.1/vocab/unit/MilliM"/>
   <qudt:numericalValue rdf:datatype="http://www.w3.org/2001/XMLSchema#double">122</qudt:numericalValue>
   <rdf:value rdf:datatype="http://www.w3.org/2001/XMLSchema#double">122</rdf:value>
   <gs1:unitCode>MMT</gs1:unitCode>
   <gs1:value>122</gs1:value>
  </gs1:QuantitativeValue>
 </gs1:inPackageHeight>  
 <sosa:isFeatureOfInterestOf>
  <rdf:Description rdf:about="#can296ml-HeightSosa">
   <rdf:type rdf:resource="http://www.w3.org/ns/sosa/Observation"/>
   <sosa:hasFeatureOfInterest rdf:resource="#can296ml"/>
   <sosa:observedProperty  rdf:resource="#height"/>
   <sosa:hasResult rdf:resource="#can296ml-Height"/>
   <sosa:hasSimpleResult rdf:datatype="http://www.qudt.org/2.1/vocab/unit/MilliM">122</sosa:hasSimpleResult>
  </rdf:Description>
 </sosa:isFeatureOfInterestOf>
 <!-- Diameter --> 
 <gs1:inPackageDiameter>
  <gs1:QuantitativeValue rdf:about="#can296ml-Diameter">
   <rdf:type rdf:resource="http://qudt.org/1.1/schema/qudt#QuantityValue"/>
   <qudt:unit rdf:resource="http://www.qudt.org/2.1/vocab/unit/MilliM"/>
   <qudt:numericalValue rdf:datatype="http://www.w3.org/2001/XMLSchema#double">60</qudt:numericalValue>
   <rdf:value rdf:datatype="http://www.w3.org/2001/XMLSchema#double">60</rdf:value>
   <gs1:unitCode>MMT</gs1:unitCode>
   <gs1:value>60</gs1:value>
  </gs1:QuantitativeValue>
 </gs1:inPackageDiameter>
 <sosa:isFeatureOfInterestOf>
  <rdf:Description rdf:about="#can296ml-DiameterSosa">
   <rdf:type rdf:resource="http://www.w3.org/ns/sosa/Observation"/>
   <sosa:hasFeatureOfInterest rdf:resource="#can296ml"/>
   <sosa:observedProperty  rdf:resource="#diameter"/>
   <sosa:hasResult rdf:resource="#can296ml-Diameter"/>
   <sosa:hasSimpleResult rdf:datatype="http://www.qudt.org/2.1/vocab/unit/MilliM">60</sosa:hasSimpleResult>
  </rdf:Description>
 </sosa:isFeatureOfInterestOf>
 <sosa:isFeatureOfInterestOf>
  <rdf:Description rdf:about="#can296ml-EndDiameterSosa">
   <rdf:type rdf:resource="http://www.w3.org/ns/sosa/Observation"/>
   <sosa:hasFeatureOfInterest rdf:resource="#can296ml"/>
   <sosa:observedProperty  rdf:resource="#endDiameter"/>
   <sosa:hasResult>
    <gs1:QuantitativeValue rdf:about="#can296ml-EndDiameter">
     <rdf:type rdf:resource="http://qudt.org/1.1/schema/qudt#QuantityValue"/>
     <qudt:unit rdf:resource="http://www.qudt.org/2.1/vocab/unit/MilliM"/>
     <qudt:numericalValue rdf:datatype="http://www.w3.org/2001/XMLSchema#double">53.55</qudt:numericalValue>
     <rdf:value rdf:datatype="http://www.w3.org/2001/XMLSchema#double">53.55</rdf:value>
     <gs1:unitCode>MMT</gs1:unitCode>
     <gs1:value>53.55</gs1:value>
    </gs1:QuantitativeValue>
   </sosa:hasResult>
   <sosa:hasSimpleResult rdf:datatype="http://www.qudt.org/2.1/vocab/unit/MilliM">53.55</sosa:hasSimpleResult>
  </rdf:Description>
 </sosa:isFeatureOfInterestOf>
 <rdfs:isDefinedBy rdf:resource="https://rdf.ag/o/beer-ONTOLOGY_DATE"/>
 <void:inDataset rdf:resource="#datasetdefinition"/>
</rdf:Description>


<rdf:Description rdf:about="#can333ml">
 <rdf:type rdf:resource="https://gs1.org/voc/PackagingDetails"/>
 <rdf:type rdf:resource="#LiquidContainer"/>
 <rdf:type rdf:resource="#BeverageCan"/>
 <rdfs:label xml:lang="en">11.3oz/333ml Metal Beverage Can</rdfs:label>
 <rdfs:label xml:lang="fr">Canette à Boisson Métallique, 11.3oz/333ml</rdfs:label>
 <skos:definition xml:lang="en">A one time use 11.3oz/333ml metal container meant to hold a liquid, commonly referred to as Standard 211-202 (Height 409).</skos:definition>
 <skos:definition xml:lang="fr">Un contenant non-réutilisable métallique de 11.3oz/333ml pour contenir un liquide, souvent appeler Standard 211-202 (Hauteur 409).</skos:definition>
 <!-- Net Content -->
 <gs1:netContent>
  <gs1:QuantitativeValue rdf:about="#can333ml-Content">
    <rdf:type rdf:resource="http://qudt.org/1.1/schema/qudt#QuantityValue"/>
    <qudt:unit rdf:resource="http://www.qudt.org/2.1/vocab/unit/MilliL"/>
    <qudt:numericalValue rdf:datatype="http://www.w3.org/2001/XMLSchema#double">333</qudt:numericalValue>
    <rdf:value rdf:datatype="http://www.w3.org/2001/XMLSchema#double">333</rdf:value>
    <gs1:unitCode>MLT</gs1:unitCode>
    <gs1:value>333</gs1:value>
  </gs1:QuantitativeValue>
 </gs1:netContent> 
 <sosa:isFeatureOfInterestOf>
  <rdf:Description rdf:about="#can333ml-ContentSosa">
   <rdf:type rdf:resource="http://www.w3.org/ns/sosa/Observation"/>
   <sosa:hasFeatureOfInterest rdf:resource="#can333ml"/>
   <sosa:observedProperty  rdf:resource="#netcontent"/>
   <sosa:hasResult rdf:resource="#can333ml-Content"/>
   <sosa:hasSimpleResult rdf:datatype="http://www.qudt.org/2.1/vocab/unit/MilliM">333</sosa:hasSimpleResult>
  </rdf:Description>
 </sosa:isFeatureOfInterestOf>
 <!-- Height -->
 <gs1:inPackageHeight>
  <gs1:QuantitativeValue rdf:about="#can333ml-Height">
   <rdf:type rdf:resource="http://qudt.org/1.1/schema/qudt#QuantityValue"/>
   <qudt:unit rdf:resource="http://www.qudt.org/2.1/vocab/unit/MilliM"/>
   <qudt:numericalValue rdf:datatype="http://www.w3.org/2001/XMLSchema#double">115</qudt:numericalValue>
   <rdf:value rdf:datatype="http://www.w3.org/2001/XMLSchema#double">115</rdf:value>
   <gs1:unitCode>MMT</gs1:unitCode>
   <gs1:value>115</gs1:value>
  </gs1:QuantitativeValue>
 </gs1:inPackageHeight>  
 <sosa:isFeatureOfInterestOf>
  <rdf:Description rdf:about="#can333ml-HeightSosa">
   <rdf:type rdf:resource="http://www.w3.org/ns/sosa/Observation"/>
   <sosa:hasFeatureOfInterest rdf:resource="#can333ml"/>
   <sosa:observedProperty  rdf:resource="#height"/>
   <sosa:hasResult rdf:resource="#can333ml-Height"/>
   <sosa:hasSimpleResult rdf:datatype="http://www.qudt.org/2.1/vocab/unit/MilliM">115</sosa:hasSimpleResult>
  </rdf:Description>
 </sosa:isFeatureOfInterestOf>
 <!-- Diameter --> 
 <gs1:inPackageDiameter>
  <gs1:QuantitativeValue rdf:about="#can333ml-Diameter">
   <rdf:type rdf:resource="http://qudt.org/1.1/schema/qudt#QuantityValue"/>
   <qudt:unit rdf:resource="http://www.qudt.org/2.1/vocab/unit/MilliM"/>
   <qudt:numericalValue rdf:datatype="http://www.w3.org/2001/XMLSchema#double">66</qudt:numericalValue>
   <rdf:value rdf:datatype="http://www.w3.org/2001/XMLSchema#double">66</rdf:value>
   <gs1:unitCode>MMT</gs1:unitCode>
   <gs1:value>66</gs1:value>
  </gs1:QuantitativeValue>
 </gs1:inPackageDiameter>
 <sosa:isFeatureOfInterestOf>
  <rdf:Description rdf:about="#can333ml-DiameterSosa">
   <rdf:type rdf:resource="http://www.w3.org/ns/sosa/Observation"/>
   <sosa:hasFeatureOfInterest rdf:resource="#can333ml"/>
   <sosa:observedProperty  rdf:resource="#diameter"/>
   <sosa:hasResult rdf:resource="#can333ml-Diameter"/>
   <sosa:hasSimpleResult rdf:datatype="http://www.qudt.org/2.1/vocab/unit/MilliM">66</sosa:hasSimpleResult>
  </rdf:Description>
 </sosa:isFeatureOfInterestOf>
 <sosa:isFeatureOfInterestOf>
  <rdf:Description rdf:about="#can333ml-EndDiameterSosa">
   <rdf:type rdf:resource="http://www.w3.org/ns/sosa/Observation"/>
   <sosa:hasFeatureOfInterest rdf:resource="#can333ml"/>
   <sosa:observedProperty  rdf:resource="#endDiameter"/>
   <sosa:hasResult>
    <gs1:QuantitativeValue rdf:about="#can333ml-EndDiameter">
     <rdf:type rdf:resource="http://qudt.org/1.1/schema/qudt#QuantityValue"/>
     <qudt:unit rdf:resource="http://www.qudt.org/2.1/vocab/unit/MilliM"/>
     <qudt:numericalValue rdf:datatype="http://www.w3.org/2001/XMLSchema#double">53.55</qudt:numericalValue>
     <rdf:value rdf:datatype="http://www.w3.org/2001/XMLSchema#double">53.55</rdf:value>
     <gs1:unitCode>MMT</gs1:unitCode>
     <gs1:value>53.55</gs1:value>
    </gs1:QuantitativeValue>
   </sosa:hasResult>
   <sosa:hasSimpleResult rdf:datatype="http://www.qudt.org/2.1/vocab/unit/MilliM">53.55</sosa:hasSimpleResult>
  </rdf:Description>
 </sosa:isFeatureOfInterestOf>
 <rdfs:isDefinedBy rdf:resource="https://rdf.ag/o/beer-ONTOLOGY_DATE"/>
 <void:inDataset rdf:resource="#datasetdefinition"/>
</rdf:Description>


<rdf:Description rdf:about="#can341ml">
 <rdf:type rdf:resource="https://gs1.org/voc/PackagingDetails"/>
 <rdf:type rdf:resource="#LiquidContainer"/>
 <rdf:type rdf:resource="#BeverageCan"/>
 <rdfs:label xml:lang="en">11.5oz/341ml Metal Beverage Can</rdfs:label>
 <rdfs:label xml:lang="fr">Canette à Boisson Métallique, 11.5oz/341ml</rdfs:label>
 <skos:definition xml:lang="en">A one time use 11.5oz/341ml metal container meant to hold a liquid, commonly referred to as Can 211-202 (Height 413).</skos:definition>
 <skos:definition xml:lang="fr">Un contenant non-réutilisable métallique de 11.5oz/341ml pour contenir un liquide, souvent appeler Can 211-202 (Hauteur 413).</skos:definition>
 <!-- Net Content -->
 <gs1:netContent>
  <gs1:QuantitativeValue rdf:about="#can341ml-Content">
    <rdf:type rdf:resource="http://qudt.org/1.1/schema/qudt#QuantityValue"/>
    <qudt:unit rdf:resource="http://www.qudt.org/2.1/vocab/unit/MilliL"/>
    <qudt:numericalValue rdf:datatype="http://www.w3.org/2001/XMLSchema#double">341</qudt:numericalValue>
    <rdf:value rdf:datatype="http://www.w3.org/2001/XMLSchema#double">341</rdf:value>
    <gs1:unitCode>MLT</gs1:unitCode>
    <gs1:value>341</gs1:value>
  </gs1:QuantitativeValue>
 </gs1:netContent> 
 <sosa:isFeatureOfInterestOf>
  <rdf:Description rdf:about="#can341ml-ContentSosa">
   <rdf:type rdf:resource="http://www.w3.org/ns/sosa/Observation"/>
   <sosa:hasFeatureOfInterest rdf:resource="#can341ml"/>
   <sosa:observedProperty  rdf:resource="#netcontent"/>
   <sosa:hasResult rdf:resource="#can341ml-Content"/>
   <sosa:hasSimpleResult rdf:datatype="http://www.qudt.org/2.1/vocab/unit/MilliM">341</sosa:hasSimpleResult>
  </rdf:Description>
 </sosa:isFeatureOfInterestOf>
 <!-- Height -->
 <gs1:inPackageHeight>
  <gs1:QuantitativeValue rdf:about="#can341ml-Height">
   <rdf:type rdf:resource="http://qudt.org/1.1/schema/qudt#QuantityValue"/>
   <qudt:unit rdf:resource="http://www.qudt.org/2.1/vocab/unit/MilliM"/>
   <qudt:numericalValue rdf:datatype="http://www.w3.org/2001/XMLSchema#double">122.4</qudt:numericalValue>
   <rdf:value rdf:datatype="http://www.w3.org/2001/XMLSchema#double">122.4</rdf:value>
   <gs1:unitCode>MMT</gs1:unitCode>
   <gs1:value>122.4</gs1:value>
  </gs1:QuantitativeValue>
 </gs1:inPackageHeight>  
 <sosa:isFeatureOfInterestOf>
  <rdf:Description rdf:about="#can341ml-HeightSosa">
   <rdf:type rdf:resource="http://www.w3.org/ns/sosa/Observation"/>
   <sosa:hasFeatureOfInterest rdf:resource="#can341ml"/>
   <sosa:observedProperty  rdf:resource="#height"/>
   <sosa:hasResult rdf:resource="#can341ml-Height"/>
   <sosa:hasSimpleResult rdf:datatype="http://www.qudt.org/2.1/vocab/unit/MilliM">122.4</sosa:hasSimpleResult>
  </rdf:Description>
 </sosa:isFeatureOfInterestOf>
 <!-- Diameter --> 
 <gs1:inPackageDiameter>
  <gs1:QuantitativeValue rdf:about="#can341ml-Diameter">
   <rdf:type rdf:resource="http://qudt.org/1.1/schema/qudt#QuantityValue"/>
   <qudt:unit rdf:resource="http://www.qudt.org/2.1/vocab/unit/MilliM"/>
   <qudt:numericalValue rdf:datatype="http://www.w3.org/2001/XMLSchema#double">66</qudt:numericalValue>
   <rdf:value rdf:datatype="http://www.w3.org/2001/XMLSchema#double">66</rdf:value>
   <gs1:unitCode>MMT</gs1:unitCode>
   <gs1:value>66</gs1:value>
  </gs1:QuantitativeValue>
 </gs1:inPackageDiameter>
 <sosa:isFeatureOfInterestOf>
  <rdf:Description rdf:about="#can341ml-DiameterSosa">
   <rdf:type rdf:resource="http://www.w3.org/ns/sosa/Observation"/>
   <sosa:hasFeatureOfInterest rdf:resource="#can341ml"/>
   <sosa:observedProperty  rdf:resource="#diameter"/>
   <sosa:hasResult rdf:resource="#can341ml-Diameter"/>
   <sosa:hasSimpleResult rdf:datatype="http://www.qudt.org/2.1/vocab/unit/MilliM">66</sosa:hasSimpleResult>
  </rdf:Description>
 </sosa:isFeatureOfInterestOf>
 <sosa:isFeatureOfInterestOf>
  <rdf:Description rdf:about="#can341ml-EndDiameterSosa">
   <rdf:type rdf:resource="http://www.w3.org/ns/sosa/Observation"/>
   <sosa:hasFeatureOfInterest rdf:resource="#can341ml"/>
   <sosa:observedProperty  rdf:resource="#endDiameter"/>
   <sosa:hasResult>
    <gs1:QuantitativeValue rdf:about="#can341ml-EndDiameter">
     <rdf:type rdf:resource="http://qudt.org/1.1/schema/qudt#QuantityValue"/>
     <qudt:unit rdf:resource="http://www.qudt.org/2.1/vocab/unit/MilliM"/>
     <qudt:numericalValue rdf:datatype="http://www.w3.org/2001/XMLSchema#double">53.55</qudt:numericalValue>
     <rdf:value rdf:datatype="http://www.w3.org/2001/XMLSchema#double">53.55</rdf:value>
     <gs1:unitCode>MMT</gs1:unitCode>
     <gs1:value>53.55</gs1:value>
    </gs1:QuantitativeValue>
   </sosa:hasResult>
   <sosa:hasSimpleResult rdf:datatype="http://www.qudt.org/2.1/vocab/unit/MilliM">53.55</sosa:hasSimpleResult>
  </rdf:Description>
 </sosa:isFeatureOfInterestOf>
 <rdfs:isDefinedBy rdf:resource="https://rdf.ag/o/beer-ONTOLOGY_DATE"/>
 <void:inDataset rdf:resource="#datasetdefinition"/>
</rdf:Description>


<rdf:Description rdf:about="#can568ml">
 <rdf:type rdf:resource="https://gs1.org/voc/PackagingDetails"/>
 <rdf:type rdf:resource="#LiquidContainer"/>
 <rdf:type rdf:resource="#BeverageCan"/>
 <rdfs:label xml:lang="en">19.2oz/568ml Metal Beverage Can</rdfs:label>
 <rdfs:label xml:lang="fr">Canette à Boisson Métallique, 19.2oz/568ml</rdfs:label>
 <skos:definition xml:lang="en">A one time use 19.2oz/568ml metal container meant to hold a liquid, commonly referred to as Standard 211-202 (Height 707).</skos:definition>
 <skos:definition xml:lang="fr">Un contenant non-réutilisable métallique de 19.2oz/568ml pour contenir un liquide, souvent appeler Standard 211-202 (Hauteur 707).</skos:definition>
 <!-- Net Content -->
 <gs1:netContent>
  <gs1:QuantitativeValue rdf:about="#can568ml-Content">
    <rdf:type rdf:resource="http://qudt.org/1.1/schema/qudt#QuantityValue"/>
    <qudt:unit rdf:resource="http://www.qudt.org/2.1/vocab/unit/MilliL"/>
    <qudt:numericalValue rdf:datatype="http://www.w3.org/2001/XMLSchema#double">568</qudt:numericalValue>
    <rdf:value rdf:datatype="http://www.w3.org/2001/XMLSchema#double">568</rdf:value>
    <gs1:unitCode>MLT</gs1:unitCode>
    <gs1:value>568</gs1:value>
  </gs1:QuantitativeValue>
 </gs1:netContent> 
 <sosa:isFeatureOfInterestOf>
  <rdf:Description rdf:about="#can568ml-ContentSosa">
   <rdf:type rdf:resource="http://www.w3.org/ns/sosa/Observation"/>
   <sosa:hasFeatureOfInterest rdf:resource="#can568ml"/>
   <sosa:observedProperty  rdf:resource="#netcontent"/>
   <sosa:hasResult rdf:resource="#can568ml-Content"/>
   <sosa:hasSimpleResult rdf:datatype="http://www.qudt.org/2.1/vocab/unit/MilliM">568</sosa:hasSimpleResult>
  </rdf:Description>
 </sosa:isFeatureOfInterestOf>
 <!-- Height -->
 <gs1:inPackageHeight>
  <gs1:QuantitativeValue rdf:about="#can568ml-Height">
   <rdf:type rdf:resource="http://qudt.org/1.1/schema/qudt#QuantityValue"/>
   <qudt:unit rdf:resource="http://www.qudt.org/2.1/vocab/unit/MilliM"/>
   <qudt:numericalValue rdf:datatype="http://www.w3.org/2001/XMLSchema#double">19.2</qudt:numericalValue>
   <rdf:value rdf:datatype="http://www.w3.org/2001/XMLSchema#double">19.2</rdf:value>
   <gs1:unitCode>MMT</gs1:unitCode>
   <gs1:value>19.2</gs1:value>
  </gs1:QuantitativeValue>
 </gs1:inPackageHeight>  
 <sosa:isFeatureOfInterestOf>
  <rdf:Description rdf:about="#can568ml-HeightSosa">
   <rdf:type rdf:resource="http://www.w3.org/ns/sosa/Observation"/>
   <sosa:hasFeatureOfInterest rdf:resource="#can568ml"/>
   <sosa:observedProperty  rdf:resource="#height"/>
   <sosa:hasResult rdf:resource="#can568ml-Height"/>
   <sosa:hasSimpleResult rdf:datatype="http://www.qudt.org/2.1/vocab/unit/MilliM">19.2</sosa:hasSimpleResult>
  </rdf:Description>
 </sosa:isFeatureOfInterestOf>
 <!-- Diameter --> 
 <gs1:inPackageDiameter>
  <gs1:QuantitativeValue rdf:about="#can568ml-Diameter">
   <rdf:type rdf:resource="http://qudt.org/1.1/schema/qudt#QuantityValue"/>
   <qudt:unit rdf:resource="http://www.qudt.org/2.1/vocab/unit/MilliM"/>
   <qudt:numericalValue rdf:datatype="http://www.w3.org/2001/XMLSchema#double">66</qudt:numericalValue>
   <rdf:value rdf:datatype="http://www.w3.org/2001/XMLSchema#double">66</rdf:value>
   <gs1:unitCode>MMT</gs1:unitCode>
   <gs1:value>66</gs1:value>
  </gs1:QuantitativeValue>
 </gs1:inPackageDiameter>
 <sosa:isFeatureOfInterestOf>
  <rdf:Description rdf:about="#can568ml-DiameterSosa">
   <rdf:type rdf:resource="http://www.w3.org/ns/sosa/Observation"/>
   <sosa:hasFeatureOfInterest rdf:resource="#can568ml"/>
   <sosa:observedProperty  rdf:resource="#diameter"/>
   <sosa:hasResult rdf:resource="#can568ml-Diameter"/>
   <sosa:hasSimpleResult rdf:datatype="http://www.qudt.org/2.1/vocab/unit/MilliM">66</sosa:hasSimpleResult>
  </rdf:Description>
 </sosa:isFeatureOfInterestOf>
 <sosa:isFeatureOfInterestOf>
  <rdf:Description rdf:about="#can568ml-EndDiameterSosa">
   <rdf:type rdf:resource="http://www.w3.org/ns/sosa/Observation"/>
   <sosa:hasFeatureOfInterest rdf:resource="#can568ml"/>
   <sosa:observedProperty  rdf:resource="#endDiameter"/>
   <sosa:hasResult>
    <gs1:QuantitativeValue rdf:about="#can568ml-EndDiameter">
     <rdf:type rdf:resource="http://qudt.org/1.1/schema/qudt#QuantityValue"/>
     <qudt:unit rdf:resource="http://www.qudt.org/2.1/vocab/unit/MilliM"/>
     <qudt:numericalValue rdf:datatype="http://www.w3.org/2001/XMLSchema#double">53.55</qudt:numericalValue>
     <rdf:value rdf:datatype="http://www.w3.org/2001/XMLSchema#double">53.55</rdf:value>
     <gs1:unitCode>MMT</gs1:unitCode>
     <gs1:value>53.55</gs1:value>
    </gs1:QuantitativeValue>
   </sosa:hasResult>
   <sosa:hasSimpleResult rdf:datatype="http://www.qudt.org/2.1/vocab/unit/MilliM">53.55</sosa:hasSimpleResult>
  </rdf:Description>
 </sosa:isFeatureOfInterestOf>
 <rdfs:isDefinedBy rdf:resource="https://rdf.ag/o/beer-ONTOLOGY_DATE"/>
 <void:inDataset rdf:resource="#datasetdefinition"/>
</rdf:Description>


<rdf:Description rdf:about="#can375ml">
 <rdf:type rdf:resource="https://gs1.org/voc/PackagingDetails"/>
 <rdf:type rdf:resource="#LiquidContainer"/>
 <rdf:type rdf:resource="#BeverageCan"/>
 <rdfs:label xml:lang="en">12.7oz/375ml Metal Beverage Can</rdfs:label>
 <rdfs:label xml:lang="fr">Canette à Boisson Métallique, 12.7oz/375ml</rdfs:label>
 <skos:definition xml:lang="en">A one time use 12.7oz/375ml metal container meant to hold a liquid, commonly referred to as Standard 211-202 (Height 502).</skos:definition>
 <skos:definition xml:lang="fr">Un contenant non-réutilisable métallique de 12.7oz/375ml pour contenir un liquide, souvent appeler Standard 211-202 (Hauteur 502).</skos:definition>
 <!-- Net Content -->
 <gs1:netContent>
  <gs1:QuantitativeValue rdf:about="#can375ml-Content">
    <rdf:type rdf:resource="http://qudt.org/1.1/schema/qudt#QuantityValue"/>
    <qudt:unit rdf:resource="http://www.qudt.org/2.1/vocab/unit/MilliL"/>
    <qudt:numericalValue rdf:datatype="http://www.w3.org/2001/XMLSchema#double">375</qudt:numericalValue>
    <rdf:value rdf:datatype="http://www.w3.org/2001/XMLSchema#double">375</rdf:value>
    <gs1:unitCode>MLT</gs1:unitCode>
    <gs1:value>375</gs1:value>
  </gs1:QuantitativeValue>
 </gs1:netContent> 
 <sosa:isFeatureOfInterestOf>
  <rdf:Description rdf:about="#can375ml-ContentSosa">
   <rdf:type rdf:resource="http://www.w3.org/ns/sosa/Observation"/>
   <sosa:hasFeatureOfInterest rdf:resource="#can375ml"/>
   <sosa:observedProperty  rdf:resource="#netcontent"/>
   <sosa:hasResult rdf:resource="#can375ml-Content"/>
   <sosa:hasSimpleResult rdf:datatype="http://www.qudt.org/2.1/vocab/unit/MilliM">375</sosa:hasSimpleResult>
  </rdf:Description>
 </sosa:isFeatureOfInterestOf>
 <!-- Height -->
 <gs1:inPackageHeight>
  <gs1:QuantitativeValue rdf:about="#can375ml-Height">
   <rdf:type rdf:resource="http://qudt.org/1.1/schema/qudt#QuantityValue"/>
   <qudt:unit rdf:resource="http://www.qudt.org/2.1/vocab/unit/MilliM"/>
   <qudt:numericalValue rdf:datatype="http://www.w3.org/2001/XMLSchema#double">12.7</qudt:numericalValue>
   <rdf:value rdf:datatype="http://www.w3.org/2001/XMLSchema#double">12.7</rdf:value>
   <gs1:unitCode>MMT</gs1:unitCode>
   <gs1:value>12.7</gs1:value>
  </gs1:QuantitativeValue>
 </gs1:inPackageHeight>  
 <sosa:isFeatureOfInterestOf>
  <rdf:Description rdf:about="#can375ml-HeightSosa">
   <rdf:type rdf:resource="http://www.w3.org/ns/sosa/Observation"/>
   <sosa:hasFeatureOfInterest rdf:resource="#can375ml"/>
   <sosa:observedProperty  rdf:resource="#height"/>
   <sosa:hasResult rdf:resource="#can375ml-Height"/>
   <sosa:hasSimpleResult rdf:datatype="http://www.qudt.org/2.1/vocab/unit/MilliM">12.7</sosa:hasSimpleResult>
  </rdf:Description>
 </sosa:isFeatureOfInterestOf>
 <!-- Diameter --> 
 <gs1:inPackageDiameter>
  <gs1:QuantitativeValue rdf:about="#can375ml-Diameter">
   <rdf:type rdf:resource="http://qudt.org/1.1/schema/qudt#QuantityValue"/>
   <qudt:unit rdf:resource="http://www.qudt.org/2.1/vocab/unit/MilliM"/>
   <qudt:numericalValue rdf:datatype="http://www.w3.org/2001/XMLSchema#double">66</qudt:numericalValue>
   <rdf:value rdf:datatype="http://www.w3.org/2001/XMLSchema#double">66</rdf:value>
   <gs1:unitCode>MMT</gs1:unitCode>
   <gs1:value>66</gs1:value>
  </gs1:QuantitativeValue>
 </gs1:inPackageDiameter>
 <sosa:isFeatureOfInterestOf>
  <rdf:Description rdf:about="#can375ml-DiameterSosa">
   <rdf:type rdf:resource="http://www.w3.org/ns/sosa/Observation"/>
   <sosa:hasFeatureOfInterest rdf:resource="#can375ml"/>
   <sosa:observedProperty  rdf:resource="#diameter"/>
   <sosa:hasResult rdf:resource="#can375ml-Diameter"/>
   <sosa:hasSimpleResult rdf:datatype="http://www.qudt.org/2.1/vocab/unit/MilliM">66</sosa:hasSimpleResult>
  </rdf:Description>
 </sosa:isFeatureOfInterestOf>
 <sosa:isFeatureOfInterestOf>
  <rdf:Description rdf:about="#can375ml-EndDiameterSosa">
   <rdf:type rdf:resource="http://www.w3.org/ns/sosa/Observation"/>
   <sosa:hasFeatureOfInterest rdf:resource="#can375ml"/>
   <sosa:observedProperty  rdf:resource="#endDiameter"/>
   <sosa:hasResult>
    <gs1:QuantitativeValue rdf:about="#can375ml-EndDiameter">
     <rdf:type rdf:resource="http://qudt.org/1.1/schema/qudt#QuantityValue"/>
     <qudt:unit rdf:resource="http://www.qudt.org/2.1/vocab/unit/MilliM"/>
     <qudt:numericalValue rdf:datatype="http://www.w3.org/2001/XMLSchema#double">53.55</qudt:numericalValue>
     <rdf:value rdf:datatype="http://www.w3.org/2001/XMLSchema#double">53.55</rdf:value>
     <gs1:unitCode>MMT</gs1:unitCode>
     <gs1:value>53.55</gs1:value>
    </gs1:QuantitativeValue>
   </sosa:hasResult>
   <sosa:hasSimpleResult rdf:datatype="http://www.qudt.org/2.1/vocab/unit/MilliM">53.55</sosa:hasSimpleResult>
  </rdf:Description>
 </sosa:isFeatureOfInterestOf>
 <rdfs:isDefinedBy rdf:resource="https://rdf.ag/o/beer-ONTOLOGY_DATE"/>
 <void:inDataset rdf:resource="#datasetdefinition"/>
</rdf:Description>


<rdf:Description rdf:about="#can440ml">
 <rdf:type rdf:resource="https://gs1.org/voc/PackagingDetails"/>
 <rdf:type rdf:resource="#LiquidContainer"/>
 <rdf:type rdf:resource="#BeverageCan"/>
 <rdfs:label xml:lang="en">14.9oz/440ml Metal Beverage Can</rdfs:label>
 <rdfs:label xml:lang="fr">Canette à Boisson Métallique, 14.9oz/440ml</rdfs:label>
 <skos:definition xml:lang="en">A one time use 14.9oz/440ml metal container meant to hold a liquid, commonly referred to as Standard 211-202 (Height 603).</skos:definition>
 <skos:definition xml:lang="fr">Un contenant non-réutilisable métallique de 14.9oz/440ml pour contenir un liquide, souvent appeler Standard 211-202 (Hauteur 603).</skos:definition>
 <!-- Net Content -->
 <gs1:netContent>
  <gs1:QuantitativeValue rdf:about="#can440ml-Content">
    <rdf:type rdf:resource="http://qudt.org/1.1/schema/qudt#QuantityValue"/>
    <qudt:unit rdf:resource="http://www.qudt.org/2.1/vocab/unit/MilliL"/>
    <qudt:numericalValue rdf:datatype="http://www.w3.org/2001/XMLSchema#double">440</qudt:numericalValue>
    <rdf:value rdf:datatype="http://www.w3.org/2001/XMLSchema#double">440</rdf:value>
    <gs1:unitCode>MLT</gs1:unitCode>
    <gs1:value>440</gs1:value>
  </gs1:QuantitativeValue>
 </gs1:netContent> 
 <sosa:isFeatureOfInterestOf>
  <rdf:Description rdf:about="#can440ml-ContentSosa">
   <rdf:type rdf:resource="http://www.w3.org/ns/sosa/Observation"/>
   <sosa:hasFeatureOfInterest rdf:resource="#can440ml"/>
   <sosa:observedProperty  rdf:resource="#netcontent"/>
   <sosa:hasResult rdf:resource="#can440ml-Content"/>
   <sosa:hasSimpleResult rdf:datatype="http://www.qudt.org/2.1/vocab/unit/MilliM">440</sosa:hasSimpleResult>
  </rdf:Description>
 </sosa:isFeatureOfInterestOf>
 <!-- Height -->
 <gs1:inPackageHeight>
  <gs1:QuantitativeValue rdf:about="#can440ml-Height">
   <rdf:type rdf:resource="http://qudt.org/1.1/schema/qudt#QuantityValue"/>
   <qudt:unit rdf:resource="http://www.qudt.org/2.1/vocab/unit/MilliM"/>
   <qudt:numericalValue rdf:datatype="http://www.w3.org/2001/XMLSchema#double">14.9</qudt:numericalValue>
   <rdf:value rdf:datatype="http://www.w3.org/2001/XMLSchema#double">14.9</rdf:value>
   <gs1:unitCode>MMT</gs1:unitCode>
   <gs1:value>14.9</gs1:value>
  </gs1:QuantitativeValue>
 </gs1:inPackageHeight>  
 <sosa:isFeatureOfInterestOf>
  <rdf:Description rdf:about="#can440ml-HeightSosa">
   <rdf:type rdf:resource="http://www.w3.org/ns/sosa/Observation"/>
   <sosa:hasFeatureOfInterest rdf:resource="#can440ml"/>
   <sosa:observedProperty  rdf:resource="#height"/>
   <sosa:hasResult rdf:resource="#can440ml-Height"/>
   <sosa:hasSimpleResult rdf:datatype="http://www.qudt.org/2.1/vocab/unit/MilliM">14.9</sosa:hasSimpleResult>
  </rdf:Description>
 </sosa:isFeatureOfInterestOf>
 <!-- Diameter --> 
 <gs1:inPackageDiameter>
  <gs1:QuantitativeValue rdf:about="#can440ml-Diameter">
   <rdf:type rdf:resource="http://qudt.org/1.1/schema/qudt#QuantityValue"/>
   <qudt:unit rdf:resource="http://www.qudt.org/2.1/vocab/unit/MilliM"/>
   <qudt:numericalValue rdf:datatype="http://www.w3.org/2001/XMLSchema#double">66</qudt:numericalValue>
   <rdf:value rdf:datatype="http://www.w3.org/2001/XMLSchema#double">66</rdf:value>
   <gs1:unitCode>MMT</gs1:unitCode>
   <gs1:value>66</gs1:value>
  </gs1:QuantitativeValue>
 </gs1:inPackageDiameter>
 <sosa:isFeatureOfInterestOf>
  <rdf:Description rdf:about="#can440ml-DiameterSosa">
   <rdf:type rdf:resource="http://www.w3.org/ns/sosa/Observation"/>
   <sosa:hasFeatureOfInterest rdf:resource="#can440ml"/>
   <sosa:observedProperty  rdf:resource="#diameter"/>
   <sosa:hasResult rdf:resource="#can440ml-Diameter"/>
   <sosa:hasSimpleResult rdf:datatype="http://www.qudt.org/2.1/vocab/unit/MilliM">66</sosa:hasSimpleResult>
  </rdf:Description>
 </sosa:isFeatureOfInterestOf>
 <sosa:isFeatureOfInterestOf>
  <rdf:Description rdf:about="#can440ml-EndDiameterSosa">
   <rdf:type rdf:resource="http://www.w3.org/ns/sosa/Observation"/>
   <sosa:hasFeatureOfInterest rdf:resource="#can440ml"/>
   <sosa:observedProperty  rdf:resource="#endDiameter"/>
   <sosa:hasResult>
    <gs1:QuantitativeValue rdf:about="#can440ml-EndDiameter">
     <rdf:type rdf:resource="http://qudt.org/1.1/schema/qudt#QuantityValue"/>
     <qudt:unit rdf:resource="http://www.qudt.org/2.1/vocab/unit/MilliM"/>
     <qudt:numericalValue rdf:datatype="http://www.w3.org/2001/XMLSchema#double">53.55</qudt:numericalValue>
     <rdf:value rdf:datatype="http://www.w3.org/2001/XMLSchema#double">53.55</rdf:value>
     <gs1:unitCode>MMT</gs1:unitCode>
     <gs1:value>53.55</gs1:value>
    </gs1:QuantitativeValue>
   </sosa:hasResult>
   <sosa:hasSimpleResult rdf:datatype="http://www.qudt.org/2.1/vocab/unit/MilliM">53.55</sosa:hasSimpleResult>
  </rdf:Description>
 </sosa:isFeatureOfInterestOf>
 <rdfs:isDefinedBy rdf:resource="https://rdf.ag/o/beer-ONTOLOGY_DATE"/>
 <void:inDataset rdf:resource="#datasetdefinition"/>
</rdf:Description>


<rdf:Description rdf:about="#can473ml">
 <rdf:type rdf:resource="https://gs1.org/voc/PackagingDetails"/>
 <rdf:type rdf:resource="#LiquidContainer"/>
 <rdf:type rdf:resource="#BeverageCan"/>
 <rdfs:label xml:lang="en">16oz/473ml Metal Beverage Can</rdfs:label>
 <rdfs:label xml:lang="fr">Canette à Boisson Métallique, 16oz/473ml</rdfs:label>
 <skos:definition xml:lang="en">A one time use 16oz/473ml metal container meant to hold a liquid, commonly referred to as Standard 211-202 (Height 603).</skos:definition>
 <skos:definition xml:lang="fr">Un contenant non-réutilisable métallique de 16oz/473ml pour contenir un liquide, souvent appeler Standard 211-202 (Hauteur 603).</skos:definition>
 <!-- Net Content -->
 <gs1:netContent>
  <gs1:QuantitativeValue rdf:about="#can473ml-Content">
    <rdf:type rdf:resource="http://qudt.org/1.1/schema/qudt#QuantityValue"/>
    <qudt:unit rdf:resource="http://www.qudt.org/2.1/vocab/unit/MilliL"/>
    <qudt:numericalValue rdf:datatype="http://www.w3.org/2001/XMLSchema#double">473</qudt:numericalValue>
    <rdf:value rdf:datatype="http://www.w3.org/2001/XMLSchema#double">473</rdf:value>
    <gs1:unitCode>MLT</gs1:unitCode>
    <gs1:value>473</gs1:value>
  </gs1:QuantitativeValue>
 </gs1:netContent> 
 <sosa:isFeatureOfInterestOf>
  <rdf:Description rdf:about="#can473ml-ContentSosa">
   <rdf:type rdf:resource="http://www.w3.org/ns/sosa/Observation"/>
   <sosa:hasFeatureOfInterest rdf:resource="#can473ml"/>
   <sosa:observedProperty  rdf:resource="#netcontent"/>
   <sosa:hasResult rdf:resource="#can473ml-Content"/>
   <sosa:hasSimpleResult rdf:datatype="http://www.qudt.org/2.1/vocab/unit/MilliM">473</sosa:hasSimpleResult>
  </rdf:Description>
 </sosa:isFeatureOfInterestOf>
 <!-- Height -->
 <gs1:inPackageHeight>
  <gs1:QuantitativeValue rdf:about="#can473ml-Height">
   <rdf:type rdf:resource="http://qudt.org/1.1/schema/qudt#QuantityValue"/>
   <qudt:unit rdf:resource="http://www.qudt.org/2.1/vocab/unit/MilliM"/>
   <qudt:numericalValue rdf:datatype="http://www.w3.org/2001/XMLSchema#double">16</qudt:numericalValue>
   <rdf:value rdf:datatype="http://www.w3.org/2001/XMLSchema#double">16</rdf:value>
   <gs1:unitCode>MMT</gs1:unitCode>
   <gs1:value>16</gs1:value>
  </gs1:QuantitativeValue>
 </gs1:inPackageHeight>  
 <sosa:isFeatureOfInterestOf>
  <rdf:Description rdf:about="#can473ml-HeightSosa">
   <rdf:type rdf:resource="http://www.w3.org/ns/sosa/Observation"/>
   <sosa:hasFeatureOfInterest rdf:resource="#can473ml"/>
   <sosa:observedProperty  rdf:resource="#height"/>
   <sosa:hasResult rdf:resource="#can473ml-Height"/>
   <sosa:hasSimpleResult rdf:datatype="http://www.qudt.org/2.1/vocab/unit/MilliM">16</sosa:hasSimpleResult>
  </rdf:Description>
 </sosa:isFeatureOfInterestOf>
 <!-- Diameter --> 
 <gs1:inPackageDiameter>
  <gs1:QuantitativeValue rdf:about="#can473ml-Diameter">
   <rdf:type rdf:resource="http://qudt.org/1.1/schema/qudt#QuantityValue"/>
   <qudt:unit rdf:resource="http://www.qudt.org/2.1/vocab/unit/MilliM"/>
   <qudt:numericalValue rdf:datatype="http://www.w3.org/2001/XMLSchema#double">66</qudt:numericalValue>
   <rdf:value rdf:datatype="http://www.w3.org/2001/XMLSchema#double">66</rdf:value>
   <gs1:unitCode>MMT</gs1:unitCode>
   <gs1:value>66</gs1:value>
  </gs1:QuantitativeValue>
 </gs1:inPackageDiameter>
 <sosa:isFeatureOfInterestOf>
  <rdf:Description rdf:about="#can473ml-DiameterSosa">
   <rdf:type rdf:resource="http://www.w3.org/ns/sosa/Observation"/>
   <sosa:hasFeatureOfInterest rdf:resource="#can473ml"/>
   <sosa:observedProperty  rdf:resource="#diameter"/>
   <sosa:hasResult rdf:resource="#can473ml-Diameter"/>
   <sosa:hasSimpleResult rdf:datatype="http://www.qudt.org/2.1/vocab/unit/MilliM">66</sosa:hasSimpleResult>
  </rdf:Description>
 </sosa:isFeatureOfInterestOf>
 <sosa:isFeatureOfInterestOf>
  <rdf:Description rdf:about="#can473ml-EndDiameterSosa">
   <rdf:type rdf:resource="http://www.w3.org/ns/sosa/Observation"/>
   <sosa:hasFeatureOfInterest rdf:resource="#can473ml"/>
   <sosa:observedProperty  rdf:resource="#endDiameter"/>
   <sosa:hasResult>
    <gs1:QuantitativeValue rdf:about="#can473ml-EndDiameter">
     <rdf:type rdf:resource="http://qudt.org/1.1/schema/qudt#QuantityValue"/>
     <qudt:unit rdf:resource="http://www.qudt.org/2.1/vocab/unit/MilliM"/>
     <qudt:numericalValue rdf:datatype="http://www.w3.org/2001/XMLSchema#double">53.55</qudt:numericalValue>
     <rdf:value rdf:datatype="http://www.w3.org/2001/XMLSchema#double">53.55</rdf:value>
     <gs1:unitCode>MMT</gs1:unitCode>
     <gs1:value>53.55</gs1:value>
    </gs1:QuantitativeValue>
   </sosa:hasResult>
   <sosa:hasSimpleResult rdf:datatype="http://www.qudt.org/2.1/vocab/unit/MilliM">53.55</sosa:hasSimpleResult>
  </rdf:Description>
 </sosa:isFeatureOfInterestOf>
 <rdfs:isDefinedBy rdf:resource="https://rdf.ag/o/beer-ONTOLOGY_DATE"/>
 <void:inDataset rdf:resource="#datasetdefinition"/>
</rdf:Description>


<rdf:Description rdf:about="#can650ml">
 <rdf:type rdf:resource="https://gs1.org/voc/PackagingDetails"/>
 <rdf:type rdf:resource="#LiquidContainer"/>
 <rdf:type rdf:resource="#BeverageCan"/>
 <rdfs:label xml:lang="en">22oz/650ml Metal Beverage Can</rdfs:label>
 <rdfs:label xml:lang="fr">Canette à Boisson Métallique, 22oz/650ml</rdfs:label>
 <skos:definition xml:lang="en">A one time use 22oz/650ml metal container meant to hold a liquid, commonly referred to as Bomber 211.2 (Height 703).</skos:definition>
 <skos:definition xml:lang="fr">Un contenant non-réutilisable métallique de 22oz/650ml pour contenir un liquide, souvent appeler Bomber 211.2 (Hauteur 703).</skos:definition>
 <!-- Net Content -->
 <gs1:netContent>
  <gs1:QuantitativeValue rdf:about="#can650ml-Content">
    <rdf:type rdf:resource="http://qudt.org/1.1/schema/qudt#QuantityValue"/>
    <qudt:unit rdf:resource="http://www.qudt.org/2.1/vocab/unit/MilliL"/>
    <qudt:numericalValue rdf:datatype="http://www.w3.org/2001/XMLSchema#double">650</qudt:numericalValue>
    <rdf:value rdf:datatype="http://www.w3.org/2001/XMLSchema#double">650</rdf:value>
    <gs1:unitCode>MLT</gs1:unitCode>
    <gs1:value>650</gs1:value>
  </gs1:QuantitativeValue>
 </gs1:netContent> 
 <sosa:isFeatureOfInterestOf>
  <rdf:Description rdf:about="#can650ml-ContentSosa">
   <rdf:type rdf:resource="http://www.w3.org/ns/sosa/Observation"/>
   <sosa:hasFeatureOfInterest rdf:resource="#can650ml"/>
   <sosa:observedProperty  rdf:resource="#netcontent"/>
   <sosa:hasResult rdf:resource="#can650ml-Content"/>
   <sosa:hasSimpleResult rdf:datatype="http://www.qudt.org/2.1/vocab/unit/MilliM">650</sosa:hasSimpleResult>
  </rdf:Description>
 </sosa:isFeatureOfInterestOf>
 <!-- Height -->
 <gs1:inPackageHeight>
  <gs1:QuantitativeValue rdf:about="#can650ml-Height">
   <rdf:type rdf:resource="http://qudt.org/1.1/schema/qudt#QuantityValue"/>
   <qudt:unit rdf:resource="http://www.qudt.org/2.1/vocab/unit/MilliM"/>
   <qudt:numericalValue rdf:datatype="http://www.w3.org/2001/XMLSchema#double">181.1</qudt:numericalValue>
   <rdf:value rdf:datatype="http://www.w3.org/2001/XMLSchema#double">181.1</rdf:value>
   <gs1:unitCode>MMT</gs1:unitCode>
   <gs1:value>181.1</gs1:value>
  </gs1:QuantitativeValue>
 </gs1:inPackageHeight>  
 <sosa:isFeatureOfInterestOf>
  <rdf:Description rdf:about="#can650ml-HeightSosa">
   <rdf:type rdf:resource="http://www.w3.org/ns/sosa/Observation"/>
   <sosa:hasFeatureOfInterest rdf:resource="#can650ml"/>
   <sosa:observedProperty  rdf:resource="#height"/>
   <sosa:hasResult rdf:resource="#can650ml-Height"/>
   <sosa:hasSimpleResult rdf:datatype="http://www.qudt.org/2.1/vocab/unit/MilliM">181.1</sosa:hasSimpleResult>
  </rdf:Description>
 </sosa:isFeatureOfInterestOf>
 <!-- Diameter --> 
 <gs1:inPackageDiameter>
  <gs1:QuantitativeValue rdf:about="#can650ml-Diameter">
   <rdf:type rdf:resource="http://qudt.org/1.1/schema/qudt#QuantityValue"/>
   <qudt:unit rdf:resource="http://www.qudt.org/2.1/vocab/unit/MilliM"/>
   <qudt:numericalValue rdf:datatype="http://www.w3.org/2001/XMLSchema#double">66</qudt:numericalValue>
   <rdf:value rdf:datatype="http://www.w3.org/2001/XMLSchema#double">66</rdf:value>
   <gs1:unitCode>MMT</gs1:unitCode>
   <gs1:value>66</gs1:value>
  </gs1:QuantitativeValue>
 </gs1:inPackageDiameter>
 <sosa:isFeatureOfInterestOf>
  <rdf:Description rdf:about="#can650ml-DiameterSosa">
   <rdf:type rdf:resource="http://www.w3.org/ns/sosa/Observation"/>
   <sosa:hasFeatureOfInterest rdf:resource="#can650ml"/>
   <sosa:observedProperty  rdf:resource="#diameter"/>
   <sosa:hasResult rdf:resource="#can650ml-Diameter"/>
   <sosa:hasSimpleResult rdf:datatype="http://www.qudt.org/2.1/vocab/unit/MilliM">66</sosa:hasSimpleResult>
  </rdf:Description>
 </sosa:isFeatureOfInterestOf>
 <rdfs:isDefinedBy rdf:resource="https://rdf.ag/o/beer-ONTOLOGY_DATE"/>
 <void:inDataset rdf:resource="#datasetdefinition"/>
</rdf:Description>


<rdf:Description rdf:about="#can710ml">
 <rdf:type rdf:resource="https://gs1.org/voc/PackagingDetails"/>
 <rdf:type rdf:resource="#LiquidContainer"/>
 <rdf:type rdf:resource="#BeverageCan"/>
 <rdfs:label xml:lang="en">24oz/710ml Metal Beverage Can</rdfs:label>
 <rdfs:label xml:lang="fr">Canette à Boisson Métallique, 24oz/710ml</rdfs:label>
 <skos:definition xml:lang="en">A one time use 24oz/710ml metal container meant to hold a liquid, commonly referred to as Tall #2, 307 (Height 509).</skos:definition>
 <skos:definition xml:lang="fr">Un contenant non-réutilisable métallique de 24oz/710ml pour contenir un liquide, souvent appeler Tall #2, 307 (Hauteur 509).</skos:definition>
 <!-- Net Content -->
 <gs1:netContent>
  <gs1:QuantitativeValue rdf:about="#can710ml-Content">
    <rdf:type rdf:resource="http://qudt.org/1.1/schema/qudt#QuantityValue"/>
    <qudt:unit rdf:resource="http://www.qudt.org/2.1/vocab/unit/MilliL"/>
    <qudt:numericalValue rdf:datatype="http://www.w3.org/2001/XMLSchema#double">710</qudt:numericalValue>
    <rdf:value rdf:datatype="http://www.w3.org/2001/XMLSchema#double">710</rdf:value>
    <gs1:unitCode>MLT</gs1:unitCode>
    <gs1:value>710</gs1:value>
  </gs1:QuantitativeValue>
 </gs1:netContent> 
 <sosa:isFeatureOfInterestOf>
  <rdf:Description rdf:about="#can710ml-ContentSosa">
   <rdf:type rdf:resource="http://www.w3.org/ns/sosa/Observation"/>
   <sosa:hasFeatureOfInterest rdf:resource="#can710ml"/>
   <sosa:observedProperty  rdf:resource="#netcontent"/>
   <sosa:hasResult rdf:resource="#can710ml-Content"/>
   <sosa:hasSimpleResult rdf:datatype="http://www.qudt.org/2.1/vocab/unit/MilliM">710</sosa:hasSimpleResult>
  </rdf:Description>
 </sosa:isFeatureOfInterestOf>
 <!-- Height -->
 <gs1:inPackageHeight>
  <gs1:QuantitativeValue rdf:about="#can710ml-Height">
   <rdf:type rdf:resource="http://qudt.org/1.1/schema/qudt#QuantityValue"/>
   <qudt:unit rdf:resource="http://www.qudt.org/2.1/vocab/unit/MilliM"/>
   <qudt:numericalValue rdf:datatype="http://www.w3.org/2001/XMLSchema#double">140.2</qudt:numericalValue>
   <rdf:value rdf:datatype="http://www.w3.org/2001/XMLSchema#double">140.2</rdf:value>
   <gs1:unitCode>MMT</gs1:unitCode>
   <gs1:value>140.2</gs1:value>
  </gs1:QuantitativeValue>
 </gs1:inPackageHeight>  
 <sosa:isFeatureOfInterestOf>
  <rdf:Description rdf:about="#can710ml-HeightSosa">
   <rdf:type rdf:resource="http://www.w3.org/ns/sosa/Observation"/>
   <sosa:hasFeatureOfInterest rdf:resource="#can710ml"/>
   <sosa:observedProperty  rdf:resource="#height"/>
   <sosa:hasResult rdf:resource="#can710ml-Height"/>
   <sosa:hasSimpleResult rdf:datatype="http://www.qudt.org/2.1/vocab/unit/MilliM">140.2</sosa:hasSimpleResult>
  </rdf:Description>
 </sosa:isFeatureOfInterestOf>
 <!-- Diameter --> 
 <gs1:inPackageDiameter>
  <gs1:QuantitativeValue rdf:about="#can710ml-Diameter">
   <rdf:type rdf:resource="http://qudt.org/1.1/schema/qudt#QuantityValue"/>
   <qudt:unit rdf:resource="http://www.qudt.org/2.1/vocab/unit/MilliM"/>
   <qudt:numericalValue rdf:datatype="http://www.w3.org/2001/XMLSchema#double">86.6</qudt:numericalValue>
   <rdf:value rdf:datatype="http://www.w3.org/2001/XMLSchema#double">86.6</rdf:value>
   <gs1:unitCode>MMT</gs1:unitCode>
   <gs1:value>86.6</gs1:value>
  </gs1:QuantitativeValue>
 </gs1:inPackageDiameter>
 <sosa:isFeatureOfInterestOf>
  <rdf:Description rdf:about="#can710ml-DiameterSosa">
   <rdf:type rdf:resource="http://www.w3.org/ns/sosa/Observation"/>
   <sosa:hasFeatureOfInterest rdf:resource="#can710ml"/>
   <sosa:observedProperty  rdf:resource="#diameter"/>
   <sosa:hasResult rdf:resource="#can710ml-Diameter"/>
   <sosa:hasSimpleResult rdf:datatype="http://www.qudt.org/2.1/vocab/unit/MilliM">86.6</sosa:hasSimpleResult>
  </rdf:Description>
 </sosa:isFeatureOfInterestOf>
 <rdfs:isDefinedBy rdf:resource="https://rdf.ag/o/beer-ONTOLOGY_DATE"/>
 <void:inDataset rdf:resource="#datasetdefinition"/>
</rdf:Description>


<rdf:Description rdf:about="#can740ml">
 <rdf:type rdf:resource="https://gs1.org/voc/PackagingDetails"/>
 <rdf:type rdf:resource="#LiquidContainer"/>
 <rdf:type rdf:resource="#BeverageCan"/>
 <rdfs:label xml:lang="en">25oz/740ml Metal Beverage Can</rdfs:label>
 <rdfs:label xml:lang="fr">Canette à Boisson Métallique, 25oz/740ml</rdfs:label>
 <skos:definition xml:lang="en">A one time use 25oz/740ml metal container meant to hold a liquid, commonly referred to as Unknown Can 210.4 (Height 711).</skos:definition>
 <skos:definition xml:lang="fr">Un contenant non-réutilisable métallique de 25oz/740ml pour contenir un liquide, souvent appeler Unknown Can 210.4 (Hauteur 711).</skos:definition>
 <!-- Net Content -->
 <gs1:netContent>
  <gs1:QuantitativeValue rdf:about="#can740ml-Content">
    <rdf:type rdf:resource="http://qudt.org/1.1/schema/qudt#QuantityValue"/>
    <qudt:unit rdf:resource="http://www.qudt.org/2.1/vocab/unit/MilliL"/>
    <qudt:numericalValue rdf:datatype="http://www.w3.org/2001/XMLSchema#double">740</qudt:numericalValue>
    <rdf:value rdf:datatype="http://www.w3.org/2001/XMLSchema#double">740</rdf:value>
    <gs1:unitCode>MLT</gs1:unitCode>
    <gs1:value>740</gs1:value>
  </gs1:QuantitativeValue>
 </gs1:netContent> 
 <sosa:isFeatureOfInterestOf>
  <rdf:Description rdf:about="#can740ml-ContentSosa">
   <rdf:type rdf:resource="http://www.w3.org/ns/sosa/Observation"/>
   <sosa:hasFeatureOfInterest rdf:resource="#can740ml"/>
   <sosa:observedProperty  rdf:resource="#netcontent"/>
   <sosa:hasResult rdf:resource="#can740ml-Content"/>
   <sosa:hasSimpleResult rdf:datatype="http://www.qudt.org/2.1/vocab/unit/MilliM">740</sosa:hasSimpleResult>
  </rdf:Description>
 </sosa:isFeatureOfInterestOf>
 <!-- Height -->
 <gs1:inPackageHeight>
  <gs1:QuantitativeValue rdf:about="#can740ml-Height">
   <rdf:type rdf:resource="http://qudt.org/1.1/schema/qudt#QuantityValue"/>
   <qudt:unit rdf:resource="http://www.qudt.org/2.1/vocab/unit/MilliM"/>
   <qudt:numericalValue rdf:datatype="http://www.w3.org/2001/XMLSchema#double">193.7</qudt:numericalValue>
   <rdf:value rdf:datatype="http://www.w3.org/2001/XMLSchema#double">193.7</rdf:value>
   <gs1:unitCode>MMT</gs1:unitCode>
   <gs1:value>193.7</gs1:value>
  </gs1:QuantitativeValue>
 </gs1:inPackageHeight>  
 <sosa:isFeatureOfInterestOf>
  <rdf:Description rdf:about="#can740ml-HeightSosa">
   <rdf:type rdf:resource="http://www.w3.org/ns/sosa/Observation"/>
   <sosa:hasFeatureOfInterest rdf:resource="#can740ml"/>
   <sosa:observedProperty  rdf:resource="#height"/>
   <sosa:hasResult rdf:resource="#can740ml-Height"/>
   <sosa:hasSimpleResult rdf:datatype="http://www.qudt.org/2.1/vocab/unit/MilliM">193.7</sosa:hasSimpleResult>
  </rdf:Description>
 </sosa:isFeatureOfInterestOf>
 <!-- Diameter --> 
 <gs1:inPackageDiameter>
  <gs1:QuantitativeValue rdf:about="#can740ml-Diameter">
   <rdf:type rdf:resource="http://qudt.org/1.1/schema/qudt#QuantityValue"/>
   <qudt:unit rdf:resource="http://www.qudt.org/2.1/vocab/unit/MilliM"/>
   <qudt:numericalValue rdf:datatype="http://www.w3.org/2001/XMLSchema#double">66.7</qudt:numericalValue>
   <rdf:value rdf:datatype="http://www.w3.org/2001/XMLSchema#double">66.7</rdf:value>
   <gs1:unitCode>MMT</gs1:unitCode>
   <gs1:value>66.7</gs1:value>
  </gs1:QuantitativeValue>
 </gs1:inPackageDiameter>
 <sosa:isFeatureOfInterestOf>
  <rdf:Description rdf:about="#can740ml-DiameterSosa">
   <rdf:type rdf:resource="http://www.w3.org/ns/sosa/Observation"/>
   <sosa:hasFeatureOfInterest rdf:resource="#can740ml"/>
   <sosa:observedProperty  rdf:resource="#diameter"/>
   <sosa:hasResult rdf:resource="#can740ml-Diameter"/>
   <sosa:hasSimpleResult rdf:datatype="http://www.qudt.org/2.1/vocab/unit/MilliM">66.7</sosa:hasSimpleResult>
  </rdf:Description>
 </sosa:isFeatureOfInterestOf>
 <rdfs:isDefinedBy rdf:resource="https://rdf.ag/o/beer-ONTOLOGY_DATE"/>
 <void:inDataset rdf:resource="#datasetdefinition"/>
</rdf:Description>


<rdf:Description rdf:about="#can750ml">
 <rdf:type rdf:resource="https://gs1.org/voc/PackagingDetails"/>
 <rdf:type rdf:resource="#LiquidContainer"/>
 <rdf:type rdf:resource="#BeverageCan"/>
 <rdfs:label xml:lang="en">25oz/750ml Metal Beverage Can</rdfs:label>
 <rdfs:label xml:lang="fr">Canette à Boisson Métallique, 25oz/750ml</rdfs:label>
 <skos:definition xml:lang="en">A one time use 25oz/750ml metal container meant to hold a liquid, commonly referred to as Crowler 307-300 (Height 603).</skos:definition>
 <skos:definition xml:lang="fr">Un contenant non-réutilisable métallique de 25oz/750ml pour contenir un liquide, souvent appeler Crowler 307-300 (Hauteur 603).</skos:definition>
 <!-- Net Content -->
 <gs1:netContent>
  <gs1:QuantitativeValue rdf:about="#can750ml-Content">
    <rdf:type rdf:resource="http://qudt.org/1.1/schema/qudt#QuantityValue"/>
    <qudt:unit rdf:resource="http://www.qudt.org/2.1/vocab/unit/MilliL"/>
    <qudt:numericalValue rdf:datatype="http://www.w3.org/2001/XMLSchema#double">750</qudt:numericalValue>
    <rdf:value rdf:datatype="http://www.w3.org/2001/XMLSchema#double">750</rdf:value>
    <gs1:unitCode>MLT</gs1:unitCode>
    <gs1:value>750</gs1:value>
  </gs1:QuantitativeValue>
 </gs1:netContent> 
 <sosa:isFeatureOfInterestOf>
  <rdf:Description rdf:about="#can750ml-ContentSosa">
   <rdf:type rdf:resource="http://www.w3.org/ns/sosa/Observation"/>
   <sosa:hasFeatureOfInterest rdf:resource="#can750ml"/>
   <sosa:observedProperty  rdf:resource="#netcontent"/>
   <sosa:hasResult rdf:resource="#can750ml-Content"/>
   <sosa:hasSimpleResult rdf:datatype="http://www.qudt.org/2.1/vocab/unit/MilliM">750</sosa:hasSimpleResult>
  </rdf:Description>
 </sosa:isFeatureOfInterestOf>
 <!-- Height -->
 <gs1:inPackageHeight>
  <gs1:QuantitativeValue rdf:about="#can750ml-Height">
   <rdf:type rdf:resource="http://qudt.org/1.1/schema/qudt#QuantityValue"/>
   <qudt:unit rdf:resource="http://www.qudt.org/2.1/vocab/unit/MilliM"/>
   <qudt:numericalValue rdf:datatype="http://www.w3.org/2001/XMLSchema#double">157.2</qudt:numericalValue>
   <rdf:value rdf:datatype="http://www.w3.org/2001/XMLSchema#double">157.2</rdf:value>
   <gs1:unitCode>MMT</gs1:unitCode>
   <gs1:value>157.2</gs1:value>
  </gs1:QuantitativeValue>
 </gs1:inPackageHeight>  
 <sosa:isFeatureOfInterestOf>
  <rdf:Description rdf:about="#can750ml-HeightSosa">
   <rdf:type rdf:resource="http://www.w3.org/ns/sosa/Observation"/>
   <sosa:hasFeatureOfInterest rdf:resource="#can750ml"/>
   <sosa:observedProperty  rdf:resource="#height"/>
   <sosa:hasResult rdf:resource="#can750ml-Height"/>
   <sosa:hasSimpleResult rdf:datatype="http://www.qudt.org/2.1/vocab/unit/MilliM">157.2</sosa:hasSimpleResult>
  </rdf:Description>
 </sosa:isFeatureOfInterestOf>
 <!-- Diameter --> 
 <gs1:inPackageDiameter>
  <gs1:QuantitativeValue rdf:about="#can750ml-Diameter">
   <rdf:type rdf:resource="http://qudt.org/1.1/schema/qudt#QuantityValue"/>
   <qudt:unit rdf:resource="http://www.qudt.org/2.1/vocab/unit/MilliM"/>
   <qudt:numericalValue rdf:datatype="http://www.w3.org/2001/XMLSchema#double">83.5</qudt:numericalValue>
   <rdf:value rdf:datatype="http://www.w3.org/2001/XMLSchema#double">83.5</rdf:value>
   <gs1:unitCode>MMT</gs1:unitCode>
   <gs1:value>83.5</gs1:value>
  </gs1:QuantitativeValue>
 </gs1:inPackageDiameter>
 <sosa:isFeatureOfInterestOf>
  <rdf:Description rdf:about="#can750ml-DiameterSosa">
   <rdf:type rdf:resource="http://www.w3.org/ns/sosa/Observation"/>
   <sosa:hasFeatureOfInterest rdf:resource="#can750ml"/>
   <sosa:observedProperty  rdf:resource="#diameter"/>
   <sosa:hasResult rdf:resource="#can750ml-Diameter"/>
   <sosa:hasSimpleResult rdf:datatype="http://www.qudt.org/2.1/vocab/unit/MilliM">83.5</sosa:hasSimpleResult>
  </rdf:Description>
 </sosa:isFeatureOfInterestOf>
 <sosa:isFeatureOfInterestOf>
  <rdf:Description rdf:about="#can750ml-EndDiameterSosa">
   <rdf:type rdf:resource="http://www.w3.org/ns/sosa/Observation"/>
   <sosa:hasFeatureOfInterest rdf:resource="#can750ml"/>
   <sosa:observedProperty  rdf:resource="#endDiameter"/>
   <sosa:hasResult>
    <gs1:QuantitativeValue rdf:about="#can750ml-EndDiameter">
     <rdf:type rdf:resource="http://qudt.org/1.1/schema/qudt#QuantityValue"/>
     <qudt:unit rdf:resource="http://www.qudt.org/2.1/vocab/unit/MilliM"/>
     <qudt:numericalValue rdf:datatype="http://www.w3.org/2001/XMLSchema#double">75.6</qudt:numericalValue>
     <rdf:value rdf:datatype="http://www.w3.org/2001/XMLSchema#double">75.6</rdf:value>
     <gs1:unitCode>MMT</gs1:unitCode>
     <gs1:value>75.6</gs1:value>
    </gs1:QuantitativeValue>
   </sosa:hasResult>
   <sosa:hasSimpleResult rdf:datatype="http://www.qudt.org/2.1/vocab/unit/MilliM">75.6</sosa:hasSimpleResult>
  </rdf:Description>
 </sosa:isFeatureOfInterestOf>
 <rdfs:isDefinedBy rdf:resource="https://rdf.ag/o/beer-ONTOLOGY_DATE"/>
 <void:inDataset rdf:resource="#datasetdefinition"/>
</rdf:Description>


<rdf:Description rdf:about="#can946ml">
 <rdf:type rdf:resource="https://gs1.org/voc/PackagingDetails"/>
 <rdf:type rdf:resource="#LiquidContainer"/>
 <rdf:type rdf:resource="#BeverageCan"/>
 <rdfs:label xml:lang="en">32oz/946ml Metal Beverage Can</rdfs:label>
 <rdfs:label xml:lang="fr">Canette à Boisson Métallique, 32oz/946ml</rdfs:label>
 <skos:definition xml:lang="en">A one time use 32oz/946ml metal container meant to hold a liquid, commonly referred to as Crowler 307-300 (Height 710).</skos:definition>
 <skos:definition xml:lang="fr">Un contenant non-réutilisable métallique de 32oz/946ml pour contenir un liquide, souvent appeler Crowler 307-300 (Hauteur 710).</skos:definition>
 <!-- Net Content -->
 <gs1:netContent>
  <gs1:QuantitativeValue rdf:about="#can946ml-Content">
    <rdf:type rdf:resource="http://qudt.org/1.1/schema/qudt#QuantityValue"/>
    <qudt:unit rdf:resource="http://www.qudt.org/2.1/vocab/unit/MilliL"/>
    <qudt:numericalValue rdf:datatype="http://www.w3.org/2001/XMLSchema#double">946</qudt:numericalValue>
    <rdf:value rdf:datatype="http://www.w3.org/2001/XMLSchema#double">946</rdf:value>
    <gs1:unitCode>MLT</gs1:unitCode>
    <gs1:value>946</gs1:value>
  </gs1:QuantitativeValue>
 </gs1:netContent> 
 <sosa:isFeatureOfInterestOf>
  <rdf:Description rdf:about="#can946ml-ContentSosa">
   <rdf:type rdf:resource="http://www.w3.org/ns/sosa/Observation"/>
   <sosa:hasFeatureOfInterest rdf:resource="#can946ml"/>
   <sosa:observedProperty  rdf:resource="#netcontent"/>
   <sosa:hasResult rdf:resource="#can946ml-Content"/>
   <sosa:hasSimpleResult rdf:datatype="http://www.qudt.org/2.1/vocab/unit/MilliM">946</sosa:hasSimpleResult>
  </rdf:Description>
 </sosa:isFeatureOfInterestOf>
 <!-- Height -->
 <gs1:inPackageHeight>
  <gs1:QuantitativeValue rdf:about="#can946ml-Height">
   <rdf:type rdf:resource="http://qudt.org/1.1/schema/qudt#QuantityValue"/>
   <qudt:unit rdf:resource="http://www.qudt.org/2.1/vocab/unit/MilliM"/>
   <qudt:numericalValue rdf:datatype="http://www.w3.org/2001/XMLSchema#double">193</qudt:numericalValue>
   <rdf:value rdf:datatype="http://www.w3.org/2001/XMLSchema#double">193</rdf:value>
   <gs1:unitCode>MMT</gs1:unitCode>
   <gs1:value>193</gs1:value>
  </gs1:QuantitativeValue>
 </gs1:inPackageHeight>  
 <sosa:isFeatureOfInterestOf>
  <rdf:Description rdf:about="#can946ml-HeightSosa">
   <rdf:type rdf:resource="http://www.w3.org/ns/sosa/Observation"/>
   <sosa:hasFeatureOfInterest rdf:resource="#can946ml"/>
   <sosa:observedProperty  rdf:resource="#height"/>
   <sosa:hasResult rdf:resource="#can946ml-Height"/>
   <sosa:hasSimpleResult rdf:datatype="http://www.qudt.org/2.1/vocab/unit/MilliM">193</sosa:hasSimpleResult>
  </rdf:Description>
 </sosa:isFeatureOfInterestOf>
 <!-- Diameter --> 
 <gs1:inPackageDiameter>
  <gs1:QuantitativeValue rdf:about="#can946ml-Diameter">
   <rdf:type rdf:resource="http://qudt.org/1.1/schema/qudt#QuantityValue"/>
   <qudt:unit rdf:resource="http://www.qudt.org/2.1/vocab/unit/MilliM"/>
   <qudt:numericalValue rdf:datatype="http://www.w3.org/2001/XMLSchema#double">83.5</qudt:numericalValue>
   <rdf:value rdf:datatype="http://www.w3.org/2001/XMLSchema#double">83.5</rdf:value>
   <gs1:unitCode>MMT</gs1:unitCode>
   <gs1:value>83.5</gs1:value>
  </gs1:QuantitativeValue>
 </gs1:inPackageDiameter>
 <sosa:isFeatureOfInterestOf>
  <rdf:Description rdf:about="#can946ml-DiameterSosa">
   <rdf:type rdf:resource="http://www.w3.org/ns/sosa/Observation"/>
   <sosa:hasFeatureOfInterest rdf:resource="#can946ml"/>
   <sosa:observedProperty  rdf:resource="#diameter"/>
   <sosa:hasResult rdf:resource="#can946ml-Diameter"/>
   <sosa:hasSimpleResult rdf:datatype="http://www.qudt.org/2.1/vocab/unit/MilliM">83.5</sosa:hasSimpleResult>
  </rdf:Description>
 </sosa:isFeatureOfInterestOf>
 <sosa:isFeatureOfInterestOf>
  <rdf:Description rdf:about="#can946ml-EndDiameterSosa">
   <rdf:type rdf:resource="http://www.w3.org/ns/sosa/Observation"/>
   <sosa:hasFeatureOfInterest rdf:resource="#can946ml"/>
   <sosa:observedProperty  rdf:resource="#endDiameter"/>
   <sosa:hasResult>
    <gs1:QuantitativeValue rdf:about="#can946ml-EndDiameter">
     <rdf:type rdf:resource="http://qudt.org/1.1/schema/qudt#QuantityValue"/>
     <qudt:unit rdf:resource="http://www.qudt.org/2.1/vocab/unit/MilliM"/>
     <qudt:numericalValue rdf:datatype="http://www.w3.org/2001/XMLSchema#double">75.6</qudt:numericalValue>
     <rdf:value rdf:datatype="http://www.w3.org/2001/XMLSchema#double">75.6</rdf:value>
     <gs1:unitCode>MMT</gs1:unitCode>
     <gs1:value>75.6</gs1:value>
    </gs1:QuantitativeValue>
   </sosa:hasResult>
   <sosa:hasSimpleResult rdf:datatype="http://www.qudt.org/2.1/vocab/unit/MilliM">75.6</sosa:hasSimpleResult>
  </rdf:Description>
 </sosa:isFeatureOfInterestOf>
 <rdfs:isDefinedBy rdf:resource="https://rdf.ag/o/beer-ONTOLOGY_DATE"/>
 <void:inDataset rdf:resource="#datasetdefinition"/>
</rdf:Description>


<rdf:Description rdf:about="#can950ml">
 <rdf:type rdf:resource="https://gs1.org/voc/PackagingDetails"/>
 <rdf:type rdf:resource="#LiquidContainer"/>
 <rdf:type rdf:resource="#BeverageCan"/>
 <rdfs:label xml:lang="en">32oz/950ml Metal Beverage Can</rdfs:label>
 <rdfs:label xml:lang="fr">Canette à Boisson Métallique, 32oz/950ml</rdfs:label>
 <skos:definition xml:lang="en">A one time use 32oz/950ml metal container meant to hold a liquid, commonly referred to as #3 Can 404 (Height 414).</skos:definition>
 <skos:definition xml:lang="fr">Un contenant non-réutilisable métallique de 32oz/950ml pour contenir un liquide, souvent appeler #3 Can 404 (Hauteur 414).</skos:definition>
 <!-- Net Content -->
 <gs1:netContent>
  <gs1:QuantitativeValue rdf:about="#can950ml-Content">
    <rdf:type rdf:resource="http://qudt.org/1.1/schema/qudt#QuantityValue"/>
    <qudt:unit rdf:resource="http://www.qudt.org/2.1/vocab/unit/MilliL"/>
    <qudt:numericalValue rdf:datatype="http://www.w3.org/2001/XMLSchema#double">950</qudt:numericalValue>
    <rdf:value rdf:datatype="http://www.w3.org/2001/XMLSchema#double">950</rdf:value>
    <gs1:unitCode>MLT</gs1:unitCode>
    <gs1:value>950</gs1:value>
  </gs1:QuantitativeValue>
 </gs1:netContent> 
 <sosa:isFeatureOfInterestOf>
  <rdf:Description rdf:about="#can950ml-ContentSosa">
   <rdf:type rdf:resource="http://www.w3.org/ns/sosa/Observation"/>
   <sosa:hasFeatureOfInterest rdf:resource="#can950ml"/>
   <sosa:observedProperty  rdf:resource="#netcontent"/>
   <sosa:hasResult rdf:resource="#can950ml-Content"/>
   <sosa:hasSimpleResult rdf:datatype="http://www.qudt.org/2.1/vocab/unit/MilliM">950</sosa:hasSimpleResult>
  </rdf:Description>
 </sosa:isFeatureOfInterestOf>
 <!-- Height -->
 <gs1:inPackageHeight>
  <gs1:QuantitativeValue rdf:about="#can950ml-Height">
   <rdf:type rdf:resource="http://qudt.org/1.1/schema/qudt#QuantityValue"/>
   <qudt:unit rdf:resource="http://www.qudt.org/2.1/vocab/unit/MilliM"/>
   <qudt:numericalValue rdf:datatype="http://www.w3.org/2001/XMLSchema#double">122.9</qudt:numericalValue>
   <rdf:value rdf:datatype="http://www.w3.org/2001/XMLSchema#double">122.9</rdf:value>
   <gs1:unitCode>MMT</gs1:unitCode>
   <gs1:value>122.9</gs1:value>
  </gs1:QuantitativeValue>
 </gs1:inPackageHeight>  
 <sosa:isFeatureOfInterestOf>
  <rdf:Description rdf:about="#can950ml-HeightSosa">
   <rdf:type rdf:resource="http://www.w3.org/ns/sosa/Observation"/>
   <sosa:hasFeatureOfInterest rdf:resource="#can950ml"/>
   <sosa:observedProperty  rdf:resource="#height"/>
   <sosa:hasResult rdf:resource="#can950ml-Height"/>
   <sosa:hasSimpleResult rdf:datatype="http://www.qudt.org/2.1/vocab/unit/MilliM">122.9</sosa:hasSimpleResult>
  </rdf:Description>
 </sosa:isFeatureOfInterestOf>
 <!-- Diameter --> 
 <gs1:inPackageDiameter>
  <gs1:QuantitativeValue rdf:about="#can950ml-Diameter">
   <rdf:type rdf:resource="http://qudt.org/1.1/schema/qudt#QuantityValue"/>
   <qudt:unit rdf:resource="http://www.qudt.org/2.1/vocab/unit/MilliM"/>
   <qudt:numericalValue rdf:datatype="http://www.w3.org/2001/XMLSchema#double">107.1</qudt:numericalValue>
   <rdf:value rdf:datatype="http://www.w3.org/2001/XMLSchema#double">107.1</rdf:value>
   <gs1:unitCode>MMT</gs1:unitCode>
   <gs1:value>107.1</gs1:value>
  </gs1:QuantitativeValue>
 </gs1:inPackageDiameter>
 <sosa:isFeatureOfInterestOf>
  <rdf:Description rdf:about="#can950ml-DiameterSosa">
   <rdf:type rdf:resource="http://www.w3.org/ns/sosa/Observation"/>
   <sosa:hasFeatureOfInterest rdf:resource="#can950ml"/>
   <sosa:observedProperty  rdf:resource="#diameter"/>
   <sosa:hasResult rdf:resource="#can950ml-Diameter"/>
   <sosa:hasSimpleResult rdf:datatype="http://www.qudt.org/2.1/vocab/unit/MilliM">107.1</sosa:hasSimpleResult>
  </rdf:Description>
 </sosa:isFeatureOfInterestOf>
 <rdfs:isDefinedBy rdf:resource="https://rdf.ag/o/beer-ONTOLOGY_DATE"/>
 <void:inDataset rdf:resource="#datasetdefinition"/>
</rdf:Description>


<rdf:Description rdf:about="#can3100ml">
 <rdf:type rdf:resource="https://gs1.org/voc/PackagingDetails"/>
 <rdf:type rdf:resource="#LiquidContainer"/>
 <rdf:type rdf:resource="#BeverageCan"/>
 <rdfs:label xml:lang="en">105oz/3100ml Metal Beverage Can</rdfs:label>
 <rdfs:label xml:lang="fr">Canette à Boisson Métallique, 105oz/3100ml</rdfs:label>
 <skos:definition xml:lang="en">A one time use 105oz/3100ml metal container meant to hold a liquid, commonly referred to as #1 Can 603 (Height 700).</skos:definition>
 <skos:definition xml:lang="fr">Un contenant non-réutilisable métallique de 105oz/3100ml pour contenir un liquide, souvent appeler #1 Can 603 (Hauteur 700).</skos:definition>
 <!-- Net Content -->
 <gs1:netContent>
  <gs1:QuantitativeValue rdf:about="#can3100ml-Content">
    <rdf:type rdf:resource="http://qudt.org/1.1/schema/qudt#QuantityValue"/>
    <qudt:unit rdf:resource="http://www.qudt.org/2.1/vocab/unit/MilliL"/>
    <qudt:numericalValue rdf:datatype="http://www.w3.org/2001/XMLSchema#double">3100</qudt:numericalValue>
    <rdf:value rdf:datatype="http://www.w3.org/2001/XMLSchema#double">3100</rdf:value>
    <gs1:unitCode>MLT</gs1:unitCode>
    <gs1:value>3100</gs1:value>
  </gs1:QuantitativeValue>
 </gs1:netContent> 
 <sosa:isFeatureOfInterestOf>
  <rdf:Description rdf:about="#can3100ml-ContentSosa">
   <rdf:type rdf:resource="http://www.w3.org/ns/sosa/Observation"/>
   <sosa:hasFeatureOfInterest rdf:resource="#can3100ml"/>
   <sosa:observedProperty  rdf:resource="#netcontent"/>
   <sosa:hasResult rdf:resource="#can3100ml-Content"/>
   <sosa:hasSimpleResult rdf:datatype="http://www.qudt.org/2.1/vocab/unit/MilliM">3100</sosa:hasSimpleResult>
  </rdf:Description>
 </sosa:isFeatureOfInterestOf>
 <!-- Height -->
 <gs1:inPackageHeight>
  <gs1:QuantitativeValue rdf:about="#can3100ml-Height">
   <rdf:type rdf:resource="http://qudt.org/1.1/schema/qudt#QuantityValue"/>
   <qudt:unit rdf:resource="http://www.qudt.org/2.1/vocab/unit/MilliM"/>
   <qudt:numericalValue rdf:datatype="http://www.w3.org/2001/XMLSchema#double">176.4</qudt:numericalValue>
   <rdf:value rdf:datatype="http://www.w3.org/2001/XMLSchema#double">176.4</rdf:value>
   <gs1:unitCode>MMT</gs1:unitCode>
   <gs1:value>176.4</gs1:value>
  </gs1:QuantitativeValue>
 </gs1:inPackageHeight>  
 <sosa:isFeatureOfInterestOf>
  <rdf:Description rdf:about="#can3100ml-HeightSosa">
   <rdf:type rdf:resource="http://www.w3.org/ns/sosa/Observation"/>
   <sosa:hasFeatureOfInterest rdf:resource="#can3100ml"/>
   <sosa:observedProperty  rdf:resource="#height"/>
   <sosa:hasResult rdf:resource="#can3100ml-Height"/>
   <sosa:hasSimpleResult rdf:datatype="http://www.qudt.org/2.1/vocab/unit/MilliM">176.4</sosa:hasSimpleResult>
  </rdf:Description>
 </sosa:isFeatureOfInterestOf>
 <!-- Diameter --> 
 <gs1:inPackageDiameter>
  <gs1:QuantitativeValue rdf:about="#can3100ml-Diameter">
   <rdf:type rdf:resource="http://qudt.org/1.1/schema/qudt#QuantityValue"/>
   <qudt:unit rdf:resource="http://www.qudt.org/2.1/vocab/unit/MilliM"/>
   <qudt:numericalValue rdf:datatype="http://www.w3.org/2001/XMLSchema#double">156</qudt:numericalValue>
   <rdf:value rdf:datatype="http://www.w3.org/2001/XMLSchema#double">156</rdf:value>
   <gs1:unitCode>MMT</gs1:unitCode>
   <gs1:value>156</gs1:value>
  </gs1:QuantitativeValue>
 </gs1:inPackageDiameter>
 <sosa:isFeatureOfInterestOf>
  <rdf:Description rdf:about="#can3100ml-DiameterSosa">
   <rdf:type rdf:resource="http://www.w3.org/ns/sosa/Observation"/>
   <sosa:hasFeatureOfInterest rdf:resource="#can3100ml"/>
   <sosa:observedProperty  rdf:resource="#diameter"/>
   <sosa:hasResult rdf:resource="#can3100ml-Diameter"/>
   <sosa:hasSimpleResult rdf:datatype="http://www.qudt.org/2.1/vocab/unit/MilliM">156</sosa:hasSimpleResult>
  </rdf:Description>
 </sosa:isFeatureOfInterestOf>
 <rdfs:isDefinedBy rdf:resource="https://rdf.ag/o/beer-ONTOLOGY_DATE"/>
 <void:inDataset rdf:resource="#datasetdefinition"/>
</rdf:Description>

<rdf:Description rdf:about="#can310ml">
 <rdf:type rdf:resource="#LiquidContainer"/>
 <rdf:type rdf:resource="#BeverageCan"/>
 <rdf:type rdf:resource="https://gs1.org/voc/PackagingDetails"/>
 <rdfs:label xml:lang="en">Any 310ml Can</rdfs:label>
 <rdfs:label xml:lang="fr">Canette à Boisson Métallique, 310ml</rdfs:label>
 <skos:definition xml:lang="en">Any 310ml Can</skos:definition>
 <skos:definition xml:lang="fr">Canette à Boisson Métallique, 310ml</skos:definition>
 <owl:oneOf>
  <rdf:List rdf:about="#can310mlList1">
   <rdf:first rdf:resource="#can310ml204200"/>
   <rdf:rest>
    <rdf:List rdf:about="#can310mlList2">
     <rdf:first rdf:resource="#can310ml204202"/>
     <rdf:rest rdf:resource="http://www.w3.org/1999/02/22-rdf-syntax-ns#nil"/>
    </rdf:List>
   </rdf:rest>
  </rdf:List>
 </owl:oneOf>       
</rdf:Description>


<rdf:Description rdf:about="#can310ml204200">
 <rdf:type rdf:resource="https://gs1.org/voc/PackagingDetails"/>
 <rdf:type rdf:resource="#LiquidContainer"/>
 <rdf:type rdf:resource="#BeverageCan"/>
 <rdfs:label xml:lang="en">10.5oz/310ml Metal Beverage Can</rdfs:label>
 <rdfs:label xml:lang="fr">Canette à Boisson Métallique, 10.5oz/310ml</rdfs:label>
 <skos:definition xml:lang="en">A one time use 10.5oz/310ml metal container meant to hold a liquid, commonly referred to as Sleek 204-200 (Height 508).</skos:definition>
 <skos:definition xml:lang="fr">Un contenant non-réutilisable métallique de 10.5oz/310ml pour contenir un liquide, souvent appeler Sleek 204-200 (Hauteur 508).</skos:definition>
 <!-- Net Content -->
 <gs1:netContent>
  <gs1:QuantitativeValue rdf:about="#can310ml204200-Content">
    <rdf:type rdf:resource="http://qudt.org/1.1/schema/qudt#QuantityValue"/>
    <qudt:unit rdf:resource="http://www.qudt.org/2.1/vocab/unit/MilliL"/>
    <qudt:numericalValue rdf:datatype="http://www.w3.org/2001/XMLSchema#double">310</qudt:numericalValue>
    <rdf:value rdf:datatype="http://www.w3.org/2001/XMLSchema#double">310</rdf:value>
    <gs1:unitCode>MLT</gs1:unitCode>
    <gs1:value>310</gs1:value>
  </gs1:QuantitativeValue>
 </gs1:netContent> 
 <sosa:isFeatureOfInterestOf>
  <rdf:Description rdf:about="#can310ml204200-ContentSosa">
   <rdf:type rdf:resource="http://www.w3.org/ns/sosa/Observation"/>
   <sosa:hasFeatureOfInterest rdf:resource="#can310ml204200"/>
   <sosa:observedProperty  rdf:resource="#netcontent"/>
   <sosa:hasResult rdf:resource="#can310ml204200-Content"/>
   <sosa:hasSimpleResult rdf:datatype="http://www.qudt.org/2.1/vocab/unit/MilliM">310</sosa:hasSimpleResult>
  </rdf:Description>
 </sosa:isFeatureOfInterestOf>
 <!-- Height -->
 <gs1:inPackageHeight>
  <gs1:QuantitativeValue rdf:about="#can310ml204200-Height">
   <rdf:type rdf:resource="http://qudt.org/1.1/schema/qudt#QuantityValue"/>
   <qudt:unit rdf:resource="http://www.qudt.org/2.1/vocab/unit/MilliM"/>
   <qudt:numericalValue rdf:datatype="http://www.w3.org/2001/XMLSchema#double">138</qudt:numericalValue>
   <rdf:value rdf:datatype="http://www.w3.org/2001/XMLSchema#double">138</rdf:value>
   <gs1:unitCode>MMT</gs1:unitCode>
   <gs1:value>138</gs1:value>
  </gs1:QuantitativeValue>
 </gs1:inPackageHeight>  
 <sosa:isFeatureOfInterestOf>
  <rdf:Description rdf:about="#can310ml204200-HeightSosa">
   <rdf:type rdf:resource="http://www.w3.org/ns/sosa/Observation"/>
   <sosa:hasFeatureOfInterest rdf:resource="#can310ml204200"/>
   <sosa:observedProperty  rdf:resource="#height"/>
   <sosa:hasResult rdf:resource="#can310ml204200-Height"/>
   <sosa:hasSimpleResult rdf:datatype="http://www.qudt.org/2.1/vocab/unit/MilliM">138</sosa:hasSimpleResult>
  </rdf:Description>
 </sosa:isFeatureOfInterestOf>
 <!-- Diameter --> 
 <gs1:inPackageDiameter>
  <gs1:QuantitativeValue rdf:about="#can310ml204200-Diameter">
   <rdf:type rdf:resource="http://qudt.org/1.1/schema/qudt#QuantityValue"/>
   <qudt:unit rdf:resource="http://www.qudt.org/2.1/vocab/unit/MilliM"/>
   <qudt:numericalValue rdf:datatype="http://www.w3.org/2001/XMLSchema#double">56.7</qudt:numericalValue>
   <rdf:value rdf:datatype="http://www.w3.org/2001/XMLSchema#double">56.7</rdf:value>
   <gs1:unitCode>MMT</gs1:unitCode>
   <gs1:value>56.7</gs1:value>
  </gs1:QuantitativeValue>
 </gs1:inPackageDiameter>
 <sosa:isFeatureOfInterestOf>
  <rdf:Description rdf:about="#can310ml204200-DiameterSosa">
   <rdf:type rdf:resource="http://www.w3.org/ns/sosa/Observation"/>
   <sosa:hasFeatureOfInterest rdf:resource="#can310ml204200"/>
   <sosa:observedProperty  rdf:resource="#diameter"/>
   <sosa:hasResult rdf:resource="#can310ml204200-Diameter"/>
   <sosa:hasSimpleResult rdf:datatype="http://www.qudt.org/2.1/vocab/unit/MilliM">56.7</sosa:hasSimpleResult>
  </rdf:Description>
 </sosa:isFeatureOfInterestOf>
 <sosa:isFeatureOfInterestOf>
  <rdf:Description rdf:about="#can310ml204200-EndDiameterSosa">
   <rdf:type rdf:resource="http://www.w3.org/ns/sosa/Observation"/>
   <sosa:hasFeatureOfInterest rdf:resource="#can310ml204200"/>
   <sosa:observedProperty  rdf:resource="#endDiameter"/>
   <sosa:hasResult>
    <gs1:QuantitativeValue rdf:about="#can310ml204200-EndDiameter">
     <rdf:type rdf:resource="http://qudt.org/1.1/schema/qudt#QuantityValue"/>
     <qudt:unit rdf:resource="http://www.qudt.org/2.1/vocab/unit/MilliM"/>
     <qudt:numericalValue rdf:datatype="http://www.w3.org/2001/XMLSchema#double">50.4</qudt:numericalValue>
     <rdf:value rdf:datatype="http://www.w3.org/2001/XMLSchema#double">50.4</rdf:value>
     <gs1:unitCode>MMT</gs1:unitCode>
     <gs1:value>50.4</gs1:value>
    </gs1:QuantitativeValue>
   </sosa:hasResult>
   <sosa:hasSimpleResult rdf:datatype="http://www.qudt.org/2.1/vocab/unit/MilliM">50.4</sosa:hasSimpleResult>
  </rdf:Description>
 </sosa:isFeatureOfInterestOf>
 <rdfs:isDefinedBy rdf:resource="https://rdf.ag/o/beer-ONTOLOGY_DATE"/>
 <void:inDataset rdf:resource="#datasetdefinition"/>
</rdf:Description>


<rdf:Description rdf:about="#can310ml204202">
 <rdf:type rdf:resource="https://gs1.org/voc/PackagingDetails"/>
 <rdf:type rdf:resource="#LiquidContainer"/>
 <rdf:type rdf:resource="#BeverageCan"/>
 <rdfs:label xml:lang="en">10.5oz/310ml Metal Beverage Can</rdfs:label>
 <rdfs:label xml:lang="fr">Canette à Boisson Métallique, 10.5oz/310ml</rdfs:label>
 <skos:definition xml:lang="en">A one time use 10.5oz/310ml metal container meant to hold a liquid, commonly referred to as Sleek 204-202 (Height 508).</skos:definition>
 <skos:definition xml:lang="fr">Un contenant non-réutilisable métallique de 10.5oz/310ml pour contenir un liquide, souvent appeler Sleek 204-202 (Hauteur 508).</skos:definition>
 <!-- Net Content -->
 <gs1:netContent>
  <gs1:QuantitativeValue rdf:about="#can310ml204202-Content">
    <rdf:type rdf:resource="http://qudt.org/1.1/schema/qudt#QuantityValue"/>
    <qudt:unit rdf:resource="http://www.qudt.org/2.1/vocab/unit/MilliL"/>
    <qudt:numericalValue rdf:datatype="http://www.w3.org/2001/XMLSchema#double">310</qudt:numericalValue>
    <rdf:value rdf:datatype="http://www.w3.org/2001/XMLSchema#double">310</rdf:value>
    <gs1:unitCode>MLT</gs1:unitCode>
    <gs1:value>310</gs1:value>
  </gs1:QuantitativeValue>
 </gs1:netContent> 
 <sosa:isFeatureOfInterestOf>
  <rdf:Description rdf:about="#can310ml204202-ContentSosa">
   <rdf:type rdf:resource="http://www.w3.org/ns/sosa/Observation"/>
   <sosa:hasFeatureOfInterest rdf:resource="#can310ml204202"/>
   <sosa:observedProperty  rdf:resource="#netcontent"/>
   <sosa:hasResult rdf:resource="#can310ml204202-Content"/>
   <sosa:hasSimpleResult rdf:datatype="http://www.qudt.org/2.1/vocab/unit/MilliM">310</sosa:hasSimpleResult>
  </rdf:Description>
 </sosa:isFeatureOfInterestOf>
 <!-- Height -->
 <gs1:inPackageHeight>
  <gs1:QuantitativeValue rdf:about="#can310ml204202-Height">
   <rdf:type rdf:resource="http://qudt.org/1.1/schema/qudt#QuantityValue"/>
   <qudt:unit rdf:resource="http://www.qudt.org/2.1/vocab/unit/MilliM"/>
   <qudt:numericalValue rdf:datatype="http://www.w3.org/2001/XMLSchema#double">138</qudt:numericalValue>
   <rdf:value rdf:datatype="http://www.w3.org/2001/XMLSchema#double">138</rdf:value>
   <gs1:unitCode>MMT</gs1:unitCode>
   <gs1:value>138</gs1:value>
  </gs1:QuantitativeValue>
 </gs1:inPackageHeight>  
 <sosa:isFeatureOfInterestOf>
  <rdf:Description rdf:about="#can310ml204202-HeightSosa">
   <rdf:type rdf:resource="http://www.w3.org/ns/sosa/Observation"/>
   <sosa:hasFeatureOfInterest rdf:resource="#can310ml204202"/>
   <sosa:observedProperty  rdf:resource="#height"/>
   <sosa:hasResult rdf:resource="#can310ml204202-Height"/>
   <sosa:hasSimpleResult rdf:datatype="http://www.qudt.org/2.1/vocab/unit/MilliM">138</sosa:hasSimpleResult>
  </rdf:Description>
 </sosa:isFeatureOfInterestOf>
 <!-- Diameter --> 
 <gs1:inPackageDiameter>
  <gs1:QuantitativeValue rdf:about="#can310ml204202-Diameter">
   <rdf:type rdf:resource="http://qudt.org/1.1/schema/qudt#QuantityValue"/>
   <qudt:unit rdf:resource="http://www.qudt.org/2.1/vocab/unit/MilliM"/>
   <qudt:numericalValue rdf:datatype="http://www.w3.org/2001/XMLSchema#double">56.7</qudt:numericalValue>
   <rdf:value rdf:datatype="http://www.w3.org/2001/XMLSchema#double">56.7</rdf:value>
   <gs1:unitCode>MMT</gs1:unitCode>
   <gs1:value>56.7</gs1:value>
  </gs1:QuantitativeValue>
 </gs1:inPackageDiameter>
 <sosa:isFeatureOfInterestOf>
  <rdf:Description rdf:about="#can310ml204202-DiameterSosa">
   <rdf:type rdf:resource="http://www.w3.org/ns/sosa/Observation"/>
   <sosa:hasFeatureOfInterest rdf:resource="#can310ml204202"/>
   <sosa:observedProperty  rdf:resource="#diameter"/>
   <sosa:hasResult rdf:resource="#can310ml204202-Diameter"/>
   <sosa:hasSimpleResult rdf:datatype="http://www.qudt.org/2.1/vocab/unit/MilliM">56.7</sosa:hasSimpleResult>
  </rdf:Description>
 </sosa:isFeatureOfInterestOf>
 <sosa:isFeatureOfInterestOf>
  <rdf:Description rdf:about="#can310ml204202-EndDiameterSosa">
   <rdf:type rdf:resource="http://www.w3.org/ns/sosa/Observation"/>
   <sosa:hasFeatureOfInterest rdf:resource="#can310ml204202"/>
   <sosa:observedProperty  rdf:resource="#endDiameter"/>
   <sosa:hasResult>
    <gs1:QuantitativeValue rdf:about="#can310ml204202-EndDiameter">
     <rdf:type rdf:resource="http://qudt.org/1.1/schema/qudt#QuantityValue"/>
     <qudt:unit rdf:resource="http://www.qudt.org/2.1/vocab/unit/MilliM"/>
     <qudt:numericalValue rdf:datatype="http://www.w3.org/2001/XMLSchema#double">53.5</qudt:numericalValue>
     <rdf:value rdf:datatype="http://www.w3.org/2001/XMLSchema#double">53.5</rdf:value>
     <gs1:unitCode>MMT</gs1:unitCode>
     <gs1:value>53.5</gs1:value>
    </gs1:QuantitativeValue>
   </sosa:hasResult>
   <sosa:hasSimpleResult rdf:datatype="http://www.qudt.org/2.1/vocab/unit/MilliM">53.5</sosa:hasSimpleResult>
  </rdf:Description>
 </sosa:isFeatureOfInterestOf>
 <rdfs:isDefinedBy rdf:resource="https://rdf.ag/o/beer-ONTOLOGY_DATE"/>
 <void:inDataset rdf:resource="#datasetdefinition"/>
</rdf:Description>


<rdf:Description rdf:about="#can330ml">
 <rdf:type rdf:resource="#LiquidContainer"/>
 <rdf:type rdf:resource="#BeverageCan"/>
 <rdf:type rdf:resource="https://gs1.org/voc/PackagingDetails"/>
 <rdfs:label xml:lang="en">Any 330ml Can</rdfs:label>
 <rdfs:label xml:lang="fr">Canette à Boisson Métallique, 330ml</rdfs:label>
 <skos:definition xml:lang="en">Any 330ml Can</skos:definition>
 <skos:definition xml:lang="fr">Canette à Boisson Métallique, 330ml</skos:definition>
 <owl:oneOf>
  <rdf:List rdf:about="#can330mlList1">
   <rdf:first rdf:resource="#can330ml211202"/>
   <rdf:rest>
    <rdf:List rdf:about="#can330mlList2">
     <rdf:first rdf:resource="#can330ml211206"/>
      <rdf:rest>
       <rdf:List rdf:about="#can330mlList3">
        <rdf:first rdf:resource="#can330ml204202"/>
        <rdf:rest rdf:resource="http://www.w3.org/1999/02/22-rdf-syntax-ns#nil"/>
       </rdf:List>
      </rdf:rest>
     </rdf:List>
    </rdf:rest>
  </rdf:List>
 </owl:oneOf>       
</rdf:Description>

<rdf:Description rdf:about="#can330ml211202">
 <rdf:type rdf:resource="https://gs1.org/voc/PackagingDetails"/>
 <rdf:type rdf:resource="#LiquidContainer"/>
 <rdf:type rdf:resource="#BeverageCan"/>
 <rdfs:label xml:lang="en">11.2oz/330ml Metal Beverage Can</rdfs:label>
 <rdfs:label xml:lang="fr">Canette à Boisson Métallique, 11.2oz/330ml</rdfs:label>
 <skos:definition xml:lang="en">A one time use 11.2oz/330ml metal container meant to hold a liquid, commonly referred to as Standard 211-202 (Height 409).</skos:definition>
 <skos:definition xml:lang="fr">Un contenant non-réutilisable métallique de 11.2oz/330ml pour contenir un liquide, souvent appeler Standard 211-202 (Hauteur 409).</skos:definition>
 <!-- Net Content -->
 <gs1:netContent>
  <gs1:QuantitativeValue rdf:about="#can330ml211202-Content">
    <rdf:type rdf:resource="http://qudt.org/1.1/schema/qudt#QuantityValue"/>
    <qudt:unit rdf:resource="http://www.qudt.org/2.1/vocab/unit/MilliL"/>
    <qudt:numericalValue rdf:datatype="http://www.w3.org/2001/XMLSchema#double">330</qudt:numericalValue>
    <rdf:value rdf:datatype="http://www.w3.org/2001/XMLSchema#double">330</rdf:value>
    <gs1:unitCode>MLT</gs1:unitCode>
    <gs1:value>330</gs1:value>
  </gs1:QuantitativeValue>
 </gs1:netContent> 
 <sosa:isFeatureOfInterestOf>
  <rdf:Description rdf:about="#can330ml211202-ContentSosa">
   <rdf:type rdf:resource="http://www.w3.org/ns/sosa/Observation"/>
   <sosa:hasFeatureOfInterest rdf:resource="#can330ml211202"/>
   <sosa:observedProperty  rdf:resource="#netcontent"/>
   <sosa:hasResult rdf:resource="#can330ml211202-Content"/>
   <sosa:hasSimpleResult rdf:datatype="http://www.qudt.org/2.1/vocab/unit/MilliM">330</sosa:hasSimpleResult>
  </rdf:Description>
 </sosa:isFeatureOfInterestOf>
 <!-- Height -->
 <gs1:inPackageHeight>
  <gs1:QuantitativeValue rdf:about="#can330ml211202-Height">
   <rdf:type rdf:resource="http://qudt.org/1.1/schema/qudt#QuantityValue"/>
   <qudt:unit rdf:resource="http://www.qudt.org/2.1/vocab/unit/MilliM"/>
   <qudt:numericalValue rdf:datatype="http://www.w3.org/2001/XMLSchema#double">115</qudt:numericalValue>
   <rdf:value rdf:datatype="http://www.w3.org/2001/XMLSchema#double">115</rdf:value>
   <gs1:unitCode>MMT</gs1:unitCode>
   <gs1:value>115</gs1:value>
  </gs1:QuantitativeValue>
 </gs1:inPackageHeight>  
 <sosa:isFeatureOfInterestOf>
  <rdf:Description rdf:about="#can330ml211202-HeightSosa">
   <rdf:type rdf:resource="http://www.w3.org/ns/sosa/Observation"/>
   <sosa:hasFeatureOfInterest rdf:resource="#can330ml211202"/>
   <sosa:observedProperty  rdf:resource="#height"/>
   <sosa:hasResult rdf:resource="#can330ml211202-Height"/>
   <sosa:hasSimpleResult rdf:datatype="http://www.qudt.org/2.1/vocab/unit/MilliM">115</sosa:hasSimpleResult>
  </rdf:Description>
 </sosa:isFeatureOfInterestOf>
 <!-- Diameter --> 
 <gs1:inPackageDiameter>
  <gs1:QuantitativeValue rdf:about="#can330ml211202-Diameter">
   <rdf:type rdf:resource="http://qudt.org/1.1/schema/qudt#QuantityValue"/>
   <qudt:unit rdf:resource="http://www.qudt.org/2.1/vocab/unit/MilliM"/>
   <qudt:numericalValue rdf:datatype="http://www.w3.org/2001/XMLSchema#double">66</qudt:numericalValue>
   <rdf:value rdf:datatype="http://www.w3.org/2001/XMLSchema#double">66</rdf:value>
   <gs1:unitCode>MMT</gs1:unitCode>
   <gs1:value>66</gs1:value>
  </gs1:QuantitativeValue>
 </gs1:inPackageDiameter>
 <sosa:isFeatureOfInterestOf>
  <rdf:Description rdf:about="#can330ml211202-DiameterSosa">
   <rdf:type rdf:resource="http://www.w3.org/ns/sosa/Observation"/>
   <sosa:hasFeatureOfInterest rdf:resource="#can330ml211202"/>
   <sosa:observedProperty  rdf:resource="#diameter"/>
   <sosa:hasResult rdf:resource="#can330ml211202-Diameter"/>
   <sosa:hasSimpleResult rdf:datatype="http://www.qudt.org/2.1/vocab/unit/MilliM">66</sosa:hasSimpleResult>
  </rdf:Description>
 </sosa:isFeatureOfInterestOf>
 <sosa:isFeatureOfInterestOf>
  <rdf:Description rdf:about="#can330ml211202-EndDiameterSosa">
   <rdf:type rdf:resource="http://www.w3.org/ns/sosa/Observation"/>
   <sosa:hasFeatureOfInterest rdf:resource="#can330ml211202"/>
   <sosa:observedProperty  rdf:resource="#endDiameter"/>
   <sosa:hasResult>
    <gs1:QuantitativeValue rdf:about="#can330ml211202-EndDiameter">
     <rdf:type rdf:resource="http://qudt.org/1.1/schema/qudt#QuantityValue"/>
     <qudt:unit rdf:resource="http://www.qudt.org/2.1/vocab/unit/MilliM"/>
     <qudt:numericalValue rdf:datatype="http://www.w3.org/2001/XMLSchema#double">53.55</qudt:numericalValue>
     <rdf:value rdf:datatype="http://www.w3.org/2001/XMLSchema#double">53.55</rdf:value>
     <gs1:unitCode>MMT</gs1:unitCode>
     <gs1:value>53.55</gs1:value>
    </gs1:QuantitativeValue>
   </sosa:hasResult>
   <sosa:hasSimpleResult rdf:datatype="http://www.qudt.org/2.1/vocab/unit/MilliM">53.55</sosa:hasSimpleResult>
  </rdf:Description>
 </sosa:isFeatureOfInterestOf>
 <rdfs:isDefinedBy rdf:resource="https://rdf.ag/o/beer-ONTOLOGY_DATE"/>
 <void:inDataset rdf:resource="#datasetdefinition"/>
</rdf:Description>


<rdf:Description rdf:about="#can330ml211206">
 <rdf:type rdf:resource="https://gs1.org/voc/PackagingDetails"/>
 <rdf:type rdf:resource="#LiquidContainer"/>
 <rdf:type rdf:resource="#BeverageCan"/>
 <rdfs:label xml:lang="en">11.2oz/330ml Metal Beverage Can</rdfs:label>
 <rdfs:label xml:lang="fr">Canette à Boisson Métallique, 11.2oz/330ml</rdfs:label>
 <skos:definition xml:lang="en">A one time use 11.2oz/330ml metal container meant to hold a liquid, commonly referred to as Standard 211-206 (Height 409).</skos:definition>
 <skos:definition xml:lang="fr">Un contenant non-réutilisable métallique de 11.2oz/330ml pour contenir un liquide, souvent appeler Standard 211-206 (Hauteur 409).</skos:definition>
 <!-- Net Content -->
 <gs1:netContent>
  <gs1:QuantitativeValue rdf:about="#can330ml211206-Content">
    <rdf:type rdf:resource="http://qudt.org/1.1/schema/qudt#QuantityValue"/>
    <qudt:unit rdf:resource="http://www.qudt.org/2.1/vocab/unit/MilliL"/>
    <qudt:numericalValue rdf:datatype="http://www.w3.org/2001/XMLSchema#double">330</qudt:numericalValue>
    <rdf:value rdf:datatype="http://www.w3.org/2001/XMLSchema#double">330</rdf:value>
    <gs1:unitCode>MLT</gs1:unitCode>
    <gs1:value>330</gs1:value>
  </gs1:QuantitativeValue>
 </gs1:netContent> 
 <sosa:isFeatureOfInterestOf>
  <rdf:Description rdf:about="#can330ml211206-ContentSosa">
   <rdf:type rdf:resource="http://www.w3.org/ns/sosa/Observation"/>
   <sosa:hasFeatureOfInterest rdf:resource="#can330ml211206"/>
   <sosa:observedProperty  rdf:resource="#netcontent"/>
   <sosa:hasResult rdf:resource="#can330ml211206-Content"/>
   <sosa:hasSimpleResult rdf:datatype="http://www.qudt.org/2.1/vocab/unit/MilliM">330</sosa:hasSimpleResult>
  </rdf:Description>
 </sosa:isFeatureOfInterestOf>
 <!-- Height -->
 <gs1:inPackageHeight>
  <gs1:QuantitativeValue rdf:about="#can330ml211206-Height">
   <rdf:type rdf:resource="http://qudt.org/1.1/schema/qudt#QuantityValue"/>
   <qudt:unit rdf:resource="http://www.qudt.org/2.1/vocab/unit/MilliM"/>
   <qudt:numericalValue rdf:datatype="http://www.w3.org/2001/XMLSchema#double">115</qudt:numericalValue>
   <rdf:value rdf:datatype="http://www.w3.org/2001/XMLSchema#double">115</rdf:value>
   <gs1:unitCode>MMT</gs1:unitCode>
   <gs1:value>115</gs1:value>
  </gs1:QuantitativeValue>
 </gs1:inPackageHeight>  
 <sosa:isFeatureOfInterestOf>
  <rdf:Description rdf:about="#can330ml211206-HeightSosa">
   <rdf:type rdf:resource="http://www.w3.org/ns/sosa/Observation"/>
   <sosa:hasFeatureOfInterest rdf:resource="#can330ml211206"/>
   <sosa:observedProperty  rdf:resource="#height"/>
   <sosa:hasResult rdf:resource="#can330ml211206-Height"/>
   <sosa:hasSimpleResult rdf:datatype="http://www.qudt.org/2.1/vocab/unit/MilliM">115</sosa:hasSimpleResult>
  </rdf:Description>
 </sosa:isFeatureOfInterestOf>
 <!-- Diameter --> 
 <gs1:inPackageDiameter>
  <gs1:QuantitativeValue rdf:about="#can330ml211206-Diameter">
   <rdf:type rdf:resource="http://qudt.org/1.1/schema/qudt#QuantityValue"/>
   <qudt:unit rdf:resource="http://www.qudt.org/2.1/vocab/unit/MilliM"/>
   <qudt:numericalValue rdf:datatype="http://www.w3.org/2001/XMLSchema#double">66</qudt:numericalValue>
   <rdf:value rdf:datatype="http://www.w3.org/2001/XMLSchema#double">66</rdf:value>
   <gs1:unitCode>MMT</gs1:unitCode>
   <gs1:value>66</gs1:value>
  </gs1:QuantitativeValue>
 </gs1:inPackageDiameter>
 <sosa:isFeatureOfInterestOf>
  <rdf:Description rdf:about="#can330ml211206-DiameterSosa">
   <rdf:type rdf:resource="http://www.w3.org/ns/sosa/Observation"/>
   <sosa:hasFeatureOfInterest rdf:resource="#can330ml211206"/>
   <sosa:observedProperty  rdf:resource="#diameter"/>
   <sosa:hasResult rdf:resource="#can330ml211206-Diameter"/>
   <sosa:hasSimpleResult rdf:datatype="http://www.qudt.org/2.1/vocab/unit/MilliM">66</sosa:hasSimpleResult>
  </rdf:Description>
 </sosa:isFeatureOfInterestOf>
 <sosa:isFeatureOfInterestOf>
  <rdf:Description rdf:about="#can330ml211206-EndDiameterSosa">
   <rdf:type rdf:resource="http://www.w3.org/ns/sosa/Observation"/>
   <sosa:hasFeatureOfInterest rdf:resource="#can330ml211206"/>
   <sosa:observedProperty  rdf:resource="#endDiameter"/>
   <sosa:hasResult>
    <gs1:QuantitativeValue rdf:about="#can330ml211206-EndDiameter">
     <rdf:type rdf:resource="http://qudt.org/1.1/schema/qudt#QuantityValue"/>
     <qudt:unit rdf:resource="http://www.qudt.org/2.1/vocab/unit/MilliM"/>
     <qudt:numericalValue rdf:datatype="http://www.w3.org/2001/XMLSchema#double">59.85</qudt:numericalValue>
     <rdf:value rdf:datatype="http://www.w3.org/2001/XMLSchema#double">59.85</rdf:value>
     <gs1:unitCode>MMT</gs1:unitCode>
     <gs1:value>59.85</gs1:value>
    </gs1:QuantitativeValue>
   </sosa:hasResult>
   <sosa:hasSimpleResult rdf:datatype="http://www.qudt.org/2.1/vocab/unit/MilliM">59.85</sosa:hasSimpleResult>
  </rdf:Description>
 </sosa:isFeatureOfInterestOf>
 <rdfs:isDefinedBy rdf:resource="https://rdf.ag/o/beer-ONTOLOGY_DATE"/>
 <void:inDataset rdf:resource="#datasetdefinition"/>
</rdf:Description>


<rdf:Description rdf:about="#can330ml204202">
 <rdf:type rdf:resource="https://gs1.org/voc/PackagingDetails"/>
 <rdf:type rdf:resource="#LiquidContainer"/>
 <rdf:type rdf:resource="#BeverageCan"/>
 <rdfs:label xml:lang="en">11.2oz/330ml Metal Beverage Can</rdfs:label>
 <rdfs:label xml:lang="fr">Canette à Boisson Métallique, 11.2oz/330ml</rdfs:label>
 <skos:definition xml:lang="en">A one time use 11.2oz/330ml metal container meant to hold a liquid, commonly referred to as Standard 204-202 (Height 512).</skos:definition>
 <skos:definition xml:lang="fr">Un contenant non-réutilisable métallique de 11.2oz/330ml pour contenir un liquide, souvent appeler Standard 204-202 (Hauteur 512).</skos:definition>
 <!-- Net Content -->
 <gs1:netContent>
  <gs1:QuantitativeValue rdf:about="#can330ml204202-Content">
    <rdf:type rdf:resource="http://qudt.org/1.1/schema/qudt#QuantityValue"/>
    <qudt:unit rdf:resource="http://www.qudt.org/2.1/vocab/unit/MilliL"/>
    <qudt:numericalValue rdf:datatype="http://www.w3.org/2001/XMLSchema#double">330</qudt:numericalValue>
    <rdf:value rdf:datatype="http://www.w3.org/2001/XMLSchema#double">330</rdf:value>
    <gs1:unitCode>MLT</gs1:unitCode>
    <gs1:value>330</gs1:value>
  </gs1:QuantitativeValue>
 </gs1:netContent> 
 <sosa:isFeatureOfInterestOf>
  <rdf:Description rdf:about="#can330ml204202-ContentSosa">
   <rdf:type rdf:resource="http://www.w3.org/ns/sosa/Observation"/>
   <sosa:hasFeatureOfInterest rdf:resource="#can330ml204202"/>
   <sosa:observedProperty  rdf:resource="#netcontent"/>
   <sosa:hasResult rdf:resource="#can330ml204202-Content"/>
   <sosa:hasSimpleResult rdf:datatype="http://www.qudt.org/2.1/vocab/unit/MilliM">330</sosa:hasSimpleResult>
  </rdf:Description>
 </sosa:isFeatureOfInterestOf>
 <!-- Height -->
 <gs1:inPackageHeight>
  <gs1:QuantitativeValue rdf:about="#can330ml204202-Height">
   <rdf:type rdf:resource="http://qudt.org/1.1/schema/qudt#QuantityValue"/>
   <qudt:unit rdf:resource="http://www.qudt.org/2.1/vocab/unit/MilliM"/>
   <qudt:numericalValue rdf:datatype="http://www.w3.org/2001/XMLSchema#double">146</qudt:numericalValue>
   <rdf:value rdf:datatype="http://www.w3.org/2001/XMLSchema#double">146</rdf:value>
   <gs1:unitCode>MMT</gs1:unitCode>
   <gs1:value>146</gs1:value>
  </gs1:QuantitativeValue>
 </gs1:inPackageHeight>  
 <sosa:isFeatureOfInterestOf>
  <rdf:Description rdf:about="#can330ml204202-HeightSosa">
   <rdf:type rdf:resource="http://www.w3.org/ns/sosa/Observation"/>
   <sosa:hasFeatureOfInterest rdf:resource="#can330ml204202"/>
   <sosa:observedProperty  rdf:resource="#height"/>
   <sosa:hasResult rdf:resource="#can330ml204202-Height"/>
   <sosa:hasSimpleResult rdf:datatype="http://www.qudt.org/2.1/vocab/unit/MilliM">146</sosa:hasSimpleResult>
  </rdf:Description>
 </sosa:isFeatureOfInterestOf>
 <!-- Diameter --> 
 <gs1:inPackageDiameter>
  <gs1:QuantitativeValue rdf:about="#can330ml204202-Diameter">
   <rdf:type rdf:resource="http://qudt.org/1.1/schema/qudt#QuantityValue"/>
   <qudt:unit rdf:resource="http://www.qudt.org/2.1/vocab/unit/MilliM"/>
   <qudt:numericalValue rdf:datatype="http://www.w3.org/2001/XMLSchema#double">56.7</qudt:numericalValue>
   <rdf:value rdf:datatype="http://www.w3.org/2001/XMLSchema#double">56.7</rdf:value>
   <gs1:unitCode>MMT</gs1:unitCode>
   <gs1:value>56.7</gs1:value>
  </gs1:QuantitativeValue>
 </gs1:inPackageDiameter>
 <sosa:isFeatureOfInterestOf>
  <rdf:Description rdf:about="#can330ml204202-DiameterSosa">
   <rdf:type rdf:resource="http://www.w3.org/ns/sosa/Observation"/>
   <sosa:hasFeatureOfInterest rdf:resource="#can330ml204202"/>
   <sosa:observedProperty  rdf:resource="#diameter"/>
   <sosa:hasResult rdf:resource="#can330ml204202-Diameter"/>
   <sosa:hasSimpleResult rdf:datatype="http://www.qudt.org/2.1/vocab/unit/MilliM">56.7</sosa:hasSimpleResult>
  </rdf:Description>
 </sosa:isFeatureOfInterestOf>
 <sosa:isFeatureOfInterestOf>
  <rdf:Description rdf:about="#can330ml204202-EndDiameterSosa">
   <rdf:type rdf:resource="http://www.w3.org/ns/sosa/Observation"/>
   <sosa:hasFeatureOfInterest rdf:resource="#can330ml204202"/>
   <sosa:observedProperty  rdf:resource="#endDiameter"/>
   <sosa:hasResult>
    <gs1:QuantitativeValue rdf:about="#can330ml204202-EndDiameter">
     <rdf:type rdf:resource="http://qudt.org/1.1/schema/qudt#QuantityValue"/>
     <qudt:unit rdf:resource="http://www.qudt.org/2.1/vocab/unit/MilliM"/>
     <qudt:numericalValue rdf:datatype="http://www.w3.org/2001/XMLSchema#double">53.55</qudt:numericalValue>
     <rdf:value rdf:datatype="http://www.w3.org/2001/XMLSchema#double">53.55</rdf:value>
     <gs1:unitCode>MMT</gs1:unitCode>
     <gs1:value>53.55</gs1:value>
    </gs1:QuantitativeValue>
   </sosa:hasResult>
   <sosa:hasSimpleResult rdf:datatype="http://www.qudt.org/2.1/vocab/unit/MilliM">53.55</sosa:hasSimpleResult>
  </rdf:Description>
 </sosa:isFeatureOfInterestOf>
 <rdfs:isDefinedBy rdf:resource="https://rdf.ag/o/beer-ONTOLOGY_DATE"/>
 <void:inDataset rdf:resource="#datasetdefinition"/>
</rdf:Description>

<!-- Compound packaging -->

 <rdf:Description rdf:about="#2xcan5000ml">
  <rdf:type rdf:resource="#LiquidContainer"/>
  <rdf:type rdf:resource="#BeverageCan"/>
  <rdf:type rdf:resource="https://gs1.org/voc/PackagingDetails"/>
  <rdfs:label xml:lang="en">2XCan5000ml</rdfs:label>
  <rdfs:label xml:lang="fr">2XCan5000ml</rdfs:label>
  <skos:definition xml:lang="en">Generic Flat, Box or Crate of 2, 5000ml Cans</skos:definition>
  <skos:definition xml:lang="fr">Une boite, caisse ou caissette générique de 2 Canettes de 5000ml</skos:definition>
  <rdfs:comment xml:lang="en">This term is meant to be used as a placeholder when no data about the aggregate packaging is known.</rdfs:comment>
  <rdfs:comment xml:lang="fr">Ce terme peut-être utilisé comme un terme générique lorsque les details de l’emballage ne sont pas certain.</rdfs:comment>
  <beer:count rdf:datatype="http://www.w3.org/2001/XMLSchema#Integer">2</beer:count>
  <beer:item rdf:resource="https://rdf.ag/o/beer#can5000ml"/>
  <rdfs:isDefinedBy rdf:resource="https://rdf.ag/o/beer-ONTOLOGY_DATE"/>
  <void:inDataset rdf:resource="#datasetdefinition"/>
  <gs1:netContent>
   <gs1:QuantitativeValue rdf:about="#2xcan5000ml-Content">
   <rdf:type rdf:resource="http://qudt.org/1.1/schema/qudt#QuantityValue"/>
   <qudt:unit rdf:resource="http://www.qudt.org/2.1/vocab/unit/MilliL"/>
   <qudt:numericalValue rdf:datatype="http://www.w3.org/2001/XMLSchema#double">10000</qudt:numericalValue>
   <rdf:value rdf:datatype="http://www.w3.org/2001/XMLSchema#double">10000</rdf:value>
   <gs1:unitCode>MLT</gs1:unitCode>
   <gs1:value>10000</gs1:value>
  </gs1:QuantitativeValue>
 </gs1:netContent>
 <sosa:isFeatureOfInterestOf>
  <rdf:Description rdf:about="#2xcan5000ml-ContentSosa">
   <rdf:type rdf:resource="http://www.w3.org/ns/sosa/Observation"/>
   <sosa:hasFeatureOfInterest rdf:resource="#2xcan5000ml"/>
   <sosa:observedProperty  rdf:resource="#netcontent"/>
   <sosa:hasResult rdf:resource="#2xcan5000ml-Content"/>
   <sosa:hasSimpleResult rdf:datatype="http://www.qudt.org/2.1/vocab/unit/MilliM">10000</sosa:hasSimpleResult>
  </rdf:Description>
 </sosa:isFeatureOfInterestOf>
 </rdf:Description>

 <rdf:Description rdf:about="#2xbottle200ml">
  <rdf:type rdf:resource="#LiquidContainer"/>
  <rdf:type rdf:resource="#BeverageBottle"/>
  <rdf:type rdf:resource="https://gs1.org/voc/PackagingDetails"/>
  <rdfs:label xml:lang="en">2XBottle200ml</rdfs:label>
  <rdfs:label xml:lang="fr">2XBottle200ml</rdfs:label>
  <skos:definition xml:lang="en">Generic Flat, Box or Crate of 2, 200ml Bottles</skos:definition>
  <skos:definition xml:lang="fr">Une boite, caisse ou caissette générique de 2 Bouteilles de 200ml</skos:definition>
  <rdfs:comment xml:lang="en">This term is meant to be used as a placeholder when no data about the aggregate packaging is known.</rdfs:comment>
  <rdfs:comment xml:lang="fr">Ce terme peut-être utilisé comme un terme générique lorsque les details de l’emballage ne sont pas certain.</rdfs:comment>
  <beer:count rdf:datatype="http://www.w3.org/2001/XMLSchema#Integer">2</beer:count>
  <beer:item rdf:resource="https://rdf.ag/o/beer#bottle200ml"/>
  <rdfs:isDefinedBy rdf:resource="https://rdf.ag/o/beer-ONTOLOGY_DATE"/>
  <void:inDataset rdf:resource="#datasetdefinition"/>
  <gs1:netContent>
   <gs1:QuantitativeValue rdf:about="#2xbottle200ml-Content">
   <rdf:type rdf:resource="http://qudt.org/1.1/schema/qudt#QuantityValue"/>
   <qudt:unit rdf:resource="http://www.qudt.org/2.1/vocab/unit/MilliL"/>
   <qudt:numericalValue rdf:datatype="http://www.w3.org/2001/XMLSchema#double">400</qudt:numericalValue>
   <rdf:value rdf:datatype="http://www.w3.org/2001/XMLSchema#double">400</rdf:value>
   <gs1:unitCode>MLT</gs1:unitCode>
   <gs1:value>400</gs1:value>
  </gs1:QuantitativeValue>
 </gs1:netContent>
 <sosa:isFeatureOfInterestOf>
  <rdf:Description rdf:about="#2xbottle200ml-ContentSosa">
   <rdf:type rdf:resource="http://www.w3.org/ns/sosa/Observation"/>
   <sosa:hasFeatureOfInterest rdf:resource="#2xbottle200ml"/>
   <sosa:observedProperty  rdf:resource="#netcontent"/>
   <sosa:hasResult rdf:resource="#2xbottle200ml-Content"/>
   <sosa:hasSimpleResult rdf:datatype="http://www.qudt.org/2.1/vocab/unit/MilliM">400</sosa:hasSimpleResult>
  </rdf:Description>
 </sosa:isFeatureOfInterestOf>
 </rdf:Description>

 <rdf:Description rdf:about="#12xbottle200ml">
  <rdf:type rdf:resource="#LiquidContainer"/>
  <rdf:type rdf:resource="#BeverageBottle"/>
  <rdf:type rdf:resource="https://gs1.org/voc/PackagingDetails"/>
  <rdfs:label xml:lang="en">12XBottle200ml</rdfs:label>
  <rdfs:label xml:lang="fr">12XBottle200ml</rdfs:label>
  <skos:definition xml:lang="en">Generic Flat, Box or Crate of 12, 200ml Bottles</skos:definition>
  <skos:definition xml:lang="fr">Une boite, caisse ou caissette générique de 12 Bouteilles de 200ml</skos:definition>
  <rdfs:comment xml:lang="en">This term is meant to be used as a placeholder when no data about the aggregate packaging is known.</rdfs:comment>
  <rdfs:comment xml:lang="fr">Ce terme peut-être utilisé comme un terme générique lorsque les details de l’emballage ne sont pas certain.</rdfs:comment>
  <beer:count rdf:datatype="http://www.w3.org/2001/XMLSchema#Integer">12</beer:count>
  <beer:item rdf:resource="https://rdf.ag/o/beer#bottle200ml"/>
  <rdfs:isDefinedBy rdf:resource="https://rdf.ag/o/beer-ONTOLOGY_DATE"/>
  <void:inDataset rdf:resource="#datasetdefinition"/>
  <gs1:netContent>
   <gs1:QuantitativeValue rdf:about="#12xbottle200ml-Content">
   <rdf:type rdf:resource="http://qudt.org/1.1/schema/qudt#QuantityValue"/>
   <qudt:unit rdf:resource="http://www.qudt.org/2.1/vocab/unit/MilliL"/>
   <qudt:numericalValue rdf:datatype="http://www.w3.org/2001/XMLSchema#double">2400</qudt:numericalValue>
   <rdf:value rdf:datatype="http://www.w3.org/2001/XMLSchema#double">2400</rdf:value>
   <gs1:unitCode>MLT</gs1:unitCode>
   <gs1:value>2400</gs1:value>
  </gs1:QuantitativeValue>
 </gs1:netContent>
 <sosa:isFeatureOfInterestOf>
  <rdf:Description rdf:about="#12xbottle200ml-ContentSosa">
   <rdf:type rdf:resource="http://www.w3.org/ns/sosa/Observation"/>
   <sosa:hasFeatureOfInterest rdf:resource="#12xbottle200ml"/>
   <sosa:observedProperty  rdf:resource="#netcontent"/>
   <sosa:hasResult rdf:resource="#12xbottle200ml-Content"/>
   <sosa:hasSimpleResult rdf:datatype="http://www.qudt.org/2.1/vocab/unit/MilliM">2400</sosa:hasSimpleResult>
  </rdf:Description>
 </sosa:isFeatureOfInterestOf>
 </rdf:Description>

 <rdf:Description rdf:about="#24xbottle200ml">
  <rdf:type rdf:resource="#LiquidContainer"/>
  <rdf:type rdf:resource="#BeverageBottle"/>
  <rdf:type rdf:resource="https://gs1.org/voc/PackagingDetails"/>
  <rdfs:label xml:lang="en">24XBottle200ml</rdfs:label>
  <rdfs:label xml:lang="fr">24XBottle200ml</rdfs:label>
  <skos:definition xml:lang="en">Generic Flat, Box or Crate of 24, 200ml Bottles</skos:definition>
  <skos:definition xml:lang="fr">Une boite, caisse ou caissette générique de 24 Bouteilles de 200ml</skos:definition>
  <rdfs:comment xml:lang="en">This term is meant to be used as a placeholder when no data about the aggregate packaging is known.</rdfs:comment>
  <rdfs:comment xml:lang="fr">Ce terme peut-être utilisé comme un terme générique lorsque les details de l’emballage ne sont pas certain.</rdfs:comment>
  <beer:count rdf:datatype="http://www.w3.org/2001/XMLSchema#Integer">24</beer:count>
  <beer:item rdf:resource="https://rdf.ag/o/beer#bottle200ml"/>
  <rdfs:isDefinedBy rdf:resource="https://rdf.ag/o/beer-ONTOLOGY_DATE"/>
  <void:inDataset rdf:resource="#datasetdefinition"/>
  <gs1:netContent>
   <gs1:QuantitativeValue rdf:about="#24xbottle200ml-Content">
   <rdf:type rdf:resource="http://qudt.org/1.1/schema/qudt#QuantityValue"/>
   <qudt:unit rdf:resource="http://www.qudt.org/2.1/vocab/unit/MilliL"/>
   <qudt:numericalValue rdf:datatype="http://www.w3.org/2001/XMLSchema#double">4800</qudt:numericalValue>
   <rdf:value rdf:datatype="http://www.w3.org/2001/XMLSchema#double">4800</rdf:value>
   <gs1:unitCode>MLT</gs1:unitCode>
   <gs1:value>4800</gs1:value>
  </gs1:QuantitativeValue>
 </gs1:netContent>
 <sosa:isFeatureOfInterestOf>
  <rdf:Description rdf:about="#24xbottle200ml-ContentSosa">
   <rdf:type rdf:resource="http://www.w3.org/ns/sosa/Observation"/>
   <sosa:hasFeatureOfInterest rdf:resource="#24xbottle200ml"/>
   <sosa:observedProperty  rdf:resource="#netcontent"/>
   <sosa:hasResult rdf:resource="#24xbottle200ml-Content"/>
   <sosa:hasSimpleResult rdf:datatype="http://www.qudt.org/2.1/vocab/unit/MilliM">4800</sosa:hasSimpleResult>
  </rdf:Description>
 </sosa:isFeatureOfInterestOf>
 </rdf:Description>

 <rdf:Description rdf:about="#6xbottle200ml">
  <rdf:type rdf:resource="#LiquidContainer"/>
  <rdf:type rdf:resource="#BeverageBottle"/>
  <rdf:type rdf:resource="https://gs1.org/voc/PackagingDetails"/>
  <rdfs:label xml:lang="en">6XBottle200ml</rdfs:label>
  <rdfs:label xml:lang="fr">6XBottle200ml</rdfs:label>
  <skos:definition xml:lang="en">Generic Flat, Box or Crate of 6, 200ml Bottles</skos:definition>
  <skos:definition xml:lang="fr">Une boite, caisse ou caissette générique de 6 Bouteilles de 200ml</skos:definition>
  <rdfs:comment xml:lang="en">This term is meant to be used as a placeholder when no data about the aggregate packaging is known.</rdfs:comment>
  <rdfs:comment xml:lang="fr">Ce terme peut-être utilisé comme un terme générique lorsque les details de l’emballage ne sont pas certain.</rdfs:comment>
  <beer:count rdf:datatype="http://www.w3.org/2001/XMLSchema#Integer">6</beer:count>
  <beer:item rdf:resource="https://rdf.ag/o/beer#bottle200ml"/>
  <rdfs:isDefinedBy rdf:resource="https://rdf.ag/o/beer-ONTOLOGY_DATE"/>
  <void:inDataset rdf:resource="#datasetdefinition"/>
  <gs1:netContent>
   <gs1:QuantitativeValue rdf:about="#6xbottle200ml-Content">
   <rdf:type rdf:resource="http://qudt.org/1.1/schema/qudt#QuantityValue"/>
   <qudt:unit rdf:resource="http://www.qudt.org/2.1/vocab/unit/MilliL"/>
   <qudt:numericalValue rdf:datatype="http://www.w3.org/2001/XMLSchema#double">1200</qudt:numericalValue>
   <rdf:value rdf:datatype="http://www.w3.org/2001/XMLSchema#double">1200</rdf:value>
   <gs1:unitCode>MLT</gs1:unitCode>
   <gs1:value>1200</gs1:value>
  </gs1:QuantitativeValue>
 </gs1:netContent>
 <sosa:isFeatureOfInterestOf>
  <rdf:Description rdf:about="#6xbottle200ml-ContentSosa">
   <rdf:type rdf:resource="http://www.w3.org/ns/sosa/Observation"/>
   <sosa:hasFeatureOfInterest rdf:resource="#6xbottle200ml"/>
   <sosa:observedProperty  rdf:resource="#netcontent"/>
   <sosa:hasResult rdf:resource="#6xbottle200ml-Content"/>
   <sosa:hasSimpleResult rdf:datatype="http://www.qudt.org/2.1/vocab/unit/MilliM">1200</sosa:hasSimpleResult>
  </rdf:Description>
 </sosa:isFeatureOfInterestOf>
 </rdf:Description>

 <rdf:Description rdf:about="#6xbottle1500ml">
  <rdf:type rdf:resource="#LiquidContainer"/>
  <rdf:type rdf:resource="#BeverageBottle"/>
  <rdf:type rdf:resource="https://gs1.org/voc/PackagingDetails"/>
  <rdfs:label xml:lang="en">6XBottle1500ml</rdfs:label>
  <rdfs:label xml:lang="fr">6XBottle1500ml</rdfs:label>
  <skos:definition xml:lang="en">Generic Flat, Box or Crate of 6, 1500ml Bottles</skos:definition>
  <skos:definition xml:lang="fr">Une boite, caisse ou caissette générique de 6 Bouteilles de 1500ml</skos:definition>
  <rdfs:comment xml:lang="en">This term is meant to be used as a placeholder when no data about the aggregate packaging is known.</rdfs:comment>
  <rdfs:comment xml:lang="fr">Ce terme peut-être utilisé comme un terme générique lorsque les details de l’emballage ne sont pas certain.</rdfs:comment>
  <beer:count rdf:datatype="http://www.w3.org/2001/XMLSchema#Integer">6</beer:count>
  <beer:item rdf:resource="https://rdf.ag/o/beer#bottle1500ml"/>
  <rdfs:isDefinedBy rdf:resource="https://rdf.ag/o/beer-ONTOLOGY_DATE"/>
  <void:inDataset rdf:resource="#datasetdefinition"/>
  <gs1:netContent>
   <gs1:QuantitativeValue rdf:about="#6xbottle1500ml-Content">
   <rdf:type rdf:resource="http://qudt.org/1.1/schema/qudt#QuantityValue"/>
   <qudt:unit rdf:resource="http://www.qudt.org/2.1/vocab/unit/MilliL"/>
   <qudt:numericalValue rdf:datatype="http://www.w3.org/2001/XMLSchema#double">9000</qudt:numericalValue>
   <rdf:value rdf:datatype="http://www.w3.org/2001/XMLSchema#double">9000</rdf:value>
   <gs1:unitCode>MLT</gs1:unitCode>
   <gs1:value>9000</gs1:value>
  </gs1:QuantitativeValue>
 </gs1:netContent>
 <sosa:isFeatureOfInterestOf>
  <rdf:Description rdf:about="#6xbottle1500ml-ContentSosa">
   <rdf:type rdf:resource="http://www.w3.org/ns/sosa/Observation"/>
   <sosa:hasFeatureOfInterest rdf:resource="#6xbottle1500ml"/>
   <sosa:observedProperty  rdf:resource="#netcontent"/>
   <sosa:hasResult rdf:resource="#6xbottle1500ml-Content"/>
   <sosa:hasSimpleResult rdf:datatype="http://www.qudt.org/2.1/vocab/unit/MilliM">9000</sosa:hasSimpleResult>
  </rdf:Description>
 </sosa:isFeatureOfInterestOf>
 </rdf:Description>

 <rdf:Description rdf:about="#20xbottle500ml">
  <rdf:type rdf:resource="#LiquidContainer"/>
  <rdf:type rdf:resource="#BeverageBottle"/>
  <rdf:type rdf:resource="https://gs1.org/voc/PackagingDetails"/>
  <rdfs:label xml:lang="en">20XBottle500ml</rdfs:label>
  <rdfs:label xml:lang="fr">20XBottle500ml</rdfs:label>
  <skos:definition xml:lang="en">Generic Flat, Box or Crate of 20, 500ml Bottles</skos:definition>
  <skos:definition xml:lang="fr">Une boite, caisse ou caissette générique de 20 Bouteilles de 500ml</skos:definition>
  <rdfs:comment xml:lang="en">This term is meant to be used as a placeholder when no data about the aggregate packaging is known.</rdfs:comment>
  <rdfs:comment xml:lang="fr">Ce terme peut-être utilisé comme un terme générique lorsque les details de l’emballage ne sont pas certain.</rdfs:comment>
  <beer:count rdf:datatype="http://www.w3.org/2001/XMLSchema#Integer">20</beer:count>
  <beer:item rdf:resource="https://rdf.ag/o/beer#bottle500ml"/>
  <rdfs:isDefinedBy rdf:resource="https://rdf.ag/o/beer-ONTOLOGY_DATE"/>
  <void:inDataset rdf:resource="#datasetdefinition"/>
  <gs1:netContent>
   <gs1:QuantitativeValue rdf:about="#20xbottle500ml-Content">
   <rdf:type rdf:resource="http://qudt.org/1.1/schema/qudt#QuantityValue"/>
   <qudt:unit rdf:resource="http://www.qudt.org/2.1/vocab/unit/MilliL"/>
   <qudt:numericalValue rdf:datatype="http://www.w3.org/2001/XMLSchema#double">10000</qudt:numericalValue>
   <rdf:value rdf:datatype="http://www.w3.org/2001/XMLSchema#double">10000</rdf:value>
   <gs1:unitCode>MLT</gs1:unitCode>
   <gs1:value>10000</gs1:value>
  </gs1:QuantitativeValue>
 </gs1:netContent>
 <sosa:isFeatureOfInterestOf>
  <rdf:Description rdf:about="#20xbottle500ml-ContentSosa">
   <rdf:type rdf:resource="http://www.w3.org/ns/sosa/Observation"/>
   <sosa:hasFeatureOfInterest rdf:resource="#20xbottle500ml"/>
   <sosa:observedProperty  rdf:resource="#netcontent"/>
   <sosa:hasResult rdf:resource="#20xbottle500ml-Content"/>
   <sosa:hasSimpleResult rdf:datatype="http://www.qudt.org/2.1/vocab/unit/MilliM">10000</sosa:hasSimpleResult>
  </rdf:Description>
 </sosa:isFeatureOfInterestOf>
 </rdf:Description>

 <rdf:Description rdf:about="#12xbottle500ml">
  <rdf:type rdf:resource="#LiquidContainer"/>
  <rdf:type rdf:resource="#BeverageBottle"/>
  <rdf:type rdf:resource="https://gs1.org/voc/PackagingDetails"/>
  <rdfs:label xml:lang="en">12XBottle500ml</rdfs:label>
  <rdfs:label xml:lang="fr">12XBottle500ml</rdfs:label>
  <skos:definition xml:lang="en">Generic Flat, Box or Crate of 12, 500ml Bottles</skos:definition>
  <skos:definition xml:lang="fr">Une boite, caisse ou caissette générique de 12 Bouteilles de 500ml</skos:definition>
  <rdfs:comment xml:lang="en">This term is meant to be used as a placeholder when no data about the aggregate packaging is known.</rdfs:comment>
  <rdfs:comment xml:lang="fr">Ce terme peut-être utilisé comme un terme générique lorsque les details de l’emballage ne sont pas certain.</rdfs:comment>
  <beer:count rdf:datatype="http://www.w3.org/2001/XMLSchema#Integer">12</beer:count>
  <beer:item rdf:resource="https://rdf.ag/o/beer#bottle500ml"/>
  <rdfs:isDefinedBy rdf:resource="https://rdf.ag/o/beer-ONTOLOGY_DATE"/>
  <void:inDataset rdf:resource="#datasetdefinition"/>
  <gs1:netContent>
   <gs1:QuantitativeValue rdf:about="#12xbottle500ml-Content">
   <rdf:type rdf:resource="http://qudt.org/1.1/schema/qudt#QuantityValue"/>
   <qudt:unit rdf:resource="http://www.qudt.org/2.1/vocab/unit/MilliL"/>
   <qudt:numericalValue rdf:datatype="http://www.w3.org/2001/XMLSchema#double">6000</qudt:numericalValue>
   <rdf:value rdf:datatype="http://www.w3.org/2001/XMLSchema#double">6000</rdf:value>
   <gs1:unitCode>MLT</gs1:unitCode>
   <gs1:value>6000</gs1:value>
  </gs1:QuantitativeValue>
 </gs1:netContent>
 <sosa:isFeatureOfInterestOf>
  <rdf:Description rdf:about="#12xbottle500ml-ContentSosa">
   <rdf:type rdf:resource="http://www.w3.org/ns/sosa/Observation"/>
   <sosa:hasFeatureOfInterest rdf:resource="#12xbottle500ml"/>
   <sosa:observedProperty  rdf:resource="#netcontent"/>
   <sosa:hasResult rdf:resource="#12xbottle500ml-Content"/>
   <sosa:hasSimpleResult rdf:datatype="http://www.qudt.org/2.1/vocab/unit/MilliM">6000</sosa:hasSimpleResult>
  </rdf:Description>
 </sosa:isFeatureOfInterestOf>
 </rdf:Description>

 <rdf:Description rdf:about="#4xbottle500ml">
  <rdf:type rdf:resource="#LiquidContainer"/>
  <rdf:type rdf:resource="#BeverageBottle"/>
  <rdf:type rdf:resource="https://gs1.org/voc/PackagingDetails"/>
  <rdfs:label xml:lang="en">4XBottle500ml</rdfs:label>
  <rdfs:label xml:lang="fr">4XBottle500ml</rdfs:label>
  <skos:definition xml:lang="en">Generic Flat, Box or Crate of 4, 500ml Bottles</skos:definition>
  <skos:definition xml:lang="fr">Une boite, caisse ou caissette générique de 4 Bouteilles de 500ml</skos:definition>
  <rdfs:comment xml:lang="en">This term is meant to be used as a placeholder when no data about the aggregate packaging is known.</rdfs:comment>
  <rdfs:comment xml:lang="fr">Ce terme peut-être utilisé comme un terme générique lorsque les details de l’emballage ne sont pas certain.</rdfs:comment>
  <beer:count rdf:datatype="http://www.w3.org/2001/XMLSchema#Integer">4</beer:count>
  <beer:item rdf:resource="https://rdf.ag/o/beer#bottle500ml"/>
  <rdfs:isDefinedBy rdf:resource="https://rdf.ag/o/beer-ONTOLOGY_DATE"/>
  <void:inDataset rdf:resource="#datasetdefinition"/>
  <gs1:netContent>
   <gs1:QuantitativeValue rdf:about="#4xbottle500ml-Content">
   <rdf:type rdf:resource="http://qudt.org/1.1/schema/qudt#QuantityValue"/>
   <qudt:unit rdf:resource="http://www.qudt.org/2.1/vocab/unit/MilliL"/>
   <qudt:numericalValue rdf:datatype="http://www.w3.org/2001/XMLSchema#double">2000</qudt:numericalValue>
   <rdf:value rdf:datatype="http://www.w3.org/2001/XMLSchema#double">2000</rdf:value>
   <gs1:unitCode>MLT</gs1:unitCode>
   <gs1:value>2000</gs1:value>
  </gs1:QuantitativeValue>
 </gs1:netContent>
 <sosa:isFeatureOfInterestOf>
  <rdf:Description rdf:about="#4xbottle500ml-ContentSosa">
   <rdf:type rdf:resource="http://www.w3.org/ns/sosa/Observation"/>
   <sosa:hasFeatureOfInterest rdf:resource="#4xbottle500ml"/>
   <sosa:observedProperty  rdf:resource="#netcontent"/>
   <sosa:hasResult rdf:resource="#4xbottle500ml-Content"/>
   <sosa:hasSimpleResult rdf:datatype="http://www.qudt.org/2.1/vocab/unit/MilliM">2000</sosa:hasSimpleResult>
  </rdf:Description>
 </sosa:isFeatureOfInterestOf>
 </rdf:Description>

 <rdf:Description rdf:about="#24xbottle500ml">
  <rdf:type rdf:resource="#LiquidContainer"/>
  <rdf:type rdf:resource="#BeverageBottle"/>
  <rdf:type rdf:resource="https://gs1.org/voc/PackagingDetails"/>
  <rdfs:label xml:lang="en">24XBottle500ml</rdfs:label>
  <rdfs:label xml:lang="fr">24XBottle500ml</rdfs:label>
  <skos:definition xml:lang="en">Generic Flat, Box or Crate of 24, 500ml Bottles</skos:definition>
  <skos:definition xml:lang="fr">Une boite, caisse ou caissette générique de 24 Bouteilles de 500ml</skos:definition>
  <rdfs:comment xml:lang="en">This term is meant to be used as a placeholder when no data about the aggregate packaging is known.</rdfs:comment>
  <rdfs:comment xml:lang="fr">Ce terme peut-être utilisé comme un terme générique lorsque les details de l’emballage ne sont pas certain.</rdfs:comment>
  <beer:count rdf:datatype="http://www.w3.org/2001/XMLSchema#Integer">24</beer:count>
  <beer:item rdf:resource="https://rdf.ag/o/beer#bottle500ml"/>
  <rdfs:isDefinedBy rdf:resource="https://rdf.ag/o/beer-ONTOLOGY_DATE"/>
  <void:inDataset rdf:resource="#datasetdefinition"/>
  <gs1:netContent>
   <gs1:QuantitativeValue rdf:about="#24xbottle500ml-Content">
   <rdf:type rdf:resource="http://qudt.org/1.1/schema/qudt#QuantityValue"/>
   <qudt:unit rdf:resource="http://www.qudt.org/2.1/vocab/unit/MilliL"/>
   <qudt:numericalValue rdf:datatype="http://www.w3.org/2001/XMLSchema#double">12000</qudt:numericalValue>
   <rdf:value rdf:datatype="http://www.w3.org/2001/XMLSchema#double">12000</rdf:value>
   <gs1:unitCode>MLT</gs1:unitCode>
   <gs1:value>12000</gs1:value>
  </gs1:QuantitativeValue>
 </gs1:netContent>
 <sosa:isFeatureOfInterestOf>
  <rdf:Description rdf:about="#24xbottle500ml-ContentSosa">
   <rdf:type rdf:resource="http://www.w3.org/ns/sosa/Observation"/>
   <sosa:hasFeatureOfInterest rdf:resource="#24xbottle500ml"/>
   <sosa:observedProperty  rdf:resource="#netcontent"/>
   <sosa:hasResult rdf:resource="#24xbottle500ml-Content"/>
   <sosa:hasSimpleResult rdf:datatype="http://www.qudt.org/2.1/vocab/unit/MilliM">12000</sosa:hasSimpleResult>
  </rdf:Description>
 </sosa:isFeatureOfInterestOf>
 </rdf:Description>

 <rdf:Description rdf:about="#6xbottle500ml">
  <rdf:type rdf:resource="#LiquidContainer"/>
  <rdf:type rdf:resource="#BeverageBottle"/>
  <rdf:type rdf:resource="https://gs1.org/voc/PackagingDetails"/>
  <rdfs:label xml:lang="en">6XBottle500ml</rdfs:label>
  <rdfs:label xml:lang="fr">6XBottle500ml</rdfs:label>
  <skos:definition xml:lang="en">Generic Flat, Box or Crate of 6, 500ml Bottles</skos:definition>
  <skos:definition xml:lang="fr">Une boite, caisse ou caissette générique de 6 Bouteilles de 500ml</skos:definition>
  <rdfs:comment xml:lang="en">This term is meant to be used as a placeholder when no data about the aggregate packaging is known.</rdfs:comment>
  <rdfs:comment xml:lang="fr">Ce terme peut-être utilisé comme un terme générique lorsque les details de l’emballage ne sont pas certain.</rdfs:comment>
  <beer:count rdf:datatype="http://www.w3.org/2001/XMLSchema#Integer">6</beer:count>
  <beer:item rdf:resource="https://rdf.ag/o/beer#bottle500ml"/>
  <rdfs:isDefinedBy rdf:resource="https://rdf.ag/o/beer-ONTOLOGY_DATE"/>
  <void:inDataset rdf:resource="#datasetdefinition"/>
  <gs1:netContent>
   <gs1:QuantitativeValue rdf:about="#6xbottle500ml-Content">
   <rdf:type rdf:resource="http://qudt.org/1.1/schema/qudt#QuantityValue"/>
   <qudt:unit rdf:resource="http://www.qudt.org/2.1/vocab/unit/MilliL"/>
   <qudt:numericalValue rdf:datatype="http://www.w3.org/2001/XMLSchema#double">3000</qudt:numericalValue>
   <rdf:value rdf:datatype="http://www.w3.org/2001/XMLSchema#double">3000</rdf:value>
   <gs1:unitCode>MLT</gs1:unitCode>
   <gs1:value>3000</gs1:value>
  </gs1:QuantitativeValue>
 </gs1:netContent>
 <sosa:isFeatureOfInterestOf>
  <rdf:Description rdf:about="#6xbottle500ml-ContentSosa">
   <rdf:type rdf:resource="http://www.w3.org/ns/sosa/Observation"/>
   <sosa:hasFeatureOfInterest rdf:resource="#6xbottle500ml"/>
   <sosa:observedProperty  rdf:resource="#netcontent"/>
   <sosa:hasResult rdf:resource="#6xbottle500ml-Content"/>
   <sosa:hasSimpleResult rdf:datatype="http://www.qudt.org/2.1/vocab/unit/MilliM">3000</sosa:hasSimpleResult>
  </rdf:Description>
 </sosa:isFeatureOfInterestOf>
 </rdf:Description>

 <rdf:Description rdf:about="#18xbottle500ml">
  <rdf:type rdf:resource="#LiquidContainer"/>
  <rdf:type rdf:resource="#BeverageBottle"/>
  <rdf:type rdf:resource="https://gs1.org/voc/PackagingDetails"/>
  <rdfs:label xml:lang="en">18XBottle500ml</rdfs:label>
  <rdfs:label xml:lang="fr">18XBottle500ml</rdfs:label>
  <skos:definition xml:lang="en">Generic Flat, Box or Crate of 18, 500ml Bottles</skos:definition>
  <skos:definition xml:lang="fr">Une boite, caisse ou caissette générique de 18 Bouteilles de 500ml</skos:definition>
  <rdfs:comment xml:lang="en">This term is meant to be used as a placeholder when no data about the aggregate packaging is known.</rdfs:comment>
  <rdfs:comment xml:lang="fr">Ce terme peut-être utilisé comme un terme générique lorsque les details de l’emballage ne sont pas certain.</rdfs:comment>
  <beer:count rdf:datatype="http://www.w3.org/2001/XMLSchema#Integer">18</beer:count>
  <beer:item rdf:resource="https://rdf.ag/o/beer#bottle500ml"/>
  <rdfs:isDefinedBy rdf:resource="https://rdf.ag/o/beer-ONTOLOGY_DATE"/>
  <void:inDataset rdf:resource="#datasetdefinition"/>
  <gs1:netContent>
   <gs1:QuantitativeValue rdf:about="#18xbottle500ml-Content">
   <rdf:type rdf:resource="http://qudt.org/1.1/schema/qudt#QuantityValue"/>
   <qudt:unit rdf:resource="http://www.qudt.org/2.1/vocab/unit/MilliL"/>
   <qudt:numericalValue rdf:datatype="http://www.w3.org/2001/XMLSchema#double">9000</qudt:numericalValue>
   <rdf:value rdf:datatype="http://www.w3.org/2001/XMLSchema#double">9000</rdf:value>
   <gs1:unitCode>MLT</gs1:unitCode>
   <gs1:value>9000</gs1:value>
  </gs1:QuantitativeValue>
 </gs1:netContent>
 <sosa:isFeatureOfInterestOf>
  <rdf:Description rdf:about="#18xbottle500ml-ContentSosa">
   <rdf:type rdf:resource="http://www.w3.org/ns/sosa/Observation"/>
   <sosa:hasFeatureOfInterest rdf:resource="#18xbottle500ml"/>
   <sosa:observedProperty  rdf:resource="#netcontent"/>
   <sosa:hasResult rdf:resource="#18xbottle500ml-Content"/>
   <sosa:hasSimpleResult rdf:datatype="http://www.qudt.org/2.1/vocab/unit/MilliM">9000</sosa:hasSimpleResult>
  </rdf:Description>
 </sosa:isFeatureOfInterestOf>
 </rdf:Description>

 <rdf:Description rdf:about="#12xcan500ml">
  <rdf:type rdf:resource="#LiquidContainer"/>
  <rdf:type rdf:resource="#BeverageCan"/>
  <rdf:type rdf:resource="https://gs1.org/voc/PackagingDetails"/>
  <rdfs:label xml:lang="en">12XCan500ml</rdfs:label>
  <rdfs:label xml:lang="fr">12XCan500ml</rdfs:label>
  <skos:definition xml:lang="en">Generic Flat, Box or Crate of 12, 500ml Cans</skos:definition>
  <skos:definition xml:lang="fr">Une boite, caisse ou caissette générique de 12 Canettes de 500ml</skos:definition>
  <rdfs:comment xml:lang="en">This term is meant to be used as a placeholder when no data about the aggregate packaging is known.</rdfs:comment>
  <rdfs:comment xml:lang="fr">Ce terme peut-être utilisé comme un terme générique lorsque les details de l’emballage ne sont pas certain.</rdfs:comment>
  <beer:count rdf:datatype="http://www.w3.org/2001/XMLSchema#Integer">12</beer:count>
  <beer:item rdf:resource="https://rdf.ag/o/beer#can500ml"/>
  <rdfs:isDefinedBy rdf:resource="https://rdf.ag/o/beer-ONTOLOGY_DATE"/>
  <void:inDataset rdf:resource="#datasetdefinition"/>
  <gs1:netContent>
   <gs1:QuantitativeValue rdf:about="#12xcan500ml-Content">
   <rdf:type rdf:resource="http://qudt.org/1.1/schema/qudt#QuantityValue"/>
   <qudt:unit rdf:resource="http://www.qudt.org/2.1/vocab/unit/MilliL"/>
   <qudt:numericalValue rdf:datatype="http://www.w3.org/2001/XMLSchema#double">6000</qudt:numericalValue>
   <rdf:value rdf:datatype="http://www.w3.org/2001/XMLSchema#double">6000</rdf:value>
   <gs1:unitCode>MLT</gs1:unitCode>
   <gs1:value>6000</gs1:value>
  </gs1:QuantitativeValue>
 </gs1:netContent>
 <sosa:isFeatureOfInterestOf>
  <rdf:Description rdf:about="#12xcan500ml-ContentSosa">
   <rdf:type rdf:resource="http://www.w3.org/ns/sosa/Observation"/>
   <sosa:hasFeatureOfInterest rdf:resource="#12xcan500ml"/>
   <sosa:observedProperty  rdf:resource="#netcontent"/>
   <sosa:hasResult rdf:resource="#12xcan500ml-Content"/>
   <sosa:hasSimpleResult rdf:datatype="http://www.qudt.org/2.1/vocab/unit/MilliM">6000</sosa:hasSimpleResult>
  </rdf:Description>
 </sosa:isFeatureOfInterestOf>
 </rdf:Description>

 <rdf:Description rdf:about="#4xcan500ml">
  <rdf:type rdf:resource="#LiquidContainer"/>
  <rdf:type rdf:resource="#BeverageCan"/>
  <rdf:type rdf:resource="https://gs1.org/voc/PackagingDetails"/>
  <rdfs:label xml:lang="en">4XCan500ml</rdfs:label>
  <rdfs:label xml:lang="fr">4XCan500ml</rdfs:label>
  <skos:definition xml:lang="en">Generic Flat, Box or Crate of 4, 500ml Cans</skos:definition>
  <skos:definition xml:lang="fr">Une boite, caisse ou caissette générique de 4 Canettes de 500ml</skos:definition>
  <rdfs:comment xml:lang="en">This term is meant to be used as a placeholder when no data about the aggregate packaging is known.</rdfs:comment>
  <rdfs:comment xml:lang="fr">Ce terme peut-être utilisé comme un terme générique lorsque les details de l’emballage ne sont pas certain.</rdfs:comment>
  <beer:count rdf:datatype="http://www.w3.org/2001/XMLSchema#Integer">4</beer:count>
  <beer:item rdf:resource="https://rdf.ag/o/beer#can500ml"/>
  <rdfs:isDefinedBy rdf:resource="https://rdf.ag/o/beer-ONTOLOGY_DATE"/>
  <void:inDataset rdf:resource="#datasetdefinition"/>
  <gs1:netContent>
   <gs1:QuantitativeValue rdf:about="#4xcan500ml-Content">
   <rdf:type rdf:resource="http://qudt.org/1.1/schema/qudt#QuantityValue"/>
   <qudt:unit rdf:resource="http://www.qudt.org/2.1/vocab/unit/MilliL"/>
   <qudt:numericalValue rdf:datatype="http://www.w3.org/2001/XMLSchema#double">2000</qudt:numericalValue>
   <rdf:value rdf:datatype="http://www.w3.org/2001/XMLSchema#double">2000</rdf:value>
   <gs1:unitCode>MLT</gs1:unitCode>
   <gs1:value>2000</gs1:value>
  </gs1:QuantitativeValue>
 </gs1:netContent>
 <sosa:isFeatureOfInterestOf>
  <rdf:Description rdf:about="#4xcan500ml-ContentSosa">
   <rdf:type rdf:resource="http://www.w3.org/ns/sosa/Observation"/>
   <sosa:hasFeatureOfInterest rdf:resource="#4xcan500ml"/>
   <sosa:observedProperty  rdf:resource="#netcontent"/>
   <sosa:hasResult rdf:resource="#4xcan500ml-Content"/>
   <sosa:hasSimpleResult rdf:datatype="http://www.qudt.org/2.1/vocab/unit/MilliM">2000</sosa:hasSimpleResult>
  </rdf:Description>
 </sosa:isFeatureOfInterestOf>
 </rdf:Description>

 <rdf:Description rdf:about="#24xcan500ml">
  <rdf:type rdf:resource="#LiquidContainer"/>
  <rdf:type rdf:resource="#BeverageCan"/>
  <rdf:type rdf:resource="https://gs1.org/voc/PackagingDetails"/>
  <rdfs:label xml:lang="en">24XCan500ml</rdfs:label>
  <rdfs:label xml:lang="fr">24XCan500ml</rdfs:label>
  <skos:definition xml:lang="en">Generic Flat, Box or Crate of 24, 500ml Cans</skos:definition>
  <skos:definition xml:lang="fr">Une boite, caisse ou caissette générique de 24 Canettes de 500ml</skos:definition>
  <rdfs:comment xml:lang="en">This term is meant to be used as a placeholder when no data about the aggregate packaging is known.</rdfs:comment>
  <rdfs:comment xml:lang="fr">Ce terme peut-être utilisé comme un terme générique lorsque les details de l’emballage ne sont pas certain.</rdfs:comment>
  <beer:count rdf:datatype="http://www.w3.org/2001/XMLSchema#Integer">24</beer:count>
  <beer:item rdf:resource="https://rdf.ag/o/beer#can500ml"/>
  <rdfs:isDefinedBy rdf:resource="https://rdf.ag/o/beer-ONTOLOGY_DATE"/>
  <void:inDataset rdf:resource="#datasetdefinition"/>
  <gs1:netContent>
   <gs1:QuantitativeValue rdf:about="#24xcan500ml-Content">
   <rdf:type rdf:resource="http://qudt.org/1.1/schema/qudt#QuantityValue"/>
   <qudt:unit rdf:resource="http://www.qudt.org/2.1/vocab/unit/MilliL"/>
   <qudt:numericalValue rdf:datatype="http://www.w3.org/2001/XMLSchema#double">12000</qudt:numericalValue>
   <rdf:value rdf:datatype="http://www.w3.org/2001/XMLSchema#double">12000</rdf:value>
   <gs1:unitCode>MLT</gs1:unitCode>
   <gs1:value>12000</gs1:value>
  </gs1:QuantitativeValue>
 </gs1:netContent>
 <sosa:isFeatureOfInterestOf>
  <rdf:Description rdf:about="#24xcan500ml-ContentSosa">
   <rdf:type rdf:resource="http://www.w3.org/ns/sosa/Observation"/>
   <sosa:hasFeatureOfInterest rdf:resource="#24xcan500ml"/>
   <sosa:observedProperty  rdf:resource="#netcontent"/>
   <sosa:hasResult rdf:resource="#24xcan500ml-Content"/>
   <sosa:hasSimpleResult rdf:datatype="http://www.qudt.org/2.1/vocab/unit/MilliM">12000</sosa:hasSimpleResult>
  </rdf:Description>
 </sosa:isFeatureOfInterestOf>
 </rdf:Description>

 <rdf:Description rdf:about="#6xcan500ml">
  <rdf:type rdf:resource="#LiquidContainer"/>
  <rdf:type rdf:resource="#BeverageCan"/>
  <rdf:type rdf:resource="https://gs1.org/voc/PackagingDetails"/>
  <rdfs:label xml:lang="en">6XCan500ml</rdfs:label>
  <rdfs:label xml:lang="fr">6XCan500ml</rdfs:label>
  <skos:definition xml:lang="en">Generic Flat, Box or Crate of 6, 500ml Cans</skos:definition>
  <skos:definition xml:lang="fr">Une boite, caisse ou caissette générique de 6 Canettes de 500ml</skos:definition>
  <rdfs:comment xml:lang="en">This term is meant to be used as a placeholder when no data about the aggregate packaging is known.</rdfs:comment>
  <rdfs:comment xml:lang="fr">Ce terme peut-être utilisé comme un terme générique lorsque les details de l’emballage ne sont pas certain.</rdfs:comment>
  <beer:count rdf:datatype="http://www.w3.org/2001/XMLSchema#Integer">6</beer:count>
  <beer:item rdf:resource="https://rdf.ag/o/beer#can500ml"/>
  <rdfs:isDefinedBy rdf:resource="https://rdf.ag/o/beer-ONTOLOGY_DATE"/>
  <void:inDataset rdf:resource="#datasetdefinition"/>
  <gs1:netContent>
   <gs1:QuantitativeValue rdf:about="#6xcan500ml-Content">
   <rdf:type rdf:resource="http://qudt.org/1.1/schema/qudt#QuantityValue"/>
   <qudt:unit rdf:resource="http://www.qudt.org/2.1/vocab/unit/MilliL"/>
   <qudt:numericalValue rdf:datatype="http://www.w3.org/2001/XMLSchema#double">3000</qudt:numericalValue>
   <rdf:value rdf:datatype="http://www.w3.org/2001/XMLSchema#double">3000</rdf:value>
   <gs1:unitCode>MLT</gs1:unitCode>
   <gs1:value>3000</gs1:value>
  </gs1:QuantitativeValue>
 </gs1:netContent>
 <sosa:isFeatureOfInterestOf>
  <rdf:Description rdf:about="#6xcan500ml-ContentSosa">
   <rdf:type rdf:resource="http://www.w3.org/ns/sosa/Observation"/>
   <sosa:hasFeatureOfInterest rdf:resource="#6xcan500ml"/>
   <sosa:observedProperty  rdf:resource="#netcontent"/>
   <sosa:hasResult rdf:resource="#6xcan500ml-Content"/>
   <sosa:hasSimpleResult rdf:datatype="http://www.qudt.org/2.1/vocab/unit/MilliM">3000</sosa:hasSimpleResult>
  </rdf:Description>
 </sosa:isFeatureOfInterestOf>
 </rdf:Description>

 <rdf:Description rdf:about="#8xcan500ml">
  <rdf:type rdf:resource="#LiquidContainer"/>
  <rdf:type rdf:resource="#BeverageCan"/>
  <rdf:type rdf:resource="https://gs1.org/voc/PackagingDetails"/>
  <rdfs:label xml:lang="en">8XCan500ml</rdfs:label>
  <rdfs:label xml:lang="fr">8XCan500ml</rdfs:label>
  <skos:definition xml:lang="en">Generic Flat, Box or Crate of 8, 500ml Cans</skos:definition>
  <skos:definition xml:lang="fr">Une boite, caisse ou caissette générique de 8 Canettes de 500ml</skos:definition>
  <rdfs:comment xml:lang="en">This term is meant to be used as a placeholder when no data about the aggregate packaging is known.</rdfs:comment>
  <rdfs:comment xml:lang="fr">Ce terme peut-être utilisé comme un terme générique lorsque les details de l’emballage ne sont pas certain.</rdfs:comment>
  <beer:count rdf:datatype="http://www.w3.org/2001/XMLSchema#Integer">8</beer:count>
  <beer:item rdf:resource="https://rdf.ag/o/beer#can500ml"/>
  <rdfs:isDefinedBy rdf:resource="https://rdf.ag/o/beer-ONTOLOGY_DATE"/>
  <void:inDataset rdf:resource="#datasetdefinition"/>
  <gs1:netContent>
   <gs1:QuantitativeValue rdf:about="#8xcan500ml-Content">
   <rdf:type rdf:resource="http://qudt.org/1.1/schema/qudt#QuantityValue"/>
   <qudt:unit rdf:resource="http://www.qudt.org/2.1/vocab/unit/MilliL"/>
   <qudt:numericalValue rdf:datatype="http://www.w3.org/2001/XMLSchema#double">4000</qudt:numericalValue>
   <rdf:value rdf:datatype="http://www.w3.org/2001/XMLSchema#double">4000</rdf:value>
   <gs1:unitCode>MLT</gs1:unitCode>
   <gs1:value>4000</gs1:value>
  </gs1:QuantitativeValue>
 </gs1:netContent>
 <sosa:isFeatureOfInterestOf>
  <rdf:Description rdf:about="#8xcan500ml-ContentSosa">
   <rdf:type rdf:resource="http://www.w3.org/ns/sosa/Observation"/>
   <sosa:hasFeatureOfInterest rdf:resource="#8xcan500ml"/>
   <sosa:observedProperty  rdf:resource="#netcontent"/>
   <sosa:hasResult rdf:resource="#8xcan500ml-Content"/>
   <sosa:hasSimpleResult rdf:datatype="http://www.qudt.org/2.1/vocab/unit/MilliM">4000</sosa:hasSimpleResult>
  </rdf:Description>
 </sosa:isFeatureOfInterestOf>
 </rdf:Description>

 <rdf:Description rdf:about="#18xcan500ml">
  <rdf:type rdf:resource="#LiquidContainer"/>
  <rdf:type rdf:resource="#BeverageCan"/>
  <rdf:type rdf:resource="https://gs1.org/voc/PackagingDetails"/>
  <rdfs:label xml:lang="en">18XCan500ml</rdfs:label>
  <rdfs:label xml:lang="fr">18XCan500ml</rdfs:label>
  <skos:definition xml:lang="en">Generic Flat, Box or Crate of 18, 500ml Cans</skos:definition>
  <skos:definition xml:lang="fr">Une boite, caisse ou caissette générique de 18 Canettes de 500ml</skos:definition>
  <rdfs:comment xml:lang="en">This term is meant to be used as a placeholder when no data about the aggregate packaging is known.</rdfs:comment>
  <rdfs:comment xml:lang="fr">Ce terme peut-être utilisé comme un terme générique lorsque les details de l’emballage ne sont pas certain.</rdfs:comment>
  <beer:count rdf:datatype="http://www.w3.org/2001/XMLSchema#Integer">18</beer:count>
  <beer:item rdf:resource="https://rdf.ag/o/beer#can500ml"/>
  <rdfs:isDefinedBy rdf:resource="https://rdf.ag/o/beer-ONTOLOGY_DATE"/>
  <void:inDataset rdf:resource="#datasetdefinition"/>
  <gs1:netContent>
   <gs1:QuantitativeValue rdf:about="#18xcan500ml-Content">
   <rdf:type rdf:resource="http://qudt.org/1.1/schema/qudt#QuantityValue"/>
   <qudt:unit rdf:resource="http://www.qudt.org/2.1/vocab/unit/MilliL"/>
   <qudt:numericalValue rdf:datatype="http://www.w3.org/2001/XMLSchema#double">9000</qudt:numericalValue>
   <rdf:value rdf:datatype="http://www.w3.org/2001/XMLSchema#double">9000</rdf:value>
   <gs1:unitCode>MLT</gs1:unitCode>
   <gs1:value>9000</gs1:value>
  </gs1:QuantitativeValue>
 </gs1:netContent>
 <sosa:isFeatureOfInterestOf>
  <rdf:Description rdf:about="#18xcan500ml-ContentSosa">
   <rdf:type rdf:resource="http://www.w3.org/ns/sosa/Observation"/>
   <sosa:hasFeatureOfInterest rdf:resource="#18xcan500ml"/>
   <sosa:observedProperty  rdf:resource="#netcontent"/>
   <sosa:hasResult rdf:resource="#18xcan500ml-Content"/>
   <sosa:hasSimpleResult rdf:datatype="http://www.qudt.org/2.1/vocab/unit/MilliM">9000</sosa:hasSimpleResult>
  </rdf:Description>
 </sosa:isFeatureOfInterestOf>
 </rdf:Description>

 <rdf:Description rdf:about="#12xbottle600ml">
  <rdf:type rdf:resource="#LiquidContainer"/>
  <rdf:type rdf:resource="#BeverageBottle"/>
  <rdf:type rdf:resource="https://gs1.org/voc/PackagingDetails"/>
  <rdfs:label xml:lang="en">12XBottle600ml</rdfs:label>
  <rdfs:label xml:lang="fr">12XBottle600ml</rdfs:label>
  <skos:definition xml:lang="en">Generic Flat, Box or Crate of 12, 600ml Bottles</skos:definition>
  <skos:definition xml:lang="fr">Une boite, caisse ou caissette générique de 12 Bouteilles de 600ml</skos:definition>
  <rdfs:comment xml:lang="en">This term is meant to be used as a placeholder when no data about the aggregate packaging is known.</rdfs:comment>
  <rdfs:comment xml:lang="fr">Ce terme peut-être utilisé comme un terme générique lorsque les details de l’emballage ne sont pas certain.</rdfs:comment>
  <beer:count rdf:datatype="http://www.w3.org/2001/XMLSchema#Integer">12</beer:count>
  <beer:item rdf:resource="https://rdf.ag/o/beer#bottle600ml"/>
  <rdfs:isDefinedBy rdf:resource="https://rdf.ag/o/beer-ONTOLOGY_DATE"/>
  <void:inDataset rdf:resource="#datasetdefinition"/>
  <gs1:netContent>
   <gs1:QuantitativeValue rdf:about="#12xbottle600ml-Content">
   <rdf:type rdf:resource="http://qudt.org/1.1/schema/qudt#QuantityValue"/>
   <qudt:unit rdf:resource="http://www.qudt.org/2.1/vocab/unit/MilliL"/>
   <qudt:numericalValue rdf:datatype="http://www.w3.org/2001/XMLSchema#double">7200</qudt:numericalValue>
   <rdf:value rdf:datatype="http://www.w3.org/2001/XMLSchema#double">7200</rdf:value>
   <gs1:unitCode>MLT</gs1:unitCode>
   <gs1:value>7200</gs1:value>
  </gs1:QuantitativeValue>
 </gs1:netContent>
 <sosa:isFeatureOfInterestOf>
  <rdf:Description rdf:about="#12xbottle600ml-ContentSosa">
   <rdf:type rdf:resource="http://www.w3.org/ns/sosa/Observation"/>
   <sosa:hasFeatureOfInterest rdf:resource="#12xbottle600ml"/>
   <sosa:observedProperty  rdf:resource="#netcontent"/>
   <sosa:hasResult rdf:resource="#12xbottle600ml-Content"/>
   <sosa:hasSimpleResult rdf:datatype="http://www.qudt.org/2.1/vocab/unit/MilliM">7200</sosa:hasSimpleResult>
  </rdf:Description>
 </sosa:isFeatureOfInterestOf>
 </rdf:Description>

 <rdf:Description rdf:about="#4xbottle600ml">
  <rdf:type rdf:resource="#LiquidContainer"/>
  <rdf:type rdf:resource="#BeverageBottle"/>
  <rdf:type rdf:resource="https://gs1.org/voc/PackagingDetails"/>
  <rdfs:label xml:lang="en">4XBottle600ml</rdfs:label>
  <rdfs:label xml:lang="fr">4XBottle600ml</rdfs:label>
  <skos:definition xml:lang="en">Generic Flat, Box or Crate of 4, 600ml Bottles</skos:definition>
  <skos:definition xml:lang="fr">Une boite, caisse ou caissette générique de 4 Bouteilles de 600ml</skos:definition>
  <rdfs:comment xml:lang="en">This term is meant to be used as a placeholder when no data about the aggregate packaging is known.</rdfs:comment>
  <rdfs:comment xml:lang="fr">Ce terme peut-être utilisé comme un terme générique lorsque les details de l’emballage ne sont pas certain.</rdfs:comment>
  <beer:count rdf:datatype="http://www.w3.org/2001/XMLSchema#Integer">4</beer:count>
  <beer:item rdf:resource="https://rdf.ag/o/beer#bottle600ml"/>
  <rdfs:isDefinedBy rdf:resource="https://rdf.ag/o/beer-ONTOLOGY_DATE"/>
  <void:inDataset rdf:resource="#datasetdefinition"/>
  <gs1:netContent>
   <gs1:QuantitativeValue rdf:about="#4xbottle600ml-Content">
   <rdf:type rdf:resource="http://qudt.org/1.1/schema/qudt#QuantityValue"/>
   <qudt:unit rdf:resource="http://www.qudt.org/2.1/vocab/unit/MilliL"/>
   <qudt:numericalValue rdf:datatype="http://www.w3.org/2001/XMLSchema#double">2400</qudt:numericalValue>
   <rdf:value rdf:datatype="http://www.w3.org/2001/XMLSchema#double">2400</rdf:value>
   <gs1:unitCode>MLT</gs1:unitCode>
   <gs1:value>2400</gs1:value>
  </gs1:QuantitativeValue>
 </gs1:netContent>
 <sosa:isFeatureOfInterestOf>
  <rdf:Description rdf:about="#4xbottle600ml-ContentSosa">
   <rdf:type rdf:resource="http://www.w3.org/ns/sosa/Observation"/>
   <sosa:hasFeatureOfInterest rdf:resource="#4xbottle600ml"/>
   <sosa:observedProperty  rdf:resource="#netcontent"/>
   <sosa:hasResult rdf:resource="#4xbottle600ml-Content"/>
   <sosa:hasSimpleResult rdf:datatype="http://www.qudt.org/2.1/vocab/unit/MilliM">2400</sosa:hasSimpleResult>
  </rdf:Description>
 </sosa:isFeatureOfInterestOf>
 </rdf:Description>

 <rdf:Description rdf:about="#16xbottle600ml">
  <rdf:type rdf:resource="#LiquidContainer"/>
  <rdf:type rdf:resource="#BeverageBottle"/>
  <rdf:type rdf:resource="https://gs1.org/voc/PackagingDetails"/>
  <rdfs:label xml:lang="en">16XBottle600ml</rdfs:label>
  <rdfs:label xml:lang="fr">16XBottle600ml</rdfs:label>
  <skos:definition xml:lang="en">Generic Flat, Box or Crate of 16, 600ml Bottles</skos:definition>
  <skos:definition xml:lang="fr">Une boite, caisse ou caissette générique de 16 Bouteilles de 600ml</skos:definition>
  <rdfs:comment xml:lang="en">This term is meant to be used as a placeholder when no data about the aggregate packaging is known.</rdfs:comment>
  <rdfs:comment xml:lang="fr">Ce terme peut-être utilisé comme un terme générique lorsque les details de l’emballage ne sont pas certain.</rdfs:comment>
  <beer:count rdf:datatype="http://www.w3.org/2001/XMLSchema#Integer">16</beer:count>
  <beer:item rdf:resource="https://rdf.ag/o/beer#bottle600ml"/>
  <rdfs:isDefinedBy rdf:resource="https://rdf.ag/o/beer-ONTOLOGY_DATE"/>
  <void:inDataset rdf:resource="#datasetdefinition"/>
  <gs1:netContent>
   <gs1:QuantitativeValue rdf:about="#16xbottle600ml-Content">
   <rdf:type rdf:resource="http://qudt.org/1.1/schema/qudt#QuantityValue"/>
   <qudt:unit rdf:resource="http://www.qudt.org/2.1/vocab/unit/MilliL"/>
   <qudt:numericalValue rdf:datatype="http://www.w3.org/2001/XMLSchema#double">9600</qudt:numericalValue>
   <rdf:value rdf:datatype="http://www.w3.org/2001/XMLSchema#double">9600</rdf:value>
   <gs1:unitCode>MLT</gs1:unitCode>
   <gs1:value>9600</gs1:value>
  </gs1:QuantitativeValue>
 </gs1:netContent>
 <sosa:isFeatureOfInterestOf>
  <rdf:Description rdf:about="#16xbottle600ml-ContentSosa">
   <rdf:type rdf:resource="http://www.w3.org/ns/sosa/Observation"/>
   <sosa:hasFeatureOfInterest rdf:resource="#16xbottle600ml"/>
   <sosa:observedProperty  rdf:resource="#netcontent"/>
   <sosa:hasResult rdf:resource="#16xbottle600ml-Content"/>
   <sosa:hasSimpleResult rdf:datatype="http://www.qudt.org/2.1/vocab/unit/MilliM">9600</sosa:hasSimpleResult>
  </rdf:Description>
 </sosa:isFeatureOfInterestOf>
 </rdf:Description>

 <rdf:Description rdf:about="#8xbottle600ml">
  <rdf:type rdf:resource="#LiquidContainer"/>
  <rdf:type rdf:resource="#BeverageBottle"/>
  <rdf:type rdf:resource="https://gs1.org/voc/PackagingDetails"/>
  <rdfs:label xml:lang="en">8XBottle600ml</rdfs:label>
  <rdfs:label xml:lang="fr">8XBottle600ml</rdfs:label>
  <skos:definition xml:lang="en">Generic Flat, Box or Crate of 8, 600ml Bottles</skos:definition>
  <skos:definition xml:lang="fr">Une boite, caisse ou caissette générique de 8 Bouteilles de 600ml</skos:definition>
  <rdfs:comment xml:lang="en">This term is meant to be used as a placeholder when no data about the aggregate packaging is known.</rdfs:comment>
  <rdfs:comment xml:lang="fr">Ce terme peut-être utilisé comme un terme générique lorsque les details de l’emballage ne sont pas certain.</rdfs:comment>
  <beer:count rdf:datatype="http://www.w3.org/2001/XMLSchema#Integer">8</beer:count>
  <beer:item rdf:resource="https://rdf.ag/o/beer#bottle600ml"/>
  <rdfs:isDefinedBy rdf:resource="https://rdf.ag/o/beer-ONTOLOGY_DATE"/>
  <void:inDataset rdf:resource="#datasetdefinition"/>
  <gs1:netContent>
   <gs1:QuantitativeValue rdf:about="#8xbottle600ml-Content">
   <rdf:type rdf:resource="http://qudt.org/1.1/schema/qudt#QuantityValue"/>
   <qudt:unit rdf:resource="http://www.qudt.org/2.1/vocab/unit/MilliL"/>
   <qudt:numericalValue rdf:datatype="http://www.w3.org/2001/XMLSchema#double">4800</qudt:numericalValue>
   <rdf:value rdf:datatype="http://www.w3.org/2001/XMLSchema#double">4800</rdf:value>
   <gs1:unitCode>MLT</gs1:unitCode>
   <gs1:value>4800</gs1:value>
  </gs1:QuantitativeValue>
 </gs1:netContent>
 <sosa:isFeatureOfInterestOf>
  <rdf:Description rdf:about="#8xbottle600ml-ContentSosa">
   <rdf:type rdf:resource="http://www.w3.org/ns/sosa/Observation"/>
   <sosa:hasFeatureOfInterest rdf:resource="#8xbottle600ml"/>
   <sosa:observedProperty  rdf:resource="#netcontent"/>
   <sosa:hasResult rdf:resource="#8xbottle600ml-Content"/>
   <sosa:hasSimpleResult rdf:datatype="http://www.qudt.org/2.1/vocab/unit/MilliM">4800</sosa:hasSimpleResult>
  </rdf:Description>
 </sosa:isFeatureOfInterestOf>
 </rdf:Description>

 <rdf:Description rdf:about="#12xbottle710ml">
  <rdf:type rdf:resource="#LiquidContainer"/>
  <rdf:type rdf:resource="#BeverageBottle"/>
  <rdf:type rdf:resource="https://gs1.org/voc/PackagingDetails"/>
  <rdfs:label xml:lang="en">12XBottle710ml</rdfs:label>
  <rdfs:label xml:lang="fr">12XBottle710ml</rdfs:label>
  <skos:definition xml:lang="en">Generic Flat, Box or Crate of 12, 710ml Bottles</skos:definition>
  <skos:definition xml:lang="fr">Une boite, caisse ou caissette générique de 12 Bouteilles de 710ml</skos:definition>
  <rdfs:comment xml:lang="en">This term is meant to be used as a placeholder when no data about the aggregate packaging is known.</rdfs:comment>
  <rdfs:comment xml:lang="fr">Ce terme peut-être utilisé comme un terme générique lorsque les details de l’emballage ne sont pas certain.</rdfs:comment>
  <beer:count rdf:datatype="http://www.w3.org/2001/XMLSchema#Integer">12</beer:count>
  <beer:item rdf:resource="https://rdf.ag/o/beer#bottle710ml"/>
  <rdfs:isDefinedBy rdf:resource="https://rdf.ag/o/beer-ONTOLOGY_DATE"/>
  <void:inDataset rdf:resource="#datasetdefinition"/>
  <gs1:netContent>
   <gs1:QuantitativeValue rdf:about="#12xbottle710ml-Content">
   <rdf:type rdf:resource="http://qudt.org/1.1/schema/qudt#QuantityValue"/>
   <qudt:unit rdf:resource="http://www.qudt.org/2.1/vocab/unit/MilliL"/>
   <qudt:numericalValue rdf:datatype="http://www.w3.org/2001/XMLSchema#double">8520</qudt:numericalValue>
   <rdf:value rdf:datatype="http://www.w3.org/2001/XMLSchema#double">8520</rdf:value>
   <gs1:unitCode>MLT</gs1:unitCode>
   <gs1:value>8520</gs1:value>
  </gs1:QuantitativeValue>
 </gs1:netContent>
 <sosa:isFeatureOfInterestOf>
  <rdf:Description rdf:about="#12xbottle710ml-ContentSosa">
   <rdf:type rdf:resource="http://www.w3.org/ns/sosa/Observation"/>
   <sosa:hasFeatureOfInterest rdf:resource="#12xbottle710ml"/>
   <sosa:observedProperty  rdf:resource="#netcontent"/>
   <sosa:hasResult rdf:resource="#12xbottle710ml-Content"/>
   <sosa:hasSimpleResult rdf:datatype="http://www.qudt.org/2.1/vocab/unit/MilliM">8520</sosa:hasSimpleResult>
  </rdf:Description>
 </sosa:isFeatureOfInterestOf>
 </rdf:Description>

 <rdf:Description rdf:about="#2xcan710ml">
  <rdf:type rdf:resource="#LiquidContainer"/>
  <rdf:type rdf:resource="#BeverageCan"/>
  <rdf:type rdf:resource="https://gs1.org/voc/PackagingDetails"/>
  <rdfs:label xml:lang="en">2XCan710ml</rdfs:label>
  <rdfs:label xml:lang="fr">2XCan710ml</rdfs:label>
  <skos:definition xml:lang="en">Generic Flat, Box or Crate of 2, 710ml Cans</skos:definition>
  <skos:definition xml:lang="fr">Une boite, caisse ou caissette générique de 2 Canettes de 710ml</skos:definition>
  <rdfs:comment xml:lang="en">This term is meant to be used as a placeholder when no data about the aggregate packaging is known.</rdfs:comment>
  <rdfs:comment xml:lang="fr">Ce terme peut-être utilisé comme un terme générique lorsque les details de l’emballage ne sont pas certain.</rdfs:comment>
  <beer:count rdf:datatype="http://www.w3.org/2001/XMLSchema#Integer">2</beer:count>
  <beer:item rdf:resource="https://rdf.ag/o/beer#can710ml"/>
  <rdfs:isDefinedBy rdf:resource="https://rdf.ag/o/beer-ONTOLOGY_DATE"/>
  <void:inDataset rdf:resource="#datasetdefinition"/>
  <gs1:netContent>
   <gs1:QuantitativeValue rdf:about="#2xcan710ml-Content">
   <rdf:type rdf:resource="http://qudt.org/1.1/schema/qudt#QuantityValue"/>
   <qudt:unit rdf:resource="http://www.qudt.org/2.1/vocab/unit/MilliL"/>
   <qudt:numericalValue rdf:datatype="http://www.w3.org/2001/XMLSchema#double">1420</qudt:numericalValue>
   <rdf:value rdf:datatype="http://www.w3.org/2001/XMLSchema#double">1420</rdf:value>
   <gs1:unitCode>MLT</gs1:unitCode>
   <gs1:value>1420</gs1:value>
  </gs1:QuantitativeValue>
 </gs1:netContent>
 <sosa:isFeatureOfInterestOf>
  <rdf:Description rdf:about="#2xcan710ml-ContentSosa">
   <rdf:type rdf:resource="http://www.w3.org/ns/sosa/Observation"/>
   <sosa:hasFeatureOfInterest rdf:resource="#2xcan710ml"/>
   <sosa:observedProperty  rdf:resource="#netcontent"/>
   <sosa:hasResult rdf:resource="#2xcan710ml-Content"/>
   <sosa:hasSimpleResult rdf:datatype="http://www.qudt.org/2.1/vocab/unit/MilliM">1420</sosa:hasSimpleResult>
  </rdf:Description>
 </sosa:isFeatureOfInterestOf>
 </rdf:Description>

 <rdf:Description rdf:about="#12xcan710ml">
  <rdf:type rdf:resource="#LiquidContainer"/>
  <rdf:type rdf:resource="#BeverageCan"/>
  <rdf:type rdf:resource="https://gs1.org/voc/PackagingDetails"/>
  <rdfs:label xml:lang="en">12XCan710ml</rdfs:label>
  <rdfs:label xml:lang="fr">12XCan710ml</rdfs:label>
  <skos:definition xml:lang="en">Generic Flat, Box or Crate of 12, 710ml Cans</skos:definition>
  <skos:definition xml:lang="fr">Une boite, caisse ou caissette générique de 12 Canettes de 710ml</skos:definition>
  <rdfs:comment xml:lang="en">This term is meant to be used as a placeholder when no data about the aggregate packaging is known.</rdfs:comment>
  <rdfs:comment xml:lang="fr">Ce terme peut-être utilisé comme un terme générique lorsque les details de l’emballage ne sont pas certain.</rdfs:comment>
  <beer:count rdf:datatype="http://www.w3.org/2001/XMLSchema#Integer">12</beer:count>
  <beer:item rdf:resource="https://rdf.ag/o/beer#can710ml"/>
  <rdfs:isDefinedBy rdf:resource="https://rdf.ag/o/beer-ONTOLOGY_DATE"/>
  <void:inDataset rdf:resource="#datasetdefinition"/>
  <gs1:netContent>
   <gs1:QuantitativeValue rdf:about="#12xcan710ml-Content">
   <rdf:type rdf:resource="http://qudt.org/1.1/schema/qudt#QuantityValue"/>
   <qudt:unit rdf:resource="http://www.qudt.org/2.1/vocab/unit/MilliL"/>
   <qudt:numericalValue rdf:datatype="http://www.w3.org/2001/XMLSchema#double">8520</qudt:numericalValue>
   <rdf:value rdf:datatype="http://www.w3.org/2001/XMLSchema#double">8520</rdf:value>
   <gs1:unitCode>MLT</gs1:unitCode>
   <gs1:value>8520</gs1:value>
  </gs1:QuantitativeValue>
 </gs1:netContent>
 <sosa:isFeatureOfInterestOf>
  <rdf:Description rdf:about="#12xcan710ml-ContentSosa">
   <rdf:type rdf:resource="http://www.w3.org/ns/sosa/Observation"/>
   <sosa:hasFeatureOfInterest rdf:resource="#12xcan710ml"/>
   <sosa:observedProperty  rdf:resource="#netcontent"/>
   <sosa:hasResult rdf:resource="#12xcan710ml-Content"/>
   <sosa:hasSimpleResult rdf:datatype="http://www.qudt.org/2.1/vocab/unit/MilliM">8520</sosa:hasSimpleResult>
  </rdf:Description>
 </sosa:isFeatureOfInterestOf>
 </rdf:Description>

 <rdf:Description rdf:about="#4xcan710ml">
  <rdf:type rdf:resource="#LiquidContainer"/>
  <rdf:type rdf:resource="#BeverageCan"/>
  <rdf:type rdf:resource="https://gs1.org/voc/PackagingDetails"/>
  <rdfs:label xml:lang="en">4XCan710ml</rdfs:label>
  <rdfs:label xml:lang="fr">4XCan710ml</rdfs:label>
  <skos:definition xml:lang="en">Generic Flat, Box or Crate of 4, 710ml Cans</skos:definition>
  <skos:definition xml:lang="fr">Une boite, caisse ou caissette générique de 4 Canettes de 710ml</skos:definition>
  <rdfs:comment xml:lang="en">This term is meant to be used as a placeholder when no data about the aggregate packaging is known.</rdfs:comment>
  <rdfs:comment xml:lang="fr">Ce terme peut-être utilisé comme un terme générique lorsque les details de l’emballage ne sont pas certain.</rdfs:comment>
  <beer:count rdf:datatype="http://www.w3.org/2001/XMLSchema#Integer">4</beer:count>
  <beer:item rdf:resource="https://rdf.ag/o/beer#can710ml"/>
  <rdfs:isDefinedBy rdf:resource="https://rdf.ag/o/beer-ONTOLOGY_DATE"/>
  <void:inDataset rdf:resource="#datasetdefinition"/>
  <gs1:netContent>
   <gs1:QuantitativeValue rdf:about="#4xcan710ml-Content">
   <rdf:type rdf:resource="http://qudt.org/1.1/schema/qudt#QuantityValue"/>
   <qudt:unit rdf:resource="http://www.qudt.org/2.1/vocab/unit/MilliL"/>
   <qudt:numericalValue rdf:datatype="http://www.w3.org/2001/XMLSchema#double">2840</qudt:numericalValue>
   <rdf:value rdf:datatype="http://www.w3.org/2001/XMLSchema#double">2840</rdf:value>
   <gs1:unitCode>MLT</gs1:unitCode>
   <gs1:value>2840</gs1:value>
  </gs1:QuantitativeValue>
 </gs1:netContent>
 <sosa:isFeatureOfInterestOf>
  <rdf:Description rdf:about="#4xcan710ml-ContentSosa">
   <rdf:type rdf:resource="http://www.w3.org/ns/sosa/Observation"/>
   <sosa:hasFeatureOfInterest rdf:resource="#4xcan710ml"/>
   <sosa:observedProperty  rdf:resource="#netcontent"/>
   <sosa:hasResult rdf:resource="#4xcan710ml-Content"/>
   <sosa:hasSimpleResult rdf:datatype="http://www.qudt.org/2.1/vocab/unit/MilliM">2840</sosa:hasSimpleResult>
  </rdf:Description>
 </sosa:isFeatureOfInterestOf>
 </rdf:Description>

 <rdf:Description rdf:about="#24xcan710ml">
  <rdf:type rdf:resource="#LiquidContainer"/>
  <rdf:type rdf:resource="#BeverageCan"/>
  <rdf:type rdf:resource="https://gs1.org/voc/PackagingDetails"/>
  <rdfs:label xml:lang="en">24XCan710ml</rdfs:label>
  <rdfs:label xml:lang="fr">24XCan710ml</rdfs:label>
  <skos:definition xml:lang="en">Generic Flat, Box or Crate of 24, 710ml Cans</skos:definition>
  <skos:definition xml:lang="fr">Une boite, caisse ou caissette générique de 24 Canettes de 710ml</skos:definition>
  <rdfs:comment xml:lang="en">This term is meant to be used as a placeholder when no data about the aggregate packaging is known.</rdfs:comment>
  <rdfs:comment xml:lang="fr">Ce terme peut-être utilisé comme un terme générique lorsque les details de l’emballage ne sont pas certain.</rdfs:comment>
  <beer:count rdf:datatype="http://www.w3.org/2001/XMLSchema#Integer">24</beer:count>
  <beer:item rdf:resource="https://rdf.ag/o/beer#can710ml"/>
  <rdfs:isDefinedBy rdf:resource="https://rdf.ag/o/beer-ONTOLOGY_DATE"/>
  <void:inDataset rdf:resource="#datasetdefinition"/>
  <gs1:netContent>
   <gs1:QuantitativeValue rdf:about="#24xcan710ml-Content">
   <rdf:type rdf:resource="http://qudt.org/1.1/schema/qudt#QuantityValue"/>
   <qudt:unit rdf:resource="http://www.qudt.org/2.1/vocab/unit/MilliL"/>
   <qudt:numericalValue rdf:datatype="http://www.w3.org/2001/XMLSchema#double">17040</qudt:numericalValue>
   <rdf:value rdf:datatype="http://www.w3.org/2001/XMLSchema#double">17040</rdf:value>
   <gs1:unitCode>MLT</gs1:unitCode>
   <gs1:value>17040</gs1:value>
  </gs1:QuantitativeValue>
 </gs1:netContent>
 <sosa:isFeatureOfInterestOf>
  <rdf:Description rdf:about="#24xcan710ml-ContentSosa">
   <rdf:type rdf:resource="http://www.w3.org/ns/sosa/Observation"/>
   <sosa:hasFeatureOfInterest rdf:resource="#24xcan710ml"/>
   <sosa:observedProperty  rdf:resource="#netcontent"/>
   <sosa:hasResult rdf:resource="#24xcan710ml-Content"/>
   <sosa:hasSimpleResult rdf:datatype="http://www.qudt.org/2.1/vocab/unit/MilliM">17040</sosa:hasSimpleResult>
  </rdf:Description>
 </sosa:isFeatureOfInterestOf>
 </rdf:Description>

 <rdf:Description rdf:about="#6xcan710ml">
  <rdf:type rdf:resource="#LiquidContainer"/>
  <rdf:type rdf:resource="#BeverageCan"/>
  <rdf:type rdf:resource="https://gs1.org/voc/PackagingDetails"/>
  <rdfs:label xml:lang="en">6XCan710ml</rdfs:label>
  <rdfs:label xml:lang="fr">6XCan710ml</rdfs:label>
  <skos:definition xml:lang="en">Generic Flat, Box or Crate of 6, 710ml Cans</skos:definition>
  <skos:definition xml:lang="fr">Une boite, caisse ou caissette générique de 6 Canettes de 710ml</skos:definition>
  <rdfs:comment xml:lang="en">This term is meant to be used as a placeholder when no data about the aggregate packaging is known.</rdfs:comment>
  <rdfs:comment xml:lang="fr">Ce terme peut-être utilisé comme un terme générique lorsque les details de l’emballage ne sont pas certain.</rdfs:comment>
  <beer:count rdf:datatype="http://www.w3.org/2001/XMLSchema#Integer">6</beer:count>
  <beer:item rdf:resource="https://rdf.ag/o/beer#can710ml"/>
  <rdfs:isDefinedBy rdf:resource="https://rdf.ag/o/beer-ONTOLOGY_DATE"/>
  <void:inDataset rdf:resource="#datasetdefinition"/>
  <gs1:netContent>
   <gs1:QuantitativeValue rdf:about="#6xcan710ml-Content">
   <rdf:type rdf:resource="http://qudt.org/1.1/schema/qudt#QuantityValue"/>
   <qudt:unit rdf:resource="http://www.qudt.org/2.1/vocab/unit/MilliL"/>
   <qudt:numericalValue rdf:datatype="http://www.w3.org/2001/XMLSchema#double">4260</qudt:numericalValue>
   <rdf:value rdf:datatype="http://www.w3.org/2001/XMLSchema#double">4260</rdf:value>
   <gs1:unitCode>MLT</gs1:unitCode>
   <gs1:value>4260</gs1:value>
  </gs1:QuantitativeValue>
 </gs1:netContent>
 <sosa:isFeatureOfInterestOf>
  <rdf:Description rdf:about="#6xcan710ml-ContentSosa">
   <rdf:type rdf:resource="http://www.w3.org/ns/sosa/Observation"/>
   <sosa:hasFeatureOfInterest rdf:resource="#6xcan710ml"/>
   <sosa:observedProperty  rdf:resource="#netcontent"/>
   <sosa:hasResult rdf:resource="#6xcan710ml-Content"/>
   <sosa:hasSimpleResult rdf:datatype="http://www.qudt.org/2.1/vocab/unit/MilliM">4260</sosa:hasSimpleResult>
  </rdf:Description>
 </sosa:isFeatureOfInterestOf>
 </rdf:Description>

 <rdf:Description rdf:about="#12xbottle330ml">
  <rdf:type rdf:resource="#LiquidContainer"/>
  <rdf:type rdf:resource="#BeverageBottle"/>
  <rdf:type rdf:resource="https://gs1.org/voc/PackagingDetails"/>
  <rdfs:label xml:lang="en">12XBottle330ml</rdfs:label>
  <rdfs:label xml:lang="fr">12XBottle330ml</rdfs:label>
  <skos:definition xml:lang="en">Generic Flat, Box or Crate of 12, 330ml Bottles</skos:definition>
  <skos:definition xml:lang="fr">Une boite, caisse ou caissette générique de 12 Bouteilles de 330ml</skos:definition>
  <rdfs:comment xml:lang="en">This term is meant to be used as a placeholder when no data about the aggregate packaging is known.</rdfs:comment>
  <rdfs:comment xml:lang="fr">Ce terme peut-être utilisé comme un terme générique lorsque les details de l’emballage ne sont pas certain.</rdfs:comment>
  <beer:count rdf:datatype="http://www.w3.org/2001/XMLSchema#Integer">12</beer:count>
  <beer:item rdf:resource="https://rdf.ag/o/beer#bottle330ml"/>
  <rdfs:isDefinedBy rdf:resource="https://rdf.ag/o/beer-ONTOLOGY_DATE"/>
  <void:inDataset rdf:resource="#datasetdefinition"/>
  <gs1:netContent>
   <gs1:QuantitativeValue rdf:about="#12xbottle330ml-Content">
   <rdf:type rdf:resource="http://qudt.org/1.1/schema/qudt#QuantityValue"/>
   <qudt:unit rdf:resource="http://www.qudt.org/2.1/vocab/unit/MilliL"/>
   <qudt:numericalValue rdf:datatype="http://www.w3.org/2001/XMLSchema#double">3960</qudt:numericalValue>
   <rdf:value rdf:datatype="http://www.w3.org/2001/XMLSchema#double">3960</rdf:value>
   <gs1:unitCode>MLT</gs1:unitCode>
   <gs1:value>3960</gs1:value>
  </gs1:QuantitativeValue>
 </gs1:netContent>
 <sosa:isFeatureOfInterestOf>
  <rdf:Description rdf:about="#12xbottle330ml-ContentSosa">
   <rdf:type rdf:resource="http://www.w3.org/ns/sosa/Observation"/>
   <sosa:hasFeatureOfInterest rdf:resource="#12xbottle330ml"/>
   <sosa:observedProperty  rdf:resource="#netcontent"/>
   <sosa:hasResult rdf:resource="#12xbottle330ml-Content"/>
   <sosa:hasSimpleResult rdf:datatype="http://www.qudt.org/2.1/vocab/unit/MilliM">3960</sosa:hasSimpleResult>
  </rdf:Description>
 </sosa:isFeatureOfInterestOf>
 </rdf:Description>

 <rdf:Description rdf:about="#4xbottle330ml">
  <rdf:type rdf:resource="#LiquidContainer"/>
  <rdf:type rdf:resource="#BeverageBottle"/>
  <rdf:type rdf:resource="https://gs1.org/voc/PackagingDetails"/>
  <rdfs:label xml:lang="en">4XBottle330ml</rdfs:label>
  <rdfs:label xml:lang="fr">4XBottle330ml</rdfs:label>
  <skos:definition xml:lang="en">Generic Flat, Box or Crate of 4, 330ml Bottles</skos:definition>
  <skos:definition xml:lang="fr">Une boite, caisse ou caissette générique de 4 Bouteilles de 330ml</skos:definition>
  <rdfs:comment xml:lang="en">This term is meant to be used as a placeholder when no data about the aggregate packaging is known.</rdfs:comment>
  <rdfs:comment xml:lang="fr">Ce terme peut-être utilisé comme un terme générique lorsque les details de l’emballage ne sont pas certain.</rdfs:comment>
  <beer:count rdf:datatype="http://www.w3.org/2001/XMLSchema#Integer">4</beer:count>
  <beer:item rdf:resource="https://rdf.ag/o/beer#bottle330ml"/>
  <rdfs:isDefinedBy rdf:resource="https://rdf.ag/o/beer-ONTOLOGY_DATE"/>
  <void:inDataset rdf:resource="#datasetdefinition"/>
  <gs1:netContent>
   <gs1:QuantitativeValue rdf:about="#4xbottle330ml-Content">
   <rdf:type rdf:resource="http://qudt.org/1.1/schema/qudt#QuantityValue"/>
   <qudt:unit rdf:resource="http://www.qudt.org/2.1/vocab/unit/MilliL"/>
   <qudt:numericalValue rdf:datatype="http://www.w3.org/2001/XMLSchema#double">1320</qudt:numericalValue>
   <rdf:value rdf:datatype="http://www.w3.org/2001/XMLSchema#double">1320</rdf:value>
   <gs1:unitCode>MLT</gs1:unitCode>
   <gs1:value>1320</gs1:value>
  </gs1:QuantitativeValue>
 </gs1:netContent>
 <sosa:isFeatureOfInterestOf>
  <rdf:Description rdf:about="#4xbottle330ml-ContentSosa">
   <rdf:type rdf:resource="http://www.w3.org/ns/sosa/Observation"/>
   <sosa:hasFeatureOfInterest rdf:resource="#4xbottle330ml"/>
   <sosa:observedProperty  rdf:resource="#netcontent"/>
   <sosa:hasResult rdf:resource="#4xbottle330ml-Content"/>
   <sosa:hasSimpleResult rdf:datatype="http://www.qudt.org/2.1/vocab/unit/MilliM">1320</sosa:hasSimpleResult>
  </rdf:Description>
 </sosa:isFeatureOfInterestOf>
 </rdf:Description>

 <rdf:Description rdf:about="#24xbottle330ml">
  <rdf:type rdf:resource="#LiquidContainer"/>
  <rdf:type rdf:resource="#BeverageBottle"/>
  <rdf:type rdf:resource="https://gs1.org/voc/PackagingDetails"/>
  <rdfs:label xml:lang="en">24XBottle330ml</rdfs:label>
  <rdfs:label xml:lang="fr">24XBottle330ml</rdfs:label>
  <skos:definition xml:lang="en">Generic Flat, Box or Crate of 24, 330ml Bottles</skos:definition>
  <skos:definition xml:lang="fr">Une boite, caisse ou caissette générique de 24 Bouteilles de 330ml</skos:definition>
  <rdfs:comment xml:lang="en">This term is meant to be used as a placeholder when no data about the aggregate packaging is known.</rdfs:comment>
  <rdfs:comment xml:lang="fr">Ce terme peut-être utilisé comme un terme générique lorsque les details de l’emballage ne sont pas certain.</rdfs:comment>
  <beer:count rdf:datatype="http://www.w3.org/2001/XMLSchema#Integer">24</beer:count>
  <beer:item rdf:resource="https://rdf.ag/o/beer#bottle330ml"/>
  <rdfs:isDefinedBy rdf:resource="https://rdf.ag/o/beer-ONTOLOGY_DATE"/>
  <void:inDataset rdf:resource="#datasetdefinition"/>
  <gs1:netContent>
   <gs1:QuantitativeValue rdf:about="#24xbottle330ml-Content">
   <rdf:type rdf:resource="http://qudt.org/1.1/schema/qudt#QuantityValue"/>
   <qudt:unit rdf:resource="http://www.qudt.org/2.1/vocab/unit/MilliL"/>
   <qudt:numericalValue rdf:datatype="http://www.w3.org/2001/XMLSchema#double">7920</qudt:numericalValue>
   <rdf:value rdf:datatype="http://www.w3.org/2001/XMLSchema#double">7920</rdf:value>
   <gs1:unitCode>MLT</gs1:unitCode>
   <gs1:value>7920</gs1:value>
  </gs1:QuantitativeValue>
 </gs1:netContent>
 <sosa:isFeatureOfInterestOf>
  <rdf:Description rdf:about="#24xbottle330ml-ContentSosa">
   <rdf:type rdf:resource="http://www.w3.org/ns/sosa/Observation"/>
   <sosa:hasFeatureOfInterest rdf:resource="#24xbottle330ml"/>
   <sosa:observedProperty  rdf:resource="#netcontent"/>
   <sosa:hasResult rdf:resource="#24xbottle330ml-Content"/>
   <sosa:hasSimpleResult rdf:datatype="http://www.qudt.org/2.1/vocab/unit/MilliM">7920</sosa:hasSimpleResult>
  </rdf:Description>
 </sosa:isFeatureOfInterestOf>
 </rdf:Description>

 <rdf:Description rdf:about="#6xbottle330ml">
  <rdf:type rdf:resource="#LiquidContainer"/>
  <rdf:type rdf:resource="#BeverageBottle"/>
  <rdf:type rdf:resource="https://gs1.org/voc/PackagingDetails"/>
  <rdfs:label xml:lang="en">6XBottle330ml</rdfs:label>
  <rdfs:label xml:lang="fr">6XBottle330ml</rdfs:label>
  <skos:definition xml:lang="en">Generic Flat, Box or Crate of 6, 330ml Bottles</skos:definition>
  <skos:definition xml:lang="fr">Une boite, caisse ou caissette générique de 6 Bouteilles de 330ml</skos:definition>
  <rdfs:comment xml:lang="en">This term is meant to be used as a placeholder when no data about the aggregate packaging is known.</rdfs:comment>
  <rdfs:comment xml:lang="fr">Ce terme peut-être utilisé comme un terme générique lorsque les details de l’emballage ne sont pas certain.</rdfs:comment>
  <beer:count rdf:datatype="http://www.w3.org/2001/XMLSchema#Integer">6</beer:count>
  <beer:item rdf:resource="https://rdf.ag/o/beer#bottle330ml"/>
  <rdfs:isDefinedBy rdf:resource="https://rdf.ag/o/beer-ONTOLOGY_DATE"/>
  <void:inDataset rdf:resource="#datasetdefinition"/>
  <gs1:netContent>
   <gs1:QuantitativeValue rdf:about="#6xbottle330ml-Content">
   <rdf:type rdf:resource="http://qudt.org/1.1/schema/qudt#QuantityValue"/>
   <qudt:unit rdf:resource="http://www.qudt.org/2.1/vocab/unit/MilliL"/>
   <qudt:numericalValue rdf:datatype="http://www.w3.org/2001/XMLSchema#double">1980</qudt:numericalValue>
   <rdf:value rdf:datatype="http://www.w3.org/2001/XMLSchema#double">1980</rdf:value>
   <gs1:unitCode>MLT</gs1:unitCode>
   <gs1:value>1980</gs1:value>
  </gs1:QuantitativeValue>
 </gs1:netContent>
 <sosa:isFeatureOfInterestOf>
  <rdf:Description rdf:about="#6xbottle330ml-ContentSosa">
   <rdf:type rdf:resource="http://www.w3.org/ns/sosa/Observation"/>
   <sosa:hasFeatureOfInterest rdf:resource="#6xbottle330ml"/>
   <sosa:observedProperty  rdf:resource="#netcontent"/>
   <sosa:hasResult rdf:resource="#6xbottle330ml-Content"/>
   <sosa:hasSimpleResult rdf:datatype="http://www.qudt.org/2.1/vocab/unit/MilliM">1980</sosa:hasSimpleResult>
  </rdf:Description>
 </sosa:isFeatureOfInterestOf>
 </rdf:Description>

 <rdf:Description rdf:about="#36xbottle330ml">
  <rdf:type rdf:resource="#LiquidContainer"/>
  <rdf:type rdf:resource="#BeverageBottle"/>
  <rdf:type rdf:resource="https://gs1.org/voc/PackagingDetails"/>
  <rdfs:label xml:lang="en">36XBottle330ml</rdfs:label>
  <rdfs:label xml:lang="fr">36XBottle330ml</rdfs:label>
  <skos:definition xml:lang="en">Generic Flat, Box or Crate of 36, 330ml Bottles</skos:definition>
  <skos:definition xml:lang="fr">Une boite, caisse ou caissette générique de 36 Bouteilles de 330ml</skos:definition>
  <rdfs:comment xml:lang="en">This term is meant to be used as a placeholder when no data about the aggregate packaging is known.</rdfs:comment>
  <rdfs:comment xml:lang="fr">Ce terme peut-être utilisé comme un terme générique lorsque les details de l’emballage ne sont pas certain.</rdfs:comment>
  <beer:count rdf:datatype="http://www.w3.org/2001/XMLSchema#Integer">36</beer:count>
  <beer:item rdf:resource="https://rdf.ag/o/beer#bottle330ml"/>
  <rdfs:isDefinedBy rdf:resource="https://rdf.ag/o/beer-ONTOLOGY_DATE"/>
  <void:inDataset rdf:resource="#datasetdefinition"/>
  <gs1:netContent>
   <gs1:QuantitativeValue rdf:about="#36xbottle330ml-Content">
   <rdf:type rdf:resource="http://qudt.org/1.1/schema/qudt#QuantityValue"/>
   <qudt:unit rdf:resource="http://www.qudt.org/2.1/vocab/unit/MilliL"/>
   <qudt:numericalValue rdf:datatype="http://www.w3.org/2001/XMLSchema#double">11880</qudt:numericalValue>
   <rdf:value rdf:datatype="http://www.w3.org/2001/XMLSchema#double">11880</rdf:value>
   <gs1:unitCode>MLT</gs1:unitCode>
   <gs1:value>11880</gs1:value>
  </gs1:QuantitativeValue>
 </gs1:netContent>
 <sosa:isFeatureOfInterestOf>
  <rdf:Description rdf:about="#36xbottle330ml-ContentSosa">
   <rdf:type rdf:resource="http://www.w3.org/ns/sosa/Observation"/>
   <sosa:hasFeatureOfInterest rdf:resource="#36xbottle330ml"/>
   <sosa:observedProperty  rdf:resource="#netcontent"/>
   <sosa:hasResult rdf:resource="#36xbottle330ml-Content"/>
   <sosa:hasSimpleResult rdf:datatype="http://www.qudt.org/2.1/vocab/unit/MilliM">11880</sosa:hasSimpleResult>
  </rdf:Description>
 </sosa:isFeatureOfInterestOf>
 </rdf:Description>

 <rdf:Description rdf:about="#8xbottle330ml">
  <rdf:type rdf:resource="#LiquidContainer"/>
  <rdf:type rdf:resource="#BeverageBottle"/>
  <rdf:type rdf:resource="https://gs1.org/voc/PackagingDetails"/>
  <rdfs:label xml:lang="en">8XBottle330ml</rdfs:label>
  <rdfs:label xml:lang="fr">8XBottle330ml</rdfs:label>
  <skos:definition xml:lang="en">Generic Flat, Box or Crate of 8, 330ml Bottles</skos:definition>
  <skos:definition xml:lang="fr">Une boite, caisse ou caissette générique de 8 Bouteilles de 330ml</skos:definition>
  <rdfs:comment xml:lang="en">This term is meant to be used as a placeholder when no data about the aggregate packaging is known.</rdfs:comment>
  <rdfs:comment xml:lang="fr">Ce terme peut-être utilisé comme un terme générique lorsque les details de l’emballage ne sont pas certain.</rdfs:comment>
  <beer:count rdf:datatype="http://www.w3.org/2001/XMLSchema#Integer">8</beer:count>
  <beer:item rdf:resource="https://rdf.ag/o/beer#bottle330ml"/>
  <rdfs:isDefinedBy rdf:resource="https://rdf.ag/o/beer-ONTOLOGY_DATE"/>
  <void:inDataset rdf:resource="#datasetdefinition"/>
  <gs1:netContent>
   <gs1:QuantitativeValue rdf:about="#8xbottle330ml-Content">
   <rdf:type rdf:resource="http://qudt.org/1.1/schema/qudt#QuantityValue"/>
   <qudt:unit rdf:resource="http://www.qudt.org/2.1/vocab/unit/MilliL"/>
   <qudt:numericalValue rdf:datatype="http://www.w3.org/2001/XMLSchema#double">2640</qudt:numericalValue>
   <rdf:value rdf:datatype="http://www.w3.org/2001/XMLSchema#double">2640</rdf:value>
   <gs1:unitCode>MLT</gs1:unitCode>
   <gs1:value>2640</gs1:value>
  </gs1:QuantitativeValue>
 </gs1:netContent>
 <sosa:isFeatureOfInterestOf>
  <rdf:Description rdf:about="#8xbottle330ml-ContentSosa">
   <rdf:type rdf:resource="http://www.w3.org/ns/sosa/Observation"/>
   <sosa:hasFeatureOfInterest rdf:resource="#8xbottle330ml"/>
   <sosa:observedProperty  rdf:resource="#netcontent"/>
   <sosa:hasResult rdf:resource="#8xbottle330ml-Content"/>
   <sosa:hasSimpleResult rdf:datatype="http://www.qudt.org/2.1/vocab/unit/MilliM">2640</sosa:hasSimpleResult>
  </rdf:Description>
 </sosa:isFeatureOfInterestOf>
 </rdf:Description>

 <rdf:Description rdf:about="#18xbottle330ml">
  <rdf:type rdf:resource="#LiquidContainer"/>
  <rdf:type rdf:resource="#BeverageBottle"/>
  <rdf:type rdf:resource="https://gs1.org/voc/PackagingDetails"/>
  <rdfs:label xml:lang="en">18XBottle330ml</rdfs:label>
  <rdfs:label xml:lang="fr">18XBottle330ml</rdfs:label>
  <skos:definition xml:lang="en">Generic Flat, Box or Crate of 18, 330ml Bottles</skos:definition>
  <skos:definition xml:lang="fr">Une boite, caisse ou caissette générique de 18 Bouteilles de 330ml</skos:definition>
  <rdfs:comment xml:lang="en">This term is meant to be used as a placeholder when no data about the aggregate packaging is known.</rdfs:comment>
  <rdfs:comment xml:lang="fr">Ce terme peut-être utilisé comme un terme générique lorsque les details de l’emballage ne sont pas certain.</rdfs:comment>
  <beer:count rdf:datatype="http://www.w3.org/2001/XMLSchema#Integer">18</beer:count>
  <beer:item rdf:resource="https://rdf.ag/o/beer#bottle330ml"/>
  <rdfs:isDefinedBy rdf:resource="https://rdf.ag/o/beer-ONTOLOGY_DATE"/>
  <void:inDataset rdf:resource="#datasetdefinition"/>
  <gs1:netContent>
   <gs1:QuantitativeValue rdf:about="#18xbottle330ml-Content">
   <rdf:type rdf:resource="http://qudt.org/1.1/schema/qudt#QuantityValue"/>
   <qudt:unit rdf:resource="http://www.qudt.org/2.1/vocab/unit/MilliL"/>
   <qudt:numericalValue rdf:datatype="http://www.w3.org/2001/XMLSchema#double">5940</qudt:numericalValue>
   <rdf:value rdf:datatype="http://www.w3.org/2001/XMLSchema#double">5940</rdf:value>
   <gs1:unitCode>MLT</gs1:unitCode>
   <gs1:value>5940</gs1:value>
  </gs1:QuantitativeValue>
 </gs1:netContent>
 <sosa:isFeatureOfInterestOf>
  <rdf:Description rdf:about="#18xbottle330ml-ContentSosa">
   <rdf:type rdf:resource="http://www.w3.org/ns/sosa/Observation"/>
   <sosa:hasFeatureOfInterest rdf:resource="#18xbottle330ml"/>
   <sosa:observedProperty  rdf:resource="#netcontent"/>
   <sosa:hasResult rdf:resource="#18xbottle330ml-Content"/>
   <sosa:hasSimpleResult rdf:datatype="http://www.qudt.org/2.1/vocab/unit/MilliM">5940</sosa:hasSimpleResult>
  </rdf:Description>
 </sosa:isFeatureOfInterestOf>
 </rdf:Description>

 <rdf:Description rdf:about="#12xcan330ml">
  <rdf:type rdf:resource="#LiquidContainer"/>
  <rdf:type rdf:resource="#BeverageCan"/>
  <rdf:type rdf:resource="https://gs1.org/voc/PackagingDetails"/>
  <rdfs:label xml:lang="en">12XCan330ml</rdfs:label>
  <rdfs:label xml:lang="fr">12XCan330ml</rdfs:label>
  <skos:definition xml:lang="en">Generic Flat, Box or Crate of 12, 330ml Cans</skos:definition>
  <skos:definition xml:lang="fr">Une boite, caisse ou caissette générique de 12 Canettes de 330ml</skos:definition>
  <rdfs:comment xml:lang="en">This term is meant to be used as a placeholder when no data about the aggregate packaging is known.</rdfs:comment>
  <rdfs:comment xml:lang="fr">Ce terme peut-être utilisé comme un terme générique lorsque les details de l’emballage ne sont pas certain.</rdfs:comment>
  <beer:count rdf:datatype="http://www.w3.org/2001/XMLSchema#Integer">12</beer:count>
  <beer:item rdf:resource="https://rdf.ag/o/beer#can330ml"/>
  <rdfs:isDefinedBy rdf:resource="https://rdf.ag/o/beer-ONTOLOGY_DATE"/>
  <void:inDataset rdf:resource="#datasetdefinition"/>
  <gs1:netContent>
   <gs1:QuantitativeValue rdf:about="#12xcan330ml-Content">
   <rdf:type rdf:resource="http://qudt.org/1.1/schema/qudt#QuantityValue"/>
   <qudt:unit rdf:resource="http://www.qudt.org/2.1/vocab/unit/MilliL"/>
   <qudt:numericalValue rdf:datatype="http://www.w3.org/2001/XMLSchema#double">3960</qudt:numericalValue>
   <rdf:value rdf:datatype="http://www.w3.org/2001/XMLSchema#double">3960</rdf:value>
   <gs1:unitCode>MLT</gs1:unitCode>
   <gs1:value>3960</gs1:value>
  </gs1:QuantitativeValue>
 </gs1:netContent>
 <sosa:isFeatureOfInterestOf>
  <rdf:Description rdf:about="#12xcan330ml-ContentSosa">
   <rdf:type rdf:resource="http://www.w3.org/ns/sosa/Observation"/>
   <sosa:hasFeatureOfInterest rdf:resource="#12xcan330ml"/>
   <sosa:observedProperty  rdf:resource="#netcontent"/>
   <sosa:hasResult rdf:resource="#12xcan330ml-Content"/>
   <sosa:hasSimpleResult rdf:datatype="http://www.qudt.org/2.1/vocab/unit/MilliM">3960</sosa:hasSimpleResult>
  </rdf:Description>
 </sosa:isFeatureOfInterestOf>
 </rdf:Description>

 <rdf:Description rdf:about="#24xcan330ml">
  <rdf:type rdf:resource="#LiquidContainer"/>
  <rdf:type rdf:resource="#BeverageCan"/>
  <rdf:type rdf:resource="https://gs1.org/voc/PackagingDetails"/>
  <rdfs:label xml:lang="en">24XCan330ml</rdfs:label>
  <rdfs:label xml:lang="fr">24XCan330ml</rdfs:label>
  <skos:definition xml:lang="en">Generic Flat, Box or Crate of 24, 330ml Cans</skos:definition>
  <skos:definition xml:lang="fr">Une boite, caisse ou caissette générique de 24 Canettes de 330ml</skos:definition>
  <rdfs:comment xml:lang="en">This term is meant to be used as a placeholder when no data about the aggregate packaging is known.</rdfs:comment>
  <rdfs:comment xml:lang="fr">Ce terme peut-être utilisé comme un terme générique lorsque les details de l’emballage ne sont pas certain.</rdfs:comment>
  <beer:count rdf:datatype="http://www.w3.org/2001/XMLSchema#Integer">24</beer:count>
  <beer:item rdf:resource="https://rdf.ag/o/beer#can330ml"/>
  <rdfs:isDefinedBy rdf:resource="https://rdf.ag/o/beer-ONTOLOGY_DATE"/>
  <void:inDataset rdf:resource="#datasetdefinition"/>
  <gs1:netContent>
   <gs1:QuantitativeValue rdf:about="#24xcan330ml-Content">
   <rdf:type rdf:resource="http://qudt.org/1.1/schema/qudt#QuantityValue"/>
   <qudt:unit rdf:resource="http://www.qudt.org/2.1/vocab/unit/MilliL"/>
   <qudt:numericalValue rdf:datatype="http://www.w3.org/2001/XMLSchema#double">7920</qudt:numericalValue>
   <rdf:value rdf:datatype="http://www.w3.org/2001/XMLSchema#double">7920</rdf:value>
   <gs1:unitCode>MLT</gs1:unitCode>
   <gs1:value>7920</gs1:value>
  </gs1:QuantitativeValue>
 </gs1:netContent>
 <sosa:isFeatureOfInterestOf>
  <rdf:Description rdf:about="#24xcan330ml-ContentSosa">
   <rdf:type rdf:resource="http://www.w3.org/ns/sosa/Observation"/>
   <sosa:hasFeatureOfInterest rdf:resource="#24xcan330ml"/>
   <sosa:observedProperty  rdf:resource="#netcontent"/>
   <sosa:hasResult rdf:resource="#24xcan330ml-Content"/>
   <sosa:hasSimpleResult rdf:datatype="http://www.qudt.org/2.1/vocab/unit/MilliM">7920</sosa:hasSimpleResult>
  </rdf:Description>
 </sosa:isFeatureOfInterestOf>
 </rdf:Description>

 <rdf:Description rdf:about="#6xcan330ml">
  <rdf:type rdf:resource="#LiquidContainer"/>
  <rdf:type rdf:resource="#BeverageCan"/>
  <rdf:type rdf:resource="https://gs1.org/voc/PackagingDetails"/>
  <rdfs:label xml:lang="en">6XCan330ml</rdfs:label>
  <rdfs:label xml:lang="fr">6XCan330ml</rdfs:label>
  <skos:definition xml:lang="en">Generic Flat, Box or Crate of 6, 330ml Cans</skos:definition>
  <skos:definition xml:lang="fr">Une boite, caisse ou caissette générique de 6 Canettes de 330ml</skos:definition>
  <rdfs:comment xml:lang="en">This term is meant to be used as a placeholder when no data about the aggregate packaging is known.</rdfs:comment>
  <rdfs:comment xml:lang="fr">Ce terme peut-être utilisé comme un terme générique lorsque les details de l’emballage ne sont pas certain.</rdfs:comment>
  <beer:count rdf:datatype="http://www.w3.org/2001/XMLSchema#Integer">6</beer:count>
  <beer:item rdf:resource="https://rdf.ag/o/beer#can330ml"/>
  <rdfs:isDefinedBy rdf:resource="https://rdf.ag/o/beer-ONTOLOGY_DATE"/>
  <void:inDataset rdf:resource="#datasetdefinition"/>
  <gs1:netContent>
   <gs1:QuantitativeValue rdf:about="#6xcan330ml-Content">
   <rdf:type rdf:resource="http://qudt.org/1.1/schema/qudt#QuantityValue"/>
   <qudt:unit rdf:resource="http://www.qudt.org/2.1/vocab/unit/MilliL"/>
   <qudt:numericalValue rdf:datatype="http://www.w3.org/2001/XMLSchema#double">1980</qudt:numericalValue>
   <rdf:value rdf:datatype="http://www.w3.org/2001/XMLSchema#double">1980</rdf:value>
   <gs1:unitCode>MLT</gs1:unitCode>
   <gs1:value>1980</gs1:value>
  </gs1:QuantitativeValue>
 </gs1:netContent>
 <sosa:isFeatureOfInterestOf>
  <rdf:Description rdf:about="#6xcan330ml-ContentSosa">
   <rdf:type rdf:resource="http://www.w3.org/ns/sosa/Observation"/>
   <sosa:hasFeatureOfInterest rdf:resource="#6xcan330ml"/>
   <sosa:observedProperty  rdf:resource="#netcontent"/>
   <sosa:hasResult rdf:resource="#6xcan330ml-Content"/>
   <sosa:hasSimpleResult rdf:datatype="http://www.qudt.org/2.1/vocab/unit/MilliM">1980</sosa:hasSimpleResult>
  </rdf:Description>
 </sosa:isFeatureOfInterestOf>
 </rdf:Description>

 <rdf:Description rdf:about="#12xcan440ml">
  <rdf:type rdf:resource="#LiquidContainer"/>
  <rdf:type rdf:resource="#BeverageCan"/>
  <rdf:type rdf:resource="https://gs1.org/voc/PackagingDetails"/>
  <rdfs:label xml:lang="en">12XCan440ml</rdfs:label>
  <rdfs:label xml:lang="fr">12XCan440ml</rdfs:label>
  <skos:definition xml:lang="en">Generic Flat, Box or Crate of 12, 440ml Cans</skos:definition>
  <skos:definition xml:lang="fr">Une boite, caisse ou caissette générique de 12 Canettes de 440ml</skos:definition>
  <rdfs:comment xml:lang="en">This term is meant to be used as a placeholder when no data about the aggregate packaging is known.</rdfs:comment>
  <rdfs:comment xml:lang="fr">Ce terme peut-être utilisé comme un terme générique lorsque les details de l’emballage ne sont pas certain.</rdfs:comment>
  <beer:count rdf:datatype="http://www.w3.org/2001/XMLSchema#Integer">12</beer:count>
  <beer:item rdf:resource="https://rdf.ag/o/beer#can440ml"/>
  <rdfs:isDefinedBy rdf:resource="https://rdf.ag/o/beer-ONTOLOGY_DATE"/>
  <void:inDataset rdf:resource="#datasetdefinition"/>
  <gs1:netContent>
   <gs1:QuantitativeValue rdf:about="#12xcan440ml-Content">
   <rdf:type rdf:resource="http://qudt.org/1.1/schema/qudt#QuantityValue"/>
   <qudt:unit rdf:resource="http://www.qudt.org/2.1/vocab/unit/MilliL"/>
   <qudt:numericalValue rdf:datatype="http://www.w3.org/2001/XMLSchema#double">5280</qudt:numericalValue>
   <rdf:value rdf:datatype="http://www.w3.org/2001/XMLSchema#double">5280</rdf:value>
   <gs1:unitCode>MLT</gs1:unitCode>
   <gs1:value>5280</gs1:value>
  </gs1:QuantitativeValue>
 </gs1:netContent>
 <sosa:isFeatureOfInterestOf>
  <rdf:Description rdf:about="#12xcan440ml-ContentSosa">
   <rdf:type rdf:resource="http://www.w3.org/ns/sosa/Observation"/>
   <sosa:hasFeatureOfInterest rdf:resource="#12xcan440ml"/>
   <sosa:observedProperty  rdf:resource="#netcontent"/>
   <sosa:hasResult rdf:resource="#12xcan440ml-Content"/>
   <sosa:hasSimpleResult rdf:datatype="http://www.qudt.org/2.1/vocab/unit/MilliM">5280</sosa:hasSimpleResult>
  </rdf:Description>
 </sosa:isFeatureOfInterestOf>
 </rdf:Description>

 <rdf:Description rdf:about="#4xcan440ml">
  <rdf:type rdf:resource="#LiquidContainer"/>
  <rdf:type rdf:resource="#BeverageCan"/>
  <rdf:type rdf:resource="https://gs1.org/voc/PackagingDetails"/>
  <rdfs:label xml:lang="en">4XCan440ml</rdfs:label>
  <rdfs:label xml:lang="fr">4XCan440ml</rdfs:label>
  <skos:definition xml:lang="en">Generic Flat, Box or Crate of 4, 440ml Cans</skos:definition>
  <skos:definition xml:lang="fr">Une boite, caisse ou caissette générique de 4 Canettes de 440ml</skos:definition>
  <rdfs:comment xml:lang="en">This term is meant to be used as a placeholder when no data about the aggregate packaging is known.</rdfs:comment>
  <rdfs:comment xml:lang="fr">Ce terme peut-être utilisé comme un terme générique lorsque les details de l’emballage ne sont pas certain.</rdfs:comment>
  <beer:count rdf:datatype="http://www.w3.org/2001/XMLSchema#Integer">4</beer:count>
  <beer:item rdf:resource="https://rdf.ag/o/beer#can440ml"/>
  <rdfs:isDefinedBy rdf:resource="https://rdf.ag/o/beer-ONTOLOGY_DATE"/>
  <void:inDataset rdf:resource="#datasetdefinition"/>
  <gs1:netContent>
   <gs1:QuantitativeValue rdf:about="#4xcan440ml-Content">
   <rdf:type rdf:resource="http://qudt.org/1.1/schema/qudt#QuantityValue"/>
   <qudt:unit rdf:resource="http://www.qudt.org/2.1/vocab/unit/MilliL"/>
   <qudt:numericalValue rdf:datatype="http://www.w3.org/2001/XMLSchema#double">1760</qudt:numericalValue>
   <rdf:value rdf:datatype="http://www.w3.org/2001/XMLSchema#double">1760</rdf:value>
   <gs1:unitCode>MLT</gs1:unitCode>
   <gs1:value>1760</gs1:value>
  </gs1:QuantitativeValue>
 </gs1:netContent>
 <sosa:isFeatureOfInterestOf>
  <rdf:Description rdf:about="#4xcan440ml-ContentSosa">
   <rdf:type rdf:resource="http://www.w3.org/ns/sosa/Observation"/>
   <sosa:hasFeatureOfInterest rdf:resource="#4xcan440ml"/>
   <sosa:observedProperty  rdf:resource="#netcontent"/>
   <sosa:hasResult rdf:resource="#4xcan440ml-Content"/>
   <sosa:hasSimpleResult rdf:datatype="http://www.qudt.org/2.1/vocab/unit/MilliM">1760</sosa:hasSimpleResult>
  </rdf:Description>
 </sosa:isFeatureOfInterestOf>
 </rdf:Description>

 <rdf:Description rdf:about="#24xcan440ml">
  <rdf:type rdf:resource="#LiquidContainer"/>
  <rdf:type rdf:resource="#BeverageCan"/>
  <rdf:type rdf:resource="https://gs1.org/voc/PackagingDetails"/>
  <rdfs:label xml:lang="en">24XCan440ml</rdfs:label>
  <rdfs:label xml:lang="fr">24XCan440ml</rdfs:label>
  <skos:definition xml:lang="en">Generic Flat, Box or Crate of 24, 440ml Cans</skos:definition>
  <skos:definition xml:lang="fr">Une boite, caisse ou caissette générique de 24 Canettes de 440ml</skos:definition>
  <rdfs:comment xml:lang="en">This term is meant to be used as a placeholder when no data about the aggregate packaging is known.</rdfs:comment>
  <rdfs:comment xml:lang="fr">Ce terme peut-être utilisé comme un terme générique lorsque les details de l’emballage ne sont pas certain.</rdfs:comment>
  <beer:count rdf:datatype="http://www.w3.org/2001/XMLSchema#Integer">24</beer:count>
  <beer:item rdf:resource="https://rdf.ag/o/beer#can440ml"/>
  <rdfs:isDefinedBy rdf:resource="https://rdf.ag/o/beer-ONTOLOGY_DATE"/>
  <void:inDataset rdf:resource="#datasetdefinition"/>
  <gs1:netContent>
   <gs1:QuantitativeValue rdf:about="#24xcan440ml-Content">
   <rdf:type rdf:resource="http://qudt.org/1.1/schema/qudt#QuantityValue"/>
   <qudt:unit rdf:resource="http://www.qudt.org/2.1/vocab/unit/MilliL"/>
   <qudt:numericalValue rdf:datatype="http://www.w3.org/2001/XMLSchema#double">10560</qudt:numericalValue>
   <rdf:value rdf:datatype="http://www.w3.org/2001/XMLSchema#double">10560</rdf:value>
   <gs1:unitCode>MLT</gs1:unitCode>
   <gs1:value>10560</gs1:value>
  </gs1:QuantitativeValue>
 </gs1:netContent>
 <sosa:isFeatureOfInterestOf>
  <rdf:Description rdf:about="#24xcan440ml-ContentSosa">
   <rdf:type rdf:resource="http://www.w3.org/ns/sosa/Observation"/>
   <sosa:hasFeatureOfInterest rdf:resource="#24xcan440ml"/>
   <sosa:observedProperty  rdf:resource="#netcontent"/>
   <sosa:hasResult rdf:resource="#24xcan440ml-Content"/>
   <sosa:hasSimpleResult rdf:datatype="http://www.qudt.org/2.1/vocab/unit/MilliM">10560</sosa:hasSimpleResult>
  </rdf:Description>
 </sosa:isFeatureOfInterestOf>
 </rdf:Description>

 <rdf:Description rdf:about="#6xcan440ml">
  <rdf:type rdf:resource="#LiquidContainer"/>
  <rdf:type rdf:resource="#BeverageCan"/>
  <rdf:type rdf:resource="https://gs1.org/voc/PackagingDetails"/>
  <rdfs:label xml:lang="en">6XCan440ml</rdfs:label>
  <rdfs:label xml:lang="fr">6XCan440ml</rdfs:label>
  <skos:definition xml:lang="en">Generic Flat, Box or Crate of 6, 440ml Cans</skos:definition>
  <skos:definition xml:lang="fr">Une boite, caisse ou caissette générique de 6 Canettes de 440ml</skos:definition>
  <rdfs:comment xml:lang="en">This term is meant to be used as a placeholder when no data about the aggregate packaging is known.</rdfs:comment>
  <rdfs:comment xml:lang="fr">Ce terme peut-être utilisé comme un terme générique lorsque les details de l’emballage ne sont pas certain.</rdfs:comment>
  <beer:count rdf:datatype="http://www.w3.org/2001/XMLSchema#Integer">6</beer:count>
  <beer:item rdf:resource="https://rdf.ag/o/beer#can440ml"/>
  <rdfs:isDefinedBy rdf:resource="https://rdf.ag/o/beer-ONTOLOGY_DATE"/>
  <void:inDataset rdf:resource="#datasetdefinition"/>
  <gs1:netContent>
   <gs1:QuantitativeValue rdf:about="#6xcan440ml-Content">
   <rdf:type rdf:resource="http://qudt.org/1.1/schema/qudt#QuantityValue"/>
   <qudt:unit rdf:resource="http://www.qudt.org/2.1/vocab/unit/MilliL"/>
   <qudt:numericalValue rdf:datatype="http://www.w3.org/2001/XMLSchema#double">2640</qudt:numericalValue>
   <rdf:value rdf:datatype="http://www.w3.org/2001/XMLSchema#double">2640</rdf:value>
   <gs1:unitCode>MLT</gs1:unitCode>
   <gs1:value>2640</gs1:value>
  </gs1:QuantitativeValue>
 </gs1:netContent>
 <sosa:isFeatureOfInterestOf>
  <rdf:Description rdf:about="#6xcan440ml-ContentSosa">
   <rdf:type rdf:resource="http://www.w3.org/ns/sosa/Observation"/>
   <sosa:hasFeatureOfInterest rdf:resource="#6xcan440ml"/>
   <sosa:observedProperty  rdf:resource="#netcontent"/>
   <sosa:hasResult rdf:resource="#6xcan440ml-Content"/>
   <sosa:hasSimpleResult rdf:datatype="http://www.qudt.org/2.1/vocab/unit/MilliM">2640</sosa:hasSimpleResult>
  </rdf:Description>
 </sosa:isFeatureOfInterestOf>
 </rdf:Description>

 <rdf:Description rdf:about="#8xcan440ml">
  <rdf:type rdf:resource="#LiquidContainer"/>
  <rdf:type rdf:resource="#BeverageCan"/>
  <rdf:type rdf:resource="https://gs1.org/voc/PackagingDetails"/>
  <rdfs:label xml:lang="en">8XCan440ml</rdfs:label>
  <rdfs:label xml:lang="fr">8XCan440ml</rdfs:label>
  <skos:definition xml:lang="en">Generic Flat, Box or Crate of 8, 440ml Cans</skos:definition>
  <skos:definition xml:lang="fr">Une boite, caisse ou caissette générique de 8 Canettes de 440ml</skos:definition>
  <rdfs:comment xml:lang="en">This term is meant to be used as a placeholder when no data about the aggregate packaging is known.</rdfs:comment>
  <rdfs:comment xml:lang="fr">Ce terme peut-être utilisé comme un terme générique lorsque les details de l’emballage ne sont pas certain.</rdfs:comment>
  <beer:count rdf:datatype="http://www.w3.org/2001/XMLSchema#Integer">8</beer:count>
  <beer:item rdf:resource="https://rdf.ag/o/beer#can440ml"/>
  <rdfs:isDefinedBy rdf:resource="https://rdf.ag/o/beer-ONTOLOGY_DATE"/>
  <void:inDataset rdf:resource="#datasetdefinition"/>
  <gs1:netContent>
   <gs1:QuantitativeValue rdf:about="#8xcan440ml-Content">
   <rdf:type rdf:resource="http://qudt.org/1.1/schema/qudt#QuantityValue"/>
   <qudt:unit rdf:resource="http://www.qudt.org/2.1/vocab/unit/MilliL"/>
   <qudt:numericalValue rdf:datatype="http://www.w3.org/2001/XMLSchema#double">3520</qudt:numericalValue>
   <rdf:value rdf:datatype="http://www.w3.org/2001/XMLSchema#double">3520</rdf:value>
   <gs1:unitCode>MLT</gs1:unitCode>
   <gs1:value>3520</gs1:value>
  </gs1:QuantitativeValue>
 </gs1:netContent>
 <sosa:isFeatureOfInterestOf>
  <rdf:Description rdf:about="#8xcan440ml-ContentSosa">
   <rdf:type rdf:resource="http://www.w3.org/ns/sosa/Observation"/>
   <sosa:hasFeatureOfInterest rdf:resource="#8xcan440ml"/>
   <sosa:observedProperty  rdf:resource="#netcontent"/>
   <sosa:hasResult rdf:resource="#8xcan440ml-Content"/>
   <sosa:hasSimpleResult rdf:datatype="http://www.qudt.org/2.1/vocab/unit/MilliM">3520</sosa:hasSimpleResult>
  </rdf:Description>
 </sosa:isFeatureOfInterestOf>
 </rdf:Description>

 <rdf:Description rdf:about="#2xcan740ml">
  <rdf:type rdf:resource="#LiquidContainer"/>
  <rdf:type rdf:resource="#BeverageCan"/>
  <rdf:type rdf:resource="https://gs1.org/voc/PackagingDetails"/>
  <rdfs:label xml:lang="en">2XCan740ml</rdfs:label>
  <rdfs:label xml:lang="fr">2XCan740ml</rdfs:label>
  <skos:definition xml:lang="en">Generic Flat, Box or Crate of 2, 740ml Cans</skos:definition>
  <skos:definition xml:lang="fr">Une boite, caisse ou caissette générique de 2 Canettes de 740ml</skos:definition>
  <rdfs:comment xml:lang="en">This term is meant to be used as a placeholder when no data about the aggregate packaging is known.</rdfs:comment>
  <rdfs:comment xml:lang="fr">Ce terme peut-être utilisé comme un terme générique lorsque les details de l’emballage ne sont pas certain.</rdfs:comment>
  <beer:count rdf:datatype="http://www.w3.org/2001/XMLSchema#Integer">2</beer:count>
  <beer:item rdf:resource="https://rdf.ag/o/beer#can740ml"/>
  <rdfs:isDefinedBy rdf:resource="https://rdf.ag/o/beer-ONTOLOGY_DATE"/>
  <void:inDataset rdf:resource="#datasetdefinition"/>
  <gs1:netContent>
   <gs1:QuantitativeValue rdf:about="#2xcan740ml-Content">
   <rdf:type rdf:resource="http://qudt.org/1.1/schema/qudt#QuantityValue"/>
   <qudt:unit rdf:resource="http://www.qudt.org/2.1/vocab/unit/MilliL"/>
   <qudt:numericalValue rdf:datatype="http://www.w3.org/2001/XMLSchema#double">1480</qudt:numericalValue>
   <rdf:value rdf:datatype="http://www.w3.org/2001/XMLSchema#double">1480</rdf:value>
   <gs1:unitCode>MLT</gs1:unitCode>
   <gs1:value>1480</gs1:value>
  </gs1:QuantitativeValue>
 </gs1:netContent>
 <sosa:isFeatureOfInterestOf>
  <rdf:Description rdf:about="#2xcan740ml-ContentSosa">
   <rdf:type rdf:resource="http://www.w3.org/ns/sosa/Observation"/>
   <sosa:hasFeatureOfInterest rdf:resource="#2xcan740ml"/>
   <sosa:observedProperty  rdf:resource="#netcontent"/>
   <sosa:hasResult rdf:resource="#2xcan740ml-Content"/>
   <sosa:hasSimpleResult rdf:datatype="http://www.qudt.org/2.1/vocab/unit/MilliM">1480</sosa:hasSimpleResult>
  </rdf:Description>
 </sosa:isFeatureOfInterestOf>
 </rdf:Description>

 <rdf:Description rdf:about="#12xcan740ml">
  <rdf:type rdf:resource="#LiquidContainer"/>
  <rdf:type rdf:resource="#BeverageCan"/>
  <rdf:type rdf:resource="https://gs1.org/voc/PackagingDetails"/>
  <rdfs:label xml:lang="en">12XCan740ml</rdfs:label>
  <rdfs:label xml:lang="fr">12XCan740ml</rdfs:label>
  <skos:definition xml:lang="en">Generic Flat, Box or Crate of 12, 740ml Cans</skos:definition>
  <skos:definition xml:lang="fr">Une boite, caisse ou caissette générique de 12 Canettes de 740ml</skos:definition>
  <rdfs:comment xml:lang="en">This term is meant to be used as a placeholder when no data about the aggregate packaging is known.</rdfs:comment>
  <rdfs:comment xml:lang="fr">Ce terme peut-être utilisé comme un terme générique lorsque les details de l’emballage ne sont pas certain.</rdfs:comment>
  <beer:count rdf:datatype="http://www.w3.org/2001/XMLSchema#Integer">12</beer:count>
  <beer:item rdf:resource="https://rdf.ag/o/beer#can740ml"/>
  <rdfs:isDefinedBy rdf:resource="https://rdf.ag/o/beer-ONTOLOGY_DATE"/>
  <void:inDataset rdf:resource="#datasetdefinition"/>
  <gs1:netContent>
   <gs1:QuantitativeValue rdf:about="#12xcan740ml-Content">
   <rdf:type rdf:resource="http://qudt.org/1.1/schema/qudt#QuantityValue"/>
   <qudt:unit rdf:resource="http://www.qudt.org/2.1/vocab/unit/MilliL"/>
   <qudt:numericalValue rdf:datatype="http://www.w3.org/2001/XMLSchema#double">8880</qudt:numericalValue>
   <rdf:value rdf:datatype="http://www.w3.org/2001/XMLSchema#double">8880</rdf:value>
   <gs1:unitCode>MLT</gs1:unitCode>
   <gs1:value>8880</gs1:value>
  </gs1:QuantitativeValue>
 </gs1:netContent>
 <sosa:isFeatureOfInterestOf>
  <rdf:Description rdf:about="#12xcan740ml-ContentSosa">
   <rdf:type rdf:resource="http://www.w3.org/ns/sosa/Observation"/>
   <sosa:hasFeatureOfInterest rdf:resource="#12xcan740ml"/>
   <sosa:observedProperty  rdf:resource="#netcontent"/>
   <sosa:hasResult rdf:resource="#12xcan740ml-Content"/>
   <sosa:hasSimpleResult rdf:datatype="http://www.qudt.org/2.1/vocab/unit/MilliM">8880</sosa:hasSimpleResult>
  </rdf:Description>
 </sosa:isFeatureOfInterestOf>
 </rdf:Description>

 <rdf:Description rdf:about="#4xcan740ml">
  <rdf:type rdf:resource="#LiquidContainer"/>
  <rdf:type rdf:resource="#BeverageCan"/>
  <rdf:type rdf:resource="https://gs1.org/voc/PackagingDetails"/>
  <rdfs:label xml:lang="en">4XCan740ml</rdfs:label>
  <rdfs:label xml:lang="fr">4XCan740ml</rdfs:label>
  <skos:definition xml:lang="en">Generic Flat, Box or Crate of 4, 740ml Cans</skos:definition>
  <skos:definition xml:lang="fr">Une boite, caisse ou caissette générique de 4 Canettes de 740ml</skos:definition>
  <rdfs:comment xml:lang="en">This term is meant to be used as a placeholder when no data about the aggregate packaging is known.</rdfs:comment>
  <rdfs:comment xml:lang="fr">Ce terme peut-être utilisé comme un terme générique lorsque les details de l’emballage ne sont pas certain.</rdfs:comment>
  <beer:count rdf:datatype="http://www.w3.org/2001/XMLSchema#Integer">4</beer:count>
  <beer:item rdf:resource="https://rdf.ag/o/beer#can740ml"/>
  <rdfs:isDefinedBy rdf:resource="https://rdf.ag/o/beer-ONTOLOGY_DATE"/>
  <void:inDataset rdf:resource="#datasetdefinition"/>
  <gs1:netContent>
   <gs1:QuantitativeValue rdf:about="#4xcan740ml-Content">
   <rdf:type rdf:resource="http://qudt.org/1.1/schema/qudt#QuantityValue"/>
   <qudt:unit rdf:resource="http://www.qudt.org/2.1/vocab/unit/MilliL"/>
   <qudt:numericalValue rdf:datatype="http://www.w3.org/2001/XMLSchema#double">2960</qudt:numericalValue>
   <rdf:value rdf:datatype="http://www.w3.org/2001/XMLSchema#double">2960</rdf:value>
   <gs1:unitCode>MLT</gs1:unitCode>
   <gs1:value>2960</gs1:value>
  </gs1:QuantitativeValue>
 </gs1:netContent>
 <sosa:isFeatureOfInterestOf>
  <rdf:Description rdf:about="#4xcan740ml-ContentSosa">
   <rdf:type rdf:resource="http://www.w3.org/ns/sosa/Observation"/>
   <sosa:hasFeatureOfInterest rdf:resource="#4xcan740ml"/>
   <sosa:observedProperty  rdf:resource="#netcontent"/>
   <sosa:hasResult rdf:resource="#4xcan740ml-Content"/>
   <sosa:hasSimpleResult rdf:datatype="http://www.qudt.org/2.1/vocab/unit/MilliM">2960</sosa:hasSimpleResult>
  </rdf:Description>
 </sosa:isFeatureOfInterestOf>
 </rdf:Description>

 <rdf:Description rdf:about="#4xcan250ml">
  <rdf:type rdf:resource="#LiquidContainer"/>
  <rdf:type rdf:resource="#BeverageCan"/>
  <rdf:type rdf:resource="https://gs1.org/voc/PackagingDetails"/>
  <rdfs:label xml:lang="en">4XCan250ml</rdfs:label>
  <rdfs:label xml:lang="fr">4XCan250ml</rdfs:label>
  <skos:definition xml:lang="en">Generic Flat, Box or Crate of 4, 250ml Cans</skos:definition>
  <skos:definition xml:lang="fr">Une boite, caisse ou caissette générique de 4 Canettes de 250ml</skos:definition>
  <rdfs:comment xml:lang="en">This term is meant to be used as a placeholder when no data about the aggregate packaging is known.</rdfs:comment>
  <rdfs:comment xml:lang="fr">Ce terme peut-être utilisé comme un terme générique lorsque les details de l’emballage ne sont pas certain.</rdfs:comment>
  <beer:count rdf:datatype="http://www.w3.org/2001/XMLSchema#Integer">4</beer:count>
  <beer:item rdf:resource="https://rdf.ag/o/beer#can250ml"/>
  <rdfs:isDefinedBy rdf:resource="https://rdf.ag/o/beer-ONTOLOGY_DATE"/>
  <void:inDataset rdf:resource="#datasetdefinition"/>
  <gs1:netContent>
   <gs1:QuantitativeValue rdf:about="#4xcan250ml-Content">
   <rdf:type rdf:resource="http://qudt.org/1.1/schema/qudt#QuantityValue"/>
   <qudt:unit rdf:resource="http://www.qudt.org/2.1/vocab/unit/MilliL"/>
   <qudt:numericalValue rdf:datatype="http://www.w3.org/2001/XMLSchema#double">1000</qudt:numericalValue>
   <rdf:value rdf:datatype="http://www.w3.org/2001/XMLSchema#double">1000</rdf:value>
   <gs1:unitCode>MLT</gs1:unitCode>
   <gs1:value>1000</gs1:value>
  </gs1:QuantitativeValue>
 </gs1:netContent>
 <sosa:isFeatureOfInterestOf>
  <rdf:Description rdf:about="#4xcan250ml-ContentSosa">
   <rdf:type rdf:resource="http://www.w3.org/ns/sosa/Observation"/>
   <sosa:hasFeatureOfInterest rdf:resource="#4xcan250ml"/>
   <sosa:observedProperty  rdf:resource="#netcontent"/>
   <sosa:hasResult rdf:resource="#4xcan250ml-Content"/>
   <sosa:hasSimpleResult rdf:datatype="http://www.qudt.org/2.1/vocab/unit/MilliM">1000</sosa:hasSimpleResult>
  </rdf:Description>
 </sosa:isFeatureOfInterestOf>
 </rdf:Description>

 <rdf:Description rdf:about="#12xbottle450ml">
  <rdf:type rdf:resource="#LiquidContainer"/>
  <rdf:type rdf:resource="#BeverageBottle"/>
  <rdf:type rdf:resource="https://gs1.org/voc/PackagingDetails"/>
  <rdfs:label xml:lang="en">12XBottle450ml</rdfs:label>
  <rdfs:label xml:lang="fr">12XBottle450ml</rdfs:label>
  <skos:definition xml:lang="en">Generic Flat, Box or Crate of 12, 450ml Bottles</skos:definition>
  <skos:definition xml:lang="fr">Une boite, caisse ou caissette générique de 12 Bouteilles de 450ml</skos:definition>
  <rdfs:comment xml:lang="en">This term is meant to be used as a placeholder when no data about the aggregate packaging is known.</rdfs:comment>
  <rdfs:comment xml:lang="fr">Ce terme peut-être utilisé comme un terme générique lorsque les details de l’emballage ne sont pas certain.</rdfs:comment>
  <beer:count rdf:datatype="http://www.w3.org/2001/XMLSchema#Integer">12</beer:count>
  <beer:item rdf:resource="https://rdf.ag/o/beer#bottle450ml"/>
  <rdfs:isDefinedBy rdf:resource="https://rdf.ag/o/beer-ONTOLOGY_DATE"/>
  <void:inDataset rdf:resource="#datasetdefinition"/>
  <gs1:netContent>
   <gs1:QuantitativeValue rdf:about="#12xbottle450ml-Content">
   <rdf:type rdf:resource="http://qudt.org/1.1/schema/qudt#QuantityValue"/>
   <qudt:unit rdf:resource="http://www.qudt.org/2.1/vocab/unit/MilliL"/>
   <qudt:numericalValue rdf:datatype="http://www.w3.org/2001/XMLSchema#double">5400</qudt:numericalValue>
   <rdf:value rdf:datatype="http://www.w3.org/2001/XMLSchema#double">5400</rdf:value>
   <gs1:unitCode>MLT</gs1:unitCode>
   <gs1:value>5400</gs1:value>
  </gs1:QuantitativeValue>
 </gs1:netContent>
 <sosa:isFeatureOfInterestOf>
  <rdf:Description rdf:about="#12xbottle450ml-ContentSosa">
   <rdf:type rdf:resource="http://www.w3.org/ns/sosa/Observation"/>
   <sosa:hasFeatureOfInterest rdf:resource="#12xbottle450ml"/>
   <sosa:observedProperty  rdf:resource="#netcontent"/>
   <sosa:hasResult rdf:resource="#12xbottle450ml-Content"/>
   <sosa:hasSimpleResult rdf:datatype="http://www.qudt.org/2.1/vocab/unit/MilliM">5400</sosa:hasSimpleResult>
  </rdf:Description>
 </sosa:isFeatureOfInterestOf>
 </rdf:Description>

 <rdf:Description rdf:about="#4xbottle450ml">
  <rdf:type rdf:resource="#LiquidContainer"/>
  <rdf:type rdf:resource="#BeverageBottle"/>
  <rdf:type rdf:resource="https://gs1.org/voc/PackagingDetails"/>
  <rdfs:label xml:lang="en">4XBottle450ml</rdfs:label>
  <rdfs:label xml:lang="fr">4XBottle450ml</rdfs:label>
  <skos:definition xml:lang="en">Generic Flat, Box or Crate of 4, 450ml Bottles</skos:definition>
  <skos:definition xml:lang="fr">Une boite, caisse ou caissette générique de 4 Bouteilles de 450ml</skos:definition>
  <rdfs:comment xml:lang="en">This term is meant to be used as a placeholder when no data about the aggregate packaging is known.</rdfs:comment>
  <rdfs:comment xml:lang="fr">Ce terme peut-être utilisé comme un terme générique lorsque les details de l’emballage ne sont pas certain.</rdfs:comment>
  <beer:count rdf:datatype="http://www.w3.org/2001/XMLSchema#Integer">4</beer:count>
  <beer:item rdf:resource="https://rdf.ag/o/beer#bottle450ml"/>
  <rdfs:isDefinedBy rdf:resource="https://rdf.ag/o/beer-ONTOLOGY_DATE"/>
  <void:inDataset rdf:resource="#datasetdefinition"/>
  <gs1:netContent>
   <gs1:QuantitativeValue rdf:about="#4xbottle450ml-Content">
   <rdf:type rdf:resource="http://qudt.org/1.1/schema/qudt#QuantityValue"/>
   <qudt:unit rdf:resource="http://www.qudt.org/2.1/vocab/unit/MilliL"/>
   <qudt:numericalValue rdf:datatype="http://www.w3.org/2001/XMLSchema#double">1800</qudt:numericalValue>
   <rdf:value rdf:datatype="http://www.w3.org/2001/XMLSchema#double">1800</rdf:value>
   <gs1:unitCode>MLT</gs1:unitCode>
   <gs1:value>1800</gs1:value>
  </gs1:QuantitativeValue>
 </gs1:netContent>
 <sosa:isFeatureOfInterestOf>
  <rdf:Description rdf:about="#4xbottle450ml-ContentSosa">
   <rdf:type rdf:resource="http://www.w3.org/ns/sosa/Observation"/>
   <sosa:hasFeatureOfInterest rdf:resource="#4xbottle450ml"/>
   <sosa:observedProperty  rdf:resource="#netcontent"/>
   <sosa:hasResult rdf:resource="#4xbottle450ml-Content"/>
   <sosa:hasSimpleResult rdf:datatype="http://www.qudt.org/2.1/vocab/unit/MilliM">1800</sosa:hasSimpleResult>
  </rdf:Description>
 </sosa:isFeatureOfInterestOf>
 </rdf:Description>

 <rdf:Description rdf:about="#24xbottle450ml">
  <rdf:type rdf:resource="#LiquidContainer"/>
  <rdf:type rdf:resource="#BeverageBottle"/>
  <rdf:type rdf:resource="https://gs1.org/voc/PackagingDetails"/>
  <rdfs:label xml:lang="en">24XBottle450ml</rdfs:label>
  <rdfs:label xml:lang="fr">24XBottle450ml</rdfs:label>
  <skos:definition xml:lang="en">Generic Flat, Box or Crate of 24, 450ml Bottles</skos:definition>
  <skos:definition xml:lang="fr">Une boite, caisse ou caissette générique de 24 Bouteilles de 450ml</skos:definition>
  <rdfs:comment xml:lang="en">This term is meant to be used as a placeholder when no data about the aggregate packaging is known.</rdfs:comment>
  <rdfs:comment xml:lang="fr">Ce terme peut-être utilisé comme un terme générique lorsque les details de l’emballage ne sont pas certain.</rdfs:comment>
  <beer:count rdf:datatype="http://www.w3.org/2001/XMLSchema#Integer">24</beer:count>
  <beer:item rdf:resource="https://rdf.ag/o/beer#bottle450ml"/>
  <rdfs:isDefinedBy rdf:resource="https://rdf.ag/o/beer-ONTOLOGY_DATE"/>
  <void:inDataset rdf:resource="#datasetdefinition"/>
  <gs1:netContent>
   <gs1:QuantitativeValue rdf:about="#24xbottle450ml-Content">
   <rdf:type rdf:resource="http://qudt.org/1.1/schema/qudt#QuantityValue"/>
   <qudt:unit rdf:resource="http://www.qudt.org/2.1/vocab/unit/MilliL"/>
   <qudt:numericalValue rdf:datatype="http://www.w3.org/2001/XMLSchema#double">10800</qudt:numericalValue>
   <rdf:value rdf:datatype="http://www.w3.org/2001/XMLSchema#double">10800</rdf:value>
   <gs1:unitCode>MLT</gs1:unitCode>
   <gs1:value>10800</gs1:value>
  </gs1:QuantitativeValue>
 </gs1:netContent>
 <sosa:isFeatureOfInterestOf>
  <rdf:Description rdf:about="#24xbottle450ml-ContentSosa">
   <rdf:type rdf:resource="http://www.w3.org/ns/sosa/Observation"/>
   <sosa:hasFeatureOfInterest rdf:resource="#24xbottle450ml"/>
   <sosa:observedProperty  rdf:resource="#netcontent"/>
   <sosa:hasResult rdf:resource="#24xbottle450ml-Content"/>
   <sosa:hasSimpleResult rdf:datatype="http://www.qudt.org/2.1/vocab/unit/MilliM">10800</sosa:hasSimpleResult>
  </rdf:Description>
 </sosa:isFeatureOfInterestOf>
 </rdf:Description>

 <rdf:Description rdf:about="#12xbottle650ml">
  <rdf:type rdf:resource="#LiquidContainer"/>
  <rdf:type rdf:resource="#BeverageBottle"/>
  <rdf:type rdf:resource="https://gs1.org/voc/PackagingDetails"/>
  <rdfs:label xml:lang="en">12XBottle650ml</rdfs:label>
  <rdfs:label xml:lang="fr">12XBottle650ml</rdfs:label>
  <skos:definition xml:lang="en">Generic Flat, Box or Crate of 12, 650ml Bottles</skos:definition>
  <skos:definition xml:lang="fr">Une boite, caisse ou caissette générique de 12 Bouteilles de 650ml</skos:definition>
  <rdfs:comment xml:lang="en">This term is meant to be used as a placeholder when no data about the aggregate packaging is known.</rdfs:comment>
  <rdfs:comment xml:lang="fr">Ce terme peut-être utilisé comme un terme générique lorsque les details de l’emballage ne sont pas certain.</rdfs:comment>
  <beer:count rdf:datatype="http://www.w3.org/2001/XMLSchema#Integer">12</beer:count>
  <beer:item rdf:resource="https://rdf.ag/o/beer#bottle650ml"/>
  <rdfs:isDefinedBy rdf:resource="https://rdf.ag/o/beer-ONTOLOGY_DATE"/>
  <void:inDataset rdf:resource="#datasetdefinition"/>
  <gs1:netContent>
   <gs1:QuantitativeValue rdf:about="#12xbottle650ml-Content">
   <rdf:type rdf:resource="http://qudt.org/1.1/schema/qudt#QuantityValue"/>
   <qudt:unit rdf:resource="http://www.qudt.org/2.1/vocab/unit/MilliL"/>
   <qudt:numericalValue rdf:datatype="http://www.w3.org/2001/XMLSchema#double">7800</qudt:numericalValue>
   <rdf:value rdf:datatype="http://www.w3.org/2001/XMLSchema#double">7800</rdf:value>
   <gs1:unitCode>MLT</gs1:unitCode>
   <gs1:value>7800</gs1:value>
  </gs1:QuantitativeValue>
 </gs1:netContent>
 <sosa:isFeatureOfInterestOf>
  <rdf:Description rdf:about="#12xbottle650ml-ContentSosa">
   <rdf:type rdf:resource="http://www.w3.org/ns/sosa/Observation"/>
   <sosa:hasFeatureOfInterest rdf:resource="#12xbottle650ml"/>
   <sosa:observedProperty  rdf:resource="#netcontent"/>
   <sosa:hasResult rdf:resource="#12xbottle650ml-Content"/>
   <sosa:hasSimpleResult rdf:datatype="http://www.qudt.org/2.1/vocab/unit/MilliM">7800</sosa:hasSimpleResult>
  </rdf:Description>
 </sosa:isFeatureOfInterestOf>
 </rdf:Description>

 <rdf:Description rdf:about="#2xcan650ml">
  <rdf:type rdf:resource="#LiquidContainer"/>
  <rdf:type rdf:resource="#BeverageCan"/>
  <rdf:type rdf:resource="https://gs1.org/voc/PackagingDetails"/>
  <rdfs:label xml:lang="en">2XCan650ml</rdfs:label>
  <rdfs:label xml:lang="fr">2XCan650ml</rdfs:label>
  <skos:definition xml:lang="en">Generic Flat, Box or Crate of 2, 650ml Cans</skos:definition>
  <skos:definition xml:lang="fr">Une boite, caisse ou caissette générique de 2 Canettes de 650ml</skos:definition>
  <rdfs:comment xml:lang="en">This term is meant to be used as a placeholder when no data about the aggregate packaging is known.</rdfs:comment>
  <rdfs:comment xml:lang="fr">Ce terme peut-être utilisé comme un terme générique lorsque les details de l’emballage ne sont pas certain.</rdfs:comment>
  <beer:count rdf:datatype="http://www.w3.org/2001/XMLSchema#Integer">2</beer:count>
  <beer:item rdf:resource="https://rdf.ag/o/beer#can650ml"/>
  <rdfs:isDefinedBy rdf:resource="https://rdf.ag/o/beer-ONTOLOGY_DATE"/>
  <void:inDataset rdf:resource="#datasetdefinition"/>
  <gs1:netContent>
   <gs1:QuantitativeValue rdf:about="#2xcan650ml-Content">
   <rdf:type rdf:resource="http://qudt.org/1.1/schema/qudt#QuantityValue"/>
   <qudt:unit rdf:resource="http://www.qudt.org/2.1/vocab/unit/MilliL"/>
   <qudt:numericalValue rdf:datatype="http://www.w3.org/2001/XMLSchema#double">1300</qudt:numericalValue>
   <rdf:value rdf:datatype="http://www.w3.org/2001/XMLSchema#double">1300</rdf:value>
   <gs1:unitCode>MLT</gs1:unitCode>
   <gs1:value>1300</gs1:value>
  </gs1:QuantitativeValue>
 </gs1:netContent>
 <sosa:isFeatureOfInterestOf>
  <rdf:Description rdf:about="#2xcan650ml-ContentSosa">
   <rdf:type rdf:resource="http://www.w3.org/ns/sosa/Observation"/>
   <sosa:hasFeatureOfInterest rdf:resource="#2xcan650ml"/>
   <sosa:observedProperty  rdf:resource="#netcontent"/>
   <sosa:hasResult rdf:resource="#2xcan650ml-Content"/>
   <sosa:hasSimpleResult rdf:datatype="http://www.qudt.org/2.1/vocab/unit/MilliM">1300</sosa:hasSimpleResult>
  </rdf:Description>
 </sosa:isFeatureOfInterestOf>
 </rdf:Description>

 <rdf:Description rdf:about="#12xcan650ml">
  <rdf:type rdf:resource="#LiquidContainer"/>
  <rdf:type rdf:resource="#BeverageCan"/>
  <rdf:type rdf:resource="https://gs1.org/voc/PackagingDetails"/>
  <rdfs:label xml:lang="en">12XCan650ml</rdfs:label>
  <rdfs:label xml:lang="fr">12XCan650ml</rdfs:label>
  <skos:definition xml:lang="en">Generic Flat, Box or Crate of 12, 650ml Cans</skos:definition>
  <skos:definition xml:lang="fr">Une boite, caisse ou caissette générique de 12 Canettes de 650ml</skos:definition>
  <rdfs:comment xml:lang="en">This term is meant to be used as a placeholder when no data about the aggregate packaging is known.</rdfs:comment>
  <rdfs:comment xml:lang="fr">Ce terme peut-être utilisé comme un terme générique lorsque les details de l’emballage ne sont pas certain.</rdfs:comment>
  <beer:count rdf:datatype="http://www.w3.org/2001/XMLSchema#Integer">12</beer:count>
  <beer:item rdf:resource="https://rdf.ag/o/beer#can650ml"/>
  <rdfs:isDefinedBy rdf:resource="https://rdf.ag/o/beer-ONTOLOGY_DATE"/>
  <void:inDataset rdf:resource="#datasetdefinition"/>
  <gs1:netContent>
   <gs1:QuantitativeValue rdf:about="#12xcan650ml-Content">
   <rdf:type rdf:resource="http://qudt.org/1.1/schema/qudt#QuantityValue"/>
   <qudt:unit rdf:resource="http://www.qudt.org/2.1/vocab/unit/MilliL"/>
   <qudt:numericalValue rdf:datatype="http://www.w3.org/2001/XMLSchema#double">7800</qudt:numericalValue>
   <rdf:value rdf:datatype="http://www.w3.org/2001/XMLSchema#double">7800</rdf:value>
   <gs1:unitCode>MLT</gs1:unitCode>
   <gs1:value>7800</gs1:value>
  </gs1:QuantitativeValue>
 </gs1:netContent>
 <sosa:isFeatureOfInterestOf>
  <rdf:Description rdf:about="#12xcan650ml-ContentSosa">
   <rdf:type rdf:resource="http://www.w3.org/ns/sosa/Observation"/>
   <sosa:hasFeatureOfInterest rdf:resource="#12xcan650ml"/>
   <sosa:observedProperty  rdf:resource="#netcontent"/>
   <sosa:hasResult rdf:resource="#12xcan650ml-Content"/>
   <sosa:hasSimpleResult rdf:datatype="http://www.qudt.org/2.1/vocab/unit/MilliM">7800</sosa:hasSimpleResult>
  </rdf:Description>
 </sosa:isFeatureOfInterestOf>
 </rdf:Description>

 <rdf:Description rdf:about="#6xcan650ml">
  <rdf:type rdf:resource="#LiquidContainer"/>
  <rdf:type rdf:resource="#BeverageCan"/>
  <rdf:type rdf:resource="https://gs1.org/voc/PackagingDetails"/>
  <rdfs:label xml:lang="en">6XCan650ml</rdfs:label>
  <rdfs:label xml:lang="fr">6XCan650ml</rdfs:label>
  <skos:definition xml:lang="en">Generic Flat, Box or Crate of 6, 650ml Cans</skos:definition>
  <skos:definition xml:lang="fr">Une boite, caisse ou caissette générique de 6 Canettes de 650ml</skos:definition>
  <rdfs:comment xml:lang="en">This term is meant to be used as a placeholder when no data about the aggregate packaging is known.</rdfs:comment>
  <rdfs:comment xml:lang="fr">Ce terme peut-être utilisé comme un terme générique lorsque les details de l’emballage ne sont pas certain.</rdfs:comment>
  <beer:count rdf:datatype="http://www.w3.org/2001/XMLSchema#Integer">6</beer:count>
  <beer:item rdf:resource="https://rdf.ag/o/beer#can650ml"/>
  <rdfs:isDefinedBy rdf:resource="https://rdf.ag/o/beer-ONTOLOGY_DATE"/>
  <void:inDataset rdf:resource="#datasetdefinition"/>
  <gs1:netContent>
   <gs1:QuantitativeValue rdf:about="#6xcan650ml-Content">
   <rdf:type rdf:resource="http://qudt.org/1.1/schema/qudt#QuantityValue"/>
   <qudt:unit rdf:resource="http://www.qudt.org/2.1/vocab/unit/MilliL"/>
   <qudt:numericalValue rdf:datatype="http://www.w3.org/2001/XMLSchema#double">3900</qudt:numericalValue>
   <rdf:value rdf:datatype="http://www.w3.org/2001/XMLSchema#double">3900</rdf:value>
   <gs1:unitCode>MLT</gs1:unitCode>
   <gs1:value>3900</gs1:value>
  </gs1:QuantitativeValue>
 </gs1:netContent>
 <sosa:isFeatureOfInterestOf>
  <rdf:Description rdf:about="#6xcan650ml-ContentSosa">
   <rdf:type rdf:resource="http://www.w3.org/ns/sosa/Observation"/>
   <sosa:hasFeatureOfInterest rdf:resource="#6xcan650ml"/>
   <sosa:observedProperty  rdf:resource="#netcontent"/>
   <sosa:hasResult rdf:resource="#6xcan650ml-Content"/>
   <sosa:hasSimpleResult rdf:datatype="http://www.qudt.org/2.1/vocab/unit/MilliM">3900</sosa:hasSimpleResult>
  </rdf:Description>
 </sosa:isFeatureOfInterestOf>
 </rdf:Description>

 <rdf:Description rdf:about="#12xbottle750ml">
  <rdf:type rdf:resource="#LiquidContainer"/>
  <rdf:type rdf:resource="#BeverageBottle"/>
  <rdf:type rdf:resource="https://gs1.org/voc/PackagingDetails"/>
  <rdfs:label xml:lang="en">12XBottle750ml</rdfs:label>
  <rdfs:label xml:lang="fr">12XBottle750ml</rdfs:label>
  <skos:definition xml:lang="en">Generic Flat, Box or Crate of 12, 750ml Bottles</skos:definition>
  <skos:definition xml:lang="fr">Une boite, caisse ou caissette générique de 12 Bouteilles de 750ml</skos:definition>
  <rdfs:comment xml:lang="en">This term is meant to be used as a placeholder when no data about the aggregate packaging is known.</rdfs:comment>
  <rdfs:comment xml:lang="fr">Ce terme peut-être utilisé comme un terme générique lorsque les details de l’emballage ne sont pas certain.</rdfs:comment>
  <beer:count rdf:datatype="http://www.w3.org/2001/XMLSchema#Integer">12</beer:count>
  <beer:item rdf:resource="https://rdf.ag/o/beer#bottle750ml"/>
  <rdfs:isDefinedBy rdf:resource="https://rdf.ag/o/beer-ONTOLOGY_DATE"/>
  <void:inDataset rdf:resource="#datasetdefinition"/>
  <gs1:netContent>
   <gs1:QuantitativeValue rdf:about="#12xbottle750ml-Content">
   <rdf:type rdf:resource="http://qudt.org/1.1/schema/qudt#QuantityValue"/>
   <qudt:unit rdf:resource="http://www.qudt.org/2.1/vocab/unit/MilliL"/>
   <qudt:numericalValue rdf:datatype="http://www.w3.org/2001/XMLSchema#double">9000</qudt:numericalValue>
   <rdf:value rdf:datatype="http://www.w3.org/2001/XMLSchema#double">9000</rdf:value>
   <gs1:unitCode>MLT</gs1:unitCode>
   <gs1:value>9000</gs1:value>
  </gs1:QuantitativeValue>
 </gs1:netContent>
 <sosa:isFeatureOfInterestOf>
  <rdf:Description rdf:about="#12xbottle750ml-ContentSosa">
   <rdf:type rdf:resource="http://www.w3.org/ns/sosa/Observation"/>
   <sosa:hasFeatureOfInterest rdf:resource="#12xbottle750ml"/>
   <sosa:observedProperty  rdf:resource="#netcontent"/>
   <sosa:hasResult rdf:resource="#12xbottle750ml-Content"/>
   <sosa:hasSimpleResult rdf:datatype="http://www.qudt.org/2.1/vocab/unit/MilliM">9000</sosa:hasSimpleResult>
  </rdf:Description>
 </sosa:isFeatureOfInterestOf>
 </rdf:Description>

 <rdf:Description rdf:about="#30xbottle341ml">
  <rdf:type rdf:resource="#LiquidContainer"/>
  <rdf:type rdf:resource="#BeverageBottle"/>
  <rdf:type rdf:resource="https://gs1.org/voc/PackagingDetails"/>
  <rdfs:label xml:lang="en">30XBottle341ml</rdfs:label>
  <rdfs:label xml:lang="fr">30XBottle341ml</rdfs:label>
  <skos:definition xml:lang="en">Generic Flat, Box or Crate of 30, 341ml Bottles</skos:definition>
  <skos:definition xml:lang="fr">Une boite, caisse ou caissette générique de 30 Bouteilles de 341ml</skos:definition>
  <rdfs:comment xml:lang="en">This term is meant to be used as a placeholder when no data about the aggregate packaging is known.</rdfs:comment>
  <rdfs:comment xml:lang="fr">Ce terme peut-être utilisé comme un terme générique lorsque les details de l’emballage ne sont pas certain.</rdfs:comment>
  <beer:count rdf:datatype="http://www.w3.org/2001/XMLSchema#Integer">30</beer:count>
  <beer:item rdf:resource="https://rdf.ag/o/beer#bottle341ml"/>
  <rdfs:isDefinedBy rdf:resource="https://rdf.ag/o/beer-ONTOLOGY_DATE"/>
  <void:inDataset rdf:resource="#datasetdefinition"/>
  <gs1:netContent>
   <gs1:QuantitativeValue rdf:about="#30xbottle341ml-Content">
   <rdf:type rdf:resource="http://qudt.org/1.1/schema/qudt#QuantityValue"/>
   <qudt:unit rdf:resource="http://www.qudt.org/2.1/vocab/unit/MilliL"/>
   <qudt:numericalValue rdf:datatype="http://www.w3.org/2001/XMLSchema#double">10230</qudt:numericalValue>
   <rdf:value rdf:datatype="http://www.w3.org/2001/XMLSchema#double">10230</rdf:value>
   <gs1:unitCode>MLT</gs1:unitCode>
   <gs1:value>10230</gs1:value>
  </gs1:QuantitativeValue>
 </gs1:netContent>
 <sosa:isFeatureOfInterestOf>
  <rdf:Description rdf:about="#30xbottle341ml-ContentSosa">
   <rdf:type rdf:resource="http://www.w3.org/ns/sosa/Observation"/>
   <sosa:hasFeatureOfInterest rdf:resource="#30xbottle341ml"/>
   <sosa:observedProperty  rdf:resource="#netcontent"/>
   <sosa:hasResult rdf:resource="#30xbottle341ml-Content"/>
   <sosa:hasSimpleResult rdf:datatype="http://www.qudt.org/2.1/vocab/unit/MilliM">10230</sosa:hasSimpleResult>
  </rdf:Description>
 </sosa:isFeatureOfInterestOf>
 </rdf:Description>

 <rdf:Description rdf:about="#12xbottle341ml">
  <rdf:type rdf:resource="#LiquidContainer"/>
  <rdf:type rdf:resource="#BeverageBottle"/>
  <rdf:type rdf:resource="https://gs1.org/voc/PackagingDetails"/>
  <rdfs:label xml:lang="en">12XBottle341ml</rdfs:label>
  <rdfs:label xml:lang="fr">12XBottle341ml</rdfs:label>
  <skos:definition xml:lang="en">Generic Flat, Box or Crate of 12, 341ml Bottles</skos:definition>
  <skos:definition xml:lang="fr">Une boite, caisse ou caissette générique de 12 Bouteilles de 341ml</skos:definition>
  <rdfs:comment xml:lang="en">This term is meant to be used as a placeholder when no data about the aggregate packaging is known.</rdfs:comment>
  <rdfs:comment xml:lang="fr">Ce terme peut-être utilisé comme un terme générique lorsque les details de l’emballage ne sont pas certain.</rdfs:comment>
  <beer:count rdf:datatype="http://www.w3.org/2001/XMLSchema#Integer">12</beer:count>
  <beer:item rdf:resource="https://rdf.ag/o/beer#bottle341ml"/>
  <rdfs:isDefinedBy rdf:resource="https://rdf.ag/o/beer-ONTOLOGY_DATE"/>
  <void:inDataset rdf:resource="#datasetdefinition"/>
  <gs1:netContent>
   <gs1:QuantitativeValue rdf:about="#12xbottle341ml-Content">
   <rdf:type rdf:resource="http://qudt.org/1.1/schema/qudt#QuantityValue"/>
   <qudt:unit rdf:resource="http://www.qudt.org/2.1/vocab/unit/MilliL"/>
   <qudt:numericalValue rdf:datatype="http://www.w3.org/2001/XMLSchema#double">4092</qudt:numericalValue>
   <rdf:value rdf:datatype="http://www.w3.org/2001/XMLSchema#double">4092</rdf:value>
   <gs1:unitCode>MLT</gs1:unitCode>
   <gs1:value>4092</gs1:value>
  </gs1:QuantitativeValue>
 </gs1:netContent>
 <sosa:isFeatureOfInterestOf>
  <rdf:Description rdf:about="#12xbottle341ml-ContentSosa">
   <rdf:type rdf:resource="http://www.w3.org/ns/sosa/Observation"/>
   <sosa:hasFeatureOfInterest rdf:resource="#12xbottle341ml"/>
   <sosa:observedProperty  rdf:resource="#netcontent"/>
   <sosa:hasResult rdf:resource="#12xbottle341ml-Content"/>
   <sosa:hasSimpleResult rdf:datatype="http://www.qudt.org/2.1/vocab/unit/MilliM">4092</sosa:hasSimpleResult>
  </rdf:Description>
 </sosa:isFeatureOfInterestOf>
 </rdf:Description>

 <rdf:Description rdf:about="#4xbottle341ml">
  <rdf:type rdf:resource="#LiquidContainer"/>
  <rdf:type rdf:resource="#BeverageBottle"/>
  <rdf:type rdf:resource="https://gs1.org/voc/PackagingDetails"/>
  <rdfs:label xml:lang="en">4XBottle341ml</rdfs:label>
  <rdfs:label xml:lang="fr">4XBottle341ml</rdfs:label>
  <skos:definition xml:lang="en">Generic Flat, Box or Crate of 4, 341ml Bottles</skos:definition>
  <skos:definition xml:lang="fr">Une boite, caisse ou caissette générique de 4 Bouteilles de 341ml</skos:definition>
  <rdfs:comment xml:lang="en">This term is meant to be used as a placeholder when no data about the aggregate packaging is known.</rdfs:comment>
  <rdfs:comment xml:lang="fr">Ce terme peut-être utilisé comme un terme générique lorsque les details de l’emballage ne sont pas certain.</rdfs:comment>
  <beer:count rdf:datatype="http://www.w3.org/2001/XMLSchema#Integer">4</beer:count>
  <beer:item rdf:resource="https://rdf.ag/o/beer#bottle341ml"/>
  <rdfs:isDefinedBy rdf:resource="https://rdf.ag/o/beer-ONTOLOGY_DATE"/>
  <void:inDataset rdf:resource="#datasetdefinition"/>
  <gs1:netContent>
   <gs1:QuantitativeValue rdf:about="#4xbottle341ml-Content">
   <rdf:type rdf:resource="http://qudt.org/1.1/schema/qudt#QuantityValue"/>
   <qudt:unit rdf:resource="http://www.qudt.org/2.1/vocab/unit/MilliL"/>
   <qudt:numericalValue rdf:datatype="http://www.w3.org/2001/XMLSchema#double">1364</qudt:numericalValue>
   <rdf:value rdf:datatype="http://www.w3.org/2001/XMLSchema#double">1364</rdf:value>
   <gs1:unitCode>MLT</gs1:unitCode>
   <gs1:value>1364</gs1:value>
  </gs1:QuantitativeValue>
 </gs1:netContent>
 <sosa:isFeatureOfInterestOf>
  <rdf:Description rdf:about="#4xbottle341ml-ContentSosa">
   <rdf:type rdf:resource="http://www.w3.org/ns/sosa/Observation"/>
   <sosa:hasFeatureOfInterest rdf:resource="#4xbottle341ml"/>
   <sosa:observedProperty  rdf:resource="#netcontent"/>
   <sosa:hasResult rdf:resource="#4xbottle341ml-Content"/>
   <sosa:hasSimpleResult rdf:datatype="http://www.qudt.org/2.1/vocab/unit/MilliM">1364</sosa:hasSimpleResult>
  </rdf:Description>
 </sosa:isFeatureOfInterestOf>
 </rdf:Description>

 <rdf:Description rdf:about="#24xbottle341ml">
  <rdf:type rdf:resource="#LiquidContainer"/>
  <rdf:type rdf:resource="#BeverageBottle"/>
  <rdf:type rdf:resource="https://gs1.org/voc/PackagingDetails"/>
  <rdfs:label xml:lang="en">24XBottle341ml</rdfs:label>
  <rdfs:label xml:lang="fr">24XBottle341ml</rdfs:label>
  <skos:definition xml:lang="en">Generic Flat, Box or Crate of 24, 341ml Bottles</skos:definition>
  <skos:definition xml:lang="fr">Une boite, caisse ou caissette générique de 24 Bouteilles de 341ml</skos:definition>
  <rdfs:comment xml:lang="en">This term is meant to be used as a placeholder when no data about the aggregate packaging is known.</rdfs:comment>
  <rdfs:comment xml:lang="fr">Ce terme peut-être utilisé comme un terme générique lorsque les details de l’emballage ne sont pas certain.</rdfs:comment>
  <beer:count rdf:datatype="http://www.w3.org/2001/XMLSchema#Integer">24</beer:count>
  <beer:item rdf:resource="https://rdf.ag/o/beer#bottle341ml"/>
  <rdfs:isDefinedBy rdf:resource="https://rdf.ag/o/beer-ONTOLOGY_DATE"/>
  <void:inDataset rdf:resource="#datasetdefinition"/>
  <gs1:netContent>
   <gs1:QuantitativeValue rdf:about="#24xbottle341ml-Content">
   <rdf:type rdf:resource="http://qudt.org/1.1/schema/qudt#QuantityValue"/>
   <qudt:unit rdf:resource="http://www.qudt.org/2.1/vocab/unit/MilliL"/>
   <qudt:numericalValue rdf:datatype="http://www.w3.org/2001/XMLSchema#double">8184</qudt:numericalValue>
   <rdf:value rdf:datatype="http://www.w3.org/2001/XMLSchema#double">8184</rdf:value>
   <gs1:unitCode>MLT</gs1:unitCode>
   <gs1:value>8184</gs1:value>
  </gs1:QuantitativeValue>
 </gs1:netContent>
 <sosa:isFeatureOfInterestOf>
  <rdf:Description rdf:about="#24xbottle341ml-ContentSosa">
   <rdf:type rdf:resource="http://www.w3.org/ns/sosa/Observation"/>
   <sosa:hasFeatureOfInterest rdf:resource="#24xbottle341ml"/>
   <sosa:observedProperty  rdf:resource="#netcontent"/>
   <sosa:hasResult rdf:resource="#24xbottle341ml-Content"/>
   <sosa:hasSimpleResult rdf:datatype="http://www.qudt.org/2.1/vocab/unit/MilliM">8184</sosa:hasSimpleResult>
  </rdf:Description>
 </sosa:isFeatureOfInterestOf>
 </rdf:Description>

 <rdf:Description rdf:about="#15xbottle341ml">
  <rdf:type rdf:resource="#LiquidContainer"/>
  <rdf:type rdf:resource="#BeverageBottle"/>
  <rdf:type rdf:resource="https://gs1.org/voc/PackagingDetails"/>
  <rdfs:label xml:lang="en">15XBottle341ml</rdfs:label>
  <rdfs:label xml:lang="fr">15XBottle341ml</rdfs:label>
  <skos:definition xml:lang="en">Generic Flat, Box or Crate of 15, 341ml Bottles</skos:definition>
  <skos:definition xml:lang="fr">Une boite, caisse ou caissette générique de 15 Bouteilles de 341ml</skos:definition>
  <rdfs:comment xml:lang="en">This term is meant to be used as a placeholder when no data about the aggregate packaging is known.</rdfs:comment>
  <rdfs:comment xml:lang="fr">Ce terme peut-être utilisé comme un terme générique lorsque les details de l’emballage ne sont pas certain.</rdfs:comment>
  <beer:count rdf:datatype="http://www.w3.org/2001/XMLSchema#Integer">15</beer:count>
  <beer:item rdf:resource="https://rdf.ag/o/beer#bottle341ml"/>
  <rdfs:isDefinedBy rdf:resource="https://rdf.ag/o/beer-ONTOLOGY_DATE"/>
  <void:inDataset rdf:resource="#datasetdefinition"/>
  <gs1:netContent>
   <gs1:QuantitativeValue rdf:about="#15xbottle341ml-Content">
   <rdf:type rdf:resource="http://qudt.org/1.1/schema/qudt#QuantityValue"/>
   <qudt:unit rdf:resource="http://www.qudt.org/2.1/vocab/unit/MilliL"/>
   <qudt:numericalValue rdf:datatype="http://www.w3.org/2001/XMLSchema#double">5115</qudt:numericalValue>
   <rdf:value rdf:datatype="http://www.w3.org/2001/XMLSchema#double">5115</rdf:value>
   <gs1:unitCode>MLT</gs1:unitCode>
   <gs1:value>5115</gs1:value>
  </gs1:QuantitativeValue>
 </gs1:netContent>
 <sosa:isFeatureOfInterestOf>
  <rdf:Description rdf:about="#15xbottle341ml-ContentSosa">
   <rdf:type rdf:resource="http://www.w3.org/ns/sosa/Observation"/>
   <sosa:hasFeatureOfInterest rdf:resource="#15xbottle341ml"/>
   <sosa:observedProperty  rdf:resource="#netcontent"/>
   <sosa:hasResult rdf:resource="#15xbottle341ml-Content"/>
   <sosa:hasSimpleResult rdf:datatype="http://www.qudt.org/2.1/vocab/unit/MilliM">5115</sosa:hasSimpleResult>
  </rdf:Description>
 </sosa:isFeatureOfInterestOf>
 </rdf:Description>

 <rdf:Description rdf:about="#6xbottle341ml">
  <rdf:type rdf:resource="#LiquidContainer"/>
  <rdf:type rdf:resource="#BeverageBottle"/>
  <rdf:type rdf:resource="https://gs1.org/voc/PackagingDetails"/>
  <rdfs:label xml:lang="en">6XBottle341ml</rdfs:label>
  <rdfs:label xml:lang="fr">6XBottle341ml</rdfs:label>
  <skos:definition xml:lang="en">Generic Flat, Box or Crate of 6, 341ml Bottles</skos:definition>
  <skos:definition xml:lang="fr">Une boite, caisse ou caissette générique de 6 Bouteilles de 341ml</skos:definition>
  <rdfs:comment xml:lang="en">This term is meant to be used as a placeholder when no data about the aggregate packaging is known.</rdfs:comment>
  <rdfs:comment xml:lang="fr">Ce terme peut-être utilisé comme un terme générique lorsque les details de l’emballage ne sont pas certain.</rdfs:comment>
  <beer:count rdf:datatype="http://www.w3.org/2001/XMLSchema#Integer">6</beer:count>
  <beer:item rdf:resource="https://rdf.ag/o/beer#bottle341ml"/>
  <rdfs:isDefinedBy rdf:resource="https://rdf.ag/o/beer-ONTOLOGY_DATE"/>
  <void:inDataset rdf:resource="#datasetdefinition"/>
  <gs1:netContent>
   <gs1:QuantitativeValue rdf:about="#6xbottle341ml-Content">
   <rdf:type rdf:resource="http://qudt.org/1.1/schema/qudt#QuantityValue"/>
   <qudt:unit rdf:resource="http://www.qudt.org/2.1/vocab/unit/MilliL"/>
   <qudt:numericalValue rdf:datatype="http://www.w3.org/2001/XMLSchema#double">2046</qudt:numericalValue>
   <rdf:value rdf:datatype="http://www.w3.org/2001/XMLSchema#double">2046</rdf:value>
   <gs1:unitCode>MLT</gs1:unitCode>
   <gs1:value>2046</gs1:value>
  </gs1:QuantitativeValue>
 </gs1:netContent>
 <sosa:isFeatureOfInterestOf>
  <rdf:Description rdf:about="#6xbottle341ml-ContentSosa">
   <rdf:type rdf:resource="http://www.w3.org/ns/sosa/Observation"/>
   <sosa:hasFeatureOfInterest rdf:resource="#6xbottle341ml"/>
   <sosa:observedProperty  rdf:resource="#netcontent"/>
   <sosa:hasResult rdf:resource="#6xbottle341ml-Content"/>
   <sosa:hasSimpleResult rdf:datatype="http://www.qudt.org/2.1/vocab/unit/MilliM">2046</sosa:hasSimpleResult>
  </rdf:Description>
 </sosa:isFeatureOfInterestOf>
 </rdf:Description>

 <rdf:Description rdf:about="#36xbottle341ml">
  <rdf:type rdf:resource="#LiquidContainer"/>
  <rdf:type rdf:resource="#BeverageBottle"/>
  <rdf:type rdf:resource="https://gs1.org/voc/PackagingDetails"/>
  <rdfs:label xml:lang="en">36XBottle341ml</rdfs:label>
  <rdfs:label xml:lang="fr">36XBottle341ml</rdfs:label>
  <skos:definition xml:lang="en">Generic Flat, Box or Crate of 36, 341ml Bottles</skos:definition>
  <skos:definition xml:lang="fr">Une boite, caisse ou caissette générique de 36 Bouteilles de 341ml</skos:definition>
  <rdfs:comment xml:lang="en">This term is meant to be used as a placeholder when no data about the aggregate packaging is known.</rdfs:comment>
  <rdfs:comment xml:lang="fr">Ce terme peut-être utilisé comme un terme générique lorsque les details de l’emballage ne sont pas certain.</rdfs:comment>
  <beer:count rdf:datatype="http://www.w3.org/2001/XMLSchema#Integer">36</beer:count>
  <beer:item rdf:resource="https://rdf.ag/o/beer#bottle341ml"/>
  <rdfs:isDefinedBy rdf:resource="https://rdf.ag/o/beer-ONTOLOGY_DATE"/>
  <void:inDataset rdf:resource="#datasetdefinition"/>
  <gs1:netContent>
   <gs1:QuantitativeValue rdf:about="#36xbottle341ml-Content">
   <rdf:type rdf:resource="http://qudt.org/1.1/schema/qudt#QuantityValue"/>
   <qudt:unit rdf:resource="http://www.qudt.org/2.1/vocab/unit/MilliL"/>
   <qudt:numericalValue rdf:datatype="http://www.w3.org/2001/XMLSchema#double">12276</qudt:numericalValue>
   <rdf:value rdf:datatype="http://www.w3.org/2001/XMLSchema#double">12276</rdf:value>
   <gs1:unitCode>MLT</gs1:unitCode>
   <gs1:value>12276</gs1:value>
  </gs1:QuantitativeValue>
 </gs1:netContent>
 <sosa:isFeatureOfInterestOf>
  <rdf:Description rdf:about="#36xbottle341ml-ContentSosa">
   <rdf:type rdf:resource="http://www.w3.org/ns/sosa/Observation"/>
   <sosa:hasFeatureOfInterest rdf:resource="#36xbottle341ml"/>
   <sosa:observedProperty  rdf:resource="#netcontent"/>
   <sosa:hasResult rdf:resource="#36xbottle341ml-Content"/>
   <sosa:hasSimpleResult rdf:datatype="http://www.qudt.org/2.1/vocab/unit/MilliM">12276</sosa:hasSimpleResult>
  </rdf:Description>
 </sosa:isFeatureOfInterestOf>
 </rdf:Description>

 <rdf:Description rdf:about="#56xbottle341ml">
  <rdf:type rdf:resource="#LiquidContainer"/>
  <rdf:type rdf:resource="#BeverageBottle"/>
  <rdf:type rdf:resource="https://gs1.org/voc/PackagingDetails"/>
  <rdfs:label xml:lang="en">56XBottle341ml</rdfs:label>
  <rdfs:label xml:lang="fr">56XBottle341ml</rdfs:label>
  <skos:definition xml:lang="en">Generic Flat, Box or Crate of 56, 341ml Bottles</skos:definition>
  <skos:definition xml:lang="fr">Une boite, caisse ou caissette générique de 56 Bouteilles de 341ml</skos:definition>
  <rdfs:comment xml:lang="en">This term is meant to be used as a placeholder when no data about the aggregate packaging is known.</rdfs:comment>
  <rdfs:comment xml:lang="fr">Ce terme peut-être utilisé comme un terme générique lorsque les details de l’emballage ne sont pas certain.</rdfs:comment>
  <beer:count rdf:datatype="http://www.w3.org/2001/XMLSchema#Integer">56</beer:count>
  <beer:item rdf:resource="https://rdf.ag/o/beer#bottle341ml"/>
  <rdfs:isDefinedBy rdf:resource="https://rdf.ag/o/beer-ONTOLOGY_DATE"/>
  <void:inDataset rdf:resource="#datasetdefinition"/>
  <gs1:netContent>
   <gs1:QuantitativeValue rdf:about="#56xbottle341ml-Content">
   <rdf:type rdf:resource="http://qudt.org/1.1/schema/qudt#QuantityValue"/>
   <qudt:unit rdf:resource="http://www.qudt.org/2.1/vocab/unit/MilliL"/>
   <qudt:numericalValue rdf:datatype="http://www.w3.org/2001/XMLSchema#double">19096</qudt:numericalValue>
   <rdf:value rdf:datatype="http://www.w3.org/2001/XMLSchema#double">19096</rdf:value>
   <gs1:unitCode>MLT</gs1:unitCode>
   <gs1:value>19096</gs1:value>
  </gs1:QuantitativeValue>
 </gs1:netContent>
 <sosa:isFeatureOfInterestOf>
  <rdf:Description rdf:about="#56xbottle341ml-ContentSosa">
   <rdf:type rdf:resource="http://www.w3.org/ns/sosa/Observation"/>
   <sosa:hasFeatureOfInterest rdf:resource="#56xbottle341ml"/>
   <sosa:observedProperty  rdf:resource="#netcontent"/>
   <sosa:hasResult rdf:resource="#56xbottle341ml-Content"/>
   <sosa:hasSimpleResult rdf:datatype="http://www.qudt.org/2.1/vocab/unit/MilliM">19096</sosa:hasSimpleResult>
  </rdf:Description>
 </sosa:isFeatureOfInterestOf>
 </rdf:Description>

 <rdf:Description rdf:about="#8xbottle341ml">
  <rdf:type rdf:resource="#LiquidContainer"/>
  <rdf:type rdf:resource="#BeverageBottle"/>
  <rdf:type rdf:resource="https://gs1.org/voc/PackagingDetails"/>
  <rdfs:label xml:lang="en">8XBottle341ml</rdfs:label>
  <rdfs:label xml:lang="fr">8XBottle341ml</rdfs:label>
  <skos:definition xml:lang="en">Generic Flat, Box or Crate of 8, 341ml Bottles</skos:definition>
  <skos:definition xml:lang="fr">Une boite, caisse ou caissette générique de 8 Bouteilles de 341ml</skos:definition>
  <rdfs:comment xml:lang="en">This term is meant to be used as a placeholder when no data about the aggregate packaging is known.</rdfs:comment>
  <rdfs:comment xml:lang="fr">Ce terme peut-être utilisé comme un terme générique lorsque les details de l’emballage ne sont pas certain.</rdfs:comment>
  <beer:count rdf:datatype="http://www.w3.org/2001/XMLSchema#Integer">8</beer:count>
  <beer:item rdf:resource="https://rdf.ag/o/beer#bottle341ml"/>
  <rdfs:isDefinedBy rdf:resource="https://rdf.ag/o/beer-ONTOLOGY_DATE"/>
  <void:inDataset rdf:resource="#datasetdefinition"/>
  <gs1:netContent>
   <gs1:QuantitativeValue rdf:about="#8xbottle341ml-Content">
   <rdf:type rdf:resource="http://qudt.org/1.1/schema/qudt#QuantityValue"/>
   <qudt:unit rdf:resource="http://www.qudt.org/2.1/vocab/unit/MilliL"/>
   <qudt:numericalValue rdf:datatype="http://www.w3.org/2001/XMLSchema#double">2728</qudt:numericalValue>
   <rdf:value rdf:datatype="http://www.w3.org/2001/XMLSchema#double">2728</rdf:value>
   <gs1:unitCode>MLT</gs1:unitCode>
   <gs1:value>2728</gs1:value>
  </gs1:QuantitativeValue>
 </gs1:netContent>
 <sosa:isFeatureOfInterestOf>
  <rdf:Description rdf:about="#8xbottle341ml-ContentSosa">
   <rdf:type rdf:resource="http://www.w3.org/ns/sosa/Observation"/>
   <sosa:hasFeatureOfInterest rdf:resource="#8xbottle341ml"/>
   <sosa:observedProperty  rdf:resource="#netcontent"/>
   <sosa:hasResult rdf:resource="#8xbottle341ml-Content"/>
   <sosa:hasSimpleResult rdf:datatype="http://www.qudt.org/2.1/vocab/unit/MilliM">2728</sosa:hasSimpleResult>
  </rdf:Description>
 </sosa:isFeatureOfInterestOf>
 </rdf:Description>

 <rdf:Description rdf:about="#18xbottle341ml">
  <rdf:type rdf:resource="#LiquidContainer"/>
  <rdf:type rdf:resource="#BeverageBottle"/>
  <rdf:type rdf:resource="https://gs1.org/voc/PackagingDetails"/>
  <rdfs:label xml:lang="en">18XBottle341ml</rdfs:label>
  <rdfs:label xml:lang="fr">18XBottle341ml</rdfs:label>
  <skos:definition xml:lang="en">Generic Flat, Box or Crate of 18, 341ml Bottles</skos:definition>
  <skos:definition xml:lang="fr">Une boite, caisse ou caissette générique de 18 Bouteilles de 341ml</skos:definition>
  <rdfs:comment xml:lang="en">This term is meant to be used as a placeholder when no data about the aggregate packaging is known.</rdfs:comment>
  <rdfs:comment xml:lang="fr">Ce terme peut-être utilisé comme un terme générique lorsque les details de l’emballage ne sont pas certain.</rdfs:comment>
  <beer:count rdf:datatype="http://www.w3.org/2001/XMLSchema#Integer">18</beer:count>
  <beer:item rdf:resource="https://rdf.ag/o/beer#bottle341ml"/>
  <rdfs:isDefinedBy rdf:resource="https://rdf.ag/o/beer-ONTOLOGY_DATE"/>
  <void:inDataset rdf:resource="#datasetdefinition"/>
  <gs1:netContent>
   <gs1:QuantitativeValue rdf:about="#18xbottle341ml-Content">
   <rdf:type rdf:resource="http://qudt.org/1.1/schema/qudt#QuantityValue"/>
   <qudt:unit rdf:resource="http://www.qudt.org/2.1/vocab/unit/MilliL"/>
   <qudt:numericalValue rdf:datatype="http://www.w3.org/2001/XMLSchema#double">6138</qudt:numericalValue>
   <rdf:value rdf:datatype="http://www.w3.org/2001/XMLSchema#double">6138</rdf:value>
   <gs1:unitCode>MLT</gs1:unitCode>
   <gs1:value>6138</gs1:value>
  </gs1:QuantitativeValue>
 </gs1:netContent>
 <sosa:isFeatureOfInterestOf>
  <rdf:Description rdf:about="#18xbottle341ml-ContentSosa">
   <rdf:type rdf:resource="http://www.w3.org/ns/sosa/Observation"/>
   <sosa:hasFeatureOfInterest rdf:resource="#18xbottle341ml"/>
   <sosa:observedProperty  rdf:resource="#netcontent"/>
   <sosa:hasResult rdf:resource="#18xbottle341ml-Content"/>
   <sosa:hasSimpleResult rdf:datatype="http://www.qudt.org/2.1/vocab/unit/MilliM">6138</sosa:hasSimpleResult>
  </rdf:Description>
 </sosa:isFeatureOfInterestOf>
 </rdf:Description>

 <rdf:Description rdf:about="#28xbottle341ml">
  <rdf:type rdf:resource="#LiquidContainer"/>
  <rdf:type rdf:resource="#BeverageBottle"/>
  <rdf:type rdf:resource="https://gs1.org/voc/PackagingDetails"/>
  <rdfs:label xml:lang="en">28XBottle341ml</rdfs:label>
  <rdfs:label xml:lang="fr">28XBottle341ml</rdfs:label>
  <skos:definition xml:lang="en">Generic Flat, Box or Crate of 28, 341ml Bottles</skos:definition>
  <skos:definition xml:lang="fr">Une boite, caisse ou caissette générique de 28 Bouteilles de 341ml</skos:definition>
  <rdfs:comment xml:lang="en">This term is meant to be used as a placeholder when no data about the aggregate packaging is known.</rdfs:comment>
  <rdfs:comment xml:lang="fr">Ce terme peut-être utilisé comme un terme générique lorsque les details de l’emballage ne sont pas certain.</rdfs:comment>
  <beer:count rdf:datatype="http://www.w3.org/2001/XMLSchema#Integer">28</beer:count>
  <beer:item rdf:resource="https://rdf.ag/o/beer#bottle341ml"/>
  <rdfs:isDefinedBy rdf:resource="https://rdf.ag/o/beer-ONTOLOGY_DATE"/>
  <void:inDataset rdf:resource="#datasetdefinition"/>
  <gs1:netContent>
   <gs1:QuantitativeValue rdf:about="#28xbottle341ml-Content">
   <rdf:type rdf:resource="http://qudt.org/1.1/schema/qudt#QuantityValue"/>
   <qudt:unit rdf:resource="http://www.qudt.org/2.1/vocab/unit/MilliL"/>
   <qudt:numericalValue rdf:datatype="http://www.w3.org/2001/XMLSchema#double">9548</qudt:numericalValue>
   <rdf:value rdf:datatype="http://www.w3.org/2001/XMLSchema#double">9548</rdf:value>
   <gs1:unitCode>MLT</gs1:unitCode>
   <gs1:value>9548</gs1:value>
  </gs1:QuantitativeValue>
 </gs1:netContent>
 <sosa:isFeatureOfInterestOf>
  <rdf:Description rdf:about="#28xbottle341ml-ContentSosa">
   <rdf:type rdf:resource="http://www.w3.org/ns/sosa/Observation"/>
   <sosa:hasFeatureOfInterest rdf:resource="#28xbottle341ml"/>
   <sosa:observedProperty  rdf:resource="#netcontent"/>
   <sosa:hasResult rdf:resource="#28xbottle341ml-Content"/>
   <sosa:hasSimpleResult rdf:datatype="http://www.qudt.org/2.1/vocab/unit/MilliM">9548</sosa:hasSimpleResult>
  </rdf:Description>
 </sosa:isFeatureOfInterestOf>
 </rdf:Description>

 <rdf:Description rdf:about="#48xbottle341ml">
  <rdf:type rdf:resource="#LiquidContainer"/>
  <rdf:type rdf:resource="#BeverageBottle"/>
  <rdf:type rdf:resource="https://gs1.org/voc/PackagingDetails"/>
  <rdfs:label xml:lang="en">48XBottle341ml</rdfs:label>
  <rdfs:label xml:lang="fr">48XBottle341ml</rdfs:label>
  <skos:definition xml:lang="en">Generic Flat, Box or Crate of 48, 341ml Bottles</skos:definition>
  <skos:definition xml:lang="fr">Une boite, caisse ou caissette générique de 48 Bouteilles de 341ml</skos:definition>
  <rdfs:comment xml:lang="en">This term is meant to be used as a placeholder when no data about the aggregate packaging is known.</rdfs:comment>
  <rdfs:comment xml:lang="fr">Ce terme peut-être utilisé comme un terme générique lorsque les details de l’emballage ne sont pas certain.</rdfs:comment>
  <beer:count rdf:datatype="http://www.w3.org/2001/XMLSchema#Integer">48</beer:count>
  <beer:item rdf:resource="https://rdf.ag/o/beer#bottle341ml"/>
  <rdfs:isDefinedBy rdf:resource="https://rdf.ag/o/beer-ONTOLOGY_DATE"/>
  <void:inDataset rdf:resource="#datasetdefinition"/>
  <gs1:netContent>
   <gs1:QuantitativeValue rdf:about="#48xbottle341ml-Content">
   <rdf:type rdf:resource="http://qudt.org/1.1/schema/qudt#QuantityValue"/>
   <qudt:unit rdf:resource="http://www.qudt.org/2.1/vocab/unit/MilliL"/>
   <qudt:numericalValue rdf:datatype="http://www.w3.org/2001/XMLSchema#double">16368</qudt:numericalValue>
   <rdf:value rdf:datatype="http://www.w3.org/2001/XMLSchema#double">16368</rdf:value>
   <gs1:unitCode>MLT</gs1:unitCode>
   <gs1:value>16368</gs1:value>
  </gs1:QuantitativeValue>
 </gs1:netContent>
 <sosa:isFeatureOfInterestOf>
  <rdf:Description rdf:about="#48xbottle341ml-ContentSosa">
   <rdf:type rdf:resource="http://www.w3.org/ns/sosa/Observation"/>
   <sosa:hasFeatureOfInterest rdf:resource="#48xbottle341ml"/>
   <sosa:observedProperty  rdf:resource="#netcontent"/>
   <sosa:hasResult rdf:resource="#48xbottle341ml-Content"/>
   <sosa:hasSimpleResult rdf:datatype="http://www.qudt.org/2.1/vocab/unit/MilliM">16368</sosa:hasSimpleResult>
  </rdf:Description>
 </sosa:isFeatureOfInterestOf>
 </rdf:Description>

 <rdf:Description rdf:about="#12xcan341ml">
  <rdf:type rdf:resource="#LiquidContainer"/>
  <rdf:type rdf:resource="#BeverageCan"/>
  <rdf:type rdf:resource="https://gs1.org/voc/PackagingDetails"/>
  <rdfs:label xml:lang="en">12XCan341ml</rdfs:label>
  <rdfs:label xml:lang="fr">12XCan341ml</rdfs:label>
  <skos:definition xml:lang="en">Generic Flat, Box or Crate of 12, 341ml Cans</skos:definition>
  <skos:definition xml:lang="fr">Une boite, caisse ou caissette générique de 12 Canettes de 341ml</skos:definition>
  <rdfs:comment xml:lang="en">This term is meant to be used as a placeholder when no data about the aggregate packaging is known.</rdfs:comment>
  <rdfs:comment xml:lang="fr">Ce terme peut-être utilisé comme un terme générique lorsque les details de l’emballage ne sont pas certain.</rdfs:comment>
  <beer:count rdf:datatype="http://www.w3.org/2001/XMLSchema#Integer">12</beer:count>
  <beer:item rdf:resource="https://rdf.ag/o/beer#can341ml"/>
  <rdfs:isDefinedBy rdf:resource="https://rdf.ag/o/beer-ONTOLOGY_DATE"/>
  <void:inDataset rdf:resource="#datasetdefinition"/>
  <gs1:netContent>
   <gs1:QuantitativeValue rdf:about="#12xcan341ml-Content">
   <rdf:type rdf:resource="http://qudt.org/1.1/schema/qudt#QuantityValue"/>
   <qudt:unit rdf:resource="http://www.qudt.org/2.1/vocab/unit/MilliL"/>
   <qudt:numericalValue rdf:datatype="http://www.w3.org/2001/XMLSchema#double">4092</qudt:numericalValue>
   <rdf:value rdf:datatype="http://www.w3.org/2001/XMLSchema#double">4092</rdf:value>
   <gs1:unitCode>MLT</gs1:unitCode>
   <gs1:value>4092</gs1:value>
  </gs1:QuantitativeValue>
 </gs1:netContent>
 <sosa:isFeatureOfInterestOf>
  <rdf:Description rdf:about="#12xcan341ml-ContentSosa">
   <rdf:type rdf:resource="http://www.w3.org/ns/sosa/Observation"/>
   <sosa:hasFeatureOfInterest rdf:resource="#12xcan341ml"/>
   <sosa:observedProperty  rdf:resource="#netcontent"/>
   <sosa:hasResult rdf:resource="#12xcan341ml-Content"/>
   <sosa:hasSimpleResult rdf:datatype="http://www.qudt.org/2.1/vocab/unit/MilliM">4092</sosa:hasSimpleResult>
  </rdf:Description>
 </sosa:isFeatureOfInterestOf>
 </rdf:Description>

 <rdf:Description rdf:about="#24xcan341ml">
  <rdf:type rdf:resource="#LiquidContainer"/>
  <rdf:type rdf:resource="#BeverageCan"/>
  <rdf:type rdf:resource="https://gs1.org/voc/PackagingDetails"/>
  <rdfs:label xml:lang="en">24XCan341ml</rdfs:label>
  <rdfs:label xml:lang="fr">24XCan341ml</rdfs:label>
  <skos:definition xml:lang="en">Generic Flat, Box or Crate of 24, 341ml Cans</skos:definition>
  <skos:definition xml:lang="fr">Une boite, caisse ou caissette générique de 24 Canettes de 341ml</skos:definition>
  <rdfs:comment xml:lang="en">This term is meant to be used as a placeholder when no data about the aggregate packaging is known.</rdfs:comment>
  <rdfs:comment xml:lang="fr">Ce terme peut-être utilisé comme un terme générique lorsque les details de l’emballage ne sont pas certain.</rdfs:comment>
  <beer:count rdf:datatype="http://www.w3.org/2001/XMLSchema#Integer">24</beer:count>
  <beer:item rdf:resource="https://rdf.ag/o/beer#can341ml"/>
  <rdfs:isDefinedBy rdf:resource="https://rdf.ag/o/beer-ONTOLOGY_DATE"/>
  <void:inDataset rdf:resource="#datasetdefinition"/>
  <gs1:netContent>
   <gs1:QuantitativeValue rdf:about="#24xcan341ml-Content">
   <rdf:type rdf:resource="http://qudt.org/1.1/schema/qudt#QuantityValue"/>
   <qudt:unit rdf:resource="http://www.qudt.org/2.1/vocab/unit/MilliL"/>
   <qudt:numericalValue rdf:datatype="http://www.w3.org/2001/XMLSchema#double">8184</qudt:numericalValue>
   <rdf:value rdf:datatype="http://www.w3.org/2001/XMLSchema#double">8184</rdf:value>
   <gs1:unitCode>MLT</gs1:unitCode>
   <gs1:value>8184</gs1:value>
  </gs1:QuantitativeValue>
 </gs1:netContent>
 <sosa:isFeatureOfInterestOf>
  <rdf:Description rdf:about="#24xcan341ml-ContentSosa">
   <rdf:type rdf:resource="http://www.w3.org/ns/sosa/Observation"/>
   <sosa:hasFeatureOfInterest rdf:resource="#24xcan341ml"/>
   <sosa:observedProperty  rdf:resource="#netcontent"/>
   <sosa:hasResult rdf:resource="#24xcan341ml-Content"/>
   <sosa:hasSimpleResult rdf:datatype="http://www.qudt.org/2.1/vocab/unit/MilliM">8184</sosa:hasSimpleResult>
  </rdf:Description>
 </sosa:isFeatureOfInterestOf>
 </rdf:Description>

 <rdf:Description rdf:about="#6xcan341ml">
  <rdf:type rdf:resource="#LiquidContainer"/>
  <rdf:type rdf:resource="#BeverageCan"/>
  <rdf:type rdf:resource="https://gs1.org/voc/PackagingDetails"/>
  <rdfs:label xml:lang="en">6XCan341ml</rdfs:label>
  <rdfs:label xml:lang="fr">6XCan341ml</rdfs:label>
  <skos:definition xml:lang="en">Generic Flat, Box or Crate of 6, 341ml Cans</skos:definition>
  <skos:definition xml:lang="fr">Une boite, caisse ou caissette générique de 6 Canettes de 341ml</skos:definition>
  <rdfs:comment xml:lang="en">This term is meant to be used as a placeholder when no data about the aggregate packaging is known.</rdfs:comment>
  <rdfs:comment xml:lang="fr">Ce terme peut-être utilisé comme un terme générique lorsque les details de l’emballage ne sont pas certain.</rdfs:comment>
  <beer:count rdf:datatype="http://www.w3.org/2001/XMLSchema#Integer">6</beer:count>
  <beer:item rdf:resource="https://rdf.ag/o/beer#can341ml"/>
  <rdfs:isDefinedBy rdf:resource="https://rdf.ag/o/beer-ONTOLOGY_DATE"/>
  <void:inDataset rdf:resource="#datasetdefinition"/>
  <gs1:netContent>
   <gs1:QuantitativeValue rdf:about="#6xcan341ml-Content">
   <rdf:type rdf:resource="http://qudt.org/1.1/schema/qudt#QuantityValue"/>
   <qudt:unit rdf:resource="http://www.qudt.org/2.1/vocab/unit/MilliL"/>
   <qudt:numericalValue rdf:datatype="http://www.w3.org/2001/XMLSchema#double">2046</qudt:numericalValue>
   <rdf:value rdf:datatype="http://www.w3.org/2001/XMLSchema#double">2046</rdf:value>
   <gs1:unitCode>MLT</gs1:unitCode>
   <gs1:value>2046</gs1:value>
  </gs1:QuantitativeValue>
 </gs1:netContent>
 <sosa:isFeatureOfInterestOf>
  <rdf:Description rdf:about="#6xcan341ml-ContentSosa">
   <rdf:type rdf:resource="http://www.w3.org/ns/sosa/Observation"/>
   <sosa:hasFeatureOfInterest rdf:resource="#6xcan341ml"/>
   <sosa:observedProperty  rdf:resource="#netcontent"/>
   <sosa:hasResult rdf:resource="#6xcan341ml-Content"/>
   <sosa:hasSimpleResult rdf:datatype="http://www.qudt.org/2.1/vocab/unit/MilliM">2046</sosa:hasSimpleResult>
  </rdf:Description>
 </sosa:isFeatureOfInterestOf>
 </rdf:Description>

 <rdf:Description rdf:about="#24xcan222ml">
  <rdf:type rdf:resource="#LiquidContainer"/>
  <rdf:type rdf:resource="#BeverageCan"/>
  <rdf:type rdf:resource="https://gs1.org/voc/PackagingDetails"/>
  <rdfs:label xml:lang="en">24XCan222ml</rdfs:label>
  <rdfs:label xml:lang="fr">24XCan222ml</rdfs:label>
  <skos:definition xml:lang="en">Generic Flat, Box or Crate of 24, 222ml Cans</skos:definition>
  <skos:definition xml:lang="fr">Une boite, caisse ou caissette générique de 24 Canettes de 222ml</skos:definition>
  <rdfs:comment xml:lang="en">This term is meant to be used as a placeholder when no data about the aggregate packaging is known.</rdfs:comment>
  <rdfs:comment xml:lang="fr">Ce terme peut-être utilisé comme un terme générique lorsque les details de l’emballage ne sont pas certain.</rdfs:comment>
  <beer:count rdf:datatype="http://www.w3.org/2001/XMLSchema#Integer">24</beer:count>
  <beer:item rdf:resource="https://rdf.ag/o/beer#can222ml"/>
  <rdfs:isDefinedBy rdf:resource="https://rdf.ag/o/beer-ONTOLOGY_DATE"/>
  <void:inDataset rdf:resource="#datasetdefinition"/>
  <gs1:netContent>
   <gs1:QuantitativeValue rdf:about="#24xcan222ml-Content">
   <rdf:type rdf:resource="http://qudt.org/1.1/schema/qudt#QuantityValue"/>
   <qudt:unit rdf:resource="http://www.qudt.org/2.1/vocab/unit/MilliL"/>
   <qudt:numericalValue rdf:datatype="http://www.w3.org/2001/XMLSchema#double">5328</qudt:numericalValue>
   <rdf:value rdf:datatype="http://www.w3.org/2001/XMLSchema#double">5328</rdf:value>
   <gs1:unitCode>MLT</gs1:unitCode>
   <gs1:value>5328</gs1:value>
  </gs1:QuantitativeValue>
 </gs1:netContent>
 <sosa:isFeatureOfInterestOf>
  <rdf:Description rdf:about="#24xcan222ml-ContentSosa">
   <rdf:type rdf:resource="http://www.w3.org/ns/sosa/Observation"/>
   <sosa:hasFeatureOfInterest rdf:resource="#24xcan222ml"/>
   <sosa:observedProperty  rdf:resource="#netcontent"/>
   <sosa:hasResult rdf:resource="#24xcan222ml-Content"/>
   <sosa:hasSimpleResult rdf:datatype="http://www.qudt.org/2.1/vocab/unit/MilliM">5328</sosa:hasSimpleResult>
  </rdf:Description>
 </sosa:isFeatureOfInterestOf>
 </rdf:Description>

 <rdf:Description rdf:about="#16xcan222ml">
  <rdf:type rdf:resource="#LiquidContainer"/>
  <rdf:type rdf:resource="#BeverageCan"/>
  <rdf:type rdf:resource="https://gs1.org/voc/PackagingDetails"/>
  <rdfs:label xml:lang="en">16XCan222ml</rdfs:label>
  <rdfs:label xml:lang="fr">16XCan222ml</rdfs:label>
  <skos:definition xml:lang="en">Generic Flat, Box or Crate of 16, 222ml Cans</skos:definition>
  <skos:definition xml:lang="fr">Une boite, caisse ou caissette générique de 16 Canettes de 222ml</skos:definition>
  <rdfs:comment xml:lang="en">This term is meant to be used as a placeholder when no data about the aggregate packaging is known.</rdfs:comment>
  <rdfs:comment xml:lang="fr">Ce terme peut-être utilisé comme un terme générique lorsque les details de l’emballage ne sont pas certain.</rdfs:comment>
  <beer:count rdf:datatype="http://www.w3.org/2001/XMLSchema#Integer">16</beer:count>
  <beer:item rdf:resource="https://rdf.ag/o/beer#can222ml"/>
  <rdfs:isDefinedBy rdf:resource="https://rdf.ag/o/beer-ONTOLOGY_DATE"/>
  <void:inDataset rdf:resource="#datasetdefinition"/>
  <gs1:netContent>
   <gs1:QuantitativeValue rdf:about="#16xcan222ml-Content">
   <rdf:type rdf:resource="http://qudt.org/1.1/schema/qudt#QuantityValue"/>
   <qudt:unit rdf:resource="http://www.qudt.org/2.1/vocab/unit/MilliL"/>
   <qudt:numericalValue rdf:datatype="http://www.w3.org/2001/XMLSchema#double">3552</qudt:numericalValue>
   <rdf:value rdf:datatype="http://www.w3.org/2001/XMLSchema#double">3552</rdf:value>
   <gs1:unitCode>MLT</gs1:unitCode>
   <gs1:value>3552</gs1:value>
  </gs1:QuantitativeValue>
 </gs1:netContent>
 <sosa:isFeatureOfInterestOf>
  <rdf:Description rdf:about="#16xcan222ml-ContentSosa">
   <rdf:type rdf:resource="http://www.w3.org/ns/sosa/Observation"/>
   <sosa:hasFeatureOfInterest rdf:resource="#16xcan222ml"/>
   <sosa:observedProperty  rdf:resource="#netcontent"/>
   <sosa:hasResult rdf:resource="#16xcan222ml-Content"/>
   <sosa:hasSimpleResult rdf:datatype="http://www.qudt.org/2.1/vocab/unit/MilliM">3552</sosa:hasSimpleResult>
  </rdf:Description>
 </sosa:isFeatureOfInterestOf>
 </rdf:Description>

 <rdf:Description rdf:about="#8xcan222ml">
  <rdf:type rdf:resource="#LiquidContainer"/>
  <rdf:type rdf:resource="#BeverageCan"/>
  <rdf:type rdf:resource="https://gs1.org/voc/PackagingDetails"/>
  <rdfs:label xml:lang="en">8XCan222ml</rdfs:label>
  <rdfs:label xml:lang="fr">8XCan222ml</rdfs:label>
  <skos:definition xml:lang="en">Generic Flat, Box or Crate of 8, 222ml Cans</skos:definition>
  <skos:definition xml:lang="fr">Une boite, caisse ou caissette générique de 8 Canettes de 222ml</skos:definition>
  <rdfs:comment xml:lang="en">This term is meant to be used as a placeholder when no data about the aggregate packaging is known.</rdfs:comment>
  <rdfs:comment xml:lang="fr">Ce terme peut-être utilisé comme un terme générique lorsque les details de l’emballage ne sont pas certain.</rdfs:comment>
  <beer:count rdf:datatype="http://www.w3.org/2001/XMLSchema#Integer">8</beer:count>
  <beer:item rdf:resource="https://rdf.ag/o/beer#can222ml"/>
  <rdfs:isDefinedBy rdf:resource="https://rdf.ag/o/beer-ONTOLOGY_DATE"/>
  <void:inDataset rdf:resource="#datasetdefinition"/>
  <gs1:netContent>
   <gs1:QuantitativeValue rdf:about="#8xcan222ml-Content">
   <rdf:type rdf:resource="http://qudt.org/1.1/schema/qudt#QuantityValue"/>
   <qudt:unit rdf:resource="http://www.qudt.org/2.1/vocab/unit/MilliL"/>
   <qudt:numericalValue rdf:datatype="http://www.w3.org/2001/XMLSchema#double">1776</qudt:numericalValue>
   <rdf:value rdf:datatype="http://www.w3.org/2001/XMLSchema#double">1776</rdf:value>
   <gs1:unitCode>MLT</gs1:unitCode>
   <gs1:value>1776</gs1:value>
  </gs1:QuantitativeValue>
 </gs1:netContent>
 <sosa:isFeatureOfInterestOf>
  <rdf:Description rdf:about="#8xcan222ml-ContentSosa">
   <rdf:type rdf:resource="http://www.w3.org/ns/sosa/Observation"/>
   <sosa:hasFeatureOfInterest rdf:resource="#8xcan222ml"/>
   <sosa:observedProperty  rdf:resource="#netcontent"/>
   <sosa:hasResult rdf:resource="#8xcan222ml-Content"/>
   <sosa:hasSimpleResult rdf:datatype="http://www.qudt.org/2.1/vocab/unit/MilliM">1776</sosa:hasSimpleResult>
  </rdf:Description>
 </sosa:isFeatureOfInterestOf>
 </rdf:Description>

 <rdf:Description rdf:about="#2xcan473ml">
  <rdf:type rdf:resource="#LiquidContainer"/>
  <rdf:type rdf:resource="#BeverageCan"/>
  <rdf:type rdf:resource="https://gs1.org/voc/PackagingDetails"/>
  <rdfs:label xml:lang="en">2XCan473ml</rdfs:label>
  <rdfs:label xml:lang="fr">2XCan473ml</rdfs:label>
  <skos:definition xml:lang="en">Generic Flat, Box or Crate of 2, 473ml Cans</skos:definition>
  <skos:definition xml:lang="fr">Une boite, caisse ou caissette générique de 2 Canettes de 473ml</skos:definition>
  <rdfs:comment xml:lang="en">This term is meant to be used as a placeholder when no data about the aggregate packaging is known.</rdfs:comment>
  <rdfs:comment xml:lang="fr">Ce terme peut-être utilisé comme un terme générique lorsque les details de l’emballage ne sont pas certain.</rdfs:comment>
  <beer:count rdf:datatype="http://www.w3.org/2001/XMLSchema#Integer">2</beer:count>
  <beer:item rdf:resource="https://rdf.ag/o/beer#can473ml"/>
  <rdfs:isDefinedBy rdf:resource="https://rdf.ag/o/beer-ONTOLOGY_DATE"/>
  <void:inDataset rdf:resource="#datasetdefinition"/>
  <gs1:netContent>
   <gs1:QuantitativeValue rdf:about="#2xcan473ml-Content">
   <rdf:type rdf:resource="http://qudt.org/1.1/schema/qudt#QuantityValue"/>
   <qudt:unit rdf:resource="http://www.qudt.org/2.1/vocab/unit/MilliL"/>
   <qudt:numericalValue rdf:datatype="http://www.w3.org/2001/XMLSchema#double">946</qudt:numericalValue>
   <rdf:value rdf:datatype="http://www.w3.org/2001/XMLSchema#double">946</rdf:value>
   <gs1:unitCode>MLT</gs1:unitCode>
   <gs1:value>946</gs1:value>
  </gs1:QuantitativeValue>
 </gs1:netContent>
 <sosa:isFeatureOfInterestOf>
  <rdf:Description rdf:about="#2xcan473ml-ContentSosa">
   <rdf:type rdf:resource="http://www.w3.org/ns/sosa/Observation"/>
   <sosa:hasFeatureOfInterest rdf:resource="#2xcan473ml"/>
   <sosa:observedProperty  rdf:resource="#netcontent"/>
   <sosa:hasResult rdf:resource="#2xcan473ml-Content"/>
   <sosa:hasSimpleResult rdf:datatype="http://www.qudt.org/2.1/vocab/unit/MilliM">946</sosa:hasSimpleResult>
  </rdf:Description>
 </sosa:isFeatureOfInterestOf>
 </rdf:Description>

 <rdf:Description rdf:about="#12xcan473ml">
  <rdf:type rdf:resource="#LiquidContainer"/>
  <rdf:type rdf:resource="#BeverageCan"/>
  <rdf:type rdf:resource="https://gs1.org/voc/PackagingDetails"/>
  <rdfs:label xml:lang="en">12XCan473ml</rdfs:label>
  <rdfs:label xml:lang="fr">12XCan473ml</rdfs:label>
  <skos:definition xml:lang="en">Generic Flat, Box or Crate of 12, 473ml Cans</skos:definition>
  <skos:definition xml:lang="fr">Une boite, caisse ou caissette générique de 12 Canettes de 473ml</skos:definition>
  <rdfs:comment xml:lang="en">This term is meant to be used as a placeholder when no data about the aggregate packaging is known.</rdfs:comment>
  <rdfs:comment xml:lang="fr">Ce terme peut-être utilisé comme un terme générique lorsque les details de l’emballage ne sont pas certain.</rdfs:comment>
  <beer:count rdf:datatype="http://www.w3.org/2001/XMLSchema#Integer">12</beer:count>
  <beer:item rdf:resource="https://rdf.ag/o/beer#can473ml"/>
  <rdfs:isDefinedBy rdf:resource="https://rdf.ag/o/beer-ONTOLOGY_DATE"/>
  <void:inDataset rdf:resource="#datasetdefinition"/>
  <gs1:netContent>
   <gs1:QuantitativeValue rdf:about="#12xcan473ml-Content">
   <rdf:type rdf:resource="http://qudt.org/1.1/schema/qudt#QuantityValue"/>
   <qudt:unit rdf:resource="http://www.qudt.org/2.1/vocab/unit/MilliL"/>
   <qudt:numericalValue rdf:datatype="http://www.w3.org/2001/XMLSchema#double">5676</qudt:numericalValue>
   <rdf:value rdf:datatype="http://www.w3.org/2001/XMLSchema#double">5676</rdf:value>
   <gs1:unitCode>MLT</gs1:unitCode>
   <gs1:value>5676</gs1:value>
  </gs1:QuantitativeValue>
 </gs1:netContent>
 <sosa:isFeatureOfInterestOf>
  <rdf:Description rdf:about="#12xcan473ml-ContentSosa">
   <rdf:type rdf:resource="http://www.w3.org/ns/sosa/Observation"/>
   <sosa:hasFeatureOfInterest rdf:resource="#12xcan473ml"/>
   <sosa:observedProperty  rdf:resource="#netcontent"/>
   <sosa:hasResult rdf:resource="#12xcan473ml-Content"/>
   <sosa:hasSimpleResult rdf:datatype="http://www.qudt.org/2.1/vocab/unit/MilliM">5676</sosa:hasSimpleResult>
  </rdf:Description>
 </sosa:isFeatureOfInterestOf>
 </rdf:Description>

 <rdf:Description rdf:about="#3xcan473ml">
  <rdf:type rdf:resource="#LiquidContainer"/>
  <rdf:type rdf:resource="#BeverageCan"/>
  <rdf:type rdf:resource="https://gs1.org/voc/PackagingDetails"/>
  <rdfs:label xml:lang="en">3XCan473ml</rdfs:label>
  <rdfs:label xml:lang="fr">3XCan473ml</rdfs:label>
  <skos:definition xml:lang="en">Generic Flat, Box or Crate of 3, 473ml Cans</skos:definition>
  <skos:definition xml:lang="fr">Une boite, caisse ou caissette générique de 3 Canettes de 473ml</skos:definition>
  <rdfs:comment xml:lang="en">This term is meant to be used as a placeholder when no data about the aggregate packaging is known.</rdfs:comment>
  <rdfs:comment xml:lang="fr">Ce terme peut-être utilisé comme un terme générique lorsque les details de l’emballage ne sont pas certain.</rdfs:comment>
  <beer:count rdf:datatype="http://www.w3.org/2001/XMLSchema#Integer">3</beer:count>
  <beer:item rdf:resource="https://rdf.ag/o/beer#can473ml"/>
  <rdfs:isDefinedBy rdf:resource="https://rdf.ag/o/beer-ONTOLOGY_DATE"/>
  <void:inDataset rdf:resource="#datasetdefinition"/>
  <gs1:netContent>
   <gs1:QuantitativeValue rdf:about="#3xcan473ml-Content">
   <rdf:type rdf:resource="http://qudt.org/1.1/schema/qudt#QuantityValue"/>
   <qudt:unit rdf:resource="http://www.qudt.org/2.1/vocab/unit/MilliL"/>
   <qudt:numericalValue rdf:datatype="http://www.w3.org/2001/XMLSchema#double">1419</qudt:numericalValue>
   <rdf:value rdf:datatype="http://www.w3.org/2001/XMLSchema#double">1419</rdf:value>
   <gs1:unitCode>MLT</gs1:unitCode>
   <gs1:value>1419</gs1:value>
  </gs1:QuantitativeValue>
 </gs1:netContent>
 <sosa:isFeatureOfInterestOf>
  <rdf:Description rdf:about="#3xcan473ml-ContentSosa">
   <rdf:type rdf:resource="http://www.w3.org/ns/sosa/Observation"/>
   <sosa:hasFeatureOfInterest rdf:resource="#3xcan473ml"/>
   <sosa:observedProperty  rdf:resource="#netcontent"/>
   <sosa:hasResult rdf:resource="#3xcan473ml-Content"/>
   <sosa:hasSimpleResult rdf:datatype="http://www.qudt.org/2.1/vocab/unit/MilliM">1419</sosa:hasSimpleResult>
  </rdf:Description>
 </sosa:isFeatureOfInterestOf>
 </rdf:Description>

 <rdf:Description rdf:about="#4xcan473ml">
  <rdf:type rdf:resource="#LiquidContainer"/>
  <rdf:type rdf:resource="#BeverageCan"/>
  <rdf:type rdf:resource="https://gs1.org/voc/PackagingDetails"/>
  <rdfs:label xml:lang="en">4XCan473ml</rdfs:label>
  <rdfs:label xml:lang="fr">4XCan473ml</rdfs:label>
  <skos:definition xml:lang="en">Generic Flat, Box or Crate of 4, 473ml Cans</skos:definition>
  <skos:definition xml:lang="fr">Une boite, caisse ou caissette générique de 4 Canettes de 473ml</skos:definition>
  <rdfs:comment xml:lang="en">This term is meant to be used as a placeholder when no data about the aggregate packaging is known.</rdfs:comment>
  <rdfs:comment xml:lang="fr">Ce terme peut-être utilisé comme un terme générique lorsque les details de l’emballage ne sont pas certain.</rdfs:comment>
  <beer:count rdf:datatype="http://www.w3.org/2001/XMLSchema#Integer">4</beer:count>
  <beer:item rdf:resource="https://rdf.ag/o/beer#can473ml"/>
  <rdfs:isDefinedBy rdf:resource="https://rdf.ag/o/beer-ONTOLOGY_DATE"/>
  <void:inDataset rdf:resource="#datasetdefinition"/>
  <gs1:netContent>
   <gs1:QuantitativeValue rdf:about="#4xcan473ml-Content">
   <rdf:type rdf:resource="http://qudt.org/1.1/schema/qudt#QuantityValue"/>
   <qudt:unit rdf:resource="http://www.qudt.org/2.1/vocab/unit/MilliL"/>
   <qudt:numericalValue rdf:datatype="http://www.w3.org/2001/XMLSchema#double">1892</qudt:numericalValue>
   <rdf:value rdf:datatype="http://www.w3.org/2001/XMLSchema#double">1892</rdf:value>
   <gs1:unitCode>MLT</gs1:unitCode>
   <gs1:value>1892</gs1:value>
  </gs1:QuantitativeValue>
 </gs1:netContent>
 <sosa:isFeatureOfInterestOf>
  <rdf:Description rdf:about="#4xcan473ml-ContentSosa">
   <rdf:type rdf:resource="http://www.w3.org/ns/sosa/Observation"/>
   <sosa:hasFeatureOfInterest rdf:resource="#4xcan473ml"/>
   <sosa:observedProperty  rdf:resource="#netcontent"/>
   <sosa:hasResult rdf:resource="#4xcan473ml-Content"/>
   <sosa:hasSimpleResult rdf:datatype="http://www.qudt.org/2.1/vocab/unit/MilliM">1892</sosa:hasSimpleResult>
  </rdf:Description>
 </sosa:isFeatureOfInterestOf>
 </rdf:Description>

 <rdf:Description rdf:about="#24xcan473ml">
  <rdf:type rdf:resource="#LiquidContainer"/>
  <rdf:type rdf:resource="#BeverageCan"/>
  <rdf:type rdf:resource="https://gs1.org/voc/PackagingDetails"/>
  <rdfs:label xml:lang="en">24XCan473ml</rdfs:label>
  <rdfs:label xml:lang="fr">24XCan473ml</rdfs:label>
  <skos:definition xml:lang="en">Generic Flat, Box or Crate of 24, 473ml Cans</skos:definition>
  <skos:definition xml:lang="fr">Une boite, caisse ou caissette générique de 24 Canettes de 473ml</skos:definition>
  <rdfs:comment xml:lang="en">This term is meant to be used as a placeholder when no data about the aggregate packaging is known.</rdfs:comment>
  <rdfs:comment xml:lang="fr">Ce terme peut-être utilisé comme un terme générique lorsque les details de l’emballage ne sont pas certain.</rdfs:comment>
  <beer:count rdf:datatype="http://www.w3.org/2001/XMLSchema#Integer">24</beer:count>
  <beer:item rdf:resource="https://rdf.ag/o/beer#can473ml"/>
  <rdfs:isDefinedBy rdf:resource="https://rdf.ag/o/beer-ONTOLOGY_DATE"/>
  <void:inDataset rdf:resource="#datasetdefinition"/>
  <gs1:netContent>
   <gs1:QuantitativeValue rdf:about="#24xcan473ml-Content">
   <rdf:type rdf:resource="http://qudt.org/1.1/schema/qudt#QuantityValue"/>
   <qudt:unit rdf:resource="http://www.qudt.org/2.1/vocab/unit/MilliL"/>
   <qudt:numericalValue rdf:datatype="http://www.w3.org/2001/XMLSchema#double">11352</qudt:numericalValue>
   <rdf:value rdf:datatype="http://www.w3.org/2001/XMLSchema#double">11352</rdf:value>
   <gs1:unitCode>MLT</gs1:unitCode>
   <gs1:value>11352</gs1:value>
  </gs1:QuantitativeValue>
 </gs1:netContent>
 <sosa:isFeatureOfInterestOf>
  <rdf:Description rdf:about="#24xcan473ml-ContentSosa">
   <rdf:type rdf:resource="http://www.w3.org/ns/sosa/Observation"/>
   <sosa:hasFeatureOfInterest rdf:resource="#24xcan473ml"/>
   <sosa:observedProperty  rdf:resource="#netcontent"/>
   <sosa:hasResult rdf:resource="#24xcan473ml-Content"/>
   <sosa:hasSimpleResult rdf:datatype="http://www.qudt.org/2.1/vocab/unit/MilliM">11352</sosa:hasSimpleResult>
  </rdf:Description>
 </sosa:isFeatureOfInterestOf>
 </rdf:Description>

 <rdf:Description rdf:about="#6xcan473ml">
  <rdf:type rdf:resource="#LiquidContainer"/>
  <rdf:type rdf:resource="#BeverageCan"/>
  <rdf:type rdf:resource="https://gs1.org/voc/PackagingDetails"/>
  <rdfs:label xml:lang="en">6XCan473ml</rdfs:label>
  <rdfs:label xml:lang="fr">6XCan473ml</rdfs:label>
  <skos:definition xml:lang="en">Generic Flat, Box or Crate of 6, 473ml Cans</skos:definition>
  <skos:definition xml:lang="fr">Une boite, caisse ou caissette générique de 6 Canettes de 473ml</skos:definition>
  <rdfs:comment xml:lang="en">This term is meant to be used as a placeholder when no data about the aggregate packaging is known.</rdfs:comment>
  <rdfs:comment xml:lang="fr">Ce terme peut-être utilisé comme un terme générique lorsque les details de l’emballage ne sont pas certain.</rdfs:comment>
  <beer:count rdf:datatype="http://www.w3.org/2001/XMLSchema#Integer">6</beer:count>
  <beer:item rdf:resource="https://rdf.ag/o/beer#can473ml"/>
  <rdfs:isDefinedBy rdf:resource="https://rdf.ag/o/beer-ONTOLOGY_DATE"/>
  <void:inDataset rdf:resource="#datasetdefinition"/>
  <gs1:netContent>
   <gs1:QuantitativeValue rdf:about="#6xcan473ml-Content">
   <rdf:type rdf:resource="http://qudt.org/1.1/schema/qudt#QuantityValue"/>
   <qudt:unit rdf:resource="http://www.qudt.org/2.1/vocab/unit/MilliL"/>
   <qudt:numericalValue rdf:datatype="http://www.w3.org/2001/XMLSchema#double">2838</qudt:numericalValue>
   <rdf:value rdf:datatype="http://www.w3.org/2001/XMLSchema#double">2838</rdf:value>
   <gs1:unitCode>MLT</gs1:unitCode>
   <gs1:value>2838</gs1:value>
  </gs1:QuantitativeValue>
 </gs1:netContent>
 <sosa:isFeatureOfInterestOf>
  <rdf:Description rdf:about="#6xcan473ml-ContentSosa">
   <rdf:type rdf:resource="http://www.w3.org/ns/sosa/Observation"/>
   <sosa:hasFeatureOfInterest rdf:resource="#6xcan473ml"/>
   <sosa:observedProperty  rdf:resource="#netcontent"/>
   <sosa:hasResult rdf:resource="#6xcan473ml-Content"/>
   <sosa:hasSimpleResult rdf:datatype="http://www.qudt.org/2.1/vocab/unit/MilliM">2838</sosa:hasSimpleResult>
  </rdf:Description>
 </sosa:isFeatureOfInterestOf>
 </rdf:Description>

 <rdf:Description rdf:about="#16xcan473ml">
  <rdf:type rdf:resource="#LiquidContainer"/>
  <rdf:type rdf:resource="#BeverageCan"/>
  <rdf:type rdf:resource="https://gs1.org/voc/PackagingDetails"/>
  <rdfs:label xml:lang="en">16XCan473ml</rdfs:label>
  <rdfs:label xml:lang="fr">16XCan473ml</rdfs:label>
  <skos:definition xml:lang="en">Generic Flat, Box or Crate of 16, 473ml Cans</skos:definition>
  <skos:definition xml:lang="fr">Une boite, caisse ou caissette générique de 16 Canettes de 473ml</skos:definition>
  <rdfs:comment xml:lang="en">This term is meant to be used as a placeholder when no data about the aggregate packaging is known.</rdfs:comment>
  <rdfs:comment xml:lang="fr">Ce terme peut-être utilisé comme un terme générique lorsque les details de l’emballage ne sont pas certain.</rdfs:comment>
  <beer:count rdf:datatype="http://www.w3.org/2001/XMLSchema#Integer">16</beer:count>
  <beer:item rdf:resource="https://rdf.ag/o/beer#can473ml"/>
  <rdfs:isDefinedBy rdf:resource="https://rdf.ag/o/beer-ONTOLOGY_DATE"/>
  <void:inDataset rdf:resource="#datasetdefinition"/>
  <gs1:netContent>
   <gs1:QuantitativeValue rdf:about="#16xcan473ml-Content">
   <rdf:type rdf:resource="http://qudt.org/1.1/schema/qudt#QuantityValue"/>
   <qudt:unit rdf:resource="http://www.qudt.org/2.1/vocab/unit/MilliL"/>
   <qudt:numericalValue rdf:datatype="http://www.w3.org/2001/XMLSchema#double">7568</qudt:numericalValue>
   <rdf:value rdf:datatype="http://www.w3.org/2001/XMLSchema#double">7568</rdf:value>
   <gs1:unitCode>MLT</gs1:unitCode>
   <gs1:value>7568</gs1:value>
  </gs1:QuantitativeValue>
 </gs1:netContent>
 <sosa:isFeatureOfInterestOf>
  <rdf:Description rdf:about="#16xcan473ml-ContentSosa">
   <rdf:type rdf:resource="http://www.w3.org/ns/sosa/Observation"/>
   <sosa:hasFeatureOfInterest rdf:resource="#16xcan473ml"/>
   <sosa:observedProperty  rdf:resource="#netcontent"/>
   <sosa:hasResult rdf:resource="#16xcan473ml-Content"/>
   <sosa:hasSimpleResult rdf:datatype="http://www.qudt.org/2.1/vocab/unit/MilliM">7568</sosa:hasSimpleResult>
  </rdf:Description>
 </sosa:isFeatureOfInterestOf>
 </rdf:Description>

 <rdf:Description rdf:about="#96xcan473ml">
  <rdf:type rdf:resource="#LiquidContainer"/>
  <rdf:type rdf:resource="#BeverageCan"/>
  <rdf:type rdf:resource="https://gs1.org/voc/PackagingDetails"/>
  <rdfs:label xml:lang="en">96XCan473ml</rdfs:label>
  <rdfs:label xml:lang="fr">96XCan473ml</rdfs:label>
  <skos:definition xml:lang="en">Generic Flat, Box or Crate of 96, 473ml Cans</skos:definition>
  <skos:definition xml:lang="fr">Une boite, caisse ou caissette générique de 96 Canettes de 473ml</skos:definition>
  <rdfs:comment xml:lang="en">This term is meant to be used as a placeholder when no data about the aggregate packaging is known.</rdfs:comment>
  <rdfs:comment xml:lang="fr">Ce terme peut-être utilisé comme un terme générique lorsque les details de l’emballage ne sont pas certain.</rdfs:comment>
  <beer:count rdf:datatype="http://www.w3.org/2001/XMLSchema#Integer">96</beer:count>
  <beer:item rdf:resource="https://rdf.ag/o/beer#can473ml"/>
  <rdfs:isDefinedBy rdf:resource="https://rdf.ag/o/beer-ONTOLOGY_DATE"/>
  <void:inDataset rdf:resource="#datasetdefinition"/>
  <gs1:netContent>
   <gs1:QuantitativeValue rdf:about="#96xcan473ml-Content">
   <rdf:type rdf:resource="http://qudt.org/1.1/schema/qudt#QuantityValue"/>
   <qudt:unit rdf:resource="http://www.qudt.org/2.1/vocab/unit/MilliL"/>
   <qudt:numericalValue rdf:datatype="http://www.w3.org/2001/XMLSchema#double">45408</qudt:numericalValue>
   <rdf:value rdf:datatype="http://www.w3.org/2001/XMLSchema#double">45408</rdf:value>
   <gs1:unitCode>MLT</gs1:unitCode>
   <gs1:value>45408</gs1:value>
  </gs1:QuantitativeValue>
 </gs1:netContent>
 <sosa:isFeatureOfInterestOf>
  <rdf:Description rdf:about="#96xcan473ml-ContentSosa">
   <rdf:type rdf:resource="http://www.w3.org/ns/sosa/Observation"/>
   <sosa:hasFeatureOfInterest rdf:resource="#96xcan473ml"/>
   <sosa:observedProperty  rdf:resource="#netcontent"/>
   <sosa:hasResult rdf:resource="#96xcan473ml-Content"/>
   <sosa:hasSimpleResult rdf:datatype="http://www.qudt.org/2.1/vocab/unit/MilliM">45408</sosa:hasSimpleResult>
  </rdf:Description>
 </sosa:isFeatureOfInterestOf>
 </rdf:Description>

 <rdf:Description rdf:about="#8xcan473ml">
  <rdf:type rdf:resource="#LiquidContainer"/>
  <rdf:type rdf:resource="#BeverageCan"/>
  <rdf:type rdf:resource="https://gs1.org/voc/PackagingDetails"/>
  <rdfs:label xml:lang="en">8XCan473ml</rdfs:label>
  <rdfs:label xml:lang="fr">8XCan473ml</rdfs:label>
  <skos:definition xml:lang="en">Generic Flat, Box or Crate of 8, 473ml Cans</skos:definition>
  <skos:definition xml:lang="fr">Une boite, caisse ou caissette générique de 8 Canettes de 473ml</skos:definition>
  <rdfs:comment xml:lang="en">This term is meant to be used as a placeholder when no data about the aggregate packaging is known.</rdfs:comment>
  <rdfs:comment xml:lang="fr">Ce terme peut-être utilisé comme un terme générique lorsque les details de l’emballage ne sont pas certain.</rdfs:comment>
  <beer:count rdf:datatype="http://www.w3.org/2001/XMLSchema#Integer">8</beer:count>
  <beer:item rdf:resource="https://rdf.ag/o/beer#can473ml"/>
  <rdfs:isDefinedBy rdf:resource="https://rdf.ag/o/beer-ONTOLOGY_DATE"/>
  <void:inDataset rdf:resource="#datasetdefinition"/>
  <gs1:netContent>
   <gs1:QuantitativeValue rdf:about="#8xcan473ml-Content">
   <rdf:type rdf:resource="http://qudt.org/1.1/schema/qudt#QuantityValue"/>
   <qudt:unit rdf:resource="http://www.qudt.org/2.1/vocab/unit/MilliL"/>
   <qudt:numericalValue rdf:datatype="http://www.w3.org/2001/XMLSchema#double">3784</qudt:numericalValue>
   <rdf:value rdf:datatype="http://www.w3.org/2001/XMLSchema#double">3784</rdf:value>
   <gs1:unitCode>MLT</gs1:unitCode>
   <gs1:value>3784</gs1:value>
  </gs1:QuantitativeValue>
 </gs1:netContent>
 <sosa:isFeatureOfInterestOf>
  <rdf:Description rdf:about="#8xcan473ml-ContentSosa">
   <rdf:type rdf:resource="http://www.w3.org/ns/sosa/Observation"/>
   <sosa:hasFeatureOfInterest rdf:resource="#8xcan473ml"/>
   <sosa:observedProperty  rdf:resource="#netcontent"/>
   <sosa:hasResult rdf:resource="#8xcan473ml-Content"/>
   <sosa:hasSimpleResult rdf:datatype="http://www.qudt.org/2.1/vocab/unit/MilliM">3784</sosa:hasSimpleResult>
  </rdf:Description>
 </sosa:isFeatureOfInterestOf>
 </rdf:Description>

 <rdf:Description rdf:about="#18xcan473ml">
  <rdf:type rdf:resource="#LiquidContainer"/>
  <rdf:type rdf:resource="#BeverageCan"/>
  <rdf:type rdf:resource="https://gs1.org/voc/PackagingDetails"/>
  <rdfs:label xml:lang="en">18XCan473ml</rdfs:label>
  <rdfs:label xml:lang="fr">18XCan473ml</rdfs:label>
  <skos:definition xml:lang="en">Generic Flat, Box or Crate of 18, 473ml Cans</skos:definition>
  <skos:definition xml:lang="fr">Une boite, caisse ou caissette générique de 18 Canettes de 473ml</skos:definition>
  <rdfs:comment xml:lang="en">This term is meant to be used as a placeholder when no data about the aggregate packaging is known.</rdfs:comment>
  <rdfs:comment xml:lang="fr">Ce terme peut-être utilisé comme un terme générique lorsque les details de l’emballage ne sont pas certain.</rdfs:comment>
  <beer:count rdf:datatype="http://www.w3.org/2001/XMLSchema#Integer">18</beer:count>
  <beer:item rdf:resource="https://rdf.ag/o/beer#can473ml"/>
  <rdfs:isDefinedBy rdf:resource="https://rdf.ag/o/beer-ONTOLOGY_DATE"/>
  <void:inDataset rdf:resource="#datasetdefinition"/>
  <gs1:netContent>
   <gs1:QuantitativeValue rdf:about="#18xcan473ml-Content">
   <rdf:type rdf:resource="http://qudt.org/1.1/schema/qudt#QuantityValue"/>
   <qudt:unit rdf:resource="http://www.qudt.org/2.1/vocab/unit/MilliL"/>
   <qudt:numericalValue rdf:datatype="http://www.w3.org/2001/XMLSchema#double">8514</qudt:numericalValue>
   <rdf:value rdf:datatype="http://www.w3.org/2001/XMLSchema#double">8514</rdf:value>
   <gs1:unitCode>MLT</gs1:unitCode>
   <gs1:value>8514</gs1:value>
  </gs1:QuantitativeValue>
 </gs1:netContent>
 <sosa:isFeatureOfInterestOf>
  <rdf:Description rdf:about="#18xcan473ml-ContentSosa">
   <rdf:type rdf:resource="http://www.w3.org/ns/sosa/Observation"/>
   <sosa:hasFeatureOfInterest rdf:resource="#18xcan473ml"/>
   <sosa:observedProperty  rdf:resource="#netcontent"/>
   <sosa:hasResult rdf:resource="#18xcan473ml-Content"/>
   <sosa:hasSimpleResult rdf:datatype="http://www.qudt.org/2.1/vocab/unit/MilliM">8514</sosa:hasSimpleResult>
  </rdf:Description>
 </sosa:isFeatureOfInterestOf>
 </rdf:Description>

 <rdf:Description rdf:about="#8xbottle1183ml">
  <rdf:type rdf:resource="#LiquidContainer"/>
  <rdf:type rdf:resource="#BeverageBottle"/>
  <rdf:type rdf:resource="https://gs1.org/voc/PackagingDetails"/>
  <rdfs:label xml:lang="en">8XBottle1183ml</rdfs:label>
  <rdfs:label xml:lang="fr">8XBottle1183ml</rdfs:label>
  <skos:definition xml:lang="en">Generic Flat, Box or Crate of 8, 1183ml Bottles</skos:definition>
  <skos:definition xml:lang="fr">Une boite, caisse ou caissette générique de 8 Bouteilles de 1183ml</skos:definition>
  <rdfs:comment xml:lang="en">This term is meant to be used as a placeholder when no data about the aggregate packaging is known.</rdfs:comment>
  <rdfs:comment xml:lang="fr">Ce terme peut-être utilisé comme un terme générique lorsque les details de l’emballage ne sont pas certain.</rdfs:comment>
  <beer:count rdf:datatype="http://www.w3.org/2001/XMLSchema#Integer">8</beer:count>
  <beer:item rdf:resource="https://rdf.ag/o/beer#bottle1183ml"/>
  <rdfs:isDefinedBy rdf:resource="https://rdf.ag/o/beer-ONTOLOGY_DATE"/>
  <void:inDataset rdf:resource="#datasetdefinition"/>
  <gs1:netContent>
   <gs1:QuantitativeValue rdf:about="#8xbottle1183ml-Content">
   <rdf:type rdf:resource="http://qudt.org/1.1/schema/qudt#QuantityValue"/>
   <qudt:unit rdf:resource="http://www.qudt.org/2.1/vocab/unit/MilliL"/>
   <qudt:numericalValue rdf:datatype="http://www.w3.org/2001/XMLSchema#double">9464</qudt:numericalValue>
   <rdf:value rdf:datatype="http://www.w3.org/2001/XMLSchema#double">9464</rdf:value>
   <gs1:unitCode>MLT</gs1:unitCode>
   <gs1:value>9464</gs1:value>
  </gs1:QuantitativeValue>
 </gs1:netContent>
 <sosa:isFeatureOfInterestOf>
  <rdf:Description rdf:about="#8xbottle1183ml-ContentSosa">
   <rdf:type rdf:resource="http://www.w3.org/ns/sosa/Observation"/>
   <sosa:hasFeatureOfInterest rdf:resource="#8xbottle1183ml"/>
   <sosa:observedProperty  rdf:resource="#netcontent"/>
   <sosa:hasResult rdf:resource="#8xbottle1183ml-Content"/>
   <sosa:hasSimpleResult rdf:datatype="http://www.qudt.org/2.1/vocab/unit/MilliM">9464</sosa:hasSimpleResult>
  </rdf:Description>
 </sosa:isFeatureOfInterestOf>
 </rdf:Description>

 <rdf:Description rdf:about="#24xbottle284ml">
  <rdf:type rdf:resource="#LiquidContainer"/>
  <rdf:type rdf:resource="#BeverageBottle"/>
  <rdf:type rdf:resource="https://gs1.org/voc/PackagingDetails"/>
  <rdfs:label xml:lang="en">24XBottle284ml</rdfs:label>
  <rdfs:label xml:lang="fr">24XBottle284ml</rdfs:label>
  <skos:definition xml:lang="en">Generic Flat, Box or Crate of 24, 284ml Bottles</skos:definition>
  <skos:definition xml:lang="fr">Une boite, caisse ou caissette générique de 24 Bouteilles de 284ml</skos:definition>
  <rdfs:comment xml:lang="en">This term is meant to be used as a placeholder when no data about the aggregate packaging is known.</rdfs:comment>
  <rdfs:comment xml:lang="fr">Ce terme peut-être utilisé comme un terme générique lorsque les details de l’emballage ne sont pas certain.</rdfs:comment>
  <beer:count rdf:datatype="http://www.w3.org/2001/XMLSchema#Integer">24</beer:count>
  <beer:item rdf:resource="https://rdf.ag/o/beer#bottle284ml"/>
  <rdfs:isDefinedBy rdf:resource="https://rdf.ag/o/beer-ONTOLOGY_DATE"/>
  <void:inDataset rdf:resource="#datasetdefinition"/>
  <gs1:netContent>
   <gs1:QuantitativeValue rdf:about="#24xbottle284ml-Content">
   <rdf:type rdf:resource="http://qudt.org/1.1/schema/qudt#QuantityValue"/>
   <qudt:unit rdf:resource="http://www.qudt.org/2.1/vocab/unit/MilliL"/>
   <qudt:numericalValue rdf:datatype="http://www.w3.org/2001/XMLSchema#double">6816</qudt:numericalValue>
   <rdf:value rdf:datatype="http://www.w3.org/2001/XMLSchema#double">6816</rdf:value>
   <gs1:unitCode>MLT</gs1:unitCode>
   <gs1:value>6816</gs1:value>
  </gs1:QuantitativeValue>
 </gs1:netContent>
 <sosa:isFeatureOfInterestOf>
  <rdf:Description rdf:about="#24xbottle284ml-ContentSosa">
   <rdf:type rdf:resource="http://www.w3.org/ns/sosa/Observation"/>
   <sosa:hasFeatureOfInterest rdf:resource="#24xbottle284ml"/>
   <sosa:observedProperty  rdf:resource="#netcontent"/>
   <sosa:hasResult rdf:resource="#24xbottle284ml-Content"/>
   <sosa:hasSimpleResult rdf:datatype="http://www.qudt.org/2.1/vocab/unit/MilliM">6816</sosa:hasSimpleResult>
  </rdf:Description>
 </sosa:isFeatureOfInterestOf>
 </rdf:Description>

 <rdf:Description rdf:about="#6xbottle284ml">
  <rdf:type rdf:resource="#LiquidContainer"/>
  <rdf:type rdf:resource="#BeverageBottle"/>
  <rdf:type rdf:resource="https://gs1.org/voc/PackagingDetails"/>
  <rdfs:label xml:lang="en">6XBottle284ml</rdfs:label>
  <rdfs:label xml:lang="fr">6XBottle284ml</rdfs:label>
  <skos:definition xml:lang="en">Generic Flat, Box or Crate of 6, 284ml Bottles</skos:definition>
  <skos:definition xml:lang="fr">Une boite, caisse ou caissette générique de 6 Bouteilles de 284ml</skos:definition>
  <rdfs:comment xml:lang="en">This term is meant to be used as a placeholder when no data about the aggregate packaging is known.</rdfs:comment>
  <rdfs:comment xml:lang="fr">Ce terme peut-être utilisé comme un terme générique lorsque les details de l’emballage ne sont pas certain.</rdfs:comment>
  <beer:count rdf:datatype="http://www.w3.org/2001/XMLSchema#Integer">6</beer:count>
  <beer:item rdf:resource="https://rdf.ag/o/beer#bottle284ml"/>
  <rdfs:isDefinedBy rdf:resource="https://rdf.ag/o/beer-ONTOLOGY_DATE"/>
  <void:inDataset rdf:resource="#datasetdefinition"/>
  <gs1:netContent>
   <gs1:QuantitativeValue rdf:about="#6xbottle284ml-Content">
   <rdf:type rdf:resource="http://qudt.org/1.1/schema/qudt#QuantityValue"/>
   <qudt:unit rdf:resource="http://www.qudt.org/2.1/vocab/unit/MilliL"/>
   <qudt:numericalValue rdf:datatype="http://www.w3.org/2001/XMLSchema#double">1704</qudt:numericalValue>
   <rdf:value rdf:datatype="http://www.w3.org/2001/XMLSchema#double">1704</rdf:value>
   <gs1:unitCode>MLT</gs1:unitCode>
   <gs1:value>1704</gs1:value>
  </gs1:QuantitativeValue>
 </gs1:netContent>
 <sosa:isFeatureOfInterestOf>
  <rdf:Description rdf:about="#6xbottle284ml-ContentSosa">
   <rdf:type rdf:resource="http://www.w3.org/ns/sosa/Observation"/>
   <sosa:hasFeatureOfInterest rdf:resource="#6xbottle284ml"/>
   <sosa:observedProperty  rdf:resource="#netcontent"/>
   <sosa:hasResult rdf:resource="#6xbottle284ml-Content"/>
   <sosa:hasSimpleResult rdf:datatype="http://www.qudt.org/2.1/vocab/unit/MilliM">1704</sosa:hasSimpleResult>
  </rdf:Description>
 </sosa:isFeatureOfInterestOf>
 </rdf:Description>

 <rdf:Description rdf:about="#12xbottle625ml">
  <rdf:type rdf:resource="#LiquidContainer"/>
  <rdf:type rdf:resource="#BeverageBottle"/>
  <rdf:type rdf:resource="https://gs1.org/voc/PackagingDetails"/>
  <rdfs:label xml:lang="en">12XBottle625ml</rdfs:label>
  <rdfs:label xml:lang="fr">12XBottle625ml</rdfs:label>
  <skos:definition xml:lang="en">Generic Flat, Box or Crate of 12, 625ml Bottles</skos:definition>
  <skos:definition xml:lang="fr">Une boite, caisse ou caissette générique de 12 Bouteilles de 625ml</skos:definition>
  <rdfs:comment xml:lang="en">This term is meant to be used as a placeholder when no data about the aggregate packaging is known.</rdfs:comment>
  <rdfs:comment xml:lang="fr">Ce terme peut-être utilisé comme un terme générique lorsque les details de l’emballage ne sont pas certain.</rdfs:comment>
  <beer:count rdf:datatype="http://www.w3.org/2001/XMLSchema#Integer">12</beer:count>
  <beer:item rdf:resource="https://rdf.ag/o/beer#bottle625ml"/>
  <rdfs:isDefinedBy rdf:resource="https://rdf.ag/o/beer-ONTOLOGY_DATE"/>
  <void:inDataset rdf:resource="#datasetdefinition"/>
  <gs1:netContent>
   <gs1:QuantitativeValue rdf:about="#12xbottle625ml-Content">
   <rdf:type rdf:resource="http://qudt.org/1.1/schema/qudt#QuantityValue"/>
   <qudt:unit rdf:resource="http://www.qudt.org/2.1/vocab/unit/MilliL"/>
   <qudt:numericalValue rdf:datatype="http://www.w3.org/2001/XMLSchema#double">7500</qudt:numericalValue>
   <rdf:value rdf:datatype="http://www.w3.org/2001/XMLSchema#double">7500</rdf:value>
   <gs1:unitCode>MLT</gs1:unitCode>
   <gs1:value>7500</gs1:value>
  </gs1:QuantitativeValue>
 </gs1:netContent>
 <sosa:isFeatureOfInterestOf>
  <rdf:Description rdf:about="#12xbottle625ml-ContentSosa">
   <rdf:type rdf:resource="http://www.w3.org/ns/sosa/Observation"/>
   <sosa:hasFeatureOfInterest rdf:resource="#12xbottle625ml"/>
   <sosa:observedProperty  rdf:resource="#netcontent"/>
   <sosa:hasResult rdf:resource="#12xbottle625ml-Content"/>
   <sosa:hasSimpleResult rdf:datatype="http://www.qudt.org/2.1/vocab/unit/MilliM">7500</sosa:hasSimpleResult>
  </rdf:Description>
 </sosa:isFeatureOfInterestOf>
 </rdf:Description>

 <rdf:Description rdf:about="#12xbottle355ml">
  <rdf:type rdf:resource="#LiquidContainer"/>
  <rdf:type rdf:resource="#BeverageBottle"/>
  <rdf:type rdf:resource="https://gs1.org/voc/PackagingDetails"/>
  <rdfs:label xml:lang="en">12XBottle355ml</rdfs:label>
  <rdfs:label xml:lang="fr">12XBottle355ml</rdfs:label>
  <skos:definition xml:lang="en">Generic Flat, Box or Crate of 12, 355ml Bottles</skos:definition>
  <skos:definition xml:lang="fr">Une boite, caisse ou caissette générique de 12 Bouteilles de 355ml</skos:definition>
  <rdfs:comment xml:lang="en">This term is meant to be used as a placeholder when no data about the aggregate packaging is known.</rdfs:comment>
  <rdfs:comment xml:lang="fr">Ce terme peut-être utilisé comme un terme générique lorsque les details de l’emballage ne sont pas certain.</rdfs:comment>
  <beer:count rdf:datatype="http://www.w3.org/2001/XMLSchema#Integer">12</beer:count>
  <beer:item rdf:resource="https://rdf.ag/o/beer#bottle355ml"/>
  <rdfs:isDefinedBy rdf:resource="https://rdf.ag/o/beer-ONTOLOGY_DATE"/>
  <void:inDataset rdf:resource="#datasetdefinition"/>
  <gs1:netContent>
   <gs1:QuantitativeValue rdf:about="#12xbottle355ml-Content">
   <rdf:type rdf:resource="http://qudt.org/1.1/schema/qudt#QuantityValue"/>
   <qudt:unit rdf:resource="http://www.qudt.org/2.1/vocab/unit/MilliL"/>
   <qudt:numericalValue rdf:datatype="http://www.w3.org/2001/XMLSchema#double">4260</qudt:numericalValue>
   <rdf:value rdf:datatype="http://www.w3.org/2001/XMLSchema#double">4260</rdf:value>
   <gs1:unitCode>MLT</gs1:unitCode>
   <gs1:value>4260</gs1:value>
  </gs1:QuantitativeValue>
 </gs1:netContent>
 <sosa:isFeatureOfInterestOf>
  <rdf:Description rdf:about="#12xbottle355ml-ContentSosa">
   <rdf:type rdf:resource="http://www.w3.org/ns/sosa/Observation"/>
   <sosa:hasFeatureOfInterest rdf:resource="#12xbottle355ml"/>
   <sosa:observedProperty  rdf:resource="#netcontent"/>
   <sosa:hasResult rdf:resource="#12xbottle355ml-Content"/>
   <sosa:hasSimpleResult rdf:datatype="http://www.qudt.org/2.1/vocab/unit/MilliM">4260</sosa:hasSimpleResult>
  </rdf:Description>
 </sosa:isFeatureOfInterestOf>
 </rdf:Description>

 <rdf:Description rdf:about="#24xbottle355ml">
  <rdf:type rdf:resource="#LiquidContainer"/>
  <rdf:type rdf:resource="#BeverageBottle"/>
  <rdf:type rdf:resource="https://gs1.org/voc/PackagingDetails"/>
  <rdfs:label xml:lang="en">24XBottle355ml</rdfs:label>
  <rdfs:label xml:lang="fr">24XBottle355ml</rdfs:label>
  <skos:definition xml:lang="en">Generic Flat, Box or Crate of 24, 355ml Bottles</skos:definition>
  <skos:definition xml:lang="fr">Une boite, caisse ou caissette générique de 24 Bouteilles de 355ml</skos:definition>
  <rdfs:comment xml:lang="en">This term is meant to be used as a placeholder when no data about the aggregate packaging is known.</rdfs:comment>
  <rdfs:comment xml:lang="fr">Ce terme peut-être utilisé comme un terme générique lorsque les details de l’emballage ne sont pas certain.</rdfs:comment>
  <beer:count rdf:datatype="http://www.w3.org/2001/XMLSchema#Integer">24</beer:count>
  <beer:item rdf:resource="https://rdf.ag/o/beer#bottle355ml"/>
  <rdfs:isDefinedBy rdf:resource="https://rdf.ag/o/beer-ONTOLOGY_DATE"/>
  <void:inDataset rdf:resource="#datasetdefinition"/>
  <gs1:netContent>
   <gs1:QuantitativeValue rdf:about="#24xbottle355ml-Content">
   <rdf:type rdf:resource="http://qudt.org/1.1/schema/qudt#QuantityValue"/>
   <qudt:unit rdf:resource="http://www.qudt.org/2.1/vocab/unit/MilliL"/>
   <qudt:numericalValue rdf:datatype="http://www.w3.org/2001/XMLSchema#double">8520</qudt:numericalValue>
   <rdf:value rdf:datatype="http://www.w3.org/2001/XMLSchema#double">8520</rdf:value>
   <gs1:unitCode>MLT</gs1:unitCode>
   <gs1:value>8520</gs1:value>
  </gs1:QuantitativeValue>
 </gs1:netContent>
 <sosa:isFeatureOfInterestOf>
  <rdf:Description rdf:about="#24xbottle355ml-ContentSosa">
   <rdf:type rdf:resource="http://www.w3.org/ns/sosa/Observation"/>
   <sosa:hasFeatureOfInterest rdf:resource="#24xbottle355ml"/>
   <sosa:observedProperty  rdf:resource="#netcontent"/>
   <sosa:hasResult rdf:resource="#24xbottle355ml-Content"/>
   <sosa:hasSimpleResult rdf:datatype="http://www.qudt.org/2.1/vocab/unit/MilliM">8520</sosa:hasSimpleResult>
  </rdf:Description>
 </sosa:isFeatureOfInterestOf>
 </rdf:Description>

 <rdf:Description rdf:about="#6xbottle355ml">
  <rdf:type rdf:resource="#LiquidContainer"/>
  <rdf:type rdf:resource="#BeverageBottle"/>
  <rdf:type rdf:resource="https://gs1.org/voc/PackagingDetails"/>
  <rdfs:label xml:lang="en">6XBottle355ml</rdfs:label>
  <rdfs:label xml:lang="fr">6XBottle355ml</rdfs:label>
  <skos:definition xml:lang="en">Generic Flat, Box or Crate of 6, 355ml Bottles</skos:definition>
  <skos:definition xml:lang="fr">Une boite, caisse ou caissette générique de 6 Bouteilles de 355ml</skos:definition>
  <rdfs:comment xml:lang="en">This term is meant to be used as a placeholder when no data about the aggregate packaging is known.</rdfs:comment>
  <rdfs:comment xml:lang="fr">Ce terme peut-être utilisé comme un terme générique lorsque les details de l’emballage ne sont pas certain.</rdfs:comment>
  <beer:count rdf:datatype="http://www.w3.org/2001/XMLSchema#Integer">6</beer:count>
  <beer:item rdf:resource="https://rdf.ag/o/beer#bottle355ml"/>
  <rdfs:isDefinedBy rdf:resource="https://rdf.ag/o/beer-ONTOLOGY_DATE"/>
  <void:inDataset rdf:resource="#datasetdefinition"/>
  <gs1:netContent>
   <gs1:QuantitativeValue rdf:about="#6xbottle355ml-Content">
   <rdf:type rdf:resource="http://qudt.org/1.1/schema/qudt#QuantityValue"/>
   <qudt:unit rdf:resource="http://www.qudt.org/2.1/vocab/unit/MilliL"/>
   <qudt:numericalValue rdf:datatype="http://www.w3.org/2001/XMLSchema#double">2130</qudt:numericalValue>
   <rdf:value rdf:datatype="http://www.w3.org/2001/XMLSchema#double">2130</rdf:value>
   <gs1:unitCode>MLT</gs1:unitCode>
   <gs1:value>2130</gs1:value>
  </gs1:QuantitativeValue>
 </gs1:netContent>
 <sosa:isFeatureOfInterestOf>
  <rdf:Description rdf:about="#6xbottle355ml-ContentSosa">
   <rdf:type rdf:resource="http://www.w3.org/ns/sosa/Observation"/>
   <sosa:hasFeatureOfInterest rdf:resource="#6xbottle355ml"/>
   <sosa:observedProperty  rdf:resource="#netcontent"/>
   <sosa:hasResult rdf:resource="#6xbottle355ml-Content"/>
   <sosa:hasSimpleResult rdf:datatype="http://www.qudt.org/2.1/vocab/unit/MilliM">2130</sosa:hasSimpleResult>
  </rdf:Description>
 </sosa:isFeatureOfInterestOf>
 </rdf:Description>

 <rdf:Description rdf:about="#28xbottle355ml">
  <rdf:type rdf:resource="#LiquidContainer"/>
  <rdf:type rdf:resource="#BeverageBottle"/>
  <rdf:type rdf:resource="https://gs1.org/voc/PackagingDetails"/>
  <rdfs:label xml:lang="en">28XBottle355ml</rdfs:label>
  <rdfs:label xml:lang="fr">28XBottle355ml</rdfs:label>
  <skos:definition xml:lang="en">Generic Flat, Box or Crate of 28, 355ml Bottles</skos:definition>
  <skos:definition xml:lang="fr">Une boite, caisse ou caissette générique de 28 Bouteilles de 355ml</skos:definition>
  <rdfs:comment xml:lang="en">This term is meant to be used as a placeholder when no data about the aggregate packaging is known.</rdfs:comment>
  <rdfs:comment xml:lang="fr">Ce terme peut-être utilisé comme un terme générique lorsque les details de l’emballage ne sont pas certain.</rdfs:comment>
  <beer:count rdf:datatype="http://www.w3.org/2001/XMLSchema#Integer">28</beer:count>
  <beer:item rdf:resource="https://rdf.ag/o/beer#bottle355ml"/>
  <rdfs:isDefinedBy rdf:resource="https://rdf.ag/o/beer-ONTOLOGY_DATE"/>
  <void:inDataset rdf:resource="#datasetdefinition"/>
  <gs1:netContent>
   <gs1:QuantitativeValue rdf:about="#28xbottle355ml-Content">
   <rdf:type rdf:resource="http://qudt.org/1.1/schema/qudt#QuantityValue"/>
   <qudt:unit rdf:resource="http://www.qudt.org/2.1/vocab/unit/MilliL"/>
   <qudt:numericalValue rdf:datatype="http://www.w3.org/2001/XMLSchema#double">9940</qudt:numericalValue>
   <rdf:value rdf:datatype="http://www.w3.org/2001/XMLSchema#double">9940</rdf:value>
   <gs1:unitCode>MLT</gs1:unitCode>
   <gs1:value>9940</gs1:value>
  </gs1:QuantitativeValue>
 </gs1:netContent>
 <sosa:isFeatureOfInterestOf>
  <rdf:Description rdf:about="#28xbottle355ml-ContentSosa">
   <rdf:type rdf:resource="http://www.w3.org/ns/sosa/Observation"/>
   <sosa:hasFeatureOfInterest rdf:resource="#28xbottle355ml"/>
   <sosa:observedProperty  rdf:resource="#netcontent"/>
   <sosa:hasResult rdf:resource="#28xbottle355ml-Content"/>
   <sosa:hasSimpleResult rdf:datatype="http://www.qudt.org/2.1/vocab/unit/MilliM">9940</sosa:hasSimpleResult>
  </rdf:Description>
 </sosa:isFeatureOfInterestOf>
 </rdf:Description>

 <rdf:Description rdf:about="#20xcan355ml">
  <rdf:type rdf:resource="#LiquidContainer"/>
  <rdf:type rdf:resource="#BeverageCan"/>
  <rdf:type rdf:resource="https://gs1.org/voc/PackagingDetails"/>
  <rdfs:label xml:lang="en">20XCan355ml</rdfs:label>
  <rdfs:label xml:lang="fr">20XCan355ml</rdfs:label>
  <skos:definition xml:lang="en">Generic Flat, Box or Crate of 20, 355ml Cans</skos:definition>
  <skos:definition xml:lang="fr">Une boite, caisse ou caissette générique de 20 Canettes de 355ml</skos:definition>
  <rdfs:comment xml:lang="en">This term is meant to be used as a placeholder when no data about the aggregate packaging is known.</rdfs:comment>
  <rdfs:comment xml:lang="fr">Ce terme peut-être utilisé comme un terme générique lorsque les details de l’emballage ne sont pas certain.</rdfs:comment>
  <beer:count rdf:datatype="http://www.w3.org/2001/XMLSchema#Integer">20</beer:count>
  <beer:item rdf:resource="https://rdf.ag/o/beer#can355ml"/>
  <rdfs:isDefinedBy rdf:resource="https://rdf.ag/o/beer-ONTOLOGY_DATE"/>
  <void:inDataset rdf:resource="#datasetdefinition"/>
  <gs1:netContent>
   <gs1:QuantitativeValue rdf:about="#20xcan355ml-Content">
   <rdf:type rdf:resource="http://qudt.org/1.1/schema/qudt#QuantityValue"/>
   <qudt:unit rdf:resource="http://www.qudt.org/2.1/vocab/unit/MilliL"/>
   <qudt:numericalValue rdf:datatype="http://www.w3.org/2001/XMLSchema#double">7100</qudt:numericalValue>
   <rdf:value rdf:datatype="http://www.w3.org/2001/XMLSchema#double">7100</rdf:value>
   <gs1:unitCode>MLT</gs1:unitCode>
   <gs1:value>7100</gs1:value>
  </gs1:QuantitativeValue>
 </gs1:netContent>
 <sosa:isFeatureOfInterestOf>
  <rdf:Description rdf:about="#20xcan355ml-ContentSosa">
   <rdf:type rdf:resource="http://www.w3.org/ns/sosa/Observation"/>
   <sosa:hasFeatureOfInterest rdf:resource="#20xcan355ml"/>
   <sosa:observedProperty  rdf:resource="#netcontent"/>
   <sosa:hasResult rdf:resource="#20xcan355ml-Content"/>
   <sosa:hasSimpleResult rdf:datatype="http://www.qudt.org/2.1/vocab/unit/MilliM">7100</sosa:hasSimpleResult>
  </rdf:Description>
 </sosa:isFeatureOfInterestOf>
 </rdf:Description>

 <rdf:Description rdf:about="#30xcan355ml">
  <rdf:type rdf:resource="#LiquidContainer"/>
  <rdf:type rdf:resource="#BeverageCan"/>
  <rdf:type rdf:resource="https://gs1.org/voc/PackagingDetails"/>
  <rdfs:label xml:lang="en">30XCan355ml</rdfs:label>
  <rdfs:label xml:lang="fr">30XCan355ml</rdfs:label>
  <skos:definition xml:lang="en">Generic Flat, Box or Crate of 30, 355ml Cans</skos:definition>
  <skos:definition xml:lang="fr">Une boite, caisse ou caissette générique de 30 Canettes de 355ml</skos:definition>
  <rdfs:comment xml:lang="en">This term is meant to be used as a placeholder when no data about the aggregate packaging is known.</rdfs:comment>
  <rdfs:comment xml:lang="fr">Ce terme peut-être utilisé comme un terme générique lorsque les details de l’emballage ne sont pas certain.</rdfs:comment>
  <beer:count rdf:datatype="http://www.w3.org/2001/XMLSchema#Integer">30</beer:count>
  <beer:item rdf:resource="https://rdf.ag/o/beer#can355ml"/>
  <rdfs:isDefinedBy rdf:resource="https://rdf.ag/o/beer-ONTOLOGY_DATE"/>
  <void:inDataset rdf:resource="#datasetdefinition"/>
  <gs1:netContent>
   <gs1:QuantitativeValue rdf:about="#30xcan355ml-Content">
   <rdf:type rdf:resource="http://qudt.org/1.1/schema/qudt#QuantityValue"/>
   <qudt:unit rdf:resource="http://www.qudt.org/2.1/vocab/unit/MilliL"/>
   <qudt:numericalValue rdf:datatype="http://www.w3.org/2001/XMLSchema#double">10650</qudt:numericalValue>
   <rdf:value rdf:datatype="http://www.w3.org/2001/XMLSchema#double">10650</rdf:value>
   <gs1:unitCode>MLT</gs1:unitCode>
   <gs1:value>10650</gs1:value>
  </gs1:QuantitativeValue>
 </gs1:netContent>
 <sosa:isFeatureOfInterestOf>
  <rdf:Description rdf:about="#30xcan355ml-ContentSosa">
   <rdf:type rdf:resource="http://www.w3.org/ns/sosa/Observation"/>
   <sosa:hasFeatureOfInterest rdf:resource="#30xcan355ml"/>
   <sosa:observedProperty  rdf:resource="#netcontent"/>
   <sosa:hasResult rdf:resource="#30xcan355ml-Content"/>
   <sosa:hasSimpleResult rdf:datatype="http://www.qudt.org/2.1/vocab/unit/MilliM">10650</sosa:hasSimpleResult>
  </rdf:Description>
 </sosa:isFeatureOfInterestOf>
 </rdf:Description>

 <rdf:Description rdf:about="#40xcan355ml">
  <rdf:type rdf:resource="#LiquidContainer"/>
  <rdf:type rdf:resource="#BeverageCan"/>
  <rdf:type rdf:resource="https://gs1.org/voc/PackagingDetails"/>
  <rdfs:label xml:lang="en">40XCan355ml</rdfs:label>
  <rdfs:label xml:lang="fr">40XCan355ml</rdfs:label>
  <skos:definition xml:lang="en">Generic Flat, Box or Crate of 40, 355ml Cans</skos:definition>
  <skos:definition xml:lang="fr">Une boite, caisse ou caissette générique de 40 Canettes de 355ml</skos:definition>
  <rdfs:comment xml:lang="en">This term is meant to be used as a placeholder when no data about the aggregate packaging is known.</rdfs:comment>
  <rdfs:comment xml:lang="fr">Ce terme peut-être utilisé comme un terme générique lorsque les details de l’emballage ne sont pas certain.</rdfs:comment>
  <beer:count rdf:datatype="http://www.w3.org/2001/XMLSchema#Integer">40</beer:count>
  <beer:item rdf:resource="https://rdf.ag/o/beer#can355ml"/>
  <rdfs:isDefinedBy rdf:resource="https://rdf.ag/o/beer-ONTOLOGY_DATE"/>
  <void:inDataset rdf:resource="#datasetdefinition"/>
  <gs1:netContent>
   <gs1:QuantitativeValue rdf:about="#40xcan355ml-Content">
   <rdf:type rdf:resource="http://qudt.org/1.1/schema/qudt#QuantityValue"/>
   <qudt:unit rdf:resource="http://www.qudt.org/2.1/vocab/unit/MilliL"/>
   <qudt:numericalValue rdf:datatype="http://www.w3.org/2001/XMLSchema#double">14200</qudt:numericalValue>
   <rdf:value rdf:datatype="http://www.w3.org/2001/XMLSchema#double">14200</rdf:value>
   <gs1:unitCode>MLT</gs1:unitCode>
   <gs1:value>14200</gs1:value>
  </gs1:QuantitativeValue>
 </gs1:netContent>
 <sosa:isFeatureOfInterestOf>
  <rdf:Description rdf:about="#40xcan355ml-ContentSosa">
   <rdf:type rdf:resource="http://www.w3.org/ns/sosa/Observation"/>
   <sosa:hasFeatureOfInterest rdf:resource="#40xcan355ml"/>
   <sosa:observedProperty  rdf:resource="#netcontent"/>
   <sosa:hasResult rdf:resource="#40xcan355ml-Content"/>
   <sosa:hasSimpleResult rdf:datatype="http://www.qudt.org/2.1/vocab/unit/MilliM">14200</sosa:hasSimpleResult>
  </rdf:Description>
 </sosa:isFeatureOfInterestOf>
 </rdf:Description>

 <rdf:Description rdf:about="#60xcan355ml">
  <rdf:type rdf:resource="#LiquidContainer"/>
  <rdf:type rdf:resource="#BeverageCan"/>
  <rdf:type rdf:resource="https://gs1.org/voc/PackagingDetails"/>
  <rdfs:label xml:lang="en">60XCan355ml</rdfs:label>
  <rdfs:label xml:lang="fr">60XCan355ml</rdfs:label>
  <skos:definition xml:lang="en">Generic Flat, Box or Crate of 60, 355ml Cans</skos:definition>
  <skos:definition xml:lang="fr">Une boite, caisse ou caissette générique de 60 Canettes de 355ml</skos:definition>
  <rdfs:comment xml:lang="en">This term is meant to be used as a placeholder when no data about the aggregate packaging is known.</rdfs:comment>
  <rdfs:comment xml:lang="fr">Ce terme peut-être utilisé comme un terme générique lorsque les details de l’emballage ne sont pas certain.</rdfs:comment>
  <beer:count rdf:datatype="http://www.w3.org/2001/XMLSchema#Integer">60</beer:count>
  <beer:item rdf:resource="https://rdf.ag/o/beer#can355ml"/>
  <rdfs:isDefinedBy rdf:resource="https://rdf.ag/o/beer-ONTOLOGY_DATE"/>
  <void:inDataset rdf:resource="#datasetdefinition"/>
  <gs1:netContent>
   <gs1:QuantitativeValue rdf:about="#60xcan355ml-Content">
   <rdf:type rdf:resource="http://qudt.org/1.1/schema/qudt#QuantityValue"/>
   <qudt:unit rdf:resource="http://www.qudt.org/2.1/vocab/unit/MilliL"/>
   <qudt:numericalValue rdf:datatype="http://www.w3.org/2001/XMLSchema#double">21300</qudt:numericalValue>
   <rdf:value rdf:datatype="http://www.w3.org/2001/XMLSchema#double">21300</rdf:value>
   <gs1:unitCode>MLT</gs1:unitCode>
   <gs1:value>21300</gs1:value>
  </gs1:QuantitativeValue>
 </gs1:netContent>
 <sosa:isFeatureOfInterestOf>
  <rdf:Description rdf:about="#60xcan355ml-ContentSosa">
   <rdf:type rdf:resource="http://www.w3.org/ns/sosa/Observation"/>
   <sosa:hasFeatureOfInterest rdf:resource="#60xcan355ml"/>
   <sosa:observedProperty  rdf:resource="#netcontent"/>
   <sosa:hasResult rdf:resource="#60xcan355ml-Content"/>
   <sosa:hasSimpleResult rdf:datatype="http://www.qudt.org/2.1/vocab/unit/MilliM">21300</sosa:hasSimpleResult>
  </rdf:Description>
 </sosa:isFeatureOfInterestOf>
 </rdf:Description>

 <rdf:Description rdf:about="#12xcan355ml">
  <rdf:type rdf:resource="#LiquidContainer"/>
  <rdf:type rdf:resource="#BeverageCan"/>
  <rdf:type rdf:resource="https://gs1.org/voc/PackagingDetails"/>
  <rdfs:label xml:lang="en">12XCan355ml</rdfs:label>
  <rdfs:label xml:lang="fr">12XCan355ml</rdfs:label>
  <skos:definition xml:lang="en">Generic Flat, Box or Crate of 12, 355ml Cans</skos:definition>
  <skos:definition xml:lang="fr">Une boite, caisse ou caissette générique de 12 Canettes de 355ml</skos:definition>
  <rdfs:comment xml:lang="en">This term is meant to be used as a placeholder when no data about the aggregate packaging is known.</rdfs:comment>
  <rdfs:comment xml:lang="fr">Ce terme peut-être utilisé comme un terme générique lorsque les details de l’emballage ne sont pas certain.</rdfs:comment>
  <beer:count rdf:datatype="http://www.w3.org/2001/XMLSchema#Integer">12</beer:count>
  <beer:item rdf:resource="https://rdf.ag/o/beer#can355ml"/>
  <rdfs:isDefinedBy rdf:resource="https://rdf.ag/o/beer-ONTOLOGY_DATE"/>
  <void:inDataset rdf:resource="#datasetdefinition"/>
  <gs1:netContent>
   <gs1:QuantitativeValue rdf:about="#12xcan355ml-Content">
   <rdf:type rdf:resource="http://qudt.org/1.1/schema/qudt#QuantityValue"/>
   <qudt:unit rdf:resource="http://www.qudt.org/2.1/vocab/unit/MilliL"/>
   <qudt:numericalValue rdf:datatype="http://www.w3.org/2001/XMLSchema#double">4260</qudt:numericalValue>
   <rdf:value rdf:datatype="http://www.w3.org/2001/XMLSchema#double">4260</rdf:value>
   <gs1:unitCode>MLT</gs1:unitCode>
   <gs1:value>4260</gs1:value>
  </gs1:QuantitativeValue>
 </gs1:netContent>
 <sosa:isFeatureOfInterestOf>
  <rdf:Description rdf:about="#12xcan355ml-ContentSosa">
   <rdf:type rdf:resource="http://www.w3.org/ns/sosa/Observation"/>
   <sosa:hasFeatureOfInterest rdf:resource="#12xcan355ml"/>
   <sosa:observedProperty  rdf:resource="#netcontent"/>
   <sosa:hasResult rdf:resource="#12xcan355ml-Content"/>
   <sosa:hasSimpleResult rdf:datatype="http://www.qudt.org/2.1/vocab/unit/MilliM">4260</sosa:hasSimpleResult>
  </rdf:Description>
 </sosa:isFeatureOfInterestOf>
 </rdf:Description>

 <rdf:Description rdf:about="#4xcan355ml">
  <rdf:type rdf:resource="#LiquidContainer"/>
  <rdf:type rdf:resource="#BeverageCan"/>
  <rdf:type rdf:resource="https://gs1.org/voc/PackagingDetails"/>
  <rdfs:label xml:lang="en">4XCan355ml</rdfs:label>
  <rdfs:label xml:lang="fr">4XCan355ml</rdfs:label>
  <skos:definition xml:lang="en">Generic Flat, Box or Crate of 4, 355ml Cans</skos:definition>
  <skos:definition xml:lang="fr">Une boite, caisse ou caissette générique de 4 Canettes de 355ml</skos:definition>
  <rdfs:comment xml:lang="en">This term is meant to be used as a placeholder when no data about the aggregate packaging is known.</rdfs:comment>
  <rdfs:comment xml:lang="fr">Ce terme peut-être utilisé comme un terme générique lorsque les details de l’emballage ne sont pas certain.</rdfs:comment>
  <beer:count rdf:datatype="http://www.w3.org/2001/XMLSchema#Integer">4</beer:count>
  <beer:item rdf:resource="https://rdf.ag/o/beer#can355ml"/>
  <rdfs:isDefinedBy rdf:resource="https://rdf.ag/o/beer-ONTOLOGY_DATE"/>
  <void:inDataset rdf:resource="#datasetdefinition"/>
  <gs1:netContent>
   <gs1:QuantitativeValue rdf:about="#4xcan355ml-Content">
   <rdf:type rdf:resource="http://qudt.org/1.1/schema/qudt#QuantityValue"/>
   <qudt:unit rdf:resource="http://www.qudt.org/2.1/vocab/unit/MilliL"/>
   <qudt:numericalValue rdf:datatype="http://www.w3.org/2001/XMLSchema#double">1420</qudt:numericalValue>
   <rdf:value rdf:datatype="http://www.w3.org/2001/XMLSchema#double">1420</rdf:value>
   <gs1:unitCode>MLT</gs1:unitCode>
   <gs1:value>1420</gs1:value>
  </gs1:QuantitativeValue>
 </gs1:netContent>
 <sosa:isFeatureOfInterestOf>
  <rdf:Description rdf:about="#4xcan355ml-ContentSosa">
   <rdf:type rdf:resource="http://www.w3.org/ns/sosa/Observation"/>
   <sosa:hasFeatureOfInterest rdf:resource="#4xcan355ml"/>
   <sosa:observedProperty  rdf:resource="#netcontent"/>
   <sosa:hasResult rdf:resource="#4xcan355ml-Content"/>
   <sosa:hasSimpleResult rdf:datatype="http://www.qudt.org/2.1/vocab/unit/MilliM">1420</sosa:hasSimpleResult>
  </rdf:Description>
 </sosa:isFeatureOfInterestOf>
 </rdf:Description>

 <rdf:Description rdf:about="#24xcan355ml">
  <rdf:type rdf:resource="#LiquidContainer"/>
  <rdf:type rdf:resource="#BeverageCan"/>
  <rdf:type rdf:resource="https://gs1.org/voc/PackagingDetails"/>
  <rdfs:label xml:lang="en">24XCan355ml</rdfs:label>
  <rdfs:label xml:lang="fr">24XCan355ml</rdfs:label>
  <skos:definition xml:lang="en">Generic Flat, Box or Crate of 24, 355ml Cans</skos:definition>
  <skos:definition xml:lang="fr">Une boite, caisse ou caissette générique de 24 Canettes de 355ml</skos:definition>
  <rdfs:comment xml:lang="en">This term is meant to be used as a placeholder when no data about the aggregate packaging is known.</rdfs:comment>
  <rdfs:comment xml:lang="fr">Ce terme peut-être utilisé comme un terme générique lorsque les details de l’emballage ne sont pas certain.</rdfs:comment>
  <beer:count rdf:datatype="http://www.w3.org/2001/XMLSchema#Integer">24</beer:count>
  <beer:item rdf:resource="https://rdf.ag/o/beer#can355ml"/>
  <rdfs:isDefinedBy rdf:resource="https://rdf.ag/o/beer-ONTOLOGY_DATE"/>
  <void:inDataset rdf:resource="#datasetdefinition"/>
  <gs1:netContent>
   <gs1:QuantitativeValue rdf:about="#24xcan355ml-Content">
   <rdf:type rdf:resource="http://qudt.org/1.1/schema/qudt#QuantityValue"/>
   <qudt:unit rdf:resource="http://www.qudt.org/2.1/vocab/unit/MilliL"/>
   <qudt:numericalValue rdf:datatype="http://www.w3.org/2001/XMLSchema#double">8520</qudt:numericalValue>
   <rdf:value rdf:datatype="http://www.w3.org/2001/XMLSchema#double">8520</rdf:value>
   <gs1:unitCode>MLT</gs1:unitCode>
   <gs1:value>8520</gs1:value>
  </gs1:QuantitativeValue>
 </gs1:netContent>
 <sosa:isFeatureOfInterestOf>
  <rdf:Description rdf:about="#24xcan355ml-ContentSosa">
   <rdf:type rdf:resource="http://www.w3.org/ns/sosa/Observation"/>
   <sosa:hasFeatureOfInterest rdf:resource="#24xcan355ml"/>
   <sosa:observedProperty  rdf:resource="#netcontent"/>
   <sosa:hasResult rdf:resource="#24xcan355ml-Content"/>
   <sosa:hasSimpleResult rdf:datatype="http://www.qudt.org/2.1/vocab/unit/MilliM">8520</sosa:hasSimpleResult>
  </rdf:Description>
 </sosa:isFeatureOfInterestOf>
 </rdf:Description>

 <rdf:Description rdf:about="#15xcan355ml">
  <rdf:type rdf:resource="#LiquidContainer"/>
  <rdf:type rdf:resource="#BeverageCan"/>
  <rdf:type rdf:resource="https://gs1.org/voc/PackagingDetails"/>
  <rdfs:label xml:lang="en">15XCan355ml</rdfs:label>
  <rdfs:label xml:lang="fr">15XCan355ml</rdfs:label>
  <skos:definition xml:lang="en">Generic Flat, Box or Crate of 15, 355ml Cans</skos:definition>
  <skos:definition xml:lang="fr">Une boite, caisse ou caissette générique de 15 Canettes de 355ml</skos:definition>
  <rdfs:comment xml:lang="en">This term is meant to be used as a placeholder when no data about the aggregate packaging is known.</rdfs:comment>
  <rdfs:comment xml:lang="fr">Ce terme peut-être utilisé comme un terme générique lorsque les details de l’emballage ne sont pas certain.</rdfs:comment>
  <beer:count rdf:datatype="http://www.w3.org/2001/XMLSchema#Integer">15</beer:count>
  <beer:item rdf:resource="https://rdf.ag/o/beer#can355ml"/>
  <rdfs:isDefinedBy rdf:resource="https://rdf.ag/o/beer-ONTOLOGY_DATE"/>
  <void:inDataset rdf:resource="#datasetdefinition"/>
  <gs1:netContent>
   <gs1:QuantitativeValue rdf:about="#15xcan355ml-Content">
   <rdf:type rdf:resource="http://qudt.org/1.1/schema/qudt#QuantityValue"/>
   <qudt:unit rdf:resource="http://www.qudt.org/2.1/vocab/unit/MilliL"/>
   <qudt:numericalValue rdf:datatype="http://www.w3.org/2001/XMLSchema#double">5325</qudt:numericalValue>
   <rdf:value rdf:datatype="http://www.w3.org/2001/XMLSchema#double">5325</rdf:value>
   <gs1:unitCode>MLT</gs1:unitCode>
   <gs1:value>5325</gs1:value>
  </gs1:QuantitativeValue>
 </gs1:netContent>
 <sosa:isFeatureOfInterestOf>
  <rdf:Description rdf:about="#15xcan355ml-ContentSosa">
   <rdf:type rdf:resource="http://www.w3.org/ns/sosa/Observation"/>
   <sosa:hasFeatureOfInterest rdf:resource="#15xcan355ml"/>
   <sosa:observedProperty  rdf:resource="#netcontent"/>
   <sosa:hasResult rdf:resource="#15xcan355ml-Content"/>
   <sosa:hasSimpleResult rdf:datatype="http://www.qudt.org/2.1/vocab/unit/MilliM">5325</sosa:hasSimpleResult>
  </rdf:Description>
 </sosa:isFeatureOfInterestOf>
 </rdf:Description>

 <rdf:Description rdf:about="#45xcan355ml">
  <rdf:type rdf:resource="#LiquidContainer"/>
  <rdf:type rdf:resource="#BeverageCan"/>
  <rdf:type rdf:resource="https://gs1.org/voc/PackagingDetails"/>
  <rdfs:label xml:lang="en">45XCan355ml</rdfs:label>
  <rdfs:label xml:lang="fr">45XCan355ml</rdfs:label>
  <skos:definition xml:lang="en">Generic Flat, Box or Crate of 45, 355ml Cans</skos:definition>
  <skos:definition xml:lang="fr">Une boite, caisse ou caissette générique de 45 Canettes de 355ml</skos:definition>
  <rdfs:comment xml:lang="en">This term is meant to be used as a placeholder when no data about the aggregate packaging is known.</rdfs:comment>
  <rdfs:comment xml:lang="fr">Ce terme peut-être utilisé comme un terme générique lorsque les details de l’emballage ne sont pas certain.</rdfs:comment>
  <beer:count rdf:datatype="http://www.w3.org/2001/XMLSchema#Integer">45</beer:count>
  <beer:item rdf:resource="https://rdf.ag/o/beer#can355ml"/>
  <rdfs:isDefinedBy rdf:resource="https://rdf.ag/o/beer-ONTOLOGY_DATE"/>
  <void:inDataset rdf:resource="#datasetdefinition"/>
  <gs1:netContent>
   <gs1:QuantitativeValue rdf:about="#45xcan355ml-Content">
   <rdf:type rdf:resource="http://qudt.org/1.1/schema/qudt#QuantityValue"/>
   <qudt:unit rdf:resource="http://www.qudt.org/2.1/vocab/unit/MilliL"/>
   <qudt:numericalValue rdf:datatype="http://www.w3.org/2001/XMLSchema#double">15975</qudt:numericalValue>
   <rdf:value rdf:datatype="http://www.w3.org/2001/XMLSchema#double">15975</rdf:value>
   <gs1:unitCode>MLT</gs1:unitCode>
   <gs1:value>15975</gs1:value>
  </gs1:QuantitativeValue>
 </gs1:netContent>
 <sosa:isFeatureOfInterestOf>
  <rdf:Description rdf:about="#45xcan355ml-ContentSosa">
   <rdf:type rdf:resource="http://www.w3.org/ns/sosa/Observation"/>
   <sosa:hasFeatureOfInterest rdf:resource="#45xcan355ml"/>
   <sosa:observedProperty  rdf:resource="#netcontent"/>
   <sosa:hasResult rdf:resource="#45xcan355ml-Content"/>
   <sosa:hasSimpleResult rdf:datatype="http://www.qudt.org/2.1/vocab/unit/MilliM">15975</sosa:hasSimpleResult>
  </rdf:Description>
 </sosa:isFeatureOfInterestOf>
 </rdf:Description>

 <rdf:Description rdf:about="#6xcan355ml">
  <rdf:type rdf:resource="#LiquidContainer"/>
  <rdf:type rdf:resource="#BeverageCan"/>
  <rdf:type rdf:resource="https://gs1.org/voc/PackagingDetails"/>
  <rdfs:label xml:lang="en">6XCan355ml</rdfs:label>
  <rdfs:label xml:lang="fr">6XCan355ml</rdfs:label>
  <skos:definition xml:lang="en">Generic Flat, Box or Crate of 6, 355ml Cans</skos:definition>
  <skos:definition xml:lang="fr">Une boite, caisse ou caissette générique de 6 Canettes de 355ml</skos:definition>
  <rdfs:comment xml:lang="en">This term is meant to be used as a placeholder when no data about the aggregate packaging is known.</rdfs:comment>
  <rdfs:comment xml:lang="fr">Ce terme peut-être utilisé comme un terme générique lorsque les details de l’emballage ne sont pas certain.</rdfs:comment>
  <beer:count rdf:datatype="http://www.w3.org/2001/XMLSchema#Integer">6</beer:count>
  <beer:item rdf:resource="https://rdf.ag/o/beer#can355ml"/>
  <rdfs:isDefinedBy rdf:resource="https://rdf.ag/o/beer-ONTOLOGY_DATE"/>
  <void:inDataset rdf:resource="#datasetdefinition"/>
  <gs1:netContent>
   <gs1:QuantitativeValue rdf:about="#6xcan355ml-Content">
   <rdf:type rdf:resource="http://qudt.org/1.1/schema/qudt#QuantityValue"/>
   <qudt:unit rdf:resource="http://www.qudt.org/2.1/vocab/unit/MilliL"/>
   <qudt:numericalValue rdf:datatype="http://www.w3.org/2001/XMLSchema#double">2130</qudt:numericalValue>
   <rdf:value rdf:datatype="http://www.w3.org/2001/XMLSchema#double">2130</rdf:value>
   <gs1:unitCode>MLT</gs1:unitCode>
   <gs1:value>2130</gs1:value>
  </gs1:QuantitativeValue>
 </gs1:netContent>
 <sosa:isFeatureOfInterestOf>
  <rdf:Description rdf:about="#6xcan355ml-ContentSosa">
   <rdf:type rdf:resource="http://www.w3.org/ns/sosa/Observation"/>
   <sosa:hasFeatureOfInterest rdf:resource="#6xcan355ml"/>
   <sosa:observedProperty  rdf:resource="#netcontent"/>
   <sosa:hasResult rdf:resource="#6xcan355ml-Content"/>
   <sosa:hasSimpleResult rdf:datatype="http://www.qudt.org/2.1/vocab/unit/MilliM">2130</sosa:hasSimpleResult>
  </rdf:Description>
 </sosa:isFeatureOfInterestOf>
 </rdf:Description>

 <rdf:Description rdf:about="#16xcan355ml">
  <rdf:type rdf:resource="#LiquidContainer"/>
  <rdf:type rdf:resource="#BeverageCan"/>
  <rdf:type rdf:resource="https://gs1.org/voc/PackagingDetails"/>
  <rdfs:label xml:lang="en">16XCan355ml</rdfs:label>
  <rdfs:label xml:lang="fr">16XCan355ml</rdfs:label>
  <skos:definition xml:lang="en">Generic Flat, Box or Crate of 16, 355ml Cans</skos:definition>
  <skos:definition xml:lang="fr">Une boite, caisse ou caissette générique de 16 Canettes de 355ml</skos:definition>
  <rdfs:comment xml:lang="en">This term is meant to be used as a placeholder when no data about the aggregate packaging is known.</rdfs:comment>
  <rdfs:comment xml:lang="fr">Ce terme peut-être utilisé comme un terme générique lorsque les details de l’emballage ne sont pas certain.</rdfs:comment>
  <beer:count rdf:datatype="http://www.w3.org/2001/XMLSchema#Integer">16</beer:count>
  <beer:item rdf:resource="https://rdf.ag/o/beer#can355ml"/>
  <rdfs:isDefinedBy rdf:resource="https://rdf.ag/o/beer-ONTOLOGY_DATE"/>
  <void:inDataset rdf:resource="#datasetdefinition"/>
  <gs1:netContent>
   <gs1:QuantitativeValue rdf:about="#16xcan355ml-Content">
   <rdf:type rdf:resource="http://qudt.org/1.1/schema/qudt#QuantityValue"/>
   <qudt:unit rdf:resource="http://www.qudt.org/2.1/vocab/unit/MilliL"/>
   <qudt:numericalValue rdf:datatype="http://www.w3.org/2001/XMLSchema#double">5680</qudt:numericalValue>
   <rdf:value rdf:datatype="http://www.w3.org/2001/XMLSchema#double">5680</rdf:value>
   <gs1:unitCode>MLT</gs1:unitCode>
   <gs1:value>5680</gs1:value>
  </gs1:QuantitativeValue>
 </gs1:netContent>
 <sosa:isFeatureOfInterestOf>
  <rdf:Description rdf:about="#16xcan355ml-ContentSosa">
   <rdf:type rdf:resource="http://www.w3.org/ns/sosa/Observation"/>
   <sosa:hasFeatureOfInterest rdf:resource="#16xcan355ml"/>
   <sosa:observedProperty  rdf:resource="#netcontent"/>
   <sosa:hasResult rdf:resource="#16xcan355ml-Content"/>
   <sosa:hasSimpleResult rdf:datatype="http://www.qudt.org/2.1/vocab/unit/MilliM">5680</sosa:hasSimpleResult>
  </rdf:Description>
 </sosa:isFeatureOfInterestOf>
 </rdf:Description>

 <rdf:Description rdf:about="#36xcan355ml">
  <rdf:type rdf:resource="#LiquidContainer"/>
  <rdf:type rdf:resource="#BeverageCan"/>
  <rdf:type rdf:resource="https://gs1.org/voc/PackagingDetails"/>
  <rdfs:label xml:lang="en">36XCan355ml</rdfs:label>
  <rdfs:label xml:lang="fr">36XCan355ml</rdfs:label>
  <skos:definition xml:lang="en">Generic Flat, Box or Crate of 36, 355ml Cans</skos:definition>
  <skos:definition xml:lang="fr">Une boite, caisse ou caissette générique de 36 Canettes de 355ml</skos:definition>
  <rdfs:comment xml:lang="en">This term is meant to be used as a placeholder when no data about the aggregate packaging is known.</rdfs:comment>
  <rdfs:comment xml:lang="fr">Ce terme peut-être utilisé comme un terme générique lorsque les details de l’emballage ne sont pas certain.</rdfs:comment>
  <beer:count rdf:datatype="http://www.w3.org/2001/XMLSchema#Integer">36</beer:count>
  <beer:item rdf:resource="https://rdf.ag/o/beer#can355ml"/>
  <rdfs:isDefinedBy rdf:resource="https://rdf.ag/o/beer-ONTOLOGY_DATE"/>
  <void:inDataset rdf:resource="#datasetdefinition"/>
  <gs1:netContent>
   <gs1:QuantitativeValue rdf:about="#36xcan355ml-Content">
   <rdf:type rdf:resource="http://qudt.org/1.1/schema/qudt#QuantityValue"/>
   <qudt:unit rdf:resource="http://www.qudt.org/2.1/vocab/unit/MilliL"/>
   <qudt:numericalValue rdf:datatype="http://www.w3.org/2001/XMLSchema#double">12780</qudt:numericalValue>
   <rdf:value rdf:datatype="http://www.w3.org/2001/XMLSchema#double">12780</rdf:value>
   <gs1:unitCode>MLT</gs1:unitCode>
   <gs1:value>12780</gs1:value>
  </gs1:QuantitativeValue>
 </gs1:netContent>
 <sosa:isFeatureOfInterestOf>
  <rdf:Description rdf:about="#36xcan355ml-ContentSosa">
   <rdf:type rdf:resource="http://www.w3.org/ns/sosa/Observation"/>
   <sosa:hasFeatureOfInterest rdf:resource="#36xcan355ml"/>
   <sosa:observedProperty  rdf:resource="#netcontent"/>
   <sosa:hasResult rdf:resource="#36xcan355ml-Content"/>
   <sosa:hasSimpleResult rdf:datatype="http://www.qudt.org/2.1/vocab/unit/MilliM">12780</sosa:hasSimpleResult>
  </rdf:Description>
 </sosa:isFeatureOfInterestOf>
 </rdf:Description>

 <rdf:Description rdf:about="#8xcan355ml">
  <rdf:type rdf:resource="#LiquidContainer"/>
  <rdf:type rdf:resource="#BeverageCan"/>
  <rdf:type rdf:resource="https://gs1.org/voc/PackagingDetails"/>
  <rdfs:label xml:lang="en">8XCan355ml</rdfs:label>
  <rdfs:label xml:lang="fr">8XCan355ml</rdfs:label>
  <skos:definition xml:lang="en">Generic Flat, Box or Crate of 8, 355ml Cans</skos:definition>
  <skos:definition xml:lang="fr">Une boite, caisse ou caissette générique de 8 Canettes de 355ml</skos:definition>
  <rdfs:comment xml:lang="en">This term is meant to be used as a placeholder when no data about the aggregate packaging is known.</rdfs:comment>
  <rdfs:comment xml:lang="fr">Ce terme peut-être utilisé comme un terme générique lorsque les details de l’emballage ne sont pas certain.</rdfs:comment>
  <beer:count rdf:datatype="http://www.w3.org/2001/XMLSchema#Integer">8</beer:count>
  <beer:item rdf:resource="https://rdf.ag/o/beer#can355ml"/>
  <rdfs:isDefinedBy rdf:resource="https://rdf.ag/o/beer-ONTOLOGY_DATE"/>
  <void:inDataset rdf:resource="#datasetdefinition"/>
  <gs1:netContent>
   <gs1:QuantitativeValue rdf:about="#8xcan355ml-Content">
   <rdf:type rdf:resource="http://qudt.org/1.1/schema/qudt#QuantityValue"/>
   <qudt:unit rdf:resource="http://www.qudt.org/2.1/vocab/unit/MilliL"/>
   <qudt:numericalValue rdf:datatype="http://www.w3.org/2001/XMLSchema#double">2840</qudt:numericalValue>
   <rdf:value rdf:datatype="http://www.w3.org/2001/XMLSchema#double">2840</rdf:value>
   <gs1:unitCode>MLT</gs1:unitCode>
   <gs1:value>2840</gs1:value>
  </gs1:QuantitativeValue>
 </gs1:netContent>
 <sosa:isFeatureOfInterestOf>
  <rdf:Description rdf:about="#8xcan355ml-ContentSosa">
   <rdf:type rdf:resource="http://www.w3.org/ns/sosa/Observation"/>
   <sosa:hasFeatureOfInterest rdf:resource="#8xcan355ml"/>
   <sosa:observedProperty  rdf:resource="#netcontent"/>
   <sosa:hasResult rdf:resource="#8xcan355ml-Content"/>
   <sosa:hasSimpleResult rdf:datatype="http://www.qudt.org/2.1/vocab/unit/MilliM">2840</sosa:hasSimpleResult>
  </rdf:Description>
 </sosa:isFeatureOfInterestOf>
 </rdf:Description>

 <rdf:Description rdf:about="#18xcan355ml">
  <rdf:type rdf:resource="#LiquidContainer"/>
  <rdf:type rdf:resource="#BeverageCan"/>
  <rdf:type rdf:resource="https://gs1.org/voc/PackagingDetails"/>
  <rdfs:label xml:lang="en">18XCan355ml</rdfs:label>
  <rdfs:label xml:lang="fr">18XCan355ml</rdfs:label>
  <skos:definition xml:lang="en">Generic Flat, Box or Crate of 18, 355ml Cans</skos:definition>
  <skos:definition xml:lang="fr">Une boite, caisse ou caissette générique de 18 Canettes de 355ml</skos:definition>
  <rdfs:comment xml:lang="en">This term is meant to be used as a placeholder when no data about the aggregate packaging is known.</rdfs:comment>
  <rdfs:comment xml:lang="fr">Ce terme peut-être utilisé comme un terme générique lorsque les details de l’emballage ne sont pas certain.</rdfs:comment>
  <beer:count rdf:datatype="http://www.w3.org/2001/XMLSchema#Integer">18</beer:count>
  <beer:item rdf:resource="https://rdf.ag/o/beer#can355ml"/>
  <rdfs:isDefinedBy rdf:resource="https://rdf.ag/o/beer-ONTOLOGY_DATE"/>
  <void:inDataset rdf:resource="#datasetdefinition"/>
  <gs1:netContent>
   <gs1:QuantitativeValue rdf:about="#18xcan355ml-Content">
   <rdf:type rdf:resource="http://qudt.org/1.1/schema/qudt#QuantityValue"/>
   <qudt:unit rdf:resource="http://www.qudt.org/2.1/vocab/unit/MilliL"/>
   <qudt:numericalValue rdf:datatype="http://www.w3.org/2001/XMLSchema#double">6390</qudt:numericalValue>
   <rdf:value rdf:datatype="http://www.w3.org/2001/XMLSchema#double">6390</rdf:value>
   <gs1:unitCode>MLT</gs1:unitCode>
   <gs1:value>6390</gs1:value>
  </gs1:QuantitativeValue>
 </gs1:netContent>
 <sosa:isFeatureOfInterestOf>
  <rdf:Description rdf:about="#18xcan355ml-ContentSosa">
   <rdf:type rdf:resource="http://www.w3.org/ns/sosa/Observation"/>
   <sosa:hasFeatureOfInterest rdf:resource="#18xcan355ml"/>
   <sosa:observedProperty  rdf:resource="#netcontent"/>
   <sosa:hasResult rdf:resource="#18xcan355ml-Content"/>
   <sosa:hasSimpleResult rdf:datatype="http://www.qudt.org/2.1/vocab/unit/MilliM">6390</sosa:hasSimpleResult>
  </rdf:Description>
 </sosa:isFeatureOfInterestOf>
 </rdf:Description>

 <rdf:Description rdf:about="#48xcan355ml">
  <rdf:type rdf:resource="#LiquidContainer"/>
  <rdf:type rdf:resource="#BeverageCan"/>
  <rdf:type rdf:resource="https://gs1.org/voc/PackagingDetails"/>
  <rdfs:label xml:lang="en">48XCan355ml</rdfs:label>
  <rdfs:label xml:lang="fr">48XCan355ml</rdfs:label>
  <skos:definition xml:lang="en">Generic Flat, Box or Crate of 48, 355ml Cans</skos:definition>
  <skos:definition xml:lang="fr">Une boite, caisse ou caissette générique de 48 Canettes de 355ml</skos:definition>
  <rdfs:comment xml:lang="en">This term is meant to be used as a placeholder when no data about the aggregate packaging is known.</rdfs:comment>
  <rdfs:comment xml:lang="fr">Ce terme peut-être utilisé comme un terme générique lorsque les details de l’emballage ne sont pas certain.</rdfs:comment>
  <beer:count rdf:datatype="http://www.w3.org/2001/XMLSchema#Integer">48</beer:count>
  <beer:item rdf:resource="https://rdf.ag/o/beer#can355ml"/>
  <rdfs:isDefinedBy rdf:resource="https://rdf.ag/o/beer-ONTOLOGY_DATE"/>
  <void:inDataset rdf:resource="#datasetdefinition"/>
  <gs1:netContent>
   <gs1:QuantitativeValue rdf:about="#48xcan355ml-Content">
   <rdf:type rdf:resource="http://qudt.org/1.1/schema/qudt#QuantityValue"/>
   <qudt:unit rdf:resource="http://www.qudt.org/2.1/vocab/unit/MilliL"/>
   <qudt:numericalValue rdf:datatype="http://www.w3.org/2001/XMLSchema#double">17040</qudt:numericalValue>
   <rdf:value rdf:datatype="http://www.w3.org/2001/XMLSchema#double">17040</rdf:value>
   <gs1:unitCode>MLT</gs1:unitCode>
   <gs1:value>17040</gs1:value>
  </gs1:QuantitativeValue>
 </gs1:netContent>
 <sosa:isFeatureOfInterestOf>
  <rdf:Description rdf:about="#48xcan355ml-ContentSosa">
   <rdf:type rdf:resource="http://www.w3.org/ns/sosa/Observation"/>
   <sosa:hasFeatureOfInterest rdf:resource="#48xcan355ml"/>
   <sosa:observedProperty  rdf:resource="#netcontent"/>
   <sosa:hasResult rdf:resource="#48xcan355ml-Content"/>
   <sosa:hasSimpleResult rdf:datatype="http://www.qudt.org/2.1/vocab/unit/MilliM">17040</sosa:hasSimpleResult>
  </rdf:Description>
 </sosa:isFeatureOfInterestOf>
 </rdf:Description>

 <rdf:Description rdf:about="#24xbottle275ml">
  <rdf:type rdf:resource="#LiquidContainer"/>
  <rdf:type rdf:resource="#BeverageBottle"/>
  <rdf:type rdf:resource="https://gs1.org/voc/PackagingDetails"/>
  <rdfs:label xml:lang="en">24XBottle275ml</rdfs:label>
  <rdfs:label xml:lang="fr">24XBottle275ml</rdfs:label>
  <skos:definition xml:lang="en">Generic Flat, Box or Crate of 24, 275ml Bottles</skos:definition>
  <skos:definition xml:lang="fr">Une boite, caisse ou caissette générique de 24 Bouteilles de 275ml</skos:definition>
  <rdfs:comment xml:lang="en">This term is meant to be used as a placeholder when no data about the aggregate packaging is known.</rdfs:comment>
  <rdfs:comment xml:lang="fr">Ce terme peut-être utilisé comme un terme générique lorsque les details de l’emballage ne sont pas certain.</rdfs:comment>
  <beer:count rdf:datatype="http://www.w3.org/2001/XMLSchema#Integer">24</beer:count>
  <beer:item rdf:resource="https://rdf.ag/o/beer#bottle275ml"/>
  <rdfs:isDefinedBy rdf:resource="https://rdf.ag/o/beer-ONTOLOGY_DATE"/>
  <void:inDataset rdf:resource="#datasetdefinition"/>
  <gs1:netContent>
   <gs1:QuantitativeValue rdf:about="#24xbottle275ml-Content">
   <rdf:type rdf:resource="http://qudt.org/1.1/schema/qudt#QuantityValue"/>
   <qudt:unit rdf:resource="http://www.qudt.org/2.1/vocab/unit/MilliL"/>
   <qudt:numericalValue rdf:datatype="http://www.w3.org/2001/XMLSchema#double">6600</qudt:numericalValue>
   <rdf:value rdf:datatype="http://www.w3.org/2001/XMLSchema#double">6600</rdf:value>
   <gs1:unitCode>MLT</gs1:unitCode>
   <gs1:value>6600</gs1:value>
  </gs1:QuantitativeValue>
 </gs1:netContent>
 <sosa:isFeatureOfInterestOf>
  <rdf:Description rdf:about="#24xbottle275ml-ContentSosa">
   <rdf:type rdf:resource="http://www.w3.org/ns/sosa/Observation"/>
   <sosa:hasFeatureOfInterest rdf:resource="#24xbottle275ml"/>
   <sosa:observedProperty  rdf:resource="#netcontent"/>
   <sosa:hasResult rdf:resource="#24xbottle275ml-Content"/>
   <sosa:hasSimpleResult rdf:datatype="http://www.qudt.org/2.1/vocab/unit/MilliM">6600</sosa:hasSimpleResult>
  </rdf:Description>
 </sosa:isFeatureOfInterestOf>
 </rdf:Description>

 <rdf:Description rdf:about="#6xbottle275ml">
  <rdf:type rdf:resource="#LiquidContainer"/>
  <rdf:type rdf:resource="#BeverageBottle"/>
  <rdf:type rdf:resource="https://gs1.org/voc/PackagingDetails"/>
  <rdfs:label xml:lang="en">6XBottle275ml</rdfs:label>
  <rdfs:label xml:lang="fr">6XBottle275ml</rdfs:label>
  <skos:definition xml:lang="en">Generic Flat, Box or Crate of 6, 275ml Bottles</skos:definition>
  <skos:definition xml:lang="fr">Une boite, caisse ou caissette générique de 6 Bouteilles de 275ml</skos:definition>
  <rdfs:comment xml:lang="en">This term is meant to be used as a placeholder when no data about the aggregate packaging is known.</rdfs:comment>
  <rdfs:comment xml:lang="fr">Ce terme peut-être utilisé comme un terme générique lorsque les details de l’emballage ne sont pas certain.</rdfs:comment>
  <beer:count rdf:datatype="http://www.w3.org/2001/XMLSchema#Integer">6</beer:count>
  <beer:item rdf:resource="https://rdf.ag/o/beer#bottle275ml"/>
  <rdfs:isDefinedBy rdf:resource="https://rdf.ag/o/beer-ONTOLOGY_DATE"/>
  <void:inDataset rdf:resource="#datasetdefinition"/>
  <gs1:netContent>
   <gs1:QuantitativeValue rdf:about="#6xbottle275ml-Content">
   <rdf:type rdf:resource="http://qudt.org/1.1/schema/qudt#QuantityValue"/>
   <qudt:unit rdf:resource="http://www.qudt.org/2.1/vocab/unit/MilliL"/>
   <qudt:numericalValue rdf:datatype="http://www.w3.org/2001/XMLSchema#double">1650</qudt:numericalValue>
   <rdf:value rdf:datatype="http://www.w3.org/2001/XMLSchema#double">1650</rdf:value>
   <gs1:unitCode>MLT</gs1:unitCode>
   <gs1:value>1650</gs1:value>
  </gs1:QuantitativeValue>
 </gs1:netContent>
 <sosa:isFeatureOfInterestOf>
  <rdf:Description rdf:about="#6xbottle275ml-ContentSosa">
   <rdf:type rdf:resource="http://www.w3.org/ns/sosa/Observation"/>
   <sosa:hasFeatureOfInterest rdf:resource="#6xbottle275ml"/>
   <sosa:observedProperty  rdf:resource="#netcontent"/>
   <sosa:hasResult rdf:resource="#6xbottle275ml-Content"/>
   <sosa:hasSimpleResult rdf:datatype="http://www.qudt.org/2.1/vocab/unit/MilliM">1650</sosa:hasSimpleResult>
  </rdf:Description>
 </sosa:isFeatureOfInterestOf>
 </rdf:Description>

 <rdf:Description rdf:about="#20xcan236ml">
  <rdf:type rdf:resource="#LiquidContainer"/>
  <rdf:type rdf:resource="#BeverageCan"/>
  <rdf:type rdf:resource="https://gs1.org/voc/PackagingDetails"/>
  <rdfs:label xml:lang="en">20XCan236ml</rdfs:label>
  <rdfs:label xml:lang="fr">20XCan236ml</rdfs:label>
  <skos:definition xml:lang="en">Generic Flat, Box or Crate of 20, 236ml Cans</skos:definition>
  <skos:definition xml:lang="fr">Une boite, caisse ou caissette générique de 20 Canettes de 236ml</skos:definition>
  <rdfs:comment xml:lang="en">This term is meant to be used as a placeholder when no data about the aggregate packaging is known.</rdfs:comment>
  <rdfs:comment xml:lang="fr">Ce terme peut-être utilisé comme un terme générique lorsque les details de l’emballage ne sont pas certain.</rdfs:comment>
  <beer:count rdf:datatype="http://www.w3.org/2001/XMLSchema#Integer">20</beer:count>
  <beer:item rdf:resource="https://rdf.ag/o/beer#can236ml"/>
  <rdfs:isDefinedBy rdf:resource="https://rdf.ag/o/beer-ONTOLOGY_DATE"/>
  <void:inDataset rdf:resource="#datasetdefinition"/>
  <gs1:netContent>
   <gs1:QuantitativeValue rdf:about="#20xcan236ml-Content">
   <rdf:type rdf:resource="http://qudt.org/1.1/schema/qudt#QuantityValue"/>
   <qudt:unit rdf:resource="http://www.qudt.org/2.1/vocab/unit/MilliL"/>
   <qudt:numericalValue rdf:datatype="http://www.w3.org/2001/XMLSchema#double">4720</qudt:numericalValue>
   <rdf:value rdf:datatype="http://www.w3.org/2001/XMLSchema#double">4720</rdf:value>
   <gs1:unitCode>MLT</gs1:unitCode>
   <gs1:value>4720</gs1:value>
  </gs1:QuantitativeValue>
 </gs1:netContent>
 <sosa:isFeatureOfInterestOf>
  <rdf:Description rdf:about="#20xcan236ml-ContentSosa">
   <rdf:type rdf:resource="http://www.w3.org/ns/sosa/Observation"/>
   <sosa:hasFeatureOfInterest rdf:resource="#20xcan236ml"/>
   <sosa:observedProperty  rdf:resource="#netcontent"/>
   <sosa:hasResult rdf:resource="#20xcan236ml-Content"/>
   <sosa:hasSimpleResult rdf:datatype="http://www.qudt.org/2.1/vocab/unit/MilliM">4720</sosa:hasSimpleResult>
  </rdf:Description>
 </sosa:isFeatureOfInterestOf>
 </rdf:Description>

 <rdf:Description rdf:about="#12xcan236ml">
  <rdf:type rdf:resource="#LiquidContainer"/>
  <rdf:type rdf:resource="#BeverageCan"/>
  <rdf:type rdf:resource="https://gs1.org/voc/PackagingDetails"/>
  <rdfs:label xml:lang="en">12XCan236ml</rdfs:label>
  <rdfs:label xml:lang="fr">12XCan236ml</rdfs:label>
  <skos:definition xml:lang="en">Generic Flat, Box or Crate of 12, 236ml Cans</skos:definition>
  <skos:definition xml:lang="fr">Une boite, caisse ou caissette générique de 12 Canettes de 236ml</skos:definition>
  <rdfs:comment xml:lang="en">This term is meant to be used as a placeholder when no data about the aggregate packaging is known.</rdfs:comment>
  <rdfs:comment xml:lang="fr">Ce terme peut-être utilisé comme un terme générique lorsque les details de l’emballage ne sont pas certain.</rdfs:comment>
  <beer:count rdf:datatype="http://www.w3.org/2001/XMLSchema#Integer">12</beer:count>
  <beer:item rdf:resource="https://rdf.ag/o/beer#can236ml"/>
  <rdfs:isDefinedBy rdf:resource="https://rdf.ag/o/beer-ONTOLOGY_DATE"/>
  <void:inDataset rdf:resource="#datasetdefinition"/>
  <gs1:netContent>
   <gs1:QuantitativeValue rdf:about="#12xcan236ml-Content">
   <rdf:type rdf:resource="http://qudt.org/1.1/schema/qudt#QuantityValue"/>
   <qudt:unit rdf:resource="http://www.qudt.org/2.1/vocab/unit/MilliL"/>
   <qudt:numericalValue rdf:datatype="http://www.w3.org/2001/XMLSchema#double">2832</qudt:numericalValue>
   <rdf:value rdf:datatype="http://www.w3.org/2001/XMLSchema#double">2832</rdf:value>
   <gs1:unitCode>MLT</gs1:unitCode>
   <gs1:value>2832</gs1:value>
  </gs1:QuantitativeValue>
 </gs1:netContent>
 <sosa:isFeatureOfInterestOf>
  <rdf:Description rdf:about="#12xcan236ml-ContentSosa">
   <rdf:type rdf:resource="http://www.w3.org/ns/sosa/Observation"/>
   <sosa:hasFeatureOfInterest rdf:resource="#12xcan236ml"/>
   <sosa:observedProperty  rdf:resource="#netcontent"/>
   <sosa:hasResult rdf:resource="#12xcan236ml-Content"/>
   <sosa:hasSimpleResult rdf:datatype="http://www.qudt.org/2.1/vocab/unit/MilliM">2832</sosa:hasSimpleResult>
  </rdf:Description>
 </sosa:isFeatureOfInterestOf>
 </rdf:Description>

 <rdf:Description rdf:about="#4xcan236ml">
  <rdf:type rdf:resource="#LiquidContainer"/>
  <rdf:type rdf:resource="#BeverageCan"/>
  <rdf:type rdf:resource="https://gs1.org/voc/PackagingDetails"/>
  <rdfs:label xml:lang="en">4XCan236ml</rdfs:label>
  <rdfs:label xml:lang="fr">4XCan236ml</rdfs:label>
  <skos:definition xml:lang="en">Generic Flat, Box or Crate of 4, 236ml Cans</skos:definition>
  <skos:definition xml:lang="fr">Une boite, caisse ou caissette générique de 4 Canettes de 236ml</skos:definition>
  <rdfs:comment xml:lang="en">This term is meant to be used as a placeholder when no data about the aggregate packaging is known.</rdfs:comment>
  <rdfs:comment xml:lang="fr">Ce terme peut-être utilisé comme un terme générique lorsque les details de l’emballage ne sont pas certain.</rdfs:comment>
  <beer:count rdf:datatype="http://www.w3.org/2001/XMLSchema#Integer">4</beer:count>
  <beer:item rdf:resource="https://rdf.ag/o/beer#can236ml"/>
  <rdfs:isDefinedBy rdf:resource="https://rdf.ag/o/beer-ONTOLOGY_DATE"/>
  <void:inDataset rdf:resource="#datasetdefinition"/>
  <gs1:netContent>
   <gs1:QuantitativeValue rdf:about="#4xcan236ml-Content">
   <rdf:type rdf:resource="http://qudt.org/1.1/schema/qudt#QuantityValue"/>
   <qudt:unit rdf:resource="http://www.qudt.org/2.1/vocab/unit/MilliL"/>
   <qudt:numericalValue rdf:datatype="http://www.w3.org/2001/XMLSchema#double">944</qudt:numericalValue>
   <rdf:value rdf:datatype="http://www.w3.org/2001/XMLSchema#double">944</rdf:value>
   <gs1:unitCode>MLT</gs1:unitCode>
   <gs1:value>944</gs1:value>
  </gs1:QuantitativeValue>
 </gs1:netContent>
 <sosa:isFeatureOfInterestOf>
  <rdf:Description rdf:about="#4xcan236ml-ContentSosa">
   <rdf:type rdf:resource="http://www.w3.org/ns/sosa/Observation"/>
   <sosa:hasFeatureOfInterest rdf:resource="#4xcan236ml"/>
   <sosa:observedProperty  rdf:resource="#netcontent"/>
   <sosa:hasResult rdf:resource="#4xcan236ml-Content"/>
   <sosa:hasSimpleResult rdf:datatype="http://www.qudt.org/2.1/vocab/unit/MilliM">944</sosa:hasSimpleResult>
  </rdf:Description>
 </sosa:isFeatureOfInterestOf>
 </rdf:Description>

 <rdf:Description rdf:about="#24xcan236ml">
  <rdf:type rdf:resource="#LiquidContainer"/>
  <rdf:type rdf:resource="#BeverageCan"/>
  <rdf:type rdf:resource="https://gs1.org/voc/PackagingDetails"/>
  <rdfs:label xml:lang="en">24XCan236ml</rdfs:label>
  <rdfs:label xml:lang="fr">24XCan236ml</rdfs:label>
  <skos:definition xml:lang="en">Generic Flat, Box or Crate of 24, 236ml Cans</skos:definition>
  <skos:definition xml:lang="fr">Une boite, caisse ou caissette générique de 24 Canettes de 236ml</skos:definition>
  <rdfs:comment xml:lang="en">This term is meant to be used as a placeholder when no data about the aggregate packaging is known.</rdfs:comment>
  <rdfs:comment xml:lang="fr">Ce terme peut-être utilisé comme un terme générique lorsque les details de l’emballage ne sont pas certain.</rdfs:comment>
  <beer:count rdf:datatype="http://www.w3.org/2001/XMLSchema#Integer">24</beer:count>
  <beer:item rdf:resource="https://rdf.ag/o/beer#can236ml"/>
  <rdfs:isDefinedBy rdf:resource="https://rdf.ag/o/beer-ONTOLOGY_DATE"/>
  <void:inDataset rdf:resource="#datasetdefinition"/>
  <gs1:netContent>
   <gs1:QuantitativeValue rdf:about="#24xcan236ml-Content">
   <rdf:type rdf:resource="http://qudt.org/1.1/schema/qudt#QuantityValue"/>
   <qudt:unit rdf:resource="http://www.qudt.org/2.1/vocab/unit/MilliL"/>
   <qudt:numericalValue rdf:datatype="http://www.w3.org/2001/XMLSchema#double">5664</qudt:numericalValue>
   <rdf:value rdf:datatype="http://www.w3.org/2001/XMLSchema#double">5664</rdf:value>
   <gs1:unitCode>MLT</gs1:unitCode>
   <gs1:value>5664</gs1:value>
  </gs1:QuantitativeValue>
 </gs1:netContent>
 <sosa:isFeatureOfInterestOf>
  <rdf:Description rdf:about="#24xcan236ml-ContentSosa">
   <rdf:type rdf:resource="http://www.w3.org/ns/sosa/Observation"/>
   <sosa:hasFeatureOfInterest rdf:resource="#24xcan236ml"/>
   <sosa:observedProperty  rdf:resource="#netcontent"/>
   <sosa:hasResult rdf:resource="#24xcan236ml-Content"/>
   <sosa:hasSimpleResult rdf:datatype="http://www.qudt.org/2.1/vocab/unit/MilliM">5664</sosa:hasSimpleResult>
  </rdf:Description>
 </sosa:isFeatureOfInterestOf>
 </rdf:Description>

 <rdf:Description rdf:about="#16xcan236ml">
  <rdf:type rdf:resource="#LiquidContainer"/>
  <rdf:type rdf:resource="#BeverageCan"/>
  <rdf:type rdf:resource="https://gs1.org/voc/PackagingDetails"/>
  <rdfs:label xml:lang="en">16XCan236ml</rdfs:label>
  <rdfs:label xml:lang="fr">16XCan236ml</rdfs:label>
  <skos:definition xml:lang="en">Generic Flat, Box or Crate of 16, 236ml Cans</skos:definition>
  <skos:definition xml:lang="fr">Une boite, caisse ou caissette générique de 16 Canettes de 236ml</skos:definition>
  <rdfs:comment xml:lang="en">This term is meant to be used as a placeholder when no data about the aggregate packaging is known.</rdfs:comment>
  <rdfs:comment xml:lang="fr">Ce terme peut-être utilisé comme un terme générique lorsque les details de l’emballage ne sont pas certain.</rdfs:comment>
  <beer:count rdf:datatype="http://www.w3.org/2001/XMLSchema#Integer">16</beer:count>
  <beer:item rdf:resource="https://rdf.ag/o/beer#can236ml"/>
  <rdfs:isDefinedBy rdf:resource="https://rdf.ag/o/beer-ONTOLOGY_DATE"/>
  <void:inDataset rdf:resource="#datasetdefinition"/>
  <gs1:netContent>
   <gs1:QuantitativeValue rdf:about="#16xcan236ml-Content">
   <rdf:type rdf:resource="http://qudt.org/1.1/schema/qudt#QuantityValue"/>
   <qudt:unit rdf:resource="http://www.qudt.org/2.1/vocab/unit/MilliL"/>
   <qudt:numericalValue rdf:datatype="http://www.w3.org/2001/XMLSchema#double">3776</qudt:numericalValue>
   <rdf:value rdf:datatype="http://www.w3.org/2001/XMLSchema#double">3776</rdf:value>
   <gs1:unitCode>MLT</gs1:unitCode>
   <gs1:value>3776</gs1:value>
  </gs1:QuantitativeValue>
 </gs1:netContent>
 <sosa:isFeatureOfInterestOf>
  <rdf:Description rdf:about="#16xcan236ml-ContentSosa">
   <rdf:type rdf:resource="http://www.w3.org/ns/sosa/Observation"/>
   <sosa:hasFeatureOfInterest rdf:resource="#16xcan236ml"/>
   <sosa:observedProperty  rdf:resource="#netcontent"/>
   <sosa:hasResult rdf:resource="#16xcan236ml-Content"/>
   <sosa:hasSimpleResult rdf:datatype="http://www.qudt.org/2.1/vocab/unit/MilliM">3776</sosa:hasSimpleResult>
  </rdf:Description>
 </sosa:isFeatureOfInterestOf>
 </rdf:Description>

 <rdf:Description rdf:about="#8xcan236ml">
  <rdf:type rdf:resource="#LiquidContainer"/>
  <rdf:type rdf:resource="#BeverageCan"/>
  <rdf:type rdf:resource="https://gs1.org/voc/PackagingDetails"/>
  <rdfs:label xml:lang="en">8XCan236ml</rdfs:label>
  <rdfs:label xml:lang="fr">8XCan236ml</rdfs:label>
  <skos:definition xml:lang="en">Generic Flat, Box or Crate of 8, 236ml Cans</skos:definition>
  <skos:definition xml:lang="fr">Une boite, caisse ou caissette générique de 8 Canettes de 236ml</skos:definition>
  <rdfs:comment xml:lang="en">This term is meant to be used as a placeholder when no data about the aggregate packaging is known.</rdfs:comment>
  <rdfs:comment xml:lang="fr">Ce terme peut-être utilisé comme un terme générique lorsque les details de l’emballage ne sont pas certain.</rdfs:comment>
  <beer:count rdf:datatype="http://www.w3.org/2001/XMLSchema#Integer">8</beer:count>
  <beer:item rdf:resource="https://rdf.ag/o/beer#can236ml"/>
  <rdfs:isDefinedBy rdf:resource="https://rdf.ag/o/beer-ONTOLOGY_DATE"/>
  <void:inDataset rdf:resource="#datasetdefinition"/>
  <gs1:netContent>
   <gs1:QuantitativeValue rdf:about="#8xcan236ml-Content">
   <rdf:type rdf:resource="http://qudt.org/1.1/schema/qudt#QuantityValue"/>
   <qudt:unit rdf:resource="http://www.qudt.org/2.1/vocab/unit/MilliL"/>
   <qudt:numericalValue rdf:datatype="http://www.w3.org/2001/XMLSchema#double">1888</qudt:numericalValue>
   <rdf:value rdf:datatype="http://www.w3.org/2001/XMLSchema#double">1888</rdf:value>
   <gs1:unitCode>MLT</gs1:unitCode>
   <gs1:value>1888</gs1:value>
  </gs1:QuantitativeValue>
 </gs1:netContent>
 <sosa:isFeatureOfInterestOf>
  <rdf:Description rdf:about="#8xcan236ml-ContentSosa">
   <rdf:type rdf:resource="http://www.w3.org/ns/sosa/Observation"/>
   <sosa:hasFeatureOfInterest rdf:resource="#8xcan236ml"/>
   <sosa:observedProperty  rdf:resource="#netcontent"/>
   <sosa:hasResult rdf:resource="#8xcan236ml-Content"/>
   <sosa:hasSimpleResult rdf:datatype="http://www.qudt.org/2.1/vocab/unit/MilliM">1888</sosa:hasSimpleResult>
  </rdf:Description>
 </sosa:isFeatureOfInterestOf>
 </rdf:Description>

 <rdf:Description rdf:about="#12xbottle207ml">
  <rdf:type rdf:resource="#LiquidContainer"/>
  <rdf:type rdf:resource="#BeverageBottle"/>
  <rdf:type rdf:resource="https://gs1.org/voc/PackagingDetails"/>
  <rdfs:label xml:lang="en">12XBottle207ml</rdfs:label>
  <rdfs:label xml:lang="fr">12XBottle207ml</rdfs:label>
  <skos:definition xml:lang="en">Generic Flat, Box or Crate of 12, 207ml Bottles</skos:definition>
  <skos:definition xml:lang="fr">Une boite, caisse ou caissette générique de 12 Bouteilles de 207ml</skos:definition>
  <rdfs:comment xml:lang="en">This term is meant to be used as a placeholder when no data about the aggregate packaging is known.</rdfs:comment>
  <rdfs:comment xml:lang="fr">Ce terme peut-être utilisé comme un terme générique lorsque les details de l’emballage ne sont pas certain.</rdfs:comment>
  <beer:count rdf:datatype="http://www.w3.org/2001/XMLSchema#Integer">12</beer:count>
  <beer:item rdf:resource="https://rdf.ag/o/beer#bottle207ml"/>
  <rdfs:isDefinedBy rdf:resource="https://rdf.ag/o/beer-ONTOLOGY_DATE"/>
  <void:inDataset rdf:resource="#datasetdefinition"/>
  <gs1:netContent>
   <gs1:QuantitativeValue rdf:about="#12xbottle207ml-Content">
   <rdf:type rdf:resource="http://qudt.org/1.1/schema/qudt#QuantityValue"/>
   <qudt:unit rdf:resource="http://www.qudt.org/2.1/vocab/unit/MilliL"/>
   <qudt:numericalValue rdf:datatype="http://www.w3.org/2001/XMLSchema#double">2484</qudt:numericalValue>
   <rdf:value rdf:datatype="http://www.w3.org/2001/XMLSchema#double">2484</rdf:value>
   <gs1:unitCode>MLT</gs1:unitCode>
   <gs1:value>2484</gs1:value>
  </gs1:QuantitativeValue>
 </gs1:netContent>
 <sosa:isFeatureOfInterestOf>
  <rdf:Description rdf:about="#12xbottle207ml-ContentSosa">
   <rdf:type rdf:resource="http://www.w3.org/ns/sosa/Observation"/>
   <sosa:hasFeatureOfInterest rdf:resource="#12xbottle207ml"/>
   <sosa:observedProperty  rdf:resource="#netcontent"/>
   <sosa:hasResult rdf:resource="#12xbottle207ml-Content"/>
   <sosa:hasSimpleResult rdf:datatype="http://www.qudt.org/2.1/vocab/unit/MilliM">2484</sosa:hasSimpleResult>
  </rdf:Description>
 </sosa:isFeatureOfInterestOf>
 </rdf:Description>

 <rdf:Description rdf:about="#24xbottle207ml">
  <rdf:type rdf:resource="#LiquidContainer"/>
  <rdf:type rdf:resource="#BeverageBottle"/>
  <rdf:type rdf:resource="https://gs1.org/voc/PackagingDetails"/>
  <rdfs:label xml:lang="en">24XBottle207ml</rdfs:label>
  <rdfs:label xml:lang="fr">24XBottle207ml</rdfs:label>
  <skos:definition xml:lang="en">Generic Flat, Box or Crate of 24, 207ml Bottles</skos:definition>
  <skos:definition xml:lang="fr">Une boite, caisse ou caissette générique de 24 Bouteilles de 207ml</skos:definition>
  <rdfs:comment xml:lang="en">This term is meant to be used as a placeholder when no data about the aggregate packaging is known.</rdfs:comment>
  <rdfs:comment xml:lang="fr">Ce terme peut-être utilisé comme un terme générique lorsque les details de l’emballage ne sont pas certain.</rdfs:comment>
  <beer:count rdf:datatype="http://www.w3.org/2001/XMLSchema#Integer">24</beer:count>
  <beer:item rdf:resource="https://rdf.ag/o/beer#bottle207ml"/>
  <rdfs:isDefinedBy rdf:resource="https://rdf.ag/o/beer-ONTOLOGY_DATE"/>
  <void:inDataset rdf:resource="#datasetdefinition"/>
  <gs1:netContent>
   <gs1:QuantitativeValue rdf:about="#24xbottle207ml-Content">
   <rdf:type rdf:resource="http://qudt.org/1.1/schema/qudt#QuantityValue"/>
   <qudt:unit rdf:resource="http://www.qudt.org/2.1/vocab/unit/MilliL"/>
   <qudt:numericalValue rdf:datatype="http://www.w3.org/2001/XMLSchema#double">4968</qudt:numericalValue>
   <rdf:value rdf:datatype="http://www.w3.org/2001/XMLSchema#double">4968</rdf:value>
   <gs1:unitCode>MLT</gs1:unitCode>
   <gs1:value>4968</gs1:value>
  </gs1:QuantitativeValue>
 </gs1:netContent>
 <sosa:isFeatureOfInterestOf>
  <rdf:Description rdf:about="#24xbottle207ml-ContentSosa">
   <rdf:type rdf:resource="http://www.w3.org/ns/sosa/Observation"/>
   <sosa:hasFeatureOfInterest rdf:resource="#24xbottle207ml"/>
   <sosa:observedProperty  rdf:resource="#netcontent"/>
   <sosa:hasResult rdf:resource="#24xbottle207ml-Content"/>
   <sosa:hasSimpleResult rdf:datatype="http://www.qudt.org/2.1/vocab/unit/MilliM">4968</sosa:hasSimpleResult>
  </rdf:Description>
 </sosa:isFeatureOfInterestOf>
 </rdf:Description>

 <rdf:Description rdf:about="#6xbottle207ml">
  <rdf:type rdf:resource="#LiquidContainer"/>
  <rdf:type rdf:resource="#BeverageBottle"/>
  <rdf:type rdf:resource="https://gs1.org/voc/PackagingDetails"/>
  <rdfs:label xml:lang="en">6XBottle207ml</rdfs:label>
  <rdfs:label xml:lang="fr">6XBottle207ml</rdfs:label>
  <skos:definition xml:lang="en">Generic Flat, Box or Crate of 6, 207ml Bottles</skos:definition>
  <skos:definition xml:lang="fr">Une boite, caisse ou caissette générique de 6 Bouteilles de 207ml</skos:definition>
  <rdfs:comment xml:lang="en">This term is meant to be used as a placeholder when no data about the aggregate packaging is known.</rdfs:comment>
  <rdfs:comment xml:lang="fr">Ce terme peut-être utilisé comme un terme générique lorsque les details de l’emballage ne sont pas certain.</rdfs:comment>
  <beer:count rdf:datatype="http://www.w3.org/2001/XMLSchema#Integer">6</beer:count>
  <beer:item rdf:resource="https://rdf.ag/o/beer#bottle207ml"/>
  <rdfs:isDefinedBy rdf:resource="https://rdf.ag/o/beer-ONTOLOGY_DATE"/>
  <void:inDataset rdf:resource="#datasetdefinition"/>
  <gs1:netContent>
   <gs1:QuantitativeValue rdf:about="#6xbottle207ml-Content">
   <rdf:type rdf:resource="http://qudt.org/1.1/schema/qudt#QuantityValue"/>
   <qudt:unit rdf:resource="http://www.qudt.org/2.1/vocab/unit/MilliL"/>
   <qudt:numericalValue rdf:datatype="http://www.w3.org/2001/XMLSchema#double">1242</qudt:numericalValue>
   <rdf:value rdf:datatype="http://www.w3.org/2001/XMLSchema#double">1242</rdf:value>
   <gs1:unitCode>MLT</gs1:unitCode>
   <gs1:value>1242</gs1:value>
  </gs1:QuantitativeValue>
 </gs1:netContent>
 <sosa:isFeatureOfInterestOf>
  <rdf:Description rdf:about="#6xbottle207ml-ContentSosa">
   <rdf:type rdf:resource="http://www.w3.org/ns/sosa/Observation"/>
   <sosa:hasFeatureOfInterest rdf:resource="#6xbottle207ml"/>
   <sosa:observedProperty  rdf:resource="#netcontent"/>
   <sosa:hasResult rdf:resource="#6xbottle207ml-Content"/>
   <sosa:hasSimpleResult rdf:datatype="http://www.qudt.org/2.1/vocab/unit/MilliM">1242</sosa:hasSimpleResult>
  </rdf:Description>
 </sosa:isFeatureOfInterestOf>
 </rdf:Description>

 <rdf:Description rdf:about="#12xcan568ml">
  <rdf:type rdf:resource="#LiquidContainer"/>
  <rdf:type rdf:resource="#BeverageCan"/>
  <rdf:type rdf:resource="https://gs1.org/voc/PackagingDetails"/>
  <rdfs:label xml:lang="en">12XCan568ml</rdfs:label>
  <rdfs:label xml:lang="fr">12XCan568ml</rdfs:label>
  <skos:definition xml:lang="en">Generic Flat, Box or Crate of 12, 568ml Cans</skos:definition>
  <skos:definition xml:lang="fr">Une boite, caisse ou caissette générique de 12 Canettes de 568ml</skos:definition>
  <rdfs:comment xml:lang="en">This term is meant to be used as a placeholder when no data about the aggregate packaging is known.</rdfs:comment>
  <rdfs:comment xml:lang="fr">Ce terme peut-être utilisé comme un terme générique lorsque les details de l’emballage ne sont pas certain.</rdfs:comment>
  <beer:count rdf:datatype="http://www.w3.org/2001/XMLSchema#Integer">12</beer:count>
  <beer:item rdf:resource="https://rdf.ag/o/beer#can568ml"/>
  <rdfs:isDefinedBy rdf:resource="https://rdf.ag/o/beer-ONTOLOGY_DATE"/>
  <void:inDataset rdf:resource="#datasetdefinition"/>
  <gs1:netContent>
   <gs1:QuantitativeValue rdf:about="#12xcan568ml-Content">
   <rdf:type rdf:resource="http://qudt.org/1.1/schema/qudt#QuantityValue"/>
   <qudt:unit rdf:resource="http://www.qudt.org/2.1/vocab/unit/MilliL"/>
   <qudt:numericalValue rdf:datatype="http://www.w3.org/2001/XMLSchema#double">6816</qudt:numericalValue>
   <rdf:value rdf:datatype="http://www.w3.org/2001/XMLSchema#double">6816</rdf:value>
   <gs1:unitCode>MLT</gs1:unitCode>
   <gs1:value>6816</gs1:value>
  </gs1:QuantitativeValue>
 </gs1:netContent>
 <sosa:isFeatureOfInterestOf>
  <rdf:Description rdf:about="#12xcan568ml-ContentSosa">
   <rdf:type rdf:resource="http://www.w3.org/ns/sosa/Observation"/>
   <sosa:hasFeatureOfInterest rdf:resource="#12xcan568ml"/>
   <sosa:observedProperty  rdf:resource="#netcontent"/>
   <sosa:hasResult rdf:resource="#12xcan568ml-Content"/>
   <sosa:hasSimpleResult rdf:datatype="http://www.qudt.org/2.1/vocab/unit/MilliM">6816</sosa:hasSimpleResult>
  </rdf:Description>
 </sosa:isFeatureOfInterestOf>
 </rdf:Description>

 <rdf:Description rdf:about="#24xcan568ml">
  <rdf:type rdf:resource="#LiquidContainer"/>
  <rdf:type rdf:resource="#BeverageCan"/>
  <rdf:type rdf:resource="https://gs1.org/voc/PackagingDetails"/>
  <rdfs:label xml:lang="en">24XCan568ml</rdfs:label>
  <rdfs:label xml:lang="fr">24XCan568ml</rdfs:label>
  <skos:definition xml:lang="en">Generic Flat, Box or Crate of 24, 568ml Cans</skos:definition>
  <skos:definition xml:lang="fr">Une boite, caisse ou caissette générique de 24 Canettes de 568ml</skos:definition>
  <rdfs:comment xml:lang="en">This term is meant to be used as a placeholder when no data about the aggregate packaging is known.</rdfs:comment>
  <rdfs:comment xml:lang="fr">Ce terme peut-être utilisé comme un terme générique lorsque les details de l’emballage ne sont pas certain.</rdfs:comment>
  <beer:count rdf:datatype="http://www.w3.org/2001/XMLSchema#Integer">24</beer:count>
  <beer:item rdf:resource="https://rdf.ag/o/beer#can568ml"/>
  <rdfs:isDefinedBy rdf:resource="https://rdf.ag/o/beer-ONTOLOGY_DATE"/>
  <void:inDataset rdf:resource="#datasetdefinition"/>
  <gs1:netContent>
   <gs1:QuantitativeValue rdf:about="#24xcan568ml-Content">
   <rdf:type rdf:resource="http://qudt.org/1.1/schema/qudt#QuantityValue"/>
   <qudt:unit rdf:resource="http://www.qudt.org/2.1/vocab/unit/MilliL"/>
   <qudt:numericalValue rdf:datatype="http://www.w3.org/2001/XMLSchema#double">13632</qudt:numericalValue>
   <rdf:value rdf:datatype="http://www.w3.org/2001/XMLSchema#double">13632</rdf:value>
   <gs1:unitCode>MLT</gs1:unitCode>
   <gs1:value>13632</gs1:value>
  </gs1:QuantitativeValue>
 </gs1:netContent>
 <sosa:isFeatureOfInterestOf>
  <rdf:Description rdf:about="#24xcan568ml-ContentSosa">
   <rdf:type rdf:resource="http://www.w3.org/ns/sosa/Observation"/>
   <sosa:hasFeatureOfInterest rdf:resource="#24xcan568ml"/>
   <sosa:observedProperty  rdf:resource="#netcontent"/>
   <sosa:hasResult rdf:resource="#24xcan568ml-Content"/>
   <sosa:hasSimpleResult rdf:datatype="http://www.qudt.org/2.1/vocab/unit/MilliM">13632</sosa:hasSimpleResult>
  </rdf:Description>
 </sosa:isFeatureOfInterestOf>
 </rdf:Description>

 <rdf:Description rdf:about="#6xcan568ml">
  <rdf:type rdf:resource="#LiquidContainer"/>
  <rdf:type rdf:resource="#BeverageCan"/>
  <rdf:type rdf:resource="https://gs1.org/voc/PackagingDetails"/>
  <rdfs:label xml:lang="en">6XCan568ml</rdfs:label>
  <rdfs:label xml:lang="fr">6XCan568ml</rdfs:label>
  <skos:definition xml:lang="en">Generic Flat, Box or Crate of 6, 568ml Cans</skos:definition>
  <skos:definition xml:lang="fr">Une boite, caisse ou caissette générique de 6 Canettes de 568ml</skos:definition>
  <rdfs:comment xml:lang="en">This term is meant to be used as a placeholder when no data about the aggregate packaging is known.</rdfs:comment>
  <rdfs:comment xml:lang="fr">Ce terme peut-être utilisé comme un terme générique lorsque les details de l’emballage ne sont pas certain.</rdfs:comment>
  <beer:count rdf:datatype="http://www.w3.org/2001/XMLSchema#Integer">6</beer:count>
  <beer:item rdf:resource="https://rdf.ag/o/beer#can568ml"/>
  <rdfs:isDefinedBy rdf:resource="https://rdf.ag/o/beer-ONTOLOGY_DATE"/>
  <void:inDataset rdf:resource="#datasetdefinition"/>
  <gs1:netContent>
   <gs1:QuantitativeValue rdf:about="#6xcan568ml-Content">
   <rdf:type rdf:resource="http://qudt.org/1.1/schema/qudt#QuantityValue"/>
   <qudt:unit rdf:resource="http://www.qudt.org/2.1/vocab/unit/MilliL"/>
   <qudt:numericalValue rdf:datatype="http://www.w3.org/2001/XMLSchema#double">3408</qudt:numericalValue>
   <rdf:value rdf:datatype="http://www.w3.org/2001/XMLSchema#double">3408</rdf:value>
   <gs1:unitCode>MLT</gs1:unitCode>
   <gs1:value>3408</gs1:value>
  </gs1:QuantitativeValue>
 </gs1:netContent>
 <sosa:isFeatureOfInterestOf>
  <rdf:Description rdf:about="#6xcan568ml-ContentSosa">
   <rdf:type rdf:resource="http://www.w3.org/ns/sosa/Observation"/>
   <sosa:hasFeatureOfInterest rdf:resource="#6xcan568ml"/>
   <sosa:observedProperty  rdf:resource="#netcontent"/>
   <sosa:hasResult rdf:resource="#6xcan568ml-Content"/>
   <sosa:hasSimpleResult rdf:datatype="http://www.qudt.org/2.1/vocab/unit/MilliM">3408</sosa:hasSimpleResult>
  </rdf:Description>
 </sosa:isFeatureOfInterestOf>
 </rdf:Description>



<!-- Nominal capacity, Actual fill capacity, height, width, weight -->

<rdf:Description rdf:about="#height">
 <rdf:type rdf:resource="http://www.w3.org/ns/sosa/ObservableProperty"/>
 <rdf:type rdf:resource="http://www.w3.org/ns/ssn/Property"/>
 <rdfs:label xml:lang="en">Height</rdfs:label>
 <rdfs:label xml:lang="fr">Hauteur</rdfs:label>
 <skos:definition xml:lang="en">The measurement from base to top of something.</skos:definition>  
 <skos:definition xml:lang="fr">La mesure de la base au sommet d'une chose.</skos:definition>  
 <rdfs:isDefinedBy rdf:resource="https://rdf.ag/o/beer-ONTOLOGY_DATE"/>
 <void:inDataset rdf:resource="#datasetdefinition"/>
</rdf:Description>

<rdf:Description rdf:about="#diameter">
 <rdf:type rdf:resource="http://www.w3.org/ns/sosa/ObservableProperty"/>
 <rdf:type rdf:resource="http://www.w3.org/ns/ssn/Property"/>
 <rdfs:label xml:lang="en">Diameter</rdfs:label>
 <rdfs:label xml:lang="fr">Diamètre</rdfs:label>
 <skos:definition xml:lang="en">A diameter is a chord that runs through the center point of the circle.</skos:definition>  
 <skos:definition xml:lang="fr">Le diamètre est un segment de droite passant par le centre.</skos:definition>  
 <rdfs:isDefinedBy rdf:resource="https://rdf.ag/o/beer-ONTOLOGY_DATE"/>
 <void:inDataset rdf:resource="#datasetdefinition"/>
</rdf:Description>

<rdf:Description rdf:about="#endDiameter">
 <rdf:type rdf:resource="http://www.w3.org/ns/sosa/ObservableProperty"/>
 <rdf:type rdf:resource="http://www.w3.org/ns/ssn/Property"/>
 <rdfs:label xml:lang="en">End Diameter</rdfs:label>
 <rdfs:label xml:lang="fr">Diamètre de Bout</rdfs:label>
 <skos:definition xml:lang="en">A diameter is a chord that runs through the center point of the circle at the extremeties of the can.</skos:definition>  
 <skos:definition xml:lang="fr">Le diamètre est un segment de droite passant par le centre à l'extrémité de la canette.</skos:definition>  
 <rdfs:isDefinedBy rdf:resource="https://rdf.ag/o/beer-ONTOLOGY_DATE"/>
 <void:inDataset rdf:resource="#datasetdefinition"/>
</rdf:Description>

<rdf:Description rdf:about="#sosaNominalCapacity">
 <rdf:type rdf:resource="http://www.w3.org/ns/sosa/ObservableProperty"/>
 <rdf:type rdf:resource="http://www.w3.org/ns/ssn/Property"/>
 <rdfs:label xml:lang="en">Nominal Capacity</rdfs:label>
 <rdfs:label xml:lang="fr">Capacité nominale</rdfs:label>
 <skos:definition xml:lang="en">The volume of the tank when filled to the top.</skos:definition>  
 <skos:definition xml:lang="fr">Le volume du réservoir lorsqu'il est rempli completement.</skos:definition>  
 <rdfs:isDefinedBy rdf:resource="https://rdf.ag/o/beer-ONTOLOGY_DATE"/>
 <void:inDataset rdf:resource="#datasetdefinition"/>
</rdf:Description>

<owl:DatatypeProperty rdf:ID="nominalCapacity">
 <rdfs:label xml:lang="en">Nominal Capacity</rdfs:label>
 <rdfs:label xml:lang="fr">Capacité nominale</rdfs:label>
 <skos:definition xml:lang="en">The volume of the tank when filled to the top.</skos:definition>  
 <skos:definition xml:lang="fr">Le volume du réservoir lorsqu'il est rempli completement.</skos:definition>  
 <rdfs:isDefinedBy rdf:resource="https://rdf.ag/o/beer-ONTOLOGY_DATE"/>
 <void:inDataset rdf:resource="#datasetdefinition"/>
</owl:DatatypeProperty>

<rdf:Description rdf:about="#netContent">
 <rdf:type rdf:resource="http://www.w3.org/ns/sosa/ObservableProperty"/>
 <rdf:type rdf:resource="http://www.w3.org/ns/ssn/Property"/>
 <rdfs:label xml:lang="en">Net Content</rdfs:label>
 <rdfs:label xml:lang="fr">Contenu Net</rdfs:label>
 <skos:definition xml:lang="en">The amount of the consumable product without packaging.</skos:definition>  
 <skos:definition xml:lang="fr">Le montant de produit consommable dans l'emballage.</skos:definition>  
 <rdfs:isDefinedBy rdf:resource="https://rdf.ag/o/beer-ONTOLOGY_DATE"/>
 <void:inDataset rdf:resource="#datasetdefinition"/>
</rdf:Description>
        
<rdf:Description rdf:about="#overflowCapacity">
 <rdf:type rdf:resource="http://www.w3.org/ns/sosa/ObservableProperty"/>
 <rdf:type rdf:resource="http://www.w3.org/ns/ssn/Property"/>
 <rdfs:label xml:lang="en">Overflow Capacity</rdfs:label>
 <rdfs:label xml:lang="fr">Capacité à débordement</rdfs:label>
 <skos:definition xml:lang="en">The exact amount of liquid the container can hold when filled to the brim.</skos:definition>  
 <skos:definition xml:lang="fr">La quantité exacte de liquide que le récipient peut contenir lorsqu'il est rempli à ras bord.</skos:definition>  
 <rdfs:isDefinedBy rdf:resource="https://rdf.ag/o/beer-ONTOLOGY_DATE"/>
 <void:inDataset rdf:resource="#datasetdefinition"/>
</rdf:Description>
    
<rdf:Description rdf:about="#standardCapacity">
 <rdf:type rdf:resource="http://www.w3.org/ns/sosa/ObservableProperty"/>
 <rdf:type rdf:resource="http://www.w3.org/ns/ssn/Property"/>
 <rdfs:label xml:lang="en">Standard Capacity</rdfs:label>
 <rdfs:label xml:lang="fr">Capacité Standard</rdfs:label>
 <skos:definition xml:lang="en">The commercial volume of a product in a bottle.</skos:definition>  
 <skos:definition xml:lang="fr">Le volume commercial d'un produit en bouteille.</skos:definition>  
 <rdfs:isDefinedBy rdf:resource="https://rdf.ag/o/beer-ONTOLOGY_DATE"/>
 <void:inDataset rdf:resource="#datasetdefinition"/>
</rdf:Description>

<rdf:Description rdf:about="#grossWeight">
 <rdf:type rdf:resource="http://www.w3.org/ns/sosa/ObservableProperty"/>
 <rdf:type rdf:resource="http://www.w3.org/ns/ssn/Property"/>
 <rdfs:label xml:lang="en">Gross Weight</rdfs:label>
 <rdfs:label xml:lang="fr">Poids Brut</rdfs:label>
 <skos:definition xml:lang="fr">La masse volumique du contenant et du produit.</skos:definition>  
 <skos:definition xml:lang="en">The weight of the product and the packaging.</skos:definition>  
 <rdfs:isDefinedBy rdf:resource="https://rdf.ag/o/beer-ONTOLOGY_DATE"/>
 <void:inDataset rdf:resource="#datasetdefinition"/>
</rdf:Description>

<rdf:Description rdf:about="#packagingWeight">
 <rdf:type rdf:resource="http://www.w3.org/ns/sosa/ObservableProperty"/>
 <rdf:type rdf:resource="http://www.w3.org/ns/ssn/Property"/>
 <rdfs:label xml:lang="en">Packaging Weight</rdfs:label>
 <rdfs:label xml:lang="fr">Poids de l'emballage</rdfs:label>
 <skos:definition xml:lang="fr">La masse volumique du contenant.</skos:definition>  
 <skos:definition xml:lang="en">The weight of the packaging.</skos:definition>  
 <rdfs:isDefinedBy rdf:resource="https://rdf.ag/o/beer-ONTOLOGY_DATE"/>
 <void:inDataset rdf:resource="#datasetdefinition"/>
</rdf:Description>

<!-- Prov/time Glue see https://www.w3.org/TR/owl-time/#time-prov-->

<rdf:Description rdf:about="http://www.w3.org/ns/prov#Activity">
 <rdfs:subClassOf rdf:resource="http://www.w3.org/2006/time#TemporalEntity"/>
</rdf:Description>

<rdf:Description rdf:about="http://www.w3.org/ns/prov#InstantaneousEvent">
 <rdfs:subClassOf rdf:resource="http://www.w3.org/2006/time#Instant"/>
</rdf:Description>

<rdf:Description rdf:about="http://www.w3.org/ns/prov#atTime">
 <rdfs:subPropertyOf rdf:resource="http://www.w3.org/2006/time#inXSDDateTime"/>
</rdf:Description>

<rdf:Description rdf:about="http://www.w3.org/ns/prov#endedAtTime">
 <owl:propertyChainAxiom>
  <rdf:Description>
   <rdf:first rdf:resource="http://www.w3.org/ns/prov#hasEnd"/>
    <rdf:rest>
     <rdf:Description>
      <rdf:first rdf:resource="http://www.w3.org/ns/prov#inXSDDateTime"/>
      <rdf:rest rdf:resource="http://www.w3.org/1999/02/22-rdf-syntax-ns#nil"/>
     </rdf:Description>
    </rdf:rest>
   </rdf:Description>
  </owl:propertyChainAxiom>
 </rdf:Description>
 <rdf:Description rdf:about="http://www.w3.org/ns/prov#startedAtTime">
  <owl:propertyChainAxiom>
   <rdf:Description>
    <rdf:first rdf:resource="http://www.w3.org/ns/prov#hasBeginning"/>
     <rdf:rest>
      <rdf:Description>
       <rdf:first rdf:resource="http://www.w3.org/ns/prov#inXSDDateTime"/>
       <rdf:rest rdf:resource="http://www.w3.org/1999/02/22-rdf-syntax-ns#nil"/>
      </rdf:Description>
     </rdf:rest>
    </rdf:Description>
   </owl:propertyChainAxiom>
 </rdf:Description>
 

 <cs:ChangeSet rdf:about="#8287522d0a97511a1ae6f711d969f799">
  <rdfs:subClassOf rdf:resource="http://www.w3.org/2006/time#TemporalEntity"/>
  <rdfs:subClassOf rdf:resource="http://www.w3.org/ns/prov#Activity"/>
  <prov:wasAttributedTo rdf:resource="#warren"/>
  <cs:addition rdf:resource="#BraggotBeer"/>
  <cs:creatorName>Rob Warren</cs:creatorName>
  <cs:createdDate>2024-02-14</cs:createdDate>
  <prov:endedAtTime rdf:datatype="http://www.w3.org/2001/XMLSchema#dateTime">2024-02-14T16:00:00-04:00</prov:endedAtTime>
  <prov:startedAtTime rdf:datatype="http://www.w3.org/2001/XMLSchema#dateTime">2024-02-14T16:00:00-04:00</prov:startedAtTime>
  <cs:changeReason xml:lang="en">Added Braggot as a beer type.</cs:changeReason>
  <cs:changeReason xml:lang="fr">Ajout de Braggot comme type de bière.</cs:changeReason>
  <rdfs:isDefinedBy rdf:resource="https://rdf.ag/o/beer-ONTOLOGY_DATE"/>
  <void:inDataset rdf:resource="#datasetdefinition"/>
  <owl:versionInfo>1.3</owl:versionInfo>
 </cs:ChangeSet>

 <cs:ChangeSet rdf:about="#4b4f5e5d9365558e0e2cd66a6ffb2f44">
  <cs:precedingChangeSet rdf:resource="#8287522d0a97511a1ae6f711d969f799"/>
  <rdfs:subClassOf rdf:resource="http://www.w3.org/2006/time#TemporalEntity"/>
  <rdfs:subClassOf rdf:resource="http://www.w3.org/ns/prov#Activity"/>
  <prov:wasAttributedTo rdf:resource="#warren"/>
  <cs:addition rdf:resource="#psw"/>
  <cs:removal rdf:resource="#myra"/>
  <cs:creatorName>Rob Warren</cs:creatorName>
  <cs:createdDate>2024-02-14</cs:createdDate>
  <prov:endedAtTime rdf:datatype="http://www.w3.org/2001/XMLSchema#dateTime">2024-02-14T16:14:43-04:00</prov:endedAtTime>
  <prov:startedAtTime rdf:datatype="http://www.w3.org/2001/XMLSchema#dateTime">2024-02-14T16:14:43-04:00</prov:startedAtTime>
  <cs:changeReason xml:lang="en">Update ontology ownership and change tracking.</cs:changeReason>
  <cs:changeReason xml:lang="fr">Mise à jour des propriétés de l’ontologie et le suivi des modifications.</cs:changeReason>
  <rdfs:isDefinedBy rdf:resource="https://rdf.ag/o/beer-ONTOLOGY_DATE"/>
  <void:inDataset rdf:resource="#datasetdefinition"/>
  <owl:versionInfo>1.3</owl:versionInfo>
 </cs:ChangeSet>  

 <cs:ChangeSet rdf:about="#f7afcbbdabbc5c2caabcbf6e173597af">
  <cs:precedingChangeSet rdf:resource="#4b4f5e5d9365558e0e2cd66a6ffb2f44"/>
  <rdfs:subClassOf rdf:resource="http://www.w3.org/2006/time#TemporalEntity"/>
  <rdfs:subClassOf rdf:resource="http://www.w3.org/ns/prov#Activity"/>
  <prov:wasAttributedTo rdf:resource="#warren"/>
  <cs:statement rdf:resource="#Distillery"/>
  <cs:statement rdf:resource="#Brewery"/>
  <cs:statement rdf:resource="#OffLicense"/>
  <cs:creatorName>Rob Warren</cs:creatorName>
  <cs:createdDate>2024-02-20</cs:createdDate>
  <prov:endedAtTime rdf:datatype="http://www.w3.org/2001/XMLSchema#dateTime">2024-02-20T14:59:32-04:00</prov:endedAtTime>
  <prov:startedAtTime rdf:datatype="http://www.w3.org/2001/XMLSchema#dateTime">2024-02-20T14:59:32-04:00</prov:startedAtTime>
  <cs:changeReason xml:lang="en">Ensure that breweries, distilleries, taprooms and offsales are proper locations. These are now subclasses of gs1:Organization, schema:Organization, org:Organization, foaf:Organization, prov:Agent, prov:Location and geosparql:Feature.</cs:changeReason>
  <cs:changeReason xml:lang="fr">Assurez que les brasseries, distilleries, taprooms et offsales sont des emplacements appropriés. Ce sont désormais des sous-classes de gs1:Organization, schema:Organization, org:Organization, foaf:Organization, prov:Agent, prov:Location and geosparql:Feature.</cs:changeReason>
  <rdfs:isDefinedBy rdf:resource="https://rdf.ag/o/beer-ONTOLOGY_DATE"/>
  <void:inDataset rdf:resource="#datasetdefinition"/>
  <owl:versionInfo>1.3</owl:versionInfo>
 </cs:ChangeSet>  

 <cs:ChangeSet rdf:about="#d41d8cd98f00b204e9800998ecf8427e">
  <cs:precedingChangeSet rdf:resource="#f7afcbbdabbc5c2caabcbf6e173597af"/>
  <rdfs:subClassOf rdf:resource="http://www.w3.org/2006/time#TemporalEntity"/>
  <rdfs:subClassOf rdf:resource="http://www.w3.org/ns/prov#Activity"/>
  <prov:wasAttributedTo rdf:resource="#warren"/>
  <cs:creatorName>Rob Warren</cs:creatorName>
  <cs:createdDate>2024-02-21</cs:createdDate>
  <prov:endedAtTime rdf:datatype="http://www.w3.org/2001/XMLSchema#dateTime">2024-02-21T17:50:32-04:00</prov:endedAtTime>
  <prov:startedAtTime rdf:datatype="http://www.w3.org/2001/XMLSchema#dateTime">2024-02-21T17:50:32-04:00</prov:startedAtTime>
  <cs:changeReason xml:lang="en">Ensure changelog is in french and english; add prov/time compatibility statements.</cs:changeReason>
  <cs:changeReason xml:lang="fr">S'assurer que le journal des modifications est en français et en anglais; ajouter des déclarations de compatibilité prov/time.</cs:changeReason>
  <rdfs:isDefinedBy rdf:resource="https://rdf.ag/o/beer-ONTOLOGY_DATE"/>
  <void:inDataset rdf:resource="#datasetdefinition"/>
  <owl:versionInfo>1.3</owl:versionInfo>
 </cs:ChangeSet>  
  
  


<!-- Various OWL compatibility statements. -->
<owl:AnnotationProperty rdf:about="http://creativecommons.org/ns#Jurisdiction"/>
<owl:AnnotationProperty rdf:about="http://creativecommons.org/ns#attributionURL"/>
<owl:AnnotationProperty rdf:about="http://creativecommons.org/ns#license"/>
<owl:AnnotationProperty rdf:about="http://purl.org/dc/terms/creator"/>
<owl:AnnotationProperty rdf:about="http://purl.org/dc/terms/date"/>
<owl:AnnotationProperty rdf:about="http://purl.org/dc/terms/description"/>
<owl:AnnotationProperty rdf:about="http://purl.org/dc/terms/rights"/>
<owl:AnnotationProperty rdf:about="http://purl.org/dc/terms/subject"/>
<owl:AnnotationProperty rdf:about="http://purl.org/dc/terms/title"/>
<owl:AnnotationProperty rdf:about="http://purl.org/vocab/vann/preferredNamespacePrefix"/>
<owl:AnnotationProperty rdf:about="http://purl.org/vocab/vann/preferredNamespaceUri"/>
<owl:AnnotationProperty rdf:about="http://xmlns.com/foaf/0.1/name"/>
<owl:AnnotationProperty rdf:about="https://schema.org/contentUrl"/>
<owl:AnnotationProperty rdf:about="https://schema.org/creator"/>
<owl:AnnotationProperty rdf:about="https://schema.org/description"/>
<owl:AnnotationProperty rdf:about="https://schema.org/distribution"/>
<owl:AnnotationProperty rdf:about="https://schema.org/email"/>
<owl:AnnotationProperty rdf:about="https://schema.org/encodingFormat"/>
<owl:AnnotationProperty rdf:about="https://schema.org/identifier"/>
<owl:AnnotationProperty rdf:about="https://schema.org/keywords"/>
<owl:AnnotationProperty rdf:about="https://schema.org/license"/>
<owl:AnnotationProperty rdf:about="https://schema.org/name"/>
<owl:AnnotationProperty rdf:about="https://schema.org/url"/>
<owl:AnnotationProperty rdf:about="https://schema.org/version"/>

    
</rdf:RDF>

